<?xml version="1.0" encoding="UTF-8"?><rdf:RDF
    xml:base="http://rdaregistry.info/Elements/u/"
    xmlns:dc="http://purl.org/dc/elements/1.1/"
    xmlns:foaf="http://xmlns.com/foaf/0.1/"
    xmlns:owl="http://www.w3.org/2002/07/owl#"
    xmlns:rdakit="http://metadataregistry.org/uri/profile/rdakit/"
    xmlns:rdf="http://www.w3.org/1999/02/22-rdf-syntax-ns#"
    xmlns:rdfs="http://www.w3.org/2000/01/rdf-schema#"
    xmlns:reg="http://metadataregistry.org/uri/profile/regap/"
    xmlns:skos="http://www.w3.org/2004/02/skos/core#">

<owl:Ontology rdf:about="http://rdaregistry.info/Elements/u"/>

<!-- Element Set: RDA Unconstrained properties -->
<rdf:Description rdf:about="http://rdaregistry.info/Elements/u/">
  <dc:title xml:lang="en">RDA Unconstrained properties</dc:title>
  <foaf:homepage rdf:resource="http://www.rdaregistry.info/Elements/u/"/>
  <skos:note  xml:lang="en">Properties derived from RDA elements and relationship designators without specific or implicit restrictions to RDA entities.</skos:note>
</rdf:Description>

<!-- Properties -->

<!-- Property: has abbreviated title -->
<owl:ObjectProperty rdf:about="http://rdaregistry.info/Elements/u/P60359">
  <rdfs:isDefinedBy rdf:resource="http://rdaregistry.info/Elements/u/" />
  <reg:status rdf:resource="http://metadataregistry.org/uri/RegStatus/1001" />
  <reg:name xml:lang="en">abbreviatedTitle</reg:name>
  <rdfs:label xml:lang="en">has abbreviated title</rdfs:label>
  <skos:definition xml:lang="en">Relates a resource to a title that has been abbreviated for purposes of indexing or identification.</skos:definition>
  <rdf:type rdf:resource="http://www.w3.org/1999/02/22-rdf-syntax-ns#Property" />
  <rdfs:subPropertyOf rdf:resource="http://rdaregistry.info/Elements/u/P60369" />
  <reg:hasSubproperty rdf:resource="http://rdaregistry.info/Elements/m/P30131" />
  <reg:lexicalAlias rdf:resource="http://rdaregistry.info/Elements/u/abbreviatedTitle.en" />
</owl:ObjectProperty>

<!-- Property: is abridged as -->
<owl:ObjectProperty rdf:about="http://rdaregistry.info/Elements/u/P60275">
  <rdfs:isDefinedBy rdf:resource="http://rdaregistry.info/Elements/u/" />
  <reg:status rdf:resource="http://metadataregistry.org/uri/RegStatus/1001" />
  <reg:name xml:lang="en">abridgedAs</reg:name>
  <rdfs:label xml:lang="en">is abridged as</rdfs:label>
  <skos:definition xml:lang="en">Relates a resource to a resource that shortens a source resource without changing a general meaning or manner of presentation.</skos:definition>
  <rdf:type rdf:resource="http://www.w3.org/1999/02/22-rdf-syntax-ns#Property" />
  <rdfs:subPropertyOf rdf:resource="http://rdaregistry.info/Elements/u/P60250" />
  <owl:inverseOf rdf:resource="http://rdaregistry.info/Elements/u/P60223" />
  <reg:hasSubproperty rdf:resource="http://rdaregistry.info/Elements/e/P20166" />
  <reg:lexicalAlias rdf:resource="http://rdaregistry.info/Elements/u/abridgedAs.en" />
</owl:ObjectProperty>

<!-- Property: is abridgement of -->
<owl:ObjectProperty rdf:about="http://rdaregistry.info/Elements/u/P60223">
  <rdfs:isDefinedBy rdf:resource="http://rdaregistry.info/Elements/u/" />
  <reg:status rdf:resource="http://metadataregistry.org/uri/RegStatus/1001" />
  <reg:name xml:lang="en">abridgementOf</reg:name>
  <rdfs:label xml:lang="en">is abridgement of</rdfs:label>
  <skos:definition xml:lang="en">Relates a resource to a resource that has been abridged, i.e., shortened without changing a general meaning or manner of presentation of a source resource.</skos:definition>
  <rdf:type rdf:resource="http://www.w3.org/1999/02/22-rdf-syntax-ns#Property" />
  <rdfs:subPropertyOf rdf:resource="http://rdaregistry.info/Elements/u/P60305" />
  <owl:inverseOf rdf:resource="http://rdaregistry.info/Elements/u/P60275" />
  <reg:hasSubproperty rdf:resource="http://rdaregistry.info/Elements/e/P20121" />
  <reg:lexicalAlias rdf:resource="http://rdaregistry.info/Elements/u/abridgementOf.en" />
</owl:ObjectProperty>

<!-- Property: has abridger -->
<owl:ObjectProperty rdf:about="http://rdaregistry.info/Elements/u/P60394">
  <rdfs:isDefinedBy rdf:resource="http://rdaregistry.info/Elements/u/" />
  <reg:status rdf:resource="http://metadataregistry.org/uri/RegStatus/1001" />
  <reg:name xml:lang="en">abridger</reg:name>
  <rdfs:label xml:lang="en">has abridger</rdfs:label>
  <skos:definition xml:lang="en">Relates a resource to an agent contributing to a resource by shortening or condensing an original resource but leaving the nature and content substantially unchanged.</skos:definition>
  <rdf:type rdf:resource="http://www.w3.org/1999/02/22-rdf-syntax-ns#Property" />
  <rdfs:subPropertyOf rdf:resource="http://rdaregistry.info/Elements/u/P60398" />
  <owl:inverseOf rdf:resource="http://rdaregistry.info/Elements/u/P60622" />
  <reg:hasSubproperty rdf:resource="http://rdaregistry.info/Elements/e/P20049" />
  <reg:lexicalAlias rdf:resource="http://rdaregistry.info/Elements/u/abridger.en" />
  <skos:scopeNote xml:lang="en">Substantial modification that results in the creation of a new resource is excluded.</skos:scopeNote>
  <rdakit:seeAlso rdf:resource="http://rdaregistry.info/Elements/u/P60434" />
</owl:ObjectProperty>

<!-- Property: is abridger of -->
<owl:ObjectProperty rdf:about="http://rdaregistry.info/Elements/u/P60622">
  <rdfs:isDefinedBy rdf:resource="http://rdaregistry.info/Elements/u/" />
  <reg:status rdf:resource="http://metadataregistry.org/uri/RegStatus/1001" />
  <reg:name xml:lang="en">abridgerOf</reg:name>
  <rdfs:label xml:lang="en">is abridger of</rdfs:label>
  <skos:definition xml:lang="en">Relates an agent contributing to a resource by shortening or condensing an original resource but leaving the nature and content substantially unchanged to a resource.</skos:definition>
  <rdf:type rdf:resource="http://www.w3.org/1999/02/22-rdf-syntax-ns#Property" />
  <rdfs:subPropertyOf rdf:resource="http://rdaregistry.info/Elements/u/P60626" />
  <owl:inverseOf rdf:resource="http://rdaregistry.info/Elements/u/P60394" />
  <reg:hasSubproperty rdf:resource="http://rdaregistry.info/Elements/a/P50157" />
  <reg:lexicalAlias rdf:resource="http://rdaregistry.info/Elements/u/abridgerOf.en" />
  <rdakit:seeAlso rdf:resource="http://rdaregistry.info/Elements/u/P60663" />
</owl:ObjectProperty>

<!-- Property: has absorbed agent -->
<owl:ObjectProperty rdf:about="http://rdaregistry.info/Elements/u/P60901">
  <rdfs:isDefinedBy rdf:resource="http://rdaregistry.info/Elements/u/" />
  <reg:status rdf:resource="http://metadataregistry.org/uri/RegStatus/1001" />
  <rdf:type rdf:resource="http://www.w3.org/1999/02/22-rdf-syntax-ns#Property" />
  <reg:name xml:lang="en">absorbedAgent</reg:name>
  <rdfs:label xml:lang="en">has absorbed agent</rdfs:label>
  <reg:lexicalAlias rdf:resource="http://rdaregistry.info/Elements/u/absorbedAgent.en" />
  <skos:definition xml:lang="en">Relates an agent to an agent that was absorbed by another agent.</skos:definition>
  <owl:inverseOf rdf:resource="http://rdaregistry.info/Elements/u/P60902" />
</owl:ObjectProperty>

<!-- Property: is absorbed by -->
<owl:ObjectProperty rdf:about="http://rdaregistry.info/Elements/u/P60247">
  <rdfs:isDefinedBy rdf:resource="http://rdaregistry.info/Elements/u/" />
  <reg:status rdf:resource="http://metadataregistry.org/uri/RegStatus/1001" />
  <reg:name xml:lang="en">absorbedBy</reg:name>
  <rdfs:label xml:lang="en">is absorbed by</rdfs:label>
  <skos:definition xml:lang="en">Relates a resource to a resource that incorporates another resource.</skos:definition>
  <rdf:type rdf:resource="http://www.w3.org/1999/02/22-rdf-syntax-ns#Property" />
  <rdfs:subPropertyOf rdf:resource="http://rdaregistry.info/Elements/u/P60278" />
  <owl:inverseOf rdf:resource="http://rdaregistry.info/Elements/u/P60574" />
  <reg:hasSubproperty rdf:resource="http://rdaregistry.info/Elements/e/P20143" />
  <reg:lexicalAlias rdf:resource="http://rdaregistry.info/Elements/u/absorbedBy.en" />
</owl:ObjectProperty>

<!-- Property: is absorbed in part by -->
<owl:ObjectProperty rdf:about="http://rdaregistry.info/Elements/u/P60248">
  <rdfs:isDefinedBy rdf:resource="http://rdaregistry.info/Elements/u/" />
  <reg:status rdf:resource="http://metadataregistry.org/uri/RegStatus/1001" />
  <reg:name xml:lang="en">absorbedInPartBy</reg:name>
  <rdfs:label xml:lang="en">is absorbed in part by</rdfs:label>
  <skos:definition xml:lang="en">Relates a resource to a resource that incorporates part of the content of another resource.</skos:definition>
  <rdf:type rdf:resource="http://www.w3.org/1999/02/22-rdf-syntax-ns#Property" />
  <rdfs:subPropertyOf rdf:resource="http://rdaregistry.info/Elements/u/P60278" />
  <owl:inverseOf rdf:resource="http://rdaregistry.info/Elements/u/P60575" />
  <reg:hasSubproperty rdf:resource="http://rdaregistry.info/Elements/e/P20144" />
  <reg:lexicalAlias rdf:resource="http://rdaregistry.info/Elements/u/absorbedInPartBy.en" />
</owl:ObjectProperty>

<!-- Property: has absorbing agent -->
<owl:ObjectProperty rdf:about="http://rdaregistry.info/Elements/u/P60902">
  <rdfs:isDefinedBy rdf:resource="http://rdaregistry.info/Elements/u/" />
  <reg:status rdf:resource="http://metadataregistry.org/uri/RegStatus/1001" />
  <rdf:type rdf:resource="http://www.w3.org/1999/02/22-rdf-syntax-ns#Property" />
  <reg:name xml:lang="en">absorbingAgent</reg:name>
  <rdfs:label xml:lang="en">has absorbing agent</rdfs:label>
  <reg:lexicalAlias rdf:resource="http://rdaregistry.info/Elements/u/absorbingAgent.en" />
  <skos:definition xml:lang="en">Relates an agent to an agent that absorbed another agent.</skos:definition>
  <owl:inverseOf rdf:resource="http://rdaregistry.info/Elements/u/P60901" />
</owl:ObjectProperty>

<!-- Property: is absorption in part of -->
<owl:ObjectProperty rdf:about="http://rdaregistry.info/Elements/u/P60575">
  <rdfs:isDefinedBy rdf:resource="http://rdaregistry.info/Elements/u/" />
  <reg:status rdf:resource="http://metadataregistry.org/uri/RegStatus/1001" />
  <reg:name xml:lang="en">absorptionInPartOf</reg:name>
  <rdfs:label xml:lang="en">is absorption in part of</rdfs:label>
  <skos:definition xml:lang="en">Relates a resource to a resource that has been partially incorporated into another resource.</skos:definition>
  <rdf:type rdf:resource="http://www.w3.org/1999/02/22-rdf-syntax-ns#Property" />
  <rdfs:subPropertyOf rdf:resource="http://rdaregistry.info/Elements/u/P60261" />
  <owl:inverseOf rdf:resource="http://rdaregistry.info/Elements/u/P60248" />
  <reg:hasSubproperty rdf:resource="http://rdaregistry.info/Elements/e/P20138" />
  <reg:lexicalAlias rdf:resource="http://rdaregistry.info/Elements/u/absorptionInPartOf.en" />
</owl:ObjectProperty>

<!-- Property: is absorption of -->
<owl:ObjectProperty rdf:about="http://rdaregistry.info/Elements/u/P60574">
  <rdfs:isDefinedBy rdf:resource="http://rdaregistry.info/Elements/u/" />
  <reg:status rdf:resource="http://metadataregistry.org/uri/RegStatus/1001" />
  <reg:name xml:lang="en">absorptionOf</reg:name>
  <rdfs:label xml:lang="en">is absorption of</rdfs:label>
  <skos:definition xml:lang="en">Relates a resource to a resource that has been incorporated into another resource.</skos:definition>
  <rdf:type rdf:resource="http://www.w3.org/1999/02/22-rdf-syntax-ns#Property" />
  <rdfs:subPropertyOf rdf:resource="http://rdaregistry.info/Elements/u/P60261" />
  <owl:inverseOf rdf:resource="http://rdaregistry.info/Elements/u/P60247" />
  <reg:hasSubproperty rdf:resource="http://rdaregistry.info/Elements/e/P20137" />
  <reg:lexicalAlias rdf:resource="http://rdaregistry.info/Elements/u/absorptionOf.en" />
</owl:ObjectProperty>

<!-- Property: is abstracted as -->
<owl:ObjectProperty rdf:about="http://rdaregistry.info/Elements/u/P60203">
  <rdfs:isDefinedBy rdf:resource="http://rdaregistry.info/Elements/u/" />
  <reg:status rdf:resource="http://metadataregistry.org/uri/RegStatus/1001" />
  <reg:name xml:lang="en">abstractedAs</reg:name>
  <rdfs:label xml:lang="en">is abstracted as</rdfs:label>
  <skos:definition xml:lang="en">Relates a resource to a resource that abbreviates a source resource in a brief, objective manner.</skos:definition>
  <rdf:type rdf:resource="http://www.w3.org/1999/02/22-rdf-syntax-ns#Property" />
  <rdfs:subPropertyOf rdf:resource="http://rdaregistry.info/Elements/u/P60250" />
  <owl:inverseOf rdf:resource="http://rdaregistry.info/Elements/u/P60224" />
  <reg:hasSubproperty rdf:resource="http://rdaregistry.info/Elements/e/P20104" />
  <reg:lexicalAlias rdf:resource="http://rdaregistry.info/Elements/u/abstractedAs.en" />
</owl:ObjectProperty>

<!-- Property: is abstracted in -->
<owl:ObjectProperty rdf:about="http://rdaregistry.info/Elements/u/P60177">
  <rdfs:isDefinedBy rdf:resource="http://rdaregistry.info/Elements/u/" />
  <reg:status rdf:resource="http://metadataregistry.org/uri/RegStatus/1001" />
  <reg:name xml:lang="en">abstractedIn</reg:name>
  <rdfs:label xml:lang="en">is abstracted in</rdfs:label>
  <skos:definition xml:lang="en">Relates a resource to a resource that is an abstracting and indexing service that abstracts the contents of a source entity.</skos:definition>
  <rdf:type rdf:resource="http://www.w3.org/1999/02/22-rdf-syntax-ns#Property" />
  <rdfs:subPropertyOf rdf:resource="http://rdaregistry.info/Elements/u/P60250" />
  <owl:inverseOf rdf:resource="http://rdaregistry.info/Elements/u/P60308" />
  <reg:hasSubproperty rdf:resource="http://rdaregistry.info/Elements/e/P20090" />
  <reg:lexicalAlias rdf:resource="http://rdaregistry.info/Elements/u/abstractedIn.en" />
</owl:ObjectProperty>

<!-- Property: is abstract of -->
<owl:ObjectProperty rdf:about="http://rdaregistry.info/Elements/u/P60224">
  <rdfs:isDefinedBy rdf:resource="http://rdaregistry.info/Elements/u/" />
  <reg:status rdf:resource="http://metadataregistry.org/uri/RegStatus/1001" />
  <reg:name xml:lang="en">abstractOf</reg:name>
  <rdfs:label xml:lang="en">is abstract of</rdfs:label>
  <skos:definition xml:lang="en">Relates a resource to a resource that has been abstracted, i.e., abbreviated in a brief, objective manner.</skos:definition>
  <rdf:type rdf:resource="http://www.w3.org/1999/02/22-rdf-syntax-ns#Property" />
  <rdfs:subPropertyOf rdf:resource="http://rdaregistry.info/Elements/u/P60305" />
  <owl:inverseOf rdf:resource="http://rdaregistry.info/Elements/u/P60203" />
  <reg:hasSubproperty rdf:resource="http://rdaregistry.info/Elements/e/P20122" />
  <reg:lexicalAlias rdf:resource="http://rdaregistry.info/Elements/u/abstractOf.en" />
</owl:ObjectProperty>

<!-- Property: is abstracts for -->
<owl:ObjectProperty rdf:about="http://rdaregistry.info/Elements/u/P60308">
  <rdfs:isDefinedBy rdf:resource="http://rdaregistry.info/Elements/u/" />
  <reg:status rdf:resource="http://metadataregistry.org/uri/RegStatus/1001" />
  <reg:name xml:lang="en">abstractsFor</reg:name>
  <rdfs:label xml:lang="en">is abstracts for</rdfs:label>
  <skos:definition xml:lang="en">Relates a resource to a resource whose contents have been abstracted by an abstracting and indexing service.</skos:definition>
  <rdf:type rdf:resource="http://www.w3.org/1999/02/22-rdf-syntax-ns#Property" />
  <rdfs:subPropertyOf rdf:resource="http://rdaregistry.info/Elements/u/P60305" />
  <owl:inverseOf rdf:resource="http://rdaregistry.info/Elements/u/P60177" />
  <reg:hasSubproperty rdf:resource="http://rdaregistry.info/Elements/e/P20193" />
  <reg:lexicalAlias rdf:resource="http://rdaregistry.info/Elements/u/abstractsFor.en" />
</owl:ObjectProperty>

<!-- Property: has academic degree -->
<owl:ObjectProperty rdf:about="http://rdaregistry.info/Elements/u/P60175">
  <rdfs:isDefinedBy rdf:resource="http://rdaregistry.info/Elements/u/" />
  <reg:status rdf:resource="http://metadataregistry.org/uri/RegStatus/1001" />
  <reg:name xml:lang="en">academicDegree</reg:name>
  <rdfs:label xml:lang="en">has academic degree</rdfs:label>
  <skos:definition xml:lang="en">Relates a resource to a rank conferred as a guarantee of academic proficiency.</skos:definition>
  <rdf:type rdf:resource="http://www.w3.org/1999/02/22-rdf-syntax-ns#Property" />
  <reg:lexicalAlias rdf:resource="http://rdaregistry.info/Elements/u/academicDegree.en" />
</owl:ObjectProperty>

<!-- Property: has accessibility content -->
<owl:ObjectProperty rdf:about="http://rdaregistry.info/Elements/u/P60487">
  <rdfs:isDefinedBy rdf:resource="http://rdaregistry.info/Elements/u/" />
  <reg:status rdf:resource="http://metadataregistry.org/uri/RegStatus/1001" />
  <reg:name xml:lang="en">accessibilityContent</reg:name>
  <rdfs:label xml:lang="en">has accessibility content</rdfs:label>
  <skos:definition xml:lang="en">Relates a resource to an indication of content that provides alternative sensory modes to perceive a primary content of a resource.</skos:definition>
  <rdf:type rdf:resource="http://www.w3.org/1999/02/22-rdf-syntax-ns#Property" />
  <reg:hasSubproperty rdf:resource="http://rdaregistry.info/Elements/e/P20208" />
  <reg:lexicalAlias rdf:resource="http://rdaregistry.info/Elements/u/accessibilityContent.en" />
  <skos:scopeNote xml:lang="en">Accessibility content includes accessible labels, audio description, captioning, image description, sign language, and subtitles. Accessibility content does not include subtitles in a language different from the spoken content.</skos:scopeNote>
</owl:ObjectProperty>

<!-- Property: is accompanied by -->
<owl:ObjectProperty rdf:about="http://rdaregistry.info/Elements/u/P60196">
  <rdfs:isDefinedBy rdf:resource="http://rdaregistry.info/Elements/u/" />
  <reg:status rdf:resource="http://metadataregistry.org/uri/RegStatus/1001" />
  <reg:name xml:lang="en">accompaniedBy</reg:name>
  <rdfs:label xml:lang="en">is accompanied by</rdfs:label>
  <skos:definition xml:lang="en">Relates a resource to a resource issued with another resource, without any relationship to its content.</skos:definition>
  <rdf:type rdf:resource="http://www.w3.org/1999/02/22-rdf-syntax-ns#Property" />
  <rdfs:subPropertyOf rdf:resource="http://rdaregistry.info/Elements/u/P60709" />
  <owl:inverseOf rdf:resource="http://rdaregistry.info/Elements/u/P60196" />
  <reg:hasSubproperty rdf:resource="http://rdaregistry.info/Elements/u/P60237" />
  <reg:hasSubproperty rdf:resource="http://rdaregistry.info/Elements/u/P60256" />
  <reg:hasSubproperty rdf:resource="http://rdaregistry.info/Elements/i/P40029" />
  <reg:hasSubproperty rdf:resource="http://rdaregistry.info/Elements/m/P30027" />
  <reg:lexicalAlias rdf:resource="http://rdaregistry.info/Elements/u/accompaniedBy.en" />
</owl:ObjectProperty>

<!-- Property: has accompanying resource relationship with -->
<owl:ObjectProperty rdf:about="http://rdaregistry.info/Elements/u/P60709">
  <rdfs:isDefinedBy rdf:resource="http://rdaregistry.info/Elements/u/" />
  <reg:status rdf:resource="http://metadataregistry.org/uri/RegStatus/1001" />
  <reg:name xml:lang="en">accompanyingResourceRelationshipWith</reg:name>
  <rdfs:label xml:lang="en">has accompanying resource relationship with</rdfs:label>
  <rdf:type rdf:resource="http://www.w3.org/1999/02/22-rdf-syntax-ns#Property" />
  <reg:hasSubproperty rdf:resource="http://rdaregistry.info/Elements/u/P60196" />
  <reg:hasSubproperty rdf:resource="http://rdaregistry.info/Elements/u/P60198" />
  <reg:hasSubproperty rdf:resource="http://rdaregistry.info/Elements/u/P60204" />
  <reg:hasSubproperty rdf:resource="http://rdaregistry.info/Elements/u/P60307" />
  <owl:inverseOf rdf:resource="http://rdaregistry.info/Elements/u/P60709" />
  <skos:definition xml:lang="en">Relates a resource to a resource that is an augmentation of, or is augmented by, or is complemented by, or accompanies, or is accompanied by a resource.</skos:definition>
  <reg:hasSubproperty rdf:resource="http://rdaregistry.info/Elements/e/P20232" />
  <reg:hasSubproperty rdf:resource="http://rdaregistry.info/Elements/i/P40051" />
  <reg:hasSubproperty rdf:resource="http://rdaregistry.info/Elements/m/P30210" />
  <reg:lexicalAlias rdf:resource="http://rdaregistry.info/Elements/u/accompanyingResourceRelationshipWith.en" />
</owl:ObjectProperty>

<!-- Property: has actor -->
<owl:ObjectProperty rdf:about="http://rdaregistry.info/Elements/u/P60142">
  <rdfs:isDefinedBy rdf:resource="http://rdaregistry.info/Elements/u/" />
  <reg:status rdf:resource="http://metadataregistry.org/uri/RegStatus/1001" />
  <reg:name xml:lang="en">actor</reg:name>
  <rdfs:label xml:lang="en">has actor</rdfs:label>
  <skos:definition xml:lang="en">Relates a resource to a performer contributing to a resource by acting as a cast member or player in a musical or dramatic presentation, etc.</skos:definition>
  <rdf:type rdf:resource="http://www.w3.org/1999/02/22-rdf-syntax-ns#Property" />
  <rdfs:subPropertyOf rdf:resource="http://rdaregistry.info/Elements/u/P60387" />
  <owl:inverseOf rdf:resource="http://rdaregistry.info/Elements/u/P60017" />
  <reg:hasSubproperty rdf:resource="http://rdaregistry.info/Elements/u/P60152" />
  <reg:hasSubproperty rdf:resource="http://rdaregistry.info/Elements/e/P20012" />
  <reg:lexicalAlias rdf:resource="http://rdaregistry.info/Elements/u/actor.en" />
</owl:ObjectProperty>

<!-- Property: is actor of -->
<owl:ObjectProperty rdf:about="http://rdaregistry.info/Elements/u/P60017">
  <rdfs:isDefinedBy rdf:resource="http://rdaregistry.info/Elements/u/" />
  <reg:status rdf:resource="http://metadataregistry.org/uri/RegStatus/1001" />
  <reg:name xml:lang="en">actorOf</reg:name>
  <rdfs:label xml:lang="en">is actor of</rdfs:label>
  <skos:definition xml:lang="en">Relates a performer contributing to a resource by acting as a cast member or player in a musical or dramatic presentation, etc. to a resource.</skos:definition>
  <rdf:type rdf:resource="http://www.w3.org/1999/02/22-rdf-syntax-ns#Property" />
  <rdfs:subPropertyOf rdf:resource="http://rdaregistry.info/Elements/u/P60615" />
  <owl:inverseOf rdf:resource="http://rdaregistry.info/Elements/u/P60142" />
  <reg:hasSubproperty rdf:resource="http://rdaregistry.info/Elements/u/P60027" />
  <reg:hasSubproperty rdf:resource="http://rdaregistry.info/Elements/a/P50071" />
  <reg:lexicalAlias rdf:resource="http://rdaregistry.info/Elements/u/actorOf.en" />
</owl:ObjectProperty>

<!-- Property: is adaptation of -->
<owl:ObjectProperty rdf:about="http://rdaregistry.info/Elements/u/P60241">
  <rdfs:isDefinedBy rdf:resource="http://rdaregistry.info/Elements/u/" />
  <reg:status rdf:resource="http://metadataregistry.org/uri/RegStatus/1001" />
  <reg:name xml:lang="en">adaptationOf</reg:name>
  <rdfs:label xml:lang="en">is adaptation of</rdfs:label>
  <skos:definition xml:lang="en">Relates a resource to a resource that has been modified for a purpose, use, or medium other than that for which it was originally intended.</skos:definition>
  <rdf:type rdf:resource="http://www.w3.org/1999/02/22-rdf-syntax-ns#Property" />
  <rdfs:subPropertyOf rdf:resource="http://rdaregistry.info/Elements/u/P60305" />
  <owl:inverseOf rdf:resource="http://rdaregistry.info/Elements/u/P60260" />
  <reg:hasSubproperty rdf:resource="http://rdaregistry.info/Elements/u/P60225" />
  <reg:hasSubproperty rdf:resource="http://rdaregistry.info/Elements/u/P60226" />
  <reg:hasSubproperty rdf:resource="http://rdaregistry.info/Elements/u/P60227" />
  <reg:hasSubproperty rdf:resource="http://rdaregistry.info/Elements/u/P60228" />
  <reg:hasSubproperty rdf:resource="http://rdaregistry.info/Elements/u/P60229" />
  <reg:hasSubproperty rdf:resource="http://rdaregistry.info/Elements/u/P60230" />
  <reg:hasSubproperty rdf:resource="http://rdaregistry.info/Elements/u/P60231" />
  <reg:hasSubproperty rdf:resource="http://rdaregistry.info/Elements/u/P60235" />
  <reg:hasSubproperty rdf:resource="http://rdaregistry.info/Elements/u/P60236" />
  <reg:hasSubproperty rdf:resource="http://rdaregistry.info/Elements/e/P20152" />
  <reg:lexicalAlias rdf:resource="http://rdaregistry.info/Elements/u/adaptationOf.en" />
  <reg:hasSubproperty rdf:resource="http://rdaregistry.info/Elements/u/P60743" />
  <reg:hasSubproperty rdf:resource="http://rdaregistry.info/Elements/u/P60745" />
  <skos:scopeNote xml:lang="en">This relationship applies to changes in form or to resources completely rewritten in the same form.</skos:scopeNote>
</owl:ObjectProperty>

<!-- Property: is adapted as -->
<owl:ObjectProperty rdf:about="http://rdaregistry.info/Elements/u/P60260">
  <rdfs:isDefinedBy rdf:resource="http://rdaregistry.info/Elements/u/" />
  <reg:status rdf:resource="http://metadataregistry.org/uri/RegStatus/1001" />
  <reg:name xml:lang="en">adaptedAs</reg:name>
  <rdfs:label xml:lang="en">is adapted as</rdfs:label>
  <skos:definition xml:lang="en">Relates a resource to a resource that modifies a source resource for a purpose, use, or medium other than that for which it was originally intended.</skos:definition>
  <rdf:type rdf:resource="http://www.w3.org/1999/02/22-rdf-syntax-ns#Property" />
  <rdfs:subPropertyOf rdf:resource="http://rdaregistry.info/Elements/u/P60250" />
  <owl:inverseOf rdf:resource="http://rdaregistry.info/Elements/u/P60241" />
  <reg:hasSubproperty rdf:resource="http://rdaregistry.info/Elements/u/P60088" />
  <reg:hasSubproperty rdf:resource="http://rdaregistry.info/Elements/u/P60106" />
  <reg:hasSubproperty rdf:resource="http://rdaregistry.info/Elements/u/P60110" />
  <reg:hasSubproperty rdf:resource="http://rdaregistry.info/Elements/u/P60138" />
  <reg:hasSubproperty rdf:resource="http://rdaregistry.info/Elements/u/P60174" />
  <reg:hasSubproperty rdf:resource="http://rdaregistry.info/Elements/u/P60185" />
  <reg:hasSubproperty rdf:resource="http://rdaregistry.info/Elements/u/P60188" />
  <reg:hasSubproperty rdf:resource="http://rdaregistry.info/Elements/u/P60354" />
  <reg:hasSubproperty rdf:resource="http://rdaregistry.info/Elements/u/P60361" />
  <reg:hasSubproperty rdf:resource="http://rdaregistry.info/Elements/e/P20153" />
  <reg:lexicalAlias rdf:resource="http://rdaregistry.info/Elements/u/adaptedAs.en" />
  <reg:hasSubproperty rdf:resource="http://rdaregistry.info/Elements/u/P60742" />
  <reg:hasSubproperty rdf:resource="http://rdaregistry.info/Elements/u/P60744" />
  <skos:scopeNote xml:lang="en">This relationship applies to changes in form or to resources completely rewritten in the same form.</skos:scopeNote>
</owl:ObjectProperty>

<!-- Property: is adapted as motion picture -->
<owl:ObjectProperty rdf:about="http://rdaregistry.info/Elements/u/P60110">
  <rdfs:isDefinedBy rdf:resource="http://rdaregistry.info/Elements/u/" />
  <reg:status rdf:resource="http://metadataregistry.org/uri/RegStatus/1001" />
  <reg:name xml:lang="en">adaptedAsAMotionPicture</reg:name>
  <rdfs:label xml:lang="en">is adapted as motion picture</rdfs:label>
  <skos:definition xml:lang="en">Relates a resource to a motion picture based on the source resource.</skos:definition>
  <rdf:type rdf:resource="http://www.w3.org/1999/02/22-rdf-syntax-ns#Property" />
  <rdfs:subPropertyOf rdf:resource="http://rdaregistry.info/Elements/u/P60260" />
  <owl:inverseOf rdf:resource="http://rdaregistry.info/Elements/u/P60227" />
  <reg:hasSubproperty rdf:resource="http://rdaregistry.info/Elements/e/P20009" />
  <reg:lexicalAlias rdf:resource="http://rdaregistry.info/Elements/u/adaptedAsAMotionPicture.en" />
</owl:ObjectProperty>

<!-- Property: is adapted as motion picture screenplay -->
<owl:ObjectProperty rdf:about="http://rdaregistry.info/Elements/u/P60184">
  <rdfs:isDefinedBy rdf:resource="http://rdaregistry.info/Elements/u/" />
  <reg:status rdf:resource="http://metadataregistry.org/uri/RegStatus/1001" />
  <reg:name xml:lang="en">adaptedAsAMotionPictureScreenplay</reg:name>
  <rdfs:label xml:lang="en">is adapted as motion picture screenplay</rdfs:label>
  <skos:definition xml:lang="en">Relates a resource to a resource consisting of a screenplay for a motion picture, based on a source resource.</skos:definition>
  <rdf:type rdf:resource="http://www.w3.org/1999/02/22-rdf-syntax-ns#Property" />
  <rdfs:subPropertyOf rdf:resource="http://rdaregistry.info/Elements/u/P60185" />
  <owl:inverseOf rdf:resource="http://rdaregistry.info/Elements/u/P60232" />
  <reg:hasSubproperty rdf:resource="http://rdaregistry.info/Elements/e/P20095" />
  <reg:lexicalAlias rdf:resource="http://rdaregistry.info/Elements/u/adaptedAsAMotionPictureScreenplay.en" />
</owl:ObjectProperty>

<!-- Property: is adapted as radio program -->
<owl:ObjectProperty rdf:about="http://rdaregistry.info/Elements/u/P60174">
  <rdfs:isDefinedBy rdf:resource="http://rdaregistry.info/Elements/u/" />
  <reg:status rdf:resource="http://metadataregistry.org/uri/RegStatus/1001" />
  <reg:name xml:lang="en">adaptedAsARadioProgram</reg:name>
  <rdfs:label xml:lang="en">is adapted as radio program</rdfs:label>
  <skos:definition xml:lang="en">Relates a resource to a radio program based on a source resource.</skos:definition>
  <rdf:type rdf:resource="http://www.w3.org/1999/02/22-rdf-syntax-ns#Property" />
  <rdfs:subPropertyOf rdf:resource="http://rdaregistry.info/Elements/u/P60260" />
  <owl:inverseOf rdf:resource="http://rdaregistry.info/Elements/u/P60229" />
  <reg:hasSubproperty rdf:resource="http://rdaregistry.info/Elements/e/P20060" />
  <reg:lexicalAlias rdf:resource="http://rdaregistry.info/Elements/u/adaptedAsARadioProgram.en" />
</owl:ObjectProperty>

<!-- Property: is adapted as radio script -->
<owl:ObjectProperty rdf:about="http://rdaregistry.info/Elements/u/P60188">
  <rdfs:isDefinedBy rdf:resource="http://rdaregistry.info/Elements/u/" />
  <reg:status rdf:resource="http://metadataregistry.org/uri/RegStatus/1001" />
  <reg:name xml:lang="en">adaptedAsARadioScript</reg:name>
  <rdfs:label xml:lang="en">is adapted as radio script</rdfs:label>
  <skos:definition xml:lang="en">Relates a resource to a resource consisting of a script for a radio program, based on a source resource.</skos:definition>
  <rdf:type rdf:resource="http://www.w3.org/1999/02/22-rdf-syntax-ns#Property" />
  <rdfs:subPropertyOf rdf:resource="http://rdaregistry.info/Elements/u/P60260" />
  <owl:inverseOf rdf:resource="http://rdaregistry.info/Elements/u/P60235" />
  <reg:hasSubproperty rdf:resource="http://rdaregistry.info/Elements/e/P20099" />
  <reg:lexicalAlias rdf:resource="http://rdaregistry.info/Elements/u/adaptedAsARadioScript.en" />
</owl:ObjectProperty>

<!-- Property: is adapted as television program -->
<owl:ObjectProperty rdf:about="http://rdaregistry.info/Elements/u/P60354">
  <rdfs:isDefinedBy rdf:resource="http://rdaregistry.info/Elements/u/" />
  <reg:status rdf:resource="http://metadataregistry.org/uri/RegStatus/1001" />
  <reg:name xml:lang="en">adaptedAsATelevisionProgram</reg:name>
  <rdfs:label xml:lang="en">is adapted as television program</rdfs:label>
  <skos:definition xml:lang="en">Relates a resource to a television program based on a source resource.</skos:definition>
  <rdf:type rdf:resource="http://www.w3.org/1999/02/22-rdf-syntax-ns#Property" />
  <rdfs:subPropertyOf rdf:resource="http://rdaregistry.info/Elements/u/P60260" />
  <owl:inverseOf rdf:resource="http://rdaregistry.info/Elements/u/P60230" />
  <reg:hasSubproperty rdf:resource="http://rdaregistry.info/Elements/e/P20066" />
  <reg:lexicalAlias rdf:resource="http://rdaregistry.info/Elements/u/adaptedAsATelevisionProgram.en" />
</owl:ObjectProperty>

<!-- Property: is adapted as television screenplay -->
<owl:ObjectProperty rdf:about="http://rdaregistry.info/Elements/u/P60186">
  <rdfs:isDefinedBy rdf:resource="http://rdaregistry.info/Elements/u/" />
  <reg:status rdf:resource="http://metadataregistry.org/uri/RegStatus/1001" />
  <reg:name xml:lang="en">adaptedAsATelevisionScreenplay</reg:name>
  <rdfs:label xml:lang="en">is adapted as television screenplay</rdfs:label>
  <skos:definition xml:lang="en">Relates a resource to a resource consisting of a screenplay for a television program, based on a source resource.</skos:definition>
  <rdf:type rdf:resource="http://www.w3.org/1999/02/22-rdf-syntax-ns#Property" />
  <rdfs:subPropertyOf rdf:resource="http://rdaregistry.info/Elements/u/P60185" />
  <owl:inverseOf rdf:resource="http://rdaregistry.info/Elements/u/P60233" />
  <reg:hasSubproperty rdf:resource="http://rdaregistry.info/Elements/e/P20097" />
  <reg:lexicalAlias rdf:resource="http://rdaregistry.info/Elements/u/adaptedAsATelevisionScreenplay.en" />
</owl:ObjectProperty>

<!-- Property: is adapted as video -->
<owl:ObjectProperty rdf:about="http://rdaregistry.info/Elements/u/P60361">
  <rdfs:isDefinedBy rdf:resource="http://rdaregistry.info/Elements/u/" />
  <reg:status rdf:resource="http://metadataregistry.org/uri/RegStatus/1001" />
  <reg:name xml:lang="en">adaptedAsAVideo</reg:name>
  <rdfs:label xml:lang="en">is adapted as video</rdfs:label>
  <skos:definition xml:lang="en">Relates a resource to a video based on a source resource.</skos:definition>
  <rdf:type rdf:resource="http://www.w3.org/1999/02/22-rdf-syntax-ns#Property" />
  <rdfs:subPropertyOf rdf:resource="http://rdaregistry.info/Elements/u/P60260" />
  <owl:inverseOf rdf:resource="http://rdaregistry.info/Elements/u/P60236" />
  <reg:hasSubproperty rdf:resource="http://rdaregistry.info/Elements/e/P20067" />
  <reg:lexicalAlias rdf:resource="http://rdaregistry.info/Elements/u/adaptedAsAVideo.en" />
</owl:ObjectProperty>

<!-- Property: is adapted as video screenplay -->
<owl:ObjectProperty rdf:about="http://rdaregistry.info/Elements/u/P60187">
  <rdfs:isDefinedBy rdf:resource="http://rdaregistry.info/Elements/u/" />
  <reg:status rdf:resource="http://metadataregistry.org/uri/RegStatus/1001" />
  <reg:name xml:lang="en">adaptedAsAVideoScreenplay</reg:name>
  <rdfs:label xml:lang="en">is adapted as video screenplay</rdfs:label>
  <skos:definition xml:lang="en">Relates a resource to a resource consisting of a screenplay for a video, based on a source resource.</skos:definition>
  <rdf:type rdf:resource="http://www.w3.org/1999/02/22-rdf-syntax-ns#Property" />
  <rdfs:subPropertyOf rdf:resource="http://rdaregistry.info/Elements/u/P60185" />
  <owl:inverseOf rdf:resource="http://rdaregistry.info/Elements/u/P60234" />
  <reg:hasSubproperty rdf:resource="http://rdaregistry.info/Elements/e/P20098" />
  <reg:lexicalAlias rdf:resource="http://rdaregistry.info/Elements/u/adaptedAsAVideoScreenplay.en" />
</owl:ObjectProperty>

<!-- Property: is adapted as choreography -->
<owl:ObjectProperty rdf:about="http://rdaregistry.info/Elements/u/P60180">
  <rdfs:isDefinedBy rdf:resource="http://rdaregistry.info/Elements/u/" />
  <reg:status rdf:resource="http://metadataregistry.org/uri/RegStatus/1001" />
  <reg:name xml:lang="en">adaptedAsChoreography</reg:name>
  <rdfs:label xml:lang="en">is adapted as choreography</rdfs:label>
  <skos:definition xml:lang="en">Relates a resource to a resource consisting of movement based on a source resource.</skos:definition>
  <rdf:type rdf:resource="http://www.w3.org/1999/02/22-rdf-syntax-ns#Property" />
  <rdfs:subPropertyOf rdf:resource="http://rdaregistry.info/Elements/u/P60250" />
  <owl:inverseOf rdf:resource="http://rdaregistry.info/Elements/u/P60293" />
  <reg:hasSubproperty rdf:resource="http://rdaregistry.info/Elements/e/P20092" />
  <reg:lexicalAlias rdf:resource="http://rdaregistry.info/Elements/u/adaptedAsChoreography.en" />
</owl:ObjectProperty>

<!-- Property: is adapted as graphic novel -->
<owl:ObjectProperty rdf:about="http://rdaregistry.info/Elements/u/P60742">
  <rdfs:isDefinedBy rdf:resource="http://rdaregistry.info/Elements/u/" />
  <reg:status rdf:resource="http://metadataregistry.org/uri/RegStatus/1001" />
  <rdf:type rdf:resource="http://www.w3.org/1999/02/22-rdf-syntax-ns#Property" />
  <reg:name xml:lang="en">adaptedAsGraphicNovel</reg:name>
  <rdfs:label xml:lang="en">is adapted as graphic novel</rdfs:label>
  <reg:lexicalAlias rdf:resource="http://rdaregistry.info/Elements/u/adaptedAsGraphicNovel.en" />
  <skos:definition xml:lang="en">Relates a resource to a graphic novel based on a source resource</skos:definition>
  <owl:inverseOf rdf:resource="http://rdaregistry.info/Elements/u/P60743" />
  <rdfs:subPropertyOf rdf:resource="http://rdaregistry.info/Elements/u/P60260" />
</owl:ObjectProperty>

<!-- Property: is adapted as libretto -->
<owl:ObjectProperty rdf:about="http://rdaregistry.info/Elements/u/P60210">
  <rdfs:isDefinedBy rdf:resource="http://rdaregistry.info/Elements/u/" />
  <reg:status rdf:resource="http://metadataregistry.org/uri/RegStatus/1001" />
  <reg:name xml:lang="en">adaptedAsLibretto</reg:name>
  <rdfs:label xml:lang="en">is adapted as libretto</rdfs:label>
  <skos:definition xml:lang="en">Relates a resource to a resource consisting of a text of an opera or other resource for a musical stage, or an oratorio, based on a source resource.</skos:definition>
  <rdf:type rdf:resource="http://www.w3.org/1999/02/22-rdf-syntax-ns#Property" />
  <rdfs:subPropertyOf rdf:resource="http://rdaregistry.info/Elements/u/P60250" />
  <owl:inverseOf rdf:resource="http://rdaregistry.info/Elements/u/P60304" />
  <reg:hasSubproperty rdf:resource="http://rdaregistry.info/Elements/e/P20110" />
  <reg:lexicalAlias rdf:resource="http://rdaregistry.info/Elements/u/adaptedAsLibretto.en" />
</owl:ObjectProperty>

<!-- Property: is adapted as musical theatre -->
<owl:ObjectProperty rdf:about="http://rdaregistry.info/Elements/u/P60721">
  <rdfs:isDefinedBy rdf:resource="http://rdaregistry.info/Elements/u/" />
  <reg:status rdf:resource="http://metadataregistry.org/uri/RegStatus/1001" />
  <reg:name xml:lang="en">adaptedAsMusicalTheatre</reg:name>
  <rdfs:label xml:lang="en">is adapted as musical theatre</rdfs:label>
  <skos:definition xml:lang="en">Relates a resource to a musical theatre resource based on a source resource.</skos:definition>
  <rdf:type rdf:resource="http://www.w3.org/1999/02/22-rdf-syntax-ns#Property" />
  <rdfs:subPropertyOf rdf:resource="http://rdaregistry.info/Elements/u/P60260" />
  <owl:inverseOf rdf:resource="http://rdaregistry.info/Elements/u/P60719" />
  <reg:hasSubproperty rdf:resource="http://rdaregistry.info/Elements/e/P20241" />
  <reg:lexicalAlias rdf:resource="http://rdaregistry.info/Elements/u/adaptedAsMusicalTheatre.en" />
</owl:ObjectProperty>

<!-- Property: is adapted as opera -->
<owl:ObjectProperty rdf:about="http://rdaregistry.info/Elements/u/P60722">
  <rdfs:isDefinedBy rdf:resource="http://rdaregistry.info/Elements/u/" />
  <reg:status rdf:resource="http://metadataregistry.org/uri/RegStatus/1001" />
  <reg:name xml:lang="en">adaptedAsOpera</reg:name>
  <rdfs:label xml:lang="en">is adapted as opera</rdfs:label>
  <skos:definition xml:lang="en">Relates a resource to an opera based on a source resource.</skos:definition>
  <rdf:type rdf:resource="http://www.w3.org/1999/02/22-rdf-syntax-ns#Property" />
  <rdfs:subPropertyOf rdf:resource="http://rdaregistry.info/Elements/u/P60260" />
  <owl:inverseOf rdf:resource="http://rdaregistry.info/Elements/u/P60720" />
  <reg:hasSubproperty rdf:resource="http://rdaregistry.info/Elements/e/P20242" />
  <reg:lexicalAlias rdf:resource="http://rdaregistry.info/Elements/u/adaptedAsOpera.en" />
</owl:ObjectProperty>

<!-- Property: is adapted as oratorio -->
<owl:ObjectProperty rdf:about="http://rdaregistry.info/Elements/u/P60831">
  <rdfs:isDefinedBy rdf:resource="http://rdaregistry.info/Elements/u/" />
  <reg:status rdf:resource="http://metadataregistry.org/uri/RegStatus/1001" />
  <rdf:type rdf:resource="http://www.w3.org/1999/02/22-rdf-syntax-ns#Property" />
  <reg:name xml:lang="en">adaptedAsOratorio</reg:name>
  <rdfs:label xml:lang="en">is adapted as oratorio</rdfs:label>
  <reg:lexicalAlias rdf:resource="http://rdaregistry.info/Elements/u/adaptedAsOratorio.en" />
  <skos:definition xml:lang="en">Relates a resource to an oratorio based on a source resource.</skos:definition>
  <owl:inverseOf rdf:resource="http://rdaregistry.info/Elements/u/P60830" />
  <reg:hasSubproperty rdf:resource="http://rdaregistry.info/Elements/e/P20282" />
  <rdfs:subPropertyOf rdf:resource="http://rdaregistry.info/Elements/u/P60250" />
</owl:ObjectProperty>

<!-- Property: is adapted as screenplay -->
<owl:ObjectProperty rdf:about="http://rdaregistry.info/Elements/u/P60185">
  <rdfs:isDefinedBy rdf:resource="http://rdaregistry.info/Elements/u/" />
  <reg:status rdf:resource="http://metadataregistry.org/uri/RegStatus/1001" />
  <reg:name xml:lang="en">adaptedAsScreenplay</reg:name>
  <rdfs:label xml:lang="en">is adapted as screenplay</rdfs:label>
  <skos:definition xml:lang="en">Relates a resource to a resource consisting of a screenplay for a motion picture, television program, or video, based on a source resource.</skos:definition>
  <rdf:type rdf:resource="http://www.w3.org/1999/02/22-rdf-syntax-ns#Property" />
  <rdfs:subPropertyOf rdf:resource="http://rdaregistry.info/Elements/u/P60260" />
  <owl:inverseOf rdf:resource="http://rdaregistry.info/Elements/u/P60231" />
  <reg:hasSubproperty rdf:resource="http://rdaregistry.info/Elements/u/P60184" />
  <reg:hasSubproperty rdf:resource="http://rdaregistry.info/Elements/u/P60186" />
  <reg:hasSubproperty rdf:resource="http://rdaregistry.info/Elements/u/P60187" />
  <reg:hasSubproperty rdf:resource="http://rdaregistry.info/Elements/e/P20096" />
  <reg:lexicalAlias rdf:resource="http://rdaregistry.info/Elements/u/adaptedAsScreenplay.en" />
</owl:ObjectProperty>

<!-- Property: is adapted as video game -->
<owl:ObjectProperty rdf:about="http://rdaregistry.info/Elements/u/P60744">
  <rdfs:isDefinedBy rdf:resource="http://rdaregistry.info/Elements/u/" />
  <reg:status rdf:resource="http://metadataregistry.org/uri/RegStatus/1001" />
  <rdf:type rdf:resource="http://www.w3.org/1999/02/22-rdf-syntax-ns#Property" />
  <reg:name xml:lang="en">adaptedAsVideoGame</reg:name>
  <rdfs:label xml:lang="en">is adapted as video game</rdfs:label>
  <reg:lexicalAlias rdf:resource="http://rdaregistry.info/Elements/u/adaptedAsVideoGame.en" />
  <skos:definition xml:lang="en">Relates a resource to relates a resource to a video game based on a source resource.</skos:definition>
  <owl:inverseOf rdf:resource="http://rdaregistry.info/Elements/u/P60745" />
  <rdfs:subPropertyOf rdf:resource="http://rdaregistry.info/Elements/u/P60260" />
</owl:ObjectProperty>

<!-- Property: is adapted in verse as -->
<owl:ObjectProperty rdf:about="http://rdaregistry.info/Elements/u/P60106">
  <rdfs:isDefinedBy rdf:resource="http://rdaregistry.info/Elements/u/" />
  <reg:status rdf:resource="http://metadataregistry.org/uri/RegStatus/1001" />
  <reg:name xml:lang="en">adaptedInVerseAs</reg:name>
  <rdfs:label xml:lang="en">is adapted in verse as</rdfs:label>
  <skos:definition xml:lang="en">Relates a resource to a literary composition in verse form adapted from a source resource.</skos:definition>
  <rdf:type rdf:resource="http://www.w3.org/1999/02/22-rdf-syntax-ns#Property" />
  <rdfs:subPropertyOf rdf:resource="http://rdaregistry.info/Elements/u/P60260" />
  <owl:inverseOf rdf:resource="http://rdaregistry.info/Elements/u/P60226" />
  <reg:hasSubproperty rdf:resource="http://rdaregistry.info/Elements/e/P20077" />
  <reg:lexicalAlias rdf:resource="http://rdaregistry.info/Elements/u/adaptedInVerseAs.en" />
</owl:ObjectProperty>

<!-- Property: is addenda -->
<owl:ObjectProperty rdf:about="http://rdaregistry.info/Elements/u/P60209">
  <rdfs:isDefinedBy rdf:resource="http://rdaregistry.info/Elements/u/" />
  <reg:status rdf:resource="http://metadataregistry.org/uri/RegStatus/1001" />
  <reg:name xml:lang="en">addenda</reg:name>
  <rdfs:label xml:lang="en">is addenda</rdfs:label>
  <skos:definition xml:lang="en">Relates a resource to a resource consisting of brief content that is essential for the completeness of another resource.</skos:definition>
  <rdf:type rdf:resource="http://www.w3.org/1999/02/22-rdf-syntax-ns#Property" />
  <rdfs:subPropertyOf rdf:resource="http://rdaregistry.info/Elements/u/P60204" />
  <owl:inverseOf rdf:resource="http://rdaregistry.info/Elements/u/P60286" />
  <reg:hasSubproperty rdf:resource="http://rdaregistry.info/Elements/e/P20109" />
  <reg:lexicalAlias rdf:resource="http://rdaregistry.info/Elements/u/addenda.en" />
</owl:ObjectProperty>

<!-- Property: is addenda to -->
<owl:ObjectProperty rdf:about="http://rdaregistry.info/Elements/u/P60286">
  <rdfs:isDefinedBy rdf:resource="http://rdaregistry.info/Elements/u/" />
  <reg:status rdf:resource="http://metadataregistry.org/uri/RegStatus/1001" />
  <reg:name xml:lang="en">addendaTo</reg:name>
  <rdfs:label xml:lang="en">is addenda to</rdfs:label>
  <skos:definition xml:lang="en">Relates a resource to a resource whose content is completed with brief content from another resource.</skos:definition>
  <rdf:type rdf:resource="http://www.w3.org/1999/02/22-rdf-syntax-ns#Property" />
  <rdfs:subPropertyOf rdf:resource="http://rdaregistry.info/Elements/u/P60307" />
  <owl:inverseOf rdf:resource="http://rdaregistry.info/Elements/u/P60209" />
  <reg:hasSubproperty rdf:resource="http://rdaregistry.info/Elements/e/P20177" />
  <reg:lexicalAlias rdf:resource="http://rdaregistry.info/Elements/u/addendaTo.en" />
</owl:ObjectProperty>

<!-- Property: has additional scale information -->
<owl:ObjectProperty rdf:about="http://rdaregistry.info/Elements/u/P60510">
  <rdfs:isDefinedBy rdf:resource="http://rdaregistry.info/Elements/u/" />
  <reg:status rdf:resource="http://metadataregistry.org/uri/RegStatus/1001" />
  <reg:name xml:lang="en">additionalScaleInformation</reg:name>
  <rdfs:label xml:lang="en">has additional scale information</rdfs:label>
  <skos:definition xml:lang="en">Relates a resource to an indication of supplemental information about scale.</skos:definition>
  <rdf:type rdf:resource="http://www.w3.org/1999/02/22-rdf-syntax-ns#Property" />
  <rdfs:subPropertyOf rdf:resource="http://rdaregistry.info/Elements/u/P60565" />
  <reg:hasSubproperty rdf:resource="http://rdaregistry.info/Elements/e/P20213" />
  <reg:lexicalAlias rdf:resource="http://rdaregistry.info/Elements/u/additionalScaleInformation.en" />
  <skos:scopeNote xml:lang="en">Statement of comparative measurements or limitation of the scale to particular parts of the content of a resource are included.</skos:scopeNote>
</owl:ObjectProperty>

<!-- Property: has addressee -->
<owl:ObjectProperty rdf:about="http://rdaregistry.info/Elements/u/P60456">
  <rdfs:isDefinedBy rdf:resource="http://rdaregistry.info/Elements/u/" />
  <reg:status rdf:resource="http://metadataregistry.org/uri/RegStatus/1001" />
  <reg:name xml:lang="en">addressee</reg:name>
  <rdfs:label xml:lang="en">has addressee</rdfs:label>
  <skos:definition xml:lang="en">Relates a resource to an agent to whom a resource or part of a resource is addressed.</skos:definition>
  <rdf:type rdf:resource="http://www.w3.org/1999/02/22-rdf-syntax-ns#Property" />
  <rdfs:subPropertyOf rdf:resource="http://rdaregistry.info/Elements/u/P60374" />
  <owl:inverseOf rdf:resource="http://rdaregistry.info/Elements/u/P60690" />
  <reg:lexicalAlias rdf:resource="http://rdaregistry.info/Elements/u/addressee.en" />
</owl:ObjectProperty>

<!-- Property: is addressee of -->
<owl:ObjectProperty rdf:about="http://rdaregistry.info/Elements/u/P60690">
  <rdfs:isDefinedBy rdf:resource="http://rdaregistry.info/Elements/u/" />
  <reg:status rdf:resource="http://metadataregistry.org/uri/RegStatus/1001" />
  <reg:name xml:lang="en">addresseeOf</reg:name>
  <rdfs:label xml:lang="en">is addressee of</rdfs:label>
  <skos:definition xml:lang="en">Relates an agent to whom a resource or part of a resource is addressed to a resource.</skos:definition>
  <rdf:type rdf:resource="http://www.w3.org/1999/02/22-rdf-syntax-ns#Property" />
  <rdfs:subPropertyOf rdf:resource="http://rdaregistry.info/Elements/u/P60602" />
  <owl:inverseOf rdf:resource="http://rdaregistry.info/Elements/u/P60456" />
  <reg:hasSubproperty rdf:resource="http://rdaregistry.info/Elements/a/P50209" />
  <reg:lexicalAlias rdf:resource="http://rdaregistry.info/Elements/u/addresseeOf.en" />
</owl:ObjectProperty>

<!-- Property: has address of agent -->
<owl:ObjectProperty rdf:about="http://rdaregistry.info/Elements/u/P60512">
  <rdfs:isDefinedBy rdf:resource="http://rdaregistry.info/Elements/u/" />
  <reg:status rdf:resource="http://metadataregistry.org/uri/RegStatus/1001" />
  <reg:name xml:lang="en">addressOfAgent</reg:name>
  <rdfs:label xml:lang="en">has address of agent</rdfs:label>
  <skos:definition xml:lang="en">Relates a resource to an address of an agent's place of residence, business, or employer, headquarters or offices, or an e-mail or internet address.</skos:definition>
  <rdf:type rdf:resource="http://www.w3.org/1999/02/22-rdf-syntax-ns#Property" />
  <reg:hasSubproperty rdf:resource="http://rdaregistry.info/Elements/a/P50036" />
  <reg:hasSubproperty rdf:resource="http://rdaregistry.info/Elements/a/P50114" />
  <reg:lexicalAlias rdf:resource="http://rdaregistry.info/Elements/u/addressOfAgent.en" />
</owl:ObjectProperty>

<!-- Property: has affiliation -->
<owl:ObjectProperty rdf:about="http://rdaregistry.info/Elements/u/P60095">
  <rdfs:isDefinedBy rdf:resource="http://rdaregistry.info/Elements/u/" />
  <reg:status rdf:resource="http://metadataregistry.org/uri/RegStatus/1001" />
  <reg:name xml:lang="en">affiliation</reg:name>
  <rdfs:label xml:lang="en">has affiliation</rdfs:label>
  <skos:definition xml:lang="en">Relates a resource to a group with which an agent is affiliated or has been affiliated through employment, membership, cultural identity, etc.</skos:definition>
  <rdf:type rdf:resource="http://www.w3.org/1999/02/22-rdf-syntax-ns#Property" />
  <reg:hasSubproperty rdf:resource="http://rdaregistry.info/Elements/a/P50101" />
  <reg:lexicalAlias rdf:resource="http://rdaregistry.info/Elements/u/affiliation.en" />
</owl:ObjectProperty>

<!-- Property: has agent history -->
<owl:ObjectProperty rdf:about="http://rdaregistry.info/Elements/u/P60484">
  <rdfs:isDefinedBy rdf:resource="http://rdaregistry.info/Elements/u/" />
  <reg:status rdf:resource="http://metadataregistry.org/uri/RegStatus/1001" />
  <reg:name xml:lang="en">agentHistory</reg:name>
  <rdfs:label xml:lang="en">has agent history</rdfs:label>
  <skos:definition xml:lang="en">Relates a resource to biographical or historical information about an agent.</skos:definition>
  <rdf:type rdf:resource="http://www.w3.org/1999/02/22-rdf-syntax-ns#Property" />
  <reg:hasSubproperty rdf:resource="http://rdaregistry.info/Elements/a/P50035" />
  <reg:hasSubproperty rdf:resource="http://rdaregistry.info/Elements/a/P50064" />
  <reg:lexicalAlias rdf:resource="http://rdaregistry.info/Elements/u/agentHistory.en" />
</owl:ObjectProperty>

<!-- Property: is also issued as -->
<owl:ObjectProperty rdf:about="http://rdaregistry.info/Elements/u/P60195">
  <rdfs:isDefinedBy rdf:resource="http://rdaregistry.info/Elements/u/" />
  <reg:status rdf:resource="http://metadataregistry.org/uri/RegStatus/1001" />
  <reg:name xml:lang="en">alsoIssuedAs</reg:name>
  <rdfs:label xml:lang="en">is also issued as</rdfs:label>
  <skos:definition xml:lang="en">Relates a resource to a resource that carries the same content of a resource in a different format.</skos:definition>
  <rdf:type rdf:resource="http://www.w3.org/1999/02/22-rdf-syntax-ns#Property" />
  <rdfs:subPropertyOf rdf:resource="http://rdaregistry.info/Elements/u/P60191" />
  <owl:inverseOf rdf:resource="http://rdaregistry.info/Elements/u/P60195" />
  <reg:hasSubproperty rdf:resource="http://rdaregistry.info/Elements/m/P30026" />
  <reg:lexicalAlias rdf:resource="http://rdaregistry.info/Elements/u/alsoIssuedAs.en" />
</owl:ObjectProperty>

<!-- Property: has alternate identity -->
<owl:ObjectProperty rdf:about="http://rdaregistry.info/Elements/u/P60036">
  <rdfs:isDefinedBy rdf:resource="http://rdaregistry.info/Elements/u/" />
  <reg:status rdf:resource="http://metadataregistry.org/uri/RegStatus/1001" />
  <reg:name xml:lang="en">alternateIdentity</reg:name>
  <rdfs:label xml:lang="en">has alternate identity</rdfs:label>
  <skos:definition xml:lang="en">Relates a pseudonymous or other identity assumed by an agent to an agent.</skos:definition>
  <rdf:type rdf:resource="http://www.w3.org/1999/02/22-rdf-syntax-ns#Property" />
  <owl:inverseOf rdf:resource="http://rdaregistry.info/Elements/u/P60037" />
  <reg:hasSubproperty rdf:resource="http://rdaregistry.info/Elements/a/P50105" />
  <reg:lexicalAlias rdf:resource="http://rdaregistry.info/Elements/u/alternateIdentity.en" />
</owl:ObjectProperty>

<!-- Property: has alternative chronological designation of first issue or part of sequence -->
<owl:ObjectProperty rdf:about="http://rdaregistry.info/Elements/u/P60818">
  <rdfs:isDefinedBy rdf:resource="http://rdaregistry.info/Elements/u/" />
  <reg:status rdf:resource="http://metadataregistry.org/uri/RegStatus/1001" />
  <rdf:type rdf:resource="http://www.w3.org/1999/02/22-rdf-syntax-ns#Property" />
  <reg:name xml:lang="en">alternativeChronologicalDesignationOfFirstIssueOrPartOfSequence</reg:name>
  <rdfs:label xml:lang="en">has alternative chronological designation of first issue or part of sequence</rdfs:label>
  <reg:lexicalAlias rdf:resource="http://rdaregistry.info/Elements/u/alternativeChronologicalDesignationOfFirstIssueOrPartOfSequence.en" />
  <skos:definition xml:lang="en">Relates a resource to a second or subsequent system of numbering presented in the form of a date on the first issue or part of a sequence of numbering for a serial.</skos:definition>
  <skos:scopeNote xml:lang="en">Designation includes a year; year and month; month, day, and year. An alternative chronological designation may include a date in a different calendar.</skos:scopeNote>
  <rdfs:subPropertyOf rdf:resource="http://rdaregistry.info/Elements/u/P60533" />
</owl:ObjectProperty>

<!-- Property: has alternative chronological designation of last issue or part of sequence -->
<owl:ObjectProperty rdf:about="http://rdaregistry.info/Elements/u/P60819">
  <rdfs:isDefinedBy rdf:resource="http://rdaregistry.info/Elements/u/" />
  <reg:status rdf:resource="http://metadataregistry.org/uri/RegStatus/1001" />
  <rdf:type rdf:resource="http://www.w3.org/1999/02/22-rdf-syntax-ns#Property" />
  <reg:name xml:lang="en">alternativeChronologicalDesignationOfLastIssueOrPartOfSequence</reg:name>
  <rdfs:label xml:lang="en">has alternative chronological designation of last issue or part of sequence</rdfs:label>
  <reg:lexicalAlias rdf:resource="http://rdaregistry.info/Elements/u/alternativeChronologicalDesignationOfLastIssueOrPartOfSequence.en" />
  <skos:definition xml:lang="en">Relates a resource to a second or subsequent system of numbering presented in the form of a date on the last issue or part of a sequence of numbering for a serial.</skos:definition>
  <skos:scopeNote xml:lang="en">Designational includes a year; year and month; month, day, and year. An alternative chronological designation may include a date in a different calendar.</skos:scopeNote>
  <rdfs:subPropertyOf rdf:resource="http://rdaregistry.info/Elements/u/P60533" />
</owl:ObjectProperty>

<!-- Property: has alternative numeric and/or alphabetic designation of first issue or part of sequence -->
<owl:ObjectProperty rdf:about="http://rdaregistry.info/Elements/u/P60820">
  <rdfs:isDefinedBy rdf:resource="http://rdaregistry.info/Elements/u/" />
  <reg:status rdf:resource="http://metadataregistry.org/uri/RegStatus/1001" />
  <rdf:type rdf:resource="http://www.w3.org/1999/02/22-rdf-syntax-ns#Property" />
  <reg:name xml:lang="en">alternativeNumericAndOrAlphabeticDesignationOfFirstIssueOrPartOfSequence</reg:name>
  <rdfs:label xml:lang="en">has alternative numeric and/or alphabetic designation of first issue or part of sequence</rdfs:label>
  <reg:lexicalAlias rdf:resource="http://rdaregistry.info/Elements/u/alternativeNumericAndOrAlphabeticDesignationOfFirstIssueOrPartOfSequence.en" />
  <skos:definition xml:lang="en">Relates a resource to a second or subsequent system of numbering presented in numeric or alphabetic form on the first issue or part of a sequence of numbering for a serial.</skos:definition>
  <rdfs:subPropertyOf rdf:resource="http://rdaregistry.info/Elements/u/P60533" />
</owl:ObjectProperty>

<!-- Property: has alternative numeric and/or alphabetic designation of last issue or part of sequence -->
<owl:ObjectProperty rdf:about="http://rdaregistry.info/Elements/u/P60821">
  <rdfs:isDefinedBy rdf:resource="http://rdaregistry.info/Elements/u/" />
  <reg:status rdf:resource="http://metadataregistry.org/uri/RegStatus/1001" />
  <rdf:type rdf:resource="http://www.w3.org/1999/02/22-rdf-syntax-ns#Property" />
  <reg:name xml:lang="en">alternativeNumericAndOrAlphabeticDesignationOfLastIssueOrPartOfSequence</reg:name>
  <rdfs:label xml:lang="en">has alternative numeric and/or alphabetic designation of last issue or part of sequence</rdfs:label>
  <reg:lexicalAlias rdf:resource="http://rdaregistry.info/Elements/u/alternativeNumericAndOrAlphabeticDesignationOfLastIssueOrPartOfSequence.en" />
  <skos:definition xml:lang="en">Relates a resource to a second or subsequent system of numbering presented in numeric or alphabetic form on the last issue or part of a sequence of numbering for a serial.</skos:definition>
  <rdfs:subPropertyOf rdf:resource="http://rdaregistry.info/Elements/u/P60533" />
</owl:ObjectProperty>

<!-- Property: is analysed in -->
<owl:ObjectProperty rdf:about="http://rdaregistry.info/Elements/u/P60219">
  <rdfs:isDefinedBy rdf:resource="http://rdaregistry.info/Elements/u/" />
  <reg:status rdf:resource="http://metadataregistry.org/uri/RegStatus/1001" />
  <reg:name xml:lang="en">analysedIn</reg:name>
  <rdfs:label xml:lang="en">is analysed in</rdfs:label>
  <skos:definition xml:lang="en">Relates a resource to a resource that examines a source resource to identify its components and their relations.</skos:definition>
  <rdf:type rdf:resource="http://www.w3.org/1999/02/22-rdf-syntax-ns#Property" />
  <rdfs:subPropertyOf rdf:resource="http://rdaregistry.info/Elements/u/P60215" />
  <owl:inverseOf rdf:resource="http://rdaregistry.info/Elements/u/P60239" />
  <reg:hasSubproperty rdf:resource="http://rdaregistry.info/Elements/e/P20270" />
  <reg:hasSubproperty rdf:resource="http://rdaregistry.info/Elements/i/P40063" />
  <reg:hasSubproperty rdf:resource="http://rdaregistry.info/Elements/m/P30255" />
  <reg:lexicalAlias rdf:resource="http://rdaregistry.info/Elements/u/analysedIn.en" />
</owl:ObjectProperty>

<!-- Property: is analysis of -->
<owl:ObjectProperty rdf:about="http://rdaregistry.info/Elements/u/P60239">
  <rdfs:isDefinedBy rdf:resource="http://rdaregistry.info/Elements/u/" />
  <reg:status rdf:resource="http://metadataregistry.org/uri/RegStatus/1001" />
  <reg:name xml:lang="en">analysisOf</reg:name>
  <rdfs:label xml:lang="en">is analysis of</rdfs:label>
  <skos:definition xml:lang="en">Relates a resource to a resource that has been examined to identify its components and their relations.</skos:definition>
  <rdf:type rdf:resource="http://www.w3.org/1999/02/22-rdf-syntax-ns#Property" />
  <rdfs:subPropertyOf rdf:resource="http://rdaregistry.info/Elements/u/P60190" />
  <owl:inverseOf rdf:resource="http://rdaregistry.info/Elements/u/P60219" />
  <reg:hasSubproperty rdf:resource="http://rdaregistry.info/Elements/w/P10266" />
  <reg:hasSubproperty rdf:resource="http://rdaregistry.info/Elements/w/P10272" />
  <reg:hasSubproperty rdf:resource="http://rdaregistry.info/Elements/w/P10278" />
  <reg:lexicalAlias rdf:resource="http://rdaregistry.info/Elements/u/analysisOf.en" />
</owl:ObjectProperty>

<!-- Property: has animator -->
<owl:ObjectProperty rdf:about="http://rdaregistry.info/Elements/u/P60378">
  <rdfs:isDefinedBy rdf:resource="http://rdaregistry.info/Elements/u/" />
  <reg:status rdf:resource="http://metadataregistry.org/uri/RegStatus/1001" />
  <reg:name xml:lang="en">animator</reg:name>
  <rdfs:label xml:lang="en">has animator</rdfs:label>
  <skos:definition xml:lang="en">Relates a resource to an agent contributing to a moving image resource or computer program by giving apparent movement to inanimate objects or drawings.</skos:definition>
  <rdf:type rdf:resource="http://www.w3.org/1999/02/22-rdf-syntax-ns#Property" />
  <rdfs:subPropertyOf rdf:resource="http://rdaregistry.info/Elements/u/P60398" />
  <owl:inverseOf rdf:resource="http://rdaregistry.info/Elements/u/P60606" />
  <reg:hasSubproperty rdf:resource="http://rdaregistry.info/Elements/e/P20028" />
  <reg:lexicalAlias rdf:resource="http://rdaregistry.info/Elements/u/animator.en" />
  <skos:scopeNote xml:lang="en">Creation of the drawings that are animated is excluded.</skos:scopeNote>
  <rdakit:seeAlso rdf:resource="http://rdaregistry.info/Elements/u/P60431" />
</owl:ObjectProperty>

<!-- Property: is animator of -->
<owl:ObjectProperty rdf:about="http://rdaregistry.info/Elements/u/P60606">
  <rdfs:isDefinedBy rdf:resource="http://rdaregistry.info/Elements/u/" />
  <reg:status rdf:resource="http://metadataregistry.org/uri/RegStatus/1001" />
  <reg:name xml:lang="en">animatorOf</reg:name>
  <rdfs:label xml:lang="en">is animator of</rdfs:label>
  <skos:definition xml:lang="en">Relates an agent contributing to a moving image resource or computer program by giving apparent movement to inanimate objects or drawings to a resource.</skos:definition>
  <rdf:type rdf:resource="http://www.w3.org/1999/02/22-rdf-syntax-ns#Property" />
  <rdfs:subPropertyOf rdf:resource="http://rdaregistry.info/Elements/u/P60626" />
  <owl:inverseOf rdf:resource="http://rdaregistry.info/Elements/u/P60378" />
  <reg:hasSubproperty rdf:resource="http://rdaregistry.info/Elements/a/P50136" />
  <reg:lexicalAlias rdf:resource="http://rdaregistry.info/Elements/u/animatorOf.en" />
  <skos:scopeNote xml:lang="en">Creation of the drawings that are animated is excluded.</skos:scopeNote>
  <rdakit:seeAlso rdf:resource="http://rdaregistry.info/Elements/u/P60660" />
</owl:ObjectProperty>

<!-- Property: has annotator -->
<owl:ObjectProperty rdf:about="http://rdaregistry.info/Elements/u/P60464">
  <rdfs:isDefinedBy rdf:resource="http://rdaregistry.info/Elements/u/" />
  <reg:status rdf:resource="http://metadataregistry.org/uri/RegStatus/1001" />
  <reg:name xml:lang="en">annotator</reg:name>
  <rdfs:label xml:lang="en">has annotator</rdfs:label>
  <skos:definition xml:lang="en">Relates a resource to an agent who makes manuscript annotations on a resource.</skos:definition>
  <rdf:type rdf:resource="http://www.w3.org/1999/02/22-rdf-syntax-ns#Property" />
  <rdfs:subPropertyOf rdf:resource="http://rdaregistry.info/Elements/u/P60374" />
  <owl:inverseOf rdf:resource="http://rdaregistry.info/Elements/u/P60700" />
  <reg:hasSubproperty rdf:resource="http://rdaregistry.info/Elements/i/P40015" />
  <reg:lexicalAlias rdf:resource="http://rdaregistry.info/Elements/u/annotator.en" />
</owl:ObjectProperty>

<!-- Property: is annotator of -->
<owl:ObjectProperty rdf:about="http://rdaregistry.info/Elements/u/P60700">
  <rdfs:isDefinedBy rdf:resource="http://rdaregistry.info/Elements/u/" />
  <reg:status rdf:resource="http://metadataregistry.org/uri/RegStatus/1001" />
  <reg:name xml:lang="en">annotatorOf</reg:name>
  <rdfs:label xml:lang="en">is annotator of</rdfs:label>
  <skos:definition xml:lang="en">Relates an agent who makes manuscript annotations on a resource to a resource.</skos:definition>
  <rdf:type rdf:resource="http://www.w3.org/1999/02/22-rdf-syntax-ns#Property" />
  <rdfs:subPropertyOf rdf:resource="http://rdaregistry.info/Elements/u/P60602" />
  <owl:inverseOf rdf:resource="http://rdaregistry.info/Elements/u/P60464" />
  <reg:hasSubproperty rdf:resource="http://rdaregistry.info/Elements/a/P50128" />
  <reg:lexicalAlias rdf:resource="http://rdaregistry.info/Elements/u/annotatorOf.en" />
</owl:ObjectProperty>

<!-- Property: has appellant -->
<owl:ObjectProperty rdf:about="http://rdaregistry.info/Elements/u/P60457">
  <rdfs:isDefinedBy rdf:resource="http://rdaregistry.info/Elements/u/" />
  <reg:status rdf:resource="http://metadataregistry.org/uri/RegStatus/1001" />
  <reg:name xml:lang="en">appellant</reg:name>
  <rdfs:label xml:lang="en">has appellant</rdfs:label>
  <skos:definition xml:lang="en">Relates a resource to an agent who appeals a decision of a lower court recorded in a legal resource of a higher court.</skos:definition>
  <rdf:type rdf:resource="http://www.w3.org/1999/02/22-rdf-syntax-ns#Property" />
  <rdfs:subPropertyOf rdf:resource="http://rdaregistry.info/Elements/u/P60374" />
  <owl:inverseOf rdf:resource="http://rdaregistry.info/Elements/u/P60691" />
  <reg:lexicalAlias rdf:resource="http://rdaregistry.info/Elements/u/appellant.en" />
</owl:ObjectProperty>

<!-- Property: is appellant of -->
<owl:ObjectProperty rdf:about="http://rdaregistry.info/Elements/u/P60691">
  <rdfs:isDefinedBy rdf:resource="http://rdaregistry.info/Elements/u/" />
  <reg:status rdf:resource="http://metadataregistry.org/uri/RegStatus/1001" />
  <reg:name xml:lang="en">appellantOf</reg:name>
  <rdfs:label xml:lang="en">is appellant of</rdfs:label>
  <skos:definition xml:lang="en">Relates an agent who appeals a decision of a lower court recorded in a legal resource of a higher court to a resource.</skos:definition>
  <rdf:type rdf:resource="http://www.w3.org/1999/02/22-rdf-syntax-ns#Property" />
  <rdfs:subPropertyOf rdf:resource="http://rdaregistry.info/Elements/u/P60602" />
  <owl:inverseOf rdf:resource="http://rdaregistry.info/Elements/u/P60457" />
  <reg:hasSubproperty rdf:resource="http://rdaregistry.info/Elements/a/P50042" />
  <reg:hasSubproperty rdf:resource="http://rdaregistry.info/Elements/a/P50088" />
  <reg:hasSubproperty rdf:resource="http://rdaregistry.info/Elements/a/P50122" />
  <reg:lexicalAlias rdf:resource="http://rdaregistry.info/Elements/u/appellantOf.en" />
</owl:ObjectProperty>

<!-- Property: has appellee -->
<owl:ObjectProperty rdf:about="http://rdaregistry.info/Elements/u/P60373">
  <rdfs:isDefinedBy rdf:resource="http://rdaregistry.info/Elements/u/" />
  <reg:status rdf:resource="http://metadataregistry.org/uri/RegStatus/1001" />
  <reg:name xml:lang="en">appellee</reg:name>
  <rdfs:label xml:lang="en">has appellee</rdfs:label>
  <skos:definition xml:lang="en">Relates a resource to an agent against whom an appeal is taken on a decision of a lower court recorded in a legal resource of a higher court.</skos:definition>
  <rdf:type rdf:resource="http://www.w3.org/1999/02/22-rdf-syntax-ns#Property" />
  <rdfs:subPropertyOf rdf:resource="http://rdaregistry.info/Elements/u/P60374" />
  <owl:inverseOf rdf:resource="http://rdaregistry.info/Elements/u/P60601" />
  <reg:lexicalAlias rdf:resource="http://rdaregistry.info/Elements/u/appellee.en" />
</owl:ObjectProperty>

<!-- Property: is appellee of -->
<owl:ObjectProperty rdf:about="http://rdaregistry.info/Elements/u/P60601">
  <rdfs:isDefinedBy rdf:resource="http://rdaregistry.info/Elements/u/" />
  <reg:status rdf:resource="http://metadataregistry.org/uri/RegStatus/1001" />
  <reg:name xml:lang="en">appelleeOf</reg:name>
  <rdfs:label xml:lang="en">is appellee of</rdfs:label>
  <skos:definition xml:lang="en">Relates an agent against whom an appeal is taken on a decision of a lower court recorded in a legal resource of a higher court to a resource.</skos:definition>
  <rdf:type rdf:resource="http://www.w3.org/1999/02/22-rdf-syntax-ns#Property" />
  <rdfs:subPropertyOf rdf:resource="http://rdaregistry.info/Elements/u/P60602" />
  <owl:inverseOf rdf:resource="http://rdaregistry.info/Elements/u/P60373" />
  <reg:hasSubproperty rdf:resource="http://rdaregistry.info/Elements/a/P50002" />
  <reg:hasSubproperty rdf:resource="http://rdaregistry.info/Elements/a/P50085" />
  <reg:hasSubproperty rdf:resource="http://rdaregistry.info/Elements/a/P50087" />
  <reg:lexicalAlias rdf:resource="http://rdaregistry.info/Elements/u/appelleeOf.en" />
</owl:ObjectProperty>

<!-- Property: is appendix -->
<owl:ObjectProperty rdf:about="http://rdaregistry.info/Elements/u/P60221">
  <rdfs:isDefinedBy rdf:resource="http://rdaregistry.info/Elements/u/" />
  <reg:status rdf:resource="http://metadataregistry.org/uri/RegStatus/1001" />
  <reg:name xml:lang="en">appendix</reg:name>
  <rdfs:label xml:lang="en">is appendix</rdfs:label>
  <skos:definition xml:lang="en">Relates a resource to a resource whose content augments another resource.</skos:definition>
  <rdf:type rdf:resource="http://www.w3.org/1999/02/22-rdf-syntax-ns#Property" />
  <rdfs:subPropertyOf rdf:resource="http://rdaregistry.info/Elements/u/P60204" />
  <owl:inverseOf rdf:resource="http://rdaregistry.info/Elements/u/P60253" />
  <reg:hasSubproperty rdf:resource="http://rdaregistry.info/Elements/e/P20118" />
  <reg:lexicalAlias rdf:resource="http://rdaregistry.info/Elements/u/appendix.en" />
</owl:ObjectProperty>

<!-- Property: is appendix to -->
<owl:ObjectProperty rdf:about="http://rdaregistry.info/Elements/u/P60253">
  <rdfs:isDefinedBy rdf:resource="http://rdaregistry.info/Elements/u/" />
  <reg:status rdf:resource="http://metadataregistry.org/uri/RegStatus/1001" />
  <reg:name xml:lang="en">appendixTo</reg:name>
  <rdfs:label xml:lang="en">is appendix to</rdfs:label>
  <skos:definition xml:lang="en">Relates a resource to a resource whose content is augmented with content from another resource.</skos:definition>
  <rdf:type rdf:resource="http://www.w3.org/1999/02/22-rdf-syntax-ns#Property" />
  <rdfs:subPropertyOf rdf:resource="http://rdaregistry.info/Elements/u/P60307" />
  <owl:inverseOf rdf:resource="http://rdaregistry.info/Elements/u/P60221" />
  <reg:hasSubproperty rdf:resource="http://rdaregistry.info/Elements/e/P20089" />
  <reg:lexicalAlias rdf:resource="http://rdaregistry.info/Elements/u/appendixTo.en" />
</owl:ObjectProperty>

<!-- Property: has applied material -->
<owl:ObjectProperty rdf:about="http://rdaregistry.info/Elements/u/P60159">
  <rdfs:isDefinedBy rdf:resource="http://rdaregistry.info/Elements/u/" />
  <reg:status rdf:resource="http://metadataregistry.org/uri/RegStatus/1001" />
  <reg:name xml:lang="en">appliedMaterial</reg:name>
  <rdfs:label xml:lang="en">has applied material</rdfs:label>
  <skos:definition xml:lang="en">Relates a resource to a physical or chemical substance applied to a base material of a resource.</skos:definition>
  <rdf:type rdf:resource="http://www.w3.org/1999/02/22-rdf-syntax-ns#Property" />
  <reg:hasSubproperty rdf:resource="http://rdaregistry.info/Elements/u/P60344" />
  <reg:hasSubproperty rdf:resource="http://rdaregistry.info/Elements/m/P30084" />
  <reg:lexicalAlias rdf:resource="http://rdaregistry.info/Elements/u/appliedMaterial.en" />
</owl:ObjectProperty>

<!-- Property: has architect -->
<owl:ObjectProperty rdf:about="http://rdaregistry.info/Elements/u/P60435">
  <rdfs:isDefinedBy rdf:resource="http://rdaregistry.info/Elements/u/" />
  <reg:status rdf:resource="http://metadataregistry.org/uri/RegStatus/1001" />
  <reg:name xml:lang="en">architect</reg:name>
  <rdfs:label xml:lang="en">has architect</rdfs:label>
  <skos:definition xml:lang="en">Relates a resource to an agent responsible for creating an architectural design, including a pictorial representation intended to show how a building, etc., will look when completed.</skos:definition>
  <rdf:type rdf:resource="http://www.w3.org/1999/02/22-rdf-syntax-ns#Property" />
  <rdfs:subPropertyOf rdf:resource="http://rdaregistry.info/Elements/u/P60447" />
  <owl:inverseOf rdf:resource="http://rdaregistry.info/Elements/u/P60664" />
  <reg:hasSubproperty rdf:resource="http://rdaregistry.info/Elements/u/P60473" />
  <reg:lexicalAlias rdf:resource="http://rdaregistry.info/Elements/u/architect.en" />
</owl:ObjectProperty>

<!-- Property: is architect of -->
<owl:ObjectProperty rdf:about="http://rdaregistry.info/Elements/u/P60664">
  <rdfs:isDefinedBy rdf:resource="http://rdaregistry.info/Elements/u/" />
  <reg:status rdf:resource="http://metadataregistry.org/uri/RegStatus/1001" />
  <reg:name xml:lang="en">architectOf</reg:name>
  <rdfs:label xml:lang="en">is architect of</rdfs:label>
  <skos:definition xml:lang="en">Relates an agent responsible for creating an architectural design, including a pictorial representation intended to show how a building, etc., will look when completed to a resource.</skos:definition>
  <rdf:type rdf:resource="http://www.w3.org/1999/02/22-rdf-syntax-ns#Property" />
  <rdfs:subPropertyOf rdf:resource="http://rdaregistry.info/Elements/u/P60672" />
  <owl:inverseOf rdf:resource="http://rdaregistry.info/Elements/u/P60435" />
  <reg:hasSubproperty rdf:resource="http://rdaregistry.info/Elements/u/P60704" />
  <reg:hasSubproperty rdf:resource="http://rdaregistry.info/Elements/a/P50196" />
  <reg:lexicalAlias rdf:resource="http://rdaregistry.info/Elements/u/architectOf.en" />
</owl:ObjectProperty>

<!-- Property: is arranged as -->
<owl:ObjectProperty rdf:about="http://rdaregistry.info/Elements/u/P60274">
  <rdfs:isDefinedBy rdf:resource="http://rdaregistry.info/Elements/u/" />
  <reg:status rdf:resource="http://metadataregistry.org/uri/RegStatus/1001" />
  <reg:name xml:lang="en">arrangedAs</reg:name>
  <rdfs:label xml:lang="en">is arranged as</rdfs:label>
  <skos:definition xml:lang="en">Relates a resource to a musical resource that rewrites a source resource for a medium of performance different from that for which a resource was originally intended.</skos:definition>
  <rdf:type rdf:resource="http://www.w3.org/1999/02/22-rdf-syntax-ns#Property" />
  <rdfs:subPropertyOf rdf:resource="http://rdaregistry.info/Elements/u/P60250" />
  <owl:inverseOf rdf:resource="http://rdaregistry.info/Elements/u/P60242" />
  <reg:hasSubproperty rdf:resource="http://rdaregistry.info/Elements/e/P20165" />
  <reg:lexicalAlias rdf:resource="http://rdaregistry.info/Elements/u/arrangedAs.en" />
</owl:ObjectProperty>

<!-- Property: is arrangement of -->
<owl:ObjectProperty rdf:about="http://rdaregistry.info/Elements/u/P60242">
  <rdfs:isDefinedBy rdf:resource="http://rdaregistry.info/Elements/u/" />
  <reg:status rdf:resource="http://metadataregistry.org/uri/RegStatus/1001" />
  <reg:name xml:lang="en">arrangementOf</reg:name>
  <rdfs:label xml:lang="en">is arrangement of</rdfs:label>
  <skos:definition xml:lang="en">Relates a resource to a musical resource that has been rewritten for a medium of performance different from that for which a resource was originally intended.</skos:definition>
  <rdf:type rdf:resource="http://www.w3.org/1999/02/22-rdf-syntax-ns#Property" />
  <rdfs:subPropertyOf rdf:resource="http://rdaregistry.info/Elements/u/P60305" />
  <owl:inverseOf rdf:resource="http://rdaregistry.info/Elements/u/P60274" />
  <reg:hasSubproperty rdf:resource="http://rdaregistry.info/Elements/e/P20139" />
  <reg:lexicalAlias rdf:resource="http://rdaregistry.info/Elements/u/arrangementOf.en" />
</owl:ObjectProperty>

<!-- Property: has arranger of music -->
<owl:ObjectProperty rdf:about="http://rdaregistry.info/Elements/u/P60379">
  <rdfs:isDefinedBy rdf:resource="http://rdaregistry.info/Elements/u/" />
  <reg:status rdf:resource="http://metadataregistry.org/uri/RegStatus/1001" />
  <reg:name xml:lang="en">arrangerOfMusic</reg:name>
  <rdfs:label xml:lang="en">has arranger of music</rdfs:label>
  <skos:definition xml:lang="en">Relates a resource to an agent contributing to a musical resource by rewriting a composition for a medium of performance different from that for which a resource was originally intended.</skos:definition>
  <rdf:type rdf:resource="http://www.w3.org/1999/02/22-rdf-syntax-ns#Property" />
  <rdfs:subPropertyOf rdf:resource="http://rdaregistry.info/Elements/u/P60398" />
  <owl:inverseOf rdf:resource="http://rdaregistry.info/Elements/u/P60607" />
  <reg:hasSubproperty rdf:resource="http://rdaregistry.info/Elements/e/P20029" />
  <reg:lexicalAlias rdf:resource="http://rdaregistry.info/Elements/u/arrangerOfMusic.en" />
  <skos:scopeNote xml:lang="en">Modification of the resource for the same medium of performance, etc., keeping the musical substance of the original composition essentially unchanged, is included.  Substantial modification that results in the creation of a new musical resource is excluded.</skos:scopeNote>
  <rdakit:seeAlso rdf:resource="http://rdaregistry.info/Elements/u/P60426" />
</owl:ObjectProperty>

<!-- Property: is arranger of music of -->
<owl:ObjectProperty rdf:about="http://rdaregistry.info/Elements/u/P60607">
  <rdfs:isDefinedBy rdf:resource="http://rdaregistry.info/Elements/u/" />
  <reg:status rdf:resource="http://metadataregistry.org/uri/RegStatus/1001" />
  <reg:name xml:lang="en">arrangerOfMusicOf</reg:name>
  <rdfs:label xml:lang="en">is arranger of music of</rdfs:label>
  <skos:definition xml:lang="en">Relates an agent contributing to a musical resource by rewriting a composition for a medium of performance different from that for which a resource was originally intended to a resource.</skos:definition>
  <rdf:type rdf:resource="http://www.w3.org/1999/02/22-rdf-syntax-ns#Property" />
  <rdfs:subPropertyOf rdf:resource="http://rdaregistry.info/Elements/u/P60626" />
  <owl:inverseOf rdf:resource="http://rdaregistry.info/Elements/u/P60379" />
  <reg:hasSubproperty rdf:resource="http://rdaregistry.info/Elements/a/P50137" />
  <reg:lexicalAlias rdf:resource="http://rdaregistry.info/Elements/u/arrangerOfMusicOf.en" />
  <rdakit:seeAlso rdf:resource="http://rdaregistry.info/Elements/u/P60655" />
</owl:ObjectProperty>

<!-- Property: has art director -->
<owl:ObjectProperty rdf:about="http://rdaregistry.info/Elements/u/P60386">
  <rdfs:isDefinedBy rdf:resource="http://rdaregistry.info/Elements/u/" />
  <reg:status rdf:resource="http://metadataregistry.org/uri/RegStatus/1001" />
  <reg:name xml:lang="en">artDirector</reg:name>
  <rdfs:label xml:lang="en">has art director</rdfs:label>
  <skos:definition xml:lang="en">Relates a resource to an agent contributing to a resource by overseeing artists and craftspeople who build sets for moving image productions.</skos:definition>
  <rdf:type rdf:resource="http://www.w3.org/1999/02/22-rdf-syntax-ns#Property" />
  <rdfs:subPropertyOf rdf:resource="http://rdaregistry.info/Elements/u/P60398" />
  <owl:inverseOf rdf:resource="http://rdaregistry.info/Elements/u/P60614" />
  <reg:hasSubproperty rdf:resource="http://rdaregistry.info/Elements/e/P20038" />
  <reg:lexicalAlias rdf:resource="http://rdaregistry.info/Elements/u/artDirector.en" />
</owl:ObjectProperty>

<!-- Property: is art director of -->
<owl:ObjectProperty rdf:about="http://rdaregistry.info/Elements/u/P60614">
  <rdfs:isDefinedBy rdf:resource="http://rdaregistry.info/Elements/u/" />
  <reg:status rdf:resource="http://metadataregistry.org/uri/RegStatus/1001" />
  <reg:name xml:lang="en">artDirectorOf</reg:name>
  <rdfs:label xml:lang="en">is art director of</rdfs:label>
  <skos:definition xml:lang="en">Relates an agent contributing to a resource by overseeing artists and craftspeople who build sets for moving image productions to a resource.</skos:definition>
  <rdf:type rdf:resource="http://www.w3.org/1999/02/22-rdf-syntax-ns#Property" />
  <rdfs:subPropertyOf rdf:resource="http://rdaregistry.info/Elements/u/P60626" />
  <owl:inverseOf rdf:resource="http://rdaregistry.info/Elements/u/P60386" />
  <reg:hasSubproperty rdf:resource="http://rdaregistry.info/Elements/a/P50146" />
  <reg:lexicalAlias rdf:resource="http://rdaregistry.info/Elements/u/artDirectorOf.en" />
</owl:ObjectProperty>

<!-- Property: has artist -->
<owl:ObjectProperty rdf:about="http://rdaregistry.info/Elements/u/P60431">
  <rdfs:isDefinedBy rdf:resource="http://rdaregistry.info/Elements/u/" />
  <reg:status rdf:resource="http://metadataregistry.org/uri/RegStatus/1001" />
  <reg:name xml:lang="en">artist</reg:name>
  <rdfs:label xml:lang="en">has artist</rdfs:label>
  <skos:definition xml:lang="en">Relates a resource to an agent responsible for creating a resource by conceiving, and often implementing, an original graphic design, drawing, painting, etc.</skos:definition>
  <rdf:type rdf:resource="http://www.w3.org/1999/02/22-rdf-syntax-ns#Property" />
  <rdfs:subPropertyOf rdf:resource="http://rdaregistry.info/Elements/u/P60447" />
  <owl:inverseOf rdf:resource="http://rdaregistry.info/Elements/u/P60660" />
  <reg:hasSubproperty rdf:resource="http://rdaregistry.info/Elements/u/P60475" />
  <reg:lexicalAlias rdf:resource="http://rdaregistry.info/Elements/u/artist.en" />
  <reg:hasSubproperty rdf:resource="http://rdaregistry.info/Elements/u/P60752" />
  <reg:hasSubproperty rdf:resource="http://rdaregistry.info/Elements/u/P60753" />
</owl:ObjectProperty>

<!-- Property: DEPRECATED -->
<owl:ObjectProperty rdf:about="http://rdaregistry.info/Elements/u/P60105">
  <rdfs:isDefinedBy rdf:resource="http://rdaregistry.info/Elements/u/" />
  <reg:status rdf:resource="http://metadataregistry.org/uri/RegStatus/1008" />
</owl:ObjectProperty>

<!-- Property: is artist of -->
<owl:ObjectProperty rdf:about="http://rdaregistry.info/Elements/u/P60660">
  <rdfs:isDefinedBy rdf:resource="http://rdaregistry.info/Elements/u/" />
  <reg:status rdf:resource="http://metadataregistry.org/uri/RegStatus/1001" />
  <reg:name xml:lang="en">artistOf</reg:name>
  <rdfs:label xml:lang="en">is artist of</rdfs:label>
  <skos:definition xml:lang="en">Relates an agent responsible for creating a resource by conceiving, and often implementing, an original graphic design, drawing, painting, etc. to a resource.</skos:definition>
  <rdf:type rdf:resource="http://www.w3.org/1999/02/22-rdf-syntax-ns#Property" />
  <rdfs:subPropertyOf rdf:resource="http://rdaregistry.info/Elements/u/P60672" />
  <owl:inverseOf rdf:resource="http://rdaregistry.info/Elements/u/P60431" />
  <reg:hasSubproperty rdf:resource="http://rdaregistry.info/Elements/u/P60705" />
  <reg:hasSubproperty rdf:resource="http://rdaregistry.info/Elements/a/P50192" />
  <reg:lexicalAlias rdf:resource="http://rdaregistry.info/Elements/u/artistOf.en" />
  <reg:hasSubproperty rdf:resource="http://rdaregistry.info/Elements/u/P60758" />
  <reg:hasSubproperty rdf:resource="http://rdaregistry.info/Elements/u/P60759" />
</owl:ObjectProperty>

<!-- Property: has aspect ratio -->
<owl:ObjectProperty rdf:about="http://rdaregistry.info/Elements/u/P60566">
  <rdfs:isDefinedBy rdf:resource="http://rdaregistry.info/Elements/u/" />
  <reg:status rdf:resource="http://metadataregistry.org/uri/RegStatus/1001" />
  <reg:name xml:lang="en">aspectRatio</reg:name>
  <rdfs:label xml:lang="en">has aspect ratio</rdfs:label>
  <skos:definition xml:lang="en">Relates a resource to a numerical ratio of the width to the height of a moving image.</skos:definition>
  <rdf:type rdf:resource="http://www.w3.org/1999/02/22-rdf-syntax-ns#Property" />
  <reg:hasSubproperty rdf:resource="http://rdaregistry.info/Elements/e/P20229" />
  <reg:lexicalAlias rdf:resource="http://rdaregistry.info/Elements/u/aspectRatio.en" />
</owl:ObjectProperty>

<!-- Property: has aspect ratio designation -->
<owl:ObjectProperty rdf:about="http://rdaregistry.info/Elements/u/P60873">
  <rdfs:isDefinedBy rdf:resource="http://rdaregistry.info/Elements/u/" />
  <reg:status rdf:resource="http://metadataregistry.org/uri/RegStatus/1001" />
  <rdf:type rdf:resource="http://www.w3.org/1999/02/22-rdf-syntax-ns#Property" />
  <reg:name xml:lang="en">aspectRatioDesignation</reg:name>
  <rdfs:label xml:lang="en">has aspect ratio designation</rdfs:label>
  <reg:lexicalAlias rdf:resource="http://rdaregistry.info/Elements/u/aspectRatioDesignation.en" />
  <skos:definition xml:lang="en">Relates a resource to a general designation of the ratio of the width to the height of a moving image.</skos:definition>
  <reg:hasSubproperty rdf:resource="http://rdaregistry.info/Elements/e/P20290" />
</owl:ObjectProperty>

<!-- Property: has assistant -->
<owl:ObjectProperty rdf:about="http://rdaregistry.info/Elements/u/P60857">
  <rdfs:isDefinedBy rdf:resource="http://rdaregistry.info/Elements/u/" />
  <reg:status rdf:resource="http://metadataregistry.org/uri/RegStatus/1001" />
  <rdf:type rdf:resource="http://www.w3.org/1999/02/22-rdf-syntax-ns#Property" />
  <reg:name xml:lang="en">assistant</reg:name>
  <rdfs:label xml:lang="en">has assistant</rdfs:label>
  <reg:lexicalAlias rdf:resource="http://rdaregistry.info/Elements/u/assistant.en" />
  <skos:definition xml:lang="en">Relates an agent to a colleague who helps another agent.</skos:definition>
  <owl:inverseOf rdf:resource="http://rdaregistry.info/Elements/u/P60588" />
  <reg:hasSubproperty rdf:resource="http://rdaregistry.info/Elements/a/P50275" />
  <rdfs:subPropertyOf rdf:resource="http://rdaregistry.info/Elements/u/P60853" />
</owl:ObjectProperty>

<!-- Property: is assistant to -->
<owl:ObjectProperty rdf:about="http://rdaregistry.info/Elements/u/P60858">
  <rdfs:isDefinedBy rdf:resource="http://rdaregistry.info/Elements/u/" />
  <reg:status rdf:resource="http://metadataregistry.org/uri/RegStatus/1001" />
  <rdf:type rdf:resource="http://www.w3.org/1999/02/22-rdf-syntax-ns#Property" />
  <reg:name xml:lang="en">assistantTo</reg:name>
  <rdfs:label xml:lang="en">is assistant to</rdfs:label>
  <reg:lexicalAlias rdf:resource="http://rdaregistry.info/Elements/u/assistantTo.en" />
  <skos:definition xml:lang="en">Relates an agent to a colleague who is helped by another agent.</skos:definition>
  <owl:inverseOf rdf:resource="http://rdaregistry.info/Elements/u/P60587" />
  <reg:hasSubproperty rdf:resource="http://rdaregistry.info/Elements/a/P50276" />
  <rdfs:subPropertyOf rdf:resource="http://rdaregistry.info/Elements/u/P60853" />
</owl:ObjectProperty>

<!-- Property: has associated institution -->
<owl:ObjectProperty rdf:about="http://rdaregistry.info/Elements/u/P60482">
  <rdfs:isDefinedBy rdf:resource="http://rdaregistry.info/Elements/u/" />
  <reg:status rdf:resource="http://metadataregistry.org/uri/RegStatus/1001" />
  <reg:name xml:lang="en">associatedInstitution</reg:name>
  <rdfs:label xml:lang="en">has associated institution</rdfs:label>
  <skos:definition xml:lang="en">Relates a resource to an institution commonly associated with an agent.</skos:definition>
  <rdf:type rdf:resource="http://www.w3.org/1999/02/22-rdf-syntax-ns#Property" />
  <reg:hasSubproperty rdf:resource="http://rdaregistry.info/Elements/a/P50034" />
  <reg:lexicalAlias rdf:resource="http://rdaregistry.info/Elements/u/associatedInstitution.en" />
</owl:ObjectProperty>

<!-- Property: has audio engineer -->
<owl:ObjectProperty rdf:about="http://rdaregistry.info/Elements/u/P60892">
  <rdfs:isDefinedBy rdf:resource="http://rdaregistry.info/Elements/u/" />
  <reg:status rdf:resource="http://metadataregistry.org/uri/RegStatus/1001" />
  <rdf:type rdf:resource="http://www.w3.org/1999/02/22-rdf-syntax-ns#Property" />
  <reg:name xml:lang="en">audioEngineer</reg:name>
  <rdfs:label xml:lang="en">has audio engineer</rdfs:label>
  <reg:lexicalAlias rdf:resource="http://rdaregistry.info/Elements/u/audioEngineer.en" />
  <skos:definition xml:lang="en">Relates a resource to an agent contributing to the audio content of a resource by managing the technical aspects of sound during the processes of recording, mixing, and reproduction.</skos:definition>
  <owl:inverseOf rdf:resource="http://rdaregistry.info/Elements/u/P60884" />
  <reg:hasSubproperty rdf:resource="http://rdaregistry.info/Elements/e/P20292" />
  <rdfs:subPropertyOf rdf:resource="http://rdaregistry.info/Elements/u/P60398" />
  <reg:hasSubproperty rdf:resource="http://rdaregistry.info/Elements/u/P60893" />
</owl:ObjectProperty>

<!-- Property: is audio engineer of -->
<owl:ObjectProperty rdf:about="http://rdaregistry.info/Elements/u/P60884">
  <rdfs:isDefinedBy rdf:resource="http://rdaregistry.info/Elements/u/" />
  <reg:status rdf:resource="http://metadataregistry.org/uri/RegStatus/1001" />
  <rdf:type rdf:resource="http://www.w3.org/1999/02/22-rdf-syntax-ns#Property" />
  <reg:name xml:lang="en">audioEngineerOf</reg:name>
  <rdfs:label xml:lang="en">is audio engineer of</rdfs:label>
  <reg:lexicalAlias rdf:resource="http://rdaregistry.info/Elements/u/audioEngineerOf.en" />
  <skos:definition xml:lang="en">Relates an agent to a resource that incorporates a contribution to the audio content of managing the technical aspects of sound during the processes of recording, mixing, and reproduction.</skos:definition>
  <owl:inverseOf rdf:resource="http://rdaregistry.info/Elements/u/P60892" />
  <rdfs:subPropertyOf rdf:resource="http://rdaregistry.info/Elements/u/P60158" />
  <reg:hasSubproperty rdf:resource="http://rdaregistry.info/Elements/u/P60885" />
  <reg:hasSubproperty rdf:resource="http://rdaregistry.info/Elements/a/P50296" />
</owl:ObjectProperty>

<!-- Property: has audio producer -->
<owl:ObjectProperty rdf:about="http://rdaregistry.info/Elements/u/P60889">
  <rdfs:isDefinedBy rdf:resource="http://rdaregistry.info/Elements/u/" />
  <reg:status rdf:resource="http://metadataregistry.org/uri/RegStatus/1001" />
  <rdf:type rdf:resource="http://www.w3.org/1999/02/22-rdf-syntax-ns#Property" />
  <reg:name xml:lang="en">audioProducer</reg:name>
  <rdfs:label xml:lang="en">has audio producer</rdfs:label>
  <reg:lexicalAlias rdf:resource="http://rdaregistry.info/Elements/u/audioProducer.en" />
  <skos:definition xml:lang="en">Relates a resource to a producer responsible for most of the business aspects of an audio recording.</skos:definition>
  <owl:inverseOf rdf:resource="http://rdaregistry.info/Elements/u/P60883" />
  <reg:hasSubproperty rdf:resource="http://rdaregistry.info/Elements/w/P10304" />
  <rdfs:subPropertyOf rdf:resource="http://rdaregistry.info/Elements/u/P60441" />
</owl:ObjectProperty>

<!-- Property: is audio producer of -->
<owl:ObjectProperty rdf:about="http://rdaregistry.info/Elements/u/P60883">
  <rdfs:isDefinedBy rdf:resource="http://rdaregistry.info/Elements/u/" />
  <reg:status rdf:resource="http://metadataregistry.org/uri/RegStatus/1001" />
  <rdf:type rdf:resource="http://www.w3.org/1999/02/22-rdf-syntax-ns#Property" />
  <reg:name xml:lang="en">audioProducerOf</reg:name>
  <rdfs:label xml:lang="en">is audio producer of</rdfs:label>
  <reg:lexicalAlias rdf:resource="http://rdaregistry.info/Elements/u/audioProducerOf.en" />
  <skos:definition xml:lang="en">Relates an agent to a resource that involves a responsibility for most of the business aspects of an audio recording.</skos:definition>
  <owl:inverseOf rdf:resource="http://rdaregistry.info/Elements/u/P60889" />
  <rdfs:subPropertyOf rdf:resource="http://rdaregistry.info/Elements/u/P60668" />
  <reg:hasSubproperty rdf:resource="http://rdaregistry.info/Elements/a/P50295" />
</owl:ObjectProperty>

<!-- Property: is augmentation of -->
<owl:ObjectProperty rdf:about="http://rdaregistry.info/Elements/u/P60307">
  <rdfs:isDefinedBy rdf:resource="http://rdaregistry.info/Elements/u/" />
  <reg:status rdf:resource="http://metadataregistry.org/uri/RegStatus/1001" />
  <reg:name xml:lang="en">augmentationOf</reg:name>
  <rdfs:label xml:lang="en">is augmentation of</rdfs:label>
  <skos:definition xml:lang="en">Relates a resource to a resource whose content is added to by another resource.</skos:definition>
  <rdf:type rdf:resource="http://www.w3.org/1999/02/22-rdf-syntax-ns#Property" />
  <rdfs:subPropertyOf rdf:resource="http://rdaregistry.info/Elements/u/P60709" />
  <owl:inverseOf rdf:resource="http://rdaregistry.info/Elements/u/P60204" />
  <reg:hasSubproperty rdf:resource="http://rdaregistry.info/Elements/u/P60116" />
  <reg:hasSubproperty rdf:resource="http://rdaregistry.info/Elements/u/P60251" />
  <reg:hasSubproperty rdf:resource="http://rdaregistry.info/Elements/u/P60252" />
  <reg:hasSubproperty rdf:resource="http://rdaregistry.info/Elements/u/P60253" />
  <reg:hasSubproperty rdf:resource="http://rdaregistry.info/Elements/u/P60254" />
  <reg:hasSubproperty rdf:resource="http://rdaregistry.info/Elements/u/P60259" />
  <reg:hasSubproperty rdf:resource="http://rdaregistry.info/Elements/u/P60286" />
  <reg:hasSubproperty rdf:resource="http://rdaregistry.info/Elements/u/P60290" />
  <reg:hasSubproperty rdf:resource="http://rdaregistry.info/Elements/u/P60291" />
  <reg:hasSubproperty rdf:resource="http://rdaregistry.info/Elements/u/P60302" />
  <reg:hasSubproperty rdf:resource="http://rdaregistry.info/Elements/u/P60474" />
  <reg:hasSubproperty rdf:resource="http://rdaregistry.info/Elements/e/P20192" />
  <reg:lexicalAlias rdf:resource="http://rdaregistry.info/Elements/u/augmentationOf.en" />
</owl:ObjectProperty>

<!-- Property: is augmented by -->
<owl:ObjectProperty rdf:about="http://rdaregistry.info/Elements/u/P60204">
  <rdfs:isDefinedBy rdf:resource="http://rdaregistry.info/Elements/u/" />
  <reg:status rdf:resource="http://metadataregistry.org/uri/RegStatus/1001" />
  <reg:name xml:lang="en">augmentedBy</reg:name>
  <rdfs:label xml:lang="en">is augmented by</rdfs:label>
  <skos:definition xml:lang="en">Relates a resource to a resource that adds to the content of a predominant resource.</skos:definition>
  <rdf:type rdf:resource="http://www.w3.org/1999/02/22-rdf-syntax-ns#Property" />
  <rdfs:subPropertyOf rdf:resource="http://rdaregistry.info/Elements/u/P60709" />
  <owl:inverseOf rdf:resource="http://rdaregistry.info/Elements/u/P60307" />
  <reg:hasSubproperty rdf:resource="http://rdaregistry.info/Elements/u/P60113" />
  <reg:hasSubproperty rdf:resource="http://rdaregistry.info/Elements/u/P60181" />
  <reg:hasSubproperty rdf:resource="http://rdaregistry.info/Elements/u/P60182" />
  <reg:hasSubproperty rdf:resource="http://rdaregistry.info/Elements/u/P60206" />
  <reg:hasSubproperty rdf:resource="http://rdaregistry.info/Elements/u/P60208" />
  <reg:hasSubproperty rdf:resource="http://rdaregistry.info/Elements/u/P60209" />
  <reg:hasSubproperty rdf:resource="http://rdaregistry.info/Elements/u/P60221" />
  <reg:hasSubproperty rdf:resource="http://rdaregistry.info/Elements/u/P60222" />
  <reg:hasSubproperty rdf:resource="http://rdaregistry.info/Elements/u/P60262" />
  <reg:hasSubproperty rdf:resource="http://rdaregistry.info/Elements/u/P60263" />
  <reg:hasSubproperty rdf:resource="http://rdaregistry.info/Elements/u/P60281" />
  <reg:hasSubproperty rdf:resource="http://rdaregistry.info/Elements/e/P20105" />
  <reg:lexicalAlias rdf:resource="http://rdaregistry.info/Elements/u/augmentedBy.en" />
</owl:ObjectProperty>

<!-- Property: has author -->
<owl:ObjectProperty rdf:about="http://rdaregistry.info/Elements/u/P60434">
  <rdfs:isDefinedBy rdf:resource="http://rdaregistry.info/Elements/u/" />
  <reg:status rdf:resource="http://metadataregistry.org/uri/RegStatus/1001" />
  <reg:name xml:lang="en">author</reg:name>
  <rdfs:label xml:lang="en">has author</rdfs:label>
  <skos:definition xml:lang="en">Relates a resource to an agent responsible for creating a resource that is primarily textual in content, regardless of media type or genre.</skos:definition>
  <rdf:type rdf:resource="http://www.w3.org/1999/02/22-rdf-syntax-ns#Property" />
  <rdfs:subPropertyOf rdf:resource="http://rdaregistry.info/Elements/u/P60447" />
  <owl:inverseOf rdf:resource="http://rdaregistry.info/Elements/u/P60663" />
  <reg:hasSubproperty rdf:resource="http://rdaregistry.info/Elements/u/P60476" />
  <reg:hasSubproperty rdf:resource="http://rdaregistry.info/Elements/u/P60477" />
  <reg:hasSubproperty rdf:resource="http://rdaregistry.info/Elements/u/P60478" />
  <reg:lexicalAlias rdf:resource="http://rdaregistry.info/Elements/u/author.en" />
  <reg:hasSubproperty rdf:resource="http://rdaregistry.info/Elements/u/P60751" />
</owl:ObjectProperty>

<!-- Property: is author of -->
<owl:ObjectProperty rdf:about="http://rdaregistry.info/Elements/u/P60663">
  <rdfs:isDefinedBy rdf:resource="http://rdaregistry.info/Elements/u/" />
  <reg:status rdf:resource="http://metadataregistry.org/uri/RegStatus/1001" />
  <reg:name xml:lang="en">authorOf</reg:name>
  <rdfs:label xml:lang="en">is author of</rdfs:label>
  <skos:definition xml:lang="en">Relates an agent responsible for creating a resource that is primarily textual in content, regardless of media  type or genre to a resource.</skos:definition>
  <rdf:type rdf:resource="http://www.w3.org/1999/02/22-rdf-syntax-ns#Property" />
  <rdfs:subPropertyOf rdf:resource="http://rdaregistry.info/Elements/u/P60672" />
  <owl:inverseOf rdf:resource="http://rdaregistry.info/Elements/u/P60434" />
  <reg:hasSubproperty rdf:resource="http://rdaregistry.info/Elements/u/P60706" />
  <reg:hasSubproperty rdf:resource="http://rdaregistry.info/Elements/u/P60707" />
  <reg:hasSubproperty rdf:resource="http://rdaregistry.info/Elements/u/P60708" />
  <reg:hasSubproperty rdf:resource="http://rdaregistry.info/Elements/a/P50195" />
  <reg:lexicalAlias rdf:resource="http://rdaregistry.info/Elements/u/authorOf.en" />
  <reg:hasSubproperty rdf:resource="http://rdaregistry.info/Elements/u/P60757" />
</owl:ObjectProperty>

<!-- Property: has autographer -->
<owl:ObjectProperty rdf:about="http://rdaregistry.info/Elements/u/P60466">
  <rdfs:isDefinedBy rdf:resource="http://rdaregistry.info/Elements/u/" />
  <reg:status rdf:resource="http://metadataregistry.org/uri/RegStatus/1001" />
  <reg:name xml:lang="en">autographer</reg:name>
  <rdfs:label xml:lang="en">has autographer</rdfs:label>
  <skos:definition xml:lang="en">Relates a resource to an agent whose manuscript signature appears on a resource.</skos:definition>
  <rdf:type rdf:resource="http://www.w3.org/1999/02/22-rdf-syntax-ns#Property" />
  <rdfs:subPropertyOf rdf:resource="http://rdaregistry.info/Elements/u/P60374" />
  <owl:inverseOf rdf:resource="http://rdaregistry.info/Elements/u/P60702" />
  <reg:hasSubproperty rdf:resource="http://rdaregistry.info/Elements/i/P40016" />
  <reg:lexicalAlias rdf:resource="http://rdaregistry.info/Elements/u/autographer.en" />
</owl:ObjectProperty>

<!-- Property: is autographer of -->
<owl:ObjectProperty rdf:about="http://rdaregistry.info/Elements/u/P60702">
  <rdfs:isDefinedBy rdf:resource="http://rdaregistry.info/Elements/u/" />
  <reg:status rdf:resource="http://metadataregistry.org/uri/RegStatus/1001" />
  <reg:name xml:lang="en">autographerOf</reg:name>
  <rdfs:label xml:lang="en">is autographer of</rdfs:label>
  <skos:definition xml:lang="en">Relates an agent whose manuscript signature appears on a resource to a resource.</skos:definition>
  <rdf:type rdf:resource="http://www.w3.org/1999/02/22-rdf-syntax-ns#Property" />
  <rdfs:subPropertyOf rdf:resource="http://rdaregistry.info/Elements/u/P60602" />
  <owl:inverseOf rdf:resource="http://rdaregistry.info/Elements/u/P60466" />
  <reg:hasSubproperty rdf:resource="http://rdaregistry.info/Elements/a/P50129" />
  <reg:lexicalAlias rdf:resource="http://rdaregistry.info/Elements/u/autographerOf.en" />
</owl:ObjectProperty>

<!-- Property: has award -->
<owl:ObjectProperty rdf:about="http://rdaregistry.info/Elements/u/P60090">
  <rdfs:isDefinedBy rdf:resource="http://rdaregistry.info/Elements/u/" />
  <reg:status rdf:resource="http://metadataregistry.org/uri/RegStatus/1001" />
  <reg:name xml:lang="en">award</reg:name>
  <rdfs:label xml:lang="en">has award</rdfs:label>
  <skos:definition xml:lang="en">Relates a resource to a formal recognition of excellence, etc., given by an award- or prize-granting body, for the content of a resource.</skos:definition>
  <rdf:type rdf:resource="http://www.w3.org/1999/02/22-rdf-syntax-ns#Property" />
  <reg:hasSubproperty rdf:resource="http://rdaregistry.info/Elements/e/P20005" />
  <reg:lexicalAlias rdf:resource="http://rdaregistry.info/Elements/u/award.en" />
</owl:ObjectProperty>

<!-- Property: is based on -->
<owl:ObjectProperty rdf:about="http://rdaregistry.info/Elements/u/P60305">
  <rdfs:isDefinedBy rdf:resource="http://rdaregistry.info/Elements/u/" />
  <reg:status rdf:resource="http://metadataregistry.org/uri/RegStatus/1001" />
  <reg:name xml:lang="en">basedOn</reg:name>
  <rdfs:label xml:lang="en">is based on</rdfs:label>
  <skos:definition xml:lang="en">Relates a resource to a resource used as a source for a derivative resource.</skos:definition>
  <rdf:type rdf:resource="http://www.w3.org/1999/02/22-rdf-syntax-ns#Property" />
  <rdfs:subPropertyOf rdf:resource="http://rdaregistry.info/Elements/u/P60710" />
  <owl:inverseOf rdf:resource="http://rdaregistry.info/Elements/u/P60250" />
  <reg:hasSubproperty rdf:resource="http://rdaregistry.info/Elements/u/P60114" />
  <reg:hasSubproperty rdf:resource="http://rdaregistry.info/Elements/u/P60223" />
  <reg:hasSubproperty rdf:resource="http://rdaregistry.info/Elements/u/P60224" />
  <reg:hasSubproperty rdf:resource="http://rdaregistry.info/Elements/u/P60238" />
  <reg:hasSubproperty rdf:resource="http://rdaregistry.info/Elements/u/P60241" />
  <reg:hasSubproperty rdf:resource="http://rdaregistry.info/Elements/u/P60242" />
  <reg:hasSubproperty rdf:resource="http://rdaregistry.info/Elements/u/P60243" />
  <reg:hasSubproperty rdf:resource="http://rdaregistry.info/Elements/u/P60244" />
  <reg:hasSubproperty rdf:resource="http://rdaregistry.info/Elements/u/P60266" />
  <reg:hasSubproperty rdf:resource="http://rdaregistry.info/Elements/u/P60289" />
  <reg:hasSubproperty rdf:resource="http://rdaregistry.info/Elements/u/P60293" />
  <reg:hasSubproperty rdf:resource="http://rdaregistry.info/Elements/u/P60294" />
  <reg:hasSubproperty rdf:resource="http://rdaregistry.info/Elements/u/P60295" />
  <reg:hasSubproperty rdf:resource="http://rdaregistry.info/Elements/u/P60296" />
  <reg:hasSubproperty rdf:resource="http://rdaregistry.info/Elements/u/P60303" />
  <reg:hasSubproperty rdf:resource="http://rdaregistry.info/Elements/u/P60304" />
  <reg:hasSubproperty rdf:resource="http://rdaregistry.info/Elements/u/P60308" />
  <reg:hasSubproperty rdf:resource="http://rdaregistry.info/Elements/u/P60309" />
  <reg:hasSubproperty rdf:resource="http://rdaregistry.info/Elements/u/P60311" />
  <reg:hasSubproperty rdf:resource="http://rdaregistry.info/Elements/e/P20204" />
  <reg:lexicalAlias rdf:resource="http://rdaregistry.info/Elements/u/basedOn.en" />
  <reg:hasSubproperty rdf:resource="http://rdaregistry.info/Elements/u/P60830" />
  <reg:hasSubproperty rdf:resource="http://rdaregistry.info/Elements/u/P60832" />
</owl:ObjectProperty>

<!-- Property: has base material -->
<owl:ObjectProperty rdf:about="http://rdaregistry.info/Elements/u/P60596">
  <rdfs:isDefinedBy rdf:resource="http://rdaregistry.info/Elements/u/" />
  <reg:status rdf:resource="http://metadataregistry.org/uri/RegStatus/1001" />
  <reg:name xml:lang="en">baseMaterial</reg:name>
  <rdfs:label xml:lang="en">has base material</rdfs:label>
  <skos:definition xml:lang="en">Relates a resource to an underlying physical material of a resource.</skos:definition>
  <rdf:type rdf:resource="http://www.w3.org/1999/02/22-rdf-syntax-ns#Property" />
  <reg:hasSubproperty rdf:resource="http://rdaregistry.info/Elements/m/P30208" />
  <reg:lexicalAlias rdf:resource="http://rdaregistry.info/Elements/u/baseMaterial.en" />
</owl:ObjectProperty>

<!-- Property: DEPRECATED -->
<owl:ObjectProperty rdf:about="http://rdaregistry.info/Elements/u/P60595">
  <rdfs:isDefinedBy rdf:resource="http://rdaregistry.info/Elements/u/" />
  <reg:status rdf:resource="http://metadataregistry.org/uri/RegStatus/1008" />
</owl:ObjectProperty>

<!-- Property: has binder -->
<owl:ObjectProperty rdf:about="http://rdaregistry.info/Elements/u/P60458">
  <rdfs:isDefinedBy rdf:resource="http://rdaregistry.info/Elements/u/" />
  <reg:status rdf:resource="http://metadataregistry.org/uri/RegStatus/1001" />
  <reg:name xml:lang="en">binder</reg:name>
  <rdfs:label xml:lang="en">has binder</rdfs:label>
  <skos:definition xml:lang="en">Relates a resource to an agent who binds a resource.</skos:definition>
  <rdf:type rdf:resource="http://www.w3.org/1999/02/22-rdf-syntax-ns#Property" />
  <rdfs:subPropertyOf rdf:resource="http://rdaregistry.info/Elements/u/P60374" />
  <owl:inverseOf rdf:resource="http://rdaregistry.info/Elements/u/P60692" />
  <reg:hasSubproperty rdf:resource="http://rdaregistry.info/Elements/i/P40013" />
  <reg:lexicalAlias rdf:resource="http://rdaregistry.info/Elements/u/binder.en" />
</owl:ObjectProperty>

<!-- Property: is binder of -->
<owl:ObjectProperty rdf:about="http://rdaregistry.info/Elements/u/P60692">
  <rdfs:isDefinedBy rdf:resource="http://rdaregistry.info/Elements/u/" />
  <reg:status rdf:resource="http://metadataregistry.org/uri/RegStatus/1001" />
  <reg:name xml:lang="en">binderOf</reg:name>
  <rdfs:label xml:lang="en">is binder of</rdfs:label>
  <skos:definition xml:lang="en">Relates an agent who binds a resource to a resource.</skos:definition>
  <rdf:type rdf:resource="http://www.w3.org/1999/02/22-rdf-syntax-ns#Property" />
  <rdfs:subPropertyOf rdf:resource="http://rdaregistry.info/Elements/u/P60602" />
  <owl:inverseOf rdf:resource="http://rdaregistry.info/Elements/u/P60458" />
  <reg:hasSubproperty rdf:resource="http://rdaregistry.info/Elements/a/P50123" />
  <reg:lexicalAlias rdf:resource="http://rdaregistry.info/Elements/u/binderOf.en" />
</owl:ObjectProperty>

<!-- Property: has biographical information -->
<owl:ObjectProperty rdf:about="http://rdaregistry.info/Elements/u/P60492">
  <rdfs:isDefinedBy rdf:resource="http://rdaregistry.info/Elements/u/" />
  <reg:status rdf:resource="http://metadataregistry.org/uri/RegStatus/1001" />
  <reg:name xml:lang="en">biographicalInformation</reg:name>
  <rdfs:label xml:lang="en">has biographical information</rdfs:label>
  <skos:definition xml:lang="en">Relates an agent to a summary of information about the life or history of an agent.</skos:definition>
  <rdf:type rdf:resource="http://www.w3.org/1999/02/22-rdf-syntax-ns#Property" />
  <reg:hasSubproperty rdf:resource="http://rdaregistry.info/Elements/a/P50113" />
  <reg:lexicalAlias rdf:resource="http://rdaregistry.info/Elements/u/biographicalInformation.en" />
</owl:ObjectProperty>

<!-- Property: has book artist -->
<owl:ObjectProperty rdf:about="http://rdaregistry.info/Elements/u/P60753">
  <rdfs:isDefinedBy rdf:resource="http://rdaregistry.info/Elements/u/" />
  <reg:status rdf:resource="http://metadataregistry.org/uri/RegStatus/1001" />
  <rdf:type rdf:resource="http://www.w3.org/1999/02/22-rdf-syntax-ns#Property" />
  <reg:name xml:lang="en">bookArtist</reg:name>
  <rdfs:label xml:lang="en">has book artist</rdfs:label>
  <reg:lexicalAlias rdf:resource="http://rdaregistry.info/Elements/u/bookArtist.en" />
  <skos:definition xml:lang="en">Relates a resource to an artist responsible for creating art resources that exploit a book form or alter its physical structure as part of a content of a resource.</skos:definition>
  <owl:inverseOf rdf:resource="http://rdaregistry.info/Elements/u/P60759" />
  <rdfs:subPropertyOf rdf:resource="http://rdaregistry.info/Elements/u/P60431" />
</owl:ObjectProperty>

<!-- Property: is book artist of -->
<owl:ObjectProperty rdf:about="http://rdaregistry.info/Elements/u/P60759">
  <rdfs:isDefinedBy rdf:resource="http://rdaregistry.info/Elements/u/" />
  <reg:status rdf:resource="http://metadataregistry.org/uri/RegStatus/1001" />
  <rdf:type rdf:resource="http://www.w3.org/1999/02/22-rdf-syntax-ns#Property" />
  <reg:name xml:lang="en">bookArtistOf</reg:name>
  <rdfs:label xml:lang="en">is book artist of</rdfs:label>
  <reg:lexicalAlias rdf:resource="http://rdaregistry.info/Elements/u/bookArtistOf.en" />
  <skos:definition xml:lang="en">Relates an artist responsible for creating art resources that exploit a book form or alter its physical structure as part of the content of a resource to a resource.</skos:definition>
  <owl:inverseOf rdf:resource="http://rdaregistry.info/Elements/u/P60753" />
  <rdfs:subPropertyOf rdf:resource="http://rdaregistry.info/Elements/u/P60660" />
</owl:ObjectProperty>

<!-- Property: has book designer -->
<owl:ObjectProperty rdf:about="http://rdaregistry.info/Elements/u/P60409">
  <rdfs:isDefinedBy rdf:resource="http://rdaregistry.info/Elements/u/" />
  <reg:status rdf:resource="http://metadataregistry.org/uri/RegStatus/1001" />
  <reg:name xml:lang="en">bookDesigner</reg:name>
  <rdfs:label xml:lang="en">has book designer</rdfs:label>
  <skos:definition xml:lang="en">Relates a resource to an agent involved in manufacturing a resource by being responsible for the entire graphic design of a book, including arrangement of type and illustration, choice of materials, and process used.</skos:definition>
  <rdf:type rdf:resource="http://www.w3.org/1999/02/22-rdf-syntax-ns#Property" />
  <rdfs:subPropertyOf rdf:resource="http://rdaregistry.info/Elements/u/P60443" />
  <owl:inverseOf rdf:resource="http://rdaregistry.info/Elements/u/P60637" />
  <reg:hasSubproperty rdf:resource="http://rdaregistry.info/Elements/m/P30069" />
  <reg:lexicalAlias rdf:resource="http://rdaregistry.info/Elements/u/bookDesigner.en" />
</owl:ObjectProperty>

<!-- Property: is book designer of -->
<owl:ObjectProperty rdf:about="http://rdaregistry.info/Elements/u/P60637">
  <rdfs:isDefinedBy rdf:resource="http://rdaregistry.info/Elements/u/" />
  <reg:status rdf:resource="http://metadataregistry.org/uri/RegStatus/1001" />
  <reg:name xml:lang="en">bookDesignerOf</reg:name>
  <rdfs:label xml:lang="en">is book designer of</rdfs:label>
  <skos:definition xml:lang="en">Relates an agent involved in manufacturing a resource by being responsible for the entire graphic design of a book, including arrangement of type and illustration, choice of materials, and process used to a resource.</skos:definition>
  <rdf:type rdf:resource="http://www.w3.org/1999/02/22-rdf-syntax-ns#Property" />
  <rdfs:subPropertyOf rdf:resource="http://rdaregistry.info/Elements/u/P60669" />
  <owl:inverseOf rdf:resource="http://rdaregistry.info/Elements/u/P60409" />
  <reg:hasSubproperty rdf:resource="http://rdaregistry.info/Elements/a/P50170" />
  <reg:lexicalAlias rdf:resource="http://rdaregistry.info/Elements/u/bookDesignerOf.en" />
</owl:ObjectProperty>

<!-- Property: has book format -->
<owl:ObjectProperty rdf:about="http://rdaregistry.info/Elements/u/P60578">
  <rdfs:isDefinedBy rdf:resource="http://rdaregistry.info/Elements/u/" />
  <reg:status rdf:resource="http://metadataregistry.org/uri/RegStatus/1001" />
  <reg:name xml:lang="en">bookFormat</reg:name>
  <rdfs:label xml:lang="en">has book format</rdfs:label>
  <skos:definition xml:lang="en">Relates a resource to the result of folding a printed sheet to form a gathering of leaves (e.g., a sheet folded once to form a folio, twice to form a quarto, three times to form an octavo, etc.).</skos:definition>
  <rdf:type rdf:resource="http://www.w3.org/1999/02/22-rdf-syntax-ns#Property" />
  <reg:hasSubproperty rdf:resource="http://rdaregistry.info/Elements/m/P30197" />
  <reg:lexicalAlias rdf:resource="http://rdaregistry.info/Elements/u/bookFormat.en" />
</owl:ObjectProperty>

<!-- Property: is bound with -->
<owl:ObjectProperty rdf:about="http://rdaregistry.info/Elements/u/P60237">
  <rdfs:isDefinedBy rdf:resource="http://rdaregistry.info/Elements/u/" />
  <reg:status rdf:resource="http://metadataregistry.org/uri/RegStatus/1001" />
  <reg:name xml:lang="en">boundWith</reg:name>
  <rdfs:label xml:lang="en">is bound with</rdfs:label>
  <skos:definition xml:lang="en">Relates a resource to a resource that has been bound within the same binding as a resource being described.</skos:definition>
  <rdf:type rdf:resource="http://www.w3.org/1999/02/22-rdf-syntax-ns#Property" />
  <rdfs:subPropertyOf rdf:resource="http://rdaregistry.info/Elements/u/P60196" />
  <owl:inverseOf rdf:resource="http://rdaregistry.info/Elements/u/P60237" />
  <reg:hasSubproperty rdf:resource="http://rdaregistry.info/Elements/i/P40032" />
  <reg:lexicalAlias rdf:resource="http://rdaregistry.info/Elements/u/boundWith.en" />
</owl:ObjectProperty>

<!-- Property: has braille embosser -->
<owl:ObjectProperty rdf:about="http://rdaregistry.info/Elements/u/P60411">
  <rdfs:isDefinedBy rdf:resource="http://rdaregistry.info/Elements/u/" />
  <reg:status rdf:resource="http://metadataregistry.org/uri/RegStatus/1001" />
  <reg:name xml:lang="en">brailleEmbosser</reg:name>
  <rdfs:label xml:lang="en">has braille embosser</rdfs:label>
  <skos:definition xml:lang="en">Relates a resource to an agent involved in manufacturing a resource by embossing braille cells using a stylus, special embossing printer, or other device.</skos:definition>
  <rdf:type rdf:resource="http://www.w3.org/1999/02/22-rdf-syntax-ns#Property" />
  <rdfs:subPropertyOf rdf:resource="http://rdaregistry.info/Elements/u/P60443" />
  <owl:inverseOf rdf:resource="http://rdaregistry.info/Elements/u/P60639" />
  <reg:hasSubproperty rdf:resource="http://rdaregistry.info/Elements/m/P30071" />
  <reg:lexicalAlias rdf:resource="http://rdaregistry.info/Elements/u/brailleEmbosser.en" />
</owl:ObjectProperty>

<!-- Property: is braille embosser of -->
<owl:ObjectProperty rdf:about="http://rdaregistry.info/Elements/u/P60639">
  <rdfs:isDefinedBy rdf:resource="http://rdaregistry.info/Elements/u/" />
  <reg:status rdf:resource="http://metadataregistry.org/uri/RegStatus/1001" />
  <reg:name xml:lang="en">brailleEmbosserOf</reg:name>
  <rdfs:label xml:lang="en">is braille embosser of</rdfs:label>
  <skos:definition xml:lang="en">Relates an agent involved in manufacturing a resource by embossing braille cells using a stylus, special embossing printer, or other device to a resource.</skos:definition>
  <rdf:type rdf:resource="http://www.w3.org/1999/02/22-rdf-syntax-ns#Property" />
  <rdfs:subPropertyOf rdf:resource="http://rdaregistry.info/Elements/u/P60669" />
  <owl:inverseOf rdf:resource="http://rdaregistry.info/Elements/u/P60411" />
  <reg:hasSubproperty rdf:resource="http://rdaregistry.info/Elements/a/P50172" />
  <reg:lexicalAlias rdf:resource="http://rdaregistry.info/Elements/u/brailleEmbosserOf.en" />
</owl:ObjectProperty>

<!-- Property: has broadcaster -->
<owl:ObjectProperty rdf:about="http://rdaregistry.info/Elements/u/P60407">
  <rdfs:isDefinedBy rdf:resource="http://rdaregistry.info/Elements/u/" />
  <reg:status rdf:resource="http://metadataregistry.org/uri/RegStatus/1001" />
  <reg:name xml:lang="en">broadcaster</reg:name>
  <rdfs:label xml:lang="en">has broadcaster</rdfs:label>
  <skos:definition xml:lang="en">Relates a resource to an agent involved in broadcasting a resource to an audience via radio, television, webcast, etc.</skos:definition>
  <rdf:type rdf:resource="http://www.w3.org/1999/02/22-rdf-syntax-ns#Property" />
  <rdfs:subPropertyOf rdf:resource="http://rdaregistry.info/Elements/u/P60444" />
  <owl:inverseOf rdf:resource="http://rdaregistry.info/Elements/u/P60635" />
  <reg:hasSubproperty rdf:resource="http://rdaregistry.info/Elements/m/P30067" />
  <reg:lexicalAlias rdf:resource="http://rdaregistry.info/Elements/u/broadcaster.en" />
</owl:ObjectProperty>

<!-- Property: is broadcaster of -->
<owl:ObjectProperty rdf:about="http://rdaregistry.info/Elements/u/P60635">
  <rdfs:isDefinedBy rdf:resource="http://rdaregistry.info/Elements/u/" />
  <reg:status rdf:resource="http://metadataregistry.org/uri/RegStatus/1001" />
  <reg:name xml:lang="en">broadcasterOf</reg:name>
  <rdfs:label xml:lang="en">is broadcaster of</rdfs:label>
  <skos:definition xml:lang="en">Relates an agent involved in broadcasting a resource to an audience via radio, television, webcast, etc. to a resource.</skos:definition>
  <rdf:type rdf:resource="http://www.w3.org/1999/02/22-rdf-syntax-ns#Property" />
  <rdfs:subPropertyOf rdf:resource="http://rdaregistry.info/Elements/u/P60670" />
  <owl:inverseOf rdf:resource="http://rdaregistry.info/Elements/u/P60407" />
  <reg:hasSubproperty rdf:resource="http://rdaregistry.info/Elements/a/P50168" />
  <reg:lexicalAlias rdf:resource="http://rdaregistry.info/Elements/u/broadcasterOf.en" />
</owl:ObjectProperty>

<!-- Property: has broadcast standard -->
<owl:ObjectProperty rdf:about="http://rdaregistry.info/Elements/u/P60349">
  <rdfs:isDefinedBy rdf:resource="http://rdaregistry.info/Elements/u/" />
  <reg:status rdf:resource="http://metadataregistry.org/uri/RegStatus/1001" />
  <reg:name xml:lang="en">broadcastStandard</reg:name>
  <rdfs:label xml:lang="en">has broadcast standard</rdfs:label>
  <skos:definition xml:lang="en">Relates a resource to a system used to format a video resource for television broadcast.</skos:definition>
  <rdf:type rdf:resource="http://www.w3.org/1999/02/22-rdf-syntax-ns#Property" />
  <rdfs:subPropertyOf rdf:resource="http://rdaregistry.info/Elements/u/P60352" />
  <reg:hasSubproperty rdf:resource="http://rdaregistry.info/Elements/m/P30123" />
  <reg:lexicalAlias rdf:resource="http://rdaregistry.info/Elements/u/broadcastStandard.en" />
</owl:ObjectProperty>

<!-- Property: has broader affiliated agent -->
<owl:ObjectProperty rdf:about="http://rdaregistry.info/Elements/u/P60738">
  <rdfs:isDefinedBy rdf:resource="http://rdaregistry.info/Elements/u/" />
  <reg:status rdf:resource="http://metadataregistry.org/uri/RegStatus/1001" />
  <rdf:type rdf:resource="http://www.w3.org/1999/02/22-rdf-syntax-ns#Property" />
  <reg:name xml:lang="en">broaderAffiliatedAgent</reg:name>
  <rdfs:label xml:lang="en">has broader affiliated agent</rdfs:label>
  <reg:lexicalAlias rdf:resource="http://rdaregistry.info/Elements/u/broaderAffiliatedAgent.en" />
  <skos:definition xml:lang="en">Relates an agent that acts for a local affiliated agent and others at a broader organizational level to an agent.</skos:definition>
</owl:ObjectProperty>

<!-- Property: is cadenza -->
<owl:ObjectProperty rdf:about="http://rdaregistry.info/Elements/u/P60113">
  <rdfs:isDefinedBy rdf:resource="http://rdaregistry.info/Elements/u/" />
  <reg:status rdf:resource="http://metadataregistry.org/uri/RegStatus/1001" />
  <reg:name xml:lang="en">cadenza</reg:name>
  <rdfs:label xml:lang="en">is cadenza</rdfs:label>
  <skos:definition xml:lang="en">Relates a resource to a musical resource consisting of an ornamental passage for a soloist, added to a musical resource such as a concerto, either by the same or a different composer.</skos:definition>
  <rdf:type rdf:resource="http://www.w3.org/1999/02/22-rdf-syntax-ns#Property" />
  <rdfs:subPropertyOf rdf:resource="http://rdaregistry.info/Elements/u/P60204" />
  <owl:inverseOf rdf:resource="http://rdaregistry.info/Elements/u/P60116" />
  <reg:hasSubproperty rdf:resource="http://rdaregistry.info/Elements/e/P20080" />
  <reg:lexicalAlias rdf:resource="http://rdaregistry.info/Elements/u/cadenza.en" />
</owl:ObjectProperty>

<!-- Property: is cadenza composed for -->
<owl:ObjectProperty rdf:about="http://rdaregistry.info/Elements/u/P60116">
  <rdfs:isDefinedBy rdf:resource="http://rdaregistry.info/Elements/u/" />
  <reg:status rdf:resource="http://metadataregistry.org/uri/RegStatus/1001" />
  <reg:name xml:lang="en">cadenzaComposedFor</reg:name>
  <rdfs:label xml:lang="en">is cadenza composed for</rdfs:label>
  <skos:definition xml:lang="en">Relates a resource to a musical resource such as a concerto for which an ornamental passage for a soloist has been composed, either by the same or a different composer.</skos:definition>
  <rdf:type rdf:resource="http://www.w3.org/1999/02/22-rdf-syntax-ns#Property" />
  <rdfs:subPropertyOf rdf:resource="http://rdaregistry.info/Elements/u/P60307" />
  <owl:inverseOf rdf:resource="http://rdaregistry.info/Elements/u/P60113" />
  <reg:hasSubproperty rdf:resource="http://rdaregistry.info/Elements/e/P20083" />
  <reg:lexicalAlias rdf:resource="http://rdaregistry.info/Elements/u/cadenzaComposedFor.en" />
</owl:ObjectProperty>

<!-- Property: has calligrapher -->
<owl:ObjectProperty rdf:about="http://rdaregistry.info/Elements/u/P60752">
  <rdfs:isDefinedBy rdf:resource="http://rdaregistry.info/Elements/u/" />
  <reg:status rdf:resource="http://metadataregistry.org/uri/RegStatus/1001" />
  <rdf:type rdf:resource="http://www.w3.org/1999/02/22-rdf-syntax-ns#Property" />
  <reg:name xml:lang="en">calligrapher</reg:name>
  <rdfs:label xml:lang="en">has calligrapher</rdfs:label>
  <reg:lexicalAlias rdf:resource="http://rdaregistry.info/Elements/u/calligrapher.en" />
  <skos:definition xml:lang="en">Relates a resource to an artist responsible for creating a resource of calligraphy where a focus of interest lies in the aesthetic value of its penmanship or graphic artistry, regardless of whether the same agent also authored the inscribed text.</skos:definition>
  <owl:inverseOf rdf:resource="http://rdaregistry.info/Elements/u/P60758" />
  <rdfs:subPropertyOf rdf:resource="http://rdaregistry.info/Elements/u/P60431" />
</owl:ObjectProperty>

<!-- Property: is calligrapher of -->
<owl:ObjectProperty rdf:about="http://rdaregistry.info/Elements/u/P60758">
  <rdfs:isDefinedBy rdf:resource="http://rdaregistry.info/Elements/u/" />
  <reg:status rdf:resource="http://metadataregistry.org/uri/RegStatus/1001" />
  <rdf:type rdf:resource="http://www.w3.org/1999/02/22-rdf-syntax-ns#Property" />
  <reg:name xml:lang="en">calligrapherOf</reg:name>
  <rdfs:label xml:lang="en">is calligrapher of</rdfs:label>
  <reg:lexicalAlias rdf:resource="http://rdaregistry.info/Elements/u/calligrapherOf.en" />
  <skos:definition xml:lang="en">Relates an artist responsible for creating a resource of calligraphy where a focus of interest lies in the aesthetic value of its penmanship or graphic artistry, regardless of whether the same agent also authored the inscribed text to a resource.</skos:definition>
  <owl:inverseOf rdf:resource="http://rdaregistry.info/Elements/u/P60752" />
  <rdfs:subPropertyOf rdf:resource="http://rdaregistry.info/Elements/u/P60660" />
</owl:ObjectProperty>

<!-- Property: has carrier type -->
<owl:ObjectProperty rdf:about="http://rdaregistry.info/Elements/u/P60048">
  <rdfs:isDefinedBy rdf:resource="http://rdaregistry.info/Elements/u/" />
  <reg:status rdf:resource="http://metadataregistry.org/uri/RegStatus/1001" />
  <reg:name xml:lang="en">carrierType</reg:name>
  <rdfs:label xml:lang="en">has carrier type</rdfs:label>
  <skos:definition xml:lang="en">Relates a resource to a categorization reflecting a format of a storage medium and housing of a carrier in combination with a type of intermediation device required to view, play, run, etc., the content of a resource.</skos:definition>
  <rdf:type rdf:resource="http://www.w3.org/1999/02/22-rdf-syntax-ns#Property" />
  <reg:hasSubproperty rdf:resource="http://rdaregistry.info/Elements/m/P30001" />
  <reg:lexicalAlias rdf:resource="http://rdaregistry.info/Elements/u/carrierType.en" />
</owl:ObjectProperty>

<!-- Property: has cartographer -->
<owl:ObjectProperty rdf:about="http://rdaregistry.info/Elements/u/P60425">
  <rdfs:isDefinedBy rdf:resource="http://rdaregistry.info/Elements/u/" />
  <reg:status rdf:resource="http://metadataregistry.org/uri/RegStatus/1001" />
  <reg:name xml:lang="en">cartographer</reg:name>
  <rdfs:label xml:lang="en">has cartographer</rdfs:label>
  <skos:definition xml:lang="en">Relates a resource to an agent responsible for creating a map, atlas, globe, or other cartographic resource.</skos:definition>
  <rdf:type rdf:resource="http://www.w3.org/1999/02/22-rdf-syntax-ns#Property" />
  <rdfs:subPropertyOf rdf:resource="http://rdaregistry.info/Elements/u/P60447" />
  <owl:inverseOf rdf:resource="http://rdaregistry.info/Elements/u/P60654" />
  <reg:hasSubproperty rdf:resource="http://rdaregistry.info/Elements/e/P20042" />
  <reg:lexicalAlias rdf:resource="http://rdaregistry.info/Elements/u/cartographer.en" />
</owl:ObjectProperty>

<!-- Property: is cartographer of -->
<owl:ObjectProperty rdf:about="http://rdaregistry.info/Elements/u/P60654">
  <rdfs:isDefinedBy rdf:resource="http://rdaregistry.info/Elements/u/" />
  <reg:status rdf:resource="http://metadataregistry.org/uri/RegStatus/1001" />
  <reg:name xml:lang="en">cartographerOf</reg:name>
  <rdfs:label xml:lang="en">is cartographer of</rdfs:label>
  <skos:definition xml:lang="en">Relates an agent responsible for creating a map, atlas, globe, or other cartographic resource to a resource.</skos:definition>
  <rdf:type rdf:resource="http://www.w3.org/1999/02/22-rdf-syntax-ns#Property" />
  <rdfs:subPropertyOf rdf:resource="http://rdaregistry.info/Elements/u/P60672" />
  <owl:inverseOf rdf:resource="http://rdaregistry.info/Elements/u/P60425" />
  <reg:hasSubproperty rdf:resource="http://rdaregistry.info/Elements/a/P50150" />
  <reg:hasSubproperty rdf:resource="http://rdaregistry.info/Elements/a/P50186" />
  <reg:lexicalAlias rdf:resource="http://rdaregistry.info/Elements/u/cartographerOf.en" />
</owl:ObjectProperty>

<!-- Property: has cartographic data type -->
<owl:ObjectProperty rdf:about="http://rdaregistry.info/Elements/u/P60875">
  <rdfs:isDefinedBy rdf:resource="http://rdaregistry.info/Elements/u/" />
  <reg:status rdf:resource="http://metadataregistry.org/uri/RegStatus/1001" />
  <rdf:type rdf:resource="http://www.w3.org/1999/02/22-rdf-syntax-ns#Property" />
  <reg:name xml:lang="en">cartographicDataType</reg:name>
  <rdfs:label xml:lang="en">has cartographic data type</rdfs:label>
  <reg:lexicalAlias rdf:resource="http://rdaregistry.info/Elements/u/cartographicDataType.en" />
  <skos:definition xml:lang="en">Relates a resource to a machine-readable representation of geospatial features.</skos:definition>
  <reg:hasSubproperty rdf:resource="http://rdaregistry.info/Elements/m/P30261" />
</owl:ObjectProperty>

<!-- Property: has caster -->
<owl:ObjectProperty rdf:about="http://rdaregistry.info/Elements/u/P60413">
  <rdfs:isDefinedBy rdf:resource="http://rdaregistry.info/Elements/u/" />
  <reg:status rdf:resource="http://metadataregistry.org/uri/RegStatus/1001" />
  <reg:name xml:lang="en">caster</reg:name>
  <rdfs:label xml:lang="en">has caster</rdfs:label>
  <skos:definition xml:lang="en">Relates a resource to an agent involved in manufacturing a resource by pouring a liquid or molten substance into a mold and leaving it to solidify to take the shape of the mold.</skos:definition>
  <rdf:type rdf:resource="http://www.w3.org/1999/02/22-rdf-syntax-ns#Property" />
  <rdfs:subPropertyOf rdf:resource="http://rdaregistry.info/Elements/u/P60443" />
  <owl:inverseOf rdf:resource="http://rdaregistry.info/Elements/u/P60641" />
  <reg:hasSubproperty rdf:resource="http://rdaregistry.info/Elements/m/P30073" />
  <reg:lexicalAlias rdf:resource="http://rdaregistry.info/Elements/u/caster.en" />
</owl:ObjectProperty>

<!-- Property: is caster of -->
<owl:ObjectProperty rdf:about="http://rdaregistry.info/Elements/u/P60641">
  <rdfs:isDefinedBy rdf:resource="http://rdaregistry.info/Elements/u/" />
  <reg:status rdf:resource="http://metadataregistry.org/uri/RegStatus/1001" />
  <reg:name xml:lang="en">casterOf</reg:name>
  <rdfs:label xml:lang="en">is caster of</rdfs:label>
  <skos:definition xml:lang="en">Relates an agent involved in manufacturing a resource by pouring a liquid or molten substance into a mold and leaving it to solidify to take the shape of the mold to a resource.</skos:definition>
  <rdf:type rdf:resource="http://www.w3.org/1999/02/22-rdf-syntax-ns#Property" />
  <rdfs:subPropertyOf rdf:resource="http://rdaregistry.info/Elements/u/P60669" />
  <owl:inverseOf rdf:resource="http://rdaregistry.info/Elements/u/P60413" />
  <reg:hasSubproperty rdf:resource="http://rdaregistry.info/Elements/a/P50174" />
  <reg:lexicalAlias rdf:resource="http://rdaregistry.info/Elements/u/casterOf.en" />
</owl:ObjectProperty>

<!-- Property: has casting director -->
<owl:ObjectProperty rdf:about="http://rdaregistry.info/Elements/u/P60890">
  <rdfs:isDefinedBy rdf:resource="http://rdaregistry.info/Elements/u/" />
  <reg:status rdf:resource="http://metadataregistry.org/uri/RegStatus/1001" />
  <rdf:type rdf:resource="http://www.w3.org/1999/02/22-rdf-syntax-ns#Property" />
  <reg:name xml:lang="en">castingDIrector</reg:name>
  <rdfs:label xml:lang="en">has casting director</rdfs:label>
  <reg:lexicalAlias rdf:resource="http://rdaregistry.info/Elements/u/castingDirector.en" />
  <skos:definition xml:lang="en">Relates a resource to an agent responsible for most aspects of assigning parts and duties to performers.</skos:definition>
  <owl:inverseOf rdf:resource="http://rdaregistry.info/Elements/u/P60882" />
  <reg:hasSubproperty rdf:resource="http://rdaregistry.info/Elements/w/P10305" />
  <rdfs:subPropertyOf rdf:resource="http://rdaregistry.info/Elements/u/P60158" />
</owl:ObjectProperty>

<!-- Property: is casting director of -->
<owl:ObjectProperty rdf:about="http://rdaregistry.info/Elements/u/P60882">
  <rdfs:isDefinedBy rdf:resource="http://rdaregistry.info/Elements/u/" />
  <reg:status rdf:resource="http://metadataregistry.org/uri/RegStatus/1001" />
  <rdf:type rdf:resource="http://www.w3.org/1999/02/22-rdf-syntax-ns#Property" />
  <reg:name xml:lang="en">castingDirectorOf</reg:name>
  <rdfs:label xml:lang="en">is casting director of</rdfs:label>
  <reg:lexicalAlias rdf:resource="http://rdaregistry.info/Elements/u/castingDirectorOf.en" />
  <skos:definition xml:lang="en">Relates an agent to a resource that incorporates a contribution of responsibility for most aspects of assigning parts and duties to performers.</skos:definition>
  <owl:inverseOf rdf:resource="http://rdaregistry.info/Elements/u/P60890" />
  <rdfs:subPropertyOf rdf:resource="http://rdaregistry.info/Elements/u/P60672" />
  <reg:hasSubproperty rdf:resource="http://rdaregistry.info/Elements/a/P50294" />
</owl:ObjectProperty>

<!-- Property: is catalogue -->
<owl:ObjectProperty rdf:about="http://rdaregistry.info/Elements/u/P60206">
  <rdfs:isDefinedBy rdf:resource="http://rdaregistry.info/Elements/u/" />
  <reg:status rdf:resource="http://metadataregistry.org/uri/RegStatus/1001" />
  <reg:name xml:lang="en">catalogue</reg:name>
  <rdfs:label xml:lang="en">is catalogue</rdfs:label>
  <skos:definition xml:lang="en">Relates a resource to a resource that consists of a complete enumeration of resources arranged systematically.</skos:definition>
  <rdf:type rdf:resource="http://www.w3.org/1999/02/22-rdf-syntax-ns#Property" />
  <rdfs:subPropertyOf rdf:resource="http://rdaregistry.info/Elements/u/P60204" />
  <owl:inverseOf rdf:resource="http://rdaregistry.info/Elements/u/P60290" />
  <reg:hasSubproperty rdf:resource="http://rdaregistry.info/Elements/e/P20107" />
  <reg:lexicalAlias rdf:resource="http://rdaregistry.info/Elements/u/catalogue.en" />
</owl:ObjectProperty>

<!-- Property: is catalogue of -->
<owl:ObjectProperty rdf:about="http://rdaregistry.info/Elements/u/P60290">
  <rdfs:isDefinedBy rdf:resource="http://rdaregistry.info/Elements/u/" />
  <reg:status rdf:resource="http://metadataregistry.org/uri/RegStatus/1001" />
  <reg:name xml:lang="en">catalogueOf</reg:name>
  <rdfs:label xml:lang="en">is catalogue of</rdfs:label>
  <skos:definition xml:lang="en">Relates a resource to a resource used as a basis for a catalogue, i.e., a complete enumeration of resources arranged systematically.</skos:definition>
  <rdf:type rdf:resource="http://www.w3.org/1999/02/22-rdf-syntax-ns#Property" />
  <rdfs:subPropertyOf rdf:resource="http://rdaregistry.info/Elements/u/P60307" />
  <owl:inverseOf rdf:resource="http://rdaregistry.info/Elements/u/P60206" />
  <reg:hasSubproperty rdf:resource="http://rdaregistry.info/Elements/e/P20180" />
  <reg:lexicalAlias rdf:resource="http://rdaregistry.info/Elements/u/catalogueOf.en" />
</owl:ObjectProperty>

<!-- Property: has censor -->
<owl:ObjectProperty rdf:about="http://rdaregistry.info/Elements/u/P60851">
  <rdfs:isDefinedBy rdf:resource="http://rdaregistry.info/Elements/u/" />
  <reg:status rdf:resource="http://metadataregistry.org/uri/RegStatus/1001" />
  <rdf:type rdf:resource="http://www.w3.org/1999/02/22-rdf-syntax-ns#Property" />
  <reg:name xml:lang="en">censor</reg:name>
  <rdfs:label xml:lang="en">has censor</rdfs:label>
  <reg:lexicalAlias rdf:resource="http://rdaregistry.info/Elements/u/censor.en" />
  <skos:definition xml:lang="en">Relates a resource to an agent contributing to a resource by revising the content for the purpose of suppressing parts deemed objectionable on moral, political, military, or other grounds, but leaving the nature and content substantially unchanged.</skos:definition>
  <owl:inverseOf rdf:resource="http://rdaregistry.info/Elements/u/P60852" />
  <reg:hasSubproperty rdf:resource="http://rdaregistry.info/Elements/e/P20287" />
  <skos:scopeNote xml:lang="en">Substantial modification that results in the creation of a new resource is excluded.</skos:scopeNote>
  <rdfs:subPropertyOf rdf:resource="http://rdaregistry.info/Elements/u/P60398" />
  <rdakit:seeAlso rdf:resource="http://rdaregistry.info/Elements/u/P60434" />
</owl:ObjectProperty>

<!-- Property: is censor of -->
<owl:ObjectProperty rdf:about="http://rdaregistry.info/Elements/u/P60852">
  <rdfs:isDefinedBy rdf:resource="http://rdaregistry.info/Elements/u/" />
  <reg:status rdf:resource="http://metadataregistry.org/uri/RegStatus/1001" />
  <rdf:type rdf:resource="http://www.w3.org/1999/02/22-rdf-syntax-ns#Property" />
  <reg:name xml:lang="en">censorOf</reg:name>
  <rdfs:label xml:lang="en">is censor of</rdfs:label>
  <reg:lexicalAlias rdf:resource="http://rdaregistry.info/Elements/u/censorOf.en" />
  <skos:definition xml:lang="en">Relates an agent contributing to a resource by revising the content for the purpose of suppressing parts deemed objectionable on moral, political, military, or other grounds, but leaving the nature and content substantially unchanged to a resource.</skos:definition>
  <owl:inverseOf rdf:resource="http://rdaregistry.info/Elements/u/P60851" />
  <reg:hasSubproperty rdf:resource="http://rdaregistry.info/Elements/a/P50271" />
  <skos:scopeNote xml:lang="en">Substantial modification that results in the creation of a new resource is excluded.</skos:scopeNote>
  <rdfs:subPropertyOf rdf:resource="http://rdaregistry.info/Elements/u/P60626" />
  <rdakit:seeAlso rdf:resource="http://rdaregistry.info/Elements/u/P60663" />
</owl:ObjectProperty>

<!-- Property: has chief executive -->
<owl:ObjectProperty rdf:about="http://rdaregistry.info/Elements/u/P60864">
  <rdfs:isDefinedBy rdf:resource="http://rdaregistry.info/Elements/u/" />
  <reg:status rdf:resource="http://metadataregistry.org/uri/RegStatus/1001" />
  <rdf:type rdf:resource="http://www.w3.org/1999/02/22-rdf-syntax-ns#Property" />
  <reg:name xml:lang="en">chiefExecutive</reg:name>
  <rdfs:label xml:lang="en">has chief executive</rdfs:label>
  <reg:lexicalAlias rdf:resource="http://rdaregistry.info/Elements/u/chiefExecutive.en" />
  <skos:definition xml:lang="en">Relates an agent to an officer who is a top ranking official of an agent.</skos:definition>
  <owl:inverseOf rdf:resource="http://rdaregistry.info/Elements/u/P60865" />
  <reg:hasSubproperty rdf:resource="http://rdaregistry.info/Elements/a/P50284" />
  <rdfs:subPropertyOf rdf:resource="http://rdaregistry.info/Elements/u/P60633" />
</owl:ObjectProperty>

<!-- Property: is chief executive of -->
<owl:ObjectProperty rdf:about="http://rdaregistry.info/Elements/u/P60865">
  <rdfs:isDefinedBy rdf:resource="http://rdaregistry.info/Elements/u/" />
  <reg:status rdf:resource="http://metadataregistry.org/uri/RegStatus/1001" />
  <rdf:type rdf:resource="http://www.w3.org/1999/02/22-rdf-syntax-ns#Property" />
  <reg:name xml:lang="en">chiefExecutiveOf</reg:name>
  <rdfs:label xml:lang="en">is chief executive of</rdfs:label>
  <reg:lexicalAlias rdf:resource="http://rdaregistry.info/Elements/u/chiefExecutiveOf.en" />
  <skos:definition xml:lang="en">Relates an agent to an agent in which an officer is a top ranking official.</skos:definition>
  <owl:inverseOf rdf:resource="http://rdaregistry.info/Elements/u/P60864" />
  <reg:hasSubproperty rdf:resource="http://rdaregistry.info/Elements/a/P50286" />
  <rdfs:subPropertyOf rdf:resource="http://rdaregistry.info/Elements/u/P60737" />
</owl:ObjectProperty>

<!-- Property: has choral conductor -->
<owl:ObjectProperty rdf:about="http://rdaregistry.info/Elements/u/P60842">
  <rdfs:isDefinedBy rdf:resource="http://rdaregistry.info/Elements/u/" />
  <reg:status rdf:resource="http://metadataregistry.org/uri/RegStatus/1001" />
  <rdf:type rdf:resource="http://www.w3.org/1999/02/22-rdf-syntax-ns#Property" />
  <reg:name xml:lang="en">choralConductor</reg:name>
  <rdfs:label xml:lang="en">has choral conductor</rdfs:label>
  <reg:lexicalAlias rdf:resource="http://rdaregistry.info/Elements/u/choralConductor.en" />
  <skos:definition xml:lang="en">Relates a resource to a conductor contributing to a musical resource by leading a choral performing group in a musical or dramatic presentation, etc.</skos:definition>
  <owl:inverseOf rdf:resource="http://rdaregistry.info/Elements/u/P60843" />
  <reg:hasSubproperty rdf:resource="http://rdaregistry.info/Elements/e/P20285" />
  <rdfs:subPropertyOf rdf:resource="http://rdaregistry.info/Elements/u/P60141" />
</owl:ObjectProperty>

<!-- Property: is choral conductor of -->
<owl:ObjectProperty rdf:about="http://rdaregistry.info/Elements/u/P60843">
  <rdfs:isDefinedBy rdf:resource="http://rdaregistry.info/Elements/u/" />
  <reg:status rdf:resource="http://metadataregistry.org/uri/RegStatus/1001" />
  <rdf:type rdf:resource="http://www.w3.org/1999/02/22-rdf-syntax-ns#Property" />
  <reg:name xml:lang="en">choralConductorOf</reg:name>
  <rdfs:label xml:lang="en">is choral conductor of</rdfs:label>
  <reg:lexicalAlias rdf:resource="http://rdaregistry.info/Elements/u/choralConductorOf.en" />
  <skos:definition xml:lang="en">Relates a conductor contributing to a musical resource by leading a choral performing group in a musical or dramatic presentation, etc. to a resource.</skos:definition>
  <owl:inverseOf rdf:resource="http://rdaregistry.info/Elements/u/P60842" />
  <reg:hasSubproperty rdf:resource="http://rdaregistry.info/Elements/a/P50268" />
  <rdfs:subPropertyOf rdf:resource="http://rdaregistry.info/Elements/u/P60016" />
</owl:ObjectProperty>

<!-- Property: has choreographer -->
<owl:ObjectProperty rdf:about="http://rdaregistry.info/Elements/u/P60433">
  <rdfs:isDefinedBy rdf:resource="http://rdaregistry.info/Elements/u/" />
  <reg:status rdf:resource="http://metadataregistry.org/uri/RegStatus/1001" />
  <reg:name xml:lang="en">choreographer</reg:name>
  <rdfs:label xml:lang="en">has choreographer</rdfs:label>
  <skos:definition xml:lang="en">Relates a resource to an agent responsible for creating a resource of movement.</skos:definition>
  <rdf:type rdf:resource="http://www.w3.org/1999/02/22-rdf-syntax-ns#Property" />
  <rdfs:subPropertyOf rdf:resource="http://rdaregistry.info/Elements/u/P60447" />
  <owl:inverseOf rdf:resource="http://rdaregistry.info/Elements/u/P60662" />
  <reg:hasSubproperty rdf:resource="http://rdaregistry.info/Elements/e/P20043" />
  <reg:lexicalAlias rdf:resource="http://rdaregistry.info/Elements/u/choreographer.en" />
</owl:ObjectProperty>

<!-- Property: is choreographer of -->
<owl:ObjectProperty rdf:about="http://rdaregistry.info/Elements/u/P60662">
  <rdfs:isDefinedBy rdf:resource="http://rdaregistry.info/Elements/u/" />
  <reg:status rdf:resource="http://metadataregistry.org/uri/RegStatus/1001" />
  <reg:name xml:lang="en">choreographerOf</reg:name>
  <rdfs:label xml:lang="en">is choreographer of</rdfs:label>
  <skos:definition xml:lang="en">Relates an agent responsible for creating a resource of movement to a resource.</skos:definition>
  <rdf:type rdf:resource="http://www.w3.org/1999/02/22-rdf-syntax-ns#Property" />
  <rdfs:subPropertyOf rdf:resource="http://rdaregistry.info/Elements/u/P60672" />
  <owl:inverseOf rdf:resource="http://rdaregistry.info/Elements/u/P60433" />
  <reg:hasSubproperty rdf:resource="http://rdaregistry.info/Elements/a/P50151" />
  <reg:hasSubproperty rdf:resource="http://rdaregistry.info/Elements/a/P50194" />
  <reg:lexicalAlias rdf:resource="http://rdaregistry.info/Elements/u/choreographerOf.en" />
</owl:ObjectProperty>

<!-- Property: is choreographic adaptation of -->
<owl:ObjectProperty rdf:about="http://rdaregistry.info/Elements/u/P60293">
  <rdfs:isDefinedBy rdf:resource="http://rdaregistry.info/Elements/u/" />
  <reg:status rdf:resource="http://metadataregistry.org/uri/RegStatus/1001" />
  <reg:name xml:lang="en">choreographicAdaptationOf</reg:name>
  <rdfs:label xml:lang="en">is choreographic adaptation of</rdfs:label>
  <skos:definition xml:lang="en">Relates a resource to a resource that has been adapted as a resource consisting of movement.</skos:definition>
  <rdf:type rdf:resource="http://www.w3.org/1999/02/22-rdf-syntax-ns#Property" />
  <rdfs:subPropertyOf rdf:resource="http://rdaregistry.info/Elements/u/P60305" />
  <owl:inverseOf rdf:resource="http://rdaregistry.info/Elements/u/P60180" />
  <reg:hasSubproperty rdf:resource="http://rdaregistry.info/Elements/e/P20183" />
  <reg:lexicalAlias rdf:resource="http://rdaregistry.info/Elements/u/choreographicAdaptationOf.en" />
</owl:ObjectProperty>

<!-- Property: is choreography -->
<owl:ObjectProperty rdf:about="http://rdaregistry.info/Elements/u/P60740">
  <rdfs:isDefinedBy rdf:resource="http://rdaregistry.info/Elements/u/" />
  <reg:status rdf:resource="http://metadataregistry.org/uri/RegStatus/1001" />
  <rdf:type rdf:resource="http://www.w3.org/1999/02/22-rdf-syntax-ns#Property" />
  <reg:name xml:lang="en">choreography</reg:name>
  <rdfs:label xml:lang="en">is choreography</rdfs:label>
  <reg:lexicalAlias rdf:resource="http://rdaregistry.info/Elements/u/choreography.en" />
  <skos:definition xml:lang="en">Relates a resource to a resource that provides choreography for use in a related resource.</skos:definition>
  <owl:inverseOf rdf:resource="http://rdaregistry.info/Elements/u/P60741" />
  <rdfs:subPropertyOf rdf:resource="http://rdaregistry.info/Elements/u/P60198" />
</owl:ObjectProperty>

<!-- Property: is choreography for -->
<owl:ObjectProperty rdf:about="http://rdaregistry.info/Elements/u/P60741">
  <rdfs:isDefinedBy rdf:resource="http://rdaregistry.info/Elements/u/" />
  <reg:status rdf:resource="http://metadataregistry.org/uri/RegStatus/1001" />
  <rdf:type rdf:resource="http://www.w3.org/1999/02/22-rdf-syntax-ns#Property" />
  <reg:name xml:lang="en">choreographyFor</reg:name>
  <rdfs:label xml:lang="en">is choreography for</rdfs:label>
  <reg:lexicalAlias rdf:resource="http://rdaregistry.info/Elements/u/choreographyFor.en" />
  <skos:definition xml:lang="en">Relates a resource to a resource that uses choreography of a related resource.</skos:definition>
  <owl:inverseOf rdf:resource="http://rdaregistry.info/Elements/u/P60740" />
  <rdfs:subPropertyOf rdf:resource="http://rdaregistry.info/Elements/u/P60198" />
</owl:ObjectProperty>

<!-- Property: has chronological designation of first issue or part of sequence -->
<owl:ObjectProperty rdf:about="http://rdaregistry.info/Elements/u/P60501">
  <rdfs:isDefinedBy rdf:resource="http://rdaregistry.info/Elements/u/" />
  <reg:status rdf:resource="http://metadataregistry.org/uri/RegStatus/1001" />
  <reg:name xml:lang="en">chronologicalDesignationOfFirstIssueOrPartOfSequence</reg:name>
  <rdfs:label xml:lang="en">has chronological designation of first issue or part of sequence</rdfs:label>
  <skos:definition xml:lang="en">Relates a resource to a designation in date form presented on the first issue or part of a serial issued in a sequence of numbering.</skos:definition>
  <rdf:type rdf:resource="http://www.w3.org/1999/02/22-rdf-syntax-ns#Property" />
  <rdfs:subPropertyOf rdf:resource="http://rdaregistry.info/Elements/u/P60533" />
  <reg:hasSubproperty rdf:resource="http://rdaregistry.info/Elements/m/P30149" />
  <reg:lexicalAlias rdf:resource="http://rdaregistry.info/Elements/u/chronologicalDesignationOfFirstIssueOrPartOfSequence.en" />
  <skos:scopeNote xml:lang="en">Designation includes a year; year and month; month, day, and year.</skos:scopeNote>
</owl:ObjectProperty>

<!-- Property: has chronological designation of last issue or part of sequence -->
<owl:ObjectProperty rdf:about="http://rdaregistry.info/Elements/u/P60502">
  <rdfs:isDefinedBy rdf:resource="http://rdaregistry.info/Elements/u/" />
  <reg:status rdf:resource="http://metadataregistry.org/uri/RegStatus/1001" />
  <reg:name xml:lang="en">chronologicalDesignationOfLastIssueOrPartOfSequence</reg:name>
  <rdfs:label xml:lang="en">has chronological designation of last issue or part of sequence</rdfs:label>
  <skos:definition xml:lang="en">Relates a resource to a designation in date form presented on the last issue or part of a serial issued in a sequence of numbering.</skos:definition>
  <rdf:type rdf:resource="http://www.w3.org/1999/02/22-rdf-syntax-ns#Property" />
  <rdfs:subPropertyOf rdf:resource="http://rdaregistry.info/Elements/u/P60533" />
  <reg:hasSubproperty rdf:resource="http://rdaregistry.info/Elements/m/P30150" />
  <reg:lexicalAlias rdf:resource="http://rdaregistry.info/Elements/u/chronologicalDesignationOfLastIssueOrPartOfSequence.en" />
  <skos:scopeNote xml:lang="en">Designation includes a year; year and month; month, day, and year.</skos:scopeNote>
</owl:ObjectProperty>

<!-- Property: has colleague -->
<owl:ObjectProperty rdf:about="http://rdaregistry.info/Elements/u/P60853">
  <rdfs:isDefinedBy rdf:resource="http://rdaregistry.info/Elements/u/" />
  <reg:status rdf:resource="http://metadataregistry.org/uri/RegStatus/1001" />
  <rdf:type rdf:resource="http://www.w3.org/1999/02/22-rdf-syntax-ns#Property" />
  <reg:name xml:lang="en">colleague</reg:name>
  <rdfs:label xml:lang="en">has colleague</rdfs:label>
  <reg:lexicalAlias rdf:resource="http://rdaregistry.info/Elements/u/colleague.en" />
  <skos:definition xml:lang="en">Relates an agent to a fellow member of a profession, staff, or academic faculty.</skos:definition>
  <owl:inverseOf rdf:resource="http://rdaregistry.info/Elements/u/P60853" />
  <reg:hasSubproperty rdf:resource="http://rdaregistry.info/Elements/a/P50274" />
  <rdfs:subPropertyOf rdf:resource="http://rdaregistry.info/Elements/u/P60454" />
  <reg:hasSubproperty rdf:resource="http://rdaregistry.info/Elements/u/P60857" />
  <reg:hasSubproperty rdf:resource="http://rdaregistry.info/Elements/u/P60858" />
  <reg:hasSubproperty rdf:resource="http://rdaregistry.info/Elements/u/P60859" />
  <reg:hasSubproperty rdf:resource="http://rdaregistry.info/Elements/u/P60860" />
</owl:ObjectProperty>

<!-- Property: has collection registrar -->
<owl:ObjectProperty rdf:about="http://rdaregistry.info/Elements/u/P60067">
  <rdfs:isDefinedBy rdf:resource="http://rdaregistry.info/Elements/u/" />
  <reg:status rdf:resource="http://metadataregistry.org/uri/RegStatus/1001" />
  <reg:name xml:lang="en">collectionRegistrar</reg:name>
  <rdfs:label xml:lang="en">has collection registrar</rdfs:label>
  <skos:definition xml:lang="en">Relates a resource to a curator who lists or inventories resources in an aggregate resource such as a collection of resources.</skos:definition>
  <rdf:type rdf:resource="http://www.w3.org/1999/02/22-rdf-syntax-ns#Property" />
  <rdfs:subPropertyOf rdf:resource="http://rdaregistry.info/Elements/u/P60376" />
  <owl:inverseOf rdf:resource="http://rdaregistry.info/Elements/u/P60007" />
  <reg:hasSubproperty rdf:resource="http://rdaregistry.info/Elements/i/P40005" />
  <reg:lexicalAlias rdf:resource="http://rdaregistry.info/Elements/u/collectionRegistrar.en" />
</owl:ObjectProperty>

<!-- Property: is collection registrar of -->
<owl:ObjectProperty rdf:about="http://rdaregistry.info/Elements/u/P60007">
  <rdfs:isDefinedBy rdf:resource="http://rdaregistry.info/Elements/u/" />
  <reg:status rdf:resource="http://metadataregistry.org/uri/RegStatus/1001" />
  <reg:name xml:lang="en">collectionRegistrarOf</reg:name>
  <rdfs:label xml:lang="en">is collection registrar of</rdfs:label>
  <skos:definition xml:lang="en">Relates a curator who lists or inventories resources in an aggregate resource such as a collection of resources to a resource.</skos:definition>
  <rdf:type rdf:resource="http://www.w3.org/1999/02/22-rdf-syntax-ns#Property" />
  <rdfs:subPropertyOf rdf:resource="http://rdaregistry.info/Elements/u/P60604" />
  <owl:inverseOf rdf:resource="http://rdaregistry.info/Elements/u/P60067" />
  <reg:hasSubproperty rdf:resource="http://rdaregistry.info/Elements/a/P50046" />
  <reg:lexicalAlias rdf:resource="http://rdaregistry.info/Elements/u/collectionRegistrarOf.en" />
</owl:ObjectProperty>

<!-- Property: has collector -->
<owl:ObjectProperty rdf:about="http://rdaregistry.info/Elements/u/P60066">
  <rdfs:isDefinedBy rdf:resource="http://rdaregistry.info/Elements/u/" />
  <reg:status rdf:resource="http://metadataregistry.org/uri/RegStatus/1001" />
  <reg:name xml:lang="en">collector</reg:name>
  <rdfs:label xml:lang="en">has collector</rdfs:label>
  <skos:definition xml:lang="en">Relates a resource to a curator who brings together resources from various sources that are then arranged, described, and cataloged as a collection.</skos:definition>
  <rdf:type rdf:resource="http://www.w3.org/1999/02/22-rdf-syntax-ns#Property" />
  <rdfs:subPropertyOf rdf:resource="http://rdaregistry.info/Elements/u/P60376" />
  <owl:inverseOf rdf:resource="http://rdaregistry.info/Elements/u/P60006" />
  <reg:hasSubproperty rdf:resource="http://rdaregistry.info/Elements/i/P40004" />
  <reg:lexicalAlias rdf:resource="http://rdaregistry.info/Elements/u/collector.en" />
</owl:ObjectProperty>

<!-- Property: is collector of -->
<owl:ObjectProperty rdf:about="http://rdaregistry.info/Elements/u/P60006">
  <rdfs:isDefinedBy rdf:resource="http://rdaregistry.info/Elements/u/" />
  <reg:status rdf:resource="http://metadataregistry.org/uri/RegStatus/1001" />
  <reg:name xml:lang="en">collectorOf</reg:name>
  <rdfs:label xml:lang="en">is collector of</rdfs:label>
  <skos:definition xml:lang="en">Relates a curator who brings together resources from various sources that are then arranged, described, and cataloged as a collection to a resource.</skos:definition>
  <rdf:type rdf:resource="http://www.w3.org/1999/02/22-rdf-syntax-ns#Property" />
  <rdfs:subPropertyOf rdf:resource="http://rdaregistry.info/Elements/u/P60604" />
  <owl:inverseOf rdf:resource="http://rdaregistry.info/Elements/u/P60066" />
  <reg:hasSubproperty rdf:resource="http://rdaregistry.info/Elements/a/P50045" />
  <reg:lexicalAlias rdf:resource="http://rdaregistry.info/Elements/u/collectorOf.en" />
</owl:ObjectProperty>

<!-- Property: has collotyper -->
<owl:ObjectProperty rdf:about="http://rdaregistry.info/Elements/u/P60417">
  <rdfs:isDefinedBy rdf:resource="http://rdaregistry.info/Elements/u/" />
  <reg:status rdf:resource="http://metadataregistry.org/uri/RegStatus/1001" />
  <reg:name xml:lang="en">collotyper</reg:name>
  <rdfs:label xml:lang="en">has collotyper</rdfs:label>
  <skos:definition xml:lang="en">Relates a resource to an agent involved in manufacturing a resource using a photomechanical process for making prints directly from a hardened film of gelatin or other colloid that has ink-receptive and ink-repellent surfaces.</skos:definition>
  <rdf:type rdf:resource="http://www.w3.org/1999/02/22-rdf-syntax-ns#Property" />
  <rdfs:subPropertyOf rdf:resource="http://rdaregistry.info/Elements/u/P60443" />
  <owl:inverseOf rdf:resource="http://rdaregistry.info/Elements/u/P60645" />
  <reg:hasSubproperty rdf:resource="http://rdaregistry.info/Elements/m/P30077" />
  <reg:lexicalAlias rdf:resource="http://rdaregistry.info/Elements/u/collotyper.en" />
</owl:ObjectProperty>

<!-- Property: is collotyper of -->
<owl:ObjectProperty rdf:about="http://rdaregistry.info/Elements/u/P60645">
  <rdfs:isDefinedBy rdf:resource="http://rdaregistry.info/Elements/u/" />
  <reg:status rdf:resource="http://metadataregistry.org/uri/RegStatus/1001" />
  <reg:name xml:lang="en">collotyperOf</reg:name>
  <rdfs:label xml:lang="en">is collotyper of</rdfs:label>
  <skos:definition xml:lang="en">Relates an agent involved in manufacturing a resource using a photomechanical process for making prints directly from a hardened film of gelatin or other colloid that has ink-receptive and ink-repellent surfaces to a resource.</skos:definition>
  <rdf:type rdf:resource="http://www.w3.org/1999/02/22-rdf-syntax-ns#Property" />
  <rdfs:subPropertyOf rdf:resource="http://rdaregistry.info/Elements/u/P60669" />
  <owl:inverseOf rdf:resource="http://rdaregistry.info/Elements/u/P60417" />
  <reg:hasSubproperty rdf:resource="http://rdaregistry.info/Elements/a/P50178" />
  <reg:lexicalAlias rdf:resource="http://rdaregistry.info/Elements/u/collotyperOf.en" />
</owl:ObjectProperty>

<!-- Property: has colour content -->
<owl:ObjectProperty rdf:about="http://rdaregistry.info/Elements/u/P60558">
  <rdfs:isDefinedBy rdf:resource="http://rdaregistry.info/Elements/u/" />
  <reg:status rdf:resource="http://metadataregistry.org/uri/RegStatus/1001" />
  <reg:name xml:lang="en">colourContent</reg:name>
  <rdfs:label xml:lang="en">has colour content</rdfs:label>
  <skos:definition xml:lang="en">Relates a resource to a presence of colour, tone, etc., in the content of a resource.</skos:definition>
  <rdf:type rdf:resource="http://www.w3.org/1999/02/22-rdf-syntax-ns#Property" />
  <reg:hasSubproperty rdf:resource="http://rdaregistry.info/Elements/e/P20224" />
  <reg:lexicalAlias rdf:resource="http://rdaregistry.info/Elements/u/colourContent.en" />
  <skos:scopeNote xml:lang="en">Black, white, single colour shades of black, single colour tints of white, and single colour tones of gray are considered to be single colours.</skos:scopeNote>
</owl:ObjectProperty>

<!-- Property: has colourist -->
<owl:ObjectProperty rdf:about="http://rdaregistry.info/Elements/u/P60838">
  <rdfs:isDefinedBy rdf:resource="http://rdaregistry.info/Elements/u/" />
  <reg:status rdf:resource="http://metadataregistry.org/uri/RegStatus/1001" />
  <rdf:type rdf:resource="http://www.w3.org/1999/02/22-rdf-syntax-ns#Property" />
  <reg:name xml:lang="en">colourist</reg:name>
  <rdfs:label xml:lang="en">has colourist</rdfs:label>
  <reg:lexicalAlias rdf:resource="http://rdaregistry.info/Elements/u/colourist.en" />
  <skos:definition xml:lang="en">Relates a resource to an agent contributing to a resource by applying colour to drawings, prints, photographs, maps, moving images, etc.</skos:definition>
  <owl:inverseOf rdf:resource="http://rdaregistry.info/Elements/u/P60839" />
  <reg:hasSubproperty rdf:resource="http://rdaregistry.info/Elements/e/P20283" />
  <rdfs:subPropertyOf rdf:resource="http://rdaregistry.info/Elements/u/P60398" />
</owl:ObjectProperty>

<!-- Property: is colourist of -->
<owl:ObjectProperty rdf:about="http://rdaregistry.info/Elements/u/P60839">
  <rdfs:isDefinedBy rdf:resource="http://rdaregistry.info/Elements/u/" />
  <reg:status rdf:resource="http://metadataregistry.org/uri/RegStatus/1001" />
  <rdf:type rdf:resource="http://www.w3.org/1999/02/22-rdf-syntax-ns#Property" />
  <reg:name xml:lang="en">colouristOf</reg:name>
  <rdfs:label xml:lang="en">is colourist of</rdfs:label>
  <reg:lexicalAlias rdf:resource="http://rdaregistry.info/Elements/u/colouristOf.en" />
  <skos:definition xml:lang="en">Relates an agent contributing to a resource by applying colour to drawings, prints, photographs, maps, moving images, etc. to a resource.</skos:definition>
  <owl:inverseOf rdf:resource="http://rdaregistry.info/Elements/u/P60838" />
  <reg:hasSubproperty rdf:resource="http://rdaregistry.info/Elements/a/P50266" />
  <rdfs:subPropertyOf rdf:resource="http://rdaregistry.info/Elements/u/P60626" />
</owl:ObjectProperty>

<!-- Property: has commemoration -->
<owl:ObjectProperty rdf:about="http://rdaregistry.info/Elements/u/P60846">
  <rdfs:isDefinedBy rdf:resource="http://rdaregistry.info/Elements/u/" />
  <reg:status rdf:resource="http://metadataregistry.org/uri/RegStatus/1001" />
  <rdf:type rdf:resource="http://www.w3.org/1999/02/22-rdf-syntax-ns#Property" />
  <reg:name xml:lang="en">commemoration</reg:name>
  <rdfs:label xml:lang="en">has commemoration</rdfs:label>
  <reg:lexicalAlias rdf:resource="http://rdaregistry.info/Elements/u/commemoration.en" />
  <skos:definition xml:lang="en">Relates a resource to a resource created to commemorate an earlier resource.</skos:definition>
  <owl:inverseOf rdf:resource="http://rdaregistry.info/Elements/u/P60847" />
  <rdfs:subPropertyOf rdf:resource="http://rdaregistry.info/Elements/u/P60848" />
</owl:ObjectProperty>

<!-- Property: is commemoration of -->
<owl:ObjectProperty rdf:about="http://rdaregistry.info/Elements/u/P60847">
  <rdfs:isDefinedBy rdf:resource="http://rdaregistry.info/Elements/u/" />
  <reg:status rdf:resource="http://metadataregistry.org/uri/RegStatus/1001" />
  <rdf:type rdf:resource="http://www.w3.org/1999/02/22-rdf-syntax-ns#Property" />
  <reg:name xml:lang="en">commemorationOf</reg:name>
  <rdfs:label xml:lang="en">is commemoration of</rdfs:label>
  <reg:lexicalAlias rdf:resource="http://rdaregistry.info/Elements/u/commemorationOf.en" />
  <skos:definition xml:lang="en">Relates a resource to a resource commemorated in a later resource.</skos:definition>
  <owl:inverseOf rdf:resource="http://rdaregistry.info/Elements/u/P60846" />
  <rdfs:subPropertyOf rdf:resource="http://rdaregistry.info/Elements/u/P60848" />
</owl:ObjectProperty>

<!-- Property: is commentary in -->
<owl:ObjectProperty rdf:about="http://rdaregistry.info/Elements/u/P60213">
  <rdfs:isDefinedBy rdf:resource="http://rdaregistry.info/Elements/u/" />
  <reg:status rdf:resource="http://metadataregistry.org/uri/RegStatus/1001" />
  <reg:name xml:lang="en">commentaryIn</reg:name>
  <rdfs:label xml:lang="en">is commentary in</rdfs:label>
  <skos:definition xml:lang="en">Relates a resource to a resource that contains a set of explanatory or critical notes on a described resource</skos:definition>
  <rdf:type rdf:resource="http://www.w3.org/1999/02/22-rdf-syntax-ns#Property" />
  <rdfs:subPropertyOf rdf:resource="http://rdaregistry.info/Elements/u/P60215" />
  <owl:inverseOf rdf:resource="http://rdaregistry.info/Elements/u/P60298" />
  <reg:hasSubproperty rdf:resource="http://rdaregistry.info/Elements/e/P20271" />
  <reg:hasSubproperty rdf:resource="http://rdaregistry.info/Elements/i/P40064" />
  <reg:hasSubproperty rdf:resource="http://rdaregistry.info/Elements/m/P30256" />
  <reg:lexicalAlias rdf:resource="http://rdaregistry.info/Elements/u/commentaryIn.en" />
</owl:ObjectProperty>

<!-- Property: is commentary on -->
<owl:ObjectProperty rdf:about="http://rdaregistry.info/Elements/u/P60298">
  <rdfs:isDefinedBy rdf:resource="http://rdaregistry.info/Elements/u/" />
  <reg:status rdf:resource="http://metadataregistry.org/uri/RegStatus/1001" />
  <reg:name xml:lang="en">commentaryOn</reg:name>
  <rdfs:label xml:lang="en">is commentary on</rdfs:label>
  <skos:definition xml:lang="en">Relates a resource to a resource used as a basis for a set of explanatory or critical notes.</skos:definition>
  <rdf:type rdf:resource="http://www.w3.org/1999/02/22-rdf-syntax-ns#Property" />
  <rdfs:subPropertyOf rdf:resource="http://rdaregistry.info/Elements/u/P60190" />
  <owl:inverseOf rdf:resource="http://rdaregistry.info/Elements/u/P60213" />
  <reg:hasSubproperty rdf:resource="http://rdaregistry.info/Elements/w/P10270" />
  <reg:hasSubproperty rdf:resource="http://rdaregistry.info/Elements/w/P10276" />
  <reg:hasSubproperty rdf:resource="http://rdaregistry.info/Elements/w/P10282" />
  <reg:lexicalAlias rdf:resource="http://rdaregistry.info/Elements/u/commentaryOn.en" />
</owl:ObjectProperty>

<!-- Property: has commentator -->
<owl:ObjectProperty rdf:about="http://rdaregistry.info/Elements/u/P60151">
  <rdfs:isDefinedBy rdf:resource="http://rdaregistry.info/Elements/u/" />
  <reg:status rdf:resource="http://metadataregistry.org/uri/RegStatus/1001" />
  <reg:name xml:lang="en">commentator</reg:name>
  <rdfs:label xml:lang="en">has commentator</rdfs:label>
  <skos:definition xml:lang="en">Relates a resource to a performer contributing to a resource by providing interpretation, analysis, or a discussion of the subject matter on a recording, film, or other audiovisual medium.</skos:definition>
  <rdf:type rdf:resource="http://www.w3.org/1999/02/22-rdf-syntax-ns#Property" />
  <rdfs:subPropertyOf rdf:resource="http://rdaregistry.info/Elements/u/P60387" />
  <owl:inverseOf rdf:resource="http://rdaregistry.info/Elements/u/P60026" />
  <reg:hasSubproperty rdf:resource="http://rdaregistry.info/Elements/e/P20021" />
  <reg:lexicalAlias rdf:resource="http://rdaregistry.info/Elements/u/commentator.en" />
</owl:ObjectProperty>

<!-- Property: is commentator of -->
<owl:ObjectProperty rdf:about="http://rdaregistry.info/Elements/u/P60026">
  <rdfs:isDefinedBy rdf:resource="http://rdaregistry.info/Elements/u/" />
  <reg:status rdf:resource="http://metadataregistry.org/uri/RegStatus/1001" />
  <reg:name xml:lang="en">commentatorOf</reg:name>
  <rdfs:label xml:lang="en">is commentator of</rdfs:label>
  <skos:definition xml:lang="en">Relates a performer contributing to a resource by providing interpretation, analysis, or a discussion of the subject matter on a recording, film, or other audiovisual medium to a resource.</skos:definition>
  <rdf:type rdf:resource="http://www.w3.org/1999/02/22-rdf-syntax-ns#Property" />
  <rdfs:subPropertyOf rdf:resource="http://rdaregistry.info/Elements/u/P60615" />
  <owl:inverseOf rdf:resource="http://rdaregistry.info/Elements/u/P60151" />
  <reg:hasSubproperty rdf:resource="http://rdaregistry.info/Elements/a/P50080" />
  <reg:lexicalAlias rdf:resource="http://rdaregistry.info/Elements/u/commentatorOf.en" />
</owl:ObjectProperty>

<!-- Property: has commissioning body -->
<owl:ObjectProperty rdf:about="http://rdaregistry.info/Elements/u/P60826">
  <rdfs:isDefinedBy rdf:resource="http://rdaregistry.info/Elements/u/" />
  <reg:status rdf:resource="http://metadataregistry.org/uri/RegStatus/1001" />
  <rdf:type rdf:resource="http://www.w3.org/1999/02/22-rdf-syntax-ns#Property" />
  <reg:name xml:lang="en">commissioningBody</reg:name>
  <rdfs:label xml:lang="en">has commissioning body</rdfs:label>
  <reg:lexicalAlias rdf:resource="http://rdaregistry.info/Elements/u/commissioningBody.en" />
  <skos:definition xml:lang="en">Relates a resource to an agent responsible for commissioning a resource.</skos:definition>
  <owl:inverseOf rdf:resource="http://rdaregistry.info/Elements/u/P60827" />
  <rdfs:subPropertyOf rdf:resource="http://rdaregistry.info/Elements/u/P60447" />
</owl:ObjectProperty>

<!-- Property: is commissioning body of -->
<owl:ObjectProperty rdf:about="http://rdaregistry.info/Elements/u/P60827">
  <rdfs:isDefinedBy rdf:resource="http://rdaregistry.info/Elements/u/" />
  <reg:status rdf:resource="http://metadataregistry.org/uri/RegStatus/1001" />
  <rdf:type rdf:resource="http://www.w3.org/1999/02/22-rdf-syntax-ns#Property" />
  <reg:name xml:lang="en">commissioningBodyOf</reg:name>
  <rdfs:label xml:lang="en">is commissioning body of</rdfs:label>
  <reg:lexicalAlias rdf:resource="http://rdaregistry.info/Elements/u/commissioningBodyOf.en" />
  <skos:definition xml:lang="en">Relates an agent responsible for commissioning a resource to a resource.</skos:definition>
  <owl:inverseOf rdf:resource="http://rdaregistry.info/Elements/u/P60826" />
  <reg:hasSubproperty rdf:resource="http://rdaregistry.info/Elements/a/P50262" />
  <rdfs:subPropertyOf rdf:resource="http://rdaregistry.info/Elements/u/P60672" />
</owl:ObjectProperty>

<!-- Property: has compiler -->
<owl:ObjectProperty rdf:about="http://rdaregistry.info/Elements/u/P60428">
  <rdfs:isDefinedBy rdf:resource="http://rdaregistry.info/Elements/u/" />
  <reg:status rdf:resource="http://metadataregistry.org/uri/RegStatus/1001" />
  <reg:name xml:lang="en">compiler</reg:name>
  <rdfs:label xml:lang="en">has compiler</rdfs:label>
  <skos:definition xml:lang="en">Relates a resource to an agent responsible for creating a new resource such as a bibliography or a directory by selecting, arranging, aggregating, and editing data, information, etc.</skos:definition>
  <rdf:type rdf:resource="http://www.w3.org/1999/02/22-rdf-syntax-ns#Property" />
  <rdfs:subPropertyOf rdf:resource="http://rdaregistry.info/Elements/u/P60447" />
  <owl:inverseOf rdf:resource="http://rdaregistry.info/Elements/u/P60657" />
  <reg:lexicalAlias rdf:resource="http://rdaregistry.info/Elements/u/compiler.en" />
  <skos:scopeNote xml:lang="en">Revising or clarifying the content, or selecting and putting together resources or parts of resources, by one or more creators is excluded</skos:scopeNote>
  <rdakit:seeAlso rdf:resource="http://rdaregistry.info/Elements/u/P60393" />
</owl:ObjectProperty>

<!-- Property: is compiler of -->
<owl:ObjectProperty rdf:about="http://rdaregistry.info/Elements/u/P60657">
  <rdfs:isDefinedBy rdf:resource="http://rdaregistry.info/Elements/u/" />
  <reg:status rdf:resource="http://metadataregistry.org/uri/RegStatus/1001" />
  <reg:name xml:lang="en">compilerOf</reg:name>
  <rdfs:label xml:lang="en">is compiler of</rdfs:label>
  <skos:definition xml:lang="en">Relates an agent responsible for creating a new resource such as a bibliography or a directory by selecting, arranging, aggregating, and editing data, information, etc., to a resource.</skos:definition>
  <rdf:type rdf:resource="http://www.w3.org/1999/02/22-rdf-syntax-ns#Property" />
  <rdfs:subPropertyOf rdf:resource="http://rdaregistry.info/Elements/u/P60672" />
  <owl:inverseOf rdf:resource="http://rdaregistry.info/Elements/u/P60428" />
  <reg:hasSubproperty rdf:resource="http://rdaregistry.info/Elements/a/P50189" />
  <reg:lexicalAlias rdf:resource="http://rdaregistry.info/Elements/u/compilerOf.en" />
  <rdakit:seeAlso rdf:resource="http://rdaregistry.info/Elements/u/P60621" />
</owl:ObjectProperty>

<!-- Property: is complemented by -->
<owl:ObjectProperty rdf:about="http://rdaregistry.info/Elements/u/P60198">
  <rdfs:isDefinedBy rdf:resource="http://rdaregistry.info/Elements/u/" />
  <reg:status rdf:resource="http://metadataregistry.org/uri/RegStatus/1001" />
  <reg:name xml:lang="en">complementedBy</reg:name>
  <rdfs:label xml:lang="en">is complemented by</rdfs:label>
  <skos:definition xml:lang="en">Relates a resource to a resource paired with another resource without either resource being considered to predominate.</skos:definition>
  <rdf:type rdf:resource="http://www.w3.org/1999/02/22-rdf-syntax-ns#Property" />
  <rdfs:subPropertyOf rdf:resource="http://rdaregistry.info/Elements/u/P60709" />
  <owl:inverseOf rdf:resource="http://rdaregistry.info/Elements/u/P60198" />
  <reg:hasSubproperty rdf:resource="http://rdaregistry.info/Elements/u/P60117" />
  <reg:hasSubproperty rdf:resource="http://rdaregistry.info/Elements/u/P60201" />
  <reg:hasSubproperty rdf:resource="http://rdaregistry.info/Elements/u/P60264" />
  <reg:hasSubproperty rdf:resource="http://rdaregistry.info/Elements/u/P60267" />
  <reg:hasSubproperty rdf:resource="http://rdaregistry.info/Elements/u/P60270" />
  <reg:hasSubproperty rdf:resource="http://rdaregistry.info/Elements/u/P60285" />
  <reg:hasSubproperty rdf:resource="http://rdaregistry.info/Elements/e/P20100" />
  <reg:lexicalAlias rdf:resource="http://rdaregistry.info/Elements/u/complementedBy.en" />
  <reg:hasSubproperty rdf:resource="http://rdaregistry.info/Elements/u/P60740" />
  <reg:hasSubproperty rdf:resource="http://rdaregistry.info/Elements/u/P60741" />
</owl:ObjectProperty>

<!-- Property: has component of merger -->
<owl:ObjectProperty rdf:about="http://rdaregistry.info/Elements/u/P60736">
  <rdfs:isDefinedBy rdf:resource="http://rdaregistry.info/Elements/u/" />
  <reg:status rdf:resource="http://metadataregistry.org/uri/RegStatus/1001" />
  <reg:name xml:lang="en">componentOfMerger</reg:name>
  <rdfs:label xml:lang="en">has component of merger</rdfs:label>
  <skos:definition xml:lang="en">Relates an agent that formed another agent by merging with one or more other agents to an agent.</skos:definition>
  <rdf:type rdf:resource="http://www.w3.org/1999/02/22-rdf-syntax-ns#Property" />
  <owl:inverseOf rdf:resource="http://rdaregistry.info/Elements/u/P60684" />
  <reg:hasSubproperty rdf:resource="http://rdaregistry.info/Elements/a/P50232" />
  <reg:lexicalAlias rdf:resource="http://rdaregistry.info/Elements/u/componentOfMerger.en" />
</owl:ObjectProperty>

<!-- Property: has composer -->
<owl:ObjectProperty rdf:about="http://rdaregistry.info/Elements/u/P60426">
  <rdfs:isDefinedBy rdf:resource="http://rdaregistry.info/Elements/u/" />
  <reg:status rdf:resource="http://metadataregistry.org/uri/RegStatus/1001" />
  <reg:name xml:lang="en">composer</reg:name>
  <rdfs:label xml:lang="en">has composer</rdfs:label>
  <skos:definition xml:lang="en">Relates a resource to an agent responsible for creating a musical resource.</skos:definition>
  <rdf:type rdf:resource="http://www.w3.org/1999/02/22-rdf-syntax-ns#Property" />
  <rdfs:subPropertyOf rdf:resource="http://rdaregistry.info/Elements/u/P60447" />
  <owl:inverseOf rdf:resource="http://rdaregistry.info/Elements/u/P60655" />
  <reg:hasSubproperty rdf:resource="http://rdaregistry.info/Elements/e/P20026" />
  <reg:lexicalAlias rdf:resource="http://rdaregistry.info/Elements/u/composer.en" />
  <skos:scopeNote xml:lang="en">Adaptation of another musical resource to form a distinct alteration, paraphrasing a resource or creating a resource in the general style of another composer, or creating a resource that is based on the music of another composer, is included.</skos:scopeNote>
</owl:ObjectProperty>

<!-- Property: is composer of -->
<owl:ObjectProperty rdf:about="http://rdaregistry.info/Elements/u/P60655">
  <rdfs:isDefinedBy rdf:resource="http://rdaregistry.info/Elements/u/" />
  <reg:status rdf:resource="http://metadataregistry.org/uri/RegStatus/1001" />
  <reg:name xml:lang="en">composerOf</reg:name>
  <rdfs:label xml:lang="en">is composer of</rdfs:label>
  <skos:definition xml:lang="en">Relates an agent responsible for creating a musical resource to a resource.</skos:definition>
  <rdf:type rdf:resource="http://www.w3.org/1999/02/22-rdf-syntax-ns#Property" />
  <rdfs:subPropertyOf rdf:resource="http://rdaregistry.info/Elements/u/P60672" />
  <owl:inverseOf rdf:resource="http://rdaregistry.info/Elements/u/P60426" />
  <reg:hasSubproperty rdf:resource="http://rdaregistry.info/Elements/a/P50134" />
  <reg:hasSubproperty rdf:resource="http://rdaregistry.info/Elements/a/P50187" />
  <reg:lexicalAlias rdf:resource="http://rdaregistry.info/Elements/u/composerOf.en" />
</owl:ObjectProperty>

<!-- Property: is concordance -->
<owl:ObjectProperty rdf:about="http://rdaregistry.info/Elements/u/P60208">
  <rdfs:isDefinedBy rdf:resource="http://rdaregistry.info/Elements/u/" />
  <reg:status rdf:resource="http://metadataregistry.org/uri/RegStatus/1001" />
  <reg:name xml:lang="en">concordance</reg:name>
  <rdfs:label xml:lang="en">is concordance</rdfs:label>
  <skos:definition xml:lang="en">Relates a resource to a resource that consists of an index of all a words in a predominant resource.</skos:definition>
  <rdf:type rdf:resource="http://www.w3.org/1999/02/22-rdf-syntax-ns#Property" />
  <rdfs:subPropertyOf rdf:resource="http://rdaregistry.info/Elements/u/P60204" />
  <owl:inverseOf rdf:resource="http://rdaregistry.info/Elements/u/P60291" />
  <reg:hasSubproperty rdf:resource="http://rdaregistry.info/Elements/e/P20108" />
  <reg:lexicalAlias rdf:resource="http://rdaregistry.info/Elements/u/concordance.en" />
</owl:ObjectProperty>

<!-- Property: is concordance to -->
<owl:ObjectProperty rdf:about="http://rdaregistry.info/Elements/u/P60291">
  <rdfs:isDefinedBy rdf:resource="http://rdaregistry.info/Elements/u/" />
  <reg:status rdf:resource="http://metadataregistry.org/uri/RegStatus/1001" />
  <reg:name xml:lang="en">concordanceTo</reg:name>
  <rdfs:label xml:lang="en">is concordance to</rdfs:label>
  <skos:definition xml:lang="en">Relates a resource to a resource used as a basis for a concordance, i.e. an index of all the words in the predominant resource.</skos:definition>
  <rdf:type rdf:resource="http://www.w3.org/1999/02/22-rdf-syntax-ns#Property" />
  <rdfs:subPropertyOf rdf:resource="http://rdaregistry.info/Elements/u/P60307" />
  <owl:inverseOf rdf:resource="http://rdaregistry.info/Elements/u/P60208" />
  <reg:hasSubproperty rdf:resource="http://rdaregistry.info/Elements/e/P20181" />
  <reg:lexicalAlias rdf:resource="http://rdaregistry.info/Elements/u/concordanceTo.en" />
</owl:ObjectProperty>

<!-- Property: has conductor -->
<owl:ObjectProperty rdf:about="http://rdaregistry.info/Elements/u/P60141">
  <rdfs:isDefinedBy rdf:resource="http://rdaregistry.info/Elements/u/" />
  <reg:status rdf:resource="http://metadataregistry.org/uri/RegStatus/1001" />
  <reg:name xml:lang="en">conductor</reg:name>
  <rdfs:label xml:lang="en">has conductor</rdfs:label>
  <skos:definition xml:lang="en">Relates a resource to a performer contributing to a musical resource by leading a performing group in a musical or dramatic presentation, etc.</skos:definition>
  <rdf:type rdf:resource="http://www.w3.org/1999/02/22-rdf-syntax-ns#Property" />
  <rdfs:subPropertyOf rdf:resource="http://rdaregistry.info/Elements/u/P60387" />
  <owl:inverseOf rdf:resource="http://rdaregistry.info/Elements/u/P60016" />
  <reg:hasSubproperty rdf:resource="http://rdaregistry.info/Elements/e/P20011" />
  <reg:lexicalAlias rdf:resource="http://rdaregistry.info/Elements/u/conductor.en" />
  <reg:hasSubproperty rdf:resource="http://rdaregistry.info/Elements/u/P60842" />
  <reg:hasSubproperty rdf:resource="http://rdaregistry.info/Elements/u/P60844" />
</owl:ObjectProperty>

<!-- Property: is conductor of -->
<owl:ObjectProperty rdf:about="http://rdaregistry.info/Elements/u/P60016">
  <rdfs:isDefinedBy rdf:resource="http://rdaregistry.info/Elements/u/" />
  <reg:status rdf:resource="http://metadataregistry.org/uri/RegStatus/1001" />
  <reg:name xml:lang="en">conductorOf</reg:name>
  <rdfs:label xml:lang="en">is conductor of</rdfs:label>
  <skos:definition xml:lang="en">Relates a performer contributing to a musical resource by leading a performing group in a musical or dramatic presentation, etc. to a resource.</skos:definition>
  <rdf:type rdf:resource="http://www.w3.org/1999/02/22-rdf-syntax-ns#Property" />
  <rdfs:subPropertyOf rdf:resource="http://rdaregistry.info/Elements/u/P60615" />
  <owl:inverseOf rdf:resource="http://rdaregistry.info/Elements/u/P60141" />
  <reg:hasSubproperty rdf:resource="http://rdaregistry.info/Elements/a/P50070" />
  <reg:lexicalAlias rdf:resource="http://rdaregistry.info/Elements/u/conductorOf.en" />
  <reg:hasSubproperty rdf:resource="http://rdaregistry.info/Elements/u/P60843" />
  <reg:hasSubproperty rdf:resource="http://rdaregistry.info/Elements/u/P60845" />
</owl:ObjectProperty>

<!-- Property: has configuration of playback channels -->
<owl:ObjectProperty rdf:about="http://rdaregistry.info/Elements/u/P60552">
  <rdfs:isDefinedBy rdf:resource="http://rdaregistry.info/Elements/u/" />
  <reg:status rdf:resource="http://metadataregistry.org/uri/RegStatus/1001" />
  <reg:name xml:lang="en">configurationOfPlaybackChannels</reg:name>
  <rdfs:label xml:lang="en">has configuration of playback channels</rdfs:label>
  <skos:definition xml:lang="en">Relates a resource to a number of sound channels used to make a recording.</skos:definition>
  <rdf:type rdf:resource="http://www.w3.org/1999/02/22-rdf-syntax-ns#Property" />
  <rdfs:subPropertyOf rdf:resource="http://rdaregistry.info/Elements/u/P60351" />
  <reg:hasSubproperty rdf:resource="http://rdaregistry.info/Elements/m/P30184" />
  <reg:lexicalAlias rdf:resource="http://rdaregistry.info/Elements/u/configurationOfPlaybackChannels.en" />
</owl:ObjectProperty>

<!-- Property: has consultant -->
<owl:ObjectProperty rdf:about="http://rdaregistry.info/Elements/u/P60465">
  <rdfs:isDefinedBy rdf:resource="http://rdaregistry.info/Elements/u/" />
  <reg:status rdf:resource="http://metadataregistry.org/uri/RegStatus/1001" />
  <reg:name xml:lang="en">consultant</reg:name>
  <rdfs:label xml:lang="en">has consultant</rdfs:label>
  <skos:definition xml:lang="en">Relates a resource to an agent who provides consultation services, and often makes recommendations, for another agent that is represented as a creator of a resource.</skos:definition>
  <rdf:type rdf:resource="http://www.w3.org/1999/02/22-rdf-syntax-ns#Property" />
  <rdfs:subPropertyOf rdf:resource="http://rdaregistry.info/Elements/u/P60447" />
  <owl:inverseOf rdf:resource="http://rdaregistry.info/Elements/u/P60701" />
  <reg:lexicalAlias rdf:resource="http://rdaregistry.info/Elements/u/consultant.en" />
</owl:ObjectProperty>

<!-- Property: is consultant of -->
<owl:ObjectProperty rdf:about="http://rdaregistry.info/Elements/u/P60701">
  <rdfs:isDefinedBy rdf:resource="http://rdaregistry.info/Elements/u/" />
  <reg:status rdf:resource="http://metadataregistry.org/uri/RegStatus/1001" />
  <reg:name xml:lang="en">consultantOf</reg:name>
  <rdfs:label xml:lang="en">is consultant of</rdfs:label>
  <skos:definition xml:lang="en">Relates an agent who provides consultation services, and often makes recommendations, for another agent that is represented as a creator of a resource to a resource.</skos:definition>
  <rdf:type rdf:resource="http://www.w3.org/1999/02/22-rdf-syntax-ns#Property" />
  <rdfs:subPropertyOf rdf:resource="http://rdaregistry.info/Elements/u/P60672" />
  <owl:inverseOf rdf:resource="http://rdaregistry.info/Elements/u/P60465" />
  <reg:hasSubproperty rdf:resource="http://rdaregistry.info/Elements/a/P50211" />
  <reg:lexicalAlias rdf:resource="http://rdaregistry.info/Elements/u/consultantOf.en" />
</owl:ObjectProperty>

<!-- Property: has contact information -->
<owl:ObjectProperty rdf:about="http://rdaregistry.info/Elements/u/P60490">
  <rdfs:isDefinedBy rdf:resource="http://rdaregistry.info/Elements/u/" />
  <reg:status rdf:resource="http://metadataregistry.org/uri/RegStatus/1001" />
  <reg:name xml:lang="en">contactInformation</reg:name>
  <rdfs:label xml:lang="en">has contact information</rdfs:label>
  <skos:definition xml:lang="en">Relates a resource to a name, address, etc., of an organization, etc., from which a resource may be obtained.</skos:definition>
  <rdf:type rdf:resource="http://www.w3.org/1999/02/22-rdf-syntax-ns#Property" />
  <reg:hasSubproperty rdf:resource="http://rdaregistry.info/Elements/m/P30141" />
  <reg:lexicalAlias rdf:resource="http://rdaregistry.info/Elements/u/contactInformation.en" />
  <skos:scopeNote xml:lang="en">Contact information includes the name, address, etc. of the publisher, distributor, etc. of a published resource, or of the archival repository that holds the resource.</skos:scopeNote>
</owl:ObjectProperty>

<!-- Property: is contained in -->
<owl:ObjectProperty rdf:about="http://rdaregistry.info/Elements/u/P60101">
  <rdfs:isDefinedBy rdf:resource="http://rdaregistry.info/Elements/u/" />
  <reg:status rdf:resource="http://metadataregistry.org/uri/RegStatus/1001" />
  <reg:name xml:lang="en">containedIn</reg:name>
  <rdfs:label xml:lang="en">is contained in</rdfs:label>
  <skos:definition xml:lang="en">Relates a resource to a larger resource of which a part is a discrete component.</skos:definition>
  <rdf:type rdf:resource="http://www.w3.org/1999/02/22-rdf-syntax-ns#Property" />
  <rdfs:subPropertyOf rdf:resource="http://rdaregistry.info/Elements/u/P60714" />
  <owl:inverseOf rdf:resource="http://rdaregistry.info/Elements/u/P60249" />
  <reg:hasSubproperty rdf:resource="http://rdaregistry.info/Elements/u/P60100" />
  <reg:hasSubproperty rdf:resource="http://rdaregistry.info/Elements/u/P60192" />
  <reg:hasSubproperty rdf:resource="http://rdaregistry.info/Elements/u/P60193" />
  <reg:hasSubproperty rdf:resource="http://rdaregistry.info/Elements/u/P60194" />
  <reg:hasSubproperty rdf:resource="http://rdaregistry.info/Elements/u/P60317" />
  <reg:hasSubproperty rdf:resource="http://rdaregistry.info/Elements/e/P20074" />
  <reg:hasSubproperty rdf:resource="http://rdaregistry.info/Elements/i/P40009" />
  <reg:hasSubproperty rdf:resource="http://rdaregistry.info/Elements/m/P30020" />
  <reg:lexicalAlias rdf:resource="http://rdaregistry.info/Elements/u/containedIn.en" />
</owl:ObjectProperty>

<!-- Property: is container of -->
<owl:ObjectProperty rdf:about="http://rdaregistry.info/Elements/u/P60249">
  <rdfs:isDefinedBy rdf:resource="http://rdaregistry.info/Elements/u/" />
  <reg:status rdf:resource="http://metadataregistry.org/uri/RegStatus/1001" />
  <reg:name xml:lang="en">containerOf</reg:name>
  <rdfs:label xml:lang="en">is container of</rdfs:label>
  <skos:definition xml:lang="en">Relates a resource to a resource that is a discrete component of a larger resource.</skos:definition>
  <rdf:type rdf:resource="http://www.w3.org/1999/02/22-rdf-syntax-ns#Property" />
  <rdfs:subPropertyOf rdf:resource="http://rdaregistry.info/Elements/u/P60714" />
  <owl:inverseOf rdf:resource="http://rdaregistry.info/Elements/u/P60101" />
  <reg:hasSubproperty rdf:resource="http://rdaregistry.info/Elements/u/P60183" />
  <reg:hasSubproperty rdf:resource="http://rdaregistry.info/Elements/u/P60207" />
  <reg:hasSubproperty rdf:resource="http://rdaregistry.info/Elements/u/P60240" />
  <reg:hasSubproperty rdf:resource="http://rdaregistry.info/Elements/u/P60300" />
  <reg:hasSubproperty rdf:resource="http://rdaregistry.info/Elements/u/P60316" />
  <reg:hasSubproperty rdf:resource="http://rdaregistry.info/Elements/e/P20145" />
  <reg:hasSubproperty rdf:resource="http://rdaregistry.info/Elements/i/P40034" />
  <reg:hasSubproperty rdf:resource="http://rdaregistry.info/Elements/m/P30033" />
  <reg:lexicalAlias rdf:resource="http://rdaregistry.info/Elements/u/containerOf.en" />
</owl:ObjectProperty>

<!-- Property: has content type -->
<owl:ObjectProperty rdf:about="http://rdaregistry.info/Elements/u/P60049">
  <rdfs:isDefinedBy rdf:resource="http://rdaregistry.info/Elements/u/" />
  <reg:status rdf:resource="http://metadataregistry.org/uri/RegStatus/1001" />
  <reg:name xml:lang="en">contentType</reg:name>
  <rdfs:label xml:lang="en">has content type</rdfs:label>
  <skos:definition xml:lang="en">Relates a resource to a categorization reflecting a fundamental form of communication in which a content is expressed and a human sense through which it is intended to be perceived.</skos:definition>
  <rdf:type rdf:resource="http://www.w3.org/1999/02/22-rdf-syntax-ns#Property" />
  <reg:hasSubproperty rdf:resource="http://rdaregistry.info/Elements/e/P20001" />
  <reg:lexicalAlias rdf:resource="http://rdaregistry.info/Elements/u/contentType.en" />
  <skos:scopeNote xml:lang="en">Content type also reflects the number of spatial dimensions and the presence or absence of movement in which content expressed in the form of an image or images is intended to be perceived.</skos:scopeNote>
</owl:ObjectProperty>

<!-- Property: is continuation in part of -->
<owl:ObjectProperty rdf:about="http://rdaregistry.info/Elements/u/P60276">
  <rdfs:isDefinedBy rdf:resource="http://rdaregistry.info/Elements/u/" />
  <reg:status rdf:resource="http://metadataregistry.org/uri/RegStatus/1001" />
  <reg:name xml:lang="en">continuationInPartOf</reg:name>
  <rdfs:label xml:lang="en">is continuation in part of</rdfs:label>
  <skos:definition xml:lang="en">Relates a resource to a resource that split into two or more separate resources with new titles.</skos:definition>
  <rdf:type rdf:resource="http://www.w3.org/1999/02/22-rdf-syntax-ns#Property" />
  <rdfs:subPropertyOf rdf:resource="http://rdaregistry.info/Elements/u/P60261" />
  <owl:inverseOf rdf:resource="http://rdaregistry.info/Elements/u/P60503" />
  <reg:hasSubproperty rdf:resource="http://rdaregistry.info/Elements/e/P20167" />
  <reg:lexicalAlias rdf:resource="http://rdaregistry.info/Elements/u/continuationInPartOf.en" />
  <skos:scopeNote xml:lang="en">This relationship applies generally to serials.</skos:scopeNote>
</owl:ObjectProperty>

<!-- Property: is continuation of -->
<owl:ObjectProperty rdf:about="http://rdaregistry.info/Elements/u/P60576">
  <rdfs:isDefinedBy rdf:resource="http://rdaregistry.info/Elements/u/" />
  <reg:status rdf:resource="http://metadataregistry.org/uri/RegStatus/1001" />
  <reg:name xml:lang="en">continuationOf</reg:name>
  <rdfs:label xml:lang="en">is continuation of</rdfs:label>
  <skos:definition xml:lang="en">Relates a resource to a resource that is continued by the content of a later resource.</skos:definition>
  <rdf:type rdf:resource="http://www.w3.org/1999/02/22-rdf-syntax-ns#Property" />
  <rdfs:subPropertyOf rdf:resource="http://rdaregistry.info/Elements/u/P60261" />
  <owl:inverseOf rdf:resource="http://rdaregistry.info/Elements/u/P60306" />
  <reg:hasSubproperty rdf:resource="http://rdaregistry.info/Elements/e/P20149" />
  <reg:lexicalAlias rdf:resource="http://rdaregistry.info/Elements/u/continuationOf.en" />
  <skos:scopeNote xml:lang="en">This relationship applies generally to serials.</skos:scopeNote>
</owl:ObjectProperty>

<!-- Property: is continued by -->
<owl:ObjectProperty rdf:about="http://rdaregistry.info/Elements/u/P60306">
  <rdfs:isDefinedBy rdf:resource="http://rdaregistry.info/Elements/u/" />
  <reg:status rdf:resource="http://metadataregistry.org/uri/RegStatus/1001" />
  <reg:name xml:lang="en">continuedBy</reg:name>
  <rdfs:label xml:lang="en">is continued by</rdfs:label>
  <skos:definition xml:lang="en">Relates a resource to a resource whose content continues an earlier resource under a new title.</skos:definition>
  <rdf:type rdf:resource="http://www.w3.org/1999/02/22-rdf-syntax-ns#Property" />
  <rdfs:subPropertyOf rdf:resource="http://rdaregistry.info/Elements/u/P60278" />
  <owl:inverseOf rdf:resource="http://rdaregistry.info/Elements/u/P60576" />
  <reg:hasSubproperty rdf:resource="http://rdaregistry.info/Elements/e/P20191" />
  <reg:lexicalAlias rdf:resource="http://rdaregistry.info/Elements/u/continuedBy.en" />
  <skos:scopeNote xml:lang="en">This relationship applies generally to serials.</skos:scopeNote>
</owl:ObjectProperty>

<!-- Property: is continued in part by -->
<owl:ObjectProperty rdf:about="http://rdaregistry.info/Elements/u/P60199">
  <rdfs:isDefinedBy rdf:resource="http://rdaregistry.info/Elements/u/" />
  <reg:status rdf:resource="http://metadataregistry.org/uri/RegStatus/1001" />
  <reg:name xml:lang="en">continuedInPartBy</reg:name>
  <rdfs:label xml:lang="en">is continued in part by</rdfs:label>
  <skos:definition xml:lang="en">Relates a resource to a resource part of whose content separated from an earlier resource to form a new resource.</skos:definition>
  <rdf:type rdf:resource="http://www.w3.org/1999/02/22-rdf-syntax-ns#Property" />
  <rdfs:subPropertyOf rdf:resource="http://rdaregistry.info/Elements/u/P60278" />
  <owl:inverseOf rdf:resource="http://rdaregistry.info/Elements/u/P60277" />
  <reg:hasSubproperty rdf:resource="http://rdaregistry.info/Elements/e/P20101" />
  <reg:lexicalAlias rdf:resource="http://rdaregistry.info/Elements/u/continuedInPartBy.en" />
  <skos:scopeNote xml:lang="en">This relationship applies generally to serials.</skos:scopeNote>
</owl:ObjectProperty>

<!-- Property: has contributor -->
<owl:ObjectProperty rdf:about="http://rdaregistry.info/Elements/u/P60398">
  <rdfs:isDefinedBy rdf:resource="http://rdaregistry.info/Elements/u/" />
  <reg:status rdf:resource="http://metadataregistry.org/uri/RegStatus/1001" />
  <reg:name xml:lang="en">contributor</reg:name>
  <rdfs:label xml:lang="en">has contributor</rdfs:label>
  <skos:definition xml:lang="en">Relates a resource to an agent contributing to a resource.</skos:definition>
  <rdf:type rdf:resource="http://www.w3.org/1999/02/22-rdf-syntax-ns#Property" />
  <skos:scopeNote xml:lang="en">Contributors include editors, translators, arrangers of music, performers, etc.</skos:scopeNote>
  <owl:inverseOf rdf:resource="http://rdaregistry.info/Elements/u/P60626" />
  <reg:hasSubproperty rdf:resource="http://rdaregistry.info/Elements/u/P60377" />
  <reg:hasSubproperty rdf:resource="http://rdaregistry.info/Elements/u/P60378" />
  <reg:hasSubproperty rdf:resource="http://rdaregistry.info/Elements/u/P60379" />
  <reg:hasSubproperty rdf:resource="http://rdaregistry.info/Elements/u/P60381" />
  <reg:hasSubproperty rdf:resource="http://rdaregistry.info/Elements/u/P60382" />
  <reg:hasSubproperty rdf:resource="http://rdaregistry.info/Elements/u/P60383" />
  <reg:hasSubproperty rdf:resource="http://rdaregistry.info/Elements/u/P60384" />
  <reg:hasSubproperty rdf:resource="http://rdaregistry.info/Elements/u/P60385" />
  <reg:hasSubproperty rdf:resource="http://rdaregistry.info/Elements/u/P60386" />
  <reg:hasSubproperty rdf:resource="http://rdaregistry.info/Elements/u/P60387" />
  <reg:hasSubproperty rdf:resource="http://rdaregistry.info/Elements/u/P60388" />
  <reg:hasSubproperty rdf:resource="http://rdaregistry.info/Elements/u/P60392" />
  <reg:hasSubproperty rdf:resource="http://rdaregistry.info/Elements/u/P60393" />
  <reg:hasSubproperty rdf:resource="http://rdaregistry.info/Elements/u/P60394" />
  <reg:hasSubproperty rdf:resource="http://rdaregistry.info/Elements/u/P60395" />
  <reg:hasSubproperty rdf:resource="http://rdaregistry.info/Elements/u/P60396" />
  <reg:hasSubproperty rdf:resource="http://rdaregistry.info/Elements/u/P60397" />
  <reg:hasSubproperty rdf:resource="http://rdaregistry.info/Elements/u/P60399" />
  <reg:hasSubproperty rdf:resource="http://rdaregistry.info/Elements/u/P60419" />
  <reg:hasSubproperty rdf:resource="http://rdaregistry.info/Elements/u/P60422" />
  <reg:hasSubproperty rdf:resource="http://rdaregistry.info/Elements/u/P60437" />
  <reg:hasSubproperty rdf:resource="http://rdaregistry.info/Elements/u/P60446" />
  <reg:hasSubproperty rdf:resource="http://rdaregistry.info/Elements/e/P20053" />
  <reg:lexicalAlias rdf:resource="http://rdaregistry.info/Elements/u/contributor.en" />
  <reg:hasSubproperty rdf:resource="http://rdaregistry.info/Elements/u/P60748" />
  <reg:hasSubproperty rdf:resource="http://rdaregistry.info/Elements/u/P60749" />
  <reg:hasSubproperty rdf:resource="http://rdaregistry.info/Elements/u/P60809" />
  <reg:hasSubproperty rdf:resource="http://rdaregistry.info/Elements/u/P60811" />
  <reg:hasSubproperty rdf:resource="http://rdaregistry.info/Elements/u/P60813" />
  <reg:hasSubproperty rdf:resource="http://rdaregistry.info/Elements/u/P60824" />
  <reg:hasSubproperty rdf:resource="http://rdaregistry.info/Elements/u/P60828" />
  <reg:hasSubproperty rdf:resource="http://rdaregistry.info/Elements/u/P60838" />
  <reg:hasSubproperty rdf:resource="http://rdaregistry.info/Elements/u/P60840" />
  <reg:hasSubproperty rdf:resource="http://rdaregistry.info/Elements/u/P60851" />
  <reg:hasSubproperty rdf:resource="http://rdaregistry.info/Elements/u/P60892" />
  <reg:hasSubproperty rdf:resource="http://rdaregistry.info/Elements/u/P60894" />
  <reg:hasSubproperty rdf:resource="http://rdaregistry.info/Elements/u/P60895" />
  <reg:hasSubproperty rdf:resource="http://rdaregistry.info/Elements/u/P60896" />
</owl:ObjectProperty>

<!-- Property: is contributor of -->
<owl:ObjectProperty rdf:about="http://rdaregistry.info/Elements/u/P60626">
  <rdfs:isDefinedBy rdf:resource="http://rdaregistry.info/Elements/u/" />
  <reg:status rdf:resource="http://metadataregistry.org/uri/RegStatus/1001" />
  <reg:name xml:lang="en">contributorOf</reg:name>
  <rdfs:label xml:lang="en">is contributor of</rdfs:label>
  <skos:definition xml:lang="en">Relates an agent contributing to an expression to a resource.</skos:definition>
  <rdf:type rdf:resource="http://www.w3.org/1999/02/22-rdf-syntax-ns#Property" />
  <owl:inverseOf rdf:resource="http://rdaregistry.info/Elements/u/P60398" />
  <reg:hasSubproperty rdf:resource="http://rdaregistry.info/Elements/u/P60605" />
  <reg:hasSubproperty rdf:resource="http://rdaregistry.info/Elements/u/P60606" />
  <reg:hasSubproperty rdf:resource="http://rdaregistry.info/Elements/u/P60607" />
  <reg:hasSubproperty rdf:resource="http://rdaregistry.info/Elements/u/P60609" />
  <reg:hasSubproperty rdf:resource="http://rdaregistry.info/Elements/u/P60610" />
  <reg:hasSubproperty rdf:resource="http://rdaregistry.info/Elements/u/P60611" />
  <reg:hasSubproperty rdf:resource="http://rdaregistry.info/Elements/u/P60612" />
  <reg:hasSubproperty rdf:resource="http://rdaregistry.info/Elements/u/P60613" />
  <reg:hasSubproperty rdf:resource="http://rdaregistry.info/Elements/u/P60614" />
  <reg:hasSubproperty rdf:resource="http://rdaregistry.info/Elements/u/P60615" />
  <reg:hasSubproperty rdf:resource="http://rdaregistry.info/Elements/u/P60616" />
  <reg:hasSubproperty rdf:resource="http://rdaregistry.info/Elements/u/P60620" />
  <reg:hasSubproperty rdf:resource="http://rdaregistry.info/Elements/u/P60621" />
  <reg:hasSubproperty rdf:resource="http://rdaregistry.info/Elements/u/P60622" />
  <reg:hasSubproperty rdf:resource="http://rdaregistry.info/Elements/u/P60623" />
  <reg:hasSubproperty rdf:resource="http://rdaregistry.info/Elements/u/P60624" />
  <reg:hasSubproperty rdf:resource="http://rdaregistry.info/Elements/u/P60625" />
  <reg:hasSubproperty rdf:resource="http://rdaregistry.info/Elements/u/P60627" />
  <reg:hasSubproperty rdf:resource="http://rdaregistry.info/Elements/u/P60647" />
  <reg:hasSubproperty rdf:resource="http://rdaregistry.info/Elements/u/P60651" />
  <reg:hasSubproperty rdf:resource="http://rdaregistry.info/Elements/u/P60666" />
  <reg:hasSubproperty rdf:resource="http://rdaregistry.info/Elements/u/P60671" />
  <reg:hasSubproperty rdf:resource="http://rdaregistry.info/Elements/a/P50161" />
  <reg:lexicalAlias rdf:resource="http://rdaregistry.info/Elements/u/contributorOf.en" />
  <reg:hasSubproperty rdf:resource="http://rdaregistry.info/Elements/u/P60754" />
  <reg:hasSubproperty rdf:resource="http://rdaregistry.info/Elements/u/P60755" />
  <reg:hasSubproperty rdf:resource="http://rdaregistry.info/Elements/u/P60810" />
  <reg:hasSubproperty rdf:resource="http://rdaregistry.info/Elements/u/P60812" />
  <reg:hasSubproperty rdf:resource="http://rdaregistry.info/Elements/u/P60814" />
  <reg:hasSubproperty rdf:resource="http://rdaregistry.info/Elements/u/P60825" />
  <reg:hasSubproperty rdf:resource="http://rdaregistry.info/Elements/u/P60829" />
  <reg:hasSubproperty rdf:resource="http://rdaregistry.info/Elements/u/P60839" />
  <reg:hasSubproperty rdf:resource="http://rdaregistry.info/Elements/u/P60841" />
  <reg:hasSubproperty rdf:resource="http://rdaregistry.info/Elements/u/P60852" />
</owl:ObjectProperty>

<!-- Property: has coordinates of cartographic content -->
<owl:ObjectProperty rdf:about="http://rdaregistry.info/Elements/u/P60109">
  <rdfs:isDefinedBy rdf:resource="http://rdaregistry.info/Elements/u/" />
  <reg:status rdf:resource="http://metadataregistry.org/uri/RegStatus/1001" />
  <reg:name xml:lang="en">coordinatesOfCartographicContent</reg:name>
  <rdfs:label xml:lang="en">has coordinates of cartographic content</rdfs:label>
  <skos:definition xml:lang="en">Relates a resource to a mathematical system for identifying an area covered by the cartographic content of a resource.</skos:definition>
  <rdf:type rdf:resource="http://www.w3.org/1999/02/22-rdf-syntax-ns#Property" />
  <reg:hasSubproperty rdf:resource="http://rdaregistry.info/Elements/u/P60345" />
  <reg:hasSubproperty rdf:resource="http://rdaregistry.info/Elements/u/P60346" />
  <reg:hasSubproperty rdf:resource="http://rdaregistry.info/Elements/u/P60347" />
  <reg:lexicalAlias rdf:resource="http://rdaregistry.info/Elements/u/coordinatesOfCartographicContent.en" />
</owl:ObjectProperty>

<!-- Property: has copyright date -->
<owl:ObjectProperty rdf:about="http://rdaregistry.info/Elements/u/P60069">
  <rdfs:isDefinedBy rdf:resource="http://rdaregistry.info/Elements/u/" />
  <reg:status rdf:resource="http://metadataregistry.org/uri/RegStatus/1001" />
  <reg:name xml:lang="en">copyrightDate</reg:name>
  <rdfs:label xml:lang="en">has copyright date</rdfs:label>
  <skos:definition xml:lang="en">Relates a resource to a date associated with a claim of protection under copyright or a similar regime.</skos:definition>
  <reg:hasSubproperty rdf:resource="http://rdaregistry.info/Elements/m/P30007" />
  <rdf:type rdf:resource="http://www.w3.org/1999/02/22-rdf-syntax-ns#Property" />
  <reg:lexicalAlias rdf:resource="http://rdaregistry.info/Elements/u/copyrightDate.en" />
</owl:ObjectProperty>

<!-- Property: has costume designer -->
<owl:ObjectProperty rdf:about="http://rdaregistry.info/Elements/u/P60384">
  <rdfs:isDefinedBy rdf:resource="http://rdaregistry.info/Elements/u/" />
  <reg:status rdf:resource="http://metadataregistry.org/uri/RegStatus/1001" />
  <reg:name xml:lang="en">costumeDesigner</reg:name>
  <rdfs:label xml:lang="en">has costume designer</rdfs:label>
  <skos:definition xml:lang="en">Relates a resource to an agent contributing to a resource by designing costumes for a moving image production or for a musical or dramatic presentation or entertainment.</skos:definition>
  <rdf:type rdf:resource="http://www.w3.org/1999/02/22-rdf-syntax-ns#Property" />
  <rdfs:subPropertyOf rdf:resource="http://rdaregistry.info/Elements/u/P60398" />
  <owl:inverseOf rdf:resource="http://rdaregistry.info/Elements/u/P60612" />
  <reg:hasSubproperty rdf:resource="http://rdaregistry.info/Elements/e/P20036" />
  <reg:lexicalAlias rdf:resource="http://rdaregistry.info/Elements/u/costumeDesigner.en" />
</owl:ObjectProperty>

<!-- Property: is costume designer of -->
<owl:ObjectProperty rdf:about="http://rdaregistry.info/Elements/u/P60612">
  <rdfs:isDefinedBy rdf:resource="http://rdaregistry.info/Elements/u/" />
  <reg:status rdf:resource="http://metadataregistry.org/uri/RegStatus/1001" />
  <reg:name xml:lang="en">costumeDesignerOf</reg:name>
  <rdfs:label xml:lang="en">is costume designer of</rdfs:label>
  <skos:definition xml:lang="en">Relates an agent contributing to a resource by designing costumes for a moving image production or for a musical or dramatic presentation or entertainment to a resource.</skos:definition>
  <rdf:type rdf:resource="http://www.w3.org/1999/02/22-rdf-syntax-ns#Property" />
  <rdfs:subPropertyOf rdf:resource="http://rdaregistry.info/Elements/u/P60626" />
  <owl:inverseOf rdf:resource="http://rdaregistry.info/Elements/u/P60384" />
  <reg:hasSubproperty rdf:resource="http://rdaregistry.info/Elements/a/P50144" />
  <reg:lexicalAlias rdf:resource="http://rdaregistry.info/Elements/u/costumeDesignerOf.en" />
</owl:ObjectProperty>

<!-- Property: has country associated with agent -->
<owl:ObjectProperty rdf:about="http://rdaregistry.info/Elements/u/P60063">
  <rdfs:isDefinedBy rdf:resource="http://rdaregistry.info/Elements/u/" />
  <reg:status rdf:resource="http://metadataregistry.org/uri/RegStatus/1001" />
  <reg:name xml:lang="en">countryAssociatedWithAgent</reg:name>
  <rdfs:label xml:lang="en">has country associated with agent</rdfs:label>
  <skos:definition xml:lang="en">Relates a resource to a country with which an agent is identified.</skos:definition>
  <reg:hasSubproperty rdf:resource="http://rdaregistry.info/Elements/a/P50097" />
  <rdf:type rdf:resource="http://www.w3.org/1999/02/22-rdf-syntax-ns#Property" />
  <reg:lexicalAlias rdf:resource="http://rdaregistry.info/Elements/u/countryAssociatedWithPerson.en" />
</owl:ObjectProperty>

<!-- Property: has court governed -->
<owl:ObjectProperty rdf:about="http://rdaregistry.info/Elements/u/P60065">
  <rdfs:isDefinedBy rdf:resource="http://rdaregistry.info/Elements/u/" />
  <reg:status rdf:resource="http://metadataregistry.org/uri/RegStatus/1001" />
  <reg:name xml:lang="en">courtGoverned</reg:name>
  <rdfs:label xml:lang="en">has court governed</rdfs:label>
  <skos:definition xml:lang="en">Relates a resource to a court governed by court rules, regardless of their official nature.</skos:definition>
  <rdf:type rdf:resource="http://www.w3.org/1999/02/22-rdf-syntax-ns#Property" />
  <rdfs:subPropertyOf rdf:resource="http://rdaregistry.info/Elements/u/P60374" />
  <owl:inverseOf rdf:resource="http://rdaregistry.info/Elements/u/P60005" />
  <reg:lexicalAlias rdf:resource="http://rdaregistry.info/Elements/u/courtGoverned.en" />
</owl:ObjectProperty>

<!-- Property: is court governed of -->
<owl:ObjectProperty rdf:about="http://rdaregistry.info/Elements/u/P60005">
  <rdfs:isDefinedBy rdf:resource="http://rdaregistry.info/Elements/u/" />
  <reg:status rdf:resource="http://metadataregistry.org/uri/RegStatus/1001" />
  <reg:name xml:lang="en">courtGovernedOf</reg:name>
  <rdfs:label xml:lang="en">is court governed of</rdfs:label>
  <skos:definition xml:lang="en">Relates a court governed by court rules, regardless of their official nature to a resource.</skos:definition>
  <rdf:type rdf:resource="http://www.w3.org/1999/02/22-rdf-syntax-ns#Property" />
  <rdfs:subPropertyOf rdf:resource="http://rdaregistry.info/Elements/u/P60602" />
  <owl:inverseOf rdf:resource="http://rdaregistry.info/Elements/u/P60065" />
  <reg:hasSubproperty rdf:resource="http://rdaregistry.info/Elements/a/P50044" />
  <reg:lexicalAlias rdf:resource="http://rdaregistry.info/Elements/u/courtGovernedOf.en" />
</owl:ObjectProperty>

<!-- Property: has court reporter -->
<owl:ObjectProperty rdf:about="http://rdaregistry.info/Elements/u/P60388">
  <rdfs:isDefinedBy rdf:resource="http://rdaregistry.info/Elements/u/" />
  <reg:status rdf:resource="http://metadataregistry.org/uri/RegStatus/1001" />
  <reg:name xml:lang="en">courtReporter</reg:name>
  <rdfs:label xml:lang="en">has court reporter</rdfs:label>
  <skos:definition xml:lang="en">Relates a resource to an agent contributing to a resource by preparing a court's opinions for publication.</skos:definition>
  <rdf:type rdf:resource="http://www.w3.org/1999/02/22-rdf-syntax-ns#Property" />
  <rdfs:subPropertyOf rdf:resource="http://rdaregistry.info/Elements/u/P60398" />
  <owl:inverseOf rdf:resource="http://rdaregistry.info/Elements/u/P60616" />
  <reg:hasSubproperty rdf:resource="http://rdaregistry.info/Elements/e/P20040" />
  <reg:lexicalAlias rdf:resource="http://rdaregistry.info/Elements/u/courtReporter.en" />
</owl:ObjectProperty>

<!-- Property: is court reporter of -->
<owl:ObjectProperty rdf:about="http://rdaregistry.info/Elements/u/P60616">
  <rdfs:isDefinedBy rdf:resource="http://rdaregistry.info/Elements/u/" />
  <reg:status rdf:resource="http://metadataregistry.org/uri/RegStatus/1001" />
  <reg:name xml:lang="en">courtReporterOf</reg:name>
  <rdfs:label xml:lang="en">is court reporter of</rdfs:label>
  <skos:definition xml:lang="en">Relates an agent contributing to a resource by preparing a court's opinions for publication to a resource.</skos:definition>
  <rdf:type rdf:resource="http://www.w3.org/1999/02/22-rdf-syntax-ns#Property" />
  <rdfs:subPropertyOf rdf:resource="http://rdaregistry.info/Elements/u/P60626" />
  <owl:inverseOf rdf:resource="http://rdaregistry.info/Elements/u/P60388" />
  <reg:hasSubproperty rdf:resource="http://rdaregistry.info/Elements/a/P50148" />
  <reg:lexicalAlias rdf:resource="http://rdaregistry.info/Elements/u/courtReporterOf.en" />
</owl:ObjectProperty>

<!-- Property: has coverage of content -->
<owl:ObjectProperty rdf:about="http://rdaregistry.info/Elements/u/P60518">
  <rdfs:isDefinedBy rdf:resource="http://rdaregistry.info/Elements/u/" />
  <reg:status rdf:resource="http://metadataregistry.org/uri/RegStatus/1001" />
  <reg:name xml:lang="en">coverageOfContent</reg:name>
  <rdfs:label xml:lang="en">has coverage of content</rdfs:label>
  <skos:definition xml:lang="en">Relates a resource to a chronological or geographic coverage of the content of a resource.</skos:definition>
  <rdf:type rdf:resource="http://www.w3.org/1999/02/22-rdf-syntax-ns#Property" />
  <reg:lexicalAlias rdf:resource="http://rdaregistry.info/Elements/u/coverageOfContent.en" />
</owl:ObjectProperty>

<!-- Property: has co-worker -->
<owl:ObjectProperty rdf:about="http://rdaregistry.info/Elements/u/P60859">
  <rdfs:isDefinedBy rdf:resource="http://rdaregistry.info/Elements/u/" />
  <reg:status rdf:resource="http://metadataregistry.org/uri/RegStatus/1001" />
  <rdf:type rdf:resource="http://www.w3.org/1999/02/22-rdf-syntax-ns#Property" />
  <reg:name xml:lang="en">coworker</reg:name>
  <rdfs:label xml:lang="en">has co-worker</rdfs:label>
  <reg:lexicalAlias rdf:resource="http://rdaregistry.info/Elements/u/coworker.en" />
  <skos:definition xml:lang="en">Relates an agent to a colleague who works with or shares a task with another agent.</skos:definition>
  <owl:inverseOf rdf:resource="http://rdaregistry.info/Elements/u/P60859" />
  <reg:hasSubproperty rdf:resource="http://rdaregistry.info/Elements/a/P50277" />
  <rdfs:subPropertyOf rdf:resource="http://rdaregistry.info/Elements/u/P60853" />
</owl:ObjectProperty>

<!-- Property: has creator -->
<owl:ObjectProperty rdf:about="http://rdaregistry.info/Elements/u/P60447">
  <rdfs:isDefinedBy rdf:resource="http://rdaregistry.info/Elements/u/" />
  <reg:status rdf:resource="http://metadataregistry.org/uri/RegStatus/1001" />
  <reg:name xml:lang="en">creator</reg:name>
  <rdfs:label xml:lang="en">has creator</rdfs:label>
  <skos:definition xml:lang="en">Relates a resource to an agent responsible for the creation of a resource</skos:definition>
  <rdf:type rdf:resource="http://www.w3.org/1999/02/22-rdf-syntax-ns#Property" />
  <owl:inverseOf rdf:resource="http://rdaregistry.info/Elements/u/P60672" />
  <reg:hasSubproperty rdf:resource="http://rdaregistry.info/Elements/u/P60045" />
  <reg:hasSubproperty rdf:resource="http://rdaregistry.info/Elements/u/P60096" />
  <reg:hasSubproperty rdf:resource="http://rdaregistry.info/Elements/u/P60420" />
  <reg:hasSubproperty rdf:resource="http://rdaregistry.info/Elements/u/P60423" />
  <reg:hasSubproperty rdf:resource="http://rdaregistry.info/Elements/u/P60424" />
  <reg:hasSubproperty rdf:resource="http://rdaregistry.info/Elements/u/P60425" />
  <reg:hasSubproperty rdf:resource="http://rdaregistry.info/Elements/u/P60426" />
  <reg:hasSubproperty rdf:resource="http://rdaregistry.info/Elements/u/P60427" />
  <reg:hasSubproperty rdf:resource="http://rdaregistry.info/Elements/u/P60428" />
  <reg:hasSubproperty rdf:resource="http://rdaregistry.info/Elements/u/P60429" />
  <reg:hasSubproperty rdf:resource="http://rdaregistry.info/Elements/u/P60430" />
  <reg:hasSubproperty rdf:resource="http://rdaregistry.info/Elements/u/P60431" />
  <reg:hasSubproperty rdf:resource="http://rdaregistry.info/Elements/u/P60432" />
  <reg:hasSubproperty rdf:resource="http://rdaregistry.info/Elements/u/P60433" />
  <reg:hasSubproperty rdf:resource="http://rdaregistry.info/Elements/u/P60434" />
  <reg:hasSubproperty rdf:resource="http://rdaregistry.info/Elements/u/P60435" />
  <reg:hasSubproperty rdf:resource="http://rdaregistry.info/Elements/u/P60436" />
  <reg:hasSubproperty rdf:resource="http://rdaregistry.info/Elements/u/P60463" />
  <reg:hasSubproperty rdf:resource="http://rdaregistry.info/Elements/u/P60465" />
  <reg:lexicalAlias rdf:resource="http://rdaregistry.info/Elements/u/creator.en" />
  <reg:hasSubproperty rdf:resource="http://rdaregistry.info/Elements/u/P60826" />
  <reg:hasSubproperty rdf:resource="http://rdaregistry.info/Elements/u/P60891" />
  <skos:scopeNote xml:lang="en">Creators include agents who are jointly responsible for the creation of a resource either performing the same role, such as in a collaboration between two writers, or performing different roles, such as in a collaboration between a composer and a lyricist.</skos:scopeNote>
</owl:ObjectProperty>

<!-- Property: is creator of -->
<owl:ObjectProperty rdf:about="http://rdaregistry.info/Elements/u/P60672">
  <rdfs:isDefinedBy rdf:resource="http://rdaregistry.info/Elements/u/" />
  <reg:status rdf:resource="http://metadataregistry.org/uri/RegStatus/1001" />
  <reg:name xml:lang="en">creatorOf</reg:name>
  <rdfs:label xml:lang="en">is creator of</rdfs:label>
  <skos:definition xml:lang="en">Relates an agent responsible for the creation of a resource to a resource.</skos:definition>
  <rdf:type rdf:resource="http://www.w3.org/1999/02/22-rdf-syntax-ns#Property" />
  <owl:inverseOf rdf:resource="http://rdaregistry.info/Elements/u/P60447" />
  <reg:hasSubproperty rdf:resource="http://rdaregistry.info/Elements/u/P60001" />
  <reg:hasSubproperty rdf:resource="http://rdaregistry.info/Elements/u/P60014" />
  <reg:hasSubproperty rdf:resource="http://rdaregistry.info/Elements/u/P60649" />
  <reg:hasSubproperty rdf:resource="http://rdaregistry.info/Elements/u/P60652" />
  <reg:hasSubproperty rdf:resource="http://rdaregistry.info/Elements/u/P60653" />
  <reg:hasSubproperty rdf:resource="http://rdaregistry.info/Elements/u/P60654" />
  <reg:hasSubproperty rdf:resource="http://rdaregistry.info/Elements/u/P60655" />
  <reg:hasSubproperty rdf:resource="http://rdaregistry.info/Elements/u/P60656" />
  <reg:hasSubproperty rdf:resource="http://rdaregistry.info/Elements/u/P60657" />
  <reg:hasSubproperty rdf:resource="http://rdaregistry.info/Elements/u/P60658" />
  <reg:hasSubproperty rdf:resource="http://rdaregistry.info/Elements/u/P60659" />
  <reg:hasSubproperty rdf:resource="http://rdaregistry.info/Elements/u/P60660" />
  <reg:hasSubproperty rdf:resource="http://rdaregistry.info/Elements/u/P60661" />
  <reg:hasSubproperty rdf:resource="http://rdaregistry.info/Elements/u/P60662" />
  <reg:hasSubproperty rdf:resource="http://rdaregistry.info/Elements/u/P60663" />
  <reg:hasSubproperty rdf:resource="http://rdaregistry.info/Elements/u/P60664" />
  <reg:hasSubproperty rdf:resource="http://rdaregistry.info/Elements/u/P60665" />
  <reg:hasSubproperty rdf:resource="http://rdaregistry.info/Elements/u/P60699" />
  <reg:hasSubproperty rdf:resource="http://rdaregistry.info/Elements/u/P60701" />
  <reg:hasSubproperty rdf:resource="http://rdaregistry.info/Elements/a/P50204" />
  <reg:lexicalAlias rdf:resource="http://rdaregistry.info/Elements/u/creatorOf.en" />
  <reg:hasSubproperty rdf:resource="http://rdaregistry.info/Elements/u/P60827" />
  <reg:hasSubproperty rdf:resource="http://rdaregistry.info/Elements/u/P60881" />
  <reg:hasSubproperty rdf:resource="http://rdaregistry.info/Elements/u/P60882" />
</owl:ObjectProperty>

<!-- Property: is critiqued in -->
<owl:ObjectProperty rdf:about="http://rdaregistry.info/Elements/u/P60212">
  <rdfs:isDefinedBy rdf:resource="http://rdaregistry.info/Elements/u/" />
  <reg:status rdf:resource="http://metadataregistry.org/uri/RegStatus/1001" />
  <reg:name xml:lang="en">critiquedIn</reg:name>
  <rdfs:label xml:lang="en">is critiqued in</rdfs:label>
  <skos:definition xml:lang="en">Relates a resource to a resource that contains a critical evaluation of a described resource.</skos:definition>
  <rdf:type rdf:resource="http://www.w3.org/1999/02/22-rdf-syntax-ns#Property" />
  <rdfs:subPropertyOf rdf:resource="http://rdaregistry.info/Elements/u/P60215" />
  <owl:inverseOf rdf:resource="http://rdaregistry.info/Elements/u/P60292" />
  <reg:hasSubproperty rdf:resource="http://rdaregistry.info/Elements/e/P20272" />
  <reg:hasSubproperty rdf:resource="http://rdaregistry.info/Elements/i/P40065" />
  <reg:hasSubproperty rdf:resource="http://rdaregistry.info/Elements/m/P30257" />
  <reg:lexicalAlias rdf:resource="http://rdaregistry.info/Elements/u/critiquedIn.en" />
</owl:ObjectProperty>

<!-- Property: is critique of -->
<owl:ObjectProperty rdf:about="http://rdaregistry.info/Elements/u/P60292">
  <rdfs:isDefinedBy rdf:resource="http://rdaregistry.info/Elements/u/" />
  <reg:status rdf:resource="http://metadataregistry.org/uri/RegStatus/1001" />
  <reg:name xml:lang="en">critiqueOf</reg:name>
  <rdfs:label xml:lang="en">is critique of</rdfs:label>
  <skos:definition xml:lang="en">Relates a resource to a resource used as a basis for a critical evaluation.</skos:definition>
  <rdf:type rdf:resource="http://www.w3.org/1999/02/22-rdf-syntax-ns#Property" />
  <rdfs:subPropertyOf rdf:resource="http://rdaregistry.info/Elements/u/P60190" />
  <owl:inverseOf rdf:resource="http://rdaregistry.info/Elements/u/P60212" />
  <reg:hasSubproperty rdf:resource="http://rdaregistry.info/Elements/w/P10269" />
  <reg:hasSubproperty rdf:resource="http://rdaregistry.info/Elements/w/P10275" />
  <reg:hasSubproperty rdf:resource="http://rdaregistry.info/Elements/w/P10281" />
  <reg:lexicalAlias rdf:resource="http://rdaregistry.info/Elements/u/critiqueOf.en" />
</owl:ObjectProperty>

<!-- Property: has curator -->
<owl:ObjectProperty rdf:about="http://rdaregistry.info/Elements/u/P60376">
  <rdfs:isDefinedBy rdf:resource="http://rdaregistry.info/Elements/u/" />
  <reg:status rdf:resource="http://metadataregistry.org/uri/RegStatus/1001" />
  <reg:name xml:lang="en">curator</reg:name>
  <rdfs:label xml:lang="en">has curator</rdfs:label>
  <skos:definition xml:lang="en">Relates a resource to an agent conceiving, aggregating, or organizing an exhibition, collection, or other resource.</skos:definition>
  <rdf:type rdf:resource="http://www.w3.org/1999/02/22-rdf-syntax-ns#Property" />
  <rdfs:subPropertyOf rdf:resource="http://rdaregistry.info/Elements/u/P60374" />
  <owl:inverseOf rdf:resource="http://rdaregistry.info/Elements/u/P60604" />
  <reg:hasSubproperty rdf:resource="http://rdaregistry.info/Elements/u/P60066" />
  <reg:hasSubproperty rdf:resource="http://rdaregistry.info/Elements/u/P60067" />
  <reg:hasSubproperty rdf:resource="http://rdaregistry.info/Elements/i/P40017" />
  <reg:lexicalAlias rdf:resource="http://rdaregistry.info/Elements/u/curator.en" />
</owl:ObjectProperty>

<!-- Property: is curator of -->
<owl:ObjectProperty rdf:about="http://rdaregistry.info/Elements/u/P60604">
  <rdfs:isDefinedBy rdf:resource="http://rdaregistry.info/Elements/u/" />
  <reg:status rdf:resource="http://metadataregistry.org/uri/RegStatus/1001" />
  <reg:name xml:lang="en">curatorOf</reg:name>
  <rdfs:label xml:lang="en">is curator of</rdfs:label>
  <skos:definition xml:lang="en">Relates an agent conceiving, aggregating, or organizing an exhibition, collection, or other resource to a resource.</skos:definition>
  <rdf:type rdf:resource="http://www.w3.org/1999/02/22-rdf-syntax-ns#Property" />
  <rdfs:subPropertyOf rdf:resource="http://rdaregistry.info/Elements/u/P60602" />
  <owl:inverseOf rdf:resource="http://rdaregistry.info/Elements/u/P60376" />
  <reg:hasSubproperty rdf:resource="http://rdaregistry.info/Elements/u/P60006" />
  <reg:hasSubproperty rdf:resource="http://rdaregistry.info/Elements/u/P60007" />
  <reg:hasSubproperty rdf:resource="http://rdaregistry.info/Elements/a/P50133" />
  <reg:lexicalAlias rdf:resource="http://rdaregistry.info/Elements/u/curatorOf.en" />
</owl:ObjectProperty>

<!-- Property: has current owner -->
<owl:ObjectProperty rdf:about="http://rdaregistry.info/Elements/u/P60400">
  <rdfs:isDefinedBy rdf:resource="http://rdaregistry.info/Elements/u/" />
  <reg:status rdf:resource="http://metadataregistry.org/uri/RegStatus/1001" />
  <reg:name xml:lang="en">currentOwner</reg:name>
  <rdfs:label xml:lang="en">has current owner</rdfs:label>
  <skos:definition xml:lang="en">Relates a resource to an agent currently having legal possession of a resource.</skos:definition>
  <rdf:type rdf:resource="http://www.w3.org/1999/02/22-rdf-syntax-ns#Property" />
  <rdfs:subPropertyOf rdf:resource="http://rdaregistry.info/Elements/u/P60404" />
  <owl:inverseOf rdf:resource="http://rdaregistry.info/Elements/u/P60628" />
  <reg:hasSubproperty rdf:resource="http://rdaregistry.info/Elements/u/P60068" />
  <reg:hasSubproperty rdf:resource="http://rdaregistry.info/Elements/i/P40018" />
  <reg:lexicalAlias rdf:resource="http://rdaregistry.info/Elements/u/currentOwner.en" />
</owl:ObjectProperty>

<!-- Property: is current owner of -->
<owl:ObjectProperty rdf:about="http://rdaregistry.info/Elements/u/P60628">
  <rdfs:isDefinedBy rdf:resource="http://rdaregistry.info/Elements/u/" />
  <reg:status rdf:resource="http://metadataregistry.org/uri/RegStatus/1001" />
  <reg:name xml:lang="en">currentOwnerOf</reg:name>
  <rdfs:label xml:lang="en">is current owner of</rdfs:label>
  <skos:definition xml:lang="en">Relates an agent currently having legal possession of a resource to a resource.</skos:definition>
  <rdf:type rdf:resource="http://www.w3.org/1999/02/22-rdf-syntax-ns#Property" />
  <rdfs:subPropertyOf rdf:resource="http://rdaregistry.info/Elements/u/P60632" />
  <owl:inverseOf rdf:resource="http://rdaregistry.info/Elements/u/P60400" />
  <reg:hasSubproperty rdf:resource="http://rdaregistry.info/Elements/u/P60008" />
  <reg:hasSubproperty rdf:resource="http://rdaregistry.info/Elements/a/P50162" />
  <reg:lexicalAlias rdf:resource="http://rdaregistry.info/Elements/u/currentOwnerOf.en" />
</owl:ObjectProperty>

<!-- Property: has custodial history of resource -->
<owl:ObjectProperty rdf:about="http://rdaregistry.info/Elements/u/P60176">
  <rdfs:isDefinedBy rdf:resource="http://rdaregistry.info/Elements/u/" />
  <reg:status rdf:resource="http://metadataregistry.org/uri/RegStatus/1001" />
  <reg:name xml:lang="en">custodialHistoryOfResource</reg:name>
  <rdfs:label xml:lang="en">has custodial history of resource</rdfs:label>
  <skos:definition xml:lang="en">Relates a resource to a record of previous ownership or custodianship of a resource.</skos:definition>
  <rdf:type rdf:resource="http://www.w3.org/1999/02/22-rdf-syntax-ns#Property" />
  <reg:hasSubproperty rdf:resource="http://rdaregistry.info/Elements/i/P40026" />
  <reg:lexicalAlias rdf:resource="http://rdaregistry.info/Elements/u/custodialHistoryOfResource.en" />
</owl:ObjectProperty>

<!-- Property: has custodian -->
<owl:ObjectProperty rdf:about="http://rdaregistry.info/Elements/u/P60402">
  <rdfs:isDefinedBy rdf:resource="http://rdaregistry.info/Elements/u/" />
  <reg:status rdf:resource="http://metadataregistry.org/uri/RegStatus/1001" />
  <reg:name xml:lang="en">custodian</reg:name>
  <rdfs:label xml:lang="en">has custodian</rdfs:label>
  <skos:definition xml:lang="en">Relates a resource to an agent having legal custody of a resource.</skos:definition>
  <rdf:type rdf:resource="http://www.w3.org/1999/02/22-rdf-syntax-ns#Property" />
  <owl:inverseOf rdf:resource="http://rdaregistry.info/Elements/u/P60631" />
  <reg:hasSubproperty rdf:resource="http://rdaregistry.info/Elements/i/P40020" />
  <reg:lexicalAlias rdf:resource="http://rdaregistry.info/Elements/u/custodian.en" />
</owl:ObjectProperty>

<!-- Property: is custodian of -->
<owl:ObjectProperty rdf:about="http://rdaregistry.info/Elements/u/P60631">
  <rdfs:isDefinedBy rdf:resource="http://rdaregistry.info/Elements/u/" />
  <reg:status rdf:resource="http://metadataregistry.org/uri/RegStatus/1001" />
  <reg:name xml:lang="en">custodianOf</reg:name>
  <rdfs:label xml:lang="en">is custodian of</rdfs:label>
  <skos:definition xml:lang="en">Relates an agent having legal custody of a resource to a resource.</skos:definition>
  <rdf:type rdf:resource="http://www.w3.org/1999/02/22-rdf-syntax-ns#Property" />
  <owl:inverseOf rdf:resource="http://rdaregistry.info/Elements/u/P60402" />
  <reg:hasSubproperty rdf:resource="http://rdaregistry.info/Elements/a/P50164" />
  <reg:lexicalAlias rdf:resource="http://rdaregistry.info/Elements/u/custodianOf.en" />
</owl:ObjectProperty>

<!-- Property: has dancer -->
<owl:ObjectProperty rdf:about="http://rdaregistry.info/Elements/u/P60144">
  <rdfs:isDefinedBy rdf:resource="http://rdaregistry.info/Elements/u/" />
  <reg:status rdf:resource="http://metadataregistry.org/uri/RegStatus/1001" />
  <reg:name xml:lang="en">dancer</reg:name>
  <rdfs:label xml:lang="en">has dancer</rdfs:label>
  <skos:definition xml:lang="en">Relates a resource to a performer contributing to a resource by dancing in a musical, dramatic, etc., presentation.</skos:definition>
  <rdf:type rdf:resource="http://www.w3.org/1999/02/22-rdf-syntax-ns#Property" />
  <rdfs:subPropertyOf rdf:resource="http://rdaregistry.info/Elements/u/P60387" />
  <owl:inverseOf rdf:resource="http://rdaregistry.info/Elements/u/P60019" />
  <reg:hasSubproperty rdf:resource="http://rdaregistry.info/Elements/e/P20014" />
  <reg:lexicalAlias rdf:resource="http://rdaregistry.info/Elements/u/dancer.en" />
</owl:ObjectProperty>

<!-- Property: is dancer of -->
<owl:ObjectProperty rdf:about="http://rdaregistry.info/Elements/u/P60019">
  <rdfs:isDefinedBy rdf:resource="http://rdaregistry.info/Elements/u/" />
  <reg:status rdf:resource="http://metadataregistry.org/uri/RegStatus/1001" />
  <reg:name xml:lang="en">dancerOf</reg:name>
  <rdfs:label xml:lang="en">is dancer of</rdfs:label>
  <skos:definition xml:lang="en">Relates a performer contributing to a resource by dancing in a musical, dramatic, etc., presentation to a resource.</skos:definition>
  <rdf:type rdf:resource="http://www.w3.org/1999/02/22-rdf-syntax-ns#Property" />
  <rdfs:subPropertyOf rdf:resource="http://rdaregistry.info/Elements/u/P60615" />
  <owl:inverseOf rdf:resource="http://rdaregistry.info/Elements/u/P60144" />
  <reg:hasSubproperty rdf:resource="http://rdaregistry.info/Elements/a/P50073" />
  <reg:lexicalAlias rdf:resource="http://rdaregistry.info/Elements/u/dancerOf.en" />
</owl:ObjectProperty>

<!-- Property: has date associated with agent -->
<owl:ObjectProperty rdf:about="http://rdaregistry.info/Elements/u/P60324">
  <rdfs:isDefinedBy rdf:resource="http://rdaregistry.info/Elements/u/" />
  <reg:status rdf:resource="http://metadataregistry.org/uri/RegStatus/1001" />
  <reg:name xml:lang="en">dateAssociatedWithAgent</reg:name>
  <rdfs:label xml:lang="en">has date associated with agent</rdfs:label>
  <skos:definition xml:lang="en">Relates a resource to a significant date associated with the history of an agent, or the date or range of dates on which a conference, etc., was held, or a date with which an agent is otherwise associated.</skos:definition>
  <rdf:type rdf:resource="http://www.w3.org/1999/02/22-rdf-syntax-ns#Property" />
  <reg:hasSubproperty rdf:resource="http://rdaregistry.info/Elements/u/P60076" />
  <reg:hasSubproperty rdf:resource="http://rdaregistry.info/Elements/u/P60524" />
  <reg:hasSubproperty rdf:resource="http://rdaregistry.info/Elements/u/P60525" />
  <reg:hasSubproperty rdf:resource="http://rdaregistry.info/Elements/u/P60526" />
  <reg:hasSubproperty rdf:resource="http://rdaregistry.info/Elements/u/P60598" />
  <reg:hasSubproperty rdf:resource="http://rdaregistry.info/Elements/u/P60599" />
  <reg:hasSubproperty rdf:resource="http://rdaregistry.info/Elements/a/P50040" />
  <reg:hasSubproperty rdf:resource="http://rdaregistry.info/Elements/a/P50058" />
  <reg:hasSubproperty rdf:resource="http://rdaregistry.info/Elements/a/P50107" />
  <reg:lexicalAlias rdf:resource="http://rdaregistry.info/Elements/u/dateAssociatedWithAgent.en" />
</owl:ObjectProperty>

<!-- Property: has date of birth -->
<owl:ObjectProperty rdf:about="http://rdaregistry.info/Elements/u/P60599">
  <rdfs:isDefinedBy rdf:resource="http://rdaregistry.info/Elements/u/" />
  <reg:status rdf:resource="http://metadataregistry.org/uri/RegStatus/1001" />
  <reg:name xml:lang="en">dateOfBirth</reg:name>
  <rdfs:label xml:lang="en">has date of birth</rdfs:label>
  <skos:definition xml:lang="en">Relates a resource to a year an agent was born.</skos:definition>
  <rdf:type rdf:resource="http://www.w3.org/1999/02/22-rdf-syntax-ns#Property" />
  <rdfs:subPropertyOf rdf:resource="http://rdaregistry.info/Elements/u/P60324" />
  <reg:hasSubproperty rdf:resource="http://rdaregistry.info/Elements/a/P50121" />
  <reg:lexicalAlias rdf:resource="http://rdaregistry.info/Elements/u/dateOfBirth.en" />
</owl:ObjectProperty>

<!-- Property: has date of capture -->
<owl:ObjectProperty rdf:about="http://rdaregistry.info/Elements/u/P60074">
  <rdfs:isDefinedBy rdf:resource="http://rdaregistry.info/Elements/u/" />
  <reg:status rdf:resource="http://metadataregistry.org/uri/RegStatus/1001" />
  <reg:name xml:lang="en">dateOfCapture</reg:name>
  <rdfs:label xml:lang="en">has date of capture</rdfs:label>
  <skos:definition xml:lang="en">Relates a resource to a date or range of dates associated with the capture (i.e., recording, filming, etc.) of the content of a resource.</skos:definition>
  <rdf:type rdf:resource="http://www.w3.org/1999/02/22-rdf-syntax-ns#Property" />
  <reg:hasSubproperty rdf:resource="http://rdaregistry.info/Elements/e/P20004" />
  <reg:lexicalAlias rdf:resource="http://rdaregistry.info/Elements/u/dateOfCapture.en" />
</owl:ObjectProperty>

<!-- Property: has date of conference, etc. -->
<owl:ObjectProperty rdf:about="http://rdaregistry.info/Elements/u/P60526">
  <rdfs:isDefinedBy rdf:resource="http://rdaregistry.info/Elements/u/" />
  <reg:status rdf:resource="http://metadataregistry.org/uri/RegStatus/1001" />
  <reg:name xml:lang="en">dateOfConferenceEtc</reg:name>
  <rdfs:label xml:lang="en">has date of conference, etc.</rdfs:label>
  <skos:definition xml:lang="en">Relates a resource to a date or range of dates on which a conference, congress, meeting, exhibition, fair, festival, etc., was held.</skos:definition>
  <rdf:type rdf:resource="http://www.w3.org/1999/02/22-rdf-syntax-ns#Property" />
  <rdfs:subPropertyOf rdf:resource="http://rdaregistry.info/Elements/u/P60324" />
  <reg:hasSubproperty rdf:resource="http://rdaregistry.info/Elements/a/P50039" />
  <reg:lexicalAlias rdf:resource="http://rdaregistry.info/Elements/u/dateOfConferenceEtc.en" />
</owl:ObjectProperty>

<!-- Property: has date of death -->
<owl:ObjectProperty rdf:about="http://rdaregistry.info/Elements/u/P60598">
  <rdfs:isDefinedBy rdf:resource="http://rdaregistry.info/Elements/u/" />
  <reg:status rdf:resource="http://metadataregistry.org/uri/RegStatus/1001" />
  <reg:name xml:lang="en">dateOfDeath</reg:name>
  <rdfs:label xml:lang="en">has date of death</rdfs:label>
  <skos:definition xml:lang="en">Relates a resource to a year an agent died.</skos:definition>
  <rdf:type rdf:resource="http://www.w3.org/1999/02/22-rdf-syntax-ns#Property" />
  <rdfs:subPropertyOf rdf:resource="http://rdaregistry.info/Elements/u/P60324" />
  <reg:hasSubproperty rdf:resource="http://rdaregistry.info/Elements/a/P50120" />
  <reg:lexicalAlias rdf:resource="http://rdaregistry.info/Elements/u/dateOfDeath.en" />
</owl:ObjectProperty>

<!-- Property: has date of distribution -->
<owl:ObjectProperty rdf:about="http://rdaregistry.info/Elements/u/P60070">
  <rdfs:isDefinedBy rdf:resource="http://rdaregistry.info/Elements/u/" />
  <reg:status rdf:resource="http://metadataregistry.org/uri/RegStatus/1001" />
  <reg:name xml:lang="en">dateOfDistribution</reg:name>
  <rdfs:label xml:lang="en">has date of distribution</rdfs:label>
  <skos:definition xml:lang="en">Relates a resource to a date associated with the distribution of a resource in a published form.</skos:definition>
  <rdf:type rdf:resource="http://www.w3.org/1999/02/22-rdf-syntax-ns#Property" />
  <reg:hasSubproperty rdf:resource="http://rdaregistry.info/Elements/m/P30008" />
  <reg:lexicalAlias rdf:resource="http://rdaregistry.info/Elements/u/dateOfDistribution.en" />
</owl:ObjectProperty>

<!-- Property: has date of establishment -->
<owl:ObjectProperty rdf:about="http://rdaregistry.info/Elements/u/P60524">
  <rdfs:isDefinedBy rdf:resource="http://rdaregistry.info/Elements/u/" />
  <reg:status rdf:resource="http://metadataregistry.org/uri/RegStatus/1001" />
  <reg:name xml:lang="en">dateOfEstablishment</reg:name>
  <rdfs:label xml:lang="en">has date of establishment</rdfs:label>
  <skos:definition xml:lang="en">Relates a resource to a date on which an agent was established or founded.</skos:definition>
  <rdf:type rdf:resource="http://www.w3.org/1999/02/22-rdf-syntax-ns#Property" />
  <rdfs:subPropertyOf rdf:resource="http://rdaregistry.info/Elements/u/P60324" />
  <reg:hasSubproperty rdf:resource="http://rdaregistry.info/Elements/a/P50037" />
  <reg:lexicalAlias rdf:resource="http://rdaregistry.info/Elements/u/dateOfEstablishment.en" />
</owl:ObjectProperty>

<!-- Property: has date of manufacture -->
<owl:ObjectProperty rdf:about="http://rdaregistry.info/Elements/u/P60072">
  <rdfs:isDefinedBy rdf:resource="http://rdaregistry.info/Elements/u/" />
  <reg:status rdf:resource="http://metadataregistry.org/uri/RegStatus/1001" />
  <reg:name xml:lang="en">dateOfManufacture</reg:name>
  <rdfs:label xml:lang="en">has date of manufacture</rdfs:label>
  <skos:definition xml:lang="en">Relates a resource to a date associated with the printing, duplicating, casting, etc., of a resource in a published form.</skos:definition>
  <rdf:type rdf:resource="http://www.w3.org/1999/02/22-rdf-syntax-ns#Property" />
  <reg:hasSubproperty rdf:resource="http://rdaregistry.info/Elements/m/P30010" />
  <reg:lexicalAlias rdf:resource="http://rdaregistry.info/Elements/u/dateOfManufacture.en" />
</owl:ObjectProperty>

<!-- Property: has date of production -->
<owl:ObjectProperty rdf:about="http://rdaregistry.info/Elements/u/P60071">
  <rdfs:isDefinedBy rdf:resource="http://rdaregistry.info/Elements/u/" />
  <reg:status rdf:resource="http://metadataregistry.org/uri/RegStatus/1001" />
  <reg:name xml:lang="en">dateOfProduction</reg:name>
  <rdfs:label xml:lang="en">has date of production</rdfs:label>
  <skos:definition xml:lang="en">Relates a resource to a date associated with the inscription, fabrication, construction, etc., of a resource in an unpublished form.</skos:definition>
  <rdf:type rdf:resource="http://www.w3.org/1999/02/22-rdf-syntax-ns#Property" />
  <reg:hasSubproperty rdf:resource="http://rdaregistry.info/Elements/m/P30009" />
  <reg:lexicalAlias rdf:resource="http://rdaregistry.info/Elements/u/dateOfProduction.en" />
</owl:ObjectProperty>

<!-- Property: has date of publication -->
<owl:ObjectProperty rdf:about="http://rdaregistry.info/Elements/u/P60073">
  <rdfs:isDefinedBy rdf:resource="http://rdaregistry.info/Elements/u/" />
  <reg:status rdf:resource="http://metadataregistry.org/uri/RegStatus/1001" />
  <reg:name xml:lang="en">dateOfPublication</reg:name>
  <rdfs:label xml:lang="en">has date of publication</rdfs:label>
  <skos:definition xml:lang="en">Relates a resource to a date associated with the publication, release, or issuing of a resource.</skos:definition>
  <rdf:type rdf:resource="http://www.w3.org/1999/02/22-rdf-syntax-ns#Property" />
  <reg:hasSubproperty rdf:resource="http://rdaregistry.info/Elements/m/P30011" />
  <reg:lexicalAlias rdf:resource="http://rdaregistry.info/Elements/u/dateOfPublication.en" />
</owl:ObjectProperty>

<!-- Property: has date of resource -->
<owl:ObjectProperty rdf:about="http://rdaregistry.info/Elements/u/P60527">
  <rdfs:isDefinedBy rdf:resource="http://rdaregistry.info/Elements/u/" />
  <reg:status rdf:resource="http://metadataregistry.org/uri/RegStatus/1001" />
  <reg:name xml:lang="en">dateOfResource</reg:name>
  <rdfs:label xml:lang="en">has date of resource</rdfs:label>
  <skos:definition xml:lang="en">Relates a resource to an earliest date associated with a resource.</skos:definition>
  <rdf:type rdf:resource="http://www.w3.org/1999/02/22-rdf-syntax-ns#Property" />
  <reg:hasSubproperty rdf:resource="http://rdaregistry.info/Elements/e/P20214" />
  <reg:lexicalAlias rdf:resource="http://rdaregistry.info/Elements/u/dateOfResource.en" />
</owl:ObjectProperty>

<!-- Property: has date of termination -->
<owl:ObjectProperty rdf:about="http://rdaregistry.info/Elements/u/P60525">
  <rdfs:isDefinedBy rdf:resource="http://rdaregistry.info/Elements/u/" />
  <reg:status rdf:resource="http://metadataregistry.org/uri/RegStatus/1001" />
  <reg:name xml:lang="en">dateOfTermination</reg:name>
  <rdfs:label xml:lang="en">has date of termination</rdfs:label>
  <skos:definition xml:lang="en">Relates a resource to a date on which an agent was terminated or dissolved.</skos:definition>
  <rdf:type rdf:resource="http://www.w3.org/1999/02/22-rdf-syntax-ns#Property" />
  <rdfs:subPropertyOf rdf:resource="http://rdaregistry.info/Elements/u/P60324" />
  <reg:hasSubproperty rdf:resource="http://rdaregistry.info/Elements/a/P50038" />
  <reg:lexicalAlias rdf:resource="http://rdaregistry.info/Elements/u/dateOfTermination.en" />
</owl:ObjectProperty>

<!-- Property: has date of usage -->
<owl:ObjectProperty rdf:about="http://rdaregistry.info/Elements/u/P60075">
  <rdfs:isDefinedBy rdf:resource="http://rdaregistry.info/Elements/u/" />
  <reg:status rdf:resource="http://metadataregistry.org/uri/RegStatus/1001" />
  <reg:name xml:lang="en">dateOfUsage</reg:name>
  <rdfs:label xml:lang="en">has date of usage</rdfs:label>
  <skos:definition xml:lang="en">Relates a name to a date or range of dates associated with the use of the name chosen as a preferred name for an agent.</skos:definition>
  <rdf:type rdf:resource="http://www.w3.org/1999/02/22-rdf-syntax-ns#Property" />
  <reg:lexicalAlias rdf:resource="http://rdaregistry.info/Elements/u/dateOfUsage.en" />
</owl:ObjectProperty>

<!-- Property: has declination -->
<owl:ObjectProperty rdf:about="http://rdaregistry.info/Elements/u/P60900">
  <rdfs:isDefinedBy rdf:resource="http://rdaregistry.info/Elements/u/" />
  <reg:status rdf:resource="http://metadataregistry.org/uri/RegStatus/1001" />
  <rdf:type rdf:resource="http://www.w3.org/1999/02/22-rdf-syntax-ns#Property" />
  <reg:name xml:lang="en">declination</reg:name>
  <rdfs:label xml:lang="en">has declination</rdfs:label>
  <reg:lexicalAlias rdf:resource="http://rdaregistry.info/Elements/u/declination.en" />
  <skos:definition xml:lang="en">Relates a resource to an angular distance to a body on the celestial sphere measured north or south through 90 from the celestial equator along the hour circle of the body.</skos:definition>
</owl:ObjectProperty>

<!-- Property: has dedicatee -->
<owl:ObjectProperty rdf:about="http://rdaregistry.info/Elements/u/P60455">
  <rdfs:isDefinedBy rdf:resource="http://rdaregistry.info/Elements/u/" />
  <reg:status rdf:resource="http://metadataregistry.org/uri/RegStatus/1001" />
  <reg:name xml:lang="en">dedicatee</reg:name>
  <rdfs:label xml:lang="en">has dedicatee</rdfs:label>
  <skos:definition xml:lang="en">Relates a resource to an agent to whom a resource is dedicated.</skos:definition>
  <rdf:type rdf:resource="http://www.w3.org/1999/02/22-rdf-syntax-ns#Property" />
  <rdfs:subPropertyOf rdf:resource="http://rdaregistry.info/Elements/u/P60374" />
  <owl:inverseOf rdf:resource="http://rdaregistry.info/Elements/u/P60689" />
  <reg:hasSubproperty rdf:resource="http://rdaregistry.info/Elements/i/P40025" />
  <reg:lexicalAlias rdf:resource="http://rdaregistry.info/Elements/u/dedicatee.en" />
</owl:ObjectProperty>

<!-- Property: is dedicatee of -->
<owl:ObjectProperty rdf:about="http://rdaregistry.info/Elements/u/P60689">
  <rdfs:isDefinedBy rdf:resource="http://rdaregistry.info/Elements/u/" />
  <reg:status rdf:resource="http://metadataregistry.org/uri/RegStatus/1001" />
  <reg:name xml:lang="en">dedicateeOf</reg:name>
  <rdfs:label xml:lang="en">is dedicatee of</rdfs:label>
  <skos:definition xml:lang="en">Relates an agent to whom a resource is dedicated to a resource.</skos:definition>
  <rdf:type rdf:resource="http://www.w3.org/1999/02/22-rdf-syntax-ns#Property" />
  <rdfs:subPropertyOf rdf:resource="http://rdaregistry.info/Elements/u/P60602" />
  <owl:inverseOf rdf:resource="http://rdaregistry.info/Elements/u/P60455" />
  <reg:hasSubproperty rdf:resource="http://rdaregistry.info/Elements/a/P50208" />
  <reg:hasSubproperty rdf:resource="http://rdaregistry.info/Elements/a/P50210" />
  <reg:lexicalAlias rdf:resource="http://rdaregistry.info/Elements/u/dedicateeOf.en" />
</owl:ObjectProperty>

<!-- Property: has dedicator -->
<owl:ObjectProperty rdf:about="http://rdaregistry.info/Elements/u/P60375">
  <rdfs:isDefinedBy rdf:resource="http://rdaregistry.info/Elements/u/" />
  <reg:status rdf:resource="http://metadataregistry.org/uri/RegStatus/1001" />
  <reg:name xml:lang="en">dedicator</reg:name>
  <rdfs:label xml:lang="en">has dedicator</rdfs:label>
  <skos:definition xml:lang="en">Relates a resource to an agent by whom a resource is dedicated.</skos:definition>
  <rdf:type rdf:resource="http://www.w3.org/1999/02/22-rdf-syntax-ns#Property" />
  <rdfs:subPropertyOf rdf:resource="http://rdaregistry.info/Elements/u/P60374" />
  <owl:inverseOf rdf:resource="http://rdaregistry.info/Elements/u/P60603" />
  <reg:lexicalAlias rdf:resource="http://rdaregistry.info/Elements/u/dedicator.en" />
</owl:ObjectProperty>

<!-- Property: is dedicator of -->
<owl:ObjectProperty rdf:about="http://rdaregistry.info/Elements/u/P60603">
  <rdfs:isDefinedBy rdf:resource="http://rdaregistry.info/Elements/u/" />
  <reg:status rdf:resource="http://metadataregistry.org/uri/RegStatus/1001" />
  <reg:name xml:lang="en">dedicatorOf</reg:name>
  <rdfs:label xml:lang="en">is dedicator of</rdfs:label>
  <skos:definition xml:lang="en">Relates an agent by whom a resource is dedicated to a resource.</skos:definition>
  <rdf:type rdf:resource="http://www.w3.org/1999/02/22-rdf-syntax-ns#Property" />
  <rdfs:subPropertyOf rdf:resource="http://rdaregistry.info/Elements/u/P60602" />
  <owl:inverseOf rdf:resource="http://rdaregistry.info/Elements/u/P60375" />
  <reg:hasSubproperty rdf:resource="http://rdaregistry.info/Elements/a/P50132" />
  <reg:lexicalAlias rdf:resource="http://rdaregistry.info/Elements/u/dedicatorOf.en" />
</owl:ObjectProperty>

<!-- Property: has defendant -->
<owl:ObjectProperty rdf:about="http://rdaregistry.info/Elements/u/P60462">
  <rdfs:isDefinedBy rdf:resource="http://rdaregistry.info/Elements/u/" />
  <reg:status rdf:resource="http://metadataregistry.org/uri/RegStatus/1001" />
  <reg:name xml:lang="en">defendant</reg:name>
  <rdfs:label xml:lang="en">has defendant</rdfs:label>
  <skos:definition xml:lang="en">Relates a resource to an agent who is accused in a criminal proceeding or sued in a civil proceeding.</skos:definition>
  <rdf:type rdf:resource="http://www.w3.org/1999/02/22-rdf-syntax-ns#Property" />
  <rdfs:subPropertyOf rdf:resource="http://rdaregistry.info/Elements/u/P60374" />
  <owl:inverseOf rdf:resource="http://rdaregistry.info/Elements/u/P60698" />
  <reg:hasSubproperty rdf:resource="http://rdaregistry.info/Elements/w/P10285" />
  <reg:hasSubproperty rdf:resource="http://rdaregistry.info/Elements/w/P10286" />
  <reg:lexicalAlias rdf:resource="http://rdaregistry.info/Elements/u/defendant.en" />
</owl:ObjectProperty>

<!-- Property: is defendant of -->
<owl:ObjectProperty rdf:about="http://rdaregistry.info/Elements/u/P60698">
  <rdfs:isDefinedBy rdf:resource="http://rdaregistry.info/Elements/u/" />
  <reg:status rdf:resource="http://metadataregistry.org/uri/RegStatus/1001" />
  <reg:name xml:lang="en">defendantOf</reg:name>
  <rdfs:label xml:lang="en">is defendant of</rdfs:label>
  <skos:definition xml:lang="en">Relates an agent who is accused in a criminal proceeding or sued in a civil proceeding to a resource.</skos:definition>
  <rdf:type rdf:resource="http://www.w3.org/1999/02/22-rdf-syntax-ns#Property" />
  <rdfs:subPropertyOf rdf:resource="http://rdaregistry.info/Elements/u/P60602" />
  <owl:inverseOf rdf:resource="http://rdaregistry.info/Elements/u/P60462" />
  <reg:hasSubproperty rdf:resource="http://rdaregistry.info/Elements/a/P50090" />
  <reg:hasSubproperty rdf:resource="http://rdaregistry.info/Elements/a/P50258" />
  <reg:hasSubproperty rdf:resource="http://rdaregistry.info/Elements/a/P50259" />
  <reg:lexicalAlias rdf:resource="http://rdaregistry.info/Elements/u/defendantOf.en" />
</owl:ObjectProperty>

<!-- Property: has degree committee member -->
<owl:ObjectProperty rdf:about="http://rdaregistry.info/Elements/u/P60815">
  <rdfs:isDefinedBy rdf:resource="http://rdaregistry.info/Elements/u/" />
  <reg:status rdf:resource="http://metadataregistry.org/uri/RegStatus/1001" />
  <rdf:type rdf:resource="http://www.w3.org/1999/02/22-rdf-syntax-ns#Property" />
  <reg:name xml:lang="en">degreeCommitteeMember</reg:name>
  <rdfs:label xml:lang="en">has degree committee member</rdfs:label>
  <reg:lexicalAlias rdf:resource="http://rdaregistry.info/Elements/u/degreeCommitteeMember.en" />
  <skos:definition xml:lang="en">Relates a resource to an agent serving on a committee that supervises a students thesis or dissertation.</skos:definition>
  <owl:inverseOf rdf:resource="http://rdaregistry.info/Elements/u/P60816" />
  <rdfs:subPropertyOf rdf:resource="http://rdaregistry.info/Elements/u/P60374" />
</owl:ObjectProperty>

<!-- Property: is degree committee member of -->
<owl:ObjectProperty rdf:about="http://rdaregistry.info/Elements/u/P60816">
  <rdfs:isDefinedBy rdf:resource="http://rdaregistry.info/Elements/u/" />
  <reg:status rdf:resource="http://metadataregistry.org/uri/RegStatus/1001" />
  <rdf:type rdf:resource="http://www.w3.org/1999/02/22-rdf-syntax-ns#Property" />
  <reg:name xml:lang="en">degreeCommitteeMemberOf</reg:name>
  <rdfs:label xml:lang="en">is degree committee member of</rdfs:label>
  <reg:lexicalAlias rdf:resource="http://rdaregistry.info/Elements/u/degreeCommitteeMemberOf.en" />
  <skos:definition xml:lang="en">Relates an agent serving on a committee that supervises a students thesis or dissertation to a resource.</skos:definition>
  <owl:inverseOf rdf:resource="http://rdaregistry.info/Elements/u/P60815" />
  <rdfs:subPropertyOf rdf:resource="http://rdaregistry.info/Elements/u/P60602" />
</owl:ObjectProperty>

<!-- Property: has degree granting institution -->
<owl:ObjectProperty rdf:about="http://rdaregistry.info/Elements/u/P60060">
  <rdfs:isDefinedBy rdf:resource="http://rdaregistry.info/Elements/u/" />
  <reg:status rdf:resource="http://metadataregistry.org/uri/RegStatus/1001" />
  <reg:name xml:lang="en">degreeGrantingInstitution</reg:name>
  <rdfs:label xml:lang="en">has degree granting institution</rdfs:label>
  <skos:definition xml:lang="en">Relates a resource to an agent granting an academic degree.</skos:definition>
  <rdf:type rdf:resource="http://www.w3.org/1999/02/22-rdf-syntax-ns#Property" />
  <rdfs:subPropertyOf rdf:resource="http://rdaregistry.info/Elements/u/P60374" />
  <owl:inverseOf rdf:resource="http://rdaregistry.info/Elements/u/P60002" />
  <reg:lexicalAlias rdf:resource="http://rdaregistry.info/Elements/u/degreeGrantingInstitution.en" />
</owl:ObjectProperty>

<!-- Property: is degree granting institution of -->
<owl:ObjectProperty rdf:about="http://rdaregistry.info/Elements/u/P60002">
  <rdfs:isDefinedBy rdf:resource="http://rdaregistry.info/Elements/u/" />
  <reg:status rdf:resource="http://metadataregistry.org/uri/RegStatus/1001" />
  <reg:name xml:lang="en">degreeGrantingInstitutionOf</reg:name>
  <rdfs:label xml:lang="en">is degree granting institution of</rdfs:label>
  <skos:definition xml:lang="en">Relates an agent granting an academic degree to a resource.</skos:definition>
  <rdf:type rdf:resource="http://www.w3.org/1999/02/22-rdf-syntax-ns#Property" />
  <rdfs:subPropertyOf rdf:resource="http://rdaregistry.info/Elements/u/P60602" />
  <owl:inverseOf rdf:resource="http://rdaregistry.info/Elements/u/P60060" />
  <reg:hasSubproperty rdf:resource="http://rdaregistry.info/Elements/a/P50003" />
  <reg:lexicalAlias rdf:resource="http://rdaregistry.info/Elements/u/degreeGrantingInstitutionOf.en" />
</owl:ObjectProperty>

<!-- Property: has degree supervisor -->
<owl:ObjectProperty rdf:about="http://rdaregistry.info/Elements/u/P60420">
  <rdfs:isDefinedBy rdf:resource="http://rdaregistry.info/Elements/u/" />
  <reg:status rdf:resource="http://metadataregistry.org/uri/RegStatus/1001" />
  <reg:name xml:lang="en">degreeSupervisor</reg:name>
  <rdfs:label xml:lang="en">has degree supervisor</rdfs:label>
  <skos:definition xml:lang="en">Relates a resource to an agent, such as an advisor or supervisor of thesis or dissertation research, overseeing either an academic degree or thesis.</skos:definition>
  <rdf:type rdf:resource="http://www.w3.org/1999/02/22-rdf-syntax-ns#Property" />
  <rdfs:subPropertyOf rdf:resource="http://rdaregistry.info/Elements/u/P60447" />
  <owl:inverseOf rdf:resource="http://rdaregistry.info/Elements/u/P60649" />
  <reg:lexicalAlias rdf:resource="http://rdaregistry.info/Elements/u/degreeSupervisor.en" />
</owl:ObjectProperty>

<!-- Property: is degree supervisor of -->
<owl:ObjectProperty rdf:about="http://rdaregistry.info/Elements/u/P60649">
  <rdfs:isDefinedBy rdf:resource="http://rdaregistry.info/Elements/u/" />
  <reg:status rdf:resource="http://metadataregistry.org/uri/RegStatus/1001" />
  <reg:name xml:lang="en">degreeSupervisorOf</reg:name>
  <rdfs:label xml:lang="en">is degree supervisor of</rdfs:label>
  <skos:definition xml:lang="en">Relates an agent, such as an advisor or supervisor of thesis or dissertation research, overseeing either an academic degree or thesis to a resource.</skos:definition>
  <rdf:type rdf:resource="http://www.w3.org/1999/02/22-rdf-syntax-ns#Property" />
  <rdfs:subPropertyOf rdf:resource="http://rdaregistry.info/Elements/u/P60672" />
  <owl:inverseOf rdf:resource="http://rdaregistry.info/Elements/u/P60420" />
  <reg:hasSubproperty rdf:resource="http://rdaregistry.info/Elements/a/P50091" />
  <reg:lexicalAlias rdf:resource="http://rdaregistry.info/Elements/u/degreeSupervisorOf.en" />
</owl:ObjectProperty>

<!-- Property: has depositor -->
<owl:ObjectProperty rdf:about="http://rdaregistry.info/Elements/u/P60068">
  <rdfs:isDefinedBy rdf:resource="http://rdaregistry.info/Elements/u/" />
  <reg:status rdf:resource="http://metadataregistry.org/uri/RegStatus/1001" />
  <reg:name xml:lang="en">depositor</reg:name>
  <rdfs:label xml:lang="en">has depositor</rdfs:label>
  <skos:definition xml:lang="en">Relates a resource to a current owner of a resource who deposited a resource into the custody of another agent, while still retaining ownership.</skos:definition>
  <rdf:type rdf:resource="http://www.w3.org/1999/02/22-rdf-syntax-ns#Property" />
  <rdfs:subPropertyOf rdf:resource="http://rdaregistry.info/Elements/u/P60400" />
  <owl:inverseOf rdf:resource="http://rdaregistry.info/Elements/u/P60008" />
  <reg:hasSubproperty rdf:resource="http://rdaregistry.info/Elements/i/P40006" />
  <reg:lexicalAlias rdf:resource="http://rdaregistry.info/Elements/u/depositor.en" />
</owl:ObjectProperty>

<!-- Property: is depositor of -->
<owl:ObjectProperty rdf:about="http://rdaregistry.info/Elements/u/P60008">
  <rdfs:isDefinedBy rdf:resource="http://rdaregistry.info/Elements/u/" />
  <reg:status rdf:resource="http://metadataregistry.org/uri/RegStatus/1001" />
  <reg:name xml:lang="en">depositorOf</reg:name>
  <rdfs:label xml:lang="en">is depositor of</rdfs:label>
  <skos:definition xml:lang="en">Relates a current owner of a resource who deposited a resource into the custody of another agent, while still retaining ownership to a resource.</skos:definition>
  <rdf:type rdf:resource="http://www.w3.org/1999/02/22-rdf-syntax-ns#Property" />
  <rdfs:subPropertyOf rdf:resource="http://rdaregistry.info/Elements/u/P60628" />
  <owl:inverseOf rdf:resource="http://rdaregistry.info/Elements/u/P60068" />
  <reg:hasSubproperty rdf:resource="http://rdaregistry.info/Elements/a/P50047" />
  <reg:lexicalAlias rdf:resource="http://rdaregistry.info/Elements/u/depositorOf.en" />
</owl:ObjectProperty>

<!-- Property: is derivative -->
<owl:ObjectProperty rdf:about="http://rdaregistry.info/Elements/u/P60250">
  <rdfs:isDefinedBy rdf:resource="http://rdaregistry.info/Elements/u/" />
  <reg:status rdf:resource="http://metadataregistry.org/uri/RegStatus/1001" />
  <reg:name xml:lang="en">derivative</reg:name>
  <rdfs:label xml:lang="en">is derivative</rdfs:label>
  <skos:definition xml:lang="en">Relates a resource to a resource that is a modification of a source resource.</skos:definition>
  <rdf:type rdf:resource="http://www.w3.org/1999/02/22-rdf-syntax-ns#Property" />
  <rdfs:subPropertyOf rdf:resource="http://rdaregistry.info/Elements/u/P60710" />
  <owl:inverseOf rdf:resource="http://rdaregistry.info/Elements/u/P60305" />
  <reg:hasSubproperty rdf:resource="http://rdaregistry.info/Elements/u/P60115" />
  <reg:hasSubproperty rdf:resource="http://rdaregistry.info/Elements/u/P60120" />
  <reg:hasSubproperty rdf:resource="http://rdaregistry.info/Elements/u/P60121" />
  <reg:hasSubproperty rdf:resource="http://rdaregistry.info/Elements/u/P60177" />
  <reg:hasSubproperty rdf:resource="http://rdaregistry.info/Elements/u/P60178" />
  <reg:hasSubproperty rdf:resource="http://rdaregistry.info/Elements/u/P60180" />
  <reg:hasSubproperty rdf:resource="http://rdaregistry.info/Elements/u/P60189" />
  <reg:hasSubproperty rdf:resource="http://rdaregistry.info/Elements/u/P60203" />
  <reg:hasSubproperty rdf:resource="http://rdaregistry.info/Elements/u/P60205" />
  <reg:hasSubproperty rdf:resource="http://rdaregistry.info/Elements/u/P60210" />
  <reg:hasSubproperty rdf:resource="http://rdaregistry.info/Elements/u/P60214" />
  <reg:hasSubproperty rdf:resource="http://rdaregistry.info/Elements/u/P60216" />
  <reg:hasSubproperty rdf:resource="http://rdaregistry.info/Elements/u/P60245" />
  <reg:hasSubproperty rdf:resource="http://rdaregistry.info/Elements/u/P60260" />
  <reg:hasSubproperty rdf:resource="http://rdaregistry.info/Elements/u/P60273" />
  <reg:hasSubproperty rdf:resource="http://rdaregistry.info/Elements/u/P60274" />
  <reg:hasSubproperty rdf:resource="http://rdaregistry.info/Elements/u/P60275" />
  <reg:hasSubproperty rdf:resource="http://rdaregistry.info/Elements/u/P60279" />
  <reg:hasSubproperty rdf:resource="http://rdaregistry.info/Elements/u/P60280" />
  <reg:hasSubproperty rdf:resource="http://rdaregistry.info/Elements/e/P20203" />
  <reg:lexicalAlias rdf:resource="http://rdaregistry.info/Elements/u/derivative.en" />
  <reg:hasSubproperty rdf:resource="http://rdaregistry.info/Elements/u/P60831" />
  <reg:hasSubproperty rdf:resource="http://rdaregistry.info/Elements/u/P60833" />
</owl:ObjectProperty>

<!-- Property: has derivative resource relationship with -->
<owl:ObjectProperty rdf:about="http://rdaregistry.info/Elements/u/P60710">
  <rdfs:isDefinedBy rdf:resource="http://rdaregistry.info/Elements/u/" />
  <reg:status rdf:resource="http://metadataregistry.org/uri/RegStatus/1001" />
  <reg:name xml:lang="en">derivativeResourceRelationshipWith</reg:name>
  <rdfs:label xml:lang="en">has derivative resource relationship with</rdfs:label>
  <rdf:type rdf:resource="http://www.w3.org/1999/02/22-rdf-syntax-ns#Property" />
  <reg:hasSubproperty rdf:resource="http://rdaregistry.info/Elements/u/P60250" />
  <reg:hasSubproperty rdf:resource="http://rdaregistry.info/Elements/u/P60305" />
  <owl:inverseOf rdf:resource="http://rdaregistry.info/Elements/u/P60710" />
  <skos:definition xml:lang="en">Relates a resource to a resource that is based on or is a derivative of a resource.</skos:definition>
  <reg:hasSubproperty rdf:resource="http://rdaregistry.info/Elements/e/P20233" />
  <reg:lexicalAlias rdf:resource="http://rdaregistry.info/Elements/u/derivativeResourceRelationshipWith.en" />
</owl:ObjectProperty>

<!-- Property: is described in -->
<owl:ObjectProperty rdf:about="http://rdaregistry.info/Elements/u/P60215">
  <rdfs:isDefinedBy rdf:resource="http://rdaregistry.info/Elements/u/" />
  <reg:status rdf:resource="http://metadataregistry.org/uri/RegStatus/1001" />
  <reg:name xml:lang="en">describedIn</reg:name>
  <rdfs:label xml:lang="en">is described in</rdfs:label>
  <skos:definition xml:lang="en">Relates a resource to a resource that describes a described entity.</skos:definition>
  <rdf:type rdf:resource="http://www.w3.org/1999/02/22-rdf-syntax-ns#Property" />
  <rdfs:subPropertyOf rdf:resource="http://rdaregistry.info/Elements/u/P60806" />
  <owl:inverseOf rdf:resource="http://rdaregistry.info/Elements/u/P60190" />
  <reg:hasSubproperty rdf:resource="http://rdaregistry.info/Elements/u/P60211" />
  <reg:hasSubproperty rdf:resource="http://rdaregistry.info/Elements/u/P60212" />
  <reg:hasSubproperty rdf:resource="http://rdaregistry.info/Elements/u/P60213" />
  <reg:hasSubproperty rdf:resource="http://rdaregistry.info/Elements/u/P60218" />
  <reg:hasSubproperty rdf:resource="http://rdaregistry.info/Elements/u/P60219" />
  <reg:hasSubproperty rdf:resource="http://rdaregistry.info/Elements/e/P20269" />
  <reg:hasSubproperty rdf:resource="http://rdaregistry.info/Elements/i/P40062" />
  <reg:hasSubproperty rdf:resource="http://rdaregistry.info/Elements/m/P30254" />
  <reg:lexicalAlias rdf:resource="http://rdaregistry.info/Elements/u/describedIn.en" />
</owl:ObjectProperty>

<!-- Property: is description of -->
<owl:ObjectProperty rdf:about="http://rdaregistry.info/Elements/u/P60190">
  <rdfs:isDefinedBy rdf:resource="http://rdaregistry.info/Elements/u/" />
  <reg:status rdf:resource="http://metadataregistry.org/uri/RegStatus/1001" />
  <reg:name xml:lang="en">descriptionOf</reg:name>
  <rdfs:label xml:lang="en">is description of</rdfs:label>
  <skos:definition xml:lang="en">Relates a resource to a resource described by a describing entity.</skos:definition>
  <rdf:type rdf:resource="http://www.w3.org/1999/02/22-rdf-syntax-ns#Property" />
  <rdfs:subPropertyOf rdf:resource="http://rdaregistry.info/Elements/u/P60805" />
  <owl:inverseOf rdf:resource="http://rdaregistry.info/Elements/u/P60215" />
  <reg:hasSubproperty rdf:resource="http://rdaregistry.info/Elements/u/P60239" />
  <reg:hasSubproperty rdf:resource="http://rdaregistry.info/Elements/u/P60255" />
  <reg:hasSubproperty rdf:resource="http://rdaregistry.info/Elements/u/P60288" />
  <reg:hasSubproperty rdf:resource="http://rdaregistry.info/Elements/u/P60292" />
  <reg:hasSubproperty rdf:resource="http://rdaregistry.info/Elements/u/P60298" />
  <reg:hasSubproperty rdf:resource="http://rdaregistry.info/Elements/w/P10265" />
  <reg:hasSubproperty rdf:resource="http://rdaregistry.info/Elements/w/P10271" />
  <reg:hasSubproperty rdf:resource="http://rdaregistry.info/Elements/w/P10277" />
  <reg:lexicalAlias rdf:resource="http://rdaregistry.info/Elements/u/descriptionOf.en" />
</owl:ObjectProperty>

<!-- Property: DEPRECATED -->
<owl:ObjectProperty rdf:about="http://rdaregistry.info/Elements/u/P60711">
  <rdfs:isDefinedBy rdf:resource="http://rdaregistry.info/Elements/u/" />
  <reg:status rdf:resource="http://metadataregistry.org/uri/RegStatus/1008" />
  <reg:hasSubproperty rdf:resource="http://rdaregistry.info/Elements/u/P60190" />
  <reg:hasSubproperty rdf:resource="http://rdaregistry.info/Elements/u/P60215" />
</owl:ObjectProperty>

<!-- Property: has designation of edition -->
<owl:ObjectProperty rdf:about="http://rdaregistry.info/Elements/u/P60365">
  <rdfs:isDefinedBy rdf:resource="http://rdaregistry.info/Elements/u/" />
  <reg:status rdf:resource="http://metadataregistry.org/uri/RegStatus/1001" />
  <reg:name xml:lang="en">designationOfEdition</reg:name>
  <rdfs:label xml:lang="en">has designation of edition</rdfs:label>
  <skos:definition xml:lang="en">Relates a resource to a word, character or group of words or characters, identifying an edition to which a resource belongs.</skos:definition>
  <rdf:type rdf:resource="http://www.w3.org/1999/02/22-rdf-syntax-ns#Property" />
  <reg:hasSubproperty rdf:resource="http://rdaregistry.info/Elements/m/P30133" />
  <reg:lexicalAlias rdf:resource="http://rdaregistry.info/Elements/u/designationOfEdition.en" />
</owl:ObjectProperty>

<!-- Property: has designation of named revision of edition -->
<owl:ObjectProperty rdf:about="http://rdaregistry.info/Elements/u/P60364">
  <rdfs:isDefinedBy rdf:resource="http://rdaregistry.info/Elements/u/" />
  <reg:status rdf:resource="http://metadataregistry.org/uri/RegStatus/1001" />
  <reg:name xml:lang="en">designationOfNamedRevisionOfEdition</reg:name>
  <rdfs:label xml:lang="en">has designation of named revision of edition</rdfs:label>
  <skos:definition xml:lang="en">Relates a resource to a word, character or group of words or characters, identifying a particular revision of a named edition.</skos:definition>
  <rdf:type rdf:resource="http://www.w3.org/1999/02/22-rdf-syntax-ns#Property" />
  <reg:hasSubproperty rdf:resource="http://rdaregistry.info/Elements/m/P30132" />
  <reg:lexicalAlias rdf:resource="http://rdaregistry.info/Elements/u/designationOfNamedRevisionOfEdition.en" />
</owl:ObjectProperty>

<!-- Property: has designer -->
<owl:ObjectProperty rdf:about="http://rdaregistry.info/Elements/u/P60424">
  <rdfs:isDefinedBy rdf:resource="http://rdaregistry.info/Elements/u/" />
  <reg:status rdf:resource="http://metadataregistry.org/uri/RegStatus/1001" />
  <reg:name xml:lang="en">designer</reg:name>
  <rdfs:label xml:lang="en">has designer</rdfs:label>
  <skos:definition xml:lang="en">Relates a resource to an agent responsible for creating a design for an object.</skos:definition>
  <rdf:type rdf:resource="http://www.w3.org/1999/02/22-rdf-syntax-ns#Property" />
  <rdfs:subPropertyOf rdf:resource="http://rdaregistry.info/Elements/u/P60447" />
  <owl:inverseOf rdf:resource="http://rdaregistry.info/Elements/u/P60653" />
  <reg:lexicalAlias rdf:resource="http://rdaregistry.info/Elements/u/designer.en" />
</owl:ObjectProperty>

<!-- Property: is designer of -->
<owl:ObjectProperty rdf:about="http://rdaregistry.info/Elements/u/P60653">
  <rdfs:isDefinedBy rdf:resource="http://rdaregistry.info/Elements/u/" />
  <reg:status rdf:resource="http://metadataregistry.org/uri/RegStatus/1001" />
  <reg:name xml:lang="en">designerOf</reg:name>
  <rdfs:label xml:lang="en">is designer of</rdfs:label>
  <skos:definition xml:lang="en">Relates an agent responsible for creating a design for an object to a resource.</skos:definition>
  <rdf:type rdf:resource="http://www.w3.org/1999/02/22-rdf-syntax-ns#Property" />
  <rdfs:subPropertyOf rdf:resource="http://rdaregistry.info/Elements/u/P60672" />
  <owl:inverseOf rdf:resource="http://rdaregistry.info/Elements/u/P60424" />
  <reg:hasSubproperty rdf:resource="http://rdaregistry.info/Elements/a/P50185" />
  <reg:lexicalAlias rdf:resource="http://rdaregistry.info/Elements/u/designerOf.en" />
</owl:ObjectProperty>

<!-- Property: has details of applied material -->
<owl:ObjectProperty rdf:about="http://rdaregistry.info/Elements/u/P60767">
  <rdfs:isDefinedBy rdf:resource="http://rdaregistry.info/Elements/u/" />
  <reg:status rdf:resource="http://metadataregistry.org/uri/RegStatus/1001" />
  <rdf:type rdf:resource="http://www.w3.org/1999/02/22-rdf-syntax-ns#Property" />
  <reg:name xml:lang="en">detailsOfAppliedMaterial</reg:name>
  <rdfs:label xml:lang="en">has details of applied material</rdfs:label>
  <reg:lexicalAlias rdf:resource="http://rdaregistry.info/Elements/u/detailsOfAppliedMaterial.en" />
  <skos:definition xml:lang="en">Relates a resource to details of a physical or chemical substance applied to a base material of a resource.</skos:definition>
  <reg:hasSubproperty rdf:resource="http://rdaregistry.info/Elements/u/P60774" />
</owl:ObjectProperty>

<!-- Property: has details of aspect ratio designation -->
<owl:ObjectProperty rdf:about="http://rdaregistry.info/Elements/u/P60760">
  <rdfs:isDefinedBy rdf:resource="http://rdaregistry.info/Elements/u/" />
  <reg:status rdf:resource="http://metadataregistry.org/uri/RegStatus/1001" />
  <rdf:type rdf:resource="http://www.w3.org/1999/02/22-rdf-syntax-ns#Property" />
  <reg:name xml:lang="en">detailsOfAspectRatioDesignation</reg:name>
  <rdfs:label xml:lang="en">has details of aspect ratio designation</rdfs:label>
  <reg:lexicalAlias rdf:resource="http://rdaregistry.info/Elements/u/detailsOfAspectRatioDesignation.en" />
  <skos:definition xml:lang="en">Relates a resource to details of the ratio of the width to the height of a moving image.</skos:definition>
</owl:ObjectProperty>

<!-- Property: has details of base material -->
<owl:ObjectProperty rdf:about="http://rdaregistry.info/Elements/u/P60768">
  <rdfs:isDefinedBy rdf:resource="http://rdaregistry.info/Elements/u/" />
  <reg:status rdf:resource="http://metadataregistry.org/uri/RegStatus/1001" />
  <rdf:type rdf:resource="http://www.w3.org/1999/02/22-rdf-syntax-ns#Property" />
  <reg:name xml:lang="en">detailsOfBaseMaterial</reg:name>
  <rdfs:label xml:lang="en">has details of base material</rdfs:label>
  <reg:lexicalAlias rdf:resource="http://rdaregistry.info/Elements/u/detailsOfBaseMaterial.en" />
  <skos:definition xml:lang="en">Relates a resource to details of an underlying physical material of a resource.</skos:definition>
</owl:ObjectProperty>

<!-- Property: has details of book format -->
<owl:ObjectProperty rdf:about="http://rdaregistry.info/Elements/u/P60769">
  <rdfs:isDefinedBy rdf:resource="http://rdaregistry.info/Elements/u/" />
  <reg:status rdf:resource="http://metadataregistry.org/uri/RegStatus/1001" />
  <rdf:type rdf:resource="http://www.w3.org/1999/02/22-rdf-syntax-ns#Property" />
  <reg:name xml:lang="en">detailsOfBookFormat</reg:name>
  <rdfs:label xml:lang="en">has details of book format</rdfs:label>
  <reg:lexicalAlias rdf:resource="http://rdaregistry.info/Elements/u/detailsOfBookFormat.en" />
  <skos:definition xml:lang="en">Relates a resource to details of a result of folding a printed sheet to form a gathering of leaves (e.g., a sheet folded once to form a folio, twice to form a quarto, three times to form an octavo, etc.).</skos:definition>
</owl:ObjectProperty>

<!-- Property: has details of broadcast standard -->
<owl:ObjectProperty rdf:about="http://rdaregistry.info/Elements/u/P60770">
  <rdfs:isDefinedBy rdf:resource="http://rdaregistry.info/Elements/u/" />
  <reg:status rdf:resource="http://metadataregistry.org/uri/RegStatus/1001" />
  <rdf:type rdf:resource="http://www.w3.org/1999/02/22-rdf-syntax-ns#Property" />
  <reg:name xml:lang="en">detailsOfBroadcastStandard</reg:name>
  <rdfs:label xml:lang="en">has details of broadcast standard</rdfs:label>
  <reg:lexicalAlias rdf:resource="http://rdaregistry.info/Elements/u/detailsOfBroadcastStandard.en" />
  <skos:definition xml:lang="en">Relates a resource to details of a system used to format a video resource for television broadcast.</skos:definition>
  <rdfs:subPropertyOf rdf:resource="http://rdaregistry.info/Elements/u/P60801" />
</owl:ObjectProperty>

<!-- Property: has details of cartographic data type -->
<owl:ObjectProperty rdf:about="http://rdaregistry.info/Elements/u/P60876">
  <rdfs:isDefinedBy rdf:resource="http://rdaregistry.info/Elements/u/" />
  <reg:status rdf:resource="http://metadataregistry.org/uri/RegStatus/1001" />
  <rdf:type rdf:resource="http://www.w3.org/1999/02/22-rdf-syntax-ns#Property" />
  <reg:name xml:lang="en">detailsOfCartographicDataType</reg:name>
  <rdfs:label xml:lang="en">has details of cartographic data type</rdfs:label>
  <reg:lexicalAlias rdf:resource="http://rdaregistry.info/Elements/u/detailsOfCartographicDataType.en" />
  <skos:definition xml:lang="en">Relates a resource to details of a machine-readable representation of geospatial features.</skos:definition>
  <reg:hasSubproperty rdf:resource="http://rdaregistry.info/Elements/m/P30262" />
</owl:ObjectProperty>

<!-- Property: has details of colour content -->
<owl:ObjectProperty rdf:about="http://rdaregistry.info/Elements/u/P60761">
  <rdfs:isDefinedBy rdf:resource="http://rdaregistry.info/Elements/u/" />
  <reg:status rdf:resource="http://metadataregistry.org/uri/RegStatus/1001" />
  <rdf:type rdf:resource="http://www.w3.org/1999/02/22-rdf-syntax-ns#Property" />
  <reg:name xml:lang="en">detailsOfColourContent</reg:name>
  <rdfs:label xml:lang="en">has details of colour content</rdfs:label>
  <reg:lexicalAlias rdf:resource="http://rdaregistry.info/Elements/u/detailsOfColourContent.en" />
  <skos:definition xml:lang="en">Relates a resource to details of the presence of colour, tone, etc., in the content of a resource, and the specific colours, tones, etc., including black and white, present.</skos:definition>
  <skos:altLabel xml:lang="en">has details of color content</skos:altLabel>
</owl:ObjectProperty>

<!-- Property: has details of configuration of playback channels -->
<owl:ObjectProperty rdf:about="http://rdaregistry.info/Elements/u/P60771">
  <rdfs:isDefinedBy rdf:resource="http://rdaregistry.info/Elements/u/" />
  <reg:status rdf:resource="http://metadataregistry.org/uri/RegStatus/1001" />
  <rdf:type rdf:resource="http://www.w3.org/1999/02/22-rdf-syntax-ns#Property" />
  <reg:name xml:lang="en">detailsOfConfigurationOfPlaybackChannels</reg:name>
  <rdfs:label xml:lang="en">has details of configuration of playback channels</rdfs:label>
  <reg:lexicalAlias rdf:resource="http://rdaregistry.info/Elements/u/detailsOfConfigurationOfPlaybackChannels.en" />
  <skos:definition xml:lang="en">Relates a resource to details of a number of sound channels used to make a recording.</skos:definition>
  <rdfs:subPropertyOf rdf:resource="http://rdaregistry.info/Elements/u/P60796" />
</owl:ObjectProperty>

<!-- Property: has details of digital file characteristic -->
<owl:ObjectProperty rdf:about="http://rdaregistry.info/Elements/u/P60772">
  <rdfs:isDefinedBy rdf:resource="http://rdaregistry.info/Elements/u/" />
  <reg:status rdf:resource="http://metadataregistry.org/uri/RegStatus/1001" />
  <rdf:type rdf:resource="http://www.w3.org/1999/02/22-rdf-syntax-ns#Property" />
  <reg:name xml:lang="en">detailsOfDigitalFileCharacteristic</reg:name>
  <rdfs:label xml:lang="en">has details of digital file characteristic</rdfs:label>
  <reg:lexicalAlias rdf:resource="http://rdaregistry.info/Elements/u/detailsOfDigitalFileCharacteristic.en" />
  <skos:definition xml:lang="en">Relates a resource to details of a technical specification relating to a digital encoding of text, image, audio, video, and other types of data in a resource.</skos:definition>
  <reg:hasSubproperty rdf:resource="http://rdaregistry.info/Elements/u/P60773" />
  <reg:hasSubproperty rdf:resource="http://rdaregistry.info/Elements/u/P60775" />
  <reg:hasSubproperty rdf:resource="http://rdaregistry.info/Elements/u/P60776" />
</owl:ObjectProperty>

<!-- Property: has details of digital representation of cartographic content -->
<owl:ObjectProperty rdf:about="http://rdaregistry.info/Elements/u/P60773">
  <rdfs:isDefinedBy rdf:resource="http://rdaregistry.info/Elements/u/" />
  <reg:status rdf:resource="http://metadataregistry.org/uri/RegStatus/1001" />
  <rdf:type rdf:resource="http://www.w3.org/1999/02/22-rdf-syntax-ns#Property" />
  <reg:name xml:lang="en">detailsOfDigitalRepresentationOfCartographicContent</reg:name>
  <rdfs:label xml:lang="en">has details of digital representation of cartographic content</rdfs:label>
  <reg:lexicalAlias rdf:resource="http://rdaregistry.info/Elements/u/detailsOfDigitalRepresentationOfCartographicContent.en" />
  <skos:definition xml:lang="en">Relates a resource to details of an encoding of geospatial information in a cartographic resource.</skos:definition>
  <rdfs:subPropertyOf rdf:resource="http://rdaregistry.info/Elements/u/P60772" />
</owl:ObjectProperty>

<!-- Property: has details of duration -->
<owl:ObjectProperty rdf:about="http://rdaregistry.info/Elements/u/P60823">
  <rdfs:isDefinedBy rdf:resource="http://rdaregistry.info/Elements/u/" />
  <reg:status rdf:resource="http://metadataregistry.org/uri/RegStatus/1001" />
  <rdf:type rdf:resource="http://www.w3.org/1999/02/22-rdf-syntax-ns#Property" />
  <reg:name xml:lang="en">detailsOfDuration</reg:name>
  <rdfs:label xml:lang="en">has details of duration</rdfs:label>
  <reg:lexicalAlias rdf:resource="http://rdaregistry.info/Elements/u/detailsOfDuration.en" />
  <skos:definition xml:lang="en">Relates a resource to details of the playing time, running time, performance time, etc., of the content of a resource.</skos:definition>
</owl:ObjectProperty>

<!-- Property: has details of emulsion on microfilm and microfiche -->
<owl:ObjectProperty rdf:about="http://rdaregistry.info/Elements/u/P60774">
  <rdfs:isDefinedBy rdf:resource="http://rdaregistry.info/Elements/u/" />
  <reg:status rdf:resource="http://metadataregistry.org/uri/RegStatus/1001" />
  <rdf:type rdf:resource="http://www.w3.org/1999/02/22-rdf-syntax-ns#Property" />
  <reg:name xml:lang="en">detailsOfEmulsionOnMicrofilmAndMicrofiche</reg:name>
  <rdfs:label xml:lang="en">has details of emulsion on microfilm and microfiche</rdfs:label>
  <reg:lexicalAlias rdf:resource="http://rdaregistry.info/Elements/u/detailsOfEmulsionOnMicrofilmAndMicrofiche.en" />
  <skos:definition xml:lang="en">Relates a resource to details of a suspension of light-sensitive chemicals used as a coating on a microfilm or microfiche.</skos:definition>
  <rdfs:subPropertyOf rdf:resource="http://rdaregistry.info/Elements/u/P60767" />
</owl:ObjectProperty>

<!-- Property: has details of encoding format -->
<owl:ObjectProperty rdf:about="http://rdaregistry.info/Elements/u/P60775">
  <rdfs:isDefinedBy rdf:resource="http://rdaregistry.info/Elements/u/" />
  <reg:status rdf:resource="http://metadataregistry.org/uri/RegStatus/1001" />
  <rdf:type rdf:resource="http://www.w3.org/1999/02/22-rdf-syntax-ns#Property" />
  <reg:name xml:lang="en">detailsOfEncodingFormat</reg:name>
  <rdfs:label xml:lang="en">has details of encoding format</rdfs:label>
  <reg:lexicalAlias rdf:resource="http://rdaregistry.info/Elements/u/detailsOfEncodingFormat.en" />
  <skos:definition xml:lang="en">Relates a resource to details of a schema, standard, etc., used to encode the digital content of a resource.</skos:definition>
  <rdfs:subPropertyOf rdf:resource="http://rdaregistry.info/Elements/u/P60772" />
</owl:ObjectProperty>

<!-- Property: has details of file type -->
<owl:ObjectProperty rdf:about="http://rdaregistry.info/Elements/u/P60776">
  <rdfs:isDefinedBy rdf:resource="http://rdaregistry.info/Elements/u/" />
  <reg:status rdf:resource="http://metadataregistry.org/uri/RegStatus/1001" />
  <rdf:type rdf:resource="http://www.w3.org/1999/02/22-rdf-syntax-ns#Property" />
  <reg:name xml:lang="en">detailsOfFileType</reg:name>
  <rdfs:label xml:lang="en">has details of file type</rdfs:label>
  <reg:lexicalAlias rdf:resource="http://rdaregistry.info/Elements/u/detailsOfFileType.en" />
  <skos:definition xml:lang="en">Relates a resource to details of a general type of data content encoded in a computer file.</skos:definition>
  <rdfs:subPropertyOf rdf:resource="http://rdaregistry.info/Elements/u/P60772" />
</owl:ObjectProperty>

<!-- Property: has details of font size -->
<owl:ObjectProperty rdf:about="http://rdaregistry.info/Elements/u/P60777">
  <rdfs:isDefinedBy rdf:resource="http://rdaregistry.info/Elements/u/" />
  <reg:status rdf:resource="http://metadataregistry.org/uri/RegStatus/1001" />
  <rdf:type rdf:resource="http://www.w3.org/1999/02/22-rdf-syntax-ns#Property" />
  <reg:name xml:lang="en">detailsOfFontSize</reg:name>
  <rdfs:label xml:lang="en">has details of font size</rdfs:label>
  <reg:lexicalAlias rdf:resource="http://rdaregistry.info/Elements/u/detailsOfFontSize.en" />
  <skos:definition xml:lang="en">Relates a resource to details of a size of the type used to represent characters and symbols in a resource.</skos:definition>
</owl:ObjectProperty>

<!-- Property: has details of format of notated music -->
<owl:ObjectProperty rdf:about="http://rdaregistry.info/Elements/u/P60764">
  <rdfs:isDefinedBy rdf:resource="http://rdaregistry.info/Elements/u/" />
  <reg:status rdf:resource="http://metadataregistry.org/uri/RegStatus/1001" />
  <rdf:type rdf:resource="http://www.w3.org/1999/02/22-rdf-syntax-ns#Property" />
  <reg:name xml:lang="en">detailsOfFormatOfNotatedMusic</reg:name>
  <rdfs:label xml:lang="en">has details of format of notated music</rdfs:label>
  <reg:lexicalAlias rdf:resource="http://rdaregistry.info/Elements/u/detailsOfFormatOfNotatedMusic.en" />
  <skos:definition xml:lang="en">Relates a resource to details of a musical or physical layout of the content of a resource that is presented in a form of musical notation.</skos:definition>
</owl:ObjectProperty>

<!-- Property: has details of form of musical notation -->
<owl:ObjectProperty rdf:about="http://rdaregistry.info/Elements/u/P60762">
  <rdfs:isDefinedBy rdf:resource="http://rdaregistry.info/Elements/u/" />
  <reg:status rdf:resource="http://metadataregistry.org/uri/RegStatus/1001" />
  <rdf:type rdf:resource="http://www.w3.org/1999/02/22-rdf-syntax-ns#Property" />
  <reg:name xml:lang="en">detailsOfFormOfMusicalNotation</reg:name>
  <rdfs:label xml:lang="en">has details of form of musical notation</rdfs:label>
  <reg:lexicalAlias rdf:resource="http://rdaregistry.info/Elements/u/detailsOfFormOfMusicalNotation.en" />
  <skos:definition xml:lang="en">Relates a resource to details of a set of characters or symbols used to express musical content of a resource.</skos:definition>
</owl:ObjectProperty>

<!-- Property: has details of form of notated movement -->
<owl:ObjectProperty rdf:about="http://rdaregistry.info/Elements/u/P60763">
  <rdfs:isDefinedBy rdf:resource="http://rdaregistry.info/Elements/u/" />
  <reg:status rdf:resource="http://metadataregistry.org/uri/RegStatus/1001" />
  <rdf:type rdf:resource="http://www.w3.org/1999/02/22-rdf-syntax-ns#Property" />
  <reg:name xml:lang="en">detailsOfFormOfNotatedMovement</reg:name>
  <rdfs:label xml:lang="en">has details of form of notated movement</rdfs:label>
  <reg:lexicalAlias rdf:resource="http://rdaregistry.info/Elements/u/detailsOfFormOfNotatedMovement.en" />
  <skos:definition xml:lang="en">Relates a resource to details of a set of characters or symbols used to express movement content of a resource.</skos:definition>
</owl:ObjectProperty>

<!-- Property: has details of form of tactile notation -->
<owl:ObjectProperty rdf:about="http://rdaregistry.info/Elements/u/P60765">
  <rdfs:isDefinedBy rdf:resource="http://rdaregistry.info/Elements/u/" />
  <reg:status rdf:resource="http://metadataregistry.org/uri/RegStatus/1001" />
  <rdf:type rdf:resource="http://www.w3.org/1999/02/22-rdf-syntax-ns#Property" />
  <reg:name xml:lang="en">detailsOfFormOfTactileNotation</reg:name>
  <rdfs:label xml:lang="en">has details of form of tactile notation</rdfs:label>
  <reg:lexicalAlias rdf:resource="http://rdaregistry.info/Elements/u/detailsOfFormOfTactileNotation.en" />
  <skos:definition xml:lang="en">Relates a resource to details of a set of characters or symbols used to express the content of a resource in a form that can be perceived through touch.</skos:definition>
</owl:ObjectProperty>

<!-- Property: has details of generation -->
<owl:ObjectProperty rdf:about="http://rdaregistry.info/Elements/u/P60803">
  <rdfs:isDefinedBy rdf:resource="http://rdaregistry.info/Elements/u/" />
  <reg:status rdf:resource="http://metadataregistry.org/uri/RegStatus/1001" />
  <rdf:type rdf:resource="http://www.w3.org/1999/02/22-rdf-syntax-ns#Property" />
  <reg:name xml:lang="en">detailsOfGeneration</reg:name>
  <rdfs:label xml:lang="en">has details of generation</rdfs:label>
  <reg:lexicalAlias rdf:resource="http://rdaregistry.info/Elements/u/detailsOfGeneration.en" />
  <skos:definition xml:lang="en">Relates a resource to details of a relationship between an original carrier and a carrier of a reproduction made from an original.</skos:definition>
  <reg:hasSubproperty rdf:resource="http://rdaregistry.info/Elements/u/P60778" />
  <reg:hasSubproperty rdf:resource="http://rdaregistry.info/Elements/u/P60779" />
  <reg:hasSubproperty rdf:resource="http://rdaregistry.info/Elements/u/P60780" />
  <reg:hasSubproperty rdf:resource="http://rdaregistry.info/Elements/u/P60781" />
  <reg:hasSubproperty rdf:resource="http://rdaregistry.info/Elements/u/P60782" />
</owl:ObjectProperty>

<!-- Property: DEPRECATED -->
<owl:ObjectProperty rdf:about="http://rdaregistry.info/Elements/u/P60778">
  <rdfs:isDefinedBy rdf:resource="http://rdaregistry.info/Elements/u/" />
  <reg:status rdf:resource="http://metadataregistry.org/uri/RegStatus/1008" />
  <rdf:type rdf:resource="http://www.w3.org/1999/02/22-rdf-syntax-ns#Property" />
  <reg:name xml:lang="en">detailsOfGenerationOfAudioRecording</reg:name>
  <reg:lexicalAlias rdf:resource="http://rdaregistry.info/Elements/u/detailsOfGenerationOfAudioRecording.en" />
  <skos:definition xml:lang="en">Relates a resource to details of the relationship between an original audio carrier and the carrier of a reproduction made from the original (e.g., a tape duplication master, a test pressing).</skos:definition>
  <rdfs:subPropertyOf rdf:resource="http://rdaregistry.info/Elements/u/P60803" />
</owl:ObjectProperty>

<!-- Property: DEPRECATED -->
<owl:ObjectProperty rdf:about="http://rdaregistry.info/Elements/u/P60779">
  <rdfs:isDefinedBy rdf:resource="http://rdaregistry.info/Elements/u/" />
  <reg:status rdf:resource="http://metadataregistry.org/uri/RegStatus/1008" />
  <rdf:type rdf:resource="http://www.w3.org/1999/02/22-rdf-syntax-ns#Property" />
  <reg:name xml:lang="en">detailsOfGenerationOfDigitalResource</reg:name>
  <reg:lexicalAlias rdf:resource="http://rdaregistry.info/Elements/u/detailsOfGenerationOfDigitalResource.en" />
  <skos:definition xml:lang="en">Relates a resource to details of the relationship between an original carrier of a digital resource and the carrier of a reproduction made from the original (e.g., a derivative master).</skos:definition>
  <rdfs:subPropertyOf rdf:resource="http://rdaregistry.info/Elements/u/P60803" />
</owl:ObjectProperty>

<!-- Property: DEPRECATED -->
<owl:ObjectProperty rdf:about="http://rdaregistry.info/Elements/u/P60780">
  <rdfs:isDefinedBy rdf:resource="http://rdaregistry.info/Elements/u/" />
  <reg:status rdf:resource="http://metadataregistry.org/uri/RegStatus/1008" />
  <rdf:type rdf:resource="http://www.w3.org/1999/02/22-rdf-syntax-ns#Property" />
  <reg:name xml:lang="en">detailsOfGenerationOfMicroform</reg:name>
  <reg:lexicalAlias rdf:resource="http://rdaregistry.info/Elements/u/detailsOfGenerationOfMicroform.en" />
  <skos:definition xml:lang="en">Relates a resource to details of the relationship between an original microform carrier and the carrier of a reproduction made from the original (e.g., a printing master).</skos:definition>
  <rdfs:subPropertyOf rdf:resource="http://rdaregistry.info/Elements/u/P60803" />
</owl:ObjectProperty>

<!-- Property: DEPRECATED -->
<owl:ObjectProperty rdf:about="http://rdaregistry.info/Elements/u/P60781">
  <rdfs:isDefinedBy rdf:resource="http://rdaregistry.info/Elements/u/" />
  <reg:status rdf:resource="http://metadataregistry.org/uri/RegStatus/1008" />
  <rdf:type rdf:resource="http://www.w3.org/1999/02/22-rdf-syntax-ns#Property" />
  <reg:name xml:lang="en">detailsOfGenerationOfMotionPictureFilm</reg:name>
  <reg:lexicalAlias rdf:resource="http://rdaregistry.info/Elements/u/detailsOfGenerationOfMotionPictureFilm.en" />
  <skos:definition xml:lang="en">Relates a resource to details of the relationship between an original carrier of a motion picture film resource and the carrier of a reproduction made from the original (e.g., a reference print).</skos:definition>
  <rdfs:subPropertyOf rdf:resource="http://rdaregistry.info/Elements/u/P60803" />
</owl:ObjectProperty>

<!-- Property: DEPRECATED -->
<owl:ObjectProperty rdf:about="http://rdaregistry.info/Elements/u/P60782">
  <rdfs:isDefinedBy rdf:resource="http://rdaregistry.info/Elements/u/" />
  <reg:status rdf:resource="http://metadataregistry.org/uri/RegStatus/1008" />
  <rdf:type rdf:resource="http://www.w3.org/1999/02/22-rdf-syntax-ns#Property" />
  <reg:name xml:lang="en">detailsOfGenerationOfVideotape</reg:name>
  <reg:lexicalAlias rdf:resource="http://rdaregistry.info/Elements/u/detailsOfGenerationOfVideotape.en" />
  <skos:definition xml:lang="en">Relates a resource to details of the relationship between an original carrier of a videotape resource and the carrier of a reproduction made from the original (e.g., a show copy).</skos:definition>
  <rdfs:subPropertyOf rdf:resource="http://rdaregistry.info/Elements/u/P60803" />
</owl:ObjectProperty>

<!-- Property: has details of groove characteristic -->
<owl:ObjectProperty rdf:about="http://rdaregistry.info/Elements/u/P60783">
  <rdfs:isDefinedBy rdf:resource="http://rdaregistry.info/Elements/u/" />
  <reg:status rdf:resource="http://metadataregistry.org/uri/RegStatus/1001" />
  <rdf:type rdf:resource="http://www.w3.org/1999/02/22-rdf-syntax-ns#Property" />
  <reg:name xml:lang="en">detailsOfGrooveCharacteristic</reg:name>
  <rdfs:label xml:lang="en">has details of groove characteristic</rdfs:label>
  <reg:lexicalAlias rdf:resource="http://rdaregistry.info/Elements/u/detailsOfGrooveCharacteristic.en" />
  <skos:definition xml:lang="en">Relates a resource to details of a groove width of an analog disc or a groove pitch of an analog cylinder.</skos:definition>
  <rdfs:subPropertyOf rdf:resource="http://rdaregistry.info/Elements/u/P60796" />
</owl:ObjectProperty>

<!-- Property: has details of illustrative content -->
<owl:ObjectProperty rdf:about="http://rdaregistry.info/Elements/u/P60804">
  <rdfs:isDefinedBy rdf:resource="http://rdaregistry.info/Elements/u/" />
  <reg:status rdf:resource="http://metadataregistry.org/uri/RegStatus/1001" />
  <rdf:type rdf:resource="http://www.w3.org/1999/02/22-rdf-syntax-ns#Property" />
  <reg:name xml:lang="en">detailsOfIllustrativeContent</reg:name>
  <rdfs:label xml:lang="en">has details of illustrative content</rdfs:label>
  <reg:lexicalAlias rdf:resource="http://rdaregistry.info/Elements/u/detailsOfIllustrativeContent.en" />
  <skos:definition xml:lang="en">Relates a resource to details of content intended to illustrate a primary content of a resource.</skos:definition>
  <skos:definition xml:lang="en">Relates a resource to details of a presence of one or more still images that accompany the primary content of a resource.</skos:definition>
</owl:ObjectProperty>

<!-- Property: has details of layout -->
<owl:ObjectProperty rdf:about="http://rdaregistry.info/Elements/u/P60784">
  <rdfs:isDefinedBy rdf:resource="http://rdaregistry.info/Elements/u/" />
  <reg:status rdf:resource="http://metadataregistry.org/uri/RegStatus/1001" />
  <rdf:type rdf:resource="http://www.w3.org/1999/02/22-rdf-syntax-ns#Property" />
  <reg:name xml:lang="en">detailsOfLayout</reg:name>
  <rdfs:label xml:lang="en">has details of layout</rdfs:label>
  <reg:lexicalAlias rdf:resource="http://rdaregistry.info/Elements/u/detailsOfLayout.en" />
  <skos:definition xml:lang="en">Relates a resource to details of an arrangement of text, images, tactile notation, etc., in a resource.</skos:definition>
</owl:ObjectProperty>

<!-- Property: has details of mount -->
<owl:ObjectProperty rdf:about="http://rdaregistry.info/Elements/u/P60785">
  <rdfs:isDefinedBy rdf:resource="http://rdaregistry.info/Elements/u/" />
  <reg:status rdf:resource="http://metadataregistry.org/uri/RegStatus/1001" />
  <rdf:type rdf:resource="http://www.w3.org/1999/02/22-rdf-syntax-ns#Property" />
  <reg:name xml:lang="en">detailsOfMount</reg:name>
  <rdfs:label xml:lang="en">has details of mount</rdfs:label>
  <reg:lexicalAlias rdf:resource="http://rdaregistry.info/Elements/u/detailsOfMount.en" />
  <skos:definition xml:lang="en">Relates a resource to details of a physical material used for the support or backing to which the base material of a resource has been attached.</skos:definition>
</owl:ObjectProperty>

<!-- Property: has details of playing speed -->
<owl:ObjectProperty rdf:about="http://rdaregistry.info/Elements/u/P60786">
  <rdfs:isDefinedBy rdf:resource="http://rdaregistry.info/Elements/u/" />
  <reg:status rdf:resource="http://metadataregistry.org/uri/RegStatus/1001" />
  <rdf:type rdf:resource="http://www.w3.org/1999/02/22-rdf-syntax-ns#Property" />
  <reg:name xml:lang="en">detailsOfPlayingSpeed</reg:name>
  <rdfs:label xml:lang="en">has details of playing speed</rdfs:label>
  <reg:lexicalAlias rdf:resource="http://rdaregistry.info/Elements/u/detailsOfPlayingSpeed.en" />
  <skos:definition xml:lang="en">Relates a resource to details of a speed at which an audio carrier must be operated to produce the sound intended.</skos:definition>
</owl:ObjectProperty>

<!-- Property: has details of polarity -->
<owl:ObjectProperty rdf:about="http://rdaregistry.info/Elements/u/P60787">
  <rdfs:isDefinedBy rdf:resource="http://rdaregistry.info/Elements/u/" />
  <reg:status rdf:resource="http://metadataregistry.org/uri/RegStatus/1001" />
  <rdf:type rdf:resource="http://www.w3.org/1999/02/22-rdf-syntax-ns#Property" />
  <reg:name xml:lang="en">detailsOfPolarity</reg:name>
  <rdfs:label xml:lang="en">has details of polarity</rdfs:label>
  <reg:lexicalAlias rdf:resource="http://rdaregistry.info/Elements/u/detailsOfPolarity.en" />
  <skos:definition xml:lang="en">Relates a resource to details of a relationship of the colours and tones in an image to the colours and tones of the object reproduced.</skos:definition>
</owl:ObjectProperty>

<!-- Property: has details of presentation format -->
<owl:ObjectProperty rdf:about="http://rdaregistry.info/Elements/u/P60788">
  <rdfs:isDefinedBy rdf:resource="http://rdaregistry.info/Elements/u/" />
  <reg:status rdf:resource="http://metadataregistry.org/uri/RegStatus/1001" />
  <rdf:type rdf:resource="http://www.w3.org/1999/02/22-rdf-syntax-ns#Property" />
  <reg:name xml:lang="en">detailsOfPresentationFormat</reg:name>
  <rdfs:label xml:lang="en">has details of presentation format</rdfs:label>
  <reg:lexicalAlias rdf:resource="http://rdaregistry.info/Elements/u/detailsOfPresentationFormat.en" />
  <skos:definition xml:lang="en">Relates a resource to details of a format used in the production of a projected image.</skos:definition>
</owl:ObjectProperty>

<!-- Property: has details of production method -->
<owl:ObjectProperty rdf:about="http://rdaregistry.info/Elements/u/P60789">
  <rdfs:isDefinedBy rdf:resource="http://rdaregistry.info/Elements/u/" />
  <reg:status rdf:resource="http://metadataregistry.org/uri/RegStatus/1001" />
  <rdf:type rdf:resource="http://www.w3.org/1999/02/22-rdf-syntax-ns#Property" />
  <reg:name xml:lang="en">detailsOfProductionMethod</reg:name>
  <rdfs:label xml:lang="en">has details of production method</rdfs:label>
  <reg:lexicalAlias rdf:resource="http://rdaregistry.info/Elements/u/detailsOfProductionMethod.en" />
  <skos:definition xml:lang="en">Relates a resource to details of a process used to produce a resource.</skos:definition>
</owl:ObjectProperty>

<!-- Property: DEPRECATED -->
<owl:ObjectProperty rdf:about="http://rdaregistry.info/Elements/u/P60790">
  <rdfs:isDefinedBy rdf:resource="http://rdaregistry.info/Elements/u/" />
  <reg:status rdf:resource="http://metadataregistry.org/uri/RegStatus/1008" />
  <rdf:type rdf:resource="http://www.w3.org/1999/02/22-rdf-syntax-ns#Property" />
  <reg:name xml:lang="en">detailsOfProductionMethodForManuscript</reg:name>
  <reg:lexicalAlias rdf:resource="http://rdaregistry.info/Elements/u/detailsOfProductionMethodForManuscript.en" />
</owl:ObjectProperty>

<!-- Property: DEPRECATED -->
<owl:ObjectProperty rdf:about="http://rdaregistry.info/Elements/u/P60791">
  <rdfs:isDefinedBy rdf:resource="http://rdaregistry.info/Elements/u/" />
  <reg:status rdf:resource="http://metadataregistry.org/uri/RegStatus/1008" />
  <rdf:type rdf:resource="http://www.w3.org/1999/02/22-rdf-syntax-ns#Property" />
  <reg:name xml:lang="en">detailsOfProductionMethodForTactileResource</reg:name>
  <reg:lexicalAlias rdf:resource="http://rdaregistry.info/Elements/u/detailsOfProductionMethodForTactileResource.en" />
</owl:ObjectProperty>

<!-- Property: has details of projection characteristic of motion picture film -->
<owl:ObjectProperty rdf:about="http://rdaregistry.info/Elements/u/P60792">
  <rdfs:isDefinedBy rdf:resource="http://rdaregistry.info/Elements/u/" />
  <reg:status rdf:resource="http://metadataregistry.org/uri/RegStatus/1001" />
  <rdf:type rdf:resource="http://www.w3.org/1999/02/22-rdf-syntax-ns#Property" />
  <reg:name xml:lang="en">detailsOfProjectionCharacteristicOfMotionPictureFilm</reg:name>
  <rdfs:label xml:lang="en">has details of projection characteristic of motion picture film</rdfs:label>
  <reg:lexicalAlias rdf:resource="http://rdaregistry.info/Elements/u/detailsOfProjectionCharacteristicOfMotionPictureFilm.en" />
  <skos:definition xml:lang="en">Relates a resource to details of a technical specification relating to the projection of a motion picture film.</skos:definition>
  <reg:hasSubproperty rdf:resource="http://rdaregistry.info/Elements/u/P60793" />
</owl:ObjectProperty>

<!-- Property: has details of projection speed -->
<owl:ObjectProperty rdf:about="http://rdaregistry.info/Elements/u/P60793">
  <rdfs:isDefinedBy rdf:resource="http://rdaregistry.info/Elements/u/" />
  <reg:status rdf:resource="http://metadataregistry.org/uri/RegStatus/1001" />
  <rdf:type rdf:resource="http://www.w3.org/1999/02/22-rdf-syntax-ns#Property" />
  <reg:name xml:lang="en">detailsOfProjectionSpeed</reg:name>
  <rdfs:label xml:lang="en">has details of projection speed</rdfs:label>
  <reg:lexicalAlias rdf:resource="http://rdaregistry.info/Elements/u/detailsOfProjectionSpeed.en" />
  <skos:definition xml:lang="en">Relates a resource to details of a speed at which a projected carrier must be operated to produce the moving image intended.</skos:definition>
  <rdfs:subPropertyOf rdf:resource="http://rdaregistry.info/Elements/u/P60792" />
</owl:ObjectProperty>

<!-- Property: has details of recording medium -->
<owl:ObjectProperty rdf:about="http://rdaregistry.info/Elements/u/P60794">
  <rdfs:isDefinedBy rdf:resource="http://rdaregistry.info/Elements/u/" />
  <reg:status rdf:resource="http://metadataregistry.org/uri/RegStatus/1001" />
  <rdf:type rdf:resource="http://www.w3.org/1999/02/22-rdf-syntax-ns#Property" />
  <reg:name xml:lang="en">detailsOfRecordingMedium</reg:name>
  <rdfs:label xml:lang="en">has details of recording medium</rdfs:label>
  <reg:lexicalAlias rdf:resource="http://rdaregistry.info/Elements/u/detailsOfRecordingMedium.en" />
  <skos:definition xml:lang="en">Relates a resource to details of a type of medium used to record sound on an audio carrier.</skos:definition>
  <rdfs:subPropertyOf rdf:resource="http://rdaregistry.info/Elements/u/P60796" />
</owl:ObjectProperty>

<!-- Property: has details of reduction ratio designation -->
<owl:ObjectProperty rdf:about="http://rdaregistry.info/Elements/u/P60795">
  <rdfs:isDefinedBy rdf:resource="http://rdaregistry.info/Elements/u/" />
  <reg:status rdf:resource="http://metadataregistry.org/uri/RegStatus/1001" />
  <rdf:type rdf:resource="http://www.w3.org/1999/02/22-rdf-syntax-ns#Property" />
  <reg:name xml:lang="en">detailsOfReductionRatioDesignation</reg:name>
  <rdfs:label xml:lang="en">has details of reduction ratio designation</rdfs:label>
  <reg:lexicalAlias rdf:resource="http://rdaregistry.info/Elements/u/detailsOfReductionRatioDesignation.en" />
  <skos:definition xml:lang="en">Relates a resource to details of a designation of the size of a micro-image to an original from which it was produced.</skos:definition>
</owl:ObjectProperty>

<!-- Property: has details of script -->
<owl:ObjectProperty rdf:about="http://rdaregistry.info/Elements/u/P60766">
  <rdfs:isDefinedBy rdf:resource="http://rdaregistry.info/Elements/u/" />
  <reg:status rdf:resource="http://metadataregistry.org/uri/RegStatus/1001" />
  <rdf:type rdf:resource="http://www.w3.org/1999/02/22-rdf-syntax-ns#Property" />
  <reg:name xml:lang="en">detailsOfScript</reg:name>
  <rdfs:label xml:lang="en">has details of script</rdfs:label>
  <reg:lexicalAlias rdf:resource="http://rdaregistry.info/Elements/u/detailsOfScript.en" />
  <skos:definition xml:lang="en">Relates a resource to details of set of characters or symbols used to express written language content of a resource.</skos:definition>
</owl:ObjectProperty>

<!-- Property: has details of sound characteristic -->
<owl:ObjectProperty rdf:about="http://rdaregistry.info/Elements/u/P60796">
  <rdfs:isDefinedBy rdf:resource="http://rdaregistry.info/Elements/u/" />
  <reg:status rdf:resource="http://metadataregistry.org/uri/RegStatus/1001" />
  <rdf:type rdf:resource="http://www.w3.org/1999/02/22-rdf-syntax-ns#Property" />
  <reg:name xml:lang="en">detailsOfSoundCharacteristic</reg:name>
  <rdfs:label xml:lang="en">has details of sound characteristic</rdfs:label>
  <reg:lexicalAlias rdf:resource="http://rdaregistry.info/Elements/u/detailsOfSoundCharacteristic.en" />
  <skos:definition xml:lang="en">Relates a resource to details of a technical specification relating to the encoding of sound in a resource.</skos:definition>
  <reg:hasSubproperty rdf:resource="http://rdaregistry.info/Elements/u/P60771" />
  <reg:hasSubproperty rdf:resource="http://rdaregistry.info/Elements/u/P60783" />
  <reg:hasSubproperty rdf:resource="http://rdaregistry.info/Elements/u/P60794" />
  <reg:hasSubproperty rdf:resource="http://rdaregistry.info/Elements/u/P60797" />
  <reg:hasSubproperty rdf:resource="http://rdaregistry.info/Elements/u/P60798" />
  <reg:hasSubproperty rdf:resource="http://rdaregistry.info/Elements/u/P60799" />
  <reg:hasSubproperty rdf:resource="http://rdaregistry.info/Elements/u/P60800" />
</owl:ObjectProperty>

<!-- Property: has details of special playback characteristic -->
<owl:ObjectProperty rdf:about="http://rdaregistry.info/Elements/u/P60797">
  <rdfs:isDefinedBy rdf:resource="http://rdaregistry.info/Elements/u/" />
  <reg:status rdf:resource="http://metadataregistry.org/uri/RegStatus/1001" />
  <rdf:type rdf:resource="http://www.w3.org/1999/02/22-rdf-syntax-ns#Property" />
  <reg:name xml:lang="en">detailsOfSpecialPlaybackCharacteristic</reg:name>
  <rdfs:label xml:lang="en">has details of special playback characteristic</rdfs:label>
  <reg:lexicalAlias rdf:resource="http://rdaregistry.info/Elements/u/detailsOfSpecialPlaybackCharacteristic.en" />
  <skos:definition xml:lang="en">Relates a resource to details of an equalization system, noise reduction system, etc., used in making an audio recording.</skos:definition>
  <rdfs:subPropertyOf rdf:resource="http://rdaregistry.info/Elements/u/P60796" />
</owl:ObjectProperty>

<!-- Property: has details of tape configuration -->
<owl:ObjectProperty rdf:about="http://rdaregistry.info/Elements/u/P60798">
  <rdfs:isDefinedBy rdf:resource="http://rdaregistry.info/Elements/u/" />
  <reg:status rdf:resource="http://metadataregistry.org/uri/RegStatus/1001" />
  <rdf:type rdf:resource="http://www.w3.org/1999/02/22-rdf-syntax-ns#Property" />
  <reg:name xml:lang="en">detailsOfTapeConfiguration</reg:name>
  <rdfs:label xml:lang="en">has details of tape configuration</rdfs:label>
  <reg:lexicalAlias rdf:resource="http://rdaregistry.info/Elements/u/detailsOfTapeConfiguration.en" />
  <skos:definition xml:lang="en">Relates a resource to details of a number of tracks on an audiotape.</skos:definition>
  <rdfs:subPropertyOf rdf:resource="http://rdaregistry.info/Elements/u/P60796" />
</owl:ObjectProperty>

<!-- Property: has details of track configuration -->
<owl:ObjectProperty rdf:about="http://rdaregistry.info/Elements/u/P60799">
  <rdfs:isDefinedBy rdf:resource="http://rdaregistry.info/Elements/u/" />
  <reg:status rdf:resource="http://metadataregistry.org/uri/RegStatus/1001" />
  <rdf:type rdf:resource="http://www.w3.org/1999/02/22-rdf-syntax-ns#Property" />
  <reg:name xml:lang="en">detailsOfTrackConfiguration</reg:name>
  <rdfs:label xml:lang="en">has details of track configuration</rdfs:label>
  <reg:lexicalAlias rdf:resource="http://rdaregistry.info/Elements/u/detailsOfTrackConfiguration.en" />
  <skos:definition xml:lang="en">Relates a resource to details of a configuration of the audio track on a sound-track film.</skos:definition>
  <rdfs:subPropertyOf rdf:resource="http://rdaregistry.info/Elements/u/P60796" />
</owl:ObjectProperty>

<!-- Property: has details of type of recording -->
<owl:ObjectProperty rdf:about="http://rdaregistry.info/Elements/u/P60800">
  <rdfs:isDefinedBy rdf:resource="http://rdaregistry.info/Elements/u/" />
  <reg:status rdf:resource="http://metadataregistry.org/uri/RegStatus/1001" />
  <rdf:type rdf:resource="http://www.w3.org/1999/02/22-rdf-syntax-ns#Property" />
  <reg:name xml:lang="en">detailsOfTypeOfRecording</reg:name>
  <rdfs:label xml:lang="en">has details of type of recording</rdfs:label>
  <reg:lexicalAlias rdf:resource="http://rdaregistry.info/Elements/u/detailsOfTypeOfRecording.en" />
  <skos:definition xml:lang="en">Relates a resource to details of a method used to encode audio content for playback.</skos:definition>
  <rdfs:subPropertyOf rdf:resource="http://rdaregistry.info/Elements/u/P60796" />
</owl:ObjectProperty>

<!-- Property: has details of video characteristic -->
<owl:ObjectProperty rdf:about="http://rdaregistry.info/Elements/u/P60801">
  <rdfs:isDefinedBy rdf:resource="http://rdaregistry.info/Elements/u/" />
  <reg:status rdf:resource="http://metadataregistry.org/uri/RegStatus/1001" />
  <rdf:type rdf:resource="http://www.w3.org/1999/02/22-rdf-syntax-ns#Property" />
  <reg:name xml:lang="en">detailsOfVideoCharacteristic</reg:name>
  <rdfs:label xml:lang="en">has details of video characteristic</rdfs:label>
  <reg:lexicalAlias rdf:resource="http://rdaregistry.info/Elements/u/detailsOfVideoCharacteristic.en" />
  <skos:definition xml:lang="en">Relates a resource to details of a technical specification relating to an encoding of video images in a resource.</skos:definition>
  <reg:hasSubproperty rdf:resource="http://rdaregistry.info/Elements/u/P60770" />
  <reg:hasSubproperty rdf:resource="http://rdaregistry.info/Elements/u/P60802" />
</owl:ObjectProperty>

<!-- Property: has details of video format -->
<owl:ObjectProperty rdf:about="http://rdaregistry.info/Elements/u/P60802">
  <rdfs:isDefinedBy rdf:resource="http://rdaregistry.info/Elements/u/" />
  <reg:status rdf:resource="http://metadataregistry.org/uri/RegStatus/1001" />
  <rdf:type rdf:resource="http://www.w3.org/1999/02/22-rdf-syntax-ns#Property" />
  <reg:name xml:lang="en">detailsOfVideoFormat</reg:name>
  <rdfs:label xml:lang="en">has details of video format</rdfs:label>
  <reg:lexicalAlias rdf:resource="http://rdaregistry.info/Elements/u/detailsOfVideoFormat.en" />
  <skos:definition xml:lang="en">Relates a resource to details of a standard, etc., used to encode the analog video content of a resource.</skos:definition>
  <rdfs:subPropertyOf rdf:resource="http://rdaregistry.info/Elements/u/P60801" />
</owl:ObjectProperty>

<!-- Property: is digested as -->
<owl:ObjectProperty rdf:about="http://rdaregistry.info/Elements/u/P60279">
  <rdfs:isDefinedBy rdf:resource="http://rdaregistry.info/Elements/u/" />
  <reg:status rdf:resource="http://metadataregistry.org/uri/RegStatus/1001" />
  <reg:name xml:lang="en">digestedAs</reg:name>
  <rdfs:label xml:lang="en">is digested as</rdfs:label>
  <skos:definition xml:lang="en">Relates a resource to a resource that systematically and comprehensively condenses a source resource.</skos:definition>
  <rdf:type rdf:resource="http://www.w3.org/1999/02/22-rdf-syntax-ns#Property" />
  <rdfs:subPropertyOf rdf:resource="http://rdaregistry.info/Elements/u/P60250" />
  <owl:inverseOf rdf:resource="http://rdaregistry.info/Elements/u/P60238" />
  <reg:hasSubproperty rdf:resource="http://rdaregistry.info/Elements/e/P20170" />
  <reg:lexicalAlias rdf:resource="http://rdaregistry.info/Elements/u/digestedAs.en" />
</owl:ObjectProperty>

<!-- Property: is digest of -->
<owl:ObjectProperty rdf:about="http://rdaregistry.info/Elements/u/P60238">
  <rdfs:isDefinedBy rdf:resource="http://rdaregistry.info/Elements/u/" />
  <reg:status rdf:resource="http://metadataregistry.org/uri/RegStatus/1001" />
  <reg:name xml:lang="en">digestOf</reg:name>
  <rdfs:label xml:lang="en">is digest of</rdfs:label>
  <skos:definition xml:lang="en">Relates a resource to a resource that has been digested, i.e., systematically and comprehensively condensed.</skos:definition>
  <rdf:type rdf:resource="http://www.w3.org/1999/02/22-rdf-syntax-ns#Property" />
  <rdfs:subPropertyOf rdf:resource="http://rdaregistry.info/Elements/u/P60305" />
  <owl:inverseOf rdf:resource="http://rdaregistry.info/Elements/u/P60279" />
  <reg:hasSubproperty rdf:resource="http://rdaregistry.info/Elements/e/P20135" />
  <reg:lexicalAlias rdf:resource="http://rdaregistry.info/Elements/u/digestOf.en" />
</owl:ObjectProperty>

<!-- Property: has digital file characteristic -->
<owl:ObjectProperty rdf:about="http://rdaregistry.info/Elements/u/P60350">
  <rdfs:isDefinedBy rdf:resource="http://rdaregistry.info/Elements/u/" />
  <reg:status rdf:resource="http://metadataregistry.org/uri/RegStatus/1001" />
  <reg:name xml:lang="en">digitalFileCharacteristic</reg:name>
  <rdfs:label xml:lang="en">has digital file characteristic</rdfs:label>
  <skos:definition xml:lang="en">Relates a resource to a technical specification relating to a digital encoding of text, image, audio, video, and other types of data in a resource.</skos:definition>
  <rdf:type rdf:resource="http://www.w3.org/1999/02/22-rdf-syntax-ns#Property" />
  <reg:hasSubproperty rdf:resource="http://rdaregistry.info/Elements/u/P60059" />
  <reg:hasSubproperty rdf:resource="http://rdaregistry.info/Elements/u/P60093" />
  <reg:hasSubproperty rdf:resource="http://rdaregistry.info/Elements/u/P60314" />
  <reg:hasSubproperty rdf:resource="http://rdaregistry.info/Elements/u/P60323" />
  <reg:hasSubproperty rdf:resource="http://rdaregistry.info/Elements/u/P60519" />
  <reg:hasSubproperty rdf:resource="http://rdaregistry.info/Elements/u/P60551" />
  <reg:hasSubproperty rdf:resource="http://rdaregistry.info/Elements/u/P60587" />
  <reg:hasSubproperty rdf:resource="http://rdaregistry.info/Elements/m/P30124" />
  <reg:lexicalAlias rdf:resource="http://rdaregistry.info/Elements/u/digitalFileCharacteristic.en" />
</owl:ObjectProperty>

<!-- Property: has digital representation of cartographic content -->
<owl:ObjectProperty rdf:about="http://rdaregistry.info/Elements/u/P60323">
  <rdfs:isDefinedBy rdf:resource="http://rdaregistry.info/Elements/u/" />
  <reg:status rdf:resource="http://metadataregistry.org/uri/RegStatus/1001" />
  <reg:name xml:lang="en">digitalRepresentationOfCartographicContent</reg:name>
  <rdfs:label xml:lang="en">has digital representation of cartographic content</rdfs:label>
  <skos:definition xml:lang="en">Relates a resource to a set of technical details relating to an encoding of geospatial information in a cartographic resource.</skos:definition>
  <rdf:type rdf:resource="http://www.w3.org/1999/02/22-rdf-syntax-ns#Property" />
  <rdfs:subPropertyOf rdf:resource="http://rdaregistry.info/Elements/u/P60350" />
  <reg:hasSubproperty rdf:resource="http://rdaregistry.info/Elements/m/P30102" />
  <reg:lexicalAlias rdf:resource="http://rdaregistry.info/Elements/u/digitalRepresentationOfCartographicContent.en" />
</owl:ObjectProperty>

<!-- Property: has digital transfer -->
<owl:ObjectProperty rdf:about="http://rdaregistry.info/Elements/u/P60200">
  <rdfs:isDefinedBy rdf:resource="http://rdaregistry.info/Elements/u/" />
  <reg:status rdf:resource="http://metadataregistry.org/uri/RegStatus/1001" />
  <reg:name xml:lang="en">digitalTransfer</reg:name>
  <rdfs:label xml:lang="en">has digital transfer</rdfs:label>
  <skos:definition xml:lang="en">Relates a resource to a resource in a digital format that results from a transfer of a resource in another digital format.</skos:definition>
  <rdf:type rdf:resource="http://www.w3.org/1999/02/22-rdf-syntax-ns#Property" />
  <rdfs:subPropertyOf rdf:resource="http://rdaregistry.info/Elements/u/P60272" />
  <owl:inverseOf rdf:resource="http://rdaregistry.info/Elements/u/P60287" />
  <reg:hasSubproperty rdf:resource="http://rdaregistry.info/Elements/i/P40056" />
  <reg:hasSubproperty rdf:resource="http://rdaregistry.info/Elements/m/P30029" />
  <reg:lexicalAlias rdf:resource="http://rdaregistry.info/Elements/u/digitalTransfer.en" />
</owl:ObjectProperty>

<!-- Property: is digital transfer of -->
<owl:ObjectProperty rdf:about="http://rdaregistry.info/Elements/u/P60287">
  <rdfs:isDefinedBy rdf:resource="http://rdaregistry.info/Elements/u/" />
  <reg:status rdf:resource="http://metadataregistry.org/uri/RegStatus/1001" />
  <reg:name xml:lang="en">digitalTransferOf</reg:name>
  <rdfs:label xml:lang="en">is digital transfer of</rdfs:label>
  <skos:definition xml:lang="en">Relates a resource to a resource in a digital format that is transferred to another digital format.</skos:definition>
  <rdf:type rdf:resource="http://www.w3.org/1999/02/22-rdf-syntax-ns#Property" />
  <rdfs:subPropertyOf rdf:resource="http://rdaregistry.info/Elements/u/P60297" />
  <owl:inverseOf rdf:resource="http://rdaregistry.info/Elements/u/P60200" />
  <reg:hasSubproperty rdf:resource="http://rdaregistry.info/Elements/i/P40039" />
  <reg:hasSubproperty rdf:resource="http://rdaregistry.info/Elements/m/P30040" />
  <reg:lexicalAlias rdf:resource="http://rdaregistry.info/Elements/u/digitalTransferOf.en" />
</owl:ObjectProperty>

<!-- Property: has dimensions -->
<owl:ObjectProperty rdf:about="http://rdaregistry.info/Elements/u/P60539">
  <rdfs:isDefinedBy rdf:resource="http://rdaregistry.info/Elements/u/" />
  <reg:status rdf:resource="http://metadataregistry.org/uri/RegStatus/1001" />
  <reg:name xml:lang="en">dimensions</reg:name>
  <rdfs:label xml:lang="en">has dimensions</rdfs:label>
  <skos:definition xml:lang="en">Relates a resource to a measurement of a carrier or a container of a resource.</skos:definition>
  <rdf:type rdf:resource="http://www.w3.org/1999/02/22-rdf-syntax-ns#Property" />
  <reg:hasSubproperty rdf:resource="http://rdaregistry.info/Elements/u/P60540" />
  <reg:hasSubproperty rdf:resource="http://rdaregistry.info/Elements/u/P60541" />
  <reg:hasSubproperty rdf:resource="http://rdaregistry.info/Elements/m/P30169" />
  <reg:lexicalAlias rdf:resource="http://rdaregistry.info/Elements/u/dimensions.en" />
</owl:ObjectProperty>

<!-- Property: has dimensions of map, etc. -->
<owl:ObjectProperty rdf:about="http://rdaregistry.info/Elements/u/P60540">
  <rdfs:isDefinedBy rdf:resource="http://rdaregistry.info/Elements/u/" />
  <reg:status rdf:resource="http://metadataregistry.org/uri/RegStatus/1001" />
  <reg:name xml:lang="en">dimensionsOfMapEtc</reg:name>
  <rdfs:label xml:lang="en">has dimensions of map, etc.</rdfs:label>
  <skos:definition xml:lang="en">Relates a resource to a measurement of a face of a map, etc.</skos:definition>
  <rdf:type rdf:resource="http://www.w3.org/1999/02/22-rdf-syntax-ns#Property" />
  <rdfs:subPropertyOf rdf:resource="http://rdaregistry.info/Elements/u/P60539" />
  <reg:hasSubproperty rdf:resource="http://rdaregistry.info/Elements/m/P30170" />
  <reg:lexicalAlias rdf:resource="http://rdaregistry.info/Elements/u/dimensionsOfMapEtc.en" />
</owl:ObjectProperty>

<!-- Property: has dimensions of still image -->
<owl:ObjectProperty rdf:about="http://rdaregistry.info/Elements/u/P60541">
  <rdfs:isDefinedBy rdf:resource="http://rdaregistry.info/Elements/u/" />
  <reg:status rdf:resource="http://metadataregistry.org/uri/RegStatus/1001" />
  <reg:name xml:lang="en">dimensionsOfStillImage</reg:name>
  <rdfs:label xml:lang="en">has dimensions of still image</rdfs:label>
  <skos:definition xml:lang="en">Relates a resource to a measurement of the pictorial area of a still image.</skos:definition>
  <rdf:type rdf:resource="http://www.w3.org/1999/02/22-rdf-syntax-ns#Property" />
  <rdfs:subPropertyOf rdf:resource="http://rdaregistry.info/Elements/u/P60539" />
  <reg:hasSubproperty rdf:resource="http://rdaregistry.info/Elements/m/P30171" />
  <reg:lexicalAlias rdf:resource="http://rdaregistry.info/Elements/u/dimensionsOfStillImage.en" />
</owl:ObjectProperty>

<!-- Property: has director -->
<owl:ObjectProperty rdf:about="http://rdaregistry.info/Elements/u/P60449">
  <rdfs:isDefinedBy rdf:resource="http://rdaregistry.info/Elements/u/" />
  <reg:status rdf:resource="http://metadataregistry.org/uri/RegStatus/1001" />
  <reg:name xml:lang="en">director</reg:name>
  <rdfs:label xml:lang="en">has director</rdfs:label>
  <skos:definition xml:lang="en">Relates a resource to an agent responsible for the general management and supervision of a filmed performance, a radio or television program, etc.</skos:definition>
  <rdf:type rdf:resource="http://www.w3.org/1999/02/22-rdf-syntax-ns#Property" />
  <rdfs:subPropertyOf rdf:resource="http://rdaregistry.info/Elements/u/P60374" />
  <owl:inverseOf rdf:resource="http://rdaregistry.info/Elements/u/P60452" />
  <reg:hasSubproperty rdf:resource="http://rdaregistry.info/Elements/u/P60084" />
  <reg:hasSubproperty rdf:resource="http://rdaregistry.info/Elements/u/P60085" />
  <reg:hasSubproperty rdf:resource="http://rdaregistry.info/Elements/u/P60086" />
  <reg:lexicalAlias rdf:resource="http://rdaregistry.info/Elements/u/director.en" />
</owl:ObjectProperty>

<!-- Property: is director of -->
<owl:ObjectProperty rdf:about="http://rdaregistry.info/Elements/u/P60673">
  <rdfs:isDefinedBy rdf:resource="http://rdaregistry.info/Elements/u/" />
  <reg:status rdf:resource="http://metadataregistry.org/uri/RegStatus/1001" />
  <reg:name xml:lang="en">directorOf</reg:name>
  <rdfs:label xml:lang="en">is director of</rdfs:label>
  <skos:definition xml:lang="en">Relates an agent responsible for the general management and supervision of a filmed performance, a radio or television program, etc. to a resource.</skos:definition>
  <rdf:type rdf:resource="http://www.w3.org/1999/02/22-rdf-syntax-ns#Property" />
  <rdfs:subPropertyOf rdf:resource="http://rdaregistry.info/Elements/u/P60602" />
  <owl:inverseOf rdf:resource="http://rdaregistry.info/Elements/u/P60449" />
  <reg:hasSubproperty rdf:resource="http://rdaregistry.info/Elements/a/P50205" />
  <reg:lexicalAlias rdf:resource="http://rdaregistry.info/Elements/u/directorOf.en" />
</owl:ObjectProperty>

<!-- Property: has director of photography -->
<owl:ObjectProperty rdf:about="http://rdaregistry.info/Elements/u/P60452">
  <rdfs:isDefinedBy rdf:resource="http://rdaregistry.info/Elements/u/" />
  <reg:status rdf:resource="http://metadataregistry.org/uri/RegStatus/1001" />
  <reg:name xml:lang="en">directorOfPhotography</reg:name>
  <rdfs:label xml:lang="en">has director of photography</rdfs:label>
  <skos:definition xml:lang="en">Relates a resource to an agent that captures images, either electronically or on film or video stock, and often selects and arranges lighting. a director of photography for a movie is also called a chief cinematographer.</skos:definition>
  <rdf:type rdf:resource="http://www.w3.org/1999/02/22-rdf-syntax-ns#Property" />
  <rdfs:subPropertyOf rdf:resource="http://rdaregistry.info/Elements/u/P60374" />
  <owl:inverseOf rdf:resource="http://rdaregistry.info/Elements/u/P60678" />
  <reg:lexicalAlias rdf:resource="http://rdaregistry.info/Elements/u/directorOfPhotography.en" />
  <reg:hasSubproperty rdf:resource="http://rdaregistry.info/Elements/u/P60009" />
  <reg:hasSubproperty rdf:resource="http://rdaregistry.info/Elements/u/P60010" />
  <reg:hasSubproperty rdf:resource="http://rdaregistry.info/Elements/u/P60011" />
</owl:ObjectProperty>

<!-- Property: is director of photography of -->
<owl:ObjectProperty rdf:about="http://rdaregistry.info/Elements/u/P60678">
  <rdfs:isDefinedBy rdf:resource="http://rdaregistry.info/Elements/u/" />
  <reg:status rdf:resource="http://metadataregistry.org/uri/RegStatus/1001" />
  <reg:name xml:lang="en">directorOfPhotographyOf</reg:name>
  <rdfs:label xml:lang="en">is director of photography of</rdfs:label>
  <skos:definition xml:lang="en">Relates an agent that captures images, either electronically or on film or video stock, and often selects and arranges lighting. a director of photography for a movie is also called a chief cinematographer to a resource.</skos:definition>
  <rdf:type rdf:resource="http://www.w3.org/1999/02/22-rdf-syntax-ns#Property" />
  <rdfs:subPropertyOf rdf:resource="http://rdaregistry.info/Elements/u/P60602" />
  <owl:inverseOf rdf:resource="http://rdaregistry.info/Elements/u/P60452" />
  <reg:hasSubproperty rdf:resource="http://rdaregistry.info/Elements/a/P50207" />
  <reg:lexicalAlias rdf:resource="http://rdaregistry.info/Elements/u/directorOfPhotographyOf.en" />
</owl:ObjectProperty>

<!-- Property: has dissertation or thesis information -->
<owl:ObjectProperty rdf:about="http://rdaregistry.info/Elements/u/P60489">
  <rdfs:isDefinedBy rdf:resource="http://rdaregistry.info/Elements/u/" />
  <reg:status rdf:resource="http://metadataregistry.org/uri/RegStatus/1001" />
  <reg:name xml:lang="en">dissertationOrThesisInformation</reg:name>
  <rdfs:label xml:lang="en">has dissertation or thesis information</rdfs:label>
  <skos:definition xml:lang="en">Relates a resource to a statement identifying an academic institution, degree, and year for which a resource was presented.</skos:definition>
  <rdf:type rdf:resource="http://www.w3.org/1999/02/22-rdf-syntax-ns#Property" />
  <reg:lexicalAlias rdf:resource="http://rdaregistry.info/Elements/u/dissertationOrThesisInformation.en" />
</owl:ObjectProperty>

<!-- Property: has distribution statement -->
<owl:ObjectProperty rdf:about="http://rdaregistry.info/Elements/u/P60330">
  <rdfs:isDefinedBy rdf:resource="http://rdaregistry.info/Elements/u/" />
  <reg:status rdf:resource="http://metadataregistry.org/uri/RegStatus/1001" />
  <reg:name xml:lang="en">distributionStatement</reg:name>
  <rdfs:label xml:lang="en">has distribution statement</rdfs:label>
  <skos:definition xml:lang="en">Relates a resource to a statement identifying a place or places of distribution, distributor or distributors, and date or dates of distribution of a resource in a published form.</skos:definition>
  <rdf:type rdf:resource="http://www.w3.org/1999/02/22-rdf-syntax-ns#Property" />
  <reg:hasSubproperty rdf:resource="http://rdaregistry.info/Elements/m/P30108" />
  <reg:lexicalAlias rdf:resource="http://rdaregistry.info/Elements/u/distributionStatement.en" />
</owl:ObjectProperty>

<!-- Property: has distributor -->
<owl:ObjectProperty rdf:about="http://rdaregistry.info/Elements/u/P60438">
  <rdfs:isDefinedBy rdf:resource="http://rdaregistry.info/Elements/u/" />
  <reg:status rdf:resource="http://metadataregistry.org/uri/RegStatus/1001" />
  <reg:name xml:lang="en">distributor</reg:name>
  <rdfs:label xml:lang="en">has distributor</rdfs:label>
  <skos:definition xml:lang="en">Relates a resource to an agent responsible for distributing a resource.</skos:definition>
  <rdf:type rdf:resource="http://www.w3.org/1999/02/22-rdf-syntax-ns#Property" />
  <owl:inverseOf rdf:resource="http://rdaregistry.info/Elements/u/P60667" />
  <reg:hasSubproperty rdf:resource="http://rdaregistry.info/Elements/u/P60408" />
  <reg:hasSubproperty rdf:resource="http://rdaregistry.info/Elements/m/P30080" />
  <reg:lexicalAlias rdf:resource="http://rdaregistry.info/Elements/u/distributor.en" />
</owl:ObjectProperty>

<!-- Property: is distributor of -->
<owl:ObjectProperty rdf:about="http://rdaregistry.info/Elements/u/P60667">
  <rdfs:isDefinedBy rdf:resource="http://rdaregistry.info/Elements/u/" />
  <reg:status rdf:resource="http://metadataregistry.org/uri/RegStatus/1001" />
  <reg:name xml:lang="en">distributorOf</reg:name>
  <rdfs:label xml:lang="en">is distributor of</rdfs:label>
  <skos:definition xml:lang="en">Relates an agent responsible for distributing a resource to a resource.</skos:definition>
  <rdf:type rdf:resource="http://www.w3.org/1999/02/22-rdf-syntax-ns#Property" />
  <owl:inverseOf rdf:resource="http://rdaregistry.info/Elements/u/P60438" />
  <reg:hasSubproperty rdf:resource="http://rdaregistry.info/Elements/u/P60636" />
  <reg:hasSubproperty rdf:resource="http://rdaregistry.info/Elements/a/P50199" />
  <reg:lexicalAlias rdf:resource="http://rdaregistry.info/Elements/u/distributorOf.en" />
</owl:ObjectProperty>

<!-- Property: has distributors name -->
<owl:ObjectProperty rdf:about="http://rdaregistry.info/Elements/u/P60544">
  <rdfs:isDefinedBy rdf:resource="http://rdaregistry.info/Elements/u/" />
  <reg:status rdf:resource="http://metadataregistry.org/uri/RegStatus/1001" />
  <reg:name xml:lang="en">distributorsName</reg:name>
  <rdfs:label xml:lang="en">has distributors name</rdfs:label>
  <skos:definition xml:lang="en">Relates a resource to a name of an agent responsible for distributing a resource in a published form.</skos:definition>
  <rdf:type rdf:resource="http://www.w3.org/1999/02/22-rdf-syntax-ns#Property" />
  <reg:hasSubproperty rdf:resource="http://rdaregistry.info/Elements/m/P30173" />
  <reg:lexicalAlias rdf:resource="http://rdaregistry.info/Elements/u/distributorsName.en" />
</owl:ObjectProperty>

<!-- Property: has DJ -->
<owl:ObjectProperty rdf:about="http://rdaregistry.info/Elements/u/P60896">
  <rdfs:isDefinedBy rdf:resource="http://rdaregistry.info/Elements/u/" />
  <reg:status rdf:resource="http://metadataregistry.org/uri/RegStatus/1001" />
  <rdf:type rdf:resource="http://www.w3.org/1999/02/22-rdf-syntax-ns#Property" />
  <reg:name xml:lang="en">DJ</reg:name>
  <rdfs:label xml:lang="en">has DJ</rdfs:label>
  <reg:lexicalAlias rdf:resource="http://rdaregistry.info/Elements/u/DJ.en" />
  <skos:definition xml:lang="en">Relates a resource to an agent who mixes recorded tracks together during a live performance or in a recording studio to appear as one continuous track.</skos:definition>
  <skos:scopeNote xml:lang="en">Remixing activities that substantially change the nature and content of the original resource, resulting in a new resource, and mixing and assembling the multiple tracks of a recording are excluded.</skos:scopeNote>
  <owl:inverseOf rdf:resource="http://rdaregistry.info/Elements/u/P60886" />
  <reg:hasSubproperty rdf:resource="http://rdaregistry.info/Elements/e/P20296" />
  <rdfs:subPropertyOf rdf:resource="http://rdaregistry.info/Elements/u/P60398" />
  <rdakit:seeAlso rdf:resource="http://rdaregistry.info/Elements/u/P60893" />
</owl:ObjectProperty>

<!-- Property: is DJ of -->
<owl:ObjectProperty rdf:about="http://rdaregistry.info/Elements/u/P60886">
  <rdfs:isDefinedBy rdf:resource="http://rdaregistry.info/Elements/u/" />
  <reg:status rdf:resource="http://metadataregistry.org/uri/RegStatus/1001" />
  <rdf:type rdf:resource="http://www.w3.org/1999/02/22-rdf-syntax-ns#Property" />
  <reg:name xml:lang="en">DJOf</reg:name>
  <rdfs:label xml:lang="en">is DJ of</rdfs:label>
  <reg:lexicalAlias rdf:resource="http://rdaregistry.info/Elements/u/DJOf.en" />
  <skos:definition xml:lang="en">Relates an agent to a resource that incorporates a contribution of mixing recorded tracks together during a live performance or in a recording studio to appear as one continuous track.</skos:definition>
  <skos:scopeNote xml:lang="en">Remixing activities that substantially change the nature and content of the original resource, resulting in a new resource, and mixing and assembling the multiple tracks of a recording are excluded.</skos:scopeNote>
  <owl:inverseOf rdf:resource="http://rdaregistry.info/Elements/u/P60896" />
  <rdfs:subPropertyOf rdf:resource="http://rdaregistry.info/Elements/u/P60158" />
  <reg:hasSubproperty rdf:resource="http://rdaregistry.info/Elements/a/P50298" />
  <rdakit:seeAlso rdf:resource="http://rdaregistry.info/Elements/u/P60885" />
</owl:ObjectProperty>

<!-- Property: has donor -->
<owl:ObjectProperty rdf:about="http://rdaregistry.info/Elements/u/P60091">
  <rdfs:isDefinedBy rdf:resource="http://rdaregistry.info/Elements/u/" />
  <reg:status rdf:resource="http://metadataregistry.org/uri/RegStatus/1001" />
  <reg:name xml:lang="en">donor</reg:name>
  <rdfs:label xml:lang="en">has donor</rdfs:label>
  <skos:definition xml:lang="en">Relates a resource to a former owner of a resource who donated that resource to another owner.</skos:definition>
  <rdf:type rdf:resource="http://www.w3.org/1999/02/22-rdf-syntax-ns#Property" />
  <rdfs:subPropertyOf rdf:resource="http://rdaregistry.info/Elements/u/P60401" />
  <owl:inverseOf rdf:resource="http://rdaregistry.info/Elements/u/P60012" />
  <reg:hasSubproperty rdf:resource="http://rdaregistry.info/Elements/i/P40007" />
  <reg:lexicalAlias rdf:resource="http://rdaregistry.info/Elements/u/donor.en" />
</owl:ObjectProperty>

<!-- Property: is donor of -->
<owl:ObjectProperty rdf:about="http://rdaregistry.info/Elements/u/P60012">
  <rdfs:isDefinedBy rdf:resource="http://rdaregistry.info/Elements/u/" />
  <reg:status rdf:resource="http://metadataregistry.org/uri/RegStatus/1001" />
  <reg:name xml:lang="en">donorOf</reg:name>
  <rdfs:label xml:lang="en">is donor of</rdfs:label>
  <skos:definition xml:lang="en">Relates a former owner of a resource who donated that resource to another owner to a resource.</skos:definition>
  <rdf:type rdf:resource="http://www.w3.org/1999/02/22-rdf-syntax-ns#Property" />
  <rdfs:subPropertyOf rdf:resource="http://rdaregistry.info/Elements/u/P60630" />
  <owl:inverseOf rdf:resource="http://rdaregistry.info/Elements/u/P60091" />
  <reg:hasSubproperty rdf:resource="http://rdaregistry.info/Elements/a/P50066" />
  <reg:lexicalAlias rdf:resource="http://rdaregistry.info/Elements/u/donorOf.en" />
</owl:ObjectProperty>

<!-- Property: has draftsman -->
<owl:ObjectProperty rdf:about="http://rdaregistry.info/Elements/u/P60381">
  <rdfs:isDefinedBy rdf:resource="http://rdaregistry.info/Elements/u/" />
  <reg:status rdf:resource="http://metadataregistry.org/uri/RegStatus/1001" />
  <reg:name xml:lang="en">draftsman</reg:name>
  <rdfs:label xml:lang="en">has draftsman</rdfs:label>
  <skos:definition xml:lang="en">Relates a resource to an agent contributing to a resource by an architect, inventor, etc., by making detailed plans or drawings for buildings, ships, aircraft, machines, objects, etc.</skos:definition>
  <rdf:type rdf:resource="http://www.w3.org/1999/02/22-rdf-syntax-ns#Property" />
  <rdfs:subPropertyOf rdf:resource="http://rdaregistry.info/Elements/u/P60398" />
  <owl:inverseOf rdf:resource="http://rdaregistry.info/Elements/u/P60609" />
  <reg:hasSubproperty rdf:resource="http://rdaregistry.info/Elements/e/P20033" />
  <reg:lexicalAlias rdf:resource="http://rdaregistry.info/Elements/u/draftsman.en" />
</owl:ObjectProperty>

<!-- Property: is draftsman of -->
<owl:ObjectProperty rdf:about="http://rdaregistry.info/Elements/u/P60609">
  <rdfs:isDefinedBy rdf:resource="http://rdaregistry.info/Elements/u/" />
  <reg:status rdf:resource="http://metadataregistry.org/uri/RegStatus/1001" />
  <reg:name xml:lang="en">draftsmanOf</reg:name>
  <rdfs:label xml:lang="en">is draftsman of</rdfs:label>
  <skos:definition xml:lang="en">Relates an agent contributing to a resource by an architect, inventor, etc., by making detailed plans or drawings for buildings, ships, aircraft, machines, objects, etc. to a resource.</skos:definition>
  <rdf:type rdf:resource="http://www.w3.org/1999/02/22-rdf-syntax-ns#Property" />
  <rdfs:subPropertyOf rdf:resource="http://rdaregistry.info/Elements/u/P60626" />
  <owl:inverseOf rdf:resource="http://rdaregistry.info/Elements/u/P60381" />
  <reg:hasSubproperty rdf:resource="http://rdaregistry.info/Elements/a/P50141" />
  <reg:lexicalAlias rdf:resource="http://rdaregistry.info/Elements/u/draftsmanOf.en" />
</owl:ObjectProperty>

<!-- Property: is dramatization of -->
<owl:ObjectProperty rdf:about="http://rdaregistry.info/Elements/u/P60225">
  <rdfs:isDefinedBy rdf:resource="http://rdaregistry.info/Elements/u/" />
  <reg:status rdf:resource="http://metadataregistry.org/uri/RegStatus/1001" />
  <reg:name xml:lang="en">dramatizationOf</reg:name>
  <rdfs:label xml:lang="en">is dramatization of</rdfs:label>
  <skos:definition xml:lang="en">Relates a resource to a resource that has been adapted as a drama.</skos:definition>
  <rdf:type rdf:resource="http://www.w3.org/1999/02/22-rdf-syntax-ns#Property" />
  <rdfs:subPropertyOf rdf:resource="http://rdaregistry.info/Elements/u/P60241" />
  <owl:inverseOf rdf:resource="http://rdaregistry.info/Elements/u/P60088" />
  <reg:hasSubproperty rdf:resource="http://rdaregistry.info/Elements/e/P20123" />
  <reg:lexicalAlias rdf:resource="http://rdaregistry.info/Elements/u/dramatizationOf.en" />
</owl:ObjectProperty>

<!-- Property: is dramatized as -->
<owl:ObjectProperty rdf:about="http://rdaregistry.info/Elements/u/P60088">
  <rdfs:isDefinedBy rdf:resource="http://rdaregistry.info/Elements/u/" />
  <reg:status rdf:resource="http://metadataregistry.org/uri/RegStatus/1001" />
  <reg:name xml:lang="en">dramatizedAs</reg:name>
  <rdfs:label xml:lang="en">is dramatized as</rdfs:label>
  <skos:definition xml:lang="en">Relates a resource to a dramatic resource adapted from a source resource.</skos:definition>
  <rdf:type rdf:resource="http://www.w3.org/1999/02/22-rdf-syntax-ns#Property" />
  <rdfs:subPropertyOf rdf:resource="http://rdaregistry.info/Elements/u/P60260" />
  <owl:inverseOf rdf:resource="http://rdaregistry.info/Elements/u/P60225" />
  <reg:hasSubproperty rdf:resource="http://rdaregistry.info/Elements/e/P20073" />
  <reg:lexicalAlias rdf:resource="http://rdaregistry.info/Elements/u/dramatizedAs.en" />
</owl:ObjectProperty>

<!-- Property: is dubbed version -->
<owl:ObjectProperty rdf:about="http://rdaregistry.info/Elements/u/P60112">
  <rdfs:isDefinedBy rdf:resource="http://rdaregistry.info/Elements/u/" />
  <reg:status rdf:resource="http://metadataregistry.org/uri/RegStatus/1001" />
  <reg:name xml:lang="en">dubbedVersion</reg:name>
  <rdfs:label xml:lang="en">is dubbed version</rdfs:label>
  <skos:definition xml:lang="en">Relates a resource to a moving image resource that translates spoken dialogue of an original resource into a different language.</skos:definition>
  <rdf:type rdf:resource="http://www.w3.org/1999/02/22-rdf-syntax-ns#Property" />
  <rdfs:subPropertyOf rdf:resource="http://rdaregistry.info/Elements/u/P60280" />
  <owl:inverseOf rdf:resource="http://rdaregistry.info/Elements/u/P60111" />
  <reg:hasSubproperty rdf:resource="http://rdaregistry.info/Elements/e/P20079" />
  <reg:lexicalAlias rdf:resource="http://rdaregistry.info/Elements/u/dubbedVersion.en" />
</owl:ObjectProperty>

<!-- Property: is dubbed version of -->
<owl:ObjectProperty rdf:about="http://rdaregistry.info/Elements/u/P60111">
  <rdfs:isDefinedBy rdf:resource="http://rdaregistry.info/Elements/u/" />
  <reg:status rdf:resource="http://metadataregistry.org/uri/RegStatus/1001" />
  <reg:name xml:lang="en">dubbedVersionOf</reg:name>
  <rdfs:label xml:lang="en">is dubbed version of</rdfs:label>
  <skos:definition xml:lang="en">Relates a resource to a moving image resource in which spoken dialogue has been translated into a language different from that of an original resource.</skos:definition>
  <rdf:type rdf:resource="http://www.w3.org/1999/02/22-rdf-syntax-ns#Property" />
  <rdfs:subPropertyOf rdf:resource="http://rdaregistry.info/Elements/u/P60244" />
  <owl:inverseOf rdf:resource="http://rdaregistry.info/Elements/u/P60112" />
  <reg:hasSubproperty rdf:resource="http://rdaregistry.info/Elements/e/P20078" />
  <reg:lexicalAlias rdf:resource="http://rdaregistry.info/Elements/u/dubbedVersionOf.en" />
</owl:ObjectProperty>

<!-- Property: has dubbing director -->
<owl:ObjectProperty rdf:about="http://rdaregistry.info/Elements/u/P60895">
  <rdfs:isDefinedBy rdf:resource="http://rdaregistry.info/Elements/u/" />
  <reg:status rdf:resource="http://metadataregistry.org/uri/RegStatus/1001" />
  <rdf:type rdf:resource="http://www.w3.org/1999/02/22-rdf-syntax-ns#Property" />
  <reg:name xml:lang="en">dubbingDirector</reg:name>
  <rdfs:label xml:lang="en">has dubbing director</rdfs:label>
  <reg:lexicalAlias rdf:resource="http://rdaregistry.info/Elements/u/dubbingDirector.en" />
  <skos:definition xml:lang="en">Relates a resource to an agent responsible for the general management and supervision of the process of adding new dialogue or other sounds to complete a sound track for a resource</skos:definition>
  <owl:inverseOf rdf:resource="http://rdaregistry.info/Elements/u/P60887" />
  <reg:hasSubproperty rdf:resource="http://rdaregistry.info/Elements/e/P20295" />
  <rdfs:subPropertyOf rdf:resource="http://rdaregistry.info/Elements/u/P60398" />
</owl:ObjectProperty>

<!-- Property: is dubbing director of -->
<owl:ObjectProperty rdf:about="http://rdaregistry.info/Elements/u/P60887">
  <rdfs:isDefinedBy rdf:resource="http://rdaregistry.info/Elements/u/" />
  <reg:status rdf:resource="http://metadataregistry.org/uri/RegStatus/1001" />
  <rdf:type rdf:resource="http://www.w3.org/1999/02/22-rdf-syntax-ns#Property" />
  <reg:name xml:lang="en">dubbingDirectorOf</reg:name>
  <rdfs:label xml:lang="en">is dubbing director of</rdfs:label>
  <reg:lexicalAlias rdf:resource="http://rdaregistry.info/Elements/u/dubbingDirectorOf.en" />
  <skos:definition xml:lang="en">Relates an agent to a resource that incorporates a contribution of responsibility for the general management and supervision of the process of adding new dialogue or other sounds to complete a sound track.</skos:definition>
  <owl:inverseOf rdf:resource="http://rdaregistry.info/Elements/u/P60895" />
  <rdfs:subPropertyOf rdf:resource="http://rdaregistry.info/Elements/u/P60158" />
  <reg:hasSubproperty rdf:resource="http://rdaregistry.info/Elements/a/P50299" />
</owl:ObjectProperty>

<!-- Property: has duration -->
<owl:ObjectProperty rdf:about="http://rdaregistry.info/Elements/u/P60557">
  <rdfs:isDefinedBy rdf:resource="http://rdaregistry.info/Elements/u/" />
  <reg:status rdf:resource="http://metadataregistry.org/uri/RegStatus/1001" />
  <reg:name xml:lang="en">duration</reg:name>
  <rdfs:label xml:lang="en">has duration</rdfs:label>
  <skos:definition xml:lang="en">Relates a resource to a playing time, running time, etc., of a content of a resource.</skos:definition>
  <rdf:type rdf:resource="http://www.w3.org/1999/02/22-rdf-syntax-ns#Property" />
  <reg:hasSubproperty rdf:resource="http://rdaregistry.info/Elements/e/P20219" />
  <reg:lexicalAlias rdf:resource="http://rdaregistry.info/Elements/u/duration.en" />
</owl:ObjectProperty>

<!-- Property: has earlier title proper -->
<owl:ObjectProperty rdf:about="http://rdaregistry.info/Elements/u/P60358">
  <rdfs:isDefinedBy rdf:resource="http://rdaregistry.info/Elements/u/" />
  <reg:status rdf:resource="http://metadataregistry.org/uri/RegStatus/1001" />
  <reg:name xml:lang="en">earlierTitleProper</reg:name>
  <rdfs:label xml:lang="en">has earlier title proper</rdfs:label>
  <skos:definition xml:lang="en">Relates a resource to a title proper appearing on an earlier iteration of an integrating resource that differs from that on a current iteration.</skos:definition>
  <rdf:type rdf:resource="http://www.w3.org/1999/02/22-rdf-syntax-ns#Property" />
  <rdfs:subPropertyOf rdf:resource="http://rdaregistry.info/Elements/u/P60369" />
  <reg:hasSubproperty rdf:resource="http://rdaregistry.info/Elements/m/P30130" />
  <reg:lexicalAlias rdf:resource="http://rdaregistry.info/Elements/u/earlierTitleProper.en" />
</owl:ObjectProperty>

<!-- Property: has edition statement -->
<owl:ObjectProperty rdf:about="http://rdaregistry.info/Elements/u/P60329">
  <rdfs:isDefinedBy rdf:resource="http://rdaregistry.info/Elements/u/" />
  <reg:status rdf:resource="http://metadataregistry.org/uri/RegStatus/1001" />
  <reg:name xml:lang="en">editionStatement</reg:name>
  <rdfs:label xml:lang="en">has edition statement</rdfs:label>
  <skos:definition xml:lang="en">Relates a resource to a statement identifying an edition to which a resource belongs.</skos:definition>
  <rdf:type rdf:resource="http://www.w3.org/1999/02/22-rdf-syntax-ns#Property" />
  <reg:hasSubproperty rdf:resource="http://rdaregistry.info/Elements/m/P30107" />
  <reg:lexicalAlias rdf:resource="http://rdaregistry.info/Elements/u/editionStatement.en" />
</owl:ObjectProperty>

<!-- Property: has editor -->
<owl:ObjectProperty rdf:about="http://rdaregistry.info/Elements/u/P60393">
  <rdfs:isDefinedBy rdf:resource="http://rdaregistry.info/Elements/u/" />
  <reg:status rdf:resource="http://metadataregistry.org/uri/RegStatus/1001" />
  <reg:name xml:lang="en">editor</reg:name>
  <rdfs:label xml:lang="en">has editor</rdfs:label>
  <skos:definition xml:lang="en">Relates a resource to an agent contributing to a resource by revising or clarifying the content, or by selecting and putting together resources, or parts of resources, by one or more creators.</skos:definition>
  <rdf:type rdf:resource="http://www.w3.org/1999/02/22-rdf-syntax-ns#Property" />
  <rdfs:subPropertyOf rdf:resource="http://rdaregistry.info/Elements/u/P60398" />
  <owl:inverseOf rdf:resource="http://rdaregistry.info/Elements/u/P60621" />
  <reg:hasSubproperty rdf:resource="http://rdaregistry.info/Elements/e/P20048" />
  <reg:lexicalAlias rdf:resource="http://rdaregistry.info/Elements/u/editor.en" />
  <skos:scopeNote xml:lang="en">Addition of an introduction, notes, or other critical matter, or preparing a resource for production, publication, or distribution is included. Major revision, adaptation, etc., that substantially changes the nature and content of the original resource, resulting in a new resource, is excluded.</skos:scopeNote>
  <rdakit:seeAlso rdf:resource="http://rdaregistry.info/Elements/u/P60434" />
</owl:ObjectProperty>

<!-- Property: has editorial director -->
<owl:ObjectProperty rdf:about="http://rdaregistry.info/Elements/u/P60869">
  <rdfs:isDefinedBy rdf:resource="http://rdaregistry.info/Elements/u/" />
  <reg:status rdf:resource="http://metadataregistry.org/uri/RegStatus/1001" />
  <rdf:type rdf:resource="http://www.w3.org/1999/02/22-rdf-syntax-ns#Property" />
  <reg:name xml:lang="en">editorialDirector</reg:name>
  <rdfs:label xml:lang="en">has editorial director</rdfs:label>
  <reg:lexicalAlias rdf:resource="http://rdaregistry.info/Elements/u/editorialDirector.en" />
  <skos:definition xml:lang="en">Relates a resource to an agent having legal or intellectual responsibility other than creation for the content of a serial, integrating resource, or multipart monographic resource.</skos:definition>
  <owl:inverseOf rdf:resource="http://rdaregistry.info/Elements/u/P60870" />
  <reg:hasSubproperty rdf:resource="http://rdaregistry.info/Elements/w/P10298" />
  <rdfs:subPropertyOf rdf:resource="http://rdaregistry.info/Elements/u/P60374" />
  <rdakit:seeAlso rdf:resource="http://rdaregistry.info/Elements/u/P60393" />
</owl:ObjectProperty>

<!-- Property: is editorial director of -->
<owl:ObjectProperty rdf:about="http://rdaregistry.info/Elements/u/P60870">
  <rdfs:isDefinedBy rdf:resource="http://rdaregistry.info/Elements/u/" />
  <reg:status rdf:resource="http://metadataregistry.org/uri/RegStatus/1001" />
  <rdf:type rdf:resource="http://www.w3.org/1999/02/22-rdf-syntax-ns#Property" />
  <reg:name xml:lang="en">editorialDirectorOf</reg:name>
  <rdfs:label xml:lang="en">is editorial director of</rdfs:label>
  <reg:lexicalAlias rdf:resource="http://rdaregistry.info/Elements/u/editorialDirectorOf.en" />
  <skos:definition xml:lang="en">Relates an agent responsible for a legal or intellectual responsibility other than creation for the content of a serial, integrating resource, or multipart monographic resource to a resource.</skos:definition>
  <owl:inverseOf rdf:resource="http://rdaregistry.info/Elements/u/P60869" />
  <rdfs:subPropertyOf rdf:resource="http://rdaregistry.info/Elements/u/P60602" />
  <rdakit:seeAlso rdf:resource="http://rdaregistry.info/Elements/u/P60621" />
</owl:ObjectProperty>

<!-- Property: is editor of -->
<owl:ObjectProperty rdf:about="http://rdaregistry.info/Elements/u/P60621">
  <rdfs:isDefinedBy rdf:resource="http://rdaregistry.info/Elements/u/" />
  <reg:status rdf:resource="http://metadataregistry.org/uri/RegStatus/1001" />
  <reg:name xml:lang="en">editorOf</reg:name>
  <rdfs:label xml:lang="en">is editor of</rdfs:label>
  <skos:definition xml:lang="en">Relates an agent contributing to a resource by revising or clarifying the content, e.g., adding an introduction, notes, or other critical matter to a resource.</skos:definition>
  <rdf:type rdf:resource="http://www.w3.org/1999/02/22-rdf-syntax-ns#Property" />
  <rdfs:subPropertyOf rdf:resource="http://rdaregistry.info/Elements/u/P60626" />
  <owl:inverseOf rdf:resource="http://rdaregistry.info/Elements/u/P60393" />
  <reg:hasSubproperty rdf:resource="http://rdaregistry.info/Elements/a/P50156" />
  <reg:lexicalAlias rdf:resource="http://rdaregistry.info/Elements/u/editorOf.en" />
</owl:ObjectProperty>

<!-- Property: has editor of moving image work -->
<owl:ObjectProperty rdf:about="http://rdaregistry.info/Elements/u/P60422">
  <rdfs:isDefinedBy rdf:resource="http://rdaregistry.info/Elements/u/" />
  <reg:status rdf:resource="http://metadataregistry.org/uri/RegStatus/1001" />
  <reg:name xml:lang="en">editorOfMovingImageResource</reg:name>
  <rdfs:label xml:lang="en">has editor of moving image work</rdfs:label>
  <skos:definition xml:lang="en">Relates a resource to an agent responsible for assembling, arranging, and trimming film, video, or other moving image formats, including both visual and audio aspects.</skos:definition>
  <rdf:type rdf:resource="http://www.w3.org/1999/02/22-rdf-syntax-ns#Property" />
  <rdfs:subPropertyOf rdf:resource="http://rdaregistry.info/Elements/u/P60398" />
  <owl:inverseOf rdf:resource="http://rdaregistry.info/Elements/u/P60651" />
  <reg:hasSubproperty rdf:resource="http://rdaregistry.info/Elements/e/P20055" />
  <reg:lexicalAlias rdf:resource="http://rdaregistry.info/Elements/u/editorOfMovingImageResource.en" />
  <rdakit:seeAlso rdf:resource="http://rdaregistry.info/Elements/u/P60663" />
</owl:ObjectProperty>

<!-- Property: is editor of moving image resource of -->
<owl:ObjectProperty rdf:about="http://rdaregistry.info/Elements/u/P60651">
  <rdfs:isDefinedBy rdf:resource="http://rdaregistry.info/Elements/u/" />
  <reg:status rdf:resource="http://metadataregistry.org/uri/RegStatus/1001" />
  <reg:name xml:lang="en">editorOfMovingImageResourceOf</reg:name>
  <rdfs:label xml:lang="en">is editor of moving image resource of</rdfs:label>
  <skos:definition xml:lang="en">Relates an agent responsible for assembling, arranging, and trimming film, video, or other moving image formats, including both visual and audio aspects to a resource.</skos:definition>
  <rdf:type rdf:resource="http://www.w3.org/1999/02/22-rdf-syntax-ns#Property" />
  <rdfs:subPropertyOf rdf:resource="http://rdaregistry.info/Elements/u/P60626" />
  <owl:inverseOf rdf:resource="http://rdaregistry.info/Elements/u/P60422" />
  <reg:hasSubproperty rdf:resource="http://rdaregistry.info/Elements/a/P50183" />
  <reg:lexicalAlias rdf:resource="http://rdaregistry.info/Elements/u/editorOfMovingImageResourceOf.en" />
</owl:ObjectProperty>

<!-- Property: has electronic reproduction -->
<owl:ObjectProperty rdf:about="http://rdaregistry.info/Elements/u/P60083">
  <rdfs:isDefinedBy rdf:resource="http://rdaregistry.info/Elements/u/" />
  <reg:status rdf:resource="http://metadataregistry.org/uri/RegStatus/1001" />
  <reg:name xml:lang="en">electronicReproduction</reg:name>
  <rdfs:label xml:lang="en">has electronic reproduction</rdfs:label>
  <skos:definition xml:lang="en">Relates a resource to a resource in a digital format that is a result of a transfer of a resource in an analog format.</skos:definition>
  <rdf:type rdf:resource="http://www.w3.org/1999/02/22-rdf-syntax-ns#Property" />
  <rdfs:subPropertyOf rdf:resource="http://rdaregistry.info/Elements/u/P60272" />
  <owl:inverseOf rdf:resource="http://rdaregistry.info/Elements/u/P60469" />
  <reg:hasSubproperty rdf:resource="http://rdaregistry.info/Elements/i/P40057" />
  <reg:hasSubproperty rdf:resource="http://rdaregistry.info/Elements/m/P30016" />
  <reg:lexicalAlias rdf:resource="http://rdaregistry.info/Elements/u/electronicReproduction.en" />
</owl:ObjectProperty>

<!-- Property: is electronic reproduction of -->
<owl:ObjectProperty rdf:about="http://rdaregistry.info/Elements/u/P60469">
  <rdfs:isDefinedBy rdf:resource="http://rdaregistry.info/Elements/u/" />
  <reg:status rdf:resource="http://metadataregistry.org/uri/RegStatus/1001" />
  <reg:name xml:lang="en">electronicReproductionOf</reg:name>
  <rdfs:label xml:lang="en">is electronic reproduction of</rdfs:label>
  <skos:definition xml:lang="en">Relates a resource to a resource in an analog format that is transferred to a digital format.</skos:definition>
  <rdf:type rdf:resource="http://www.w3.org/1999/02/22-rdf-syntax-ns#Property" />
  <rdfs:subPropertyOf rdf:resource="http://rdaregistry.info/Elements/u/P60297" />
  <owl:inverseOf rdf:resource="http://rdaregistry.info/Elements/u/P60083" />
  <reg:hasSubproperty rdf:resource="http://rdaregistry.info/Elements/i/P40027" />
  <reg:hasSubproperty rdf:resource="http://rdaregistry.info/Elements/m/P30136" />
  <reg:lexicalAlias rdf:resource="http://rdaregistry.info/Elements/u/electronicReproductionOf.en" />
</owl:ObjectProperty>

<!-- Property: has employee -->
<owl:ObjectProperty rdf:about="http://rdaregistry.info/Elements/u/P60629">
  <rdfs:isDefinedBy rdf:resource="http://rdaregistry.info/Elements/u/" />
  <reg:status rdf:resource="http://metadataregistry.org/uri/RegStatus/1001" />
  <reg:name xml:lang="en">employee</reg:name>
  <rdfs:label xml:lang="en">has employee</rdfs:label>
  <skos:definition xml:lang="en">Relates an agent employed by an agent to an agent.</skos:definition>
  <rdf:type rdf:resource="http://www.w3.org/1999/02/22-rdf-syntax-ns#Property" />
  <owl:inverseOf rdf:resource="http://rdaregistry.info/Elements/u/P60679" />
  <reg:hasSubproperty rdf:resource="http://rdaregistry.info/Elements/a/P50026" />
  <reg:lexicalAlias rdf:resource="http://rdaregistry.info/Elements/u/employee.en" />
</owl:ObjectProperty>

<!-- Property: has employer -->
<owl:ObjectProperty rdf:about="http://rdaregistry.info/Elements/u/P60679">
  <rdfs:isDefinedBy rdf:resource="http://rdaregistry.info/Elements/u/" />
  <reg:status rdf:resource="http://metadataregistry.org/uri/RegStatus/1001" />
  <reg:name xml:lang="en">employer</reg:name>
  <rdfs:label xml:lang="en">has employer</rdfs:label>
  <skos:definition xml:lang="en">Relates an agent that employs an agent to an agent.</skos:definition>
  <rdf:type rdf:resource="http://www.w3.org/1999/02/22-rdf-syntax-ns#Property" />
  <owl:inverseOf rdf:resource="http://rdaregistry.info/Elements/u/P60629" />
  <reg:hasSubproperty rdf:resource="http://rdaregistry.info/Elements/a/P50096" />
  <reg:lexicalAlias rdf:resource="http://rdaregistry.info/Elements/u/employer.en" />
</owl:ObjectProperty>

<!-- Property: has emulsion on microfilm and microfiche -->
<owl:ObjectProperty rdf:about="http://rdaregistry.info/Elements/u/P60344">
  <rdfs:isDefinedBy rdf:resource="http://rdaregistry.info/Elements/u/" />
  <reg:status rdf:resource="http://metadataregistry.org/uri/RegStatus/1001" />
  <reg:name xml:lang="en">emulsionOnMicrofilmAndMicrofiche</reg:name>
  <rdfs:label xml:lang="en">has emulsion on microfilm and microfiche</rdfs:label>
  <skos:definition xml:lang="en">Relates a resource to a suspension of light-sensitive chemicals used as a coating on a microfilm or microfiche.</skos:definition>
  <rdf:type rdf:resource="http://www.w3.org/1999/02/22-rdf-syntax-ns#Property" />
  <rdfs:subPropertyOf rdf:resource="http://rdaregistry.info/Elements/u/P60159" />
  <reg:hasSubproperty rdf:resource="http://rdaregistry.info/Elements/m/P30122" />
  <reg:lexicalAlias rdf:resource="http://rdaregistry.info/Elements/u/emulsionOnMicrofilmAndMicrofiche.en" />
</owl:ObjectProperty>

<!-- Property: has enacting jurisdiction -->
<owl:ObjectProperty rdf:about="http://rdaregistry.info/Elements/u/P60096">
  <rdfs:isDefinedBy rdf:resource="http://rdaregistry.info/Elements/u/" />
  <reg:status rdf:resource="http://metadataregistry.org/uri/RegStatus/1001" />
  <reg:name xml:lang="en">enactingJurisdiction</reg:name>
  <rdfs:label xml:lang="en">has enacting jurisdiction</rdfs:label>
  <skos:definition xml:lang="en">Relates a resource to a jurisdiction enacting a law, regulation, constitution, court rule, etc.</skos:definition>
  <rdf:type rdf:resource="http://www.w3.org/1999/02/22-rdf-syntax-ns#Property" />
  <rdfs:subPropertyOf rdf:resource="http://rdaregistry.info/Elements/u/P60447" />
  <owl:inverseOf rdf:resource="http://rdaregistry.info/Elements/u/P60014" />
  <reg:lexicalAlias rdf:resource="http://rdaregistry.info/Elements/u/enactingJurisdiction.en" />
</owl:ObjectProperty>

<!-- Property: is enacting jurisdiction of -->
<owl:ObjectProperty rdf:about="http://rdaregistry.info/Elements/u/P60014">
  <rdfs:isDefinedBy rdf:resource="http://rdaregistry.info/Elements/u/" />
  <reg:status rdf:resource="http://metadataregistry.org/uri/RegStatus/1001" />
  <reg:name xml:lang="en">enactingJurisdictionOf</reg:name>
  <rdfs:label xml:lang="en">is enacting jurisdiction of</rdfs:label>
  <skos:definition xml:lang="en">Relates a jurisdiction enacting a law, regulation, constitution, court rule, etc. to a resource.</skos:definition>
  <rdf:type rdf:resource="http://www.w3.org/1999/02/22-rdf-syntax-ns#Property" />
  <rdfs:subPropertyOf rdf:resource="http://rdaregistry.info/Elements/u/P60672" />
  <owl:inverseOf rdf:resource="http://rdaregistry.info/Elements/u/P60096" />
  <reg:hasSubproperty rdf:resource="http://rdaregistry.info/Elements/a/P50068" />
  <reg:lexicalAlias rdf:resource="http://rdaregistry.info/Elements/u/enactingJurisdictionOf.en" />
</owl:ObjectProperty>

<!-- Property: has encoded bitrate -->
<owl:ObjectProperty rdf:about="http://rdaregistry.info/Elements/u/P60587">
  <rdfs:isDefinedBy rdf:resource="http://rdaregistry.info/Elements/u/" />
  <reg:status rdf:resource="http://metadataregistry.org/uri/RegStatus/1001" />
  <reg:name xml:lang="en">encodedBitrate</reg:name>
  <rdfs:label xml:lang="en">has encoded bitrate</rdfs:label>
  <skos:definition xml:lang="en">Relates a resource to a speed at which streaming audio, video, etc., is designed to play.</skos:definition>
  <rdf:type rdf:resource="http://www.w3.org/1999/02/22-rdf-syntax-ns#Property" />
  <rdfs:subPropertyOf rdf:resource="http://rdaregistry.info/Elements/u/P60350" />
  <reg:hasSubproperty rdf:resource="http://rdaregistry.info/Elements/m/P30202" />
  <reg:lexicalAlias rdf:resource="http://rdaregistry.info/Elements/u/encodedBitrate.en" />
  <owl:inverseOf rdf:resource="http://rdaregistry.info/Elements/u/P60858" />
</owl:ObjectProperty>

<!-- Property: has encoding format -->
<owl:ObjectProperty rdf:about="http://rdaregistry.info/Elements/u/P60314">
  <rdfs:isDefinedBy rdf:resource="http://rdaregistry.info/Elements/u/" />
  <reg:status rdf:resource="http://metadataregistry.org/uri/RegStatus/1001" />
  <reg:name xml:lang="en">encodingFormat</reg:name>
  <rdfs:label xml:lang="en">has encoding format</rdfs:label>
  <skos:definition xml:lang="en">Relates a resource to a schema, standard, etc., used to encode the digital content of a resource.</skos:definition>
  <rdf:type rdf:resource="http://www.w3.org/1999/02/22-rdf-syntax-ns#Property" />
  <rdfs:subPropertyOf rdf:resource="http://rdaregistry.info/Elements/u/P60350" />
  <reg:hasSubproperty rdf:resource="http://rdaregistry.info/Elements/m/P30096" />
  <reg:lexicalAlias rdf:resource="http://rdaregistry.info/Elements/u/encodingFormat.en" />
</owl:ObjectProperty>

<!-- Property: has engraver -->
<owl:ObjectProperty rdf:about="http://rdaregistry.info/Elements/u/P60410">
  <rdfs:isDefinedBy rdf:resource="http://rdaregistry.info/Elements/u/" />
  <reg:status rdf:resource="http://metadataregistry.org/uri/RegStatus/1001" />
  <reg:name xml:lang="en">engraver</reg:name>
  <rdfs:label xml:lang="en">has engraver</rdfs:label>
  <skos:definition xml:lang="en">Relates a resource to an agent involved in manufacturing a resource by cutting letters, figures, etc., on a surface such as a wooden or metal plate used for printing.</skos:definition>
  <rdf:type rdf:resource="http://www.w3.org/1999/02/22-rdf-syntax-ns#Property" />
  <rdfs:subPropertyOf rdf:resource="http://rdaregistry.info/Elements/u/P60443" />
  <owl:inverseOf rdf:resource="http://rdaregistry.info/Elements/u/P60638" />
  <reg:hasSubproperty rdf:resource="http://rdaregistry.info/Elements/m/P30070" />
  <reg:lexicalAlias rdf:resource="http://rdaregistry.info/Elements/u/engraver.en" />
</owl:ObjectProperty>

<!-- Property: is engraver of -->
<owl:ObjectProperty rdf:about="http://rdaregistry.info/Elements/u/P60638">
  <rdfs:isDefinedBy rdf:resource="http://rdaregistry.info/Elements/u/" />
  <reg:status rdf:resource="http://metadataregistry.org/uri/RegStatus/1001" />
  <reg:name xml:lang="en">engraverOf</reg:name>
  <rdfs:label xml:lang="en">is engraver of</rdfs:label>
  <skos:definition xml:lang="en">Relates an agent involved in manufacturing a resource by cutting letters, figures, etc., on a surface such as a wooden or metal plate used for printing to a resource.</skos:definition>
  <rdf:type rdf:resource="http://www.w3.org/1999/02/22-rdf-syntax-ns#Property" />
  <rdfs:subPropertyOf rdf:resource="http://rdaregistry.info/Elements/u/P60669" />
  <owl:inverseOf rdf:resource="http://rdaregistry.info/Elements/u/P60410" />
  <reg:hasSubproperty rdf:resource="http://rdaregistry.info/Elements/a/P50171" />
  <reg:lexicalAlias rdf:resource="http://rdaregistry.info/Elements/u/engraverOf.en" />
</owl:ObjectProperty>

<!-- Property: has enrolled student -->
<owl:ObjectProperty rdf:about="http://rdaregistry.info/Elements/u/P60855">
  <rdfs:isDefinedBy rdf:resource="http://rdaregistry.info/Elements/u/" />
  <reg:status rdf:resource="http://metadataregistry.org/uri/RegStatus/1001" />
  <rdf:type rdf:resource="http://www.w3.org/1999/02/22-rdf-syntax-ns#Property" />
  <reg:name xml:lang="en">enrolledStudent</reg:name>
  <rdfs:label xml:lang="en">has enrolled student</rdfs:label>
  <reg:lexicalAlias rdf:resource="http://rdaregistry.info/Elements/u/enrolledStudent.en" />
  <skos:definition xml:lang="en">Relates an agent to an agent who receives instruction at an educational institution.</skos:definition>
  <owl:inverseOf rdf:resource="http://rdaregistry.info/Elements/u/P60856" />
  <reg:hasSubproperty rdf:resource="http://rdaregistry.info/Elements/a/P50283" />
  <rdfs:subPropertyOf rdf:resource="http://rdaregistry.info/Elements/u/P60454" />
</owl:ObjectProperty>

<!-- Property: has epoch -->
<owl:ObjectProperty rdf:about="http://rdaregistry.info/Elements/u/P60472">
  <rdfs:isDefinedBy rdf:resource="http://rdaregistry.info/Elements/u/" />
  <reg:status rdf:resource="http://metadataregistry.org/uri/RegStatus/1001" />
  <reg:name xml:lang="en">epoch</reg:name>
  <rdfs:label xml:lang="en">has epoch</rdfs:label>
  <skos:definition xml:lang="en">Relates a resource to an arbitrary moment in time to which measurements of position for a body or orientation for an orbit are referred.</skos:definition>
  <rdf:type rdf:resource="http://www.w3.org/1999/02/22-rdf-syntax-ns#Property" />
  <reg:lexicalAlias rdf:resource="http://rdaregistry.info/Elements/u/epoch.en" />
</owl:ObjectProperty>

<!-- Property: has equinox -->
<owl:ObjectProperty rdf:about="http://rdaregistry.info/Elements/u/P60506">
  <rdfs:isDefinedBy rdf:resource="http://rdaregistry.info/Elements/u/" />
  <reg:status rdf:resource="http://metadataregistry.org/uri/RegStatus/1001" />
  <reg:name xml:lang="en">equinox</reg:name>
  <rdfs:label xml:lang="en">has equinox</rdfs:label>
  <skos:definition xml:lang="en">Relates a resource to a point of intersection of the ecliptic and the celestial equator, occupied by the sun when its declination is 0.</skos:definition>
  <rdf:type rdf:resource="http://www.w3.org/1999/02/22-rdf-syntax-ns#Property" />
  <reg:lexicalAlias rdf:resource="http://rdaregistry.info/Elements/u/equinox.en" />
</owl:ObjectProperty>

<!-- Property: has equipment or system requirement -->
<owl:ObjectProperty rdf:about="http://rdaregistry.info/Elements/u/P60528">
  <rdfs:isDefinedBy rdf:resource="http://rdaregistry.info/Elements/u/" />
  <reg:status rdf:resource="http://metadataregistry.org/uri/RegStatus/1001" />
  <reg:name xml:lang="en">equipmentOrSystemRequirement</reg:name>
  <rdfs:label xml:lang="en">has equipment or system requirement</rdfs:label>
  <skos:definition xml:lang="en">Relates a resource to a system or equipment required for use, playback, etc., of an analog, digital, etc., resource.</skos:definition>
  <rdf:type rdf:resource="http://www.w3.org/1999/02/22-rdf-syntax-ns#Property" />
  <reg:hasSubproperty rdf:resource="http://rdaregistry.info/Elements/m/P30162" />
  <reg:lexicalAlias rdf:resource="http://rdaregistry.info/Elements/u/equipmentOrSystemRequirement.en" />
</owl:ObjectProperty>

<!-- Property: has equivalent -->
<owl:ObjectProperty rdf:about="http://rdaregistry.info/Elements/u/P60191">
  <rdfs:isDefinedBy rdf:resource="http://rdaregistry.info/Elements/u/" />
  <reg:status rdf:resource="http://metadataregistry.org/uri/RegStatus/1001" />
  <reg:name xml:lang="en">equivalent</reg:name>
  <rdfs:label xml:lang="en">has equivalent</rdfs:label>
  <skos:definition xml:lang="en">Relates a resource to a resource that carries the same content as a resource.</skos:definition>
  <rdf:type rdf:resource="http://www.w3.org/1999/02/22-rdf-syntax-ns#Property" />
  <rdfs:subPropertyOf rdf:resource="http://rdaregistry.info/Elements/u/P60712" />
  <owl:inverseOf rdf:resource="http://rdaregistry.info/Elements/u/P60191" />
  <reg:hasSubproperty rdf:resource="http://rdaregistry.info/Elements/u/P60195" />
  <reg:hasSubproperty rdf:resource="http://rdaregistry.info/Elements/u/P60197" />
  <reg:hasSubproperty rdf:resource="http://rdaregistry.info/Elements/u/P60272" />
  <reg:hasSubproperty rdf:resource="http://rdaregistry.info/Elements/u/P60297" />
  <reg:hasSubproperty rdf:resource="http://rdaregistry.info/Elements/i/P40031" />
  <reg:hasSubproperty rdf:resource="http://rdaregistry.info/Elements/m/P30024" />
  <reg:lexicalAlias rdf:resource="http://rdaregistry.info/Elements/u/equivalent.en" />
</owl:ObjectProperty>

<!-- Property: has equivalent resource relationship with -->
<owl:ObjectProperty rdf:about="http://rdaregistry.info/Elements/u/P60712">
  <rdfs:isDefinedBy rdf:resource="http://rdaregistry.info/Elements/u/" />
  <reg:status rdf:resource="http://metadataregistry.org/uri/RegStatus/1001" />
  <reg:name xml:lang="en">equivalentResourceRelationshipWith</reg:name>
  <rdfs:label xml:lang="en">has equivalent resource relationship with</rdfs:label>
  <rdf:type rdf:resource="http://www.w3.org/1999/02/22-rdf-syntax-ns#Property" />
  <reg:hasSubproperty rdf:resource="http://rdaregistry.info/Elements/u/P60191" />
  <owl:inverseOf rdf:resource="http://rdaregistry.info/Elements/u/P60712" />
  <skos:definition xml:lang="en">Relates a resource to a resource that is equivalent to a resource.</skos:definition>
  <reg:hasSubproperty rdf:resource="http://rdaregistry.info/Elements/i/P40053" />
  <reg:hasSubproperty rdf:resource="http://rdaregistry.info/Elements/m/P30212" />
  <reg:lexicalAlias rdf:resource="http://rdaregistry.info/Elements/u/equivalentResourceRelationshipWith.en" />
</owl:ObjectProperty>

<!-- Property: is errata -->
<owl:ObjectProperty rdf:about="http://rdaregistry.info/Elements/u/P60181">
  <rdfs:isDefinedBy rdf:resource="http://rdaregistry.info/Elements/u/" />
  <reg:status rdf:resource="http://metadataregistry.org/uri/RegStatus/1001" />
  <reg:name xml:lang="en">errata</reg:name>
  <rdfs:label xml:lang="en">is errata</rdfs:label>
  <skos:definition xml:lang="en">Relates a resource to a resource consisting of errors discovered after the publication of a predominant resource, with their corrections.</skos:definition>
  <rdf:type rdf:resource="http://www.w3.org/1999/02/22-rdf-syntax-ns#Property" />
  <rdfs:subPropertyOf rdf:resource="http://rdaregistry.info/Elements/u/P60204" />
  <owl:inverseOf rdf:resource="http://rdaregistry.info/Elements/u/P60251" />
  <reg:hasSubproperty rdf:resource="http://rdaregistry.info/Elements/e/P20093" />
  <reg:lexicalAlias rdf:resource="http://rdaregistry.info/Elements/u/errata.en" />
</owl:ObjectProperty>

<!-- Property: is errata to -->
<owl:ObjectProperty rdf:about="http://rdaregistry.info/Elements/u/P60251">
  <rdfs:isDefinedBy rdf:resource="http://rdaregistry.info/Elements/u/" />
  <reg:status rdf:resource="http://metadataregistry.org/uri/RegStatus/1001" />
  <reg:name xml:lang="en">errataTo</reg:name>
  <rdfs:label xml:lang="en">is errata to</rdfs:label>
  <skos:definition xml:lang="en">Relates a resource to a resource that is augmented by a list of errors in a predominant resource, discovered after publication, with their corrections.</skos:definition>
  <rdf:type rdf:resource="http://www.w3.org/1999/02/22-rdf-syntax-ns#Property" />
  <rdfs:subPropertyOf rdf:resource="http://rdaregistry.info/Elements/u/P60307" />
  <owl:inverseOf rdf:resource="http://rdaregistry.info/Elements/u/P60181" />
  <reg:hasSubproperty rdf:resource="http://rdaregistry.info/Elements/e/P20146" />
  <reg:lexicalAlias rdf:resource="http://rdaregistry.info/Elements/u/errataTo.en" />
</owl:ObjectProperty>

<!-- Property: has etcher -->
<owl:ObjectProperty rdf:about="http://rdaregistry.info/Elements/u/P60416">
  <rdfs:isDefinedBy rdf:resource="http://rdaregistry.info/Elements/u/" />
  <reg:status rdf:resource="http://metadataregistry.org/uri/RegStatus/1001" />
  <reg:name xml:lang="en">etcher</reg:name>
  <rdfs:label xml:lang="en">has etcher</rdfs:label>
  <skos:definition xml:lang="en">Relates a resource to an agent involved in manufacturing a resource by subjecting metal, glass, or some other surface used for printing, to acid or another corrosive substance.</skos:definition>
  <rdf:type rdf:resource="http://www.w3.org/1999/02/22-rdf-syntax-ns#Property" />
  <rdfs:subPropertyOf rdf:resource="http://rdaregistry.info/Elements/u/P60443" />
  <owl:inverseOf rdf:resource="http://rdaregistry.info/Elements/u/P60644" />
  <reg:hasSubproperty rdf:resource="http://rdaregistry.info/Elements/m/P30076" />
  <reg:lexicalAlias rdf:resource="http://rdaregistry.info/Elements/u/etcher.en" />
</owl:ObjectProperty>

<!-- Property: is etcher of -->
<owl:ObjectProperty rdf:about="http://rdaregistry.info/Elements/u/P60644">
  <rdfs:isDefinedBy rdf:resource="http://rdaregistry.info/Elements/u/" />
  <reg:status rdf:resource="http://metadataregistry.org/uri/RegStatus/1001" />
  <reg:name xml:lang="en">etcherOf</reg:name>
  <rdfs:label xml:lang="en">is etcher of</rdfs:label>
  <skos:definition xml:lang="en">Relates an agent involved in manufacturing a resource by subjecting metal, glass, or some other surface used for printing, to acid or another corrosive substance to a resource.</skos:definition>
  <rdf:type rdf:resource="http://www.w3.org/1999/02/22-rdf-syntax-ns#Property" />
  <rdfs:subPropertyOf rdf:resource="http://rdaregistry.info/Elements/u/P60669" />
  <owl:inverseOf rdf:resource="http://rdaregistry.info/Elements/u/P60416" />
  <reg:hasSubproperty rdf:resource="http://rdaregistry.info/Elements/a/P50177" />
  <reg:lexicalAlias rdf:resource="http://rdaregistry.info/Elements/u/etcherOf.en" />
</owl:ObjectProperty>

<!-- Property: is evaluated in -->
<owl:ObjectProperty rdf:about="http://rdaregistry.info/Elements/u/P60218">
  <rdfs:isDefinedBy rdf:resource="http://rdaregistry.info/Elements/u/" />
  <reg:status rdf:resource="http://metadataregistry.org/uri/RegStatus/1001" />
  <reg:name xml:lang="en">evaluatedIn</reg:name>
  <rdfs:label xml:lang="en">is evaluated in</rdfs:label>
  <skos:definition xml:lang="en">Relates a resource to a resource that examines or judges a described resource.</skos:definition>
  <rdf:type rdf:resource="http://www.w3.org/1999/02/22-rdf-syntax-ns#Property" />
  <rdfs:subPropertyOf rdf:resource="http://rdaregistry.info/Elements/u/P60215" />
  <owl:inverseOf rdf:resource="http://rdaregistry.info/Elements/u/P60255" />
  <reg:hasSubproperty rdf:resource="http://rdaregistry.info/Elements/e/P20273" />
  <reg:hasSubproperty rdf:resource="http://rdaregistry.info/Elements/i/P40066" />
  <reg:hasSubproperty rdf:resource="http://rdaregistry.info/Elements/m/P30258" />
  <reg:lexicalAlias rdf:resource="http://rdaregistry.info/Elements/u/evaluatedIn.en" />
</owl:ObjectProperty>

<!-- Property: is evaluation of -->
<owl:ObjectProperty rdf:about="http://rdaregistry.info/Elements/u/P60255">
  <rdfs:isDefinedBy rdf:resource="http://rdaregistry.info/Elements/u/" />
  <reg:status rdf:resource="http://metadataregistry.org/uri/RegStatus/1001" />
  <reg:name xml:lang="en">evaluationOf</reg:name>
  <rdfs:label xml:lang="en">is evaluation of</rdfs:label>
  <skos:definition xml:lang="en">Relates a resource to a resource that is examined or judged.</skos:definition>
  <rdf:type rdf:resource="http://www.w3.org/1999/02/22-rdf-syntax-ns#Property" />
  <rdfs:subPropertyOf rdf:resource="http://rdaregistry.info/Elements/u/P60190" />
  <owl:inverseOf rdf:resource="http://rdaregistry.info/Elements/u/P60218" />
  <reg:hasSubproperty rdf:resource="http://rdaregistry.info/Elements/w/P10267" />
  <reg:hasSubproperty rdf:resource="http://rdaregistry.info/Elements/w/P10273" />
  <reg:hasSubproperty rdf:resource="http://rdaregistry.info/Elements/w/P10279" />
  <reg:lexicalAlias rdf:resource="http://rdaregistry.info/Elements/u/evaluationOf.en" />
</owl:ObjectProperty>

<!-- Property: is expanded as -->
<owl:ObjectProperty rdf:about="http://rdaregistry.info/Elements/u/P60216">
  <rdfs:isDefinedBy rdf:resource="http://rdaregistry.info/Elements/u/" />
  <reg:status rdf:resource="http://metadataregistry.org/uri/RegStatus/1001" />
  <reg:name xml:lang="en">expandedAs</reg:name>
  <rdfs:label xml:lang="en">is expanded as</rdfs:label>
  <skos:definition xml:lang="en">Relates a resource to a resource that enlarges upon the content of a source resource.</skos:definition>
  <rdf:type rdf:resource="http://www.w3.org/1999/02/22-rdf-syntax-ns#Property" />
  <rdfs:subPropertyOf rdf:resource="http://rdaregistry.info/Elements/u/P60250" />
  <owl:inverseOf rdf:resource="http://rdaregistry.info/Elements/u/P60294" />
  <reg:hasSubproperty rdf:resource="http://rdaregistry.info/Elements/e/P20115" />
  <reg:lexicalAlias rdf:resource="http://rdaregistry.info/Elements/u/expandedAs.en" />
</owl:ObjectProperty>

<!-- Property: is expanded version of -->
<owl:ObjectProperty rdf:about="http://rdaregistry.info/Elements/u/P60294">
  <rdfs:isDefinedBy rdf:resource="http://rdaregistry.info/Elements/u/" />
  <reg:status rdf:resource="http://metadataregistry.org/uri/RegStatus/1001" />
  <reg:name xml:lang="en">expandedVersionOf</reg:name>
  <rdfs:label xml:lang="en">is expanded version of</rdfs:label>
  <skos:definition xml:lang="en">Relates a resource to a resource used as a basis for a derivative resource that enlarges upon the content of a source resource.</skos:definition>
  <rdf:type rdf:resource="http://www.w3.org/1999/02/22-rdf-syntax-ns#Property" />
  <rdfs:subPropertyOf rdf:resource="http://rdaregistry.info/Elements/u/P60305" />
  <owl:inverseOf rdf:resource="http://rdaregistry.info/Elements/u/P60216" />
  <reg:hasSubproperty rdf:resource="http://rdaregistry.info/Elements/e/P20184" />
  <reg:lexicalAlias rdf:resource="http://rdaregistry.info/Elements/u/expandedVersionOf.en" />
</owl:ObjectProperty>

<!-- Property: has extent -->
<owl:ObjectProperty rdf:about="http://rdaregistry.info/Elements/u/P60550">
  <rdfs:isDefinedBy rdf:resource="http://rdaregistry.info/Elements/u/" />
  <reg:status rdf:resource="http://metadataregistry.org/uri/RegStatus/1001" />
  <reg:name xml:lang="en">extent</reg:name>
  <rdfs:label xml:lang="en">has extent</rdfs:label>
  <skos:definition xml:lang="en">Relates a resource to a number and type of unit or subunit of a resource.</skos:definition>
  <rdf:type rdf:resource="http://www.w3.org/1999/02/22-rdf-syntax-ns#Property" />
  <reg:hasSubproperty rdf:resource="http://rdaregistry.info/Elements/m/P30177" />
  <reg:hasSubproperty rdf:resource="http://rdaregistry.info/Elements/m/P30178" />
  <reg:hasSubproperty rdf:resource="http://rdaregistry.info/Elements/m/P30179" />
  <reg:hasSubproperty rdf:resource="http://rdaregistry.info/Elements/m/P30180" />
  <reg:hasSubproperty rdf:resource="http://rdaregistry.info/Elements/m/P30181" />
  <reg:hasSubproperty rdf:resource="http://rdaregistry.info/Elements/m/P30182" />
  <reg:lexicalAlias rdf:resource="http://rdaregistry.info/Elements/u/extent.en" />
</owl:ObjectProperty>

<!-- Property: has facsimile -->
<owl:ObjectProperty rdf:about="http://rdaregistry.info/Elements/u/P60217">
  <rdfs:isDefinedBy rdf:resource="http://rdaregistry.info/Elements/u/" />
  <reg:status rdf:resource="http://metadataregistry.org/uri/RegStatus/1001" />
  <reg:name xml:lang="en">facsimile</reg:name>
  <rdfs:label xml:lang="en">has facsimile</rdfs:label>
  <skos:definition xml:lang="en">Relates a resource to a resource that exactly reproduces another resource embodying a resource.</skos:definition>
  <rdf:type rdf:resource="http://www.w3.org/1999/02/22-rdf-syntax-ns#Property" />
  <rdfs:subPropertyOf rdf:resource="http://rdaregistry.info/Elements/u/P60272" />
  <owl:inverseOf rdf:resource="http://rdaregistry.info/Elements/u/P60301" />
  <reg:hasSubproperty rdf:resource="http://rdaregistry.info/Elements/u/P60179" />
  <reg:hasSubproperty rdf:resource="http://rdaregistry.info/Elements/i/P40058" />
  <reg:hasSubproperty rdf:resource="http://rdaregistry.info/Elements/m/P30031" />
  <reg:lexicalAlias rdf:resource="http://rdaregistry.info/Elements/u/facsimile.en" />
</owl:ObjectProperty>

<!-- Property: is facsimile contained in -->
<owl:ObjectProperty rdf:about="http://rdaregistry.info/Elements/u/P60100">
  <rdfs:isDefinedBy rdf:resource="http://rdaregistry.info/Elements/u/" />
  <reg:status rdf:resource="http://metadataregistry.org/uri/RegStatus/1001" />
  <reg:name xml:lang="en">facsimileContainedIn</reg:name>
  <rdfs:label xml:lang="en">is facsimile contained in</rdfs:label>
  <skos:definition xml:lang="en">Relates a resource to a larger resource of which a part is a discrete component that exactly reproduces another resource embodying a resource.</skos:definition>
  <rdf:type rdf:resource="http://www.w3.org/1999/02/22-rdf-syntax-ns#Property" />
  <rdfs:subPropertyOf rdf:resource="http://rdaregistry.info/Elements/u/P60101" />
  <owl:inverseOf rdf:resource="http://rdaregistry.info/Elements/u/P60300" />
  <reg:hasSubproperty rdf:resource="http://rdaregistry.info/Elements/m/P30019" />
  <reg:lexicalAlias rdf:resource="http://rdaregistry.info/Elements/u/facsimileContainedIn.en" />
</owl:ObjectProperty>

<!-- Property: is facsimile container of -->
<owl:ObjectProperty rdf:about="http://rdaregistry.info/Elements/u/P60300">
  <rdfs:isDefinedBy rdf:resource="http://rdaregistry.info/Elements/u/" />
  <reg:status rdf:resource="http://metadataregistry.org/uri/RegStatus/1001" />
  <reg:name xml:lang="en">facsimileContainerOf</reg:name>
  <rdfs:label xml:lang="en">is facsimile container of</rdfs:label>
  <skos:definition xml:lang="en">Relates a resource to a resource used as a basis for an exact reproduction that is a discrete component of a larger entity.</skos:definition>
  <rdf:type rdf:resource="http://www.w3.org/1999/02/22-rdf-syntax-ns#Property" />
  <rdfs:subPropertyOf rdf:resource="http://rdaregistry.info/Elements/u/P60249" />
  <owl:inverseOf rdf:resource="http://rdaregistry.info/Elements/u/P60100" />
  <reg:hasSubproperty rdf:resource="http://rdaregistry.info/Elements/m/P30046" />
  <reg:lexicalAlias rdf:resource="http://rdaregistry.info/Elements/u/facsimileContainerOf.en" />
</owl:ObjectProperty>

<!-- Property: is facsimile of -->
<owl:ObjectProperty rdf:about="http://rdaregistry.info/Elements/u/P60301">
  <rdfs:isDefinedBy rdf:resource="http://rdaregistry.info/Elements/u/" />
  <reg:status rdf:resource="http://metadataregistry.org/uri/RegStatus/1001" />
  <reg:name xml:lang="en">facsimileOf</reg:name>
  <rdfs:label xml:lang="en">is facsimile of</rdfs:label>
  <skos:definition xml:lang="en">Relates a resource to a resource that is used as a basis for an exact reproduction.</skos:definition>
  <rdf:type rdf:resource="http://www.w3.org/1999/02/22-rdf-syntax-ns#Property" />
  <rdfs:subPropertyOf rdf:resource="http://rdaregistry.info/Elements/u/P60297" />
  <owl:inverseOf rdf:resource="http://rdaregistry.info/Elements/u/P60217" />
  <reg:hasSubproperty rdf:resource="http://rdaregistry.info/Elements/u/P60299" />
  <reg:hasSubproperty rdf:resource="http://rdaregistry.info/Elements/i/P40045" />
  <reg:hasSubproperty rdf:resource="http://rdaregistry.info/Elements/m/P30047" />
  <reg:lexicalAlias rdf:resource="http://rdaregistry.info/Elements/u/facsimileOf.en" />
</owl:ObjectProperty>

<!-- Property: has fellow student -->
<owl:ObjectProperty rdf:about="http://rdaregistry.info/Elements/u/P60861">
  <rdfs:isDefinedBy rdf:resource="http://rdaregistry.info/Elements/u/" />
  <reg:status rdf:resource="http://metadataregistry.org/uri/RegStatus/1001" />
  <rdf:type rdf:resource="http://www.w3.org/1999/02/22-rdf-syntax-ns#Property" />
  <reg:name xml:lang="en">fellowStudent</reg:name>
  <rdfs:label xml:lang="en">has fellow student</rdfs:label>
  <reg:lexicalAlias rdf:resource="http://rdaregistry.info/Elements/u/fellowStudent.en" />
  <skos:definition xml:lang="en">Relates an agent to an associate of another student who is also formally engaged in learning.</skos:definition>
  <owl:inverseOf rdf:resource="http://rdaregistry.info/Elements/u/P60861" />
  <reg:hasSubproperty rdf:resource="http://rdaregistry.info/Elements/a/P50279" />
  <rdfs:subPropertyOf rdf:resource="http://rdaregistry.info/Elements/u/P60454" />
</owl:ObjectProperty>

<!-- Property: has field of activity of agent -->
<owl:ObjectProperty rdf:about="http://rdaregistry.info/Elements/u/P60089">
  <rdfs:isDefinedBy rdf:resource="http://rdaregistry.info/Elements/u/" />
  <reg:status rdf:resource="http://metadataregistry.org/uri/RegStatus/1001" />
  <reg:name xml:lang="en">fieldOfActivityOfAgent</reg:name>
  <rdfs:label xml:lang="en">has field of activity of agent</rdfs:label>
  <skos:definition xml:lang="en">Relates a resource to a field of endeavour, area of expertise, competence, responsibility, jurisdiction etc., in which an agent is engaged or was engaged.</skos:definition>
  <rdf:type rdf:resource="http://www.w3.org/1999/02/22-rdf-syntax-ns#Property" />
  <reg:hasSubproperty rdf:resource="http://rdaregistry.info/Elements/a/P50022" />
  <reg:hasSubproperty rdf:resource="http://rdaregistry.info/Elements/a/P50100" />
  <reg:lexicalAlias rdf:resource="http://rdaregistry.info/Elements/u/fieldOfActivityOfAgent.en" />
</owl:ObjectProperty>

<!-- Property: has file size -->
<owl:ObjectProperty rdf:about="http://rdaregistry.info/Elements/u/P60551">
  <rdfs:isDefinedBy rdf:resource="http://rdaregistry.info/Elements/u/" />
  <reg:status rdf:resource="http://metadataregistry.org/uri/RegStatus/1001" />
  <reg:name xml:lang="en">fileSize</reg:name>
  <rdfs:label xml:lang="en">has file size</rdfs:label>
  <skos:definition xml:lang="en">Relates a resource to a number of bytes in a digital file.</skos:definition>
  <rdf:type rdf:resource="http://www.w3.org/1999/02/22-rdf-syntax-ns#Property" />
  <rdfs:subPropertyOf rdf:resource="http://rdaregistry.info/Elements/u/P60350" />
  <reg:hasSubproperty rdf:resource="http://rdaregistry.info/Elements/m/P30183" />
  <reg:lexicalAlias rdf:resource="http://rdaregistry.info/Elements/u/fileSize.en" />
</owl:ObjectProperty>

<!-- Property: has file type -->
<owl:ObjectProperty rdf:about="http://rdaregistry.info/Elements/u/P60093">
  <rdfs:isDefinedBy rdf:resource="http://rdaregistry.info/Elements/u/" />
  <reg:status rdf:resource="http://metadataregistry.org/uri/RegStatus/1001" />
  <reg:name xml:lang="en">fileType</reg:name>
  <rdfs:label xml:lang="en">has file type</rdfs:label>
  <skos:definition xml:lang="en">Relates a resource to a general type of data content encoded in a computer file.</skos:definition>
  <rdf:type rdf:resource="http://www.w3.org/1999/02/22-rdf-syntax-ns#Property" />
  <rdfs:subPropertyOf rdf:resource="http://rdaregistry.info/Elements/u/P60350" />
  <reg:hasSubproperty rdf:resource="http://rdaregistry.info/Elements/m/P30018" />
  <reg:lexicalAlias rdf:resource="http://rdaregistry.info/Elements/u/fileType.en" />
</owl:ObjectProperty>

<!-- Property: has film director -->
<owl:ObjectProperty rdf:about="http://rdaregistry.info/Elements/u/P60084">
  <rdfs:isDefinedBy rdf:resource="http://rdaregistry.info/Elements/u/" />
  <reg:status rdf:resource="http://metadataregistry.org/uri/RegStatus/1001" />
  <reg:name xml:lang="en">filmDirector</reg:name>
  <rdfs:label xml:lang="en">has film director</rdfs:label>
  <skos:definition xml:lang="en">Relates a resource to a director responsible for the general management and supervision of a filmed performance.</skos:definition>
  <rdf:type rdf:resource="http://www.w3.org/1999/02/22-rdf-syntax-ns#Property" />
  <rdfs:subPropertyOf rdf:resource="http://rdaregistry.info/Elements/u/P60449" />
  <owl:inverseOf rdf:resource="http://rdaregistry.info/Elements/u/P60009" />
  <reg:lexicalAlias rdf:resource="http://rdaregistry.info/Elements/u/filmDirector.en" />
</owl:ObjectProperty>

<!-- Property: is film director of -->
<owl:ObjectProperty rdf:about="http://rdaregistry.info/Elements/u/P60009">
  <rdfs:isDefinedBy rdf:resource="http://rdaregistry.info/Elements/u/" />
  <reg:status rdf:resource="http://metadataregistry.org/uri/RegStatus/1001" />
  <reg:name xml:lang="en">filmDirectorOf</reg:name>
  <rdfs:label xml:lang="en">is film director of</rdfs:label>
  <skos:definition xml:lang="en">Relates a director responsible for the general management and supervision of a filmed performance to a resource.</skos:definition>
  <rdf:type rdf:resource="http://www.w3.org/1999/02/22-rdf-syntax-ns#Property" />
  <rdfs:subPropertyOf rdf:resource="http://rdaregistry.info/Elements/u/P60673" />
  <owl:inverseOf rdf:resource="http://rdaregistry.info/Elements/u/P60084" />
  <reg:hasSubproperty rdf:resource="http://rdaregistry.info/Elements/a/P50048" />
  <reg:lexicalAlias rdf:resource="http://rdaregistry.info/Elements/u/filmDirectorOf.en" />
</owl:ObjectProperty>

<!-- Property: has film distributor -->
<owl:ObjectProperty rdf:about="http://rdaregistry.info/Elements/u/P60408">
  <rdfs:isDefinedBy rdf:resource="http://rdaregistry.info/Elements/u/" />
  <reg:status rdf:resource="http://metadataregistry.org/uri/RegStatus/1001" />
  <reg:name xml:lang="en">filmDistributor</reg:name>
  <rdfs:label xml:lang="en">has film distributor</rdfs:label>
  <skos:definition xml:lang="en">Relates a resource to an agent involved in distributing a moving image resource to theatres or other distribution channels.</skos:definition>
  <rdf:type rdf:resource="http://www.w3.org/1999/02/22-rdf-syntax-ns#Property" />
  <rdfs:subPropertyOf rdf:resource="http://rdaregistry.info/Elements/u/P60438" />
  <owl:inverseOf rdf:resource="http://rdaregistry.info/Elements/u/P60636" />
  <reg:hasSubproperty rdf:resource="http://rdaregistry.info/Elements/m/P30068" />
  <reg:lexicalAlias rdf:resource="http://rdaregistry.info/Elements/u/filmDistributor.en" />
</owl:ObjectProperty>

<!-- Property: is film distributor of -->
<owl:ObjectProperty rdf:about="http://rdaregistry.info/Elements/u/P60636">
  <rdfs:isDefinedBy rdf:resource="http://rdaregistry.info/Elements/u/" />
  <reg:status rdf:resource="http://metadataregistry.org/uri/RegStatus/1001" />
  <reg:name xml:lang="en">filmDistributorOf</reg:name>
  <rdfs:label xml:lang="en">is film distributor of</rdfs:label>
  <skos:definition xml:lang="en">Relates an agent involved in distributing a moving image resource to theatres or other distribution channels to a resource.</skos:definition>
  <rdf:type rdf:resource="http://www.w3.org/1999/02/22-rdf-syntax-ns#Property" />
  <rdfs:subPropertyOf rdf:resource="http://rdaregistry.info/Elements/u/P60667" />
  <owl:inverseOf rdf:resource="http://rdaregistry.info/Elements/u/P60408" />
  <reg:hasSubproperty rdf:resource="http://rdaregistry.info/Elements/a/P50169" />
  <reg:lexicalAlias rdf:resource="http://rdaregistry.info/Elements/u/filmDistributorOf.en" />
</owl:ObjectProperty>

<!-- Property: is filmed with -->
<owl:ObjectProperty rdf:about="http://rdaregistry.info/Elements/u/P60258">
  <rdfs:isDefinedBy rdf:resource="http://rdaregistry.info/Elements/u/" />
  <reg:status rdf:resource="http://metadataregistry.org/uri/RegStatus/1001" />
  <reg:name xml:lang="en">filmedWith</reg:name>
  <rdfs:label xml:lang="en">is filmed with</rdfs:label>
  <skos:definition xml:lang="en">Relates a resource to a resource that is issued on the same microform with a resource being described.</skos:definition>
  <rdf:type rdf:resource="http://www.w3.org/1999/02/22-rdf-syntax-ns#Property" />
  <rdfs:subPropertyOf rdf:resource="http://rdaregistry.info/Elements/u/P60256" />
  <owl:inverseOf rdf:resource="http://rdaregistry.info/Elements/u/P60258" />
  <reg:hasSubproperty rdf:resource="http://rdaregistry.info/Elements/i/P40036" />
  <reg:hasSubproperty rdf:resource="http://rdaregistry.info/Elements/m/P30037" />
  <reg:lexicalAlias rdf:resource="http://rdaregistry.info/Elements/u/filmedWith.en" />
</owl:ObjectProperty>

<!-- Property: has filmmaker -->
<owl:ObjectProperty rdf:about="http://rdaregistry.info/Elements/u/P60436">
  <rdfs:isDefinedBy rdf:resource="http://rdaregistry.info/Elements/u/" />
  <reg:status rdf:resource="http://metadataregistry.org/uri/RegStatus/1001" />
  <reg:name xml:lang="en">filmmaker</reg:name>
  <rdfs:label xml:lang="en">has filmmaker</rdfs:label>
  <skos:definition xml:lang="en">Relates a resource to an agent responsible for creating an independent or personal film.</skos:definition>
  <rdf:type rdf:resource="http://www.w3.org/1999/02/22-rdf-syntax-ns#Property" />
  <rdfs:subPropertyOf rdf:resource="http://rdaregistry.info/Elements/u/P60447" />
  <owl:inverseOf rdf:resource="http://rdaregistry.info/Elements/u/P60665" />
  <reg:lexicalAlias rdf:resource="http://rdaregistry.info/Elements/u/filmmaker.en" />
</owl:ObjectProperty>

<!-- Property: is filmmaker of -->
<owl:ObjectProperty rdf:about="http://rdaregistry.info/Elements/u/P60665">
  <rdfs:isDefinedBy rdf:resource="http://rdaregistry.info/Elements/u/" />
  <reg:status rdf:resource="http://metadataregistry.org/uri/RegStatus/1001" />
  <reg:name xml:lang="en">filmmakerOf</reg:name>
  <rdfs:label xml:lang="en">is filmmaker of</rdfs:label>
  <skos:definition xml:lang="en">Relates an agent responsible for creating an independent or personal film to a resource.</skos:definition>
  <rdf:type rdf:resource="http://www.w3.org/1999/02/22-rdf-syntax-ns#Property" />
  <rdfs:subPropertyOf rdf:resource="http://rdaregistry.info/Elements/u/P60672" />
  <owl:inverseOf rdf:resource="http://rdaregistry.info/Elements/u/P60436" />
  <reg:hasSubproperty rdf:resource="http://rdaregistry.info/Elements/a/P50197" />
  <reg:lexicalAlias rdf:resource="http://rdaregistry.info/Elements/u/filmmakerOf.en" />
</owl:ObjectProperty>

<!-- Property: has film producer -->
<owl:ObjectProperty rdf:about="http://rdaregistry.info/Elements/u/P60169">
  <rdfs:isDefinedBy rdf:resource="http://rdaregistry.info/Elements/u/" />
  <reg:status rdf:resource="http://metadataregistry.org/uri/RegStatus/1001" />
  <reg:name xml:lang="en">filmProducer</reg:name>
  <rdfs:label xml:lang="en">has film producer</rdfs:label>
  <skos:definition xml:lang="en">Relates a resource to a producer responsible for most of the business aspects of a film.</skos:definition>
  <rdf:type rdf:resource="http://www.w3.org/1999/02/22-rdf-syntax-ns#Property" />
  <rdfs:subPropertyOf rdf:resource="http://rdaregistry.info/Elements/u/P60441" />
  <owl:inverseOf rdf:resource="http://rdaregistry.info/Elements/u/P60033" />
  <reg:lexicalAlias rdf:resource="http://rdaregistry.info/Elements/u/filmProducer.en" />
</owl:ObjectProperty>

<!-- Property: is film producer of -->
<owl:ObjectProperty rdf:about="http://rdaregistry.info/Elements/u/P60033">
  <rdfs:isDefinedBy rdf:resource="http://rdaregistry.info/Elements/u/" />
  <reg:status rdf:resource="http://metadataregistry.org/uri/RegStatus/1001" />
  <reg:name xml:lang="en">filmProducerOf</reg:name>
  <rdfs:label xml:lang="en">is film producer of</rdfs:label>
  <skos:definition xml:lang="en">Relates a producer responsible for most of the business aspects of a film to a resource.</skos:definition>
  <rdf:type rdf:resource="http://www.w3.org/1999/02/22-rdf-syntax-ns#Property" />
  <rdfs:subPropertyOf rdf:resource="http://rdaregistry.info/Elements/u/P60668" />
  <owl:inverseOf rdf:resource="http://rdaregistry.info/Elements/u/P60169" />
  <reg:hasSubproperty rdf:resource="http://rdaregistry.info/Elements/a/P50213" />
  <reg:lexicalAlias rdf:resource="http://rdaregistry.info/Elements/u/filmProducerOf.en" />
</owl:ObjectProperty>

<!-- Property: is finding aid -->
<owl:ObjectProperty rdf:about="http://rdaregistry.info/Elements/u/P60262">
  <rdfs:isDefinedBy rdf:resource="http://rdaregistry.info/Elements/u/" />
  <reg:status rdf:resource="http://metadataregistry.org/uri/RegStatus/1001" />
  <reg:name xml:lang="en">findingAid</reg:name>
  <rdfs:label xml:lang="en">is finding aid</rdfs:label>
  <skos:definition xml:lang="en">Relates a resource to a resource that provides a guide to an organization, arrangement, and contents of an archival collection.</skos:definition>
  <rdf:type rdf:resource="http://www.w3.org/1999/02/22-rdf-syntax-ns#Property" />
  <rdfs:subPropertyOf rdf:resource="http://rdaregistry.info/Elements/u/P60204" />
  <owl:inverseOf rdf:resource="http://rdaregistry.info/Elements/u/P60474" />
  <reg:hasSubproperty rdf:resource="http://rdaregistry.info/Elements/e/P20155" />
  <reg:lexicalAlias rdf:resource="http://rdaregistry.info/Elements/u/findingAid.en" />
</owl:ObjectProperty>

<!-- Property: is finding aid for -->
<owl:ObjectProperty rdf:about="http://rdaregistry.info/Elements/u/P60474">
  <rdfs:isDefinedBy rdf:resource="http://rdaregistry.info/Elements/u/" />
  <reg:status rdf:resource="http://metadataregistry.org/uri/RegStatus/1001" />
  <reg:name xml:lang="en">findingAidFor</reg:name>
  <rdfs:label xml:lang="en">is finding aid for</rdfs:label>
  <skos:definition xml:lang="en">Relates a resource to an archival collection that is described in a finding aid, i.e., a guide to an organization, arrangement, and contents of a collection.</skos:definition>
  <rdf:type rdf:resource="http://www.w3.org/1999/02/22-rdf-syntax-ns#Property" />
  <rdfs:subPropertyOf rdf:resource="http://rdaregistry.info/Elements/u/P60307" />
  <owl:inverseOf rdf:resource="http://rdaregistry.info/Elements/u/P60262" />
  <reg:hasSubproperty rdf:resource="http://rdaregistry.info/Elements/e/P20197" />
  <reg:lexicalAlias rdf:resource="http://rdaregistry.info/Elements/u/findingAidFor.en" />
</owl:ObjectProperty>

<!-- Property: has font size -->
<owl:ObjectProperty rdf:about="http://rdaregistry.info/Elements/u/P60582">
  <rdfs:isDefinedBy rdf:resource="http://rdaregistry.info/Elements/u/" />
  <reg:status rdf:resource="http://metadataregistry.org/uri/RegStatus/1001" />
  <reg:name xml:lang="en">fontSize</reg:name>
  <rdfs:label xml:lang="en">has font size</rdfs:label>
  <skos:definition xml:lang="en">Relates a resource to a size of the type used to represent characters and symbols in a resource.</skos:definition>
  <rdf:type rdf:resource="http://www.w3.org/1999/02/22-rdf-syntax-ns#Property" />
  <reg:hasSubproperty rdf:resource="http://rdaregistry.info/Elements/m/P30199" />
  <reg:lexicalAlias rdf:resource="http://rdaregistry.info/Elements/u/fontSize.en" />
</owl:ObjectProperty>

<!-- Property: has format of notated music -->
<owl:ObjectProperty rdf:about="http://rdaregistry.info/Elements/u/P60488">
  <rdfs:isDefinedBy rdf:resource="http://rdaregistry.info/Elements/u/" />
  <reg:status rdf:resource="http://metadataregistry.org/uri/RegStatus/1001" />
  <reg:name xml:lang="en">formatOfNotatedMusic</reg:name>
  <rdfs:label xml:lang="en">has format of notated music</rdfs:label>
  <skos:definition xml:lang="en">Relates a resource to a musical or physical layout of the content of a resource that is presented in the form of musical notation.</skos:definition>
  <rdf:type rdf:resource="http://www.w3.org/1999/02/22-rdf-syntax-ns#Property" />
  <reg:hasSubproperty rdf:resource="http://rdaregistry.info/Elements/e/P20209" />
  <reg:lexicalAlias rdf:resource="http://rdaregistry.info/Elements/u/formatOfNotatedMusic.en" />
</owl:ObjectProperty>

<!-- Property: has former owner -->
<owl:ObjectProperty rdf:about="http://rdaregistry.info/Elements/u/P60401">
  <rdfs:isDefinedBy rdf:resource="http://rdaregistry.info/Elements/u/" />
  <reg:status rdf:resource="http://metadataregistry.org/uri/RegStatus/1001" />
  <reg:name xml:lang="en">formerOwner</reg:name>
  <rdfs:label xml:lang="en">has former owner</rdfs:label>
  <skos:definition xml:lang="en">Relates a resource to an agent formerly having legal possession of a resource.</skos:definition>
  <rdf:type rdf:resource="http://www.w3.org/1999/02/22-rdf-syntax-ns#Property" />
  <rdfs:subPropertyOf rdf:resource="http://rdaregistry.info/Elements/u/P60404" />
  <owl:inverseOf rdf:resource="http://rdaregistry.info/Elements/u/P60630" />
  <reg:hasSubproperty rdf:resource="http://rdaregistry.info/Elements/u/P60091" />
  <reg:hasSubproperty rdf:resource="http://rdaregistry.info/Elements/u/P60092" />
  <reg:hasSubproperty rdf:resource="http://rdaregistry.info/Elements/i/P40019" />
  <reg:lexicalAlias rdf:resource="http://rdaregistry.info/Elements/u/formerOwner.en" />
</owl:ObjectProperty>

<!-- Property: is former owner of -->
<owl:ObjectProperty rdf:about="http://rdaregistry.info/Elements/u/P60630">
  <rdfs:isDefinedBy rdf:resource="http://rdaregistry.info/Elements/u/" />
  <reg:status rdf:resource="http://metadataregistry.org/uri/RegStatus/1001" />
  <reg:name xml:lang="en">formerOwnerOf</reg:name>
  <rdfs:label xml:lang="en">is former owner of</rdfs:label>
  <skos:definition xml:lang="en">Relates an agent formerly having legal possession of a resource to a resource.</skos:definition>
  <rdf:type rdf:resource="http://www.w3.org/1999/02/22-rdf-syntax-ns#Property" />
  <rdfs:subPropertyOf rdf:resource="http://rdaregistry.info/Elements/u/P60632" />
  <owl:inverseOf rdf:resource="http://rdaregistry.info/Elements/u/P60401" />
  <reg:hasSubproperty rdf:resource="http://rdaregistry.info/Elements/u/P60012" />
  <reg:hasSubproperty rdf:resource="http://rdaregistry.info/Elements/u/P60013" />
  <reg:hasSubproperty rdf:resource="http://rdaregistry.info/Elements/a/P50163" />
  <reg:lexicalAlias rdf:resource="http://rdaregistry.info/Elements/u/formerOwnerOf.en" />
</owl:ObjectProperty>

<!-- Property: has form of musical notation -->
<owl:ObjectProperty rdf:about="http://rdaregistry.info/Elements/u/P60321">
  <rdfs:isDefinedBy rdf:resource="http://rdaregistry.info/Elements/u/" />
  <reg:status rdf:resource="http://metadataregistry.org/uri/RegStatus/1001" />
  <reg:name xml:lang="en">formOfMusicalNotation</reg:name>
  <rdfs:label xml:lang="en">has form of musical notation</rdfs:label>
  <skos:definition xml:lang="en">Relates a resource to a set of characters or symbols used to express musical content of a resource.</skos:definition>
  <rdf:type rdf:resource="http://www.w3.org/1999/02/22-rdf-syntax-ns#Property" />
  <rdfs:subPropertyOf rdf:resource="http://rdaregistry.info/Elements/u/P60319" />
  <reg:hasSubproperty rdf:resource="http://rdaregistry.info/Elements/e/P20064" />
  <reg:lexicalAlias rdf:resource="http://rdaregistry.info/Elements/u/formOfMusicalNotation.en" />
</owl:ObjectProperty>

<!-- Property: has form of notated movement -->
<owl:ObjectProperty rdf:about="http://rdaregistry.info/Elements/u/P60320">
  <rdfs:isDefinedBy rdf:resource="http://rdaregistry.info/Elements/u/" />
  <reg:status rdf:resource="http://metadataregistry.org/uri/RegStatus/1001" />
  <reg:name xml:lang="en">formOfNotatedMovement</reg:name>
  <rdfs:label xml:lang="en">has form of notated movement</rdfs:label>
  <skos:definition xml:lang="en">Relates a resource to a set of characters or symbols used to express movement content of a resource.</skos:definition>
  <rdf:type rdf:resource="http://www.w3.org/1999/02/22-rdf-syntax-ns#Property" />
  <rdfs:subPropertyOf rdf:resource="http://rdaregistry.info/Elements/u/P60319" />
  <reg:hasSubproperty rdf:resource="http://rdaregistry.info/Elements/e/P20063" />
  <reg:lexicalAlias rdf:resource="http://rdaregistry.info/Elements/u/formOfNotatedMovement.en" />
</owl:ObjectProperty>

<!-- Property: has form of notation -->
<owl:ObjectProperty rdf:about="http://rdaregistry.info/Elements/u/P60319">
  <rdfs:isDefinedBy rdf:resource="http://rdaregistry.info/Elements/u/" />
  <reg:status rdf:resource="http://metadataregistry.org/uri/RegStatus/1001" />
  <reg:name xml:lang="en">formOfNotation</reg:name>
  <rdfs:label xml:lang="en">has form of notation</rdfs:label>
  <skos:definition xml:lang="en">Relates a resource to a set of characters or symbols used to express the content of a resource.</skos:definition>
  <rdf:type rdf:resource="http://www.w3.org/1999/02/22-rdf-syntax-ns#Property" />
  <reg:hasSubproperty rdf:resource="http://rdaregistry.info/Elements/u/P60318" />
  <reg:hasSubproperty rdf:resource="http://rdaregistry.info/Elements/u/P60320" />
  <reg:hasSubproperty rdf:resource="http://rdaregistry.info/Elements/u/P60321" />
  <reg:hasSubproperty rdf:resource="http://rdaregistry.info/Elements/u/P60322" />
  <reg:hasSubproperty rdf:resource="http://rdaregistry.info/Elements/e/P20062" />
  <reg:lexicalAlias rdf:resource="http://rdaregistry.info/Elements/u/formOfNotation.en" />
</owl:ObjectProperty>

<!-- Property: has form of resource -->
<owl:ObjectProperty rdf:about="http://rdaregistry.info/Elements/u/P60058">
  <rdfs:isDefinedBy rdf:resource="http://rdaregistry.info/Elements/u/" />
  <reg:status rdf:resource="http://metadataregistry.org/uri/RegStatus/1001" />
  <reg:name xml:lang="en">formOfResource</reg:name>
  <rdfs:label xml:lang="en">has form of resource</rdfs:label>
  <skos:definition xml:lang="en">Relates a resource to a class or genre to which a resource belongs.</skos:definition>
  <rdf:type rdf:resource="http://www.w3.org/1999/02/22-rdf-syntax-ns#Property" />
  <reg:lexicalAlias rdf:resource="http://rdaregistry.info/Elements/u/formOfResource.en" />
</owl:ObjectProperty>

<!-- Property: has form of tactile notation -->
<owl:ObjectProperty rdf:about="http://rdaregistry.info/Elements/u/P60318">
  <rdfs:isDefinedBy rdf:resource="http://rdaregistry.info/Elements/u/" />
  <reg:status rdf:resource="http://metadataregistry.org/uri/RegStatus/1001" />
  <reg:name xml:lang="en">formOfTactileNotation</reg:name>
  <rdfs:label xml:lang="en">has form of tactile notation</rdfs:label>
  <skos:definition xml:lang="en">Relates a resource to a set of characters or symbols used to express the content of a resource in a form that can be perceived through touch.</skos:definition>
  <rdf:type rdf:resource="http://www.w3.org/1999/02/22-rdf-syntax-ns#Property" />
  <rdfs:subPropertyOf rdf:resource="http://rdaregistry.info/Elements/u/P60319" />
  <reg:hasSubproperty rdf:resource="http://rdaregistry.info/Elements/e/P20061" />
  <reg:lexicalAlias rdf:resource="http://rdaregistry.info/Elements/u/formOfTactileNotation.en" />
</owl:ObjectProperty>

<!-- Property: has founded entity -->
<owl:ObjectProperty rdf:about="http://rdaregistry.info/Elements/u/P60687">
  <rdfs:isDefinedBy rdf:resource="http://rdaregistry.info/Elements/u/" />
  <reg:status rdf:resource="http://metadataregistry.org/uri/RegStatus/1001" />
  <reg:name xml:lang="en">foundedEntity</reg:name>
  <rdfs:label xml:lang="en">has founded entity</rdfs:label>
  <skos:definition xml:lang="en">Relates an agent that an agent founded to an agent.</skos:definition>
  <rdf:type rdf:resource="http://www.w3.org/1999/02/22-rdf-syntax-ns#Property" />
  <owl:inverseOf rdf:resource="http://rdaregistry.info/Elements/u/P60694" />
  <reg:hasSubproperty rdf:resource="http://rdaregistry.info/Elements/a/P50017" />
  <reg:hasSubproperty rdf:resource="http://rdaregistry.info/Elements/a/P50062" />
  <reg:hasSubproperty rdf:resource="http://rdaregistry.info/Elements/a/P50112" />
  <reg:lexicalAlias rdf:resource="http://rdaregistry.info/Elements/u/foundedEntity.en" />
</owl:ObjectProperty>

<!-- Property: has founder -->
<owl:ObjectProperty rdf:about="http://rdaregistry.info/Elements/u/P60694">
  <rdfs:isDefinedBy rdf:resource="http://rdaregistry.info/Elements/u/" />
  <reg:status rdf:resource="http://metadataregistry.org/uri/RegStatus/1001" />
  <reg:name xml:lang="en">founder</reg:name>
  <rdfs:label xml:lang="en">has founder</rdfs:label>
  <skos:definition xml:lang="en">Relates an agent who founded an agent to an agent.</skos:definition>
  <rdf:type rdf:resource="http://www.w3.org/1999/02/22-rdf-syntax-ns#Property" />
  <owl:inverseOf rdf:resource="http://rdaregistry.info/Elements/u/P60687" />
  <reg:hasSubproperty rdf:resource="http://rdaregistry.info/Elements/a/P50007" />
  <reg:hasSubproperty rdf:resource="http://rdaregistry.info/Elements/a/P50020" />
  <reg:hasSubproperty rdf:resource="http://rdaregistry.info/Elements/a/P50029" />
  <reg:lexicalAlias rdf:resource="http://rdaregistry.info/Elements/u/founder.en" />
</owl:ObjectProperty>

<!-- Property: has founder of resource -->
<owl:ObjectProperty rdf:about="http://rdaregistry.info/Elements/u/P60871">
  <rdfs:isDefinedBy rdf:resource="http://rdaregistry.info/Elements/u/" />
  <reg:status rdf:resource="http://metadataregistry.org/uri/RegStatus/1001" />
  <rdf:type rdf:resource="http://www.w3.org/1999/02/22-rdf-syntax-ns#Property" />
  <reg:name xml:lang="en">founderOfResource</reg:name>
  <rdfs:label xml:lang="en">has founder of resource</rdfs:label>
  <reg:lexicalAlias rdf:resource="http://rdaregistry.info/Elements/u/founderOfResource.en" />
  <skos:definition xml:lang="en">Relates a resource to an agent responsible for establishing a serial, integrating resource, or multipart monographic resource.</skos:definition>
  <owl:inverseOf rdf:resource="http://rdaregistry.info/Elements/u/P60872" />
  <reg:hasSubproperty rdf:resource="http://rdaregistry.info/Elements/w/P10299" />
  <rdfs:subPropertyOf rdf:resource="http://rdaregistry.info/Elements/u/P60374" />
</owl:ObjectProperty>

<!-- Property: is founder of resource of -->
<owl:ObjectProperty rdf:about="http://rdaregistry.info/Elements/u/P60872">
  <rdfs:isDefinedBy rdf:resource="http://rdaregistry.info/Elements/u/" />
  <reg:status rdf:resource="http://metadataregistry.org/uri/RegStatus/1001" />
  <rdf:type rdf:resource="http://www.w3.org/1999/02/22-rdf-syntax-ns#Property" />
  <reg:name xml:lang="en">founderOfResourceOf</reg:name>
  <rdfs:label xml:lang="en">is founder of resource of</rdfs:label>
  <reg:lexicalAlias rdf:resource="http://rdaregistry.info/Elements/u/founderOfResourceOf.en" />
  <skos:definition xml:lang="en">Relates an agent responsible for establishing a serial, integrating resource, or multipart monograph to a resource.</skos:definition>
  <owl:inverseOf rdf:resource="http://rdaregistry.info/Elements/u/P60871" />
  <rdfs:subPropertyOf rdf:resource="http://rdaregistry.info/Elements/u/P60602" />
</owl:ObjectProperty>

<!-- Property: is freely translated as -->
<owl:ObjectProperty rdf:about="http://rdaregistry.info/Elements/u/P60189">
  <rdfs:isDefinedBy rdf:resource="http://rdaregistry.info/Elements/u/" />
  <reg:status rdf:resource="http://metadataregistry.org/uri/RegStatus/1001" />
  <reg:name xml:lang="en">freelyTranslatedAs</reg:name>
  <rdfs:label xml:lang="en">is freely translated as</rdfs:label>
  <skos:definition xml:lang="en">Relates a resource to a resource that is both an adaptation and a translation into another language of a source resource.</skos:definition>
  <rdf:type rdf:resource="http://www.w3.org/1999/02/22-rdf-syntax-ns#Property" />
  <rdfs:subPropertyOf rdf:resource="http://rdaregistry.info/Elements/u/P60250" />
  <owl:inverseOf rdf:resource="http://rdaregistry.info/Elements/u/P60243" />
  <reg:hasSubproperty rdf:resource="http://rdaregistry.info/Elements/e/P20119" />
  <reg:lexicalAlias rdf:resource="http://rdaregistry.info/Elements/u/freelyTranslatedAs.en" />
</owl:ObjectProperty>

<!-- Property: is free translation of -->
<owl:ObjectProperty rdf:about="http://rdaregistry.info/Elements/u/P60243">
  <rdfs:isDefinedBy rdf:resource="http://rdaregistry.info/Elements/u/" />
  <reg:status rdf:resource="http://metadataregistry.org/uri/RegStatus/1001" />
  <reg:name xml:lang="en">freeTranslationOf</reg:name>
  <rdfs:label xml:lang="en">is free translation of</rdfs:label>
  <skos:definition xml:lang="en">Relates a resource to a resource that has been adapted and translated into another language.</skos:definition>
  <rdf:type rdf:resource="http://www.w3.org/1999/02/22-rdf-syntax-ns#Property" />
  <rdfs:subPropertyOf rdf:resource="http://rdaregistry.info/Elements/u/P60305" />
  <owl:inverseOf rdf:resource="http://rdaregistry.info/Elements/u/P60189" />
  <reg:hasSubproperty rdf:resource="http://rdaregistry.info/Elements/e/P20140" />
  <reg:lexicalAlias rdf:resource="http://rdaregistry.info/Elements/u/freeTranslationOf.en" />
</owl:ObjectProperty>

<!-- Property: has frequency -->
<owl:ObjectProperty rdf:about="http://rdaregistry.info/Elements/u/P60538">
  <rdfs:isDefinedBy rdf:resource="http://rdaregistry.info/Elements/u/" />
  <reg:status rdf:resource="http://metadataregistry.org/uri/RegStatus/1001" />
  <reg:name xml:lang="en">frequency</reg:name>
  <rdfs:label xml:lang="en">has frequency</rdfs:label>
  <skos:definition xml:lang="en">Relates a resource to an interval at which an issue or part of a serial or an update to an integrating resource is issued.</skos:definition>
  <rdf:type rdf:resource="http://www.w3.org/1999/02/22-rdf-syntax-ns#Property" />
  <reg:hasSubproperty rdf:resource="http://rdaregistry.info/Elements/m/P30168" />
  <reg:lexicalAlias rdf:resource="http://rdaregistry.info/Elements/u/frequency.en" />
</owl:ObjectProperty>

<!-- Property: has friend -->
<owl:ObjectProperty rdf:about="http://rdaregistry.info/Elements/u/P60854">
  <rdfs:isDefinedBy rdf:resource="http://rdaregistry.info/Elements/u/" />
  <reg:status rdf:resource="http://metadataregistry.org/uri/RegStatus/1001" />
  <rdf:type rdf:resource="http://www.w3.org/1999/02/22-rdf-syntax-ns#Property" />
  <reg:name xml:lang="en">friend</reg:name>
  <rdfs:label xml:lang="en">has friend</rdfs:label>
  <reg:lexicalAlias rdf:resource="http://rdaregistry.info/Elements/u/friend.en" />
  <skos:definition xml:lang="en">Relates an agent to an agent who shares a bond of mutual affection or regard with another agent.</skos:definition>
  <owl:inverseOf rdf:resource="http://rdaregistry.info/Elements/u/P60854" />
  <reg:hasSubproperty rdf:resource="http://rdaregistry.info/Elements/a/P50280" />
  <rdfs:subPropertyOf rdf:resource="http://rdaregistry.info/Elements/u/P60454" />
</owl:ObjectProperty>

<!-- Property: has fuller form of name -->
<owl:ObjectProperty rdf:about="http://rdaregistry.info/Elements/u/P60530">
  <rdfs:isDefinedBy rdf:resource="http://rdaregistry.info/Elements/u/" />
  <reg:status rdf:resource="http://metadataregistry.org/uri/RegStatus/1001" />
  <reg:name xml:lang="en">fullerFormOfName</reg:name>
  <rdfs:label xml:lang="en">has fuller form of name</rdfs:label>
  <skos:definition xml:lang="en">Relates a resource to a full form of a part of a name represented only by an initial or abbreviation in a form chosen as a preferred name, or a part of a name not included in a form chosen as a preferred name.</skos:definition>
  <rdf:type rdf:resource="http://www.w3.org/1999/02/22-rdf-syntax-ns#Property" />
  <reg:hasSubproperty rdf:resource="http://rdaregistry.info/Elements/a/P50115" />
  <reg:lexicalAlias rdf:resource="http://rdaregistry.info/Elements/u/fullerFormOfName.en" />
</owl:ObjectProperty>

<!-- Property: has gender -->
<owl:ObjectProperty rdf:about="http://rdaregistry.info/Elements/u/P60531">
  <rdfs:isDefinedBy rdf:resource="http://rdaregistry.info/Elements/u/" />
  <reg:status rdf:resource="http://metadataregistry.org/uri/RegStatus/1001" />
  <reg:name xml:lang="en">gender</reg:name>
  <rdfs:label xml:lang="en">has gender</rdfs:label>
  <skos:definition xml:lang="en">Relates a resource to a gender with which an agent identifies.</skos:definition>
  <rdf:type rdf:resource="http://www.w3.org/1999/02/22-rdf-syntax-ns#Property" />
  <reg:hasSubproperty rdf:resource="http://rdaregistry.info/Elements/a/P50116" />
  <reg:lexicalAlias rdf:resource="http://rdaregistry.info/Elements/u/gender.en" />
</owl:ObjectProperty>

<!-- Property: has generation -->
<owl:ObjectProperty rdf:about="http://rdaregistry.info/Elements/u/P60568">
  <rdfs:isDefinedBy rdf:resource="http://rdaregistry.info/Elements/u/" />
  <reg:status rdf:resource="http://metadataregistry.org/uri/RegStatus/1001" />
  <reg:name xml:lang="en">generation</reg:name>
  <rdfs:label xml:lang="en">has generation</rdfs:label>
  <skos:definition xml:lang="en">Relates a resource to a relationship between an original carrier and a carrier of a reproduction made from an original.</skos:definition>
  <rdf:type rdf:resource="http://www.w3.org/1999/02/22-rdf-syntax-ns#Property" />
  <reg:hasSubproperty rdf:resource="http://rdaregistry.info/Elements/u/P60567" />
  <reg:hasSubproperty rdf:resource="http://rdaregistry.info/Elements/u/P60569" />
  <reg:hasSubproperty rdf:resource="http://rdaregistry.info/Elements/u/P60570" />
  <reg:hasSubproperty rdf:resource="http://rdaregistry.info/Elements/u/P60571" />
  <reg:hasSubproperty rdf:resource="http://rdaregistry.info/Elements/u/P60572" />
  <reg:hasSubproperty rdf:resource="http://rdaregistry.info/Elements/m/P30191" />
  <reg:lexicalAlias rdf:resource="http://rdaregistry.info/Elements/u/generation.en" />
</owl:ObjectProperty>

<!-- Property: DEPRECATED -->
<owl:ObjectProperty rdf:about="http://rdaregistry.info/Elements/u/P60567">
  <rdfs:isDefinedBy rdf:resource="http://rdaregistry.info/Elements/u/" />
  <reg:status rdf:resource="http://metadataregistry.org/uri/RegStatus/1008" />
  <reg:name xml:lang="en">generationOfAudioRecording</reg:name>
  <skos:definition xml:lang="en">Relates a resource to the relationship between an original audio carrier and the carrier of a reproduction made from the original (e.g., a tape duplication master, a test pressing).</skos:definition>
  <rdf:type rdf:resource="http://www.w3.org/1999/02/22-rdf-syntax-ns#Property" />
  <rdfs:subPropertyOf rdf:resource="http://rdaregistry.info/Elements/u/P60568" />
  <reg:hasSubproperty rdf:resource="http://rdaregistry.info/Elements/m/P30190" />
  <reg:lexicalAlias rdf:resource="http://rdaregistry.info/Elements/u/generationOfAudioRecording.en" />
</owl:ObjectProperty>

<!-- Property: DEPRECATED -->
<owl:ObjectProperty rdf:about="http://rdaregistry.info/Elements/u/P60569">
  <rdfs:isDefinedBy rdf:resource="http://rdaregistry.info/Elements/u/" />
  <reg:status rdf:resource="http://metadataregistry.org/uri/RegStatus/1008" />
  <reg:name xml:lang="en">generationOfDigitalResource</reg:name>
  <skos:definition xml:lang="en">Relates a resource to the relationship between an original carrier of a digital resource and the carrier of a reproduction made from the original (e.g., a derivative master).</skos:definition>
  <rdf:type rdf:resource="http://www.w3.org/1999/02/22-rdf-syntax-ns#Property" />
  <rdfs:subPropertyOf rdf:resource="http://rdaregistry.info/Elements/u/P60568" />
  <reg:hasSubproperty rdf:resource="http://rdaregistry.info/Elements/m/P30192" />
  <reg:lexicalAlias rdf:resource="http://rdaregistry.info/Elements/u/generationOfDigitalResource.en" />
</owl:ObjectProperty>

<!-- Property: DEPRECATED -->
<owl:ObjectProperty rdf:about="http://rdaregistry.info/Elements/u/P60572">
  <rdfs:isDefinedBy rdf:resource="http://rdaregistry.info/Elements/u/" />
  <reg:status rdf:resource="http://metadataregistry.org/uri/RegStatus/1008" />
  <reg:name xml:lang="en">generationOfMicroform</reg:name>
  <skos:definition xml:lang="en">Relates a resource to the relationship between an original microform carrier and the carrier of a reproduction made from the original (e.g., a printing master).</skos:definition>
  <rdf:type rdf:resource="http://www.w3.org/1999/02/22-rdf-syntax-ns#Property" />
  <rdfs:subPropertyOf rdf:resource="http://rdaregistry.info/Elements/u/P60568" />
  <reg:hasSubproperty rdf:resource="http://rdaregistry.info/Elements/m/P30195" />
  <reg:lexicalAlias rdf:resource="http://rdaregistry.info/Elements/u/generationOfMicroform.en" />
</owl:ObjectProperty>

<!-- Property: DEPRECATED -->
<owl:ObjectProperty rdf:about="http://rdaregistry.info/Elements/u/P60570">
  <rdfs:isDefinedBy rdf:resource="http://rdaregistry.info/Elements/u/" />
  <reg:status rdf:resource="http://metadataregistry.org/uri/RegStatus/1008" />
  <reg:name xml:lang="en">generationOfMotionPictureFilm</reg:name>
  <skos:definition xml:lang="en">Relates a resource to the relationship between an original carrier of a motion picture film resource and the carrier of a reproduction made from the original (e.g., a reference print).</skos:definition>
  <rdf:type rdf:resource="http://www.w3.org/1999/02/22-rdf-syntax-ns#Property" />
  <rdfs:subPropertyOf rdf:resource="http://rdaregistry.info/Elements/u/P60568" />
  <reg:hasSubproperty rdf:resource="http://rdaregistry.info/Elements/m/P30193" />
  <reg:lexicalAlias rdf:resource="http://rdaregistry.info/Elements/u/generationOfMotionPictureFilm.en" />
</owl:ObjectProperty>

<!-- Property: DEPRECATED -->
<owl:ObjectProperty rdf:about="http://rdaregistry.info/Elements/u/P60571">
  <rdfs:isDefinedBy rdf:resource="http://rdaregistry.info/Elements/u/" />
  <reg:status rdf:resource="http://metadataregistry.org/uri/RegStatus/1008" />
  <reg:name xml:lang="en">generationOfVideotape</reg:name>
  <skos:definition xml:lang="en">Relates a resource to the relationship between an original carrier of a videotape resource and the carrier of a reproduction made from the original (e.g., a show copy).</skos:definition>
  <rdf:type rdf:resource="http://www.w3.org/1999/02/22-rdf-syntax-ns#Property" />
  <rdfs:subPropertyOf rdf:resource="http://rdaregistry.info/Elements/u/P60568" />
  <reg:hasSubproperty rdf:resource="http://rdaregistry.info/Elements/m/P30194" />
  <reg:lexicalAlias rdf:resource="http://rdaregistry.info/Elements/u/generationOfVideotape.en" />
</owl:ObjectProperty>

<!-- Property: has given name -->
<owl:ObjectProperty rdf:about="http://rdaregistry.info/Elements/u/P60879">
  <rdfs:isDefinedBy rdf:resource="http://rdaregistry.info/Elements/u/" />
  <reg:status rdf:resource="http://metadataregistry.org/uri/RegStatus/1001" />
  <rdf:type rdf:resource="http://www.w3.org/1999/02/22-rdf-syntax-ns#Property" />
  <reg:name xml:lang="en">givenName</reg:name>
  <rdfs:label xml:lang="en">has given name</rdfs:label>
  <reg:lexicalAlias rdf:resource="http://rdaregistry.info/Elements/u/givenName.en" />
  <skos:definition xml:lang="en">Relates an agent to a name given to an agent at birth or at some later point in addition to, or instead of, a surname.</skos:definition>
  <reg:hasSubproperty rdf:resource="http://rdaregistry.info/Elements/a/P50292" />
</owl:ObjectProperty>

<!-- Property: has graduate -->
<owl:ObjectProperty rdf:about="http://rdaregistry.info/Elements/u/P60807">
  <rdfs:isDefinedBy rdf:resource="http://rdaregistry.info/Elements/u/" />
  <reg:status rdf:resource="http://metadataregistry.org/uri/RegStatus/1001" />
  <rdf:type rdf:resource="http://www.w3.org/1999/02/22-rdf-syntax-ns#Property" />
  <reg:name xml:lang="en">graduate</reg:name>
  <rdfs:label xml:lang="en">has graduate</rdfs:label>
  <reg:lexicalAlias rdf:resource="http://rdaregistry.info/Elements/u/graduate.en" />
  <skos:definition xml:lang="en">Relates an agent to an agent who receives an academic degree from a granting institution or faculty.</skos:definition>
  <owl:inverseOf rdf:resource="http://rdaregistry.info/Elements/u/P60808" />
</owl:ObjectProperty>

<!-- Property: is graduate of -->
<owl:ObjectProperty rdf:about="http://rdaregistry.info/Elements/u/P60808">
  <rdfs:isDefinedBy rdf:resource="http://rdaregistry.info/Elements/u/" />
  <reg:status rdf:resource="http://metadataregistry.org/uri/RegStatus/1001" />
  <rdf:type rdf:resource="http://www.w3.org/1999/02/22-rdf-syntax-ns#Property" />
  <reg:name xml:lang="en">graduateOf</reg:name>
  <rdfs:label xml:lang="en">is graduate of</rdfs:label>
  <reg:lexicalAlias rdf:resource="http://rdaregistry.info/Elements/u/graduateOf.en" />
  <skos:definition xml:lang="en">Relates an agent to an institution or faculty that granted an academic degree to an agent.</skos:definition>
  <owl:inverseOf rdf:resource="http://rdaregistry.info/Elements/u/P60807" />
</owl:ObjectProperty>

<!-- Property: has granting institution or faculty -->
<owl:ObjectProperty rdf:about="http://rdaregistry.info/Elements/u/P60483">
  <rdfs:isDefinedBy rdf:resource="http://rdaregistry.info/Elements/u/" />
  <reg:status rdf:resource="http://metadataregistry.org/uri/RegStatus/1001" />
  <reg:name xml:lang="en">grantingInstitutionOrFaculty</reg:name>
  <rdfs:label xml:lang="en">has granting institution or faculty</rdfs:label>
  <skos:definition xml:lang="en">Relates a resource to an institution or faculty conferring an academic degree on a candidate.</skos:definition>
  <rdf:type rdf:resource="http://www.w3.org/1999/02/22-rdf-syntax-ns#Property" />
  <reg:lexicalAlias rdf:resource="http://rdaregistry.info/Elements/u/grantingInstitutionOrFaculty.en" />
</owl:ObjectProperty>

<!-- Property: is graphic novelization of -->
<owl:ObjectProperty rdf:about="http://rdaregistry.info/Elements/u/P60743">
  <rdfs:isDefinedBy rdf:resource="http://rdaregistry.info/Elements/u/" />
  <reg:status rdf:resource="http://metadataregistry.org/uri/RegStatus/1001" />
  <rdf:type rdf:resource="http://www.w3.org/1999/02/22-rdf-syntax-ns#Property" />
  <reg:name xml:lang="en">graphicNovelizationOf</reg:name>
  <rdfs:label xml:lang="en">is graphic novelization of</rdfs:label>
  <reg:lexicalAlias rdf:resource="http://rdaregistry.info/Elements/u/graphicNovelizationOf.en" />
  <skos:definition xml:lang="en">Relates a resourcce to a resource that has been adapted as a graphic novel.</skos:definition>
  <owl:inverseOf rdf:resource="http://rdaregistry.info/Elements/u/P60742" />
  <rdfs:subPropertyOf rdf:resource="http://rdaregistry.info/Elements/u/P60241" />
</owl:ObjectProperty>

<!-- Property: has groove characteristic -->
<owl:ObjectProperty rdf:about="http://rdaregistry.info/Elements/u/P60532">
  <rdfs:isDefinedBy rdf:resource="http://rdaregistry.info/Elements/u/" />
  <reg:status rdf:resource="http://metadataregistry.org/uri/RegStatus/1001" />
  <reg:name xml:lang="en">grooveCharacteristic</reg:name>
  <rdfs:label xml:lang="en">has groove characteristic</rdfs:label>
  <skos:definition xml:lang="en">Relates a resource to a groove width of an analog disc or a groove pitch of an analog cylinder.</skos:definition>
  <rdf:type rdf:resource="http://www.w3.org/1999/02/22-rdf-syntax-ns#Property" />
  <rdfs:subPropertyOf rdf:resource="http://rdaregistry.info/Elements/u/P60351" />
  <reg:hasSubproperty rdf:resource="http://rdaregistry.info/Elements/m/P30164" />
  <reg:lexicalAlias rdf:resource="http://rdaregistry.info/Elements/u/grooveCharacteristic.en" />
</owl:ObjectProperty>

<!-- Property: is guide -->
<owl:ObjectProperty rdf:about="http://rdaregistry.info/Elements/u/P60222">
  <rdfs:isDefinedBy rdf:resource="http://rdaregistry.info/Elements/u/" />
  <reg:status rdf:resource="http://metadataregistry.org/uri/RegStatus/1001" />
  <reg:name xml:lang="en">guide</reg:name>
  <rdfs:label xml:lang="en">is guide</rdfs:label>
  <skos:definition xml:lang="en">Relates a resource to a resource that guides a user through the use of a predominant resource, using notes, learning and study aids, exercises, problems, questions and answers, instructor or student materials, etc.</skos:definition>
  <rdf:type rdf:resource="http://www.w3.org/1999/02/22-rdf-syntax-ns#Property" />
  <rdfs:subPropertyOf rdf:resource="http://rdaregistry.info/Elements/u/P60204" />
  <owl:inverseOf rdf:resource="http://rdaregistry.info/Elements/u/P60252" />
  <reg:hasSubproperty rdf:resource="http://rdaregistry.info/Elements/e/P20120" />
  <reg:lexicalAlias rdf:resource="http://rdaregistry.info/Elements/u/guide.en" />
</owl:ObjectProperty>

<!-- Property: is guide to -->
<owl:ObjectProperty rdf:about="http://rdaregistry.info/Elements/u/P60252">
  <rdfs:isDefinedBy rdf:resource="http://rdaregistry.info/Elements/u/" />
  <reg:status rdf:resource="http://metadataregistry.org/uri/RegStatus/1001" />
  <reg:name xml:lang="en">guideTo</reg:name>
  <rdfs:label xml:lang="en">is guide to</rdfs:label>
  <skos:definition xml:lang="en">Relates a resource to a resource that is augmented by another resource consisting of material, such as notes, learning and study aids, exercises, problems, questions and answers, instructor or student materials, etc., to help a user of a predominant resource.</skos:definition>
  <rdf:type rdf:resource="http://www.w3.org/1999/02/22-rdf-syntax-ns#Property" />
  <rdfs:subPropertyOf rdf:resource="http://rdaregistry.info/Elements/u/P60307" />
  <owl:inverseOf rdf:resource="http://rdaregistry.info/Elements/u/P60222" />
  <reg:hasSubproperty rdf:resource="http://rdaregistry.info/Elements/e/P20147" />
  <reg:lexicalAlias rdf:resource="http://rdaregistry.info/Elements/u/guideTo.en" />
</owl:ObjectProperty>

<!-- Property: has hereditary title -->
<owl:ObjectProperty rdf:about="http://rdaregistry.info/Elements/u/P60356">
  <rdfs:isDefinedBy rdf:resource="http://rdaregistry.info/Elements/u/" />
  <reg:status rdf:resource="http://metadataregistry.org/uri/RegStatus/1001" />
  <reg:name xml:lang="en">hereditaryTitle</reg:name>
  <rdfs:label xml:lang="en">has hereditary title</rdfs:label>
  <skos:definition xml:lang="en">Relates a resource to a title of nobility, etc., associated with an agent.</skos:definition>
  <rdf:type rdf:resource="http://www.w3.org/1999/02/22-rdf-syntax-ns#Property" />
  <reg:hasSubproperty rdf:resource="http://rdaregistry.info/Elements/a/P50059" />
  <reg:lexicalAlias rdf:resource="http://rdaregistry.info/Elements/u/hereditaryTitle.en" />
</owl:ObjectProperty>

<!-- Property: has hierarchical subordinate -->
<owl:ObjectProperty rdf:about="http://rdaregistry.info/Elements/u/P60681">
  <rdfs:isDefinedBy rdf:resource="http://rdaregistry.info/Elements/u/" />
  <reg:status rdf:resource="http://metadataregistry.org/uri/RegStatus/1001" />
  <reg:name xml:lang="en">hierarchicalSubordinate</reg:name>
  <rdfs:label xml:lang="en">has hierarchical subordinate</rdfs:label>
  <skos:definition xml:lang="en">Relates an agent that is subordinate to another agent to an agent.</skos:definition>
  <rdf:type rdf:resource="http://www.w3.org/1999/02/22-rdf-syntax-ns#Property" />
  <owl:inverseOf rdf:resource="http://rdaregistry.info/Elements/u/P60680" />
  <reg:hasSubproperty rdf:resource="http://rdaregistry.info/Elements/a/P50010" />
  <reg:lexicalAlias rdf:resource="http://rdaregistry.info/Elements/u/hierarchicalSubordinate.en" />
</owl:ObjectProperty>

<!-- Property: has hierarchical superior -->
<owl:ObjectProperty rdf:about="http://rdaregistry.info/Elements/u/P60680">
  <rdfs:isDefinedBy rdf:resource="http://rdaregistry.info/Elements/u/" />
  <reg:status rdf:resource="http://metadataregistry.org/uri/RegStatus/1001" />
  <reg:name xml:lang="en">hierarchicalSuperior</reg:name>
  <rdfs:label xml:lang="en">has hierarchical superior</rdfs:label>
  <skos:definition xml:lang="en">Relates an agent that is hierarchically superior to another agent to an agent.</skos:definition>
  <rdf:type rdf:resource="http://www.w3.org/1999/02/22-rdf-syntax-ns#Property" />
  <owl:inverseOf rdf:resource="http://rdaregistry.info/Elements/u/P60681" />
  <reg:hasSubproperty rdf:resource="http://rdaregistry.info/Elements/a/P50008" />
  <reg:lexicalAlias rdf:resource="http://rdaregistry.info/Elements/u/hierarchicalSuperior.en" />
</owl:ObjectProperty>

<!-- Property: has history of resource -->
<owl:ObjectProperty rdf:about="http://rdaregistry.info/Elements/u/P60491">
  <rdfs:isDefinedBy rdf:resource="http://rdaregistry.info/Elements/u/" />
  <reg:status rdf:resource="http://metadataregistry.org/uri/RegStatus/1001" />
  <reg:name xml:lang="en">historyOfResource</reg:name>
  <rdfs:label xml:lang="en">has history of resource</rdfs:label>
  <skos:definition xml:lang="en">Relates a resource to a summary of information about the history of a resource.</skos:definition>
  <rdf:type rdf:resource="http://www.w3.org/1999/02/22-rdf-syntax-ns#Property" />
  <reg:lexicalAlias rdf:resource="http://rdaregistry.info/Elements/u/historyOfTheResource.en" />
</owl:ObjectProperty>

<!-- Property: has honouree -->
<owl:ObjectProperty rdf:about="http://rdaregistry.info/Elements/u/P60406">
  <rdfs:isDefinedBy rdf:resource="http://rdaregistry.info/Elements/u/" />
  <reg:status rdf:resource="http://metadataregistry.org/uri/RegStatus/1001" />
  <reg:name xml:lang="en">honouree</reg:name>
  <rdfs:label xml:lang="en">has honouree</rdfs:label>
  <skos:definition xml:lang="en">Relates a resource to an agent honoured by a resource.</skos:definition>
  <rdf:type rdf:resource="http://www.w3.org/1999/02/22-rdf-syntax-ns#Property" />
  <rdfs:subPropertyOf rdf:resource="http://rdaregistry.info/Elements/u/P60374" />
  <owl:inverseOf rdf:resource="http://rdaregistry.info/Elements/u/P60634" />
  <reg:hasSubproperty rdf:resource="http://rdaregistry.info/Elements/i/P40022" />
  <reg:lexicalAlias rdf:resource="http://rdaregistry.info/Elements/u/honouree.en" />
  <skos:altLabel xml:lang="en">has honoree</skos:altLabel>
</owl:ObjectProperty>

<!-- Property: is honouree of -->
<owl:ObjectProperty rdf:about="http://rdaregistry.info/Elements/u/P60634">
  <rdfs:isDefinedBy rdf:resource="http://rdaregistry.info/Elements/u/" />
  <reg:status rdf:resource="http://metadataregistry.org/uri/RegStatus/1001" />
  <reg:name xml:lang="en">honoureeOf</reg:name>
  <rdfs:label xml:lang="en">is honouree of</rdfs:label>
  <skos:definition xml:lang="en">Relates an agent honoured by a resource to a resource.</skos:definition>
  <rdf:type rdf:resource="http://www.w3.org/1999/02/22-rdf-syntax-ns#Property" />
  <rdfs:subPropertyOf rdf:resource="http://rdaregistry.info/Elements/u/P60602" />
  <owl:inverseOf rdf:resource="http://rdaregistry.info/Elements/u/P60406" />
  <reg:hasSubproperty rdf:resource="http://rdaregistry.info/Elements/a/P50166" />
  <reg:hasSubproperty rdf:resource="http://rdaregistry.info/Elements/a/P50167" />
  <reg:lexicalAlias rdf:resource="http://rdaregistry.info/Elements/u/honoureeOf.en" />
  <skos:altLabel xml:lang="en">honoree of</skos:altLabel>
</owl:ObjectProperty>

<!-- Property: has horizontal scale of cartographic content -->
<owl:ObjectProperty rdf:about="http://rdaregistry.info/Elements/u/P60563">
  <rdfs:isDefinedBy rdf:resource="http://rdaregistry.info/Elements/u/" />
  <reg:status rdf:resource="http://metadataregistry.org/uri/RegStatus/1001" />
  <reg:name xml:lang="en">horizontalScaleOfCartographicContent</reg:name>
  <rdfs:label xml:lang="en">has horizontal scale of cartographic content</rdfs:label>
  <skos:definition xml:lang="en">Relates a resource to a ratio of horizontal distances in the cartographic content of a resource to the actual distances they represent.</skos:definition>
  <rdf:type rdf:resource="http://www.w3.org/1999/02/22-rdf-syntax-ns#Property" />
  <rdfs:subPropertyOf rdf:resource="http://rdaregistry.info/Elements/u/P60565" />
  <reg:hasSubproperty rdf:resource="http://rdaregistry.info/Elements/e/P20226" />
  <reg:lexicalAlias rdf:resource="http://rdaregistry.info/Elements/u/horizontalScaleOfCartographicContent.en" />
</owl:ObjectProperty>

<!-- Property: has host -->
<owl:ObjectProperty rdf:about="http://rdaregistry.info/Elements/u/P60146">
  <rdfs:isDefinedBy rdf:resource="http://rdaregistry.info/Elements/u/" />
  <reg:status rdf:resource="http://metadataregistry.org/uri/RegStatus/1001" />
  <reg:name xml:lang="en">host</reg:name>
  <rdfs:label xml:lang="en">has host</rdfs:label>
  <skos:definition xml:lang="en">Relates a resource to a performer contributing to a resource by leading a program, often broadcast, that includes other guests, performers, etc.</skos:definition>
  <rdf:type rdf:resource="http://www.w3.org/1999/02/22-rdf-syntax-ns#Property" />
  <rdfs:subPropertyOf rdf:resource="http://rdaregistry.info/Elements/u/P60387" />
  <owl:inverseOf rdf:resource="http://rdaregistry.info/Elements/u/P60021" />
  <reg:hasSubproperty rdf:resource="http://rdaregistry.info/Elements/e/P20016" />
  <reg:lexicalAlias rdf:resource="http://rdaregistry.info/Elements/u/host.en" />
</owl:ObjectProperty>

<!-- Property: has host institution -->
<owl:ObjectProperty rdf:about="http://rdaregistry.info/Elements/u/P60061">
  <rdfs:isDefinedBy rdf:resource="http://rdaregistry.info/Elements/u/" />
  <reg:status rdf:resource="http://metadataregistry.org/uri/RegStatus/1001" />
  <reg:name xml:lang="en">host institution</reg:name>
  <rdfs:label xml:lang="en">has host institution</rdfs:label>
  <skos:definition xml:lang="en">Relates a resource to an agent hosting the event, exhibit, conference, etc., which gave rise to a resource, but having little or no responsibility for the content.</skos:definition>
  <rdf:type rdf:resource="http://www.w3.org/1999/02/22-rdf-syntax-ns#Property" />
  <rdfs:subPropertyOf rdf:resource="http://rdaregistry.info/Elements/u/P60374" />
  <owl:inverseOf rdf:resource="http://rdaregistry.info/Elements/u/P60003" />
  <reg:lexicalAlias rdf:resource="http://rdaregistry.info/Elements/u/hostInstitution.en" />
</owl:ObjectProperty>

<!-- Property: is host institution of -->
<owl:ObjectProperty rdf:about="http://rdaregistry.info/Elements/u/P60003">
  <rdfs:isDefinedBy rdf:resource="http://rdaregistry.info/Elements/u/" />
  <reg:status rdf:resource="http://metadataregistry.org/uri/RegStatus/1001" />
  <reg:name xml:lang="en">hostInstitutionOf</reg:name>
  <rdfs:label xml:lang="en">is host institution of</rdfs:label>
  <skos:definition xml:lang="en">Relates an agent hosting an event, exhibit, conference, etc., which gave rise to a resource to a resource.</skos:definition>
  <rdf:type rdf:resource="http://www.w3.org/1999/02/22-rdf-syntax-ns#Property" />
  <rdfs:subPropertyOf rdf:resource="http://rdaregistry.info/Elements/u/P60602" />
  <owl:inverseOf rdf:resource="http://rdaregistry.info/Elements/u/P60061" />
  <reg:hasSubproperty rdf:resource="http://rdaregistry.info/Elements/a/P50004" />
  <reg:lexicalAlias rdf:resource="http://rdaregistry.info/Elements/u/hostInstitutionOf.en" />
</owl:ObjectProperty>

<!-- Property: is host of -->
<owl:ObjectProperty rdf:about="http://rdaregistry.info/Elements/u/P60021">
  <rdfs:isDefinedBy rdf:resource="http://rdaregistry.info/Elements/u/" />
  <reg:status rdf:resource="http://metadataregistry.org/uri/RegStatus/1001" />
  <reg:name xml:lang="en">hostOf</reg:name>
  <rdfs:label xml:lang="en">is host of</rdfs:label>
  <skos:definition xml:lang="en">Relates a performer contributing to a resource by leading a program, often broadcast, that includes other guests, performers, etc., to a resource.</skos:definition>
  <rdf:type rdf:resource="http://www.w3.org/1999/02/22-rdf-syntax-ns#Property" />
  <rdfs:subPropertyOf rdf:resource="http://rdaregistry.info/Elements/u/P60615" />
  <owl:inverseOf rdf:resource="http://rdaregistry.info/Elements/u/P60146" />
  <reg:hasSubproperty rdf:resource="http://rdaregistry.info/Elements/a/P50075" />
  <reg:lexicalAlias rdf:resource="http://rdaregistry.info/Elements/u/hostOf.en" />
</owl:ObjectProperty>

<!-- Property: has identifier for agent -->
<owl:ObjectProperty rdf:about="http://rdaregistry.info/Elements/u/P60053">
  <rdfs:isDefinedBy rdf:resource="http://rdaregistry.info/Elements/u/" />
  <reg:status rdf:resource="http://metadataregistry.org/uri/RegStatus/1001" />
  <reg:name xml:lang="en">identifierForAgent</reg:name>
  <rdfs:label xml:lang="en">has identifier for agent</rdfs:label>
  <skos:definition xml:lang="en">Relates a resource to a character string uniquely associated with an agent, or with a surrogate for an agent such as an authority record.</skos:definition>
  <rdf:type rdf:resource="http://www.w3.org/1999/02/22-rdf-syntax-ns#Property" />
  <reg:hasSubproperty rdf:resource="http://rdaregistry.info/Elements/a/P50006" />
  <reg:hasSubproperty rdf:resource="http://rdaregistry.info/Elements/a/P50052" />
  <reg:hasSubproperty rdf:resource="http://rdaregistry.info/Elements/a/P50094" />
  <reg:lexicalAlias rdf:resource="http://rdaregistry.info/Elements/u/identifierForAgent.en" />
</owl:ObjectProperty>

<!-- Property: has identifier for resource -->
<owl:ObjectProperty rdf:about="http://rdaregistry.info/Elements/u/P60052">
  <rdfs:isDefinedBy rdf:resource="http://rdaregistry.info/Elements/u/" />
  <reg:status rdf:resource="http://metadataregistry.org/uri/RegStatus/1001" />
  <reg:name xml:lang="en">identifierForResource</reg:name>
  <rdfs:label xml:lang="en">has identifier for resource</rdfs:label>
  <skos:definition xml:lang="en">Relates a resource to a character string associated with a resource that serves to differentiate a resource from other resources.</skos:definition>
  <rdf:type rdf:resource="http://www.w3.org/1999/02/22-rdf-syntax-ns#Property" />
  <reg:hasSubproperty rdf:resource="http://rdaregistry.info/Elements/u/P60139" />
  <reg:hasSubproperty rdf:resource="http://rdaregistry.info/Elements/u/P60140" />
  <reg:hasSubproperty rdf:resource="http://rdaregistry.info/Elements/e/P20002" />
  <reg:hasSubproperty rdf:resource="http://rdaregistry.info/Elements/i/P40001" />
  <reg:hasSubproperty rdf:resource="http://rdaregistry.info/Elements/m/P30004" />
  <reg:lexicalAlias rdf:resource="http://rdaregistry.info/Elements/u/identifierForResource.en" />
</owl:ObjectProperty>

<!-- Property: has illuminator -->
<owl:ObjectProperty rdf:about="http://rdaregistry.info/Elements/u/P60421">
  <rdfs:isDefinedBy rdf:resource="http://rdaregistry.info/Elements/u/" />
  <reg:status rdf:resource="http://metadataregistry.org/uri/RegStatus/1001" />
  <reg:name xml:lang="en">illuminator</reg:name>
  <rdfs:label xml:lang="en">has illuminator</rdfs:label>
  <skos:definition xml:lang="en">Relates a resource to an agent providing decoration to a specific resource using precious metals or color, often with elaborate designs and motifs.</skos:definition>
  <rdf:type rdf:resource="http://www.w3.org/1999/02/22-rdf-syntax-ns#Property" />
  <rdfs:subPropertyOf rdf:resource="http://rdaregistry.info/Elements/u/P60374" />
  <owl:inverseOf rdf:resource="http://rdaregistry.info/Elements/u/P60650" />
  <reg:hasSubproperty rdf:resource="http://rdaregistry.info/Elements/i/P40012" />
  <reg:lexicalAlias rdf:resource="http://rdaregistry.info/Elements/u/illuminator.en" />
</owl:ObjectProperty>

<!-- Property: is illuminator of -->
<owl:ObjectProperty rdf:about="http://rdaregistry.info/Elements/u/P60650">
  <rdfs:isDefinedBy rdf:resource="http://rdaregistry.info/Elements/u/" />
  <reg:status rdf:resource="http://metadataregistry.org/uri/RegStatus/1001" />
  <reg:name xml:lang="en">illuminatorOf</reg:name>
  <rdfs:label xml:lang="en">is illuminator of</rdfs:label>
  <skos:definition xml:lang="en">Relates an agent providing decoration to a specific resource using precious metals or color, often with elaborate designs and motifs to a resource.</skos:definition>
  <rdf:type rdf:resource="http://www.w3.org/1999/02/22-rdf-syntax-ns#Property" />
  <rdfs:subPropertyOf rdf:resource="http://rdaregistry.info/Elements/u/P60602" />
  <owl:inverseOf rdf:resource="http://rdaregistry.info/Elements/u/P60421" />
  <reg:hasSubproperty rdf:resource="http://rdaregistry.info/Elements/a/P50092" />
  <reg:lexicalAlias rdf:resource="http://rdaregistry.info/Elements/u/illuminatorOf.en" />
</owl:ObjectProperty>

<!-- Property: is illustrations -->
<owl:ObjectProperty rdf:about="http://rdaregistry.info/Elements/u/P60182">
  <rdfs:isDefinedBy rdf:resource="http://rdaregistry.info/Elements/u/" />
  <reg:status rdf:resource="http://metadataregistry.org/uri/RegStatus/1001" />
  <reg:name xml:lang="en">illustrations</reg:name>
  <rdfs:label xml:lang="en">is illustrations</rdfs:label>
  <skos:definition xml:lang="en">Relates a resource to a resource consisting of pictorial content designed to explain or decorate an augmented resource.</skos:definition>
  <rdf:type rdf:resource="http://www.w3.org/1999/02/22-rdf-syntax-ns#Property" />
  <rdfs:subPropertyOf rdf:resource="http://rdaregistry.info/Elements/u/P60204" />
  <owl:inverseOf rdf:resource="http://rdaregistry.info/Elements/u/P60254" />
  <reg:hasSubproperty rdf:resource="http://rdaregistry.info/Elements/e/P20094" />
  <reg:lexicalAlias rdf:resource="http://rdaregistry.info/Elements/u/illustrations.en" />
</owl:ObjectProperty>

<!-- Property: is illustrations for -->
<owl:ObjectProperty rdf:about="http://rdaregistry.info/Elements/u/P60254">
  <rdfs:isDefinedBy rdf:resource="http://rdaregistry.info/Elements/u/" />
  <reg:status rdf:resource="http://metadataregistry.org/uri/RegStatus/1001" />
  <reg:name xml:lang="en">illustrationsFor</reg:name>
  <rdfs:label xml:lang="en">is illustrations for</rdfs:label>
  <skos:definition xml:lang="en">Relates a resource to a resource that is augmented by pictorial content designed to explain or decorate it.</skos:definition>
  <rdf:type rdf:resource="http://www.w3.org/1999/02/22-rdf-syntax-ns#Property" />
  <rdfs:subPropertyOf rdf:resource="http://rdaregistry.info/Elements/u/P60307" />
  <owl:inverseOf rdf:resource="http://rdaregistry.info/Elements/u/P60182" />
  <reg:hasSubproperty rdf:resource="http://rdaregistry.info/Elements/e/P20148" />
  <reg:lexicalAlias rdf:resource="http://rdaregistry.info/Elements/u/illustrationsFor.en" />
</owl:ObjectProperty>

<!-- Property: has illustrative content -->
<owl:ObjectProperty rdf:about="http://rdaregistry.info/Elements/u/P60486">
  <rdfs:isDefinedBy rdf:resource="http://rdaregistry.info/Elements/u/" />
  <reg:status rdf:resource="http://metadataregistry.org/uri/RegStatus/1001" />
  <reg:name xml:lang="en">illustrativeContent</reg:name>
  <rdfs:label xml:lang="en">has illustrative content</rdfs:label>
  <skos:definition xml:lang="en">Relates a resource to a presence of one or more still images that accompany a primary content of a resource.</skos:definition>
  <rdf:type rdf:resource="http://www.w3.org/1999/02/22-rdf-syntax-ns#Property" />
  <reg:hasSubproperty rdf:resource="http://rdaregistry.info/Elements/e/P20207" />
  <reg:lexicalAlias rdf:resource="http://rdaregistry.info/Elements/u/illustrativeContent.en" />
</owl:ObjectProperty>

<!-- Property: has illustrator -->
<owl:ObjectProperty rdf:about="http://rdaregistry.info/Elements/u/P60396">
  <rdfs:isDefinedBy rdf:resource="http://rdaregistry.info/Elements/u/" />
  <reg:status rdf:resource="http://metadataregistry.org/uri/RegStatus/1001" />
  <reg:name xml:lang="en">illustrator</reg:name>
  <rdfs:label xml:lang="en">has illustrator</rdfs:label>
  <skos:definition xml:lang="en">Relates a resource to an agent contributing to a resource by supplementing a primary content with drawings, diagrams, photographs, etc.</skos:definition>
  <rdf:type rdf:resource="http://www.w3.org/1999/02/22-rdf-syntax-ns#Property" />
  <rdfs:subPropertyOf rdf:resource="http://rdaregistry.info/Elements/u/P60398" />
  <owl:inverseOf rdf:resource="http://rdaregistry.info/Elements/u/P60624" />
  <reg:hasSubproperty rdf:resource="http://rdaregistry.info/Elements/e/P20051" />
  <reg:lexicalAlias rdf:resource="http://rdaregistry.info/Elements/u/illustrator.en" />
  <skos:scopeNote xml:lang="en">Creation of content that is primarily artistic is excluded.</skos:scopeNote>
  <reg:hasSubproperty rdf:resource="http://rdaregistry.info/Elements/u/P60750" />
</owl:ObjectProperty>

<!-- Property: is illustrator of -->
<owl:ObjectProperty rdf:about="http://rdaregistry.info/Elements/u/P60624">
  <rdfs:isDefinedBy rdf:resource="http://rdaregistry.info/Elements/u/" />
  <reg:status rdf:resource="http://metadataregistry.org/uri/RegStatus/1001" />
  <reg:name xml:lang="en">illustratorOf</reg:name>
  <rdfs:label xml:lang="en">is illustrator of</rdfs:label>
  <skos:definition xml:lang="en">Relates an agent contributing to a resource by supplementing a primary content with drawings, diagrams, photographs, etc. to a resource.</skos:definition>
  <rdf:type rdf:resource="http://www.w3.org/1999/02/22-rdf-syntax-ns#Property" />
  <rdfs:subPropertyOf rdf:resource="http://rdaregistry.info/Elements/u/P60626" />
  <owl:inverseOf rdf:resource="http://rdaregistry.info/Elements/u/P60396" />
  <reg:hasSubproperty rdf:resource="http://rdaregistry.info/Elements/a/P50159" />
  <reg:lexicalAlias rdf:resource="http://rdaregistry.info/Elements/u/illustratorOf.en" />
  <skos:scopeNote xml:lang="en">Creation of content that is primarily artistic is excluded.</skos:scopeNote>
  <reg:hasSubproperty rdf:resource="http://rdaregistry.info/Elements/u/P60756" />
  <rdakit:seeAlso rdf:resource="http://rdaregistry.info/Elements/u/P60660" />
</owl:ObjectProperty>

<!-- Property: is imitated as -->
<owl:ObjectProperty rdf:about="http://rdaregistry.info/Elements/u/P60214">
  <rdfs:isDefinedBy rdf:resource="http://rdaregistry.info/Elements/u/" />
  <reg:status rdf:resource="http://metadataregistry.org/uri/RegStatus/1001" />
  <reg:name xml:lang="en">imitatedAs</reg:name>
  <rdfs:label xml:lang="en">is imitated as</rdfs:label>
  <skos:definition xml:lang="en">Relates a resource to a resource that copies the style or content of a source resource.</skos:definition>
  <rdf:type rdf:resource="http://www.w3.org/1999/02/22-rdf-syntax-ns#Property" />
  <rdfs:subPropertyOf rdf:resource="http://rdaregistry.info/Elements/u/P60250" />
  <owl:inverseOf rdf:resource="http://rdaregistry.info/Elements/u/P60311" />
  <reg:hasSubproperty rdf:resource="http://rdaregistry.info/Elements/u/P60246" />
  <reg:hasSubproperty rdf:resource="http://rdaregistry.info/Elements/e/P20114" />
  <reg:lexicalAlias rdf:resource="http://rdaregistry.info/Elements/u/imitatedAs.en" />
</owl:ObjectProperty>

<!-- Property: is imitation of -->
<owl:ObjectProperty rdf:about="http://rdaregistry.info/Elements/u/P60311">
  <rdfs:isDefinedBy rdf:resource="http://rdaregistry.info/Elements/u/" />
  <reg:status rdf:resource="http://metadataregistry.org/uri/RegStatus/1001" />
  <reg:name xml:lang="en">imitationOf</reg:name>
  <rdfs:label xml:lang="en">is imitation of</rdfs:label>
  <skos:definition xml:lang="en">Relates a resource to a resource whose style or content is copied in a derivative resource.</skos:definition>
  <rdf:type rdf:resource="http://www.w3.org/1999/02/22-rdf-syntax-ns#Property" />
  <rdfs:subPropertyOf rdf:resource="http://rdaregistry.info/Elements/u/P60305" />
  <owl:inverseOf rdf:resource="http://rdaregistry.info/Elements/u/P60214" />
  <reg:hasSubproperty rdf:resource="http://rdaregistry.info/Elements/u/P60312" />
  <reg:hasSubproperty rdf:resource="http://rdaregistry.info/Elements/e/P20195" />
  <reg:lexicalAlias rdf:resource="http://rdaregistry.info/Elements/u/imitationOf.en" />
</owl:ObjectProperty>

<!-- Property: has immediate source of acquisition of resource -->
<owl:ObjectProperty rdf:about="http://rdaregistry.info/Elements/u/P60583">
  <rdfs:isDefinedBy rdf:resource="http://rdaregistry.info/Elements/u/" />
  <reg:status rdf:resource="http://metadataregistry.org/uri/RegStatus/1001" />
  <reg:name xml:lang="en">immediateSourceOfAcquisitionOfResource</reg:name>
  <rdfs:label xml:lang="en">has immediate source of acquisition of resource</rdfs:label>
  <skos:definition xml:lang="en">Relates a resource to a source from which an agency directly acquired a resource and the circumstances under which it was received.</skos:definition>
  <rdf:type rdf:resource="http://www.w3.org/1999/02/22-rdf-syntax-ns#Property" />
  <reg:hasSubproperty rdf:resource="http://rdaregistry.info/Elements/i/P40050" />
  <reg:lexicalAlias rdf:resource="http://rdaregistry.info/Elements/u/immediateSourceOfAcquisitionOfResource.en" />
</owl:ObjectProperty>

<!-- Property: is incidental music -->
<owl:ObjectProperty rdf:about="http://rdaregistry.info/Elements/u/P60118">
  <rdfs:isDefinedBy rdf:resource="http://rdaregistry.info/Elements/u/" />
  <reg:status rdf:resource="http://metadataregistry.org/uri/RegStatus/1001" />
  <reg:name xml:lang="en">incidentalMusic</reg:name>
  <rdfs:label xml:lang="en">is incidental music</rdfs:label>
  <skos:definition xml:lang="en">Relates a resource to a musical resource that provides incidental music for a play or other spoken resource for the stage.</skos:definition>
  <rdf:type rdf:resource="http://www.w3.org/1999/02/22-rdf-syntax-ns#Property" />
  <owl:inverseOf rdf:resource="http://rdaregistry.info/Elements/u/P60202" />
  <reg:hasSubproperty rdf:resource="http://rdaregistry.info/Elements/e/P20085" />
  <reg:lexicalAlias rdf:resource="http://rdaregistry.info/Elements/u/incidentalMusic.en" />
  <rdfs:subPropertyOf rdf:resource="http://rdaregistry.info/Elements/u/P60723" />
</owl:ObjectProperty>

<!-- Property: is incidental music for -->
<owl:ObjectProperty rdf:about="http://rdaregistry.info/Elements/u/P60202">
  <rdfs:isDefinedBy rdf:resource="http://rdaregistry.info/Elements/u/" />
  <reg:status rdf:resource="http://metadataregistry.org/uri/RegStatus/1001" />
  <reg:name xml:lang="en">incidentalMusicFor</reg:name>
  <rdfs:label xml:lang="en">is incidental music for</rdfs:label>
  <skos:definition xml:lang="en">Relates a resource to a resource such as a play or other spoken resource for the stage that uses a musical resource as incidental music.</skos:definition>
  <rdf:type rdf:resource="http://www.w3.org/1999/02/22-rdf-syntax-ns#Property" />
  <owl:inverseOf rdf:resource="http://rdaregistry.info/Elements/u/P60118" />
  <reg:hasSubproperty rdf:resource="http://rdaregistry.info/Elements/e/P20103" />
  <reg:lexicalAlias rdf:resource="http://rdaregistry.info/Elements/u/incidentalMusicFor.en" />
  <rdfs:subPropertyOf rdf:resource="http://rdaregistry.info/Elements/u/P60724" />
</owl:ObjectProperty>

<!-- Property: is index -->
<owl:ObjectProperty rdf:about="http://rdaregistry.info/Elements/u/P60263">
  <rdfs:isDefinedBy rdf:resource="http://rdaregistry.info/Elements/u/" />
  <reg:status rdf:resource="http://metadataregistry.org/uri/RegStatus/1001" />
  <reg:name xml:lang="en">index</reg:name>
  <rdfs:label xml:lang="en">is index</rdfs:label>
  <skos:definition xml:lang="en">Relates a resource to a resource that provides a systematic, alphabetical guide to the contents of a predominant resource, usually keyed to page numbers or other reference codes.</skos:definition>
  <rdf:type rdf:resource="http://www.w3.org/1999/02/22-rdf-syntax-ns#Property" />
  <rdfs:subPropertyOf rdf:resource="http://rdaregistry.info/Elements/u/P60204" />
  <owl:inverseOf rdf:resource="http://rdaregistry.info/Elements/u/P60302" />
  <reg:hasSubproperty rdf:resource="http://rdaregistry.info/Elements/e/P20156" />
  <reg:lexicalAlias rdf:resource="http://rdaregistry.info/Elements/u/index.en" />
</owl:ObjectProperty>

<!-- Property: is indexed in -->
<owl:ObjectProperty rdf:about="http://rdaregistry.info/Elements/u/P60178">
  <rdfs:isDefinedBy rdf:resource="http://rdaregistry.info/Elements/u/" />
  <reg:status rdf:resource="http://metadataregistry.org/uri/RegStatus/1001" />
  <reg:name xml:lang="en">indexedIn</reg:name>
  <rdfs:label xml:lang="en">is indexed in</rdfs:label>
  <skos:definition xml:lang="en">Relates a resource to a resource that is an abstracting and indexing service that indexes the contents of a source resource.</skos:definition>
  <rdf:type rdf:resource="http://www.w3.org/1999/02/22-rdf-syntax-ns#Property" />
  <rdfs:subPropertyOf rdf:resource="http://rdaregistry.info/Elements/u/P60250" />
  <owl:inverseOf rdf:resource="http://rdaregistry.info/Elements/u/P60309" />
  <reg:hasSubproperty rdf:resource="http://rdaregistry.info/Elements/e/P20091" />
  <reg:lexicalAlias rdf:resource="http://rdaregistry.info/Elements/u/indexedIn.en" />
</owl:ObjectProperty>

<!-- Property: is indexing for -->
<owl:ObjectProperty rdf:about="http://rdaregistry.info/Elements/u/P60309">
  <rdfs:isDefinedBy rdf:resource="http://rdaregistry.info/Elements/u/" />
  <reg:status rdf:resource="http://metadataregistry.org/uri/RegStatus/1001" />
  <reg:name xml:lang="en">indexingFor</reg:name>
  <rdfs:label xml:lang="en">is indexing for</rdfs:label>
  <skos:definition xml:lang="en">Relates a resource to a resource whose contents have been indexed by an abstracting and indexing service.</skos:definition>
  <rdf:type rdf:resource="http://www.w3.org/1999/02/22-rdf-syntax-ns#Property" />
  <rdfs:subPropertyOf rdf:resource="http://rdaregistry.info/Elements/u/P60305" />
  <owl:inverseOf rdf:resource="http://rdaregistry.info/Elements/u/P60178" />
  <reg:hasSubproperty rdf:resource="http://rdaregistry.info/Elements/e/P20194" />
  <reg:lexicalAlias rdf:resource="http://rdaregistry.info/Elements/u/indexingFor.en" />
</owl:ObjectProperty>

<!-- Property: is index to -->
<owl:ObjectProperty rdf:about="http://rdaregistry.info/Elements/u/P60302">
  <rdfs:isDefinedBy rdf:resource="http://rdaregistry.info/Elements/u/" />
  <reg:status rdf:resource="http://metadataregistry.org/uri/RegStatus/1001" />
  <reg:name xml:lang="en">indexTo</reg:name>
  <rdfs:label xml:lang="en">is index to</rdfs:label>
  <skos:definition xml:lang="en">Relates a resource to a resource used as a basis for an index, i.e., a systematic, alphabetical guide to the contents of a predominant resource, usually keyed to page numbers or other reference codes.</skos:definition>
  <rdf:type rdf:resource="http://www.w3.org/1999/02/22-rdf-syntax-ns#Property" />
  <rdfs:subPropertyOf rdf:resource="http://rdaregistry.info/Elements/u/P60307" />
  <owl:inverseOf rdf:resource="http://rdaregistry.info/Elements/u/P60263" />
  <reg:hasSubproperty rdf:resource="http://rdaregistry.info/Elements/e/P20188" />
  <reg:lexicalAlias rdf:resource="http://rdaregistry.info/Elements/u/indexTo.en" />
</owl:ObjectProperty>

<!-- Property: has inscriber -->
<owl:ObjectProperty rdf:about="http://rdaregistry.info/Elements/u/P60460">
  <rdfs:isDefinedBy rdf:resource="http://rdaregistry.info/Elements/u/" />
  <reg:status rdf:resource="http://metadataregistry.org/uri/RegStatus/1001" />
  <reg:name xml:lang="en">inscriber</reg:name>
  <rdfs:label xml:lang="en">has inscriber</rdfs:label>
  <skos:definition xml:lang="en">Relates a resource to an agent who has written a statement of dedication or gift on a resource.</skos:definition>
  <rdf:type rdf:resource="http://www.w3.org/1999/02/22-rdf-syntax-ns#Property" />
  <rdfs:subPropertyOf rdf:resource="http://rdaregistry.info/Elements/u/P60374" />
  <owl:inverseOf rdf:resource="http://rdaregistry.info/Elements/u/P60695" />
  <reg:hasSubproperty rdf:resource="http://rdaregistry.info/Elements/i/P40014" />
  <reg:lexicalAlias rdf:resource="http://rdaregistry.info/Elements/u/inscriber.en" />
</owl:ObjectProperty>

<!-- Property: is inscriber of -->
<owl:ObjectProperty rdf:about="http://rdaregistry.info/Elements/u/P60695">
  <rdfs:isDefinedBy rdf:resource="http://rdaregistry.info/Elements/u/" />
  <reg:status rdf:resource="http://metadataregistry.org/uri/RegStatus/1001" />
  <reg:name xml:lang="en">inscriberOf</reg:name>
  <rdfs:label xml:lang="en">is inscriber of</rdfs:label>
  <skos:definition xml:lang="en">Relates an agent who has written a statement of dedication or gift on a resource to a resource.</skos:definition>
  <rdf:type rdf:resource="http://www.w3.org/1999/02/22-rdf-syntax-ns#Property" />
  <rdfs:subPropertyOf rdf:resource="http://rdaregistry.info/Elements/u/P60602" />
  <owl:inverseOf rdf:resource="http://rdaregistry.info/Elements/u/P60460" />
  <reg:hasSubproperty rdf:resource="http://rdaregistry.info/Elements/a/P50125" />
  <reg:lexicalAlias rdf:resource="http://rdaregistry.info/Elements/u/inscriberOf.en" />
</owl:ObjectProperty>

<!-- Property: is in series -->
<owl:ObjectProperty rdf:about="http://rdaregistry.info/Elements/u/P60193">
  <rdfs:isDefinedBy rdf:resource="http://rdaregistry.info/Elements/u/" />
  <reg:status rdf:resource="http://metadataregistry.org/uri/RegStatus/1001" />
  <reg:name xml:lang="en">inSeries</reg:name>
  <rdfs:label xml:lang="en">is in series</rdfs:label>
  <skos:definition xml:lang="en">Relates a resource to a resource in which a part has been issued; a title of a larger resource appears on a part.</skos:definition>
  <rdf:type rdf:resource="http://www.w3.org/1999/02/22-rdf-syntax-ns#Property" />
  <rdfs:subPropertyOf rdf:resource="http://rdaregistry.info/Elements/u/P60101" />
  <owl:inverseOf rdf:resource="http://rdaregistry.info/Elements/u/P60240" />
  <reg:lexicalAlias rdf:resource="http://rdaregistry.info/Elements/u/inSeries.en" />
</owl:ObjectProperty>

<!-- Property: is insert -->
<owl:ObjectProperty rdf:about="http://rdaregistry.info/Elements/u/P60183">
  <rdfs:isDefinedBy rdf:resource="http://rdaregistry.info/Elements/u/" />
  <reg:status rdf:resource="http://metadataregistry.org/uri/RegStatus/1001" />
  <reg:name xml:lang="en">insert</reg:name>
  <rdfs:label xml:lang="en">is insert</rdfs:label>
  <skos:definition xml:lang="en">Relates a resource to a resource in which a part has been issued; a title of a larger resource appears on a part.</skos:definition>
  <rdf:type rdf:resource="http://www.w3.org/1999/02/22-rdf-syntax-ns#Property" />
  <rdfs:subPropertyOf rdf:resource="http://rdaregistry.info/Elements/u/P60249" />
  <owl:inverseOf rdf:resource="http://rdaregistry.info/Elements/u/P60194" />
  <reg:hasSubproperty rdf:resource="http://rdaregistry.info/Elements/m/P30022" />
  <reg:lexicalAlias rdf:resource="http://rdaregistry.info/Elements/u/insert.en" />
</owl:ObjectProperty>

<!-- Property: is inserted in -->
<owl:ObjectProperty rdf:about="http://rdaregistry.info/Elements/u/P60194">
  <rdfs:isDefinedBy rdf:resource="http://rdaregistry.info/Elements/u/" />
  <reg:status rdf:resource="http://metadataregistry.org/uri/RegStatus/1001" />
  <reg:name xml:lang="en">insertedIn</reg:name>
  <rdfs:label xml:lang="en">is inserted in</rdfs:label>
  <skos:definition xml:lang="en">Relates a resource to a resource into which material has been inserted that is not an integral part of the publication.</skos:definition>
  <rdf:type rdf:resource="http://www.w3.org/1999/02/22-rdf-syntax-ns#Property" />
  <rdfs:subPropertyOf rdf:resource="http://rdaregistry.info/Elements/u/P60101" />
  <owl:inverseOf rdf:resource="http://rdaregistry.info/Elements/u/P60183" />
  <reg:hasSubproperty rdf:resource="http://rdaregistry.info/Elements/m/P30025" />
  <reg:lexicalAlias rdf:resource="http://rdaregistry.info/Elements/u/insertedIn.en" />
</owl:ObjectProperty>

<!-- Property: is inspiration for -->
<owl:ObjectProperty rdf:about="http://rdaregistry.info/Elements/u/P60833">
  <rdfs:isDefinedBy rdf:resource="http://rdaregistry.info/Elements/u/" />
  <reg:status rdf:resource="http://metadataregistry.org/uri/RegStatus/1001" />
  <rdf:type rdf:resource="http://www.w3.org/1999/02/22-rdf-syntax-ns#Property" />
  <reg:name xml:lang="en">inspirationFor</reg:name>
  <rdfs:label xml:lang="en">is inspiration for</rdfs:label>
  <reg:lexicalAlias rdf:resource="http://rdaregistry.info/Elements/u/inspirationFor.en" />
  <skos:definition xml:lang="en">Relates a resource to a resource which was inspired by another resource.</skos:definition>
  <owl:inverseOf rdf:resource="http://rdaregistry.info/Elements/u/P60832" />
  <rdfs:subPropertyOf rdf:resource="http://rdaregistry.info/Elements/u/P60250" />
</owl:ObjectProperty>

<!-- Property: is inspired by -->
<owl:ObjectProperty rdf:about="http://rdaregistry.info/Elements/u/P60832">
  <rdfs:isDefinedBy rdf:resource="http://rdaregistry.info/Elements/u/" />
  <reg:status rdf:resource="http://metadataregistry.org/uri/RegStatus/1001" />
  <rdf:type rdf:resource="http://www.w3.org/1999/02/22-rdf-syntax-ns#Property" />
  <reg:name xml:lang="en">inspiredBy</reg:name>
  <rdfs:label xml:lang="en">is inspired by</rdfs:label>
  <reg:lexicalAlias rdf:resource="http://rdaregistry.info/Elements/u/inspiredBy.en" />
  <skos:definition xml:lang="en">Relates a resource to a resource which serves as the inspiration for another resource.</skos:definition>
  <owl:inverseOf rdf:resource="http://rdaregistry.info/Elements/u/P60833" />
  <rdfs:subPropertyOf rdf:resource="http://rdaregistry.info/Elements/u/P60305" />
</owl:ObjectProperty>

<!-- Property: has instrumental conductor -->
<owl:ObjectProperty rdf:about="http://rdaregistry.info/Elements/u/P60844">
  <rdfs:isDefinedBy rdf:resource="http://rdaregistry.info/Elements/u/" />
  <reg:status rdf:resource="http://metadataregistry.org/uri/RegStatus/1001" />
  <rdf:type rdf:resource="http://www.w3.org/1999/02/22-rdf-syntax-ns#Property" />
  <reg:name xml:lang="en">instrumentalConductor</reg:name>
  <rdfs:label xml:lang="en">has instrumental conductor</rdfs:label>
  <reg:lexicalAlias rdf:resource="http://rdaregistry.info/Elements/u/instrumentalConductor.en" />
  <skos:definition xml:lang="en">Relates a resource to a conductor contributing to a musical resource by leading an instrumental performing group in a musical or dramatic presentation, etc.</skos:definition>
  <owl:inverseOf rdf:resource="http://rdaregistry.info/Elements/u/P60845" />
  <reg:hasSubproperty rdf:resource="http://rdaregistry.info/Elements/e/P20286" />
  <rdfs:subPropertyOf rdf:resource="http://rdaregistry.info/Elements/u/P60141" />
</owl:ObjectProperty>

<!-- Property: is instrumental conductor of -->
<owl:ObjectProperty rdf:about="http://rdaregistry.info/Elements/u/P60845">
  <rdfs:isDefinedBy rdf:resource="http://rdaregistry.info/Elements/u/" />
  <reg:status rdf:resource="http://metadataregistry.org/uri/RegStatus/1001" />
  <rdf:type rdf:resource="http://www.w3.org/1999/02/22-rdf-syntax-ns#Property" />
  <reg:name xml:lang="en">instrumentalConductorOf</reg:name>
  <rdfs:label xml:lang="en">is instrumental conductor of</rdfs:label>
  <reg:lexicalAlias rdf:resource="http://rdaregistry.info/Elements/u/instrumentalConductorOf.en" />
  <skos:definition xml:lang="en">Relates a conductor contributing to a musical resource by leading an instrumental performing group in a musical or dramatic presentation, etc. to a resource</skos:definition>
  <owl:inverseOf rdf:resource="http://rdaregistry.info/Elements/u/P60844" />
  <reg:hasSubproperty rdf:resource="http://rdaregistry.info/Elements/a/P50269" />
  <rdfs:subPropertyOf rdf:resource="http://rdaregistry.info/Elements/u/P60016" />
</owl:ObjectProperty>

<!-- Property: has instrumentalist -->
<owl:ObjectProperty rdf:about="http://rdaregistry.info/Elements/u/P60150">
  <rdfs:isDefinedBy rdf:resource="http://rdaregistry.info/Elements/u/" />
  <reg:status rdf:resource="http://metadataregistry.org/uri/RegStatus/1001" />
  <reg:name xml:lang="en">instrumentalist</reg:name>
  <rdfs:label xml:lang="en">has instrumentalist</rdfs:label>
  <skos:definition xml:lang="en">Relates a resource to a performer contributing to a resource by playing a musical instrument.</skos:definition>
  <rdf:type rdf:resource="http://www.w3.org/1999/02/22-rdf-syntax-ns#Property" />
  <rdfs:subPropertyOf rdf:resource="http://rdaregistry.info/Elements/u/P60387" />
  <owl:inverseOf rdf:resource="http://rdaregistry.info/Elements/u/P60025" />
  <reg:hasSubproperty rdf:resource="http://rdaregistry.info/Elements/e/P20020" />
  <reg:lexicalAlias rdf:resource="http://rdaregistry.info/Elements/u/instrumentalist.en" />
</owl:ObjectProperty>

<!-- Property: is instrumentalist of -->
<owl:ObjectProperty rdf:about="http://rdaregistry.info/Elements/u/P60025">
  <rdfs:isDefinedBy rdf:resource="http://rdaregistry.info/Elements/u/" />
  <reg:status rdf:resource="http://metadataregistry.org/uri/RegStatus/1001" />
  <reg:name xml:lang="en">instrumentalistOf</reg:name>
  <rdfs:label xml:lang="en">is instrumentalist of</rdfs:label>
  <skos:definition xml:lang="en">Relates a performer contributing to a resource by playing a musical instrument to a resource.</skos:definition>
  <rdf:type rdf:resource="http://www.w3.org/1999/02/22-rdf-syntax-ns#Property" />
  <rdfs:subPropertyOf rdf:resource="http://rdaregistry.info/Elements/u/P60615" />
  <owl:inverseOf rdf:resource="http://rdaregistry.info/Elements/u/P60150" />
  <reg:hasSubproperty rdf:resource="http://rdaregistry.info/Elements/a/P50079" />
  <reg:lexicalAlias rdf:resource="http://rdaregistry.info/Elements/u/instrumentalistOf.en" />
</owl:ObjectProperty>

<!-- Property: has intended audience -->
<owl:ObjectProperty rdf:about="http://rdaregistry.info/Elements/u/P60520">
  <rdfs:isDefinedBy rdf:resource="http://rdaregistry.info/Elements/u/" />
  <reg:status rdf:resource="http://metadataregistry.org/uri/RegStatus/1001" />
  <reg:name xml:lang="en">intendedAudience</reg:name>
  <rdfs:label xml:lang="en">has intended audience</rdfs:label>
  <skos:definition xml:lang="en">Relates a resource to a category of user for which the content of a resource is intended, or for whom the content is considered suitable.</skos:definition>
  <rdf:type rdf:resource="http://www.w3.org/1999/02/22-rdf-syntax-ns#Property" />
  <reg:lexicalAlias rdf:resource="http://rdaregistry.info/Elements/u/intendedAudience.en" />
</owl:ObjectProperty>

<!-- Property: has interviewee -->
<owl:ObjectProperty rdf:about="http://rdaregistry.info/Elements/u/P60432">
  <rdfs:isDefinedBy rdf:resource="http://rdaregistry.info/Elements/u/" />
  <reg:status rdf:resource="http://metadataregistry.org/uri/RegStatus/1001" />
  <reg:name xml:lang="en">interviewee</reg:name>
  <rdfs:label xml:lang="en">has interviewee</rdfs:label>
  <skos:definition xml:lang="en">Relates a resource to an agent responsible for creating a resource by responding to an interviewer, usually a reporter, pollster, or some other information gathering agent.</skos:definition>
  <rdf:type rdf:resource="http://www.w3.org/1999/02/22-rdf-syntax-ns#Property" />
  <rdfs:subPropertyOf rdf:resource="http://rdaregistry.info/Elements/u/P60447" />
  <owl:inverseOf rdf:resource="http://rdaregistry.info/Elements/u/P60661" />
  <reg:hasSubproperty rdf:resource="http://rdaregistry.info/Elements/e/P20047" />
  <reg:lexicalAlias rdf:resource="http://rdaregistry.info/Elements/u/interviewee.en" />
</owl:ObjectProperty>

<!-- Property: is interviewee of -->
<owl:ObjectProperty rdf:about="http://rdaregistry.info/Elements/u/P60661">
  <rdfs:isDefinedBy rdf:resource="http://rdaregistry.info/Elements/u/" />
  <reg:status rdf:resource="http://metadataregistry.org/uri/RegStatus/1001" />
  <reg:name xml:lang="en">intervieweeOf</reg:name>
  <rdfs:label xml:lang="en">is interviewee of</rdfs:label>
  <skos:definition xml:lang="en">Relates an agent responsible for creating a resource by responding to an interviewer, usually a reporter, pollster, or some other information gathering agent to a resource.</skos:definition>
  <rdf:type rdf:resource="http://www.w3.org/1999/02/22-rdf-syntax-ns#Property" />
  <rdfs:subPropertyOf rdf:resource="http://rdaregistry.info/Elements/u/P60672" />
  <owl:inverseOf rdf:resource="http://rdaregistry.info/Elements/u/P60432" />
  <reg:hasSubproperty rdf:resource="http://rdaregistry.info/Elements/a/P50155" />
  <reg:hasSubproperty rdf:resource="http://rdaregistry.info/Elements/a/P50193" />
  <reg:lexicalAlias rdf:resource="http://rdaregistry.info/Elements/u/intervieweeOf.en" />
</owl:ObjectProperty>

<!-- Property: has interviewer -->
<owl:ObjectProperty rdf:about="http://rdaregistry.info/Elements/u/P60430">
  <rdfs:isDefinedBy rdf:resource="http://rdaregistry.info/Elements/u/" />
  <reg:status rdf:resource="http://metadataregistry.org/uri/RegStatus/1001" />
  <reg:name xml:lang="en">interviewer</reg:name>
  <rdfs:label xml:lang="en">has interviewer</rdfs:label>
  <skos:definition xml:lang="en">Relates a resource to an agent responsible for creating a resource by acting as an interviewer, reporter, pollster, or some other information gathering agent.</skos:definition>
  <rdf:type rdf:resource="http://www.w3.org/1999/02/22-rdf-syntax-ns#Property" />
  <rdfs:subPropertyOf rdf:resource="http://rdaregistry.info/Elements/u/P60447" />
  <owl:inverseOf rdf:resource="http://rdaregistry.info/Elements/u/P60659" />
  <reg:hasSubproperty rdf:resource="http://rdaregistry.info/Elements/e/P20032" />
  <reg:lexicalAlias rdf:resource="http://rdaregistry.info/Elements/u/interviewer.en" />
</owl:ObjectProperty>

<!-- Property: is interviewer of -->
<owl:ObjectProperty rdf:about="http://rdaregistry.info/Elements/u/P60659">
  <rdfs:isDefinedBy rdf:resource="http://rdaregistry.info/Elements/u/" />
  <reg:status rdf:resource="http://metadataregistry.org/uri/RegStatus/1001" />
  <reg:name xml:lang="en">interviewerOf</reg:name>
  <rdfs:label xml:lang="en">is interviewer of</rdfs:label>
  <skos:definition xml:lang="en">Relates an agent responsible for creating a resource by acting as an interviewer, reporter, pollster, or some other information gathering agent to a resource.</skos:definition>
  <rdf:type rdf:resource="http://www.w3.org/1999/02/22-rdf-syntax-ns#Property" />
  <rdfs:subPropertyOf rdf:resource="http://rdaregistry.info/Elements/u/P60672" />
  <owl:inverseOf rdf:resource="http://rdaregistry.info/Elements/u/P60430" />
  <reg:hasSubproperty rdf:resource="http://rdaregistry.info/Elements/a/P50140" />
  <reg:hasSubproperty rdf:resource="http://rdaregistry.info/Elements/a/P50191" />
  <reg:lexicalAlias rdf:resource="http://rdaregistry.info/Elements/u/interviewerOf.en" />
</owl:ObjectProperty>

<!-- Property: has inventor -->
<owl:ObjectProperty rdf:about="http://rdaregistry.info/Elements/u/P60427">
  <rdfs:isDefinedBy rdf:resource="http://rdaregistry.info/Elements/u/" />
  <reg:status rdf:resource="http://metadataregistry.org/uri/RegStatus/1001" />
  <reg:name xml:lang="en">inventor</reg:name>
  <rdfs:label xml:lang="en">has inventor</rdfs:label>
  <skos:definition xml:lang="en">Relates a resource to an agent responsible for creating a new device or process.</skos:definition>
  <rdf:type rdf:resource="http://www.w3.org/1999/02/22-rdf-syntax-ns#Property" />
  <rdfs:subPropertyOf rdf:resource="http://rdaregistry.info/Elements/u/P60447" />
  <owl:inverseOf rdf:resource="http://rdaregistry.info/Elements/u/P60656" />
  <reg:lexicalAlias rdf:resource="http://rdaregistry.info/Elements/u/inventor.en" />
</owl:ObjectProperty>

<!-- Property: is inventor of -->
<owl:ObjectProperty rdf:about="http://rdaregistry.info/Elements/u/P60656">
  <rdfs:isDefinedBy rdf:resource="http://rdaregistry.info/Elements/u/" />
  <reg:status rdf:resource="http://metadataregistry.org/uri/RegStatus/1001" />
  <reg:name xml:lang="en">inventorOf</reg:name>
  <rdfs:label xml:lang="en">is inventor of</rdfs:label>
  <skos:definition xml:lang="en">Relates an agent responsible for creating a new device or process to a resource.</skos:definition>
  <rdf:type rdf:resource="http://www.w3.org/1999/02/22-rdf-syntax-ns#Property" />
  <rdfs:subPropertyOf rdf:resource="http://rdaregistry.info/Elements/u/P60672" />
  <owl:inverseOf rdf:resource="http://rdaregistry.info/Elements/u/P60427" />
  <reg:hasSubproperty rdf:resource="http://rdaregistry.info/Elements/a/P50188" />
  <reg:lexicalAlias rdf:resource="http://rdaregistry.info/Elements/u/inventorOf.en" />
</owl:ObjectProperty>

<!-- Property: has ISSN of series -->
<owl:ObjectProperty rdf:about="http://rdaregistry.info/Elements/u/P60534">
  <rdfs:isDefinedBy rdf:resource="http://rdaregistry.info/Elements/u/" />
  <reg:status rdf:resource="http://metadataregistry.org/uri/RegStatus/1001" />
  <reg:name xml:lang="en">issnOfSeries</reg:name>
  <rdfs:label xml:lang="en">has ISSN of series</rdfs:label>
  <skos:definition xml:lang="en">Relates a resource to an identifier assigned to a series by an ISSN registration agency.</skos:definition>
  <rdf:type rdf:resource="http://www.w3.org/1999/02/22-rdf-syntax-ns#Property" />
  <reg:hasSubproperty rdf:resource="http://rdaregistry.info/Elements/m/P30166" />
  <reg:lexicalAlias rdf:resource="http://rdaregistry.info/Elements/u/issnOfSeries.en" />
</owl:ObjectProperty>

<!-- Property: has ISSN of subseries -->
<owl:ObjectProperty rdf:about="http://rdaregistry.info/Elements/u/P60535">
  <rdfs:isDefinedBy rdf:resource="http://rdaregistry.info/Elements/u/" />
  <reg:status rdf:resource="http://metadataregistry.org/uri/RegStatus/1001" />
  <reg:name xml:lang="en">issnOfSubseries</reg:name>
  <rdfs:label xml:lang="en">has ISSN of subseries</rdfs:label>
  <skos:definition xml:lang="en">Relates a resource to an identifier assigned to a subseries by an ISSN registration agency.</skos:definition>
  <rdf:type rdf:resource="http://www.w3.org/1999/02/22-rdf-syntax-ns#Property" />
  <reg:hasSubproperty rdf:resource="http://rdaregistry.info/Elements/m/P30167" />
  <reg:lexicalAlias rdf:resource="http://rdaregistry.info/Elements/u/issnOfSubseries.en" />
</owl:ObjectProperty>

<!-- Property: is issued with -->
<owl:ObjectProperty rdf:about="http://rdaregistry.info/Elements/u/P60256">
  <rdfs:isDefinedBy rdf:resource="http://rdaregistry.info/Elements/u/" />
  <reg:status rdf:resource="http://metadataregistry.org/uri/RegStatus/1001" />
  <reg:name xml:lang="en">issuedWith</reg:name>
  <rdfs:label xml:lang="en">is issued with</rdfs:label>
  <skos:definition xml:lang="en">Relates a resource to a resource that is issued on the same carrier as a resource being described.</skos:definition>
  <rdf:type rdf:resource="http://www.w3.org/1999/02/22-rdf-syntax-ns#Property" />
  <rdfs:subPropertyOf rdf:resource="http://rdaregistry.info/Elements/u/P60196" />
  <owl:inverseOf rdf:resource="http://rdaregistry.info/Elements/u/P60256" />
  <reg:hasSubproperty rdf:resource="http://rdaregistry.info/Elements/u/P60257" />
  <reg:hasSubproperty rdf:resource="http://rdaregistry.info/Elements/u/P60258" />
  <reg:hasSubproperty rdf:resource="http://rdaregistry.info/Elements/m/P30035" />
  <reg:lexicalAlias rdf:resource="http://rdaregistry.info/Elements/u/issuedWith.en" />
</owl:ObjectProperty>

<!-- Property: has issuing body -->
<owl:ObjectProperty rdf:about="http://rdaregistry.info/Elements/u/P60467">
  <rdfs:isDefinedBy rdf:resource="http://rdaregistry.info/Elements/u/" />
  <reg:status rdf:resource="http://metadataregistry.org/uri/RegStatus/1001" />
  <reg:name xml:lang="en">issuingBody</reg:name>
  <rdfs:label xml:lang="en">has issuing body</rdfs:label>
  <skos:definition xml:lang="en">Relates a resource to an agent issuing a resource, such as an official organ of the agent.</skos:definition>
  <rdf:type rdf:resource="http://www.w3.org/1999/02/22-rdf-syntax-ns#Property" />
  <rdfs:subPropertyOf rdf:resource="http://rdaregistry.info/Elements/u/P60374" />
  <owl:inverseOf rdf:resource="http://rdaregistry.info/Elements/u/P60703" />
  <reg:lexicalAlias rdf:resource="http://rdaregistry.info/Elements/u/issuingBody.en" />
</owl:ObjectProperty>

<!-- Property: is issuing body of -->
<owl:ObjectProperty rdf:about="http://rdaregistry.info/Elements/u/P60703">
  <rdfs:isDefinedBy rdf:resource="http://rdaregistry.info/Elements/u/" />
  <reg:status rdf:resource="http://metadataregistry.org/uri/RegStatus/1001" />
  <reg:name xml:lang="en">issuingBodyOf</reg:name>
  <rdfs:label xml:lang="en">is issuing body of</rdfs:label>
  <skos:definition xml:lang="en">Relates an agent issuing a resource, such as an official organ of the agent, to a resource.</skos:definition>
  <rdf:type rdf:resource="http://www.w3.org/1999/02/22-rdf-syntax-ns#Property" />
  <rdfs:subPropertyOf rdf:resource="http://rdaregistry.info/Elements/u/P60602" />
  <owl:inverseOf rdf:resource="http://rdaregistry.info/Elements/u/P60467" />
  <reg:hasSubproperty rdf:resource="http://rdaregistry.info/Elements/a/P50130" />
  <reg:lexicalAlias rdf:resource="http://rdaregistry.info/Elements/u/issuingBodyOf.en" />
</owl:ObjectProperty>

<!-- Property: DEPRECATED -->
<owl:ObjectProperty rdf:about="http://rdaregistry.info/Elements/u/P60055">
  <rdfs:isDefinedBy rdf:resource="http://rdaregistry.info/Elements/u/" />
  <reg:status rdf:resource="http://metadataregistry.org/uri/RegStatus/1008" />
</owl:ObjectProperty>

<!-- Property: has jointly held conference -->
<owl:ObjectProperty rdf:about="http://rdaregistry.info/Elements/u/P60903">
  <rdfs:isDefinedBy rdf:resource="http://rdaregistry.info/Elements/u/" />
  <reg:status rdf:resource="http://metadataregistry.org/uri/RegStatus/1001" />
  <rdf:type rdf:resource="http://www.w3.org/1999/02/22-rdf-syntax-ns#Property" />
  <reg:name xml:lang="en">jointlyHeldConference</reg:name>
  <rdfs:label xml:lang="en">has jointly held conference</rdfs:label>
  <reg:lexicalAlias rdf:resource="http://rdaregistry.info/Elements/u/jointlyHeldConference.en" />
  <skos:definition xml:lang="en">Relates a conference to a conference that is jointly held with another conference.</skos:definition>
  <owl:inverseOf rdf:resource="http://rdaregistry.info/Elements/u/P60903" />
</owl:ObjectProperty>

<!-- Property: has judge -->
<owl:ObjectProperty rdf:about="http://rdaregistry.info/Elements/u/P60461">
  <rdfs:isDefinedBy rdf:resource="http://rdaregistry.info/Elements/u/" />
  <reg:status rdf:resource="http://metadataregistry.org/uri/RegStatus/1001" />
  <reg:name xml:lang="en">judge</reg:name>
  <rdfs:label xml:lang="en">has judge</rdfs:label>
  <skos:definition xml:lang="en">Relates a resource to an agent who hears and decides on legal matters in court.</skos:definition>
  <rdf:type rdf:resource="http://www.w3.org/1999/02/22-rdf-syntax-ns#Property" />
  <rdfs:subPropertyOf rdf:resource="http://rdaregistry.info/Elements/u/P60374" />
  <owl:inverseOf rdf:resource="http://rdaregistry.info/Elements/u/P60696" />
  <reg:lexicalAlias rdf:resource="http://rdaregistry.info/Elements/u/judge.en" />
</owl:ObjectProperty>

<!-- Property: is judge of -->
<owl:ObjectProperty rdf:about="http://rdaregistry.info/Elements/u/P60696">
  <rdfs:isDefinedBy rdf:resource="http://rdaregistry.info/Elements/u/" />
  <reg:status rdf:resource="http://metadataregistry.org/uri/RegStatus/1001" />
  <reg:name xml:lang="en">judgeOf</reg:name>
  <rdfs:label xml:lang="en">is judge of</rdfs:label>
  <skos:definition xml:lang="en">Relates an agent who hears and decides on legal matters in court to a resource.</skos:definition>
  <rdf:type rdf:resource="http://www.w3.org/1999/02/22-rdf-syntax-ns#Property" />
  <rdfs:subPropertyOf rdf:resource="http://rdaregistry.info/Elements/u/P60602" />
  <owl:inverseOf rdf:resource="http://rdaregistry.info/Elements/u/P60461" />
  <reg:hasSubproperty rdf:resource="http://rdaregistry.info/Elements/a/P50126" />
  <reg:lexicalAlias rdf:resource="http://rdaregistry.info/Elements/u/judgeOf.en" />
</owl:ObjectProperty>

<!-- Property: has jurisdiction governed -->
<owl:ObjectProperty rdf:about="http://rdaregistry.info/Elements/u/P60097">
  <rdfs:isDefinedBy rdf:resource="http://rdaregistry.info/Elements/u/" />
  <reg:status rdf:resource="http://metadataregistry.org/uri/RegStatus/1001" />
  <reg:name xml:lang="en">jurisdictionGoverned</reg:name>
  <rdfs:label xml:lang="en">has jurisdiction governed</rdfs:label>
  <skos:definition xml:lang="en">Relates a resource to a jurisdiction governed by a law, regulation, etc., that was enacted by another jurisdiction.</skos:definition>
  <rdf:type rdf:resource="http://www.w3.org/1999/02/22-rdf-syntax-ns#Property" />
  <rdfs:subPropertyOf rdf:resource="http://rdaregistry.info/Elements/u/P60374" />
  <owl:inverseOf rdf:resource="http://rdaregistry.info/Elements/u/P60015" />
  <reg:lexicalAlias rdf:resource="http://rdaregistry.info/Elements/u/jurisdictionGoverned.en" />
</owl:ObjectProperty>

<!-- Property: is jurisdiction governed of -->
<owl:ObjectProperty rdf:about="http://rdaregistry.info/Elements/u/P60015">
  <rdfs:isDefinedBy rdf:resource="http://rdaregistry.info/Elements/u/" />
  <reg:status rdf:resource="http://metadataregistry.org/uri/RegStatus/1001" />
  <reg:name xml:lang="en">jurisdictionGovernedOf</reg:name>
  <rdfs:label xml:lang="en">is jurisdiction governed of</rdfs:label>
  <skos:definition xml:lang="en">Relates a jurisdiction governed by a law, regulation, etc., that was enacted by another jurisdiction to a resource.</skos:definition>
  <rdf:type rdf:resource="http://www.w3.org/1999/02/22-rdf-syntax-ns#Property" />
  <rdfs:subPropertyOf rdf:resource="http://rdaregistry.info/Elements/u/P60602" />
  <owl:inverseOf rdf:resource="http://rdaregistry.info/Elements/u/P60097" />
  <reg:hasSubproperty rdf:resource="http://rdaregistry.info/Elements/a/P50069" />
  <reg:lexicalAlias rdf:resource="http://rdaregistry.info/Elements/u/jurisdictionGovernedOf.en" />
</owl:ObjectProperty>

<!-- Property: has key -->
<owl:ObjectProperty rdf:about="http://rdaregistry.info/Elements/u/P60580">
  <rdfs:isDefinedBy rdf:resource="http://rdaregistry.info/Elements/u/" />
  <reg:status rdf:resource="http://metadataregistry.org/uri/RegStatus/1001" />
  <reg:name xml:lang="en">key</reg:name>
  <rdfs:label xml:lang="en">has key</rdfs:label>
  <skos:definition xml:lang="en">Relates a resource to a set of pitch relationships that establishes a tonal centre, or principal tonal centre, of a musical resource.</skos:definition>
  <rdf:type rdf:resource="http://www.w3.org/1999/02/22-rdf-syntax-ns#Property" />
  <reg:lexicalAlias rdf:resource="http://rdaregistry.info/Elements/u/key.en" />
</owl:ObjectProperty>

<!-- Property: has key title -->
<owl:ObjectProperty rdf:about="http://rdaregistry.info/Elements/u/P60597">
  <rdfs:isDefinedBy rdf:resource="http://rdaregistry.info/Elements/u/" />
  <reg:status rdf:resource="http://metadataregistry.org/uri/RegStatus/1001" />
  <reg:name xml:lang="en">keyTitle</reg:name>
  <rdfs:label xml:lang="en">has key title</rdfs:label>
  <skos:definition xml:lang="en">Relates a resource to a unique name assigned to a resource by an ISSN registration agency.</skos:definition>
  <rdf:type rdf:resource="http://www.w3.org/1999/02/22-rdf-syntax-ns#Property" />
  <rdfs:subPropertyOf rdf:resource="http://rdaregistry.info/Elements/u/P60369" />
  <reg:hasSubproperty rdf:resource="http://rdaregistry.info/Elements/m/P30209" />
  <reg:lexicalAlias rdf:resource="http://rdaregistry.info/Elements/u/keyTitle.en" />
</owl:ObjectProperty>

<!-- Property: has landscape architect -->
<owl:ObjectProperty rdf:about="http://rdaregistry.info/Elements/u/P60473">
  <rdfs:isDefinedBy rdf:resource="http://rdaregistry.info/Elements/u/" />
  <reg:status rdf:resource="http://metadataregistry.org/uri/RegStatus/1001" />
  <reg:name xml:lang="en">landscapeArchitect</reg:name>
  <rdfs:label xml:lang="en">has landscape architect</rdfs:label>
  <skos:definition xml:lang="en">Relates a resource to an architect responsible for creating landscape resources.</skos:definition>
  <rdf:type rdf:resource="http://www.w3.org/1999/02/22-rdf-syntax-ns#Property" />
  <rdfs:subPropertyOf rdf:resource="http://rdaregistry.info/Elements/u/P60435" />
  <owl:inverseOf rdf:resource="http://rdaregistry.info/Elements/u/P60704" />
  <reg:lexicalAlias rdf:resource="http://rdaregistry.info/Elements/u/landscapeArchitect.en" />
</owl:ObjectProperty>

<!-- Property: is landscape architect of -->
<owl:ObjectProperty rdf:about="http://rdaregistry.info/Elements/u/P60704">
  <rdfs:isDefinedBy rdf:resource="http://rdaregistry.info/Elements/u/" />
  <reg:status rdf:resource="http://metadataregistry.org/uri/RegStatus/1001" />
  <reg:name xml:lang="en">landscapeArchitectOf</reg:name>
  <rdfs:label xml:lang="en">is landscape architect of</rdfs:label>
  <skos:definition xml:lang="en">Relates an architect responsible for creating landscape resources to a resource.</skos:definition>
  <rdf:type rdf:resource="http://www.w3.org/1999/02/22-rdf-syntax-ns#Property" />
  <rdfs:subPropertyOf rdf:resource="http://rdaregistry.info/Elements/u/P60664" />
  <owl:inverseOf rdf:resource="http://rdaregistry.info/Elements/u/P60473" />
  <reg:hasSubproperty rdf:resource="http://rdaregistry.info/Elements/a/P50221" />
  <reg:lexicalAlias rdf:resource="http://rdaregistry.info/Elements/u/landscapeArchitectOf.en" />
</owl:ObjectProperty>

<!-- Property: has language of agent -->
<owl:ObjectProperty rdf:about="http://rdaregistry.info/Elements/u/P60098">
  <rdfs:isDefinedBy rdf:resource="http://rdaregistry.info/Elements/u/" />
  <reg:status rdf:resource="http://metadataregistry.org/uri/RegStatus/1001" />
  <reg:name xml:lang="en">languageOfAgent</reg:name>
  <rdfs:label xml:lang="en">has language of agent</rdfs:label>
  <skos:definition xml:lang="en">Relates a resource to a language an agent uses in its communications, when writing for publication, broadcasting, etc.</skos:definition>
  <rdf:type rdf:resource="http://www.w3.org/1999/02/22-rdf-syntax-ns#Property" />
  <reg:hasSubproperty rdf:resource="http://rdaregistry.info/Elements/a/P50023" />
  <reg:hasSubproperty rdf:resource="http://rdaregistry.info/Elements/a/P50102" />
  <reg:hasSubproperty rdf:resource="http://rdaregistry.info/Elements/a/P50235" />
  <reg:lexicalAlias rdf:resource="http://rdaregistry.info/Elements/u/languageOfAgent.en" />
</owl:ObjectProperty>

<!-- Property: has language of content -->
<owl:ObjectProperty rdf:about="http://rdaregistry.info/Elements/u/P60099">
  <rdfs:isDefinedBy rdf:resource="http://rdaregistry.info/Elements/u/" />
  <reg:status rdf:resource="http://metadataregistry.org/uri/RegStatus/1001" />
  <reg:name xml:lang="en">languageOfContent</reg:name>
  <rdfs:label xml:lang="en">has language of content</rdfs:label>
  <skos:definition xml:lang="en">Relates a resource to a language used to express the content of a resource.</skos:definition>
  <rdf:type rdf:resource="http://www.w3.org/1999/02/22-rdf-syntax-ns#Property" />
  <reg:hasSubproperty rdf:resource="http://rdaregistry.info/Elements/e/P20006" />
  <reg:hasSubproperty rdf:resource="http://rdaregistry.info/Elements/e/P20007" />
  <reg:lexicalAlias rdf:resource="http://rdaregistry.info/Elements/u/languageOfContent.en" />
</owl:ObjectProperty>

<!-- Property: has later title proper -->
<owl:ObjectProperty rdf:about="http://rdaregistry.info/Elements/u/P60357">
  <rdfs:isDefinedBy rdf:resource="http://rdaregistry.info/Elements/u/" />
  <reg:status rdf:resource="http://metadataregistry.org/uri/RegStatus/1001" />
  <reg:name xml:lang="en">laterTitleProper</reg:name>
  <rdfs:label xml:lang="en">has later title proper</rdfs:label>
  <skos:definition xml:lang="en">Relates a resource to a title proper appearing on a later issue or part of a multipart monograph or serial that differs from that on the first or earliest issue or part.</skos:definition>
  <rdf:type rdf:resource="http://www.w3.org/1999/02/22-rdf-syntax-ns#Property" />
  <rdfs:subPropertyOf rdf:resource="http://rdaregistry.info/Elements/u/P60369" />
  <reg:hasSubproperty rdf:resource="http://rdaregistry.info/Elements/m/P30129" />
  <reg:lexicalAlias rdf:resource="http://rdaregistry.info/Elements/u/laterTitleProper.en" />
</owl:ObjectProperty>

<!-- Property: has latitude -->
<owl:ObjectProperty rdf:about="http://rdaregistry.info/Elements/u/P60897">
  <rdfs:isDefinedBy rdf:resource="http://rdaregistry.info/Elements/u/" />
  <reg:status rdf:resource="http://metadataregistry.org/uri/RegStatus/1001" />
  <rdf:type rdf:resource="http://www.w3.org/1999/02/22-rdf-syntax-ns#Property" />
  <reg:name xml:lang="en">latitude</reg:name>
  <rdfs:label xml:lang="en">has latitude</rdfs:label>
  <reg:lexicalAlias rdf:resource="http://rdaregistry.info/Elements/u/latitude.en" />
  <skos:definition xml:lang="en">Relates a resource to a distance of a point on a planet or satellite measured north and south from the equator.</skos:definition>
</owl:ObjectProperty>

<!-- Property: has layout -->
<owl:ObjectProperty rdf:about="http://rdaregistry.info/Elements/u/P60513">
  <rdfs:isDefinedBy rdf:resource="http://rdaregistry.info/Elements/u/" />
  <reg:status rdf:resource="http://metadataregistry.org/uri/RegStatus/1001" />
  <reg:name xml:lang="en">layout</reg:name>
  <rdfs:label xml:lang="en">has layout</rdfs:label>
  <skos:definition xml:lang="en">Relates a resource to an arrangement of text, images, tactile notation, etc., in a resource.</skos:definition>
  <rdf:type rdf:resource="http://www.w3.org/1999/02/22-rdf-syntax-ns#Property" />
  <reg:hasSubproperty rdf:resource="http://rdaregistry.info/Elements/m/P30155" />
  <reg:lexicalAlias rdf:resource="http://rdaregistry.info/Elements/u/layout.en" />
</owl:ObjectProperty>

<!-- Property: has letterer -->
<owl:ObjectProperty rdf:about="http://rdaregistry.info/Elements/u/P60750">
  <rdfs:isDefinedBy rdf:resource="http://rdaregistry.info/Elements/u/" />
  <reg:status rdf:resource="http://metadataregistry.org/uri/RegStatus/1001" />
  <rdf:type rdf:resource="http://www.w3.org/1999/02/22-rdf-syntax-ns#Property" />
  <reg:name xml:lang="en">letterer</reg:name>
  <rdfs:label xml:lang="en">has letterer</rdfs:label>
  <reg:lexicalAlias rdf:resource="http://rdaregistry.info/Elements/u/letterer.en" />
  <skos:definition xml:lang="en">Relates a resource to an illustrator contributing to a comic book, graphic novel, etc., by drawing text and graphic sound effects.</skos:definition>
  <owl:inverseOf rdf:resource="http://rdaregistry.info/Elements/u/P60756" />
  <rdfs:subPropertyOf rdf:resource="http://rdaregistry.info/Elements/u/P60396" />
</owl:ObjectProperty>

<!-- Property: is letterer of -->
<owl:ObjectProperty rdf:about="http://rdaregistry.info/Elements/u/P60756">
  <rdfs:isDefinedBy rdf:resource="http://rdaregistry.info/Elements/u/" />
  <reg:status rdf:resource="http://metadataregistry.org/uri/RegStatus/1001" />
  <rdf:type rdf:resource="http://www.w3.org/1999/02/22-rdf-syntax-ns#Property" />
  <reg:name xml:lang="en">lettererOf</reg:name>
  <rdfs:label xml:lang="en">is letterer of</rdfs:label>
  <reg:lexicalAlias rdf:resource="http://rdaregistry.info/Elements/u/lettererOf.en" />
  <skos:definition xml:lang="en">Relates an illustrator contributing to a comic book, graphic novel, etc., by drawing text and graphic sound effects to a resource.</skos:definition>
  <owl:inverseOf rdf:resource="http://rdaregistry.info/Elements/u/P60750" />
  <rdfs:subPropertyOf rdf:resource="http://rdaregistry.info/Elements/u/P60624" />
</owl:ObjectProperty>

<!-- Property: has librettist -->
<owl:ObjectProperty rdf:about="http://rdaregistry.info/Elements/u/P60478">
  <rdfs:isDefinedBy rdf:resource="http://rdaregistry.info/Elements/u/" />
  <reg:status rdf:resource="http://metadataregistry.org/uri/RegStatus/1001" />
  <reg:name xml:lang="en">librettist</reg:name>
  <rdfs:label xml:lang="en">has librettist</rdfs:label>
  <skos:definition xml:lang="en">Relates a resource to an author of words of an opera or other musical stage resource or an oratorio.</skos:definition>
  <rdf:type rdf:resource="http://www.w3.org/1999/02/22-rdf-syntax-ns#Property" />
  <rdfs:subPropertyOf rdf:resource="http://rdaregistry.info/Elements/u/P60434" />
  <owl:inverseOf rdf:resource="http://rdaregistry.info/Elements/u/P60708" />
  <reg:lexicalAlias rdf:resource="http://rdaregistry.info/Elements/u/librettist.en" />
  <skos:scopeNote xml:lang="en">Authoring of the words of just the songs from a musical is excluded.</skos:scopeNote>
  <rdakit:seeAlso rdf:resource="http://rdaregistry.info/Elements/u/P60477" />
</owl:ObjectProperty>

<!-- Property: is librettist of -->
<owl:ObjectProperty rdf:about="http://rdaregistry.info/Elements/u/P60708">
  <rdfs:isDefinedBy rdf:resource="http://rdaregistry.info/Elements/u/" />
  <reg:status rdf:resource="http://metadataregistry.org/uri/RegStatus/1001" />
  <reg:name xml:lang="en">librettistOf</reg:name>
  <rdfs:label xml:lang="en">is librettist of</rdfs:label>
  <skos:definition xml:lang="en">Relates an author of words of an opera or other musical stage resource or an oratorio to a resource.</skos:definition>
  <rdf:type rdf:resource="http://www.w3.org/1999/02/22-rdf-syntax-ns#Property" />
  <rdfs:subPropertyOf rdf:resource="http://rdaregistry.info/Elements/u/P60663" />
  <owl:inverseOf rdf:resource="http://rdaregistry.info/Elements/u/P60478" />
  <reg:hasSubproperty rdf:resource="http://rdaregistry.info/Elements/a/P50225" />
  <reg:lexicalAlias rdf:resource="http://rdaregistry.info/Elements/u/librettistOf.en" />
  <rdakit:seeAlso rdf:resource="http://rdaregistry.info/Elements/u/P60707" />
</owl:ObjectProperty>

<!-- Property: is libretto -->
<owl:ObjectProperty rdf:about="http://rdaregistry.info/Elements/u/P60270">
  <rdfs:isDefinedBy rdf:resource="http://rdaregistry.info/Elements/u/" />
  <reg:status rdf:resource="http://metadataregistry.org/uri/RegStatus/1001" />
  <reg:name xml:lang="en">libretto</reg:name>
  <rdfs:label xml:lang="en">is libretto</rdfs:label>
  <skos:definition xml:lang="en">Relates a resource to a resource that provides a text of an opera or other resource for the musical stage, or an oratorio.</skos:definition>
  <rdf:type rdf:resource="http://www.w3.org/1999/02/22-rdf-syntax-ns#Property" />
  <rdfs:subPropertyOf rdf:resource="http://rdaregistry.info/Elements/u/P60198" />
  <owl:inverseOf rdf:resource="http://rdaregistry.info/Elements/u/P60117" />
  <reg:hasSubproperty rdf:resource="http://rdaregistry.info/Elements/e/P20163" />
  <reg:lexicalAlias rdf:resource="http://rdaregistry.info/Elements/u/libretto.en" />
</owl:ObjectProperty>

<!-- Property: is libretto based on -->
<owl:ObjectProperty rdf:about="http://rdaregistry.info/Elements/u/P60304">
  <rdfs:isDefinedBy rdf:resource="http://rdaregistry.info/Elements/u/" />
  <reg:status rdf:resource="http://metadataregistry.org/uri/RegStatus/1001" />
  <reg:name xml:lang="en">librettoBasedOn</reg:name>
  <rdfs:label xml:lang="en">is libretto based on</rdfs:label>
  <skos:definition xml:lang="en">Relates a resource to a resource that has been adapted as a text of an opera or other resource for the musical stage, or an oratorio.</skos:definition>
  <rdf:type rdf:resource="http://www.w3.org/1999/02/22-rdf-syntax-ns#Property" />
  <rdfs:subPropertyOf rdf:resource="http://rdaregistry.info/Elements/u/P60305" />
  <owl:inverseOf rdf:resource="http://rdaregistry.info/Elements/u/P60210" />
  <reg:hasSubproperty rdf:resource="http://rdaregistry.info/Elements/e/P20190" />
  <reg:lexicalAlias rdf:resource="http://rdaregistry.info/Elements/u/librettoBasedOn.en" />
</owl:ObjectProperty>

<!-- Property: is libretto for -->
<owl:ObjectProperty rdf:about="http://rdaregistry.info/Elements/u/P60117">
  <rdfs:isDefinedBy rdf:resource="http://rdaregistry.info/Elements/u/" />
  <reg:status rdf:resource="http://metadataregistry.org/uri/RegStatus/1001" />
  <reg:name xml:lang="en">librettoFor</reg:name>
  <rdfs:label xml:lang="en">is libretto for</rdfs:label>
  <skos:definition xml:lang="en">Relates a resource to a musical resource such as an opera or other resource for the musical stage, or an oratorio, that uses a text of a related resource.</skos:definition>
  <rdf:type rdf:resource="http://www.w3.org/1999/02/22-rdf-syntax-ns#Property" />
  <rdfs:subPropertyOf rdf:resource="http://rdaregistry.info/Elements/u/P60198" />
  <owl:inverseOf rdf:resource="http://rdaregistry.info/Elements/u/P60270" />
  <reg:hasSubproperty rdf:resource="http://rdaregistry.info/Elements/e/P20084" />
  <reg:lexicalAlias rdf:resource="http://rdaregistry.info/Elements/u/librettoFor.en" />
</owl:ObjectProperty>

<!-- Property: has lighting designer -->
<owl:ObjectProperty rdf:about="http://rdaregistry.info/Elements/u/P60813">
  <rdfs:isDefinedBy rdf:resource="http://rdaregistry.info/Elements/u/" />
  <reg:status rdf:resource="http://metadataregistry.org/uri/RegStatus/1001" />
  <rdf:type rdf:resource="http://www.w3.org/1999/02/22-rdf-syntax-ns#Property" />
  <reg:name xml:lang="en">lightingDesigner</reg:name>
  <rdfs:label xml:lang="en">has lighting designer</rdfs:label>
  <reg:lexicalAlias rdf:resource="http://rdaregistry.info/Elements/u/lightingDesigner.en" />
  <skos:definition xml:lang="en">Relates a resource to an agent contributing to a resource by designing and creating lighting components.</skos:definition>
  <owl:inverseOf rdf:resource="http://rdaregistry.info/Elements/u/P60814" />
  <rdfs:subPropertyOf rdf:resource="http://rdaregistry.info/Elements/u/P60398" />
</owl:ObjectProperty>

<!-- Property: is lighting designer of -->
<owl:ObjectProperty rdf:about="http://rdaregistry.info/Elements/u/P60814">
  <rdfs:isDefinedBy rdf:resource="http://rdaregistry.info/Elements/u/" />
  <reg:status rdf:resource="http://metadataregistry.org/uri/RegStatus/1001" />
  <rdf:type rdf:resource="http://www.w3.org/1999/02/22-rdf-syntax-ns#Property" />
  <reg:name xml:lang="en">lightingDesignerOf</reg:name>
  <rdfs:label xml:lang="en">is lighting designer of</rdfs:label>
  <reg:lexicalAlias rdf:resource="http://rdaregistry.info/Elements/u/lightingDesignerOf.en" />
  <skos:definition xml:lang="en">Relates an agent contributing to a resource by designing and creating lighting components to a resource.</skos:definition>
  <owl:inverseOf rdf:resource="http://rdaregistry.info/Elements/u/P60813" />
  <rdfs:subPropertyOf rdf:resource="http://rdaregistry.info/Elements/u/P60626" />
</owl:ObjectProperty>

<!-- Property: has lithographer -->
<owl:ObjectProperty rdf:about="http://rdaregistry.info/Elements/u/P60414">
  <rdfs:isDefinedBy rdf:resource="http://rdaregistry.info/Elements/u/" />
  <reg:status rdf:resource="http://metadataregistry.org/uri/RegStatus/1001" />
  <reg:name xml:lang="en">lithographer</reg:name>
  <rdfs:label xml:lang="en">has lithographer</rdfs:label>
  <skos:definition xml:lang="en">Relates a resource to an agent involved in manufacturing a resource by preparing a stone or plate for lithographic printing.</skos:definition>
  <rdf:type rdf:resource="http://www.w3.org/1999/02/22-rdf-syntax-ns#Property" />
  <rdfs:subPropertyOf rdf:resource="http://rdaregistry.info/Elements/u/P60443" />
  <owl:inverseOf rdf:resource="http://rdaregistry.info/Elements/u/P60642" />
  <reg:hasSubproperty rdf:resource="http://rdaregistry.info/Elements/m/P30074" />
  <reg:lexicalAlias rdf:resource="http://rdaregistry.info/Elements/u/lithographer.en" />
  <skos:scopeNote xml:lang="en">A lithographer includes a graphic artist creating a design directly on the surface from which printing will be done.</skos:scopeNote>
</owl:ObjectProperty>

<!-- Property: is lithographer of -->
<owl:ObjectProperty rdf:about="http://rdaregistry.info/Elements/u/P60642">
  <rdfs:isDefinedBy rdf:resource="http://rdaregistry.info/Elements/u/" />
  <reg:status rdf:resource="http://metadataregistry.org/uri/RegStatus/1001" />
  <reg:name xml:lang="en">lithographerOf</reg:name>
  <rdfs:label xml:lang="en">is lithographer of</rdfs:label>
  <skos:definition xml:lang="en">Relates an agent involved in manufacturing a resource by preparing a stone or plate for lithographic printing.</skos:definition>
  <rdf:type rdf:resource="http://www.w3.org/1999/02/22-rdf-syntax-ns#Property" />
  <rdfs:subPropertyOf rdf:resource="http://rdaregistry.info/Elements/u/P60669" />
  <owl:inverseOf rdf:resource="http://rdaregistry.info/Elements/u/P60414" />
  <reg:hasSubproperty rdf:resource="http://rdaregistry.info/Elements/a/P50175" />
  <reg:lexicalAlias rdf:resource="http://rdaregistry.info/Elements/u/lithographerOf.en" />
  <skos:scopeNote xml:lang="en">A lithographer includes a graphic artist creating a design directly on the surface from which printing will be done.</skos:scopeNote>
</owl:ObjectProperty>

<!-- Property: has local affiliate -->
<owl:ObjectProperty rdf:about="http://rdaregistry.info/Elements/u/P60739">
  <rdfs:isDefinedBy rdf:resource="http://rdaregistry.info/Elements/u/" />
  <reg:status rdf:resource="http://metadataregistry.org/uri/RegStatus/1001" />
  <rdf:type rdf:resource="http://www.w3.org/1999/02/22-rdf-syntax-ns#Property" />
  <reg:name xml:lang="en">localAffiliate</reg:name>
  <rdfs:label xml:lang="en">has local affiliate</rdfs:label>
  <reg:lexicalAlias rdf:resource="http://rdaregistry.info/Elements/u/localAffiliate.en" />
  <skos:definition xml:lang="en">Relates a local agent affiliated with a broader agent which acts for it and others at a broader organizational level to an agent.</skos:definition>
</owl:ObjectProperty>

<!-- Property: has location of conference, etc. -->
<owl:ObjectProperty rdf:about="http://rdaregistry.info/Elements/u/P60107">
  <rdfs:isDefinedBy rdf:resource="http://rdaregistry.info/Elements/u/" />
  <reg:status rdf:resource="http://metadataregistry.org/uri/RegStatus/1001" />
  <reg:name xml:lang="en">locationOfConferenceEtc</reg:name>
  <rdfs:label xml:lang="en">has location of conference, etc.</rdfs:label>
  <skos:definition xml:lang="en">Relates a resource to a local place in which a conference, congress, meeting, exhibition, fair, festival, etc., was held.</skos:definition>
  <rdf:type rdf:resource="http://www.w3.org/1999/02/22-rdf-syntax-ns#Property" />
  <rdfs:subPropertyOf rdf:resource="http://rdaregistry.info/Elements/u/P60325" />
  <reg:hasSubproperty rdf:resource="http://rdaregistry.info/Elements/a/P50024" />
  <reg:lexicalAlias rdf:resource="http://rdaregistry.info/Elements/u/locationOfConferenceEtc.en" />
</owl:ObjectProperty>

<!-- Property: DEPRECATED -->
<owl:ObjectProperty rdf:about="http://rdaregistry.info/Elements/u/P60064">
  <rdfs:isDefinedBy rdf:resource="http://rdaregistry.info/Elements/u/" />
  <reg:status rdf:resource="http://metadataregistry.org/uri/RegStatus/1008" />
  <reg:name xml:lang="en">locationOfHeadquarters</reg:name>
  <rdf:type rdf:resource="http://www.w3.org/1999/02/22-rdf-syntax-ns#Property" />
  <rdfs:subPropertyOf rdf:resource="http://rdaregistry.info/Elements/u/P60325" />
  <reg:lexicalAlias rdf:resource="http://rdaregistry.info/Elements/u/locationOfHeadquarters.en" />
</owl:ObjectProperty>

<!-- Property: has longitude -->
<owl:ObjectProperty rdf:about="http://rdaregistry.info/Elements/u/P60898">
  <rdfs:isDefinedBy rdf:resource="http://rdaregistry.info/Elements/u/" />
  <reg:status rdf:resource="http://metadataregistry.org/uri/RegStatus/1001" />
  <rdf:type rdf:resource="http://www.w3.org/1999/02/22-rdf-syntax-ns#Property" />
  <reg:name xml:lang="en">longitude</reg:name>
  <rdfs:label xml:lang="en">has longitude</rdfs:label>
  <reg:lexicalAlias rdf:resource="http://rdaregistry.info/Elements/u/longitude.en" />
  <skos:definition xml:lang="en">Relates a resource to a distance of a point on a planet or satellite measured east and west from a reference meridian.</skos:definition>
</owl:ObjectProperty>

<!-- Property: has longitude and latitude -->
<owl:ObjectProperty rdf:about="http://rdaregistry.info/Elements/u/P60345">
  <rdfs:isDefinedBy rdf:resource="http://rdaregistry.info/Elements/u/" />
  <reg:status rdf:resource="http://metadataregistry.org/uri/RegStatus/1001" />
  <reg:name xml:lang="en">longitudeAndLatitude</reg:name>
  <rdfs:label xml:lang="en">has longitude and latitude</rdfs:label>
  <skos:definition xml:lang="en">Relates a resource to a system for identifying the area covered by the cartographic content of a resource using longitude of the westernmost and easternmost boundaries and latitude of the northernmost and southernmost boundaries.</skos:definition>
  <rdf:type rdf:resource="http://www.w3.org/1999/02/22-rdf-syntax-ns#Property" />
  <rdfs:subPropertyOf rdf:resource="http://rdaregistry.info/Elements/u/P60109" />
  <reg:lexicalAlias rdf:resource="http://rdaregistry.info/Elements/u/longitudeAndLatitude.en" />
</owl:ObjectProperty>

<!-- Property: has lyricist -->
<owl:ObjectProperty rdf:about="http://rdaregistry.info/Elements/u/P60477">
  <rdfs:isDefinedBy rdf:resource="http://rdaregistry.info/Elements/u/" />
  <reg:status rdf:resource="http://metadataregistry.org/uri/RegStatus/1001" />
  <reg:name xml:lang="en">lyricist</reg:name>
  <rdfs:label xml:lang="en">has lyricist</rdfs:label>
  <skos:definition xml:lang="en">Relates a resource to an author of the words of a popular song, including a song or songs from a musical.</skos:definition>
  <rdf:type rdf:resource="http://www.w3.org/1999/02/22-rdf-syntax-ns#Property" />
  <rdfs:subPropertyOf rdf:resource="http://rdaregistry.info/Elements/u/P60434" />
  <owl:inverseOf rdf:resource="http://rdaregistry.info/Elements/u/P60707" />
  <reg:lexicalAlias rdf:resource="http://rdaregistry.info/Elements/u/lyricist.en" />
  <skos:scopeNote xml:lang="en">Authoring of just dialogue from a musical is excluded</skos:scopeNote>
  <rdakit:seeAlso rdf:resource="http://rdaregistry.info/Elements/u/P60478" />
</owl:ObjectProperty>

<!-- Property: is lyricist of -->
<owl:ObjectProperty rdf:about="http://rdaregistry.info/Elements/u/P60707">
  <rdfs:isDefinedBy rdf:resource="http://rdaregistry.info/Elements/u/" />
  <reg:status rdf:resource="http://metadataregistry.org/uri/RegStatus/1001" />
  <reg:name xml:lang="en">lyricistOf</reg:name>
  <rdfs:label xml:lang="en">is lyricist of</rdfs:label>
  <skos:definition xml:lang="en">Relates an author of the words of a popular song, including a song or songs from a musical to a resource.</skos:definition>
  <rdf:type rdf:resource="http://www.w3.org/1999/02/22-rdf-syntax-ns#Property" />
  <rdfs:subPropertyOf rdf:resource="http://rdaregistry.info/Elements/u/P60663" />
  <owl:inverseOf rdf:resource="http://rdaregistry.info/Elements/u/P60477" />
  <reg:hasSubproperty rdf:resource="http://rdaregistry.info/Elements/a/P50224" />
  <reg:lexicalAlias rdf:resource="http://rdaregistry.info/Elements/u/lyricistOf.en" />
  <rdakit:seeAlso rdf:resource="http://rdaregistry.info/Elements/u/P60708" />
</owl:ObjectProperty>

<!-- Property: has make-up artist -->
<owl:ObjectProperty rdf:about="http://rdaregistry.info/Elements/u/P60840">
  <rdfs:isDefinedBy rdf:resource="http://rdaregistry.info/Elements/u/" />
  <reg:status rdf:resource="http://metadataregistry.org/uri/RegStatus/1001" />
  <rdf:type rdf:resource="http://www.w3.org/1999/02/22-rdf-syntax-ns#Property" />
  <reg:name xml:lang="en">makeUpArtist</reg:name>
  <rdfs:label xml:lang="en">has make-up artist</rdfs:label>
  <reg:lexicalAlias rdf:resource="http://rdaregistry.info/Elements/u/makeUpArtist.en" />
  <skos:definition xml:lang="en">Relates a resource to an agent contributing to a resource by applying make-up and prosthetics for a moving image production or for a musical or dramatic presentation or entertainment.</skos:definition>
  <owl:inverseOf rdf:resource="http://rdaregistry.info/Elements/u/P60841" />
  <reg:hasSubproperty rdf:resource="http://rdaregistry.info/Elements/e/P20284" />
  <rdfs:subPropertyOf rdf:resource="http://rdaregistry.info/Elements/u/P60398" />
</owl:ObjectProperty>

<!-- Property: is make-up artist of -->
<owl:ObjectProperty rdf:about="http://rdaregistry.info/Elements/u/P60841">
  <rdfs:isDefinedBy rdf:resource="http://rdaregistry.info/Elements/u/" />
  <reg:status rdf:resource="http://metadataregistry.org/uri/RegStatus/1001" />
  <rdf:type rdf:resource="http://www.w3.org/1999/02/22-rdf-syntax-ns#Property" />
  <reg:name xml:lang="en">makeUpArtistOf</reg:name>
  <rdfs:label xml:lang="en">is make-up artist of</rdfs:label>
  <reg:lexicalAlias rdf:resource="http://rdaregistry.info/Elements/u/makeUpArtistOf.en" />
  <skos:definition xml:lang="en">Relates an agent contributing to a resource by applying make-up and prosthetics for a moving image production or for a musical or dramatic presentation or entertainment to a resource.</skos:definition>
  <owl:inverseOf rdf:resource="http://rdaregistry.info/Elements/u/P60840" />
  <reg:hasSubproperty rdf:resource="http://rdaregistry.info/Elements/a/P50267" />
  <rdfs:subPropertyOf rdf:resource="http://rdaregistry.info/Elements/u/P60626" />
</owl:ObjectProperty>

<!-- Property: has manufacturer -->
<owl:ObjectProperty rdf:about="http://rdaregistry.info/Elements/u/P60443">
  <rdfs:isDefinedBy rdf:resource="http://rdaregistry.info/Elements/u/" />
  <reg:status rdf:resource="http://metadataregistry.org/uri/RegStatus/1001" />
  <reg:name xml:lang="en">manufacturer</reg:name>
  <rdfs:label xml:lang="en">has manufacturer</rdfs:label>
  <skos:definition xml:lang="en">Relates a resource to an agent responsible for printing, duplicating, casting, etc., a resource in a published form.</skos:definition>
  <rdf:type rdf:resource="http://www.w3.org/1999/02/22-rdf-syntax-ns#Property" />
  <owl:inverseOf rdf:resource="http://rdaregistry.info/Elements/u/P60669" />
  <reg:hasSubproperty rdf:resource="http://rdaregistry.info/Elements/u/P60409" />
  <reg:hasSubproperty rdf:resource="http://rdaregistry.info/Elements/u/P60410" />
  <reg:hasSubproperty rdf:resource="http://rdaregistry.info/Elements/u/P60411" />
  <reg:hasSubproperty rdf:resource="http://rdaregistry.info/Elements/u/P60412" />
  <reg:hasSubproperty rdf:resource="http://rdaregistry.info/Elements/u/P60413" />
  <reg:hasSubproperty rdf:resource="http://rdaregistry.info/Elements/u/P60414" />
  <reg:hasSubproperty rdf:resource="http://rdaregistry.info/Elements/u/P60415" />
  <reg:hasSubproperty rdf:resource="http://rdaregistry.info/Elements/u/P60416" />
  <reg:hasSubproperty rdf:resource="http://rdaregistry.info/Elements/u/P60417" />
  <reg:hasSubproperty rdf:resource="http://rdaregistry.info/Elements/u/P60418" />
  <reg:hasSubproperty rdf:resource="http://rdaregistry.info/Elements/m/P30082" />
  <reg:lexicalAlias rdf:resource="http://rdaregistry.info/Elements/u/manufacturer.en" />
  <reg:hasSubproperty rdf:resource="http://rdaregistry.info/Elements/u/P60746" />
</owl:ObjectProperty>

<!-- Property: is manufacturer of -->
<owl:ObjectProperty rdf:about="http://rdaregistry.info/Elements/u/P60669">
  <rdfs:isDefinedBy rdf:resource="http://rdaregistry.info/Elements/u/" />
  <reg:status rdf:resource="http://metadataregistry.org/uri/RegStatus/1001" />
  <reg:name xml:lang="en">manufacturerOf</reg:name>
  <rdfs:label xml:lang="en">is manufacturer of</rdfs:label>
  <skos:definition xml:lang="en">Relates an agent responsible for printing, duplicating, casting, etc., a resource in a published form to a resource.</skos:definition>
  <rdf:type rdf:resource="http://www.w3.org/1999/02/22-rdf-syntax-ns#Property" />
  <owl:inverseOf rdf:resource="http://rdaregistry.info/Elements/u/P60443" />
  <reg:hasSubproperty rdf:resource="http://rdaregistry.info/Elements/u/P60637" />
  <reg:hasSubproperty rdf:resource="http://rdaregistry.info/Elements/u/P60638" />
  <reg:hasSubproperty rdf:resource="http://rdaregistry.info/Elements/u/P60639" />
  <reg:hasSubproperty rdf:resource="http://rdaregistry.info/Elements/u/P60640" />
  <reg:hasSubproperty rdf:resource="http://rdaregistry.info/Elements/u/P60641" />
  <reg:hasSubproperty rdf:resource="http://rdaregistry.info/Elements/u/P60642" />
  <reg:hasSubproperty rdf:resource="http://rdaregistry.info/Elements/u/P60643" />
  <reg:hasSubproperty rdf:resource="http://rdaregistry.info/Elements/u/P60644" />
  <reg:hasSubproperty rdf:resource="http://rdaregistry.info/Elements/u/P60645" />
  <reg:hasSubproperty rdf:resource="http://rdaregistry.info/Elements/u/P60646" />
  <reg:hasSubproperty rdf:resource="http://rdaregistry.info/Elements/a/P50202" />
  <reg:lexicalAlias rdf:resource="http://rdaregistry.info/Elements/u/manufacturerOf.en" />
  <reg:hasSubproperty rdf:resource="http://rdaregistry.info/Elements/u/P60747" />
</owl:ObjectProperty>

<!-- Property: has manufacturers name -->
<owl:ObjectProperty rdf:about="http://rdaregistry.info/Elements/u/P60546">
  <rdfs:isDefinedBy rdf:resource="http://rdaregistry.info/Elements/u/" />
  <reg:status rdf:resource="http://metadataregistry.org/uri/RegStatus/1001" />
  <reg:name xml:lang="en">manufacturersName</reg:name>
  <rdfs:label xml:lang="en">has manufacturers name</rdfs:label>
  <skos:definition xml:lang="en">Relates a resource to a name of an agent responsible for printing, duplicating, casting, etc., a resource in a published form.</skos:definition>
  <rdf:type rdf:resource="http://www.w3.org/1999/02/22-rdf-syntax-ns#Property" />
  <reg:hasSubproperty rdf:resource="http://rdaregistry.info/Elements/m/P30175" />
  <reg:lexicalAlias rdf:resource="http://rdaregistry.info/Elements/u/manufacturersName.en" />
</owl:ObjectProperty>

<!-- Property: has manufacture statement -->
<owl:ObjectProperty rdf:about="http://rdaregistry.info/Elements/u/P60331">
  <rdfs:isDefinedBy rdf:resource="http://rdaregistry.info/Elements/u/" />
  <reg:status rdf:resource="http://metadataregistry.org/uri/RegStatus/1001" />
  <reg:name xml:lang="en">manufactureStatement</reg:name>
  <rdfs:label xml:lang="en">has manufacture statement</rdfs:label>
  <skos:definition xml:lang="en">Relates a resource to a statement identifying a place or places of manufacture, manufacturer or manufacturers, and date or dates of manufacture of a resource in a published form.</skos:definition>
  <rdf:type rdf:resource="http://www.w3.org/1999/02/22-rdf-syntax-ns#Property" />
  <reg:hasSubproperty rdf:resource="http://rdaregistry.info/Elements/m/P30109" />
  <reg:lexicalAlias rdf:resource="http://rdaregistry.info/Elements/u/manufactureStatement.en" />
</owl:ObjectProperty>

<!-- Property: has media type -->
<owl:ObjectProperty rdf:about="http://rdaregistry.info/Elements/u/P60050">
  <rdfs:isDefinedBy rdf:resource="http://rdaregistry.info/Elements/u/" />
  <reg:status rdf:resource="http://metadataregistry.org/uri/RegStatus/1001" />
  <reg:name xml:lang="en">mediaType</reg:name>
  <rdfs:label xml:lang="en">has media type</rdfs:label>
  <skos:definition xml:lang="en">Relates a resource to a categorization reflecting a general type of intermediation device required to view, play, run, etc., the content of a resource.</skos:definition>
  <rdf:type rdf:resource="http://www.w3.org/1999/02/22-rdf-syntax-ns#Property" />
  <reg:hasSubproperty rdf:resource="http://rdaregistry.info/Elements/m/P30002" />
  <reg:lexicalAlias rdf:resource="http://rdaregistry.info/Elements/u/mediaType.en" />
</owl:ObjectProperty>

<!-- Property: has medium -->
<owl:ObjectProperty rdf:about="http://rdaregistry.info/Elements/u/P60157">
  <rdfs:isDefinedBy rdf:resource="http://rdaregistry.info/Elements/u/" />
  <reg:status rdf:resource="http://metadataregistry.org/uri/RegStatus/1001" />
  <reg:name xml:lang="en">medium</reg:name>
  <rdfs:label xml:lang="en">has medium</rdfs:label>
  <skos:definition xml:lang="en">Relates a resource to an agent held to be a channel of communication between the earthly world and a world of spirits.</skos:definition>
  <rdf:type rdf:resource="http://www.w3.org/1999/02/22-rdf-syntax-ns#Property" />
  <rdfs:subPropertyOf rdf:resource="http://rdaregistry.info/Elements/u/P60374" />
  <owl:inverseOf rdf:resource="http://rdaregistry.info/Elements/u/P60032" />
  <reg:lexicalAlias rdf:resource="http://rdaregistry.info/Elements/u/medium.en" />
</owl:ObjectProperty>

<!-- Property: is medium of -->
<owl:ObjectProperty rdf:about="http://rdaregistry.info/Elements/u/P60032">
  <rdfs:isDefinedBy rdf:resource="http://rdaregistry.info/Elements/u/" />
  <reg:status rdf:resource="http://metadataregistry.org/uri/RegStatus/1001" />
  <reg:name xml:lang="en">mediumOf</reg:name>
  <rdfs:label xml:lang="en">is medium of</rdfs:label>
  <skos:definition xml:lang="en">Relates an agent held to be a channel of communication between the earthly world and a world of spirits to a resource.</skos:definition>
  <rdf:type rdf:resource="http://www.w3.org/1999/02/22-rdf-syntax-ns#Property" />
  <rdfs:subPropertyOf rdf:resource="http://rdaregistry.info/Elements/u/P60602" />
  <owl:inverseOf rdf:resource="http://rdaregistry.info/Elements/u/P60157" />
  <reg:hasSubproperty rdf:resource="http://rdaregistry.info/Elements/a/P50086" />
  <reg:lexicalAlias rdf:resource="http://rdaregistry.info/Elements/u/mediumOf.en" />
</owl:ObjectProperty>

<!-- Property: has medium of performance -->
<owl:ObjectProperty rdf:about="http://rdaregistry.info/Elements/u/P60536">
  <rdfs:isDefinedBy rdf:resource="http://rdaregistry.info/Elements/u/" />
  <reg:status rdf:resource="http://metadataregistry.org/uri/RegStatus/1001" />
  <reg:name xml:lang="en">mediumOfPerformance</reg:name>
  <rdfs:label xml:lang="en">has medium of performance</rdfs:label>
  <skos:definition xml:lang="en">Relates a resource to an instrument, voice, or ensemble for which a musical resource was originally conceived.</skos:definition>
  <rdf:type rdf:resource="http://www.w3.org/1999/02/22-rdf-syntax-ns#Property" />
  <reg:lexicalAlias rdf:resource="http://rdaregistry.info/Elements/u/mediumOfPerformance.en" />
</owl:ObjectProperty>

<!-- Property: has medium of performance of musical content -->
<owl:ObjectProperty rdf:about="http://rdaregistry.info/Elements/u/P60537">
  <rdfs:isDefinedBy rdf:resource="http://rdaregistry.info/Elements/u/" />
  <reg:status rdf:resource="http://metadataregistry.org/uri/RegStatus/1001" />
  <reg:name xml:lang="en">mediumOfPerformanceOfMusicalContent</reg:name>
  <rdfs:label xml:lang="en">has medium of performance of musical content</rdfs:label>
  <skos:definition xml:lang="en">Relates a resource to an instrument, voice, or ensemble used, or intended to be used, for performance of musical content.</skos:definition>
  <rdf:type rdf:resource="http://www.w3.org/1999/02/22-rdf-syntax-ns#Property" />
  <reg:hasSubproperty rdf:resource="http://rdaregistry.info/Elements/e/P20215" />
  <reg:lexicalAlias rdf:resource="http://rdaregistry.info/Elements/u/mediumOfPerformanceOfMusicalContent.en" />
</owl:ObjectProperty>

<!-- Property: has member -->
<owl:ObjectProperty rdf:about="http://rdaregistry.info/Elements/u/P60697">
  <rdfs:isDefinedBy rdf:resource="http://rdaregistry.info/Elements/u/" />
  <reg:status rdf:resource="http://metadataregistry.org/uri/RegStatus/1001" />
  <reg:name xml:lang="en">member</reg:name>
  <rdfs:label xml:lang="en">has member</rdfs:label>
  <skos:definition xml:lang="en">Relates an agent who is a member of an agent to an agent.</skos:definition>
  <rdf:type rdf:resource="http://www.w3.org/1999/02/22-rdf-syntax-ns#Property" />
  <owl:inverseOf rdf:resource="http://rdaregistry.info/Elements/u/P60648" />
  <reg:hasSubproperty rdf:resource="http://rdaregistry.info/Elements/a/P50030" />
  <reg:hasSubproperty rdf:resource="http://rdaregistry.info/Elements/a/P50231" />
  <reg:hasSubproperty rdf:resource="http://rdaregistry.info/Elements/a/P50233" />
  <reg:lexicalAlias rdf:resource="http://rdaregistry.info/Elements/u/member.en" />
</owl:ObjectProperty>

<!-- Property: has member of -->
<owl:ObjectProperty rdf:about="http://rdaregistry.info/Elements/u/P60648">
  <rdfs:isDefinedBy rdf:resource="http://rdaregistry.info/Elements/u/" />
  <reg:status rdf:resource="http://metadataregistry.org/uri/RegStatus/1001" />
  <reg:name xml:lang="en">memberOf</reg:name>
  <rdfs:label xml:lang="en">has member of</rdfs:label>
  <skos:definition xml:lang="en">Relates an agent of which an agent is a member to an agent.</skos:definition>
  <rdf:type rdf:resource="http://www.w3.org/1999/02/22-rdf-syntax-ns#Property" />
  <owl:inverseOf rdf:resource="http://rdaregistry.info/Elements/u/P60697" />
  <reg:hasSubproperty rdf:resource="http://rdaregistry.info/Elements/a/P50056" />
  <reg:hasSubproperty rdf:resource="http://rdaregistry.info/Elements/a/P50095" />
  <reg:hasSubproperty rdf:resource="http://rdaregistry.info/Elements/a/P50230" />
  <reg:lexicalAlias rdf:resource="http://rdaregistry.info/Elements/u/memberOf.en" />
</owl:ObjectProperty>

<!-- Property: is merged to form -->
<owl:ObjectProperty rdf:about="http://rdaregistry.info/Elements/u/P60504">
  <rdfs:isDefinedBy rdf:resource="http://rdaregistry.info/Elements/u/" />
  <reg:status rdf:resource="http://metadataregistry.org/uri/RegStatus/1001" />
  <reg:name xml:lang="en">mergedToForm</reg:name>
  <rdfs:label xml:lang="en">is merged to form</rdfs:label>
  <skos:definition xml:lang="en">Relates a resource to a resource formed from a coming together of two or more resources.</skos:definition>
  <rdf:type rdf:resource="http://www.w3.org/1999/02/22-rdf-syntax-ns#Property" />
  <rdfs:subPropertyOf rdf:resource="http://rdaregistry.info/Elements/u/P60278" />
  <owl:inverseOf rdf:resource="http://rdaregistry.info/Elements/u/P60505" />
  <reg:hasSubproperty rdf:resource="http://rdaregistry.info/Elements/e/P20212" />
  <reg:lexicalAlias rdf:resource="http://rdaregistry.info/Elements/u/mergedToForm.en" />
</owl:ObjectProperty>

<!-- Property: has mergee -->
<owl:ObjectProperty rdf:about="http://rdaregistry.info/Elements/u/P60682">
  <rdfs:isDefinedBy rdf:resource="http://rdaregistry.info/Elements/u/" />
  <reg:status rdf:resource="http://metadataregistry.org/uri/RegStatus/1001" />
  <reg:name xml:lang="en">mergee</reg:name>
  <rdfs:label xml:lang="en">has mergee</rdfs:label>
  <skos:definition xml:lang="en">Relates a agent that merged with another agent to form a third to an agent.</skos:definition>
  <rdf:type rdf:resource="http://www.w3.org/1999/02/22-rdf-syntax-ns#Property" />
  <owl:inverseOf rdf:resource="http://rdaregistry.info/Elements/u/P60682" />
  <reg:hasSubproperty rdf:resource="http://rdaregistry.info/Elements/a/P50011" />
  <reg:lexicalAlias rdf:resource="http://rdaregistry.info/Elements/u/mergee.en" />
</owl:ObjectProperty>

<!-- Property: is merger of -->
<owl:ObjectProperty rdf:about="http://rdaregistry.info/Elements/u/P60505">
  <rdfs:isDefinedBy rdf:resource="http://rdaregistry.info/Elements/u/" />
  <reg:status rdf:resource="http://metadataregistry.org/uri/RegStatus/1001" />
  <reg:name xml:lang="en">mergerOf</reg:name>
  <rdfs:label xml:lang="en">is merger of</rdfs:label>
  <skos:definition xml:lang="en">Relates a resource to a resource that came together with one or more other resources to form a new resource.</skos:definition>
  <rdf:type rdf:resource="http://www.w3.org/1999/02/22-rdf-syntax-ns#Property" />
  <rdfs:subPropertyOf rdf:resource="http://rdaregistry.info/Elements/u/P60261" />
  <owl:inverseOf rdf:resource="http://rdaregistry.info/Elements/u/P60504" />
  <reg:hasSubproperty rdf:resource="http://rdaregistry.info/Elements/e/P20201" />
  <reg:lexicalAlias rdf:resource="http://rdaregistry.info/Elements/u/mergerOf.en" />
</owl:ObjectProperty>

<!-- Property: has minute taker -->
<owl:ObjectProperty rdf:about="http://rdaregistry.info/Elements/u/P60446">
  <rdfs:isDefinedBy rdf:resource="http://rdaregistry.info/Elements/u/" />
  <reg:status rdf:resource="http://metadataregistry.org/uri/RegStatus/1001" />
  <reg:name xml:lang="en">minuteTaker</reg:name>
  <rdfs:label xml:lang="en">has minute taker</rdfs:label>
  <skos:definition xml:lang="en">Relates a resource to an agent responsible for recording the minutes of a meeting.</skos:definition>
  <rdf:type rdf:resource="http://www.w3.org/1999/02/22-rdf-syntax-ns#Property" />
  <rdfs:subPropertyOf rdf:resource="http://rdaregistry.info/Elements/u/P60398" />
  <owl:inverseOf rdf:resource="http://rdaregistry.info/Elements/u/P60671" />
  <reg:hasSubproperty rdf:resource="http://rdaregistry.info/Elements/e/P20058" />
  <reg:lexicalAlias rdf:resource="http://rdaregistry.info/Elements/u/minuteTaker.en" />
</owl:ObjectProperty>

<!-- Property: is minute taker of -->
<owl:ObjectProperty rdf:about="http://rdaregistry.info/Elements/u/P60671">
  <rdfs:isDefinedBy rdf:resource="http://rdaregistry.info/Elements/u/" />
  <reg:status rdf:resource="http://metadataregistry.org/uri/RegStatus/1001" />
  <reg:name xml:lang="en">minuteTakerOf</reg:name>
  <rdfs:label xml:lang="en">is minute taker of</rdfs:label>
  <skos:definition xml:lang="en">Relates an agent responsible for recording the minutes of a meeting to a resource.</skos:definition>
  <rdf:type rdf:resource="http://www.w3.org/1999/02/22-rdf-syntax-ns#Property" />
  <rdfs:subPropertyOf rdf:resource="http://rdaregistry.info/Elements/u/P60626" />
  <owl:inverseOf rdf:resource="http://rdaregistry.info/Elements/u/P60446" />
  <reg:hasSubproperty rdf:resource="http://rdaregistry.info/Elements/a/P50212" />
  <reg:lexicalAlias rdf:resource="http://rdaregistry.info/Elements/u/minuteTakerOf.en" />
</owl:ObjectProperty>

<!-- Property: is mirror site -->
<owl:ObjectProperty rdf:about="http://rdaregistry.info/Elements/u/P60197">
  <rdfs:isDefinedBy rdf:resource="http://rdaregistry.info/Elements/u/" />
  <reg:status rdf:resource="http://metadataregistry.org/uri/RegStatus/1001" />
  <reg:name xml:lang="en">mirrorSite</reg:name>
  <rdfs:label xml:lang="en">is mirror site</rdfs:label>
  <skos:definition xml:lang="en">Relates a resource to a resource that is an exact copy of a website, used to reduce network traffic or improve the availability of the content of the original site.</skos:definition>
  <rdf:type rdf:resource="http://www.w3.org/1999/02/22-rdf-syntax-ns#Property" />
  <rdfs:subPropertyOf rdf:resource="http://rdaregistry.info/Elements/u/P60191" />
  <owl:inverseOf rdf:resource="http://rdaregistry.info/Elements/u/P60197" />
  <reg:hasSubproperty rdf:resource="http://rdaregistry.info/Elements/m/P30028" />
  <reg:lexicalAlias rdf:resource="http://rdaregistry.info/Elements/u/mirrorSite.en" />
</owl:ObjectProperty>

<!-- Property: has mixing engineer -->
<owl:ObjectProperty rdf:about="http://rdaregistry.info/Elements/u/P60893">
  <rdfs:isDefinedBy rdf:resource="http://rdaregistry.info/Elements/u/" />
  <reg:status rdf:resource="http://metadataregistry.org/uri/RegStatus/1001" />
  <rdf:type rdf:resource="http://www.w3.org/1999/02/22-rdf-syntax-ns#Property" />
  <reg:name xml:lang="en">mixingEngineer</reg:name>
  <rdfs:label xml:lang="en">has mixing engineer</rdfs:label>
  <reg:lexicalAlias rdf:resource="http://rdaregistry.info/Elements/u/mixingEngineer.en" />
  <skos:definition xml:lang="en">Relates a resource to an audio engineer contributing to the audio content of a resource by manipulating, mixing, and assembling the multiple tracks of a recording.</skos:definition>
  <skos:scopeNote xml:lang="en">Remixing activities that substantially change the nature and content of the original resource, resulting in a new resource, are excluded.</skos:scopeNote>
  <owl:inverseOf rdf:resource="http://rdaregistry.info/Elements/u/P60885" />
  <reg:hasSubproperty rdf:resource="http://rdaregistry.info/Elements/e/P20293" />
  <rdfs:subPropertyOf rdf:resource="http://rdaregistry.info/Elements/u/P60892" />
  <rdakit:seeAlso rdf:resource="http://rdaregistry.info/Elements/u/P60891" />
</owl:ObjectProperty>

<!-- Property: is mixing engineer of -->
<owl:ObjectProperty rdf:about="http://rdaregistry.info/Elements/u/P60885">
  <rdfs:isDefinedBy rdf:resource="http://rdaregistry.info/Elements/u/" />
  <reg:status rdf:resource="http://metadataregistry.org/uri/RegStatus/1001" />
  <rdf:type rdf:resource="http://www.w3.org/1999/02/22-rdf-syntax-ns#Property" />
  <reg:name xml:lang="en">mixingEngineerOf</reg:name>
  <rdfs:label xml:lang="en">is mixing engineer of</rdfs:label>
  <reg:lexicalAlias rdf:resource="http://rdaregistry.info/Elements/u/mixingEngineerOf.en" />
  <skos:definition xml:lang="en">Relates an agent to a resource that incorporates a contribution to the audio content of manipulating, mixing and assembling the multiple tracks of a recording.</skos:definition>
  <skos:scopeNote xml:lang="en">Remixing activities that substantially change the nature and content of the original resource, resulting in a new resource, are excluded.</skos:scopeNote>
  <owl:inverseOf rdf:resource="http://rdaregistry.info/Elements/u/P60893" />
  <rdfs:subPropertyOf rdf:resource="http://rdaregistry.info/Elements/u/P60884" />
  <reg:hasSubproperty rdf:resource="http://rdaregistry.info/Elements/a/P50297" />
  <rdakit:seeAlso rdf:resource="http://rdaregistry.info/Elements/u/P60881" />
</owl:ObjectProperty>

<!-- Property: has mode of issuance -->
<owl:ObjectProperty rdf:about="http://rdaregistry.info/Elements/u/P60051">
  <rdfs:isDefinedBy rdf:resource="http://rdaregistry.info/Elements/u/" />
  <reg:status rdf:resource="http://metadataregistry.org/uri/RegStatus/1001" />
  <reg:name xml:lang="en">modeOfIssuance</reg:name>
  <rdfs:label xml:lang="en">has mode of issuance</rdfs:label>
  <skos:definition xml:lang="en">Relates a resource to a categorization reflecting whether a resource is issued in one or more parts, the way it is updated, and its intended termination.</skos:definition>
  <rdf:type rdf:resource="http://www.w3.org/1999/02/22-rdf-syntax-ns#Property" />
  <reg:hasSubproperty rdf:resource="http://rdaregistry.info/Elements/m/P30003" />
  <reg:lexicalAlias rdf:resource="http://rdaregistry.info/Elements/u/modeOfIssuance.en" />
</owl:ObjectProperty>

<!-- Property: has moderator -->
<owl:ObjectProperty rdf:about="http://rdaregistry.info/Elements/u/P60147">
  <rdfs:isDefinedBy rdf:resource="http://rdaregistry.info/Elements/u/" />
  <reg:status rdf:resource="http://metadataregistry.org/uri/RegStatus/1001" />
  <reg:name xml:lang="en">moderator</reg:name>
  <rdfs:label xml:lang="en">has moderator</rdfs:label>
  <skos:definition xml:lang="en">Relates a resource to a performer contributing to a resource by leading a program, often broadcast, where topics are discussed, usually with participation of experts in fields related to the discussion.</skos:definition>
  <rdf:type rdf:resource="http://www.w3.org/1999/02/22-rdf-syntax-ns#Property" />
  <rdfs:subPropertyOf rdf:resource="http://rdaregistry.info/Elements/u/P60387" />
  <owl:inverseOf rdf:resource="http://rdaregistry.info/Elements/u/P60022" />
  <reg:hasSubproperty rdf:resource="http://rdaregistry.info/Elements/e/P20017" />
  <reg:lexicalAlias rdf:resource="http://rdaregistry.info/Elements/u/moderator.en" />
</owl:ObjectProperty>

<!-- Property: is moderator of -->
<owl:ObjectProperty rdf:about="http://rdaregistry.info/Elements/u/P60022">
  <rdfs:isDefinedBy rdf:resource="http://rdaregistry.info/Elements/u/" />
  <reg:status rdf:resource="http://metadataregistry.org/uri/RegStatus/1001" />
  <reg:name xml:lang="en">moderatorOf</reg:name>
  <rdfs:label xml:lang="en">is moderator of</rdfs:label>
  <skos:definition xml:lang="en">Relates a performer contributing to a resource by leading a program, often broadcast, where topics are discussed, usually with participation of experts in fields related to the discussion to a resource.</skos:definition>
  <rdf:type rdf:resource="http://www.w3.org/1999/02/22-rdf-syntax-ns#Property" />
  <rdfs:subPropertyOf rdf:resource="http://rdaregistry.info/Elements/u/P60615" />
  <owl:inverseOf rdf:resource="http://rdaregistry.info/Elements/u/P60147" />
  <reg:hasSubproperty rdf:resource="http://rdaregistry.info/Elements/a/P50076" />
  <reg:lexicalAlias rdf:resource="http://rdaregistry.info/Elements/u/moderatorOf.en" />
</owl:ObjectProperty>

<!-- Property: is modified by variation as -->
<owl:ObjectProperty rdf:about="http://rdaregistry.info/Elements/u/P60115">
  <rdfs:isDefinedBy rdf:resource="http://rdaregistry.info/Elements/u/" />
  <reg:status rdf:resource="http://metadataregistry.org/uri/RegStatus/1001" />
  <reg:name xml:lang="en">modifiedByVariationAs</reg:name>
  <rdfs:label xml:lang="en">is modified by variation as</rdfs:label>
  <skos:definition xml:lang="en">Relates a resource to a musical resource in which melodic, thematic, or harmonic material taken from a source resource forms a discrete theme, which is repeated one or more times with subsequent modifications.</skos:definition>
  <rdf:type rdf:resource="http://www.w3.org/1999/02/22-rdf-syntax-ns#Property" />
  <rdfs:subPropertyOf rdf:resource="http://rdaregistry.info/Elements/u/P60250" />
  <owl:inverseOf rdf:resource="http://rdaregistry.info/Elements/u/P60114" />
  <reg:hasSubproperty rdf:resource="http://rdaregistry.info/Elements/e/P20082" />
  <reg:lexicalAlias rdf:resource="http://rdaregistry.info/Elements/u/modifiedByVariationAs.en" />
</owl:ObjectProperty>

<!-- Property: is motion picture adaptation of -->
<owl:ObjectProperty rdf:about="http://rdaregistry.info/Elements/u/P60227">
  <rdfs:isDefinedBy rdf:resource="http://rdaregistry.info/Elements/u/" />
  <reg:status rdf:resource="http://metadataregistry.org/uri/RegStatus/1001" />
  <reg:name xml:lang="en">motionPictureAdaptationOf</reg:name>
  <rdfs:label xml:lang="en">is motion picture adaptation of</rdfs:label>
  <skos:definition xml:lang="en">Relates a resource to a resource that has been adapted as a motion picture.</skos:definition>
  <rdf:type rdf:resource="http://www.w3.org/1999/02/22-rdf-syntax-ns#Property" />
  <rdfs:subPropertyOf rdf:resource="http://rdaregistry.info/Elements/u/P60241" />
  <owl:inverseOf rdf:resource="http://rdaregistry.info/Elements/u/P60110" />
  <reg:hasSubproperty rdf:resource="http://rdaregistry.info/Elements/e/P20125" />
  <reg:lexicalAlias rdf:resource="http://rdaregistry.info/Elements/u/motionPictureAdaptationOf.en" />
</owl:ObjectProperty>

<!-- Property: is motion picture music -->
<owl:ObjectProperty rdf:about="http://rdaregistry.info/Elements/u/P60732">
  <rdfs:isDefinedBy rdf:resource="http://rdaregistry.info/Elements/u/" />
  <reg:status rdf:resource="http://metadataregistry.org/uri/RegStatus/1001" />
  <reg:name xml:lang="en">motionPictureMusic</reg:name>
  <rdfs:label xml:lang="en">is motion picture music</rdfs:label>
  <skos:definition xml:lang="en">Relates a resource to a musical resource that is used in a motion picture.</skos:definition>
  <rdf:type rdf:resource="http://www.w3.org/1999/02/22-rdf-syntax-ns#Property" />
  <rdfs:subPropertyOf rdf:resource="http://rdaregistry.info/Elements/u/P60724" />
  <owl:inverseOf rdf:resource="http://rdaregistry.info/Elements/u/P60731" />
  <reg:hasSubproperty rdf:resource="http://rdaregistry.info/Elements/e/P20252" />
  <reg:lexicalAlias rdf:resource="http://rdaregistry.info/Elements/u/motionPictureMusic.en" />
</owl:ObjectProperty>

<!-- Property: is motion picture screenplay -->
<owl:ObjectProperty rdf:about="http://rdaregistry.info/Elements/u/P60265">
  <rdfs:isDefinedBy rdf:resource="http://rdaregistry.info/Elements/u/" />
  <reg:status rdf:resource="http://metadataregistry.org/uri/RegStatus/1001" />
  <reg:name xml:lang="en">motionPictureScreenplay</reg:name>
  <rdfs:label xml:lang="en">is motion picture screenplay</rdfs:label>
  <skos:definition xml:lang="en">Relates a resource to a resource that provides text for a motion picture.</skos:definition>
  <rdf:type rdf:resource="http://www.w3.org/1999/02/22-rdf-syntax-ns#Property" />
  <rdfs:subPropertyOf rdf:resource="http://rdaregistry.info/Elements/u/P60264" />
  <owl:inverseOf rdf:resource="http://rdaregistry.info/Elements/u/P60282" />
  <reg:hasSubproperty rdf:resource="http://rdaregistry.info/Elements/e/P20158" />
  <reg:lexicalAlias rdf:resource="http://rdaregistry.info/Elements/u/motionPictureScreenplay.en" />
</owl:ObjectProperty>

<!-- Property: is motion picture screenplay based on -->
<owl:ObjectProperty rdf:about="http://rdaregistry.info/Elements/u/P60232">
  <rdfs:isDefinedBy rdf:resource="http://rdaregistry.info/Elements/u/" />
  <reg:status rdf:resource="http://metadataregistry.org/uri/RegStatus/1001" />
  <reg:name xml:lang="en">motionPictureScreenplayBasedOn</reg:name>
  <rdfs:label xml:lang="en">is motion picture screenplay based on</rdfs:label>
  <skos:definition xml:lang="en">Relates a resource to a resource that has been adapted as a screenplay for a motion picture.</skos:definition>
  <rdf:type rdf:resource="http://www.w3.org/1999/02/22-rdf-syntax-ns#Property" />
  <rdfs:subPropertyOf rdf:resource="http://rdaregistry.info/Elements/u/P60231" />
  <owl:inverseOf rdf:resource="http://rdaregistry.info/Elements/u/P60184" />
  <reg:hasSubproperty rdf:resource="http://rdaregistry.info/Elements/e/P20130" />
  <reg:lexicalAlias rdf:resource="http://rdaregistry.info/Elements/u/motionPictureScreenplayBasedOn.en" />
</owl:ObjectProperty>

<!-- Property: has mount -->
<owl:ObjectProperty rdf:about="http://rdaregistry.info/Elements/u/P60554">
  <rdfs:isDefinedBy rdf:resource="http://rdaregistry.info/Elements/u/" />
  <reg:status rdf:resource="http://metadataregistry.org/uri/RegStatus/1001" />
  <reg:name xml:lang="en">mount</reg:name>
  <rdfs:label xml:lang="en">has mount</rdfs:label>
  <skos:definition xml:lang="en">Relates a resource to a physical material used for the support or backing to which the base material of a resource has been attached.</skos:definition>
  <rdf:type rdf:resource="http://www.w3.org/1999/02/22-rdf-syntax-ns#Property" />
  <reg:hasSubproperty rdf:resource="http://rdaregistry.info/Elements/m/P30186" />
  <reg:lexicalAlias rdf:resource="http://rdaregistry.info/Elements/u/mount.en" />
</owl:ObjectProperty>

<!-- Property: is music -->
<owl:ObjectProperty rdf:about="http://rdaregistry.info/Elements/u/P60723">
  <rdfs:isDefinedBy rdf:resource="http://rdaregistry.info/Elements/u/" />
  <reg:status rdf:resource="http://metadataregistry.org/uri/RegStatus/1001" />
  <reg:name xml:lang="en">music</reg:name>
  <rdfs:label xml:lang="en">is music</rdfs:label>
  <skos:definition xml:lang="en">Relates a resource to a musical resource that is used in a motion picture, play, television program, etc.</skos:definition>
  <rdf:type rdf:resource="http://www.w3.org/1999/02/22-rdf-syntax-ns#Property" />
  <rdfs:subPropertyOf rdf:resource="http://rdaregistry.info/Elements/u/P60198" />
  <owl:inverseOf rdf:resource="http://rdaregistry.info/Elements/u/P60724" />
  <reg:hasSubproperty rdf:resource="http://rdaregistry.info/Elements/e/P20243" />
  <reg:hasSubproperty rdf:resource="http://rdaregistry.info/Elements/w/P10237" />
  <reg:lexicalAlias rdf:resource="http://rdaregistry.info/Elements/u/music.en" />
  <reg:hasSubproperty rdf:resource="http://rdaregistry.info/Elements/u/P60118" />
</owl:ObjectProperty>

<!-- Property: has musical director -->
<owl:ObjectProperty rdf:about="http://rdaregistry.info/Elements/u/P60383">
  <rdfs:isDefinedBy rdf:resource="http://rdaregistry.info/Elements/u/" />
  <reg:status rdf:resource="http://metadataregistry.org/uri/RegStatus/1001" />
  <reg:name xml:lang="en">musicalDirector</reg:name>
  <rdfs:label xml:lang="en">has musical director</rdfs:label>
  <skos:definition xml:lang="en">Relates a resource to an agent contributing to a resource by coordinating the activities of composers, sound editors, and sound mixers for a moving image production or for a musical or dramatic presentation or entertainment.</skos:definition>
  <rdf:type rdf:resource="http://www.w3.org/1999/02/22-rdf-syntax-ns#Property" />
  <rdfs:subPropertyOf rdf:resource="http://rdaregistry.info/Elements/u/P60398" />
  <owl:inverseOf rdf:resource="http://rdaregistry.info/Elements/u/P60611" />
  <reg:hasSubproperty rdf:resource="http://rdaregistry.info/Elements/e/P20035" />
  <reg:lexicalAlias rdf:resource="http://rdaregistry.info/Elements/u/musicalDirector.en" />
</owl:ObjectProperty>

<!-- Property: is musical director of -->
<owl:ObjectProperty rdf:about="http://rdaregistry.info/Elements/u/P60611">
  <rdfs:isDefinedBy rdf:resource="http://rdaregistry.info/Elements/u/" />
  <reg:status rdf:resource="http://metadataregistry.org/uri/RegStatus/1001" />
  <reg:name xml:lang="en">musicalDirectorOf</reg:name>
  <rdfs:label xml:lang="en">is musical director of</rdfs:label>
  <skos:definition xml:lang="en">Relates an agent contributing to a resource by coordinating the activities of composers, sound editors, and sound mixers for a moving image production or for a musical or dramatic presentation or entertainment to a resource.</skos:definition>
  <rdf:type rdf:resource="http://www.w3.org/1999/02/22-rdf-syntax-ns#Property" />
  <rdfs:subPropertyOf rdf:resource="http://rdaregistry.info/Elements/u/P60626" />
  <owl:inverseOf rdf:resource="http://rdaregistry.info/Elements/u/P60383" />
  <reg:hasSubproperty rdf:resource="http://rdaregistry.info/Elements/a/P50143" />
  <reg:lexicalAlias rdf:resource="http://rdaregistry.info/Elements/u/musicalDirectorOf.en" />
</owl:ObjectProperty>

<!-- Property: is musical setting of -->
<owl:ObjectProperty rdf:about="http://rdaregistry.info/Elements/u/P60266">
  <rdfs:isDefinedBy rdf:resource="http://rdaregistry.info/Elements/u/" />
  <reg:status rdf:resource="http://metadataregistry.org/uri/RegStatus/1001" />
  <reg:name xml:lang="en">musicalSettingOf</reg:name>
  <rdfs:label xml:lang="en">is musical setting of</rdfs:label>
  <skos:definition xml:lang="en">Relates a resource to a resource that provides text for a non-dramatic musical resource, other than an oratorio.</skos:definition>
  <rdf:type rdf:resource="http://www.w3.org/1999/02/22-rdf-syntax-ns#Property" />
  <rdfs:subPropertyOf rdf:resource="http://rdaregistry.info/Elements/u/P60305" />
  <owl:inverseOf rdf:resource="http://rdaregistry.info/Elements/u/P60121" />
  <reg:hasSubproperty rdf:resource="http://rdaregistry.info/Elements/e/P20159" />
  <reg:lexicalAlias rdf:resource="http://rdaregistry.info/Elements/u/musicalSettingOf.en" />
</owl:ObjectProperty>

<!-- Property: is musical theatre adaptation of -->
<owl:ObjectProperty rdf:about="http://rdaregistry.info/Elements/u/P60719">
  <rdfs:isDefinedBy rdf:resource="http://rdaregistry.info/Elements/u/" />
  <reg:status rdf:resource="http://metadataregistry.org/uri/RegStatus/1001" />
  <reg:name xml:lang="en">musicalTheatreAdaptationOf</reg:name>
  <rdfs:label xml:lang="en">is musical theatre adaptation of</rdfs:label>
  <skos:definition xml:lang="en">Relates a resource to a resource that has been adapted as a musical theatre resource.</skos:definition>
  <rdf:type rdf:resource="http://www.w3.org/1999/02/22-rdf-syntax-ns#Property" />
  <rdfs:subPropertyOf rdf:resource="http://rdaregistry.info/Elements/u/P60241" />
  <owl:inverseOf rdf:resource="http://rdaregistry.info/Elements/u/P60721" />
  <reg:hasSubproperty rdf:resource="http://rdaregistry.info/Elements/e/P20239" />
  <reg:lexicalAlias rdf:resource="http://rdaregistry.info/Elements/u/musicalTheatreAdaptationOf.en" />
</owl:ObjectProperty>

<!-- Property: is music for -->
<owl:ObjectProperty rdf:about="http://rdaregistry.info/Elements/u/P60724">
  <rdfs:isDefinedBy rdf:resource="http://rdaregistry.info/Elements/u/" />
  <reg:status rdf:resource="http://metadataregistry.org/uri/RegStatus/1001" />
  <reg:name xml:lang="en">musicFor</reg:name>
  <rdfs:label xml:lang="en">is music for</rdfs:label>
  <skos:definition xml:lang="en">Relates a resource to a resource such as a motion picture, play, television program, etc., that uses a musical resource.</skos:definition>
  <rdf:type rdf:resource="http://www.w3.org/1999/02/22-rdf-syntax-ns#Property" />
  <rdfs:subPropertyOf rdf:resource="http://rdaregistry.info/Elements/u/P60198" />
  <owl:inverseOf rdf:resource="http://rdaregistry.info/Elements/u/P60723" />
  <reg:hasSubproperty rdf:resource="http://rdaregistry.info/Elements/e/P20244" />
  <reg:hasSubproperty rdf:resource="http://rdaregistry.info/Elements/w/P10238" />
  <reg:lexicalAlias rdf:resource="http://rdaregistry.info/Elements/u/musicFor.en" />
  <reg:hasSubproperty rdf:resource="http://rdaregistry.info/Elements/u/P60202" />
</owl:ObjectProperty>

<!-- Property: is music for motion picture -->
<owl:ObjectProperty rdf:about="http://rdaregistry.info/Elements/u/P60731">
  <rdfs:isDefinedBy rdf:resource="http://rdaregistry.info/Elements/u/" />
  <reg:status rdf:resource="http://metadataregistry.org/uri/RegStatus/1001" />
  <reg:name xml:lang="en">musicForMotionPicture</reg:name>
  <rdfs:label xml:lang="en">is music for motion picture</rdfs:label>
  <skos:definition xml:lang="en">Relates a resource to a resource that uses a musical resource in a motion picture.</skos:definition>
  <rdf:type rdf:resource="http://www.w3.org/1999/02/22-rdf-syntax-ns#Property" />
  <rdfs:subPropertyOf rdf:resource="http://rdaregistry.info/Elements/u/P60723" />
  <owl:inverseOf rdf:resource="http://rdaregistry.info/Elements/u/P60732" />
  <reg:hasSubproperty rdf:resource="http://rdaregistry.info/Elements/e/P20251" />
  <reg:lexicalAlias rdf:resource="http://rdaregistry.info/Elements/u/musicForMotionPicture.en" />
</owl:ObjectProperty>

<!-- Property: is music for radio program -->
<owl:ObjectProperty rdf:about="http://rdaregistry.info/Elements/u/P60730">
  <rdfs:isDefinedBy rdf:resource="http://rdaregistry.info/Elements/u/" />
  <reg:status rdf:resource="http://metadataregistry.org/uri/RegStatus/1001" />
  <reg:name xml:lang="en">musicForRadioProgram</reg:name>
  <rdfs:label xml:lang="en">is music for radio program</rdfs:label>
  <skos:definition xml:lang="en">Relates a resource to a resource that uses a musical resource in a radio program.</skos:definition>
  <rdf:type rdf:resource="http://www.w3.org/1999/02/22-rdf-syntax-ns#Property" />
  <rdfs:subPropertyOf rdf:resource="http://rdaregistry.info/Elements/u/P60724" />
  <owl:inverseOf rdf:resource="http://rdaregistry.info/Elements/u/P60729" />
  <reg:hasSubproperty rdf:resource="http://rdaregistry.info/Elements/e/P20250" />
  <reg:lexicalAlias rdf:resource="http://rdaregistry.info/Elements/u/musicForRadioProgram.en" />
</owl:ObjectProperty>

<!-- Property: is music for television program -->
<owl:ObjectProperty rdf:about="http://rdaregistry.info/Elements/u/P60728">
  <rdfs:isDefinedBy rdf:resource="http://rdaregistry.info/Elements/u/" />
  <reg:status rdf:resource="http://metadataregistry.org/uri/RegStatus/1001" />
  <reg:name xml:lang="en">musicForTelevisionProgram</reg:name>
  <rdfs:label xml:lang="en">is music for television program</rdfs:label>
  <skos:definition xml:lang="en">Relates a resource to a resource that uses a musical resource in a television program.</skos:definition>
  <rdf:type rdf:resource="http://www.w3.org/1999/02/22-rdf-syntax-ns#Property" />
  <rdfs:subPropertyOf rdf:resource="http://rdaregistry.info/Elements/u/P60724" />
  <owl:inverseOf rdf:resource="http://rdaregistry.info/Elements/u/P60727" />
  <reg:hasSubproperty rdf:resource="http://rdaregistry.info/Elements/e/P20248" />
  <reg:lexicalAlias rdf:resource="http://rdaregistry.info/Elements/u/musicForTelevisionProgram.en" />
</owl:ObjectProperty>

<!-- Property: is music for video -->
<owl:ObjectProperty rdf:about="http://rdaregistry.info/Elements/u/P60726">
  <rdfs:isDefinedBy rdf:resource="http://rdaregistry.info/Elements/u/" />
  <reg:status rdf:resource="http://metadataregistry.org/uri/RegStatus/1001" />
  <reg:name xml:lang="en">musicForVideo</reg:name>
  <rdfs:label xml:lang="en">is music for video</rdfs:label>
  <skos:definition xml:lang="en">Relates a resource to a resource that uses a musical resource in a video.</skos:definition>
  <rdf:type rdf:resource="http://www.w3.org/1999/02/22-rdf-syntax-ns#Property" />
  <rdfs:subPropertyOf rdf:resource="http://rdaregistry.info/Elements/u/P60724" />
  <owl:inverseOf rdf:resource="http://rdaregistry.info/Elements/u/P60725" />
  <reg:hasSubproperty rdf:resource="http://rdaregistry.info/Elements/e/P20246" />
  <reg:lexicalAlias rdf:resource="http://rdaregistry.info/Elements/u/musicForVideo.en" />
</owl:ObjectProperty>

<!-- Property: has music programmer -->
<owl:ObjectProperty rdf:about="http://rdaregistry.info/Elements/u/P60894">
  <rdfs:isDefinedBy rdf:resource="http://rdaregistry.info/Elements/u/" />
  <reg:status rdf:resource="http://metadataregistry.org/uri/RegStatus/1001" />
  <rdf:type rdf:resource="http://www.w3.org/1999/02/22-rdf-syntax-ns#Property" />
  <reg:name xml:lang="en">musicProgrammer</reg:name>
  <rdfs:label xml:lang="en">has music programmer</rdfs:label>
  <reg:lexicalAlias rdf:resource="http://rdaregistry.info/Elements/u/musicProgrammer.en" />
  <skos:definition xml:lang="en">Relates a resource to an agent contributing to a musical resource by using electronic audio devices or computer software to generate sounds.</skos:definition>
  <skos:scopeNote xml:lang="en">The creation of a new musical resource is excluded.</skos:scopeNote>
  <owl:inverseOf rdf:resource="http://rdaregistry.info/Elements/u/P60888" />
  <reg:hasSubproperty rdf:resource="http://rdaregistry.info/Elements/e/P20294" />
  <rdfs:subPropertyOf rdf:resource="http://rdaregistry.info/Elements/u/P60398" />
  <rdakit:seeAlso rdf:resource="http://rdaregistry.info/Elements/u/P60426" />
</owl:ObjectProperty>

<!-- Property: is music programmer of -->
<owl:ObjectProperty rdf:about="http://rdaregistry.info/Elements/u/P60888">
  <rdfs:isDefinedBy rdf:resource="http://rdaregistry.info/Elements/u/" />
  <reg:status rdf:resource="http://metadataregistry.org/uri/RegStatus/1001" />
  <rdf:type rdf:resource="http://www.w3.org/1999/02/22-rdf-syntax-ns#Property" />
  <reg:name xml:lang="en">musicProgrammerOf</reg:name>
  <rdfs:label xml:lang="en">is music programmer of</rdfs:label>
  <reg:lexicalAlias rdf:resource="http://rdaregistry.info/Elements/u/musicProgrammerOf.en" />
  <skos:definition xml:lang="en">Relates an agent to a musical resource that incorporates a contribution of using electronic audio devices or computer software to generate sounds.</skos:definition>
  <owl:inverseOf rdf:resource="http://rdaregistry.info/Elements/u/P60894" />
  <rdfs:subPropertyOf rdf:resource="http://rdaregistry.info/Elements/u/P60158" />
  <reg:hasSubproperty rdf:resource="http://rdaregistry.info/Elements/a/P50300" />
  <rdakit:seeAlso rdf:resource="http://rdaregistry.info/Elements/u/P60655" />
</owl:ObjectProperty>

<!-- Property: has name of agent -->
<owl:ObjectProperty rdf:about="http://rdaregistry.info/Elements/u/P60368">
  <rdfs:isDefinedBy rdf:resource="http://rdaregistry.info/Elements/u/" />
  <reg:status rdf:resource="http://metadataregistry.org/uri/RegStatus/1001" />
  <reg:name xml:lang="en">nameOfAgent</reg:name>
  <rdfs:label xml:lang="en">has name of agent</rdfs:label>
  <skos:definition xml:lang="en">Relates a resource to a word, character, or group of words or characters by which an agent is known.</skos:definition>
  <rdf:type rdf:resource="http://www.w3.org/1999/02/22-rdf-syntax-ns#Property" />
  <reg:hasSubproperty rdf:resource="http://rdaregistry.info/Elements/u/P60119" />
  <reg:hasSubproperty rdf:resource="http://rdaregistry.info/Elements/u/P60549" />
  <reg:hasSubproperty rdf:resource="http://rdaregistry.info/Elements/a/P50032" />
  <reg:hasSubproperty rdf:resource="http://rdaregistry.info/Elements/a/P50061" />
  <reg:hasSubproperty rdf:resource="http://rdaregistry.info/Elements/a/P50111" />
  <reg:lexicalAlias rdf:resource="http://rdaregistry.info/Elements/u/nameOfAgent.en" />
</owl:ObjectProperty>

<!-- Property: has name of place -->
<owl:ObjectProperty rdf:about="http://rdaregistry.info/Elements/u/P60366">
  <rdfs:isDefinedBy rdf:resource="http://rdaregistry.info/Elements/u/" />
  <reg:status rdf:resource="http://metadataregistry.org/uri/RegStatus/1001" />
  <reg:name xml:lang="en">nameOfPlace</reg:name>
  <rdfs:label xml:lang="en">has name of place</rdfs:label>
  <skos:definition xml:lang="en">Relates a resource to a word, character, or group of words or characters by which a place is known.</skos:definition>
  <rdf:type rdf:resource="http://www.w3.org/1999/02/22-rdf-syntax-ns#Property" />
  <reg:hasSubproperty rdf:resource="http://rdaregistry.info/Elements/u/P60548" />
  <reg:lexicalAlias rdf:resource="http://rdaregistry.info/Elements/u/nameOfPlace.en" />
  <reg:hasSubproperty rdf:resource="http://rdaregistry.info/Elements/p/P70001" />
</owl:ObjectProperty>

<!-- Property: has narrator -->
<owl:ObjectProperty rdf:about="http://rdaregistry.info/Elements/u/P60153">
  <rdfs:isDefinedBy rdf:resource="http://rdaregistry.info/Elements/u/" />
  <reg:status rdf:resource="http://metadataregistry.org/uri/RegStatus/1001" />
  <reg:name xml:lang="en">narrator</reg:name>
  <rdfs:label xml:lang="en">has narrator</rdfs:label>
  <skos:definition xml:lang="en">Relates a resource to a performer contributing to a resource by reading aloud or giving an account of an act, occurrence, course of events, etc.</skos:definition>
  <rdf:type rdf:resource="http://www.w3.org/1999/02/22-rdf-syntax-ns#Property" />
  <rdfs:subPropertyOf rdf:resource="http://rdaregistry.info/Elements/u/P60387" />
  <owl:inverseOf rdf:resource="http://rdaregistry.info/Elements/u/P60028" />
  <reg:hasSubproperty rdf:resource="http://rdaregistry.info/Elements/e/P20022" />
  <reg:lexicalAlias rdf:resource="http://rdaregistry.info/Elements/u/narrator.en" />
</owl:ObjectProperty>

<!-- Property: is narrator of -->
<owl:ObjectProperty rdf:about="http://rdaregistry.info/Elements/u/P60028">
  <rdfs:isDefinedBy rdf:resource="http://rdaregistry.info/Elements/u/" />
  <reg:status rdf:resource="http://metadataregistry.org/uri/RegStatus/1001" />
  <reg:name xml:lang="en">narratorOf</reg:name>
  <rdfs:label xml:lang="en">is narrator of</rdfs:label>
  <skos:definition xml:lang="en">Relates a performer contributing to a resource by reading aloud or giving an account of an act, occurrence, course of events, etc. to a resource.</skos:definition>
  <rdf:type rdf:resource="http://www.w3.org/1999/02/22-rdf-syntax-ns#Property" />
  <rdfs:subPropertyOf rdf:resource="http://rdaregistry.info/Elements/u/P60615" />
  <owl:inverseOf rdf:resource="http://rdaregistry.info/Elements/u/P60153" />
  <reg:hasSubproperty rdf:resource="http://rdaregistry.info/Elements/a/P50081" />
  <reg:lexicalAlias rdf:resource="http://rdaregistry.info/Elements/u/narratorOf.en" />
</owl:ObjectProperty>

<!-- Property: has nature of content -->
<owl:ObjectProperty rdf:about="http://rdaregistry.info/Elements/u/P60584">
  <rdfs:isDefinedBy rdf:resource="http://rdaregistry.info/Elements/u/" />
  <reg:status rdf:resource="http://metadataregistry.org/uri/RegStatus/1001" />
  <reg:name xml:lang="en">natureOfContent</reg:name>
  <rdfs:label xml:lang="en">has nature of content</rdfs:label>
  <skos:definition xml:lang="en">Relates a resource to a specific character of a primary content of a resource.</skos:definition>
  <rdf:type rdf:resource="http://www.w3.org/1999/02/22-rdf-syntax-ns#Property" />
  <reg:lexicalAlias rdf:resource="http://rdaregistry.info/Elements/u/natureOfContent.en" />
</owl:ObjectProperty>

<!-- Property: has note on changes in carrier characteristics -->
<owl:ObjectProperty rdf:about="http://rdaregistry.info/Elements/u/P60124">
  <rdfs:isDefinedBy rdf:resource="http://rdaregistry.info/Elements/u/" />
  <reg:status rdf:resource="http://metadataregistry.org/uri/RegStatus/1001" />
  <reg:name xml:lang="en">noteOnChangesInCarrierCharacteristics</reg:name>
  <rdfs:label xml:lang="en">has note on changes in carrier characteristics</rdfs:label>
  <skos:definition xml:lang="en">Relates a resource to a note on changes in the characteristics of a carrier that occur in subsequent issues or parts of a resource issued in successive parts or between iterations of an integrating resource.</skos:definition>
  <rdf:type rdf:resource="http://www.w3.org/1999/02/22-rdf-syntax-ns#Property" />
  <reg:hasSubproperty rdf:resource="http://rdaregistry.info/Elements/m/P30051" />
  <reg:lexicalAlias rdf:resource="http://rdaregistry.info/Elements/u/noteOnChangesInCarrierCharacteristics.en" />
  <rdfs:subPropertyOf rdf:resource="http://rdaregistry.info/Elements/u/P60470" />
</owl:ObjectProperty>

<!-- Property: has note on changes in content characteristics -->
<owl:ObjectProperty rdf:about="http://rdaregistry.info/Elements/u/P60123">
  <rdfs:isDefinedBy rdf:resource="http://rdaregistry.info/Elements/u/" />
  <reg:status rdf:resource="http://metadataregistry.org/uri/RegStatus/1001" />
  <reg:name xml:lang="en">noteOnChangesInContentCharacteristics</reg:name>
  <rdfs:label xml:lang="en">has note on changes in content characteristics</rdfs:label>
  <skos:definition xml:lang="en">Relates a resource to a note on changes in content characteristics that occur in subsequent issues or parts of a resource issued in successive parts or between iterations of an integrating resource.</skos:definition>
  <rdf:type rdf:resource="http://www.w3.org/1999/02/22-rdf-syntax-ns#Property" />
  <rdfs:subPropertyOf rdf:resource="http://rdaregistry.info/Elements/u/P60470" />
  <reg:hasSubproperty rdf:resource="http://rdaregistry.info/Elements/e/P20010" />
  <reg:lexicalAlias rdf:resource="http://rdaregistry.info/Elements/u/noteOnChangesInContentCharacteristics.en" />
</owl:ObjectProperty>

<!-- Property: has note on copyright date -->
<owl:ObjectProperty rdf:about="http://rdaregistry.info/Elements/u/P60132">
  <rdfs:isDefinedBy rdf:resource="http://rdaregistry.info/Elements/u/" />
  <reg:status rdf:resource="http://metadataregistry.org/uri/RegStatus/1001" />
  <reg:name xml:lang="en">noteOnCopyrightDate</reg:name>
  <rdfs:label xml:lang="en">has note on copyright date</rdfs:label>
  <skos:definition xml:lang="en">Relates a resource to a note providing information on copyright dates not recorded as part of a copyright date element.</skos:definition>
  <rdf:type rdf:resource="http://www.w3.org/1999/02/22-rdf-syntax-ns#Property" />
  <reg:hasSubproperty rdf:resource="http://rdaregistry.info/Elements/m/P30059" />
  <reg:lexicalAlias rdf:resource="http://rdaregistry.info/Elements/u/noteOnCopyrightDate.en" />
  <rdfs:subPropertyOf rdf:resource="http://rdaregistry.info/Elements/u/P60470" />
</owl:ObjectProperty>

<!-- Property: has note on dimensions of resource -->
<owl:ObjectProperty rdf:about="http://rdaregistry.info/Elements/u/P60133">
  <rdfs:isDefinedBy rdf:resource="http://rdaregistry.info/Elements/u/" />
  <reg:status rdf:resource="http://metadataregistry.org/uri/RegStatus/1001" />
  <reg:name xml:lang="en">noteOnDimensionsOfResource</reg:name>
  <rdfs:label xml:lang="en">has note on dimensions of resource</rdfs:label>
  <skos:definition xml:lang="en">Relates a resource to a note providing information on the dimensions of a resource that is not recorded as part of a dimensions element.</skos:definition>
  <rdf:type rdf:resource="http://www.w3.org/1999/02/22-rdf-syntax-ns#Property" />
  <reg:hasSubproperty rdf:resource="http://rdaregistry.info/Elements/i/P40010" />
  <reg:hasSubproperty rdf:resource="http://rdaregistry.info/Elements/m/P30060" />
  <reg:lexicalAlias rdf:resource="http://rdaregistry.info/Elements/u/noteOnDimensionsOfResource.en" />
  <rdfs:subPropertyOf rdf:resource="http://rdaregistry.info/Elements/u/P60470" />
</owl:ObjectProperty>

<!-- Property: has note on distribution statement -->
<owl:ObjectProperty rdf:about="http://rdaregistry.info/Elements/u/P60125">
  <rdfs:isDefinedBy rdf:resource="http://rdaregistry.info/Elements/u/" />
  <reg:status rdf:resource="http://metadataregistry.org/uri/RegStatus/1001" />
  <reg:name xml:lang="en">noteOnDistributionStatement</reg:name>
  <rdfs:label xml:lang="en">has note on distribution statement</rdfs:label>
  <skos:definition xml:lang="en">Relates a resource to a note providing details on place of distribution, distributor, or date of distribution, or information on changes in the place of distribution, distributor, or distributors name.</skos:definition>
  <rdf:type rdf:resource="http://www.w3.org/1999/02/22-rdf-syntax-ns#Property" />
  <reg:hasSubproperty rdf:resource="http://rdaregistry.info/Elements/m/P30052" />
  <reg:lexicalAlias rdf:resource="http://rdaregistry.info/Elements/u/noteOnDistributionStatement.en" />
  <rdfs:subPropertyOf rdf:resource="http://rdaregistry.info/Elements/u/P60470" />
</owl:ObjectProperty>

<!-- Property: has note on edition statement -->
<owl:ObjectProperty rdf:about="http://rdaregistry.info/Elements/u/P60137">
  <rdfs:isDefinedBy rdf:resource="http://rdaregistry.info/Elements/u/" />
  <reg:status rdf:resource="http://metadataregistry.org/uri/RegStatus/1001" />
  <reg:name xml:lang="en">noteOnEditionStatement</reg:name>
  <rdfs:label xml:lang="en">has note on edition statement</rdfs:label>
  <skos:definition xml:lang="en">Relates a resource to a note providing information on a source of an edition statement, on edition statements relating to issues, parts, etc., on changes in edition statements, or other information relating to an edition statement.</skos:definition>
  <rdf:type rdf:resource="http://www.w3.org/1999/02/22-rdf-syntax-ns#Property" />
  <reg:hasSubproperty rdf:resource="http://rdaregistry.info/Elements/m/P30064" />
  <reg:lexicalAlias rdf:resource="http://rdaregistry.info/Elements/u/noteOnEditionStatement.en" />
  <rdfs:subPropertyOf rdf:resource="http://rdaregistry.info/Elements/u/P60470" />
</owl:ObjectProperty>

<!-- Property: has note on extent of resource -->
<owl:ObjectProperty rdf:about="http://rdaregistry.info/Elements/u/P60134">
  <rdfs:isDefinedBy rdf:resource="http://rdaregistry.info/Elements/u/" />
  <reg:status rdf:resource="http://metadataregistry.org/uri/RegStatus/1001" />
  <reg:name xml:lang="en">noteOnExtentOfResource</reg:name>
  <rdfs:label xml:lang="en">has note on extent of resource</rdfs:label>
  <skos:definition xml:lang="en">Relates a resource to a note providing information on the extent of a resource that is not recorded as part of an extent element.</skos:definition>
  <rdf:type rdf:resource="http://www.w3.org/1999/02/22-rdf-syntax-ns#Property" />
  <reg:hasSubproperty rdf:resource="http://rdaregistry.info/Elements/i/P40011" />
  <reg:hasSubproperty rdf:resource="http://rdaregistry.info/Elements/m/P30061" />
  <reg:lexicalAlias rdf:resource="http://rdaregistry.info/Elements/u/noteOnExtentOfResource.en" />
  <rdfs:subPropertyOf rdf:resource="http://rdaregistry.info/Elements/u/P60470" />
</owl:ObjectProperty>

<!-- Property: has note on frequency -->
<owl:ObjectProperty rdf:about="http://rdaregistry.info/Elements/u/P60129">
  <rdfs:isDefinedBy rdf:resource="http://rdaregistry.info/Elements/u/" />
  <reg:status rdf:resource="http://metadataregistry.org/uri/RegStatus/1001" />
  <reg:name xml:lang="en">noteOnFrequency</reg:name>
  <rdfs:label xml:lang="en">has note on frequency</rdfs:label>
  <skos:definition xml:lang="en">Relates a resource to a note providing details on the currency of the contents, on the frequency of release of issues or parts of a serial or the frequency of updates to an integrating resource, or on changes in frequency.</skos:definition>
  <rdf:type rdf:resource="http://www.w3.org/1999/02/22-rdf-syntax-ns#Property" />
  <reg:hasSubproperty rdf:resource="http://rdaregistry.info/Elements/m/P30056" />
  <reg:lexicalAlias rdf:resource="http://rdaregistry.info/Elements/u/noteOnFrequency.en" />
  <rdfs:subPropertyOf rdf:resource="http://rdaregistry.info/Elements/u/P60470" />
</owl:ObjectProperty>

<!-- Property: has note on identifier for resource -->
<owl:ObjectProperty rdf:about="http://rdaregistry.info/Elements/u/P60868">
  <rdfs:isDefinedBy rdf:resource="http://rdaregistry.info/Elements/u/" />
  <reg:status rdf:resource="http://metadataregistry.org/uri/RegStatus/1001" />
  <rdf:type rdf:resource="http://www.w3.org/1999/02/22-rdf-syntax-ns#Property" />
  <reg:name xml:lang="en">noteOnIdentifierForResource</reg:name>
  <rdfs:label xml:lang="en">has note on identifier for resource</rdfs:label>
  <reg:lexicalAlias rdf:resource="http://rdaregistry.info/Elements/u/noteOnIdentifierForResource.en" />
  <skos:definition xml:lang="en">Relates a resource to a note providing information on identifiers for a resource not recorded as part of an identifier for a resource element.</skos:definition>
  <rdfs:subPropertyOf rdf:resource="http://rdaregistry.info/Elements/u/P60470" />
</owl:ObjectProperty>

<!-- Property: has note on issue, part, or iteration used as basis for identification of resource -->
<owl:ObjectProperty rdf:about="http://rdaregistry.info/Elements/u/P60122">
  <rdfs:isDefinedBy rdf:resource="http://rdaregistry.info/Elements/u/" />
  <reg:status rdf:resource="http://metadataregistry.org/uri/RegStatus/1001" />
  <reg:name xml:lang="en">noteOnIssuePartOrIterationUsedAsBasisForIdentificationOfResource</reg:name>
  <rdfs:label xml:lang="en">has note on issue, part, or iteration used as basis for identification of resource</rdfs:label>
  <skos:definition xml:lang="en">Relates a resource to a note identifying an issue or part of a multipart monograph or serial, or an iteration of an integrating resource that has been used as a basis for the identification of a resource.</skos:definition>
  <rdf:type rdf:resource="http://www.w3.org/1999/02/22-rdf-syntax-ns#Property" />
  <reg:hasSubproperty rdf:resource="http://rdaregistry.info/Elements/m/P30050" />
  <reg:lexicalAlias rdf:resource="http://rdaregistry.info/Elements/u/noteOnIssuePartOrIterationUsedAsBasisForIdentificationOfResource.en" />
  <rdfs:subPropertyOf rdf:resource="http://rdaregistry.info/Elements/u/P60470" />
</owl:ObjectProperty>

<!-- Property: DEPRECATED -->
<owl:ObjectProperty rdf:about="http://rdaregistry.info/Elements/u/P60471">
  <rdfs:isDefinedBy rdf:resource="http://rdaregistry.info/Elements/u/" />
  <reg:status rdf:resource="http://metadataregistry.org/uri/RegStatus/1008" />
</owl:ObjectProperty>

<!-- Property: has note on manufacture statement -->
<owl:ObjectProperty rdf:about="http://rdaregistry.info/Elements/u/P60126">
  <rdfs:isDefinedBy rdf:resource="http://rdaregistry.info/Elements/u/" />
  <reg:status rdf:resource="http://metadataregistry.org/uri/RegStatus/1001" />
  <reg:name xml:lang="en">noteOnManufactureStatement</reg:name>
  <rdfs:label xml:lang="en">has note on manufacture statement</rdfs:label>
  <skos:definition xml:lang="en">Relates a resource to a note providing details on place of manufacture, manufacturer, or date of manufacture, or information on changes in place of manufacture, manufacturer, or manufacturers name.</skos:definition>
  <rdf:type rdf:resource="http://www.w3.org/1999/02/22-rdf-syntax-ns#Property" />
  <reg:hasSubproperty rdf:resource="http://rdaregistry.info/Elements/m/P30053" />
  <reg:lexicalAlias rdf:resource="http://rdaregistry.info/Elements/u/noteOnManufactureStatement.en" />
  <rdfs:subPropertyOf rdf:resource="http://rdaregistry.info/Elements/u/P60470" />
</owl:ObjectProperty>

<!-- Property: has note on numbering of serials -->
<owl:ObjectProperty rdf:about="http://rdaregistry.info/Elements/u/P60135">
  <rdfs:isDefinedBy rdf:resource="http://rdaregistry.info/Elements/u/" />
  <reg:status rdf:resource="http://metadataregistry.org/uri/RegStatus/1001" />
  <reg:name xml:lang="en">noteOnNumberingOfSerials</reg:name>
  <rdfs:label xml:lang="en">has note on numbering of serials</rdfs:label>
  <skos:definition xml:lang="en">Relates a resource to a note providing information on the numbering of the first or last issue or part, on complex or irregular numbering including numbering errors, on a period covered by a volume, issue, part, etc., or on other information relating to numbering of serials.</skos:definition>
  <rdf:type rdf:resource="http://www.w3.org/1999/02/22-rdf-syntax-ns#Property" />
  <reg:hasSubproperty rdf:resource="http://rdaregistry.info/Elements/m/P30062" />
  <reg:lexicalAlias rdf:resource="http://rdaregistry.info/Elements/u/noteOnNumberingOfSerials.en" />
  <rdfs:subPropertyOf rdf:resource="http://rdaregistry.info/Elements/u/P60470" />
</owl:ObjectProperty>

<!-- Property: has note on production statement -->
<owl:ObjectProperty rdf:about="http://rdaregistry.info/Elements/u/P60127">
  <rdfs:isDefinedBy rdf:resource="http://rdaregistry.info/Elements/u/" />
  <reg:status rdf:resource="http://metadataregistry.org/uri/RegStatus/1001" />
  <reg:name xml:lang="en">noteOnProductionStatement</reg:name>
  <rdfs:label xml:lang="en">has note on production statement</rdfs:label>
  <skos:definition xml:lang="en">Relates a resource to a note providing details on place of production, producer, or date of production, or information on changes in place of production, producer, or producers name.</skos:definition>
  <rdf:type rdf:resource="http://www.w3.org/1999/02/22-rdf-syntax-ns#Property" />
  <reg:hasSubproperty rdf:resource="http://rdaregistry.info/Elements/m/P30054" />
  <reg:lexicalAlias rdf:resource="http://rdaregistry.info/Elements/u/noteOnProductionStatement.en" />
  <rdfs:subPropertyOf rdf:resource="http://rdaregistry.info/Elements/u/P60470" />
</owl:ObjectProperty>

<!-- Property: has note on publication statement -->
<owl:ObjectProperty rdf:about="http://rdaregistry.info/Elements/u/P60128">
  <rdfs:isDefinedBy rdf:resource="http://rdaregistry.info/Elements/u/" />
  <reg:status rdf:resource="http://metadataregistry.org/uri/RegStatus/1001" />
  <reg:name xml:lang="en">noteOnPublicationStatement</reg:name>
  <rdfs:label xml:lang="en">has note on publication statement</rdfs:label>
  <skos:definition xml:lang="en">Relates a resource to a note providing details on place of publication, publisher, or date of publication, information on changes in place of publication, publisher, or publishers name, or on suspension of publication.</skos:definition>
  <rdf:type rdf:resource="http://www.w3.org/1999/02/22-rdf-syntax-ns#Property" />
  <reg:hasSubproperty rdf:resource="http://rdaregistry.info/Elements/m/P30055" />
  <reg:lexicalAlias rdf:resource="http://rdaregistry.info/Elements/u/noteOnPublicationStatement.en" />
  <rdfs:subPropertyOf rdf:resource="http://rdaregistry.info/Elements/u/P60470" />
</owl:ObjectProperty>

<!-- Property: has note on resource -->
<owl:ObjectProperty rdf:about="http://rdaregistry.info/Elements/u/P60470">
  <rdfs:isDefinedBy rdf:resource="http://rdaregistry.info/Elements/u/" />
  <reg:status rdf:resource="http://metadataregistry.org/uri/RegStatus/1001" />
  <reg:name xml:lang="en">noteOnResource</reg:name>
  <rdfs:label xml:lang="en">has note on resource</rdfs:label>
  <skos:definition xml:lang="en">Relates a resource to a note providing additional information about content recorded as a resource attribute.</skos:definition>
  <rdf:type rdf:resource="http://www.w3.org/1999/02/22-rdf-syntax-ns#Property" />
  <reg:hasSubproperty rdf:resource="http://rdaregistry.info/Elements/u/P60123" />
  <reg:hasSubproperty rdf:resource="http://rdaregistry.info/Elements/e/P20071" />
  <reg:hasSubproperty rdf:resource="http://rdaregistry.info/Elements/i/P40028" />
  <reg:hasSubproperty rdf:resource="http://rdaregistry.info/Elements/m/P30137" />
  <reg:hasSubproperty rdf:resource="http://rdaregistry.info/Elements/m/P30214" />
  <reg:lexicalAlias rdf:resource="http://rdaregistry.info/Elements/u/noteOnResource.en" />
  <reg:hasSubproperty rdf:resource="http://rdaregistry.info/Elements/u/P60122" />
  <reg:hasSubproperty rdf:resource="http://rdaregistry.info/Elements/u/P60124" />
  <reg:hasSubproperty rdf:resource="http://rdaregistry.info/Elements/u/P60125" />
  <reg:hasSubproperty rdf:resource="http://rdaregistry.info/Elements/u/P60126" />
  <reg:hasSubproperty rdf:resource="http://rdaregistry.info/Elements/u/P60127" />
  <reg:hasSubproperty rdf:resource="http://rdaregistry.info/Elements/u/P60128" />
  <reg:hasSubproperty rdf:resource="http://rdaregistry.info/Elements/u/P60129" />
  <reg:hasSubproperty rdf:resource="http://rdaregistry.info/Elements/u/P60130" />
  <reg:hasSubproperty rdf:resource="http://rdaregistry.info/Elements/u/P60131" />
  <reg:hasSubproperty rdf:resource="http://rdaregistry.info/Elements/u/P60132" />
  <reg:hasSubproperty rdf:resource="http://rdaregistry.info/Elements/u/P60133" />
  <reg:hasSubproperty rdf:resource="http://rdaregistry.info/Elements/u/P60134" />
  <reg:hasSubproperty rdf:resource="http://rdaregistry.info/Elements/u/P60135" />
  <reg:hasSubproperty rdf:resource="http://rdaregistry.info/Elements/u/P60136" />
  <reg:hasSubproperty rdf:resource="http://rdaregistry.info/Elements/u/P60137" />
  <reg:hasSubproperty rdf:resource="http://rdaregistry.info/Elements/u/P60868" />
</owl:ObjectProperty>

<!-- Property: has note on resource-specific carrier characteristic -->
<owl:ObjectProperty rdf:about="http://rdaregistry.info/Elements/u/P60056">
  <rdfs:isDefinedBy rdf:resource="http://rdaregistry.info/Elements/u/" />
  <reg:status rdf:resource="http://metadataregistry.org/uri/RegStatus/1001" />
  <reg:name xml:lang="en">noteOnResourceSpecificCarrierCharacteristic</reg:name>
  <rdfs:label xml:lang="en">has note on resource-specific carrier characteristic</rdfs:label>
  <skos:definition xml:lang="en">Relates a resource to a note providing information about additional characteristics that are specific to a resource being described and are assumed not to apply to other resources exemplifying the same resource.</skos:definition>
  <rdf:type rdf:resource="http://www.w3.org/1999/02/22-rdf-syntax-ns#Property" />
  <reg:hasSubproperty rdf:resource="http://rdaregistry.info/Elements/u/P60055" />
  <reg:hasSubproperty rdf:resource="http://rdaregistry.info/Elements/i/P40003" />
  <reg:lexicalAlias rdf:resource="http://rdaregistry.info/Elements/u/noteOnResourceSpecificCarrierCharacteristic.en" />
</owl:ObjectProperty>

<!-- Property: has note on series statement -->
<owl:ObjectProperty rdf:about="http://rdaregistry.info/Elements/u/P60131">
  <rdfs:isDefinedBy rdf:resource="http://rdaregistry.info/Elements/u/" />
  <reg:status rdf:resource="http://metadataregistry.org/uri/RegStatus/1001" />
  <reg:name xml:lang="en">noteOnSeriesStatement</reg:name>
  <rdfs:label xml:lang="en">has note on series statement</rdfs:label>
  <skos:definition xml:lang="en">Relates a resource to a note providing information on complex series statements, incorrect numbering within series, or changes in series statements.</skos:definition>
  <rdf:type rdf:resource="http://www.w3.org/1999/02/22-rdf-syntax-ns#Property" />
  <reg:hasSubproperty rdf:resource="http://rdaregistry.info/Elements/m/P30058" />
  <reg:lexicalAlias rdf:resource="http://rdaregistry.info/Elements/u/noteOnSeriesStatement.en" />
  <rdfs:subPropertyOf rdf:resource="http://rdaregistry.info/Elements/u/P60470" />
</owl:ObjectProperty>

<!-- Property: has note on statement of responsibility -->
<owl:ObjectProperty rdf:about="http://rdaregistry.info/Elements/u/P60130">
  <rdfs:isDefinedBy rdf:resource="http://rdaregistry.info/Elements/u/" />
  <reg:status rdf:resource="http://metadataregistry.org/uri/RegStatus/1001" />
  <reg:name xml:lang="en">noteOnStatementOfResponsibility</reg:name>
  <rdfs:label xml:lang="en">has note on statement of responsibility</rdfs:label>
  <skos:definition xml:lang="en">Relates a resource to a note providing information on an agent not named in a statement of responsibility to whom responsibility for the creation of, or contribution to a realization of, the intellectual or artistic content of a resource has been attributed, on variant forms of names appearing in the resource, on changes in statements of responsibility, or on other details relating to a statement of responsibility.</skos:definition>
  <rdf:type rdf:resource="http://www.w3.org/1999/02/22-rdf-syntax-ns#Property" />
  <reg:hasSubproperty rdf:resource="http://rdaregistry.info/Elements/m/P30057" />
  <reg:lexicalAlias rdf:resource="http://rdaregistry.info/Elements/u/noteOnStatementOfResponsibility.en" />
  <rdfs:subPropertyOf rdf:resource="http://rdaregistry.info/Elements/u/P60470" />
</owl:ObjectProperty>

<!-- Property: has note on title -->
<owl:ObjectProperty rdf:about="http://rdaregistry.info/Elements/u/P60136">
  <rdfs:isDefinedBy rdf:resource="http://rdaregistry.info/Elements/u/" />
  <reg:status rdf:resource="http://metadataregistry.org/uri/RegStatus/1001" />
  <reg:name xml:lang="en">noteOnTitle</reg:name>
  <rdfs:label xml:lang="en">has note on title</rdfs:label>
  <skos:definition xml:lang="en">Relates a resource to a note providing information on a source from which a title was taken, on the date a title was viewed, on variations in titles, on inaccuracies, deletions, etc., or other information relating to a title.</skos:definition>
  <rdf:type rdf:resource="http://www.w3.org/1999/02/22-rdf-syntax-ns#Property" />
  <reg:hasSubproperty rdf:resource="http://rdaregistry.info/Elements/m/P30063" />
  <reg:lexicalAlias rdf:resource="http://rdaregistry.info/Elements/u/noteOnTitle.en" />
  <rdfs:subPropertyOf rdf:resource="http://rdaregistry.info/Elements/u/P60470" />
</owl:ObjectProperty>

<!-- Property: is adapted as novel -->
<owl:ObjectProperty rdf:about="http://rdaregistry.info/Elements/u/P60138">
  <rdfs:isDefinedBy rdf:resource="http://rdaregistry.info/Elements/u/" />
  <reg:status rdf:resource="http://metadataregistry.org/uri/RegStatus/1001" />
  <reg:name xml:lang="en">novelization</reg:name>
  <rdfs:label xml:lang="en">is adapted as novel</rdfs:label>
  <skos:definition xml:lang="en">Relates a resource to a novel adapted from a source resource.</skos:definition>
  <rdf:type rdf:resource="http://www.w3.org/1999/02/22-rdf-syntax-ns#Property" />
  <rdfs:subPropertyOf rdf:resource="http://rdaregistry.info/Elements/u/P60260" />
  <owl:inverseOf rdf:resource="http://rdaregistry.info/Elements/u/P60228" />
  <reg:hasSubproperty rdf:resource="http://rdaregistry.info/Elements/e/P20088" />
  <reg:lexicalAlias rdf:resource="http://rdaregistry.info/Elements/u/adaptedAsNovel.en" />
</owl:ObjectProperty>

<!-- Property: is novelization of -->
<owl:ObjectProperty rdf:about="http://rdaregistry.info/Elements/u/P60228">
  <rdfs:isDefinedBy rdf:resource="http://rdaregistry.info/Elements/u/" />
  <reg:status rdf:resource="http://metadataregistry.org/uri/RegStatus/1001" />
  <reg:name xml:lang="en">novelizationOf</reg:name>
  <rdfs:label xml:lang="en">is novelization of</rdfs:label>
  <skos:definition xml:lang="en">Relates a resource to a resource that has been adapted as a novel.</skos:definition>
  <rdf:type rdf:resource="http://www.w3.org/1999/02/22-rdf-syntax-ns#Property" />
  <rdfs:subPropertyOf rdf:resource="http://rdaregistry.info/Elements/u/P60241" />
  <owl:inverseOf rdf:resource="http://rdaregistry.info/Elements/u/P60138" />
  <reg:hasSubproperty rdf:resource="http://rdaregistry.info/Elements/e/P20126" />
  <reg:lexicalAlias rdf:resource="http://rdaregistry.info/Elements/u/novelizationOf.en" />
</owl:ObjectProperty>

<!-- Property: has numbering of part -->
<owl:ObjectProperty rdf:about="http://rdaregistry.info/Elements/u/P60080">
  <rdfs:isDefinedBy rdf:resource="http://rdaregistry.info/Elements/u/" />
  <reg:status rdf:resource="http://metadataregistry.org/uri/RegStatus/1001" />
  <reg:name xml:lang="en">numberingOfPart</reg:name>
  <rdfs:label xml:lang="en">has numbering of part</rdfs:label>
  <skos:definition xml:lang="en">Relates a resource to a designation of a sequencing of a part or parts within a larger resource.</skos:definition>
  <rdf:type rdf:resource="http://www.w3.org/1999/02/22-rdf-syntax-ns#Property" />
  <reg:lexicalAlias rdf:resource="http://rdaregistry.info/Elements/u/numberingOfPart.en" />
  <skos:scopeNote xml:lang="en">Numbering includes a numeral, a letter, any other character, or the combination of these with or without an accompanying caption, and/or a chronological designation.</skos:scopeNote>
</owl:ObjectProperty>

<!-- Property: has numbering of serials -->
<owl:ObjectProperty rdf:about="http://rdaregistry.info/Elements/u/P60533">
  <rdfs:isDefinedBy rdf:resource="http://rdaregistry.info/Elements/u/" />
  <reg:status rdf:resource="http://metadataregistry.org/uri/RegStatus/1001" />
  <reg:name xml:lang="en">numberingOfSerials</reg:name>
  <rdfs:label xml:lang="en">has numbering of serials</rdfs:label>
  <skos:definition xml:lang="en">Relates a resource to a designation for each of the issues or parts of a serial.</skos:definition>
  <rdf:type rdf:resource="http://www.w3.org/1999/02/22-rdf-syntax-ns#Property" />
  <reg:hasSubproperty rdf:resource="http://rdaregistry.info/Elements/u/P60499" />
  <reg:hasSubproperty rdf:resource="http://rdaregistry.info/Elements/u/P60500" />
  <reg:hasSubproperty rdf:resource="http://rdaregistry.info/Elements/u/P60501" />
  <reg:hasSubproperty rdf:resource="http://rdaregistry.info/Elements/u/P60502" />
  <reg:hasSubproperty rdf:resource="http://rdaregistry.info/Elements/m/P30165" />
  <reg:lexicalAlias rdf:resource="http://rdaregistry.info/Elements/u/numberingOfSerials.en" />
  <skos:scopeNote xml:lang="en">Numbering includes a numeral, a letter, any other character, or the combination of these with or without an accompanying caption and/or a chronological designation.</skos:scopeNote>
  <reg:hasSubproperty rdf:resource="http://rdaregistry.info/Elements/u/P60818" />
  <reg:hasSubproperty rdf:resource="http://rdaregistry.info/Elements/u/P60819" />
  <reg:hasSubproperty rdf:resource="http://rdaregistry.info/Elements/u/P60820" />
  <reg:hasSubproperty rdf:resource="http://rdaregistry.info/Elements/u/P60821" />
</owl:ObjectProperty>

<!-- Property: has numbering within series -->
<owl:ObjectProperty rdf:about="http://rdaregistry.info/Elements/u/P60081">
  <rdfs:isDefinedBy rdf:resource="http://rdaregistry.info/Elements/u/" />
  <reg:status rdf:resource="http://metadataregistry.org/uri/RegStatus/1001" />
  <reg:name xml:lang="en">numberingWithinSeries</reg:name>
  <rdfs:label xml:lang="en">has numbering within series</rdfs:label>
  <skos:definition xml:lang="en">Relates a resource to a designation of a sequencing of a part or parts within a series.</skos:definition>
  <rdf:type rdf:resource="http://www.w3.org/1999/02/22-rdf-syntax-ns#Property" />
  <reg:hasSubproperty rdf:resource="http://rdaregistry.info/Elements/m/P30014" />
  <reg:lexicalAlias rdf:resource="http://rdaregistry.info/Elements/u/numberingWithinSeries.en" />
  <skos:scopeNote xml:lang="en">Numbering includes a numeral, a letter, any other character, or the combination of these with or without an accompanying caption and/or a chronological designation.</skos:scopeNote>
</owl:ObjectProperty>

<!-- Property: has numbering within subseries -->
<owl:ObjectProperty rdf:about="http://rdaregistry.info/Elements/u/P60082">
  <rdfs:isDefinedBy rdf:resource="http://rdaregistry.info/Elements/u/" />
  <reg:status rdf:resource="http://metadataregistry.org/uri/RegStatus/1001" />
  <reg:name xml:lang="en">numberingWithinSubseries</reg:name>
  <rdfs:label xml:lang="en">has numbering within subseries</rdfs:label>
  <skos:definition xml:lang="en">Relates a resource to a designation of a sequencing of a part or parts within a subseries.</skos:definition>
  <rdf:type rdf:resource="http://www.w3.org/1999/02/22-rdf-syntax-ns#Property" />
  <reg:hasSubproperty rdf:resource="http://rdaregistry.info/Elements/m/P30015" />
  <reg:lexicalAlias rdf:resource="http://rdaregistry.info/Elements/u/numberingWithinSubseries.en" />
  <skos:scopeNote xml:lang="en">Numbering includes a numeral, a letter, any other character, or the combination of these with or without an accompanying caption and/or a chronological designation.</skos:scopeNote>
</owl:ObjectProperty>

<!-- Property: has number of conference, etc. -->
<owl:ObjectProperty rdf:about="http://rdaregistry.info/Elements/u/P60079">
  <rdfs:isDefinedBy rdf:resource="http://rdaregistry.info/Elements/u/" />
  <reg:status rdf:resource="http://metadataregistry.org/uri/RegStatus/1001" />
  <reg:name xml:lang="en">numberOfConferenceEtc</reg:name>
  <rdfs:label xml:lang="en">has number of conference, etc.</rdfs:label>
  <skos:definition xml:lang="en">Relates a resource to a designation of a sequencing of a conference, etc., within a series of conferences, etc.</skos:definition>
  <rdf:type rdf:resource="http://www.w3.org/1999/02/22-rdf-syntax-ns#Property" />
  <reg:hasSubproperty rdf:resource="http://rdaregistry.info/Elements/a/P50019" />
  <reg:lexicalAlias rdf:resource="http://rdaregistry.info/Elements/u/numberOfConferenceEtc.en" />
</owl:ObjectProperty>

<!-- Property: has numeric and/or alphabetic designation of first issue or part of sequence -->
<owl:ObjectProperty rdf:about="http://rdaregistry.info/Elements/u/P60499">
  <rdfs:isDefinedBy rdf:resource="http://rdaregistry.info/Elements/u/" />
  <reg:status rdf:resource="http://metadataregistry.org/uri/RegStatus/1001" />
  <reg:name xml:lang="en">numericAndOrAlphabeticDesignationOfFirstIssueOrPartOfSequence</reg:name>
  <rdfs:label xml:lang="en">has numeric and/or alphabetic designation of first issue or part of sequence</rdfs:label>
  <skos:definition xml:lang="en">Relates a resource to a designation in numeric or alphabetic form presented on the first issue or part of a serial issued in a sequence of numbering.</skos:definition>
  <rdf:type rdf:resource="http://www.w3.org/1999/02/22-rdf-syntax-ns#Property" />
  <rdfs:subPropertyOf rdf:resource="http://rdaregistry.info/Elements/u/P60533" />
  <reg:hasSubproperty rdf:resource="http://rdaregistry.info/Elements/m/P30147" />
  <reg:lexicalAlias rdf:resource="http://rdaregistry.info/Elements/u/numericAndOrAlphabeticDesignationOfFirstIssueOrPartOfSequence.en" />
</owl:ObjectProperty>

<!-- Property: has numeric and/or alphabetic designation of last issue or part of sequence -->
<owl:ObjectProperty rdf:about="http://rdaregistry.info/Elements/u/P60500">
  <rdfs:isDefinedBy rdf:resource="http://rdaregistry.info/Elements/u/" />
  <reg:status rdf:resource="http://metadataregistry.org/uri/RegStatus/1001" />
  <reg:name xml:lang="en">numericAndOrAlphabeticDesignationOfLastIssueOrPartOfSequence</reg:name>
  <rdfs:label xml:lang="en">has numeric and/or alphabetic designation of last issue or part of sequence</rdfs:label>
  <skos:definition xml:lang="en">Relates a resource to a designation in numeric or alphabetic form presented on the last issue or part of a serial issued in a sequence of numbering.</skos:definition>
  <rdf:type rdf:resource="http://www.w3.org/1999/02/22-rdf-syntax-ns#Property" />
  <rdfs:subPropertyOf rdf:resource="http://rdaregistry.info/Elements/u/P60533" />
  <reg:hasSubproperty rdf:resource="http://rdaregistry.info/Elements/m/P30148" />
  <reg:lexicalAlias rdf:resource="http://rdaregistry.info/Elements/u/numericAndOrAlphabeticDesignationOfLastIssueOrPartOfSequence.en" />
</owl:ObjectProperty>

<!-- Property: has numeric designation of musical resource -->
<owl:ObjectProperty rdf:about="http://rdaregistry.info/Elements/u/P60315">
  <rdfs:isDefinedBy rdf:resource="http://rdaregistry.info/Elements/u/" />
  <reg:status rdf:resource="http://metadataregistry.org/uri/RegStatus/1001" />
  <reg:name xml:lang="en">numericDesignationOfMusicalResource</reg:name>
  <rdfs:label xml:lang="en">has numeric designation of musical resource</rdfs:label>
  <skos:definition xml:lang="en">Relates a resource to a serial number, opus number, or thematic index number assigned to a musical resource by a composer, publisher, or a musicologist.</skos:definition>
  <rdf:type rdf:resource="http://www.w3.org/1999/02/22-rdf-syntax-ns#Property" />
  <reg:lexicalAlias rdf:resource="http://rdaregistry.info/Elements/u/numericDesignationOfMusicalResource.en" />
  <skos:scopeNote xml:lang="en">A numeric designation of a musical resource includes a caption such as e.g., no., op., BWV, and it may include a numeral, a letter, a word, any other character, or the combination of these.</skos:scopeNote>
</owl:ObjectProperty>

<!-- Property: has officer -->
<owl:ObjectProperty rdf:about="http://rdaregistry.info/Elements/u/P60633">
  <rdfs:isDefinedBy rdf:resource="http://rdaregistry.info/Elements/u/" />
  <reg:status rdf:resource="http://metadataregistry.org/uri/RegStatus/1001" />
  <reg:name xml:lang="en">officer</reg:name>
  <rdfs:label xml:lang="en">has officer</rdfs:label>
  <skos:definition xml:lang="en">Relates an agent holding an office in or commanding an agent to an agent.</skos:definition>
  <rdf:type rdf:resource="http://www.w3.org/1999/02/22-rdf-syntax-ns#Property" />
  <reg:hasSubproperty rdf:resource="http://rdaregistry.info/Elements/a/P50027" />
  <reg:lexicalAlias rdf:resource="http://rdaregistry.info/Elements/u/officer.en" />
  <owl:inverseOf rdf:resource="http://rdaregistry.info/Elements/u/P60737" />
  <reg:hasSubproperty rdf:resource="http://rdaregistry.info/Elements/u/P60864" />
  <reg:hasSubproperty rdf:resource="http://rdaregistry.info/Elements/u/P60866" />
  <rdfs:subPropertyOf rdf:resource="http://rdaregistry.info/Elements/u/P60454" />
</owl:ObjectProperty>

<!-- Property: has officer of -->
<owl:ObjectProperty rdf:about="http://rdaregistry.info/Elements/u/P60737">
  <rdfs:isDefinedBy rdf:resource="http://rdaregistry.info/Elements/u/" />
  <reg:status rdf:resource="http://metadataregistry.org/uri/RegStatus/1001" />
  <reg:name xml:lang="en">officerOf</reg:name>
  <rdfs:label xml:lang="en">has officer of</rdfs:label>
  <skos:definition xml:lang="en">Relates an agent to an agent holding an office in or commanding an agent.</skos:definition>
  <rdf:type rdf:resource="http://www.w3.org/1999/02/22-rdf-syntax-ns#Property" />
  <owl:inverseOf rdf:resource="http://rdaregistry.info/Elements/u/P60633" />
  <reg:hasSubproperty rdf:resource="http://rdaregistry.info/Elements/a/P50234" />
  <reg:lexicalAlias rdf:resource="http://rdaregistry.info/Elements/u/officerOf.en" />
  <rdfs:subPropertyOf rdf:resource="http://rdaregistry.info/Elements/u/P60454" />
  <reg:hasSubproperty rdf:resource="http://rdaregistry.info/Elements/u/P60865" />
  <reg:hasSubproperty rdf:resource="http://rdaregistry.info/Elements/u/P60867" />
</owl:ObjectProperty>

<!-- Property: is on disc with -->
<owl:ObjectProperty rdf:about="http://rdaregistry.info/Elements/u/P60257">
  <rdfs:isDefinedBy rdf:resource="http://rdaregistry.info/Elements/u/" />
  <reg:status rdf:resource="http://metadataregistry.org/uri/RegStatus/1001" />
  <reg:name xml:lang="en">onDiscWith</reg:name>
  <rdfs:label xml:lang="en">is on disc with</rdfs:label>
  <skos:definition xml:lang="en">Relates a resource to a resource that is issued on the same disc with a resource being described.</skos:definition>
  <rdf:type rdf:resource="http://www.w3.org/1999/02/22-rdf-syntax-ns#Property" />
  <rdfs:subPropertyOf rdf:resource="http://rdaregistry.info/Elements/u/P60256" />
  <owl:inverseOf rdf:resource="http://rdaregistry.info/Elements/u/P60257" />
  <reg:hasSubproperty rdf:resource="http://rdaregistry.info/Elements/i/P40035" />
  <reg:hasSubproperty rdf:resource="http://rdaregistry.info/Elements/m/P30036" />
  <reg:lexicalAlias rdf:resource="http://rdaregistry.info/Elements/u/onDiscWith.en" />
</owl:ObjectProperty>

<!-- Property: has on-screen participant -->
<owl:ObjectProperty rdf:about="http://rdaregistry.info/Elements/u/P60824">
  <rdfs:isDefinedBy rdf:resource="http://rdaregistry.info/Elements/u/" />
  <reg:status rdf:resource="http://metadataregistry.org/uri/RegStatus/1001" />
  <rdf:type rdf:resource="http://www.w3.org/1999/02/22-rdf-syntax-ns#Property" />
  <reg:name xml:lang="en">onScreenParticipant</reg:name>
  <rdfs:label xml:lang="en">has on-screen participant</rdfs:label>
  <reg:lexicalAlias rdf:resource="http://rdaregistry.info/Elements/u/onScreenParticipant.en" />
  <skos:definition xml:lang="en">Relates a resource to an agent contributing to a nonfiction moving image resource by taking an active role as a participant.</skos:definition>
  <owl:inverseOf rdf:resource="http://rdaregistry.info/Elements/u/P60825" />
  <reg:hasSubproperty rdf:resource="http://rdaregistry.info/Elements/e/P20279" />
  <skos:scopeNote xml:lang="en">Appearance on screen to provide contextual or background information is excluded.</skos:scopeNote>
  <rdfs:subPropertyOf rdf:resource="http://rdaregistry.info/Elements/u/P60398" />
  <rdakit:seeAlso rdf:resource="http://rdaregistry.info/Elements/u/P60143" />
</owl:ObjectProperty>

<!-- Property: is on-screen participant of -->
<owl:ObjectProperty rdf:about="http://rdaregistry.info/Elements/u/P60825">
  <rdfs:isDefinedBy rdf:resource="http://rdaregistry.info/Elements/u/" />
  <reg:status rdf:resource="http://metadataregistry.org/uri/RegStatus/1001" />
  <rdf:type rdf:resource="http://www.w3.org/1999/02/22-rdf-syntax-ns#Property" />
  <reg:name xml:lang="en">onScreenParticipantOf</reg:name>
  <rdfs:label xml:lang="en">is on-screen participant of</rdfs:label>
  <reg:lexicalAlias rdf:resource="http://rdaregistry.info/Elements/u/onScreenParticipantOf.en" />
  <skos:definition xml:lang="en">Relates an agent contributing to a nonfiction moving image resource by taking an active role as a participant to a resource.</skos:definition>
  <owl:inverseOf rdf:resource="http://rdaregistry.info/Elements/u/P60824" />
  <reg:hasSubproperty rdf:resource="http://rdaregistry.info/Elements/a/P50261" />
  <skos:scopeNote xml:lang="en">Appearance on screen to provide contextual or background information is excluded.</skos:scopeNote>
  <rdfs:subPropertyOf rdf:resource="http://rdaregistry.info/Elements/u/P60626" />
  <rdakit:seeAlso rdf:resource="http://rdaregistry.info/Elements/u/P60018" />
</owl:ObjectProperty>

<!-- Property: has on-screen presenter -->
<owl:ObjectProperty rdf:about="http://rdaregistry.info/Elements/u/P60143">
  <rdfs:isDefinedBy rdf:resource="http://rdaregistry.info/Elements/u/" />
  <reg:status rdf:resource="http://metadataregistry.org/uri/RegStatus/1001" />
  <reg:name xml:lang="en">onScreenPresenter</reg:name>
  <rdfs:label xml:lang="en">has on-screen presenter</rdfs:label>
  <skos:definition xml:lang="en">Relates a resource to a performer contributing to a resource by appearing on screen to provide contextual or background information. an on-screen presenter may appear in nonfiction moving image materials or in introductions to fiction moving image materials.</skos:definition>
  <rdf:type rdf:resource="http://www.w3.org/1999/02/22-rdf-syntax-ns#Property" />
  <rdfs:subPropertyOf rdf:resource="http://rdaregistry.info/Elements/u/P60387" />
  <owl:inverseOf rdf:resource="http://rdaregistry.info/Elements/u/P60018" />
  <reg:hasSubproperty rdf:resource="http://rdaregistry.info/Elements/e/P20013" />
  <reg:lexicalAlias rdf:resource="http://rdaregistry.info/Elements/u/onScreenPresenter.en" />
  <skos:scopeNote xml:lang="en">Appearance in nonfiction moving image materials or in introductions to fiction moving image materials is included. Appearance on screen in a non-performing role is excluded.</skos:scopeNote>
  <rdakit:seeAlso rdf:resource="http://rdaregistry.info/Elements/u/P60824" />
</owl:ObjectProperty>

<!-- Property: is on-screen presenter of -->
<owl:ObjectProperty rdf:about="http://rdaregistry.info/Elements/u/P60018">
  <rdfs:isDefinedBy rdf:resource="http://rdaregistry.info/Elements/u/" />
  <reg:status rdf:resource="http://metadataregistry.org/uri/RegStatus/1001" />
  <reg:name xml:lang="en">onScreenPresenterOf</reg:name>
  <rdfs:label xml:lang="en">is on-screen presenter of</rdfs:label>
  <skos:definition xml:lang="en">Relates a performer contributing to a resource by appearing on screen to provide contextual or background information. an on-screen presenter may appear in nonfiction moving image materials or in introductions to fiction moving image materials to a resource.</skos:definition>
  <rdf:type rdf:resource="http://www.w3.org/1999/02/22-rdf-syntax-ns#Property" />
  <rdfs:subPropertyOf rdf:resource="http://rdaregistry.info/Elements/u/P60615" />
  <owl:inverseOf rdf:resource="http://rdaregistry.info/Elements/u/P60143" />
  <reg:hasSubproperty rdf:resource="http://rdaregistry.info/Elements/a/P50072" />
  <reg:lexicalAlias rdf:resource="http://rdaregistry.info/Elements/u/onScreenPresenterOf.en" />
  <skos:scopeNote xml:lang="en">Appearance in nonfiction moving image materials or in introductions to fiction moving image materials is included. Appearance on screen in a non-performing role is excluded.</skos:scopeNote>
  <rdakit:seeAlso rdf:resource="http://rdaregistry.info/Elements/u/P60825" />
</owl:ObjectProperty>

<!-- Property: is opera adaptation of -->
<owl:ObjectProperty rdf:about="http://rdaregistry.info/Elements/u/P60720">
  <rdfs:isDefinedBy rdf:resource="http://rdaregistry.info/Elements/u/" />
  <reg:status rdf:resource="http://metadataregistry.org/uri/RegStatus/1001" />
  <reg:name xml:lang="en">operaAdaptationOf</reg:name>
  <rdfs:label xml:lang="en">is opera adaptation of</rdfs:label>
  <skos:definition xml:lang="en">Relates a resource to a resource that has been adapted as an opera.</skos:definition>
  <rdf:type rdf:resource="http://www.w3.org/1999/02/22-rdf-syntax-ns#Property" />
  <rdfs:subPropertyOf rdf:resource="http://rdaregistry.info/Elements/u/P60241" />
  <owl:inverseOf rdf:resource="http://rdaregistry.info/Elements/u/P60722" />
  <reg:hasSubproperty rdf:resource="http://rdaregistry.info/Elements/e/P20240" />
  <reg:lexicalAlias rdf:resource="http://rdaregistry.info/Elements/u/operaAdaptationOf.en" />
</owl:ObjectProperty>

<!-- Property: is oratorio adaptation of -->
<owl:ObjectProperty rdf:about="http://rdaregistry.info/Elements/u/P60830">
  <rdfs:isDefinedBy rdf:resource="http://rdaregistry.info/Elements/u/" />
  <reg:status rdf:resource="http://metadataregistry.org/uri/RegStatus/1001" />
  <rdf:type rdf:resource="http://www.w3.org/1999/02/22-rdf-syntax-ns#Property" />
  <reg:name xml:lang="en">oratorioAdaptationOf</reg:name>
  <rdfs:label xml:lang="en">is oratorio adaptation of</rdfs:label>
  <reg:lexicalAlias rdf:resource="http://rdaregistry.info/Elements/u/oratorioAdaptationOf.en" />
  <skos:definition xml:lang="en">Relates a resource to a resource that has been adapted as an oratorio.</skos:definition>
  <owl:inverseOf rdf:resource="http://rdaregistry.info/Elements/u/P60831" />
  <reg:hasSubproperty rdf:resource="http://rdaregistry.info/Elements/e/P20281" />
  <rdfs:subPropertyOf rdf:resource="http://rdaregistry.info/Elements/u/P60305" />
</owl:ObjectProperty>

<!-- Property: has organizer -->
<owl:ObjectProperty rdf:about="http://rdaregistry.info/Elements/u/P60849">
  <rdfs:isDefinedBy rdf:resource="http://rdaregistry.info/Elements/u/" />
  <reg:status rdf:resource="http://metadataregistry.org/uri/RegStatus/1001" />
  <rdf:type rdf:resource="http://www.w3.org/1999/02/22-rdf-syntax-ns#Property" />
  <reg:name xml:lang="en">organizer</reg:name>
  <rdfs:label xml:lang="en">has organizer</rdfs:label>
  <reg:lexicalAlias rdf:resource="http://rdaregistry.info/Elements/u/organizer.en" />
  <skos:definition xml:lang="en">Relates a resource to an agent organizing an exhibit, event, conference, course, program, etc., which gave rise to a resource.</skos:definition>
  <owl:inverseOf rdf:resource="http://rdaregistry.info/Elements/u/P60850" />
  <reg:hasSubproperty rdf:resource="http://rdaregistry.info/Elements/w/P10297" />
  <rdfs:subPropertyOf rdf:resource="http://rdaregistry.info/Elements/u/P60374" />
</owl:ObjectProperty>

<!-- Property: is organizer of -->
<owl:ObjectProperty rdf:about="http://rdaregistry.info/Elements/u/P60850">
  <rdfs:isDefinedBy rdf:resource="http://rdaregistry.info/Elements/u/" />
  <reg:status rdf:resource="http://metadataregistry.org/uri/RegStatus/1001" />
  <rdf:type rdf:resource="http://www.w3.org/1999/02/22-rdf-syntax-ns#Property" />
  <reg:name xml:lang="en">organizerOf</reg:name>
  <rdfs:label xml:lang="en">is organizer of</rdfs:label>
  <reg:lexicalAlias rdf:resource="http://rdaregistry.info/Elements/u/organizerOf.en" />
  <skos:definition xml:lang="en">Relates an agent organizing an exhibit, event, conference, course, program, etc., which gave rise to a resource to a resource.</skos:definition>
  <owl:inverseOf rdf:resource="http://rdaregistry.info/Elements/u/P60849" />
  <reg:hasSubproperty rdf:resource="http://rdaregistry.info/Elements/a/P50270" />
  <rdfs:subPropertyOf rdf:resource="http://rdaregistry.info/Elements/u/P60602" />
</owl:ObjectProperty>

<!-- Property: DEPRECATED -->
<owl:ObjectProperty rdf:about="http://rdaregistry.info/Elements/u/P60158">
  <rdfs:isDefinedBy rdf:resource="http://rdaregistry.info/Elements/u/" />
  <reg:status rdf:resource="http://metadataregistry.org/uri/RegStatus/1008" />
  <reg:hasSubproperty rdf:resource="http://rdaregistry.info/Elements/u/P60884" />
  <reg:hasSubproperty rdf:resource="http://rdaregistry.info/Elements/u/P60886" />
  <reg:hasSubproperty rdf:resource="http://rdaregistry.info/Elements/u/P60887" />
  <reg:hasSubproperty rdf:resource="http://rdaregistry.info/Elements/u/P60888" />
  <reg:hasSubproperty rdf:resource="http://rdaregistry.info/Elements/u/P60890" />
</owl:ObjectProperty>

<!-- Property: has other agent associated with resource -->
<owl:ObjectProperty rdf:about="http://rdaregistry.info/Elements/u/P60374">
  <rdfs:isDefinedBy rdf:resource="http://rdaregistry.info/Elements/u/" />
  <reg:status rdf:resource="http://metadataregistry.org/uri/RegStatus/1001" />
  <reg:name xml:lang="en">otherAgentAssociatedWithResource</reg:name>
  <rdfs:label xml:lang="en">has other agent associated with resource</rdfs:label>
  <skos:definition xml:lang="en">Relates a resource to an agent other than a creator, custodian, owner, producer, publisher, distributor, or manufacturer associated with a resource.</skos:definition>
  <rdf:type rdf:resource="http://www.w3.org/1999/02/22-rdf-syntax-ns#Property" />
  <owl:inverseOf rdf:resource="http://rdaregistry.info/Elements/u/P60602" />
  <reg:hasSubproperty rdf:resource="http://rdaregistry.info/Elements/u/P60060" />
  <reg:hasSubproperty rdf:resource="http://rdaregistry.info/Elements/u/P60061" />
  <reg:hasSubproperty rdf:resource="http://rdaregistry.info/Elements/u/P60062" />
  <reg:hasSubproperty rdf:resource="http://rdaregistry.info/Elements/u/P60065" />
  <reg:hasSubproperty rdf:resource="http://rdaregistry.info/Elements/u/P60097" />
  <reg:hasSubproperty rdf:resource="http://rdaregistry.info/Elements/u/P60157" />
  <reg:hasSubproperty rdf:resource="http://rdaregistry.info/Elements/u/P60373" />
  <reg:hasSubproperty rdf:resource="http://rdaregistry.info/Elements/u/P60375" />
  <reg:hasSubproperty rdf:resource="http://rdaregistry.info/Elements/u/P60376" />
  <reg:hasSubproperty rdf:resource="http://rdaregistry.info/Elements/u/P60406" />
  <reg:hasSubproperty rdf:resource="http://rdaregistry.info/Elements/u/P60421" />
  <reg:hasSubproperty rdf:resource="http://rdaregistry.info/Elements/u/P60441" />
  <reg:hasSubproperty rdf:resource="http://rdaregistry.info/Elements/u/P60449" />
  <reg:hasSubproperty rdf:resource="http://rdaregistry.info/Elements/u/P60450" />
  <reg:hasSubproperty rdf:resource="http://rdaregistry.info/Elements/u/P60451" />
  <reg:hasSubproperty rdf:resource="http://rdaregistry.info/Elements/u/P60455" />
  <reg:hasSubproperty rdf:resource="http://rdaregistry.info/Elements/u/P60456" />
  <reg:hasSubproperty rdf:resource="http://rdaregistry.info/Elements/u/P60457" />
  <reg:hasSubproperty rdf:resource="http://rdaregistry.info/Elements/u/P60458" />
  <reg:hasSubproperty rdf:resource="http://rdaregistry.info/Elements/u/P60459" />
  <reg:hasSubproperty rdf:resource="http://rdaregistry.info/Elements/u/P60460" />
  <reg:hasSubproperty rdf:resource="http://rdaregistry.info/Elements/u/P60461" />
  <reg:hasSubproperty rdf:resource="http://rdaregistry.info/Elements/u/P60462" />
  <reg:hasSubproperty rdf:resource="http://rdaregistry.info/Elements/u/P60464" />
  <reg:hasSubproperty rdf:resource="http://rdaregistry.info/Elements/u/P60466" />
  <reg:hasSubproperty rdf:resource="http://rdaregistry.info/Elements/u/P60467" />
  <reg:hasSubproperty rdf:resource="http://rdaregistry.info/Elements/i/P40023" />
  <reg:hasSubproperty rdf:resource="http://rdaregistry.info/Elements/m/P30079" />
  <reg:lexicalAlias rdf:resource="http://rdaregistry.info/Elements/u/otherAgentAssociatedWithResource.en" />
  <reg:hasSubproperty rdf:resource="http://rdaregistry.info/Elements/u/P60815" />
  <reg:hasSubproperty rdf:resource="http://rdaregistry.info/Elements/u/P60834" />
  <reg:hasSubproperty rdf:resource="http://rdaregistry.info/Elements/u/P60836" />
  <reg:hasSubproperty rdf:resource="http://rdaregistry.info/Elements/u/P60849" />
  <reg:hasSubproperty rdf:resource="http://rdaregistry.info/Elements/u/P60869" />
  <reg:hasSubproperty rdf:resource="http://rdaregistry.info/Elements/u/P60871" />
</owl:ObjectProperty>

<!-- Property: is other agent associated with resource of -->
<owl:ObjectProperty rdf:about="http://rdaregistry.info/Elements/u/P60602">
  <rdfs:isDefinedBy rdf:resource="http://rdaregistry.info/Elements/u/" />
  <reg:status rdf:resource="http://metadataregistry.org/uri/RegStatus/1001" />
  <reg:name xml:lang="en">otherAgentAssociatedWithResourceOf</reg:name>
  <rdfs:label xml:lang="en">is other agent associated with resource of</rdfs:label>
  <skos:definition xml:lang="en">Relates an agent other than a creator, custodian, owner, producer, publisher, distributor or manufacturer associated with a resource to a resource.</skos:definition>
  <rdf:type rdf:resource="http://www.w3.org/1999/02/22-rdf-syntax-ns#Property" />
  <owl:inverseOf rdf:resource="http://rdaregistry.info/Elements/u/P60374" />
  <reg:hasSubproperty rdf:resource="http://rdaregistry.info/Elements/u/P60002" />
  <reg:hasSubproperty rdf:resource="http://rdaregistry.info/Elements/u/P60003" />
  <reg:hasSubproperty rdf:resource="http://rdaregistry.info/Elements/u/P60004" />
  <reg:hasSubproperty rdf:resource="http://rdaregistry.info/Elements/u/P60005" />
  <reg:hasSubproperty rdf:resource="http://rdaregistry.info/Elements/u/P60015" />
  <reg:hasSubproperty rdf:resource="http://rdaregistry.info/Elements/u/P60032" />
  <reg:hasSubproperty rdf:resource="http://rdaregistry.info/Elements/u/P60601" />
  <reg:hasSubproperty rdf:resource="http://rdaregistry.info/Elements/u/P60603" />
  <reg:hasSubproperty rdf:resource="http://rdaregistry.info/Elements/u/P60604" />
  <reg:hasSubproperty rdf:resource="http://rdaregistry.info/Elements/u/P60634" />
  <reg:hasSubproperty rdf:resource="http://rdaregistry.info/Elements/u/P60650" />
  <reg:hasSubproperty rdf:resource="http://rdaregistry.info/Elements/u/P60668" />
  <reg:hasSubproperty rdf:resource="http://rdaregistry.info/Elements/u/P60673" />
  <reg:hasSubproperty rdf:resource="http://rdaregistry.info/Elements/u/P60674" />
  <reg:hasSubproperty rdf:resource="http://rdaregistry.info/Elements/u/P60675" />
  <reg:hasSubproperty rdf:resource="http://rdaregistry.info/Elements/u/P60678" />
  <reg:hasSubproperty rdf:resource="http://rdaregistry.info/Elements/u/P60689" />
  <reg:hasSubproperty rdf:resource="http://rdaregistry.info/Elements/u/P60690" />
  <reg:hasSubproperty rdf:resource="http://rdaregistry.info/Elements/u/P60691" />
  <reg:hasSubproperty rdf:resource="http://rdaregistry.info/Elements/u/P60692" />
  <reg:hasSubproperty rdf:resource="http://rdaregistry.info/Elements/u/P60693" />
  <reg:hasSubproperty rdf:resource="http://rdaregistry.info/Elements/u/P60695" />
  <reg:hasSubproperty rdf:resource="http://rdaregistry.info/Elements/u/P60696" />
  <reg:hasSubproperty rdf:resource="http://rdaregistry.info/Elements/u/P60698" />
  <reg:hasSubproperty rdf:resource="http://rdaregistry.info/Elements/u/P60700" />
  <reg:hasSubproperty rdf:resource="http://rdaregistry.info/Elements/u/P60702" />
  <reg:hasSubproperty rdf:resource="http://rdaregistry.info/Elements/u/P60703" />
  <reg:hasSubproperty rdf:resource="http://rdaregistry.info/Elements/a/P50131" />
  <reg:hasSubproperty rdf:resource="http://rdaregistry.info/Elements/a/P50181" />
  <reg:hasSubproperty rdf:resource="http://rdaregistry.info/Elements/a/P50182" />
  <reg:lexicalAlias rdf:resource="http://rdaregistry.info/Elements/u/otherAgentAssociatedWithResourceOf.en" />
  <reg:hasSubproperty rdf:resource="http://rdaregistry.info/Elements/u/P60816" />
  <reg:hasSubproperty rdf:resource="http://rdaregistry.info/Elements/u/P60835" />
  <reg:hasSubproperty rdf:resource="http://rdaregistry.info/Elements/u/P60837" />
  <reg:hasSubproperty rdf:resource="http://rdaregistry.info/Elements/u/P60850" />
  <reg:hasSubproperty rdf:resource="http://rdaregistry.info/Elements/u/P60870" />
  <reg:hasSubproperty rdf:resource="http://rdaregistry.info/Elements/u/P60872" />
</owl:ObjectProperty>

<!-- Property: has other designation associated with agent -->
<owl:ObjectProperty rdf:about="http://rdaregistry.info/Elements/u/P60370">
  <rdfs:isDefinedBy rdf:resource="http://rdaregistry.info/Elements/u/" />
  <reg:status rdf:resource="http://metadataregistry.org/uri/RegStatus/1001" />
  <reg:name xml:lang="en">otherDesignationAssociatedWithAgent</reg:name>
  <rdfs:label xml:lang="en">has other designation associated with agent</rdfs:label>
  <skos:definition xml:lang="en">Relates a resource to a word, phrase, or abbreviation indicating incorporation or legal status of an agent, or any term serving to differentiate a an agent from other agents, etc., or a term other than a title that is associated with an agents name.</skos:definition>
  <rdf:type rdf:resource="http://www.w3.org/1999/02/22-rdf-syntax-ns#Property" />
  <reg:hasSubproperty rdf:resource="http://rdaregistry.info/Elements/a/P50239" />
  <reg:hasSubproperty rdf:resource="http://rdaregistry.info/Elements/a/P50033" />
  <reg:hasSubproperty rdf:resource="http://rdaregistry.info/Elements/a/P50108" />
  <reg:lexicalAlias rdf:resource="http://rdaregistry.info/Elements/u/otherDesignationAssociatedWithAgent.en" />
</owl:ObjectProperty>

<!-- Property: has other details of cartographic content -->
<owl:ObjectProperty rdf:about="http://rdaregistry.info/Elements/u/P60498">
  <rdfs:isDefinedBy rdf:resource="http://rdaregistry.info/Elements/u/" />
  <reg:status rdf:resource="http://metadataregistry.org/uri/RegStatus/1001" />
  <reg:name xml:lang="en">otherDetailsOfCartographicContent</reg:name>
  <rdfs:label xml:lang="en">has other details of cartographic content</rdfs:label>
  <skos:definition xml:lang="en">Relates a resource to an indication of mathematical data and other features of the cartographic content of a resource not recorded in statements of scale, projection, and coordinates.</skos:definition>
  <rdf:type rdf:resource="http://www.w3.org/1999/02/22-rdf-syntax-ns#Property" />
  <reg:hasSubproperty rdf:resource="http://rdaregistry.info/Elements/e/P20210" />
  <reg:lexicalAlias rdf:resource="http://rdaregistry.info/Elements/u/otherDetailsOfCartographicContent.en" />
</owl:ObjectProperty>

<!-- Property: has other distinguishing characteristic of resource -->
<owl:ObjectProperty rdf:about="http://rdaregistry.info/Elements/u/P60054">
  <rdfs:isDefinedBy rdf:resource="http://rdaregistry.info/Elements/u/" />
  <reg:status rdf:resource="http://metadataregistry.org/uri/RegStatus/1001" />
  <reg:name xml:lang="en">otherDistinguishingCharacteristicOfResource</reg:name>
  <rdfs:label xml:lang="en">has other distinguishing characteristic of resource</rdfs:label>
  <skos:definition xml:lang="en">Relates a resource to a characteristic other than form of resource, date of resource, place of origin of a resource, content type, or language of resource serving to differentiate a resource from another resource with the same title or from a name of an agent.</skos:definition>
  <rdf:type rdf:resource="http://www.w3.org/1999/02/22-rdf-syntax-ns#Property" />
  <reg:hasSubproperty rdf:resource="http://rdaregistry.info/Elements/e/P20003" />
  <reg:lexicalAlias rdf:resource="http://rdaregistry.info/Elements/u/otherDistinguishingCharacteristicOfResource.en" />
</owl:ObjectProperty>

<!-- Property: has other title information -->
<owl:ObjectProperty rdf:about="http://rdaregistry.info/Elements/u/P60493">
  <rdfs:isDefinedBy rdf:resource="http://rdaregistry.info/Elements/u/" />
  <reg:status rdf:resource="http://metadataregistry.org/uri/RegStatus/1001" />
  <reg:name xml:lang="en">otherTitleInformation</reg:name>
  <rdfs:label xml:lang="en">has other title information</rdfs:label>
  <skos:definition xml:lang="en">Relates a resource to a word, character, or group of words or characters that appears in conjunction with, and is subordinate to, a title proper of a resource.</skos:definition>
  <rdf:type rdf:resource="http://www.w3.org/1999/02/22-rdf-syntax-ns#Property" />
  <rdfs:subPropertyOf rdf:resource="http://rdaregistry.info/Elements/u/P60369" />
  <reg:hasSubproperty rdf:resource="http://rdaregistry.info/Elements/m/P30142" />
  <reg:lexicalAlias rdf:resource="http://rdaregistry.info/Elements/u/otherTitleInformation.en" />
</owl:ObjectProperty>

<!-- Property: has other title information of series -->
<owl:ObjectProperty rdf:about="http://rdaregistry.info/Elements/u/P60494">
  <rdfs:isDefinedBy rdf:resource="http://rdaregistry.info/Elements/u/" />
  <reg:status rdf:resource="http://metadataregistry.org/uri/RegStatus/1001" />
  <reg:name xml:lang="en">otherTitleInformationOfSeries</reg:name>
  <rdfs:label xml:lang="en">has other title information of series</rdfs:label>
  <skos:definition xml:lang="en">Relates a resource to a word, character, or group of words or characters that appears in conjunction with, and is subordinate to, a title proper of a series.</skos:definition>
  <rdf:type rdf:resource="http://www.w3.org/1999/02/22-rdf-syntax-ns#Property" />
  <reg:hasSubproperty rdf:resource="http://rdaregistry.info/Elements/m/P30143" />
  <reg:lexicalAlias rdf:resource="http://rdaregistry.info/Elements/u/otherTitleInformationOfSeries.en" />
</owl:ObjectProperty>

<!-- Property: has other title information of subseries -->
<owl:ObjectProperty rdf:about="http://rdaregistry.info/Elements/u/P60495">
  <rdfs:isDefinedBy rdf:resource="http://rdaregistry.info/Elements/u/" />
  <reg:status rdf:resource="http://metadataregistry.org/uri/RegStatus/1001" />
  <reg:name xml:lang="en">otherTitleInformationOfSubseries</reg:name>
  <rdfs:label xml:lang="en">has other title information of subseries</rdfs:label>
  <skos:definition xml:lang="en">Relates a resource to a word, character, or group of words or characters that appears in conjunction with, and is subordinate to, a title proper of a subseries.</skos:definition>
  <rdf:type rdf:resource="http://www.w3.org/1999/02/22-rdf-syntax-ns#Property" />
  <reg:hasSubproperty rdf:resource="http://rdaregistry.info/Elements/m/P30144" />
  <reg:lexicalAlias rdf:resource="http://rdaregistry.info/Elements/u/otherTitleInformationOfSubseries.en" />
</owl:ObjectProperty>

<!-- Property: has owner -->
<owl:ObjectProperty rdf:about="http://rdaregistry.info/Elements/u/P60404">
  <rdfs:isDefinedBy rdf:resource="http://rdaregistry.info/Elements/u/" />
  <reg:status rdf:resource="http://metadataregistry.org/uri/RegStatus/1001" />
  <reg:name xml:lang="en">owner</reg:name>
  <rdfs:label xml:lang="en">has owner</rdfs:label>
  <skos:definition xml:lang="en">Relates a resource to an agent having legal possession of a resource.</skos:definition>
  <rdf:type rdf:resource="http://www.w3.org/1999/02/22-rdf-syntax-ns#Property" />
  <owl:inverseOf rdf:resource="http://rdaregistry.info/Elements/u/P60632" />
  <reg:hasSubproperty rdf:resource="http://rdaregistry.info/Elements/u/P60400" />
  <reg:hasSubproperty rdf:resource="http://rdaregistry.info/Elements/u/P60401" />
  <reg:hasSubproperty rdf:resource="http://rdaregistry.info/Elements/i/P40021" />
  <reg:lexicalAlias rdf:resource="http://rdaregistry.info/Elements/u/owner.en" />
</owl:ObjectProperty>

<!-- Property: is owner of -->
<owl:ObjectProperty rdf:about="http://rdaregistry.info/Elements/u/P60632">
  <rdfs:isDefinedBy rdf:resource="http://rdaregistry.info/Elements/u/" />
  <reg:status rdf:resource="http://metadataregistry.org/uri/RegStatus/1001" />
  <reg:name xml:lang="en">ownerOf</reg:name>
  <rdfs:label xml:lang="en">is owner of</rdfs:label>
  <skos:definition xml:lang="en">Relates an agent having legal possession of a resource to a resource.</skos:definition>
  <rdf:type rdf:resource="http://www.w3.org/1999/02/22-rdf-syntax-ns#Property" />
  <owl:inverseOf rdf:resource="http://rdaregistry.info/Elements/u/P60404" />
  <reg:hasSubproperty rdf:resource="http://rdaregistry.info/Elements/u/P60628" />
  <reg:hasSubproperty rdf:resource="http://rdaregistry.info/Elements/u/P60630" />
  <reg:hasSubproperty rdf:resource="http://rdaregistry.info/Elements/a/P50165" />
  <reg:lexicalAlias rdf:resource="http://rdaregistry.info/Elements/u/ownerOf.en" />
</owl:ObjectProperty>

<!-- Property: has panelist -->
<owl:ObjectProperty rdf:about="http://rdaregistry.info/Elements/u/P60149">
  <rdfs:isDefinedBy rdf:resource="http://rdaregistry.info/Elements/u/" />
  <reg:status rdf:resource="http://metadataregistry.org/uri/RegStatus/1001" />
  <reg:name xml:lang="en">panelist</reg:name>
  <rdfs:label xml:lang="en">has panelist</rdfs:label>
  <skos:definition xml:lang="en">Relates a resource to a performer contributing to a resource by participating in a program, often broadcast, where topics are discussed, usually with participation of experts in fields related to the discussion.</skos:definition>
  <rdf:type rdf:resource="http://www.w3.org/1999/02/22-rdf-syntax-ns#Property" />
  <rdfs:subPropertyOf rdf:resource="http://rdaregistry.info/Elements/u/P60387" />
  <owl:inverseOf rdf:resource="http://rdaregistry.info/Elements/u/P60024" />
  <reg:hasSubproperty rdf:resource="http://rdaregistry.info/Elements/e/P20019" />
  <reg:lexicalAlias rdf:resource="http://rdaregistry.info/Elements/u/panelist.en" />
</owl:ObjectProperty>

<!-- Property: is panelist of -->
<owl:ObjectProperty rdf:about="http://rdaregistry.info/Elements/u/P60024">
  <rdfs:isDefinedBy rdf:resource="http://rdaregistry.info/Elements/u/" />
  <reg:status rdf:resource="http://metadataregistry.org/uri/RegStatus/1001" />
  <reg:name xml:lang="en">panelistOf</reg:name>
  <rdfs:label xml:lang="en">is panelist of</rdfs:label>
  <skos:definition xml:lang="en">Relates a performer contributing to a resource by participating in a program, often broadcast, where topics are discussed, usually with participation of experts in fields related to the discussion to a resource.</skos:definition>
  <rdf:type rdf:resource="http://www.w3.org/1999/02/22-rdf-syntax-ns#Property" />
  <rdfs:subPropertyOf rdf:resource="http://rdaregistry.info/Elements/u/P60615" />
  <owl:inverseOf rdf:resource="http://rdaregistry.info/Elements/u/P60149" />
  <reg:hasSubproperty rdf:resource="http://rdaregistry.info/Elements/a/P50078" />
  <reg:lexicalAlias rdf:resource="http://rdaregistry.info/Elements/u/panelistOf.en" />
</owl:ObjectProperty>

<!-- Property: has papermaker -->
<owl:ObjectProperty rdf:about="http://rdaregistry.info/Elements/u/P60746">
  <rdfs:isDefinedBy rdf:resource="http://rdaregistry.info/Elements/u/" />
  <reg:status rdf:resource="http://metadataregistry.org/uri/RegStatus/1001" />
  <rdf:type rdf:resource="http://www.w3.org/1999/02/22-rdf-syntax-ns#Property" />
  <reg:name xml:lang="en">papermaker</reg:name>
  <rdfs:label xml:lang="en">has papermaker</rdfs:label>
  <reg:lexicalAlias rdf:resource="http://rdaregistry.info/Elements/u/papermaker.en" />
  <skos:definition xml:lang="en">Relates a resource to an agent responsible for the production of paper used to manufacture a resource.</skos:definition>
  <owl:inverseOf rdf:resource="http://rdaregistry.info/Elements/u/P60747" />
  <rdfs:subPropertyOf rdf:resource="http://rdaregistry.info/Elements/u/P60443" />
</owl:ObjectProperty>

<!-- Property: is papermaker of -->
<owl:ObjectProperty rdf:about="http://rdaregistry.info/Elements/u/P60747">
  <rdfs:isDefinedBy rdf:resource="http://rdaregistry.info/Elements/u/" />
  <reg:status rdf:resource="http://metadataregistry.org/uri/RegStatus/1001" />
  <rdf:type rdf:resource="http://www.w3.org/1999/02/22-rdf-syntax-ns#Property" />
  <reg:name xml:lang="en">papermakerOf</reg:name>
  <rdfs:label xml:lang="en">is papermaker of</rdfs:label>
  <reg:lexicalAlias rdf:resource="http://rdaregistry.info/Elements/u/papermakerOf.en" />
  <skos:definition xml:lang="en">Relates an agent responsible for the production of paper used to manufacture a resource to a resource.</skos:definition>
  <owl:inverseOf rdf:resource="http://rdaregistry.info/Elements/u/P60746" />
  <rdfs:subPropertyOf rdf:resource="http://rdaregistry.info/Elements/u/P60669" />
</owl:ObjectProperty>

<!-- Property: has parallel designation of edition -->
<owl:ObjectProperty rdf:about="http://rdaregistry.info/Elements/u/P60078">
  <rdfs:isDefinedBy rdf:resource="http://rdaregistry.info/Elements/u/" />
  <reg:status rdf:resource="http://metadataregistry.org/uri/RegStatus/1001" />
  <reg:name xml:lang="en">parallelDesignationOfEdition</reg:name>
  <rdfs:label xml:lang="en">has parallel designation of edition</rdfs:label>
  <skos:definition xml:lang="en">Relates a resource to a designation of edition in a language or script that differs from that recorded in a designation of edition element.</skos:definition>
  <rdf:type rdf:resource="http://www.w3.org/1999/02/22-rdf-syntax-ns#Property" />
  <reg:hasSubproperty rdf:resource="http://rdaregistry.info/Elements/m/P30013" />
  <reg:lexicalAlias rdf:resource="http://rdaregistry.info/Elements/u/parallelDesignationOfEdition.en" />
</owl:ObjectProperty>

<!-- Property: has parallel designation of named revision of edition -->
<owl:ObjectProperty rdf:about="http://rdaregistry.info/Elements/u/P60077">
  <rdfs:isDefinedBy rdf:resource="http://rdaregistry.info/Elements/u/" />
  <reg:status rdf:resource="http://metadataregistry.org/uri/RegStatus/1001" />
  <reg:name xml:lang="en">parallelDesignationOfNamedRevisionOfEdition</reg:name>
  <rdfs:label xml:lang="en">has parallel designation of named revision of edition</rdfs:label>
  <skos:definition xml:lang="en">Relates a resource to a designation of a named revision of an edition in a language or script that differs from that recorded in a designation of a named revision of an edition element.</skos:definition>
  <rdf:type rdf:resource="http://www.w3.org/1999/02/22-rdf-syntax-ns#Property" />
  <reg:hasSubproperty rdf:resource="http://rdaregistry.info/Elements/m/P30012" />
  <reg:lexicalAlias rdf:resource="http://rdaregistry.info/Elements/u/parallelDesignationOfNamedRevisionOfEdition.en" />
</owl:ObjectProperty>

<!-- Property: has parallel distributors name -->
<owl:ObjectProperty rdf:about="http://rdaregistry.info/Elements/u/P60087">
  <rdfs:isDefinedBy rdf:resource="http://rdaregistry.info/Elements/u/" />
  <reg:status rdf:resource="http://metadataregistry.org/uri/RegStatus/1001" />
  <reg:name xml:lang="en">parallelDistributorsName</reg:name>
  <rdfs:label xml:lang="en">has parallel distributors name</rdfs:label>
  <skos:definition xml:lang="en">Relates a resource to a distributor's name in a language or script that differs from that recorded in a distributor's name element.</skos:definition>
  <rdf:type rdf:resource="http://www.w3.org/1999/02/22-rdf-syntax-ns#Property" />
  <reg:hasSubproperty rdf:resource="http://rdaregistry.info/Elements/m/P30017" />
  <reg:lexicalAlias rdf:resource="http://rdaregistry.info/Elements/u/parallelDistributorsName.en" />
</owl:ObjectProperty>

<!-- Property: has parallel manufacturers name -->
<owl:ObjectProperty rdf:about="http://rdaregistry.info/Elements/u/P60108">
  <rdfs:isDefinedBy rdf:resource="http://rdaregistry.info/Elements/u/" />
  <reg:status rdf:resource="http://metadataregistry.org/uri/RegStatus/1001" />
  <reg:name xml:lang="en">parallelManufacturersName</reg:name>
  <rdfs:label xml:lang="en">has parallel manufacturers name</rdfs:label>
  <skos:definition xml:lang="en">Relates a resource to a manufacturer's name in a language or script that differs from that recorded in a manufacturer's name element.</skos:definition>
  <rdf:type rdf:resource="http://www.w3.org/1999/02/22-rdf-syntax-ns#Property" />
  <reg:hasSubproperty rdf:resource="http://rdaregistry.info/Elements/m/P30049" />
  <reg:lexicalAlias rdf:resource="http://rdaregistry.info/Elements/u/parallelManufacturersName.en" />
</owl:ObjectProperty>

<!-- Property: has parallel other title information -->
<owl:ObjectProperty rdf:about="http://rdaregistry.info/Elements/u/P60507">
  <rdfs:isDefinedBy rdf:resource="http://rdaregistry.info/Elements/u/" />
  <reg:status rdf:resource="http://metadataregistry.org/uri/RegStatus/1001" />
  <reg:name xml:lang="en">parallelOtherTitleInformation</reg:name>
  <rdfs:label xml:lang="en">has parallel other title information</rdfs:label>
  <skos:definition xml:lang="en">Relates a resource to an other title information in a language or script that differs from that recorded in an other title information element.</skos:definition>
  <rdf:type rdf:resource="http://www.w3.org/1999/02/22-rdf-syntax-ns#Property" />
  <rdfs:subPropertyOf rdf:resource="http://rdaregistry.info/Elements/u/P60369" />
  <reg:hasSubproperty rdf:resource="http://rdaregistry.info/Elements/m/P30151" />
  <reg:lexicalAlias rdf:resource="http://rdaregistry.info/Elements/u/parallelOtherTitleInformation.en" />
</owl:ObjectProperty>

<!-- Property: has parallel other title information of series -->
<owl:ObjectProperty rdf:about="http://rdaregistry.info/Elements/u/P60508">
  <rdfs:isDefinedBy rdf:resource="http://rdaregistry.info/Elements/u/" />
  <reg:status rdf:resource="http://metadataregistry.org/uri/RegStatus/1001" />
  <reg:name xml:lang="en">parallelOtherTitleInformationOfSeries</reg:name>
  <rdfs:label xml:lang="en">has parallel other title information of series</rdfs:label>
  <skos:definition xml:lang="en">Relates a resource to an other title information of a series in a language or script that differs from that recorded in an other title information of series element.</skos:definition>
  <rdf:type rdf:resource="http://www.w3.org/1999/02/22-rdf-syntax-ns#Property" />
  <reg:hasSubproperty rdf:resource="http://rdaregistry.info/Elements/m/P30152" />
  <reg:lexicalAlias rdf:resource="http://rdaregistry.info/Elements/u/parallelOtherTitleInformationOfSeries.en" />
</owl:ObjectProperty>

<!-- Property: has parallel other title information of subseries -->
<owl:ObjectProperty rdf:about="http://rdaregistry.info/Elements/u/P60509">
  <rdfs:isDefinedBy rdf:resource="http://rdaregistry.info/Elements/u/" />
  <reg:status rdf:resource="http://metadataregistry.org/uri/RegStatus/1001" />
  <reg:name xml:lang="en">parallelOtherTitleInformationOfSubseries</reg:name>
  <rdfs:label xml:lang="en">has parallel other title information of subseries</rdfs:label>
  <skos:definition xml:lang="en">Relates a resource to an other title information of a subseries in a language or script that differs from that recorded in an other title information of subseries element.</skos:definition>
  <rdf:type rdf:resource="http://www.w3.org/1999/02/22-rdf-syntax-ns#Property" />
  <reg:hasSubproperty rdf:resource="http://rdaregistry.info/Elements/m/P30153" />
  <reg:lexicalAlias rdf:resource="http://rdaregistry.info/Elements/u/parallelOtherTitleInformationOfSubseries.en" />
</owl:ObjectProperty>

<!-- Property: has parallel place of distribution -->
<owl:ObjectProperty rdf:about="http://rdaregistry.info/Elements/u/P60164">
  <rdfs:isDefinedBy rdf:resource="http://rdaregistry.info/Elements/u/" />
  <reg:status rdf:resource="http://metadataregistry.org/uri/RegStatus/1001" />
  <reg:name xml:lang="en">parallelPlaceOfDistribution</reg:name>
  <rdfs:label xml:lang="en">has parallel place of distribution</rdfs:label>
  <skos:definition xml:lang="en">Relates a resource to a place of distribution in a language or script that differs from that recorded in a place of distribution element.</skos:definition>
  <rdf:type rdf:resource="http://www.w3.org/1999/02/22-rdf-syntax-ns#Property" />
  <reg:hasSubproperty rdf:resource="http://rdaregistry.info/Elements/m/P30089" />
  <reg:lexicalAlias rdf:resource="http://rdaregistry.info/Elements/u/parallelPlaceOfDistribution.en" />
</owl:ObjectProperty>

<!-- Property: has parallel place of manufacture -->
<owl:ObjectProperty rdf:about="http://rdaregistry.info/Elements/u/P60165">
  <rdfs:isDefinedBy rdf:resource="http://rdaregistry.info/Elements/u/" />
  <reg:status rdf:resource="http://metadataregistry.org/uri/RegStatus/1001" />
  <reg:name xml:lang="en">parallelPlaceOfManufacture</reg:name>
  <rdfs:label xml:lang="en">has parallel place of manufacture</rdfs:label>
  <skos:definition xml:lang="en">Relates a resource to a place of manufacture in a language or script that differs from that recorded in a place of manufacture element.</skos:definition>
  <rdf:type rdf:resource="http://www.w3.org/1999/02/22-rdf-syntax-ns#Property" />
  <reg:hasSubproperty rdf:resource="http://rdaregistry.info/Elements/m/P30090" />
  <reg:lexicalAlias rdf:resource="http://rdaregistry.info/Elements/u/parallelPlaceOfManufacture.en" />
</owl:ObjectProperty>

<!-- Property: has parallel place of production -->
<owl:ObjectProperty rdf:about="http://rdaregistry.info/Elements/u/P60166">
  <rdfs:isDefinedBy rdf:resource="http://rdaregistry.info/Elements/u/" />
  <reg:status rdf:resource="http://metadataregistry.org/uri/RegStatus/1001" />
  <reg:name xml:lang="en">parallelPlaceOfProduction</reg:name>
  <rdfs:label xml:lang="en">has parallel place of production</rdfs:label>
  <skos:definition xml:lang="en">Relates a resource to a place of production in a language or script that differs from that recorded in a place of production element.</skos:definition>
  <rdf:type rdf:resource="http://www.w3.org/1999/02/22-rdf-syntax-ns#Property" />
  <reg:hasSubproperty rdf:resource="http://rdaregistry.info/Elements/m/P30091" />
  <reg:lexicalAlias rdf:resource="http://rdaregistry.info/Elements/u/parallelPlaceOfProduction.en" />
</owl:ObjectProperty>

<!-- Property: has parallel place of publication -->
<owl:ObjectProperty rdf:about="http://rdaregistry.info/Elements/u/P60167">
  <rdfs:isDefinedBy rdf:resource="http://rdaregistry.info/Elements/u/" />
  <reg:status rdf:resource="http://metadataregistry.org/uri/RegStatus/1001" />
  <reg:name xml:lang="en">parallelPlaceOfPublication</reg:name>
  <rdfs:label xml:lang="en">has parallel place of publication</rdfs:label>
  <skos:definition xml:lang="en">Relates a resource to a place of publication in a language or script that differs from that recorded in a place of publication element.</skos:definition>
  <rdf:type rdf:resource="http://www.w3.org/1999/02/22-rdf-syntax-ns#Property" />
  <reg:hasSubproperty rdf:resource="http://rdaregistry.info/Elements/m/P30092" />
  <reg:lexicalAlias rdf:resource="http://rdaregistry.info/Elements/u/parallelPlaceOfPublication.en" />
</owl:ObjectProperty>

<!-- Property: has parallel producers name -->
<owl:ObjectProperty rdf:about="http://rdaregistry.info/Elements/u/P60172">
  <rdfs:isDefinedBy rdf:resource="http://rdaregistry.info/Elements/u/" />
  <reg:status rdf:resource="http://metadataregistry.org/uri/RegStatus/1001" />
  <reg:name xml:lang="en">parallelProducersName</reg:name>
  <rdfs:label xml:lang="en">has parallel producers name</rdfs:label>
  <skos:definition xml:lang="en">Relates a resource to a producer's name in a language or script that differs from that recorded in a producer's name element.</skos:definition>
  <rdf:type rdf:resource="http://www.w3.org/1999/02/22-rdf-syntax-ns#Property" />
  <reg:hasSubproperty rdf:resource="http://rdaregistry.info/Elements/m/P30094" />
  <reg:lexicalAlias rdf:resource="http://rdaregistry.info/Elements/u/parallelProducersName.en" />
</owl:ObjectProperty>

<!-- Property: has parallel publishers name -->
<owl:ObjectProperty rdf:about="http://rdaregistry.info/Elements/u/P60173">
  <rdfs:isDefinedBy rdf:resource="http://rdaregistry.info/Elements/u/" />
  <reg:status rdf:resource="http://metadataregistry.org/uri/RegStatus/1001" />
  <reg:name xml:lang="en">parallelPublishersName</reg:name>
  <rdfs:label xml:lang="en">has parallel publishers name</rdfs:label>
  <skos:definition xml:lang="en">Relates a resource to a publisher's name in a language or script that differs from that recorded in a publisher's name element.</skos:definition>
  <rdf:type rdf:resource="http://www.w3.org/1999/02/22-rdf-syntax-ns#Property" />
  <reg:hasSubproperty rdf:resource="http://rdaregistry.info/Elements/m/P30095" />
  <reg:lexicalAlias rdf:resource="http://rdaregistry.info/Elements/u/parallelPublishersName.en" />
</owl:ObjectProperty>

<!-- Property: has parallel statement of responsibility relating to edition -->
<owl:ObjectProperty rdf:about="http://rdaregistry.info/Elements/u/P60337">
  <rdfs:isDefinedBy rdf:resource="http://rdaregistry.info/Elements/u/" />
  <reg:status rdf:resource="http://metadataregistry.org/uri/RegStatus/1001" />
  <reg:name xml:lang="en">parallelStatementOfResponsibilityRelatingToEdition</reg:name>
  <rdfs:label xml:lang="en">has parallel statement of responsibility relating to edition</rdfs:label>
  <skos:definition xml:lang="en">Relates a resource to a statement of responsibility relating to an edition in a language or script that differs from that recorded in a statement of responsibility relating to an edition element.</skos:definition>
  <rdf:type rdf:resource="http://www.w3.org/1999/02/22-rdf-syntax-ns#Property" />
  <reg:hasSubproperty rdf:resource="http://rdaregistry.info/Elements/m/P30115" />
  <reg:lexicalAlias rdf:resource="http://rdaregistry.info/Elements/u/parallelStatementOfResponsibilityRelatingToEdition.en" />
</owl:ObjectProperty>

<!-- Property: has parallel statement of responsibility relating to named revision of edition -->
<owl:ObjectProperty rdf:about="http://rdaregistry.info/Elements/u/P60334">
  <rdfs:isDefinedBy rdf:resource="http://rdaregistry.info/Elements/u/" />
  <reg:status rdf:resource="http://metadataregistry.org/uri/RegStatus/1001" />
  <reg:name xml:lang="en">parallelStatementOfResponsibilityRelatingToNamedRevisionOfEdition</reg:name>
  <rdfs:label xml:lang="en">has parallel statement of responsibility relating to named revision of edition</rdfs:label>
  <skos:definition xml:lang="en">Relates a resource to a statement of responsibility relating to a named revision of an edition in a language or script that differs from that recorded in a statement of responsibility relating to a named revision of an edition element.</skos:definition>
  <rdf:type rdf:resource="http://www.w3.org/1999/02/22-rdf-syntax-ns#Property" />
  <reg:hasSubproperty rdf:resource="http://rdaregistry.info/Elements/m/P30112" />
  <reg:lexicalAlias rdf:resource="http://rdaregistry.info/Elements/u/parallelStatementOfResponsibilityRelatingToNamedRevisionOfEdition.en" />
</owl:ObjectProperty>

<!-- Property: has parallel statement of responsibility relating to series -->
<owl:ObjectProperty rdf:about="http://rdaregistry.info/Elements/u/P60335">
  <rdfs:isDefinedBy rdf:resource="http://rdaregistry.info/Elements/u/" />
  <reg:status rdf:resource="http://metadataregistry.org/uri/RegStatus/1001" />
  <reg:name xml:lang="en">parallelStatementOfResponsibilityRelatingToSeries</reg:name>
  <rdfs:label xml:lang="en">has parallel statement of responsibility relating to series</rdfs:label>
  <skos:definition xml:lang="en">Relates a resource to a statement of responsibility relating to series in a language or script that differs from that recorded in a statement of responsibility relating to series element.</skos:definition>
  <rdf:type rdf:resource="http://www.w3.org/1999/02/22-rdf-syntax-ns#Property" />
  <reg:hasSubproperty rdf:resource="http://rdaregistry.info/Elements/m/P30113" />
  <reg:lexicalAlias rdf:resource="http://rdaregistry.info/Elements/u/parallelStatementOfResponsibilityRelatingToSeries.en" />
</owl:ObjectProperty>

<!-- Property: has parallel statement of responsibility relating to subseries -->
<owl:ObjectProperty rdf:about="http://rdaregistry.info/Elements/u/P60336">
  <rdfs:isDefinedBy rdf:resource="http://rdaregistry.info/Elements/u/" />
  <reg:status rdf:resource="http://metadataregistry.org/uri/RegStatus/1001" />
  <reg:name xml:lang="en">parallelStatementOfResponsibilityRelatingToSubseries</reg:name>
  <rdfs:label xml:lang="en">has parallel statement of responsibility relating to subseries</rdfs:label>
  <skos:definition xml:lang="en">Relates a resource to a statement of responsibility relating to subseries in a language or script that differs from that recorded in a statement of responsibility relating to subseries element.</skos:definition>
  <rdf:type rdf:resource="http://www.w3.org/1999/02/22-rdf-syntax-ns#Property" />
  <reg:hasSubproperty rdf:resource="http://rdaregistry.info/Elements/m/P30114" />
  <reg:lexicalAlias rdf:resource="http://rdaregistry.info/Elements/u/parallelStatementOfResponsibilityRelatingToSubseries.en" />
</owl:ObjectProperty>

<!-- Property: has parallel statement of responsibility relating to title proper -->
<owl:ObjectProperty rdf:about="http://rdaregistry.info/Elements/u/P60338">
  <rdfs:isDefinedBy rdf:resource="http://rdaregistry.info/Elements/u/" />
  <reg:status rdf:resource="http://metadataregistry.org/uri/RegStatus/1001" />
  <reg:name xml:lang="en">parallelStatementOfResponsibilityRelatingToTitleProper</reg:name>
  <rdfs:label xml:lang="en">has parallel statement of responsibility relating to title proper</rdfs:label>
  <skos:definition xml:lang="en">Relates a resource to a statement of responsibility relating to title proper in a language or script that differs from that recorded in a statement of responsibility relating to title proper element.</skos:definition>
  <rdf:type rdf:resource="http://www.w3.org/1999/02/22-rdf-syntax-ns#Property" />
  <rdfs:subPropertyOf rdf:resource="http://rdaregistry.info/Elements/u/P60339" />
  <reg:hasSubproperty rdf:resource="http://rdaregistry.info/Elements/m/P30116" />
  <reg:lexicalAlias rdf:resource="http://rdaregistry.info/Elements/u/parallelStatementOfResponsibilityRelatingToTitleProper.en" />
</owl:ObjectProperty>

<!-- Property: has parallel title proper -->
<owl:ObjectProperty rdf:about="http://rdaregistry.info/Elements/u/P60589">
  <rdfs:isDefinedBy rdf:resource="http://rdaregistry.info/Elements/u/" />
  <reg:status rdf:resource="http://metadataregistry.org/uri/RegStatus/1001" />
  <reg:name xml:lang="en">parallelTitleProper</reg:name>
  <rdfs:label xml:lang="en">has parallel title proper</rdfs:label>
  <skos:definition xml:lang="en">Relates a resource to a title proper in another language or script.</skos:definition>
  <rdf:type rdf:resource="http://www.w3.org/1999/02/22-rdf-syntax-ns#Property" />
  <rdfs:subPropertyOf rdf:resource="http://rdaregistry.info/Elements/u/P60369" />
  <reg:hasSubproperty rdf:resource="http://rdaregistry.info/Elements/m/P30203" />
  <reg:lexicalAlias rdf:resource="http://rdaregistry.info/Elements/u/parallelTitleProper.en" />
  <skos:scopeNote xml:lang="en">An alternative title in another language and/or script is treated as part of the parallel title proper.</skos:scopeNote>
</owl:ObjectProperty>

<!-- Property: has parallel title proper of series -->
<owl:ObjectProperty rdf:about="http://rdaregistry.info/Elements/u/P60590">
  <rdfs:isDefinedBy rdf:resource="http://rdaregistry.info/Elements/u/" />
  <reg:status rdf:resource="http://metadataregistry.org/uri/RegStatus/1001" />
  <reg:name xml:lang="en">parallelTitleProperOfSeries</reg:name>
  <rdfs:label xml:lang="en">has parallel title proper of series</rdfs:label>
  <skos:definition xml:lang="en">Relates a resource to a title proper of a series in another language or script.</skos:definition>
  <rdf:type rdf:resource="http://www.w3.org/1999/02/22-rdf-syntax-ns#Property" />
  <reg:hasSubproperty rdf:resource="http://rdaregistry.info/Elements/m/P30204" />
  <reg:lexicalAlias rdf:resource="http://rdaregistry.info/Elements/u/parallelTitleProperOfSeries.en" />
</owl:ObjectProperty>

<!-- Property: has parallel title proper of subseries -->
<owl:ObjectProperty rdf:about="http://rdaregistry.info/Elements/u/P60591">
  <rdfs:isDefinedBy rdf:resource="http://rdaregistry.info/Elements/u/" />
  <reg:status rdf:resource="http://metadataregistry.org/uri/RegStatus/1001" />
  <reg:name xml:lang="en">parallelTitleProperOfSubseries</reg:name>
  <rdfs:label xml:lang="en">has parallel title proper of subseries</rdfs:label>
  <skos:definition xml:lang="en">Relates a resource to a title proper of a subseries in another language or script.</skos:definition>
  <rdf:type rdf:resource="http://www.w3.org/1999/02/22-rdf-syntax-ns#Property" />
  <reg:hasSubproperty rdf:resource="http://rdaregistry.info/Elements/m/P30205" />
  <reg:lexicalAlias rdf:resource="http://rdaregistry.info/Elements/u/parallelTitleProperOfSubseries.en" />
</owl:ObjectProperty>

<!-- Property: is paraphrased as -->
<owl:ObjectProperty rdf:about="http://rdaregistry.info/Elements/u/P60273">
  <rdfs:isDefinedBy rdf:resource="http://rdaregistry.info/Elements/u/" />
  <reg:status rdf:resource="http://metadataregistry.org/uri/RegStatus/1001" />
  <reg:name xml:lang="en">paraphrasedAs</reg:name>
  <rdfs:label xml:lang="en">is paraphrased as</rdfs:label>
  <skos:definition xml:lang="en">Relates a resource to a resource that restates a content of a source resource in a different form.</skos:definition>
  <rdf:type rdf:resource="http://www.w3.org/1999/02/22-rdf-syntax-ns#Property" />
  <rdfs:subPropertyOf rdf:resource="http://rdaregistry.info/Elements/u/P60250" />
  <owl:inverseOf rdf:resource="http://rdaregistry.info/Elements/u/P60296" />
  <reg:hasSubproperty rdf:resource="http://rdaregistry.info/Elements/e/P20164" />
  <reg:lexicalAlias rdf:resource="http://rdaregistry.info/Elements/u/paraphrasedAs.en" />
</owl:ObjectProperty>

<!-- Property: is paraphrase of -->
<owl:ObjectProperty rdf:about="http://rdaregistry.info/Elements/u/P60296">
  <rdfs:isDefinedBy rdf:resource="http://rdaregistry.info/Elements/u/" />
  <reg:status rdf:resource="http://metadataregistry.org/uri/RegStatus/1001" />
  <reg:name xml:lang="en">paraphraseOf</reg:name>
  <rdfs:label xml:lang="en">is paraphrase of</rdfs:label>
  <skos:definition xml:lang="en">Relates a resource to a resource used as a basis for a paraphrase, i.e., a restating of the content of the source resource in a different form.</skos:definition>
  <rdf:type rdf:resource="http://www.w3.org/1999/02/22-rdf-syntax-ns#Property" />
  <rdfs:subPropertyOf rdf:resource="http://rdaregistry.info/Elements/u/P60305" />
  <owl:inverseOf rdf:resource="http://rdaregistry.info/Elements/u/P60273" />
  <reg:hasSubproperty rdf:resource="http://rdaregistry.info/Elements/e/P20186" />
  <reg:lexicalAlias rdf:resource="http://rdaregistry.info/Elements/u/paraphraseOf.en" />
</owl:ObjectProperty>

<!-- Property: is parodied as -->
<owl:ObjectProperty rdf:about="http://rdaregistry.info/Elements/u/P60246">
  <rdfs:isDefinedBy rdf:resource="http://rdaregistry.info/Elements/u/" />
  <reg:status rdf:resource="http://metadataregistry.org/uri/RegStatus/1001" />
  <reg:name xml:lang="en">parodiedAs</reg:name>
  <rdfs:label xml:lang="en">is parodied as</rdfs:label>
  <skos:definition xml:lang="en">Relates a resource to a resource that imitates the style or content of the source resource for comic effect.</skos:definition>
  <rdf:type rdf:resource="http://www.w3.org/1999/02/22-rdf-syntax-ns#Property" />
  <rdfs:subPropertyOf rdf:resource="http://rdaregistry.info/Elements/u/P60214" />
  <owl:inverseOf rdf:resource="http://rdaregistry.info/Elements/u/P60312" />
  <reg:hasSubproperty rdf:resource="http://rdaregistry.info/Elements/e/P20142" />
  <reg:lexicalAlias rdf:resource="http://rdaregistry.info/Elements/u/parodiedAs.en" />
</owl:ObjectProperty>

<!-- Property: is parody of -->
<owl:ObjectProperty rdf:about="http://rdaregistry.info/Elements/u/P60312">
  <rdfs:isDefinedBy rdf:resource="http://rdaregistry.info/Elements/u/" />
  <reg:status rdf:resource="http://metadataregistry.org/uri/RegStatus/1001" />
  <reg:name xml:lang="en">parodyOf</reg:name>
  <rdfs:label xml:lang="en">is parody of</rdfs:label>
  <skos:definition xml:lang="en">Relates a resource to a resource whose style or content is imitated for comic effect.</skos:definition>
  <rdf:type rdf:resource="http://www.w3.org/1999/02/22-rdf-syntax-ns#Property" />
  <rdfs:subPropertyOf rdf:resource="http://rdaregistry.info/Elements/u/P60311" />
  <owl:inverseOf rdf:resource="http://rdaregistry.info/Elements/u/P60246" />
  <reg:hasSubproperty rdf:resource="http://rdaregistry.info/Elements/e/P20196" />
  <reg:lexicalAlias rdf:resource="http://rdaregistry.info/Elements/u/parodyOf.en" />
</owl:ObjectProperty>

<!-- Property: has participant in treaty -->
<owl:ObjectProperty rdf:about="http://rdaregistry.info/Elements/u/P60834">
  <rdfs:isDefinedBy rdf:resource="http://rdaregistry.info/Elements/u/" />
  <reg:status rdf:resource="http://metadataregistry.org/uri/RegStatus/1001" />
  <rdf:type rdf:resource="http://www.w3.org/1999/02/22-rdf-syntax-ns#Property" />
  <reg:name xml:lang="en">participantInTreaty</reg:name>
  <rdfs:label xml:lang="en">has participant in treaty</rdfs:label>
  <reg:lexicalAlias rdf:resource="http://rdaregistry.info/Elements/u/participantInTreaty.en" />
  <skos:definition xml:lang="en">Relates a resource to a government, international intergovernmental body, or other agent that has signed, ratified, or acceded to a treaty.</skos:definition>
  <owl:inverseOf rdf:resource="http://rdaregistry.info/Elements/u/P60835" />
  <rdfs:subPropertyOf rdf:resource="http://rdaregistry.info/Elements/u/P60374" />
</owl:ObjectProperty>

<!-- Property: is participant in treaty of -->
<owl:ObjectProperty rdf:about="http://rdaregistry.info/Elements/u/P60835">
  <rdfs:isDefinedBy rdf:resource="http://rdaregistry.info/Elements/u/" />
  <reg:status rdf:resource="http://metadataregistry.org/uri/RegStatus/1001" />
  <rdf:type rdf:resource="http://www.w3.org/1999/02/22-rdf-syntax-ns#Property" />
  <reg:name xml:lang="en">participantInTreatyOf</reg:name>
  <rdfs:label xml:lang="en">is participant in treaty of</rdfs:label>
  <reg:lexicalAlias rdf:resource="http://rdaregistry.info/Elements/u/participantInTreatyOf.en" />
  <skos:definition xml:lang="en">Relates a government, international intergovernmental body, or other agent that has signed, ratified, or acceded to a treaty to a resource.</skos:definition>
  <owl:inverseOf rdf:resource="http://rdaregistry.info/Elements/u/P60834" />
  <reg:hasSubproperty rdf:resource="http://rdaregistry.info/Elements/a/P50264" />
  <rdfs:subPropertyOf rdf:resource="http://rdaregistry.info/Elements/u/P60602" />
</owl:ObjectProperty>

<!-- Property: has partner -->
<owl:ObjectProperty rdf:about="http://rdaregistry.info/Elements/u/P60860">
  <rdfs:isDefinedBy rdf:resource="http://rdaregistry.info/Elements/u/" />
  <reg:status rdf:resource="http://metadataregistry.org/uri/RegStatus/1001" />
  <rdf:type rdf:resource="http://www.w3.org/1999/02/22-rdf-syntax-ns#Property" />
  <reg:name xml:lang="en">partner</reg:name>
  <rdfs:label xml:lang="en">has partner</rdfs:label>
  <reg:lexicalAlias rdf:resource="http://rdaregistry.info/Elements/u/partner.en" />
  <skos:definition xml:lang="en">Relates an agent to a colleague working with another agent in an activity of common interest, most often a business partnership.</skos:definition>
  <owl:inverseOf rdf:resource="http://rdaregistry.info/Elements/u/P60860" />
  <reg:hasSubproperty rdf:resource="http://rdaregistry.info/Elements/a/P50278" />
  <rdfs:subPropertyOf rdf:resource="http://rdaregistry.info/Elements/u/P60853" />
</owl:ObjectProperty>

<!-- Property: has performer -->
<owl:ObjectProperty rdf:about="http://rdaregistry.info/Elements/u/P60387">
  <rdfs:isDefinedBy rdf:resource="http://rdaregistry.info/Elements/u/" />
  <reg:status rdf:resource="http://metadataregistry.org/uri/RegStatus/1001" />
  <reg:name xml:lang="en">performer</reg:name>
  <rdfs:label xml:lang="en">has performer</rdfs:label>
  <skos:definition xml:lang="en">Relates a resource to an agent contributing to a resource by performing music, acting, dancing, speaking, etc., often in a musical or dramatic presentation, etc.</skos:definition>
  <rdf:type rdf:resource="http://www.w3.org/1999/02/22-rdf-syntax-ns#Property" />
  <rdfs:subPropertyOf rdf:resource="http://rdaregistry.info/Elements/u/P60398" />
  <owl:inverseOf rdf:resource="http://rdaregistry.info/Elements/u/P60615" />
  <reg:hasSubproperty rdf:resource="http://rdaregistry.info/Elements/u/P60141" />
  <reg:hasSubproperty rdf:resource="http://rdaregistry.info/Elements/u/P60142" />
  <reg:hasSubproperty rdf:resource="http://rdaregistry.info/Elements/u/P60143" />
  <reg:hasSubproperty rdf:resource="http://rdaregistry.info/Elements/u/P60144" />
  <reg:hasSubproperty rdf:resource="http://rdaregistry.info/Elements/u/P60145" />
  <reg:hasSubproperty rdf:resource="http://rdaregistry.info/Elements/u/P60146" />
  <reg:hasSubproperty rdf:resource="http://rdaregistry.info/Elements/u/P60147" />
  <reg:hasSubproperty rdf:resource="http://rdaregistry.info/Elements/u/P60148" />
  <reg:hasSubproperty rdf:resource="http://rdaregistry.info/Elements/u/P60149" />
  <reg:hasSubproperty rdf:resource="http://rdaregistry.info/Elements/u/P60150" />
  <reg:hasSubproperty rdf:resource="http://rdaregistry.info/Elements/u/P60151" />
  <reg:hasSubproperty rdf:resource="http://rdaregistry.info/Elements/u/P60153" />
  <reg:hasSubproperty rdf:resource="http://rdaregistry.info/Elements/u/P60154" />
  <reg:hasSubproperty rdf:resource="http://rdaregistry.info/Elements/u/P60155" />
  <reg:hasSubproperty rdf:resource="http://rdaregistry.info/Elements/u/P60156" />
  <reg:hasSubproperty rdf:resource="http://rdaregistry.info/Elements/e/P20039" />
  <reg:lexicalAlias rdf:resource="http://rdaregistry.info/Elements/u/performer.en" />
</owl:ObjectProperty>

<!-- Property: DEPRECATED -->
<owl:ObjectProperty rdf:about="http://rdaregistry.info/Elements/u/P60442">
  <rdfs:isDefinedBy rdf:resource="http://rdaregistry.info/Elements/u/" />
  <reg:status rdf:resource="http://metadataregistry.org/uri/RegStatus/1008" />
</owl:ObjectProperty>

<!-- Property: is performer of -->
<owl:ObjectProperty rdf:about="http://rdaregistry.info/Elements/u/P60615">
  <rdfs:isDefinedBy rdf:resource="http://rdaregistry.info/Elements/u/" />
  <reg:status rdf:resource="http://metadataregistry.org/uri/RegStatus/1001" />
  <reg:name xml:lang="en">performerOf</reg:name>
  <rdfs:label xml:lang="en">is performer of</rdfs:label>
  <skos:definition xml:lang="en">Relates an agent contributing to a resource by performing music, acting, dancing, speaking, etc., often in a musical or dramatic presentation, etc. to a resource.</skos:definition>
  <rdf:type rdf:resource="http://www.w3.org/1999/02/22-rdf-syntax-ns#Property" />
  <rdfs:subPropertyOf rdf:resource="http://rdaregistry.info/Elements/u/P60626" />
  <owl:inverseOf rdf:resource="http://rdaregistry.info/Elements/u/P60387" />
  <reg:hasSubproperty rdf:resource="http://rdaregistry.info/Elements/u/P60016" />
  <reg:hasSubproperty rdf:resource="http://rdaregistry.info/Elements/u/P60017" />
  <reg:hasSubproperty rdf:resource="http://rdaregistry.info/Elements/u/P60018" />
  <reg:hasSubproperty rdf:resource="http://rdaregistry.info/Elements/u/P60019" />
  <reg:hasSubproperty rdf:resource="http://rdaregistry.info/Elements/u/P60020" />
  <reg:hasSubproperty rdf:resource="http://rdaregistry.info/Elements/u/P60021" />
  <reg:hasSubproperty rdf:resource="http://rdaregistry.info/Elements/u/P60022" />
  <reg:hasSubproperty rdf:resource="http://rdaregistry.info/Elements/u/P60023" />
  <reg:hasSubproperty rdf:resource="http://rdaregistry.info/Elements/u/P60024" />
  <reg:hasSubproperty rdf:resource="http://rdaregistry.info/Elements/u/P60025" />
  <reg:hasSubproperty rdf:resource="http://rdaregistry.info/Elements/u/P60026" />
  <reg:hasSubproperty rdf:resource="http://rdaregistry.info/Elements/u/P60028" />
  <reg:hasSubproperty rdf:resource="http://rdaregistry.info/Elements/u/P60029" />
  <reg:hasSubproperty rdf:resource="http://rdaregistry.info/Elements/u/P60030" />
  <reg:hasSubproperty rdf:resource="http://rdaregistry.info/Elements/u/P60031" />
  <reg:hasSubproperty rdf:resource="http://rdaregistry.info/Elements/a/P50147" />
  <reg:lexicalAlias rdf:resource="http://rdaregistry.info/Elements/u/performerOf.en" />
</owl:ObjectProperty>

<!-- Property: has period of activity of agent -->
<owl:ObjectProperty rdf:about="http://rdaregistry.info/Elements/u/P60076">
  <rdfs:isDefinedBy rdf:resource="http://rdaregistry.info/Elements/u/" />
  <reg:status rdf:resource="http://metadataregistry.org/uri/RegStatus/1001" />
  <reg:name xml:lang="en">periodOfActivityOfAgent</reg:name>
  <rdfs:label xml:lang="en">has period of activity of agent</rdfs:label>
  <skos:definition xml:lang="en">Relates a resource to a date or range of dates indicative of a period in which an agent was active in its primary field of endeavour.</skos:definition>
  <rdf:type rdf:resource="http://www.w3.org/1999/02/22-rdf-syntax-ns#Property" />
  <rdfs:subPropertyOf rdf:resource="http://rdaregistry.info/Elements/u/P60324" />
  <reg:hasSubproperty rdf:resource="http://rdaregistry.info/Elements/a/P50098" />
  <reg:hasSubproperty rdf:resource="http://rdaregistry.info/Elements/a/P50236" />
  <reg:lexicalAlias rdf:resource="http://rdaregistry.info/Elements/u/periodOfActivityOfAgent.en" />
</owl:ObjectProperty>

<!-- Property: has photographer -->
<owl:ObjectProperty rdf:about="http://rdaregistry.info/Elements/u/P60429">
  <rdfs:isDefinedBy rdf:resource="http://rdaregistry.info/Elements/u/" />
  <reg:status rdf:resource="http://metadataregistry.org/uri/RegStatus/1001" />
  <reg:name xml:lang="en">photographer</reg:name>
  <rdfs:label xml:lang="en">has photographer</rdfs:label>
  <skos:definition xml:lang="en">Relates a resource to an agent responsible for creating a photographic resource.</skos:definition>
  <rdf:type rdf:resource="http://www.w3.org/1999/02/22-rdf-syntax-ns#Property" />
  <rdfs:subPropertyOf rdf:resource="http://rdaregistry.info/Elements/u/P60447" />
  <owl:inverseOf rdf:resource="http://rdaregistry.info/Elements/u/P60658" />
  <reg:lexicalAlias rdf:resource="http://rdaregistry.info/Elements/u/photographer.en" />
  <reg:hasSubproperty rdf:resource="http://rdaregistry.info/Elements/e/P20288" />
</owl:ObjectProperty>

<!-- Property: is photographer of -->
<owl:ObjectProperty rdf:about="http://rdaregistry.info/Elements/u/P60658">
  <rdfs:isDefinedBy rdf:resource="http://rdaregistry.info/Elements/u/" />
  <reg:status rdf:resource="http://metadataregistry.org/uri/RegStatus/1001" />
  <reg:name xml:lang="en">photographerOf</reg:name>
  <rdfs:label xml:lang="en">is photographer of</rdfs:label>
  <skos:definition xml:lang="en">Relates an agent responsible for creating a photographic resource to a resource.</skos:definition>
  <rdf:type rdf:resource="http://www.w3.org/1999/02/22-rdf-syntax-ns#Property" />
  <rdfs:subPropertyOf rdf:resource="http://rdaregistry.info/Elements/u/P60672" />
  <owl:inverseOf rdf:resource="http://rdaregistry.info/Elements/u/P60429" />
  <reg:hasSubproperty rdf:resource="http://rdaregistry.info/Elements/a/P50190" />
  <reg:lexicalAlias rdf:resource="http://rdaregistry.info/Elements/u/photographerOf.en" />
  <reg:hasSubproperty rdf:resource="http://rdaregistry.info/Elements/a/P50272" />
</owl:ObjectProperty>

<!-- Property: has place and date of capture -->
<owl:ObjectProperty rdf:about="http://rdaregistry.info/Elements/u/P60555">
  <rdfs:isDefinedBy rdf:resource="http://rdaregistry.info/Elements/u/" />
  <reg:status rdf:resource="http://metadataregistry.org/uri/RegStatus/1001" />
  <reg:name xml:lang="en">placeAndDateOfCapture</reg:name>
  <rdfs:label xml:lang="en">has place and date of capture</rdfs:label>
  <skos:definition xml:lang="en">Relates a resource to a place and date associated with the capture (i.e., recording, filming, etc.) of the content of a resource.</skos:definition>
  <rdf:type rdf:resource="http://www.w3.org/1999/02/22-rdf-syntax-ns#Property" />
  <reg:hasSubproperty rdf:resource="http://rdaregistry.info/Elements/e/P20217" />
  <reg:lexicalAlias rdf:resource="http://rdaregistry.info/Elements/u/placeAndDateOfCapture.en" />
</owl:ObjectProperty>

<!-- Property: has place associated with agent -->
<owl:ObjectProperty rdf:about="http://rdaregistry.info/Elements/u/P60325">
  <rdfs:isDefinedBy rdf:resource="http://rdaregistry.info/Elements/u/" />
  <reg:status rdf:resource="http://metadataregistry.org/uri/RegStatus/1001" />
  <reg:name xml:lang="en">placeAssociatedWithAgent</reg:name>
  <rdfs:label xml:lang="en">has place associated with agent</rdfs:label>
  <skos:definition xml:lang="en">Relates a resource to a significant location associated with an agent, or a place where an agent resides or has resided or has some connection.</skos:definition>
  <rdf:type rdf:resource="http://www.w3.org/1999/02/22-rdf-syntax-ns#Property" />
  <reg:hasSubproperty rdf:resource="http://rdaregistry.info/Elements/u/P60064" />
  <reg:hasSubproperty rdf:resource="http://rdaregistry.info/Elements/u/P60107" />
  <reg:hasSubproperty rdf:resource="http://rdaregistry.info/Elements/a/P50031" />
  <reg:hasSubproperty rdf:resource="http://rdaregistry.info/Elements/a/P50057" />
  <reg:hasSubproperty rdf:resource="http://rdaregistry.info/Elements/a/P50260" />
  <reg:lexicalAlias rdf:resource="http://rdaregistry.info/Elements/u/placeAssociatedWithAgent.en" />
</owl:ObjectProperty>

<!-- Property: has place of birth -->
<owl:ObjectProperty rdf:about="http://rdaregistry.info/Elements/u/P60593">
  <rdfs:isDefinedBy rdf:resource="http://rdaregistry.info/Elements/u/" />
  <reg:status rdf:resource="http://metadataregistry.org/uri/RegStatus/1001" />
  <reg:name xml:lang="en">placeOfBirth</reg:name>
  <rdfs:label xml:lang="en">has place of birth</rdfs:label>
  <skos:definition xml:lang="en">Relates a resource to a town, city, province, state, or country in which an agent was born.</skos:definition>
  <rdf:type rdf:resource="http://www.w3.org/1999/02/22-rdf-syntax-ns#Property" />
  <reg:hasSubproperty rdf:resource="http://rdaregistry.info/Elements/a/P50119" />
  <reg:lexicalAlias rdf:resource="http://rdaregistry.info/Elements/u/placeOfBirth.en" />
</owl:ObjectProperty>

<!-- Property: has place of capture -->
<owl:ObjectProperty rdf:about="http://rdaregistry.info/Elements/u/P60556">
  <rdfs:isDefinedBy rdf:resource="http://rdaregistry.info/Elements/u/" />
  <reg:status rdf:resource="http://metadataregistry.org/uri/RegStatus/1001" />
  <reg:name xml:lang="en">placeOfCapture</reg:name>
  <rdfs:label xml:lang="en">has place of capture</rdfs:label>
  <skos:definition xml:lang="en">Relates a resource to a place associated with the capture (i.e., recording, filming, etc.) of the content of a resource.</skos:definition>
  <rdf:type rdf:resource="http://www.w3.org/1999/02/22-rdf-syntax-ns#Property" />
  <reg:hasSubproperty rdf:resource="http://rdaregistry.info/Elements/e/P20218" />
  <reg:lexicalAlias rdf:resource="http://rdaregistry.info/Elements/u/placeOfCapture.en" />
</owl:ObjectProperty>

<!-- Property: has place of death -->
<owl:ObjectProperty rdf:about="http://rdaregistry.info/Elements/u/P60592">
  <rdfs:isDefinedBy rdf:resource="http://rdaregistry.info/Elements/u/" />
  <reg:status rdf:resource="http://metadataregistry.org/uri/RegStatus/1001" />
  <reg:name xml:lang="en">placeOfDeath</reg:name>
  <rdfs:label xml:lang="en">has place of death</rdfs:label>
  <skos:definition xml:lang="en">Relates a resource to a town, city, province, state, or country in which an agent died.</skos:definition>
  <rdf:type rdf:resource="http://www.w3.org/1999/02/22-rdf-syntax-ns#Property" />
  <reg:hasSubproperty rdf:resource="http://rdaregistry.info/Elements/a/P50118" />
  <reg:lexicalAlias rdf:resource="http://rdaregistry.info/Elements/u/placeOfDeath.en" />
</owl:ObjectProperty>

<!-- Property: has place of distribution -->
<owl:ObjectProperty rdf:about="http://rdaregistry.info/Elements/u/P60160">
  <rdfs:isDefinedBy rdf:resource="http://rdaregistry.info/Elements/u/" />
  <reg:status rdf:resource="http://metadataregistry.org/uri/RegStatus/1001" />
  <reg:name xml:lang="en">placeOfDistribution</reg:name>
  <rdfs:label xml:lang="en">has place of distribution</rdfs:label>
  <skos:definition xml:lang="en">Relates a resource to a place associated with a distribution of a resource in a published form.</skos:definition>
  <rdf:type rdf:resource="http://www.w3.org/1999/02/22-rdf-syntax-ns#Property" />
  <reg:hasSubproperty rdf:resource="http://rdaregistry.info/Elements/m/P30085" />
  <reg:lexicalAlias rdf:resource="http://rdaregistry.info/Elements/u/placeOfDistribution.en" />
</owl:ObjectProperty>

<!-- Property: has place of manufacture -->
<owl:ObjectProperty rdf:about="http://rdaregistry.info/Elements/u/P60162">
  <rdfs:isDefinedBy rdf:resource="http://rdaregistry.info/Elements/u/" />
  <reg:status rdf:resource="http://metadataregistry.org/uri/RegStatus/1001" />
  <reg:name xml:lang="en">placeOfManufacture</reg:name>
  <rdfs:label xml:lang="en">has place of manufacture</rdfs:label>
  <skos:definition xml:lang="en">Relates a resource to a place associated with the printing, duplicating, casting, etc., of a resource in a published form.</skos:definition>
  <rdf:type rdf:resource="http://www.w3.org/1999/02/22-rdf-syntax-ns#Property" />
  <reg:hasSubproperty rdf:resource="http://rdaregistry.info/Elements/m/P30087" />
  <reg:lexicalAlias rdf:resource="http://rdaregistry.info/Elements/u/placeOfManufacture.en" />
</owl:ObjectProperty>

<!-- Property: has place of origin of resource -->
<owl:ObjectProperty rdf:about="http://rdaregistry.info/Elements/u/P60523">
  <rdfs:isDefinedBy rdf:resource="http://rdaregistry.info/Elements/u/" />
  <reg:status rdf:resource="http://metadataregistry.org/uri/RegStatus/1001" />
  <reg:name xml:lang="en">placeOfOriginOfResource</reg:name>
  <rdfs:label xml:lang="en">has place of origin of resource</rdfs:label>
  <skos:definition xml:lang="en">Relates a resource to a country or other territorial jurisdiction from which a resource originated.</skos:definition>
  <rdf:type rdf:resource="http://www.w3.org/1999/02/22-rdf-syntax-ns#Property" />
  <reg:lexicalAlias rdf:resource="http://rdaregistry.info/Elements/u/placeOfOriginOfResource.en" />
</owl:ObjectProperty>

<!-- Property: has place of production -->
<owl:ObjectProperty rdf:about="http://rdaregistry.info/Elements/u/P60161">
  <rdfs:isDefinedBy rdf:resource="http://rdaregistry.info/Elements/u/" />
  <reg:status rdf:resource="http://metadataregistry.org/uri/RegStatus/1001" />
  <reg:name xml:lang="en">placeOfProduction</reg:name>
  <rdfs:label xml:lang="en">has place of production</rdfs:label>
  <skos:definition xml:lang="en">Relates a resource to a place associated with the inscription, fabrication, construction, etc., of a resource in an unpublished form.</skos:definition>
  <rdf:type rdf:resource="http://www.w3.org/1999/02/22-rdf-syntax-ns#Property" />
  <reg:hasSubproperty rdf:resource="http://rdaregistry.info/Elements/m/P30086" />
  <reg:lexicalAlias rdf:resource="http://rdaregistry.info/Elements/u/placeOfProduction.en" />
</owl:ObjectProperty>

<!-- Property: has place of publication -->
<owl:ObjectProperty rdf:about="http://rdaregistry.info/Elements/u/P60163">
  <rdfs:isDefinedBy rdf:resource="http://rdaregistry.info/Elements/u/" />
  <reg:status rdf:resource="http://metadataregistry.org/uri/RegStatus/1001" />
  <reg:name xml:lang="en">placeOfPublication</reg:name>
  <rdfs:label xml:lang="en">has place of publication</rdfs:label>
  <skos:definition xml:lang="en">Relates a resource to a place associated with the publication, release, or issuing of a resource.</skos:definition>
  <rdf:type rdf:resource="http://www.w3.org/1999/02/22-rdf-syntax-ns#Property" />
  <reg:hasSubproperty rdf:resource="http://rdaregistry.info/Elements/m/P30088" />
  <reg:lexicalAlias rdf:resource="http://rdaregistry.info/Elements/u/placeOfPublication.en" />
</owl:ObjectProperty>

<!-- Property: has place of residence, etc. -->
<owl:ObjectProperty rdf:about="http://rdaregistry.info/Elements/u/P60360">
  <rdfs:isDefinedBy rdf:resource="http://rdaregistry.info/Elements/u/" />
  <reg:status rdf:resource="http://metadataregistry.org/uri/RegStatus/1001" />
  <reg:name xml:lang="en">placeOfResidenceEtc</reg:name>
  <rdfs:label xml:lang="en">has place of residence, etc.</rdfs:label>
  <skos:definition xml:lang="en">Relates a resource to a town, city, province, state, or country in which an agent resides or has resided, or another significant place associated with an agent other than place of birth, place of death, or residence.</skos:definition>
  <rdf:type rdf:resource="http://www.w3.org/1999/02/22-rdf-syntax-ns#Property" />
  <reg:hasSubproperty rdf:resource="http://rdaregistry.info/Elements/a/P50109" />
  <reg:lexicalAlias rdf:resource="http://rdaregistry.info/Elements/u/placeOfResidenceEtc.en" />
  <skos:scopeNote xml:lang="en">A place where an agent has worked or studied is included.</skos:scopeNote>
</owl:ObjectProperty>

<!-- Property: has plaintiff -->
<owl:ObjectProperty rdf:about="http://rdaregistry.info/Elements/u/P60459">
  <rdfs:isDefinedBy rdf:resource="http://rdaregistry.info/Elements/u/" />
  <reg:status rdf:resource="http://metadataregistry.org/uri/RegStatus/1001" />
  <reg:name xml:lang="en">plaintiff</reg:name>
  <rdfs:label xml:lang="en">has plaintiff</rdfs:label>
  <skos:definition xml:lang="en">Relates a resource to an agent who brings a suit in a civil proceeding.</skos:definition>
  <rdf:type rdf:resource="http://www.w3.org/1999/02/22-rdf-syntax-ns#Property" />
  <rdfs:subPropertyOf rdf:resource="http://rdaregistry.info/Elements/u/P60374" />
  <owl:inverseOf rdf:resource="http://rdaregistry.info/Elements/u/P60693" />
  <reg:lexicalAlias rdf:resource="http://rdaregistry.info/Elements/u/plaintiff.en" />
</owl:ObjectProperty>

<!-- Property: is plaintiff of -->
<owl:ObjectProperty rdf:about="http://rdaregistry.info/Elements/u/P60693">
  <rdfs:isDefinedBy rdf:resource="http://rdaregistry.info/Elements/u/" />
  <reg:status rdf:resource="http://metadataregistry.org/uri/RegStatus/1001" />
  <reg:name xml:lang="en">plaintiffOf</reg:name>
  <rdfs:label xml:lang="en">is plaintiff of</rdfs:label>
  <skos:definition xml:lang="en">Relates an agent who brings a suit in a civil proceeding to a resource.</skos:definition>
  <rdf:type rdf:resource="http://www.w3.org/1999/02/22-rdf-syntax-ns#Property" />
  <rdfs:subPropertyOf rdf:resource="http://rdaregistry.info/Elements/u/P60602" />
  <owl:inverseOf rdf:resource="http://rdaregistry.info/Elements/u/P60459" />
  <reg:hasSubproperty rdf:resource="http://rdaregistry.info/Elements/a/P50043" />
  <reg:hasSubproperty rdf:resource="http://rdaregistry.info/Elements/a/P50089" />
  <reg:hasSubproperty rdf:resource="http://rdaregistry.info/Elements/a/P50124" />
  <reg:lexicalAlias rdf:resource="http://rdaregistry.info/Elements/u/plaintiffOf.en" />
</owl:ObjectProperty>

<!-- Property: has platemaker -->
<owl:ObjectProperty rdf:about="http://rdaregistry.info/Elements/u/P60415">
  <rdfs:isDefinedBy rdf:resource="http://rdaregistry.info/Elements/u/" />
  <reg:status rdf:resource="http://metadataregistry.org/uri/RegStatus/1001" />
  <reg:name xml:lang="en">platemaker</reg:name>
  <rdfs:label xml:lang="en">has platemaker</rdfs:label>
  <skos:definition xml:lang="en">Relates a resource to an agent involved in manufacturing a resource by preparing plates used in the production of printed images or text.</skos:definition>
  <rdf:type rdf:resource="http://www.w3.org/1999/02/22-rdf-syntax-ns#Property" />
  <rdfs:subPropertyOf rdf:resource="http://rdaregistry.info/Elements/u/P60443" />
  <owl:inverseOf rdf:resource="http://rdaregistry.info/Elements/u/P60643" />
  <reg:hasSubproperty rdf:resource="http://rdaregistry.info/Elements/m/P30075" />
  <reg:lexicalAlias rdf:resource="http://rdaregistry.info/Elements/u/platemaker.en" />
</owl:ObjectProperty>

<!-- Property: is platemaker of -->
<owl:ObjectProperty rdf:about="http://rdaregistry.info/Elements/u/P60643">
  <rdfs:isDefinedBy rdf:resource="http://rdaregistry.info/Elements/u/" />
  <reg:status rdf:resource="http://metadataregistry.org/uri/RegStatus/1001" />
  <reg:name xml:lang="en">platemakerOf</reg:name>
  <rdfs:label xml:lang="en">is platemaker of</rdfs:label>
  <skos:definition xml:lang="en">Relates an agent involved in manufacturing a resource by preparing plates used in the production of printed images or text to a resource.</skos:definition>
  <rdf:type rdf:resource="http://www.w3.org/1999/02/22-rdf-syntax-ns#Property" />
  <rdfs:subPropertyOf rdf:resource="http://rdaregistry.info/Elements/u/P60669" />
  <owl:inverseOf rdf:resource="http://rdaregistry.info/Elements/u/P60415" />
  <reg:hasSubproperty rdf:resource="http://rdaregistry.info/Elements/a/P50176" />
  <reg:lexicalAlias rdf:resource="http://rdaregistry.info/Elements/u/platemakerOf.en" />
</owl:ObjectProperty>

<!-- Property: has plate number for music -->
<owl:ObjectProperty rdf:about="http://rdaregistry.info/Elements/u/P60140">
  <rdfs:isDefinedBy rdf:resource="http://rdaregistry.info/Elements/u/" />
  <reg:status rdf:resource="http://metadataregistry.org/uri/RegStatus/1001" />
  <reg:name xml:lang="en">plateNumberForMusic</reg:name>
  <rdfs:label xml:lang="en">has plate number for music</rdfs:label>
  <skos:definition xml:lang="en">Relates a resource to a numbering designation assigned to a notated music resource by a publisher.</skos:definition>
  <rdf:type rdf:resource="http://www.w3.org/1999/02/22-rdf-syntax-ns#Property" />
  <rdfs:subPropertyOf rdf:resource="http://rdaregistry.info/Elements/u/P60052" />
  <reg:hasSubproperty rdf:resource="http://rdaregistry.info/Elements/m/P30066" />
  <reg:lexicalAlias rdf:resource="http://rdaregistry.info/Elements/u/plateNumberForMusic.en" />
  <skos:scopeNote xml:lang="en">A plate number for notated music sometimes includes initials, abbreviations, or words identifying the publisher and is sometimes followed by a number corresponding to the number of pages or plates.</skos:scopeNote>
</owl:ObjectProperty>

<!-- Property: has playing speed -->
<owl:ObjectProperty rdf:about="http://rdaregistry.info/Elements/u/P60586">
  <rdfs:isDefinedBy rdf:resource="http://rdaregistry.info/Elements/u/" />
  <reg:status rdf:resource="http://metadataregistry.org/uri/RegStatus/1001" />
  <reg:name xml:lang="en">playingSpeed</reg:name>
  <rdfs:label xml:lang="en">has playing speed</rdfs:label>
  <skos:definition xml:lang="en">Relates a resource to a speed at which an audio carrier must be operated to produce the sound intended.</skos:definition>
  <rdf:type rdf:resource="http://www.w3.org/1999/02/22-rdf-syntax-ns#Property" />
  <rdfs:subPropertyOf rdf:resource="http://rdaregistry.info/Elements/u/P60351" />
  <reg:hasSubproperty rdf:resource="http://rdaregistry.info/Elements/m/P30201" />
  <reg:lexicalAlias rdf:resource="http://rdaregistry.info/Elements/u/playingSpeed.en" />
</owl:ObjectProperty>

<!-- Property: has polarity -->
<owl:ObjectProperty rdf:about="http://rdaregistry.info/Elements/u/P60573">
  <rdfs:isDefinedBy rdf:resource="http://rdaregistry.info/Elements/u/" />
  <reg:status rdf:resource="http://metadataregistry.org/uri/RegStatus/1001" />
  <reg:name xml:lang="en">polarity</reg:name>
  <rdfs:label xml:lang="en">has polarity</rdfs:label>
  <skos:definition xml:lang="en">Relates a resource to a relationship of the colours and tones in an image to the colours and tones of the object reproduced.</skos:definition>
  <rdf:type rdf:resource="http://www.w3.org/1999/02/22-rdf-syntax-ns#Property" />
  <reg:hasSubproperty rdf:resource="http://rdaregistry.info/Elements/m/P30196" />
  <reg:lexicalAlias rdf:resource="http://rdaregistry.info/Elements/u/polarity.en" />
</owl:ObjectProperty>

<!-- Property: has praeses -->
<owl:ObjectProperty rdf:about="http://rdaregistry.info/Elements/u/P60463">
  <rdfs:isDefinedBy rdf:resource="http://rdaregistry.info/Elements/u/" />
  <reg:status rdf:resource="http://metadataregistry.org/uri/RegStatus/1001" />
  <reg:name xml:lang="en">praeses</reg:name>
  <rdfs:label xml:lang="en">has praeses</rdfs:label>
  <skos:definition xml:lang="en">Relates a resource to an agent who is a faculty moderator of an academic disputation, normally proposing a thesis and participating in an ensuing disputation.</skos:definition>
  <rdf:type rdf:resource="http://www.w3.org/1999/02/22-rdf-syntax-ns#Property" />
  <rdfs:subPropertyOf rdf:resource="http://rdaregistry.info/Elements/u/P60447" />
  <owl:inverseOf rdf:resource="http://rdaregistry.info/Elements/u/P60699" />
  <reg:lexicalAlias rdf:resource="http://rdaregistry.info/Elements/u/praeses.en" />
</owl:ObjectProperty>

<!-- Property: is praeses of -->
<owl:ObjectProperty rdf:about="http://rdaregistry.info/Elements/u/P60699">
  <rdfs:isDefinedBy rdf:resource="http://rdaregistry.info/Elements/u/" />
  <reg:status rdf:resource="http://metadataregistry.org/uri/RegStatus/1001" />
  <reg:name xml:lang="en">praesesOf</reg:name>
  <rdfs:label xml:lang="en">is praeses of</rdfs:label>
  <skos:definition xml:lang="en">Relates an agent who is a faculty moderator of an academic disputation, normally proposing a thesis and participating in an ensuing disputation to a resource.</skos:definition>
  <rdf:type rdf:resource="http://www.w3.org/1999/02/22-rdf-syntax-ns#Property" />
  <rdfs:subPropertyOf rdf:resource="http://rdaregistry.info/Elements/u/P60672" />
  <owl:inverseOf rdf:resource="http://rdaregistry.info/Elements/u/P60463" />
  <reg:hasSubproperty rdf:resource="http://rdaregistry.info/Elements/a/P50127" />
  <reg:lexicalAlias rdf:resource="http://rdaregistry.info/Elements/u/praesesOf.en" />
</owl:ObjectProperty>

<!-- Property: is preceded by -->
<owl:ObjectProperty rdf:about="http://rdaregistry.info/Elements/u/P60261">
  <rdfs:isDefinedBy rdf:resource="http://rdaregistry.info/Elements/u/" />
  <reg:status rdf:resource="http://metadataregistry.org/uri/RegStatus/1001" />
  <reg:name xml:lang="en">precededBy</reg:name>
  <rdfs:label xml:lang="en">is preceded by</rdfs:label>
  <skos:definition xml:lang="en">Relates a resource to a resource that precedes, that is, is earlier in time or before in a narrative, etc., a succeeding resource.</skos:definition>
  <rdf:type rdf:resource="http://www.w3.org/1999/02/22-rdf-syntax-ns#Property" />
  <rdfs:subPropertyOf rdf:resource="http://rdaregistry.info/Elements/u/P60713" />
  <owl:inverseOf rdf:resource="http://rdaregistry.info/Elements/u/P60278" />
  <reg:hasSubproperty rdf:resource="http://rdaregistry.info/Elements/u/P60220" />
  <reg:hasSubproperty rdf:resource="http://rdaregistry.info/Elements/u/P60276" />
  <reg:hasSubproperty rdf:resource="http://rdaregistry.info/Elements/u/P60277" />
  <reg:hasSubproperty rdf:resource="http://rdaregistry.info/Elements/u/P60479" />
  <reg:hasSubproperty rdf:resource="http://rdaregistry.info/Elements/u/P60480" />
  <reg:hasSubproperty rdf:resource="http://rdaregistry.info/Elements/u/P60505" />
  <reg:hasSubproperty rdf:resource="http://rdaregistry.info/Elements/u/P60574" />
  <reg:hasSubproperty rdf:resource="http://rdaregistry.info/Elements/u/P60575" />
  <reg:hasSubproperty rdf:resource="http://rdaregistry.info/Elements/u/P60576" />
  <reg:hasSubproperty rdf:resource="http://rdaregistry.info/Elements/u/P60577" />
  <reg:hasSubproperty rdf:resource="http://rdaregistry.info/Elements/e/P20154" />
  <reg:lexicalAlias rdf:resource="http://rdaregistry.info/Elements/u/precededBy.en" />
</owl:ObjectProperty>

<!-- Property: has predecessor -->
<owl:ObjectProperty rdf:about="http://rdaregistry.info/Elements/u/P60683">
  <rdfs:isDefinedBy rdf:resource="http://rdaregistry.info/Elements/u/" />
  <reg:status rdf:resource="http://metadataregistry.org/uri/RegStatus/1001" />
  <reg:name xml:lang="en">predecessor</reg:name>
  <rdfs:label xml:lang="en">has predecessor</rdfs:label>
  <skos:definition xml:lang="en">Relates an agent that precedes another agent to an agent.</skos:definition>
  <rdf:type rdf:resource="http://www.w3.org/1999/02/22-rdf-syntax-ns#Property" />
  <owl:inverseOf rdf:resource="http://rdaregistry.info/Elements/u/P60686" />
  <reg:hasSubproperty rdf:resource="http://rdaregistry.info/Elements/a/P50012" />
  <reg:hasSubproperty rdf:resource="http://rdaregistry.info/Elements/a/P50055" />
  <reg:lexicalAlias rdf:resource="http://rdaregistry.info/Elements/u/predecessor.en" />
</owl:ObjectProperty>

<!-- Property: has predecessor of split -->
<owl:ObjectProperty rdf:about="http://rdaregistry.info/Elements/u/P60733">
  <rdfs:isDefinedBy rdf:resource="http://rdaregistry.info/Elements/u/" />
  <reg:status rdf:resource="http://metadataregistry.org/uri/RegStatus/1001" />
  <reg:name xml:lang="en">predecessorOfSplit</reg:name>
  <rdfs:label xml:lang="en">has predecessor of split</rdfs:label>
  <skos:definition xml:lang="en">Relates an agent that split or divided into another agent to an agent.</skos:definition>
  <rdf:type rdf:resource="http://www.w3.org/1999/02/22-rdf-syntax-ns#Property" />
  <owl:inverseOf rdf:resource="http://rdaregistry.info/Elements/u/P60685" />
  <reg:hasSubproperty rdf:resource="http://rdaregistry.info/Elements/a/P50229" />
  <reg:lexicalAlias rdf:resource="http://rdaregistry.info/Elements/u/predecessorOfSplit.en" />
</owl:ObjectProperty>

<!-- Property: has preferred citation -->
<owl:ObjectProperty rdf:about="http://rdaregistry.info/Elements/u/P60057">
  <rdfs:isDefinedBy rdf:resource="http://rdaregistry.info/Elements/u/" />
  <reg:status rdf:resource="http://metadataregistry.org/uri/RegStatus/1001" />
  <reg:name xml:lang="en">preferredCitation</reg:name>
  <rdfs:label xml:lang="en">has preferred citation</rdfs:label>
  <skos:definition xml:lang="en">Relates a resource to a citation for a resource in a form preferred by a creator, publisher, custodian, indexing or abstracting service, etc.</skos:definition>
  <rdf:type rdf:resource="http://www.w3.org/1999/02/22-rdf-syntax-ns#Property" />
  <reg:hasSubproperty rdf:resource="http://rdaregistry.info/Elements/m/P30005" />
  <reg:lexicalAlias rdf:resource="http://rdaregistry.info/Elements/u/preferredCitation.en" />
</owl:ObjectProperty>

<!-- Property: has preferred name for agent -->
<owl:ObjectProperty rdf:about="http://rdaregistry.info/Elements/u/P60549">
  <rdfs:isDefinedBy rdf:resource="http://rdaregistry.info/Elements/u/" />
  <reg:status rdf:resource="http://metadataregistry.org/uri/RegStatus/1001" />
  <reg:name xml:lang="en">preferredNameForAgent</reg:name>
  <rdfs:label xml:lang="en">has preferred name for agent</rdfs:label>
  <skos:definition xml:lang="en">Relates a resource to a name or form of name chosen to identify an agent.</skos:definition>
  <rdf:type rdf:resource="http://www.w3.org/1999/02/22-rdf-syntax-ns#Property" />
  <rdfs:subPropertyOf rdf:resource="http://rdaregistry.info/Elements/u/P60368" />
  <reg:hasSubproperty rdf:resource="http://rdaregistry.info/Elements/a/P50041" />
  <reg:hasSubproperty rdf:resource="http://rdaregistry.info/Elements/a/P50065" />
  <reg:hasSubproperty rdf:resource="http://rdaregistry.info/Elements/a/P50117" />
  <reg:lexicalAlias rdf:resource="http://rdaregistry.info/Elements/u/preferredNameForAgent.en" />
</owl:ObjectProperty>

<!-- Property: has preferred name of place -->
<owl:ObjectProperty rdf:about="http://rdaregistry.info/Elements/u/P60548">
  <rdfs:isDefinedBy rdf:resource="http://rdaregistry.info/Elements/u/" />
  <reg:status rdf:resource="http://metadataregistry.org/uri/RegStatus/1001" />
  <reg:name xml:lang="en">preferredNameOfPlace</reg:name>
  <rdfs:label xml:lang="en">has preferred name of place</rdfs:label>
  <skos:definition xml:lang="en">Relates a resource to a name or form of name chosen to identify a place.</skos:definition>
  <rdf:type rdf:resource="http://www.w3.org/1999/02/22-rdf-syntax-ns#Property" />
  <rdfs:subPropertyOf rdf:resource="http://rdaregistry.info/Elements/u/P60366" />
  <reg:lexicalAlias rdf:resource="http://rdaregistry.info/Elements/u/preferredNameOfPlace.en" />
  <reg:hasSubproperty rdf:resource="http://rdaregistry.info/Elements/p/P70002" />
</owl:ObjectProperty>

<!-- Property: has preferred title for resource -->
<owl:ObjectProperty rdf:about="http://rdaregistry.info/Elements/u/P60588">
  <rdfs:isDefinedBy rdf:resource="http://rdaregistry.info/Elements/u/" />
  <reg:status rdf:resource="http://metadataregistry.org/uri/RegStatus/1001" />
  <reg:name xml:lang="en">preferredTitleForResource</reg:name>
  <rdfs:label xml:lang="en">has preferred title for resource</rdfs:label>
  <skos:definition xml:lang="en">Relates a resource to a title or form of title chosen to identify a resource.</skos:definition>
  <rdf:type rdf:resource="http://www.w3.org/1999/02/22-rdf-syntax-ns#Property" />
  <rdfs:subPropertyOf rdf:resource="http://rdaregistry.info/Elements/u/P60367" />
  <reg:lexicalAlias rdf:resource="http://rdaregistry.info/Elements/u/preferredTitleForResource.en" />
  <owl:inverseOf rdf:resource="http://rdaregistry.info/Elements/u/P60857" />
</owl:ObjectProperty>

<!-- Property: is prequel -->
<owl:ObjectProperty rdf:about="http://rdaregistry.info/Elements/u/P60220">
  <rdfs:isDefinedBy rdf:resource="http://rdaregistry.info/Elements/u/" />
  <reg:status rdf:resource="http://metadataregistry.org/uri/RegStatus/1001" />
  <reg:name xml:lang="en">prequel</reg:name>
  <rdfs:label xml:lang="en">is prequel</rdfs:label>
  <skos:definition xml:lang="en">Relates a resource to a resource that extends the narrative of an earlier resource backwards in time.</skos:definition>
  <rdf:type rdf:resource="http://www.w3.org/1999/02/22-rdf-syntax-ns#Property" />
  <rdfs:subPropertyOf rdf:resource="http://rdaregistry.info/Elements/u/P60261" />
  <owl:inverseOf rdf:resource="http://rdaregistry.info/Elements/u/P60310" />
  <reg:lexicalAlias rdf:resource="http://rdaregistry.info/Elements/u/prequel.en" />
</owl:ObjectProperty>

<!-- Property: is prequel to -->
<owl:ObjectProperty rdf:about="http://rdaregistry.info/Elements/u/P60310">
  <rdfs:isDefinedBy rdf:resource="http://rdaregistry.info/Elements/u/" />
  <reg:status rdf:resource="http://metadataregistry.org/uri/RegStatus/1001" />
  <reg:name xml:lang="en">prequelTo</reg:name>
  <rdfs:label xml:lang="en">is prequel to</rdfs:label>
  <skos:definition xml:lang="en">Relates a resource to a resource whose narrative is extended backwards in time by the later resource.</skos:definition>
  <rdf:type rdf:resource="http://www.w3.org/1999/02/22-rdf-syntax-ns#Property" />
  <rdfs:subPropertyOf rdf:resource="http://rdaregistry.info/Elements/u/P60278" />
  <owl:inverseOf rdf:resource="http://rdaregistry.info/Elements/u/P60220" />
  <reg:lexicalAlias rdf:resource="http://rdaregistry.info/Elements/u/prequelTo.en" />
</owl:ObjectProperty>

<!-- Property: has presentation format -->
<owl:ObjectProperty rdf:about="http://rdaregistry.info/Elements/u/P60529">
  <rdfs:isDefinedBy rdf:resource="http://rdaregistry.info/Elements/u/" />
  <reg:status rdf:resource="http://metadataregistry.org/uri/RegStatus/1001" />
  <reg:name xml:lang="en">presentationFormat</reg:name>
  <rdfs:label xml:lang="en">has presentation format</rdfs:label>
  <skos:definition xml:lang="en">Relates a resource to a format used in the production of a projected image.</skos:definition>
  <rdf:type rdf:resource="http://www.w3.org/1999/02/22-rdf-syntax-ns#Property" />
  <rdfs:subPropertyOf rdf:resource="http://rdaregistry.info/Elements/u/P60353" />
  <reg:hasSubproperty rdf:resource="http://rdaregistry.info/Elements/m/P30163" />
  <reg:lexicalAlias rdf:resource="http://rdaregistry.info/Elements/u/presentationFormat.en" />
</owl:ObjectProperty>

<!-- Property: has presenter -->
<owl:ObjectProperty rdf:about="http://rdaregistry.info/Elements/u/P60419">
  <rdfs:isDefinedBy rdf:resource="http://rdaregistry.info/Elements/u/" />
  <reg:status rdf:resource="http://metadataregistry.org/uri/RegStatus/1001" />
  <reg:name xml:lang="en">presenter</reg:name>
  <rdfs:label xml:lang="en">has presenter</rdfs:label>
  <skos:definition xml:lang="en">Relates a resource to an agent mentioned in an "X presents" credit for moving image materials and who is probably associated with production, finance, or distribution in some way.</skos:definition>
  <rdf:type rdf:resource="http://www.w3.org/1999/02/22-rdf-syntax-ns#Property" />
  <rdfs:subPropertyOf rdf:resource="http://rdaregistry.info/Elements/u/P60398" />
  <owl:inverseOf rdf:resource="http://rdaregistry.info/Elements/u/P60647" />
  <reg:hasSubproperty rdf:resource="http://rdaregistry.info/Elements/e/P20054" />
  <reg:lexicalAlias rdf:resource="http://rdaregistry.info/Elements/u/presenter.en" />
</owl:ObjectProperty>

<!-- Property: is presenter of -->
<owl:ObjectProperty rdf:about="http://rdaregistry.info/Elements/u/P60647">
  <rdfs:isDefinedBy rdf:resource="http://rdaregistry.info/Elements/u/" />
  <reg:status rdf:resource="http://metadataregistry.org/uri/RegStatus/1001" />
  <reg:name xml:lang="en">presenterOf</reg:name>
  <rdfs:label xml:lang="en">is presenter of</rdfs:label>
  <skos:definition xml:lang="en">Relates an agent mentioned in an "X presents" credit for moving image materials and who is probably associated with production, finance, or distribution in some way to a resource.</skos:definition>
  <rdf:type rdf:resource="http://www.w3.org/1999/02/22-rdf-syntax-ns#Property" />
  <rdfs:subPropertyOf rdf:resource="http://rdaregistry.info/Elements/u/P60626" />
  <owl:inverseOf rdf:resource="http://rdaregistry.info/Elements/u/P60419" />
  <reg:hasSubproperty rdf:resource="http://rdaregistry.info/Elements/a/P50180" />
  <reg:lexicalAlias rdf:resource="http://rdaregistry.info/Elements/u/presenterOf.en" />
</owl:ObjectProperty>

<!-- Property: has preservation facsimile -->
<owl:ObjectProperty rdf:about="http://rdaregistry.info/Elements/u/P60179">
  <rdfs:isDefinedBy rdf:resource="http://rdaregistry.info/Elements/u/" />
  <reg:status rdf:resource="http://metadataregistry.org/uri/RegStatus/1001" />
  <reg:name xml:lang="en">preservationFacsimile</reg:name>
  <rdfs:label xml:lang="en">has preservation facsimile</rdfs:label>
  <skos:definition xml:lang="en">Relates a resource to a resource that consists of an exact reproduction on preservation-quality media, such as acid-free permanent or archival paper.</skos:definition>
  <rdf:type rdf:resource="http://www.w3.org/1999/02/22-rdf-syntax-ns#Property" />
  <rdfs:subPropertyOf rdf:resource="http://rdaregistry.info/Elements/u/P60217" />
  <owl:inverseOf rdf:resource="http://rdaregistry.info/Elements/u/P60299" />
  <reg:hasSubproperty rdf:resource="http://rdaregistry.info/Elements/i/P40059" />
  <reg:hasSubproperty rdf:resource="http://rdaregistry.info/Elements/m/P30021" />
  <reg:lexicalAlias rdf:resource="http://rdaregistry.info/Elements/u/preservationFacsimile.en" />
</owl:ObjectProperty>

<!-- Property: is preservation facsimile of -->
<owl:ObjectProperty rdf:about="http://rdaregistry.info/Elements/u/P60299">
  <rdfs:isDefinedBy rdf:resource="http://rdaregistry.info/Elements/u/" />
  <reg:status rdf:resource="http://metadataregistry.org/uri/RegStatus/1001" />
  <reg:name xml:lang="en">preservationFacsimileOf</reg:name>
  <rdfs:label xml:lang="en">is preservation facsimile of</rdfs:label>
  <skos:definition xml:lang="en">Relates a resource to a resource that is used as a basis for an exact reproduction on preservation-quality media, such as acid-free permanent or archival paper.</skos:definition>
  <rdf:type rdf:resource="http://www.w3.org/1999/02/22-rdf-syntax-ns#Property" />
  <rdfs:subPropertyOf rdf:resource="http://rdaregistry.info/Elements/u/P60301" />
  <owl:inverseOf rdf:resource="http://rdaregistry.info/Elements/u/P60179" />
  <reg:hasSubproperty rdf:resource="http://rdaregistry.info/Elements/i/P40044" />
  <reg:hasSubproperty rdf:resource="http://rdaregistry.info/Elements/m/P30045" />
  <reg:lexicalAlias rdf:resource="http://rdaregistry.info/Elements/u/preservationFacsimileOf.en" />
</owl:ObjectProperty>

<!-- Property: has printer -->
<owl:ObjectProperty rdf:about="http://rdaregistry.info/Elements/u/P60418">
  <rdfs:isDefinedBy rdf:resource="http://rdaregistry.info/Elements/u/" />
  <reg:status rdf:resource="http://metadataregistry.org/uri/RegStatus/1001" />
  <reg:name xml:lang="en">printer</reg:name>
  <rdfs:label xml:lang="en">has printer</rdfs:label>
  <skos:definition xml:lang="en">Relates a resource to an agent involved in manufacturing a resource of printed text, notated music, etc., from type or plates, such as a book, newspaper, magazine, broadside, score, etc.</skos:definition>
  <rdf:type rdf:resource="http://www.w3.org/1999/02/22-rdf-syntax-ns#Property" />
  <rdfs:subPropertyOf rdf:resource="http://rdaregistry.info/Elements/u/P60443" />
  <owl:inverseOf rdf:resource="http://rdaregistry.info/Elements/u/P60646" />
  <reg:hasSubproperty rdf:resource="http://rdaregistry.info/Elements/m/P30078" />
  <reg:lexicalAlias rdf:resource="http://rdaregistry.info/Elements/u/printer.en" />
</owl:ObjectProperty>

<!-- Property: is printer of -->
<owl:ObjectProperty rdf:about="http://rdaregistry.info/Elements/u/P60646">
  <rdfs:isDefinedBy rdf:resource="http://rdaregistry.info/Elements/u/" />
  <reg:status rdf:resource="http://metadataregistry.org/uri/RegStatus/1001" />
  <reg:name xml:lang="en">printerOf</reg:name>
  <rdfs:label xml:lang="en">is printer of</rdfs:label>
  <skos:definition xml:lang="en">Relates an agent involved in manufacturing a resource of printed text, notated music, etc., from type or plates, such as a book, newspaper, magazine, broadside, score, etc. to a resource.</skos:definition>
  <rdf:type rdf:resource="http://www.w3.org/1999/02/22-rdf-syntax-ns#Property" />
  <rdfs:subPropertyOf rdf:resource="http://rdaregistry.info/Elements/u/P60669" />
  <owl:inverseOf rdf:resource="http://rdaregistry.info/Elements/u/P60418" />
  <reg:hasSubproperty rdf:resource="http://rdaregistry.info/Elements/a/P50179" />
  <reg:lexicalAlias rdf:resource="http://rdaregistry.info/Elements/u/printerOf.en" />
</owl:ObjectProperty>

<!-- Property: has printmaker -->
<owl:ObjectProperty rdf:about="http://rdaregistry.info/Elements/u/P60412">
  <rdfs:isDefinedBy rdf:resource="http://rdaregistry.info/Elements/u/" />
  <reg:status rdf:resource="http://metadataregistry.org/uri/RegStatus/1001" />
  <reg:name xml:lang="en">printmaker</reg:name>
  <rdfs:label xml:lang="en">has printmaker</rdfs:label>
  <skos:definition xml:lang="en">Relates a resource to an agent involved in manufacturing a resource by making a relief, intaglio, or planographic printing surface.</skos:definition>
  <rdf:type rdf:resource="http://www.w3.org/1999/02/22-rdf-syntax-ns#Property" />
  <rdfs:subPropertyOf rdf:resource="http://rdaregistry.info/Elements/u/P60443" />
  <owl:inverseOf rdf:resource="http://rdaregistry.info/Elements/u/P60640" />
  <reg:hasSubproperty rdf:resource="http://rdaregistry.info/Elements/m/P30072" />
  <reg:lexicalAlias rdf:resource="http://rdaregistry.info/Elements/u/printmaker.en" />
</owl:ObjectProperty>

<!-- Property: is printmaker of -->
<owl:ObjectProperty rdf:about="http://rdaregistry.info/Elements/u/P60640">
  <rdfs:isDefinedBy rdf:resource="http://rdaregistry.info/Elements/u/" />
  <reg:status rdf:resource="http://metadataregistry.org/uri/RegStatus/1001" />
  <reg:name xml:lang="en">printmakerOf</reg:name>
  <rdfs:label xml:lang="en">is printmaker of</rdfs:label>
  <skos:definition xml:lang="en">Relates an agent involved in manufacturing a resource by making a relief, intaglio, or planographic printing surface to a resource.</skos:definition>
  <rdf:type rdf:resource="http://www.w3.org/1999/02/22-rdf-syntax-ns#Property" />
  <rdfs:subPropertyOf rdf:resource="http://rdaregistry.info/Elements/u/P60669" />
  <owl:inverseOf rdf:resource="http://rdaregistry.info/Elements/u/P60412" />
  <reg:hasSubproperty rdf:resource="http://rdaregistry.info/Elements/a/P50173" />
  <reg:lexicalAlias rdf:resource="http://rdaregistry.info/Elements/u/printmakerOf.en" />
</owl:ObjectProperty>

<!-- Property: has producer -->
<owl:ObjectProperty rdf:about="http://rdaregistry.info/Elements/u/P60441">
  <rdfs:isDefinedBy rdf:resource="http://rdaregistry.info/Elements/u/" />
  <reg:status rdf:resource="http://metadataregistry.org/uri/RegStatus/1001" />
  <reg:name xml:lang="en">producer</reg:name>
  <rdfs:label xml:lang="en">has producer</rdfs:label>
  <skos:definition xml:lang="en">Relates a resource to an agent responsible for most of the business aspects of a production for screen, sound recording, television, webcast, etc. a producer is generally responsible for fund raising, managing the production, hiring key personnel, arranging for distributors, etc.</skos:definition>
  <rdf:type rdf:resource="http://www.w3.org/1999/02/22-rdf-syntax-ns#Property" />
  <rdfs:subPropertyOf rdf:resource="http://rdaregistry.info/Elements/u/P60374" />
  <owl:inverseOf rdf:resource="http://rdaregistry.info/Elements/u/P60668" />
  <reg:hasSubproperty rdf:resource="http://rdaregistry.info/Elements/u/P60169" />
  <reg:hasSubproperty rdf:resource="http://rdaregistry.info/Elements/u/P60170" />
  <reg:hasSubproperty rdf:resource="http://rdaregistry.info/Elements/u/P60171" />
  <reg:lexicalAlias rdf:resource="http://rdaregistry.info/Elements/u/producer.en" />
  <reg:hasSubproperty rdf:resource="http://rdaregistry.info/Elements/u/P60889" />
</owl:ObjectProperty>

<!-- Property: is producer of -->
<owl:ObjectProperty rdf:about="http://rdaregistry.info/Elements/u/P60668">
  <rdfs:isDefinedBy rdf:resource="http://rdaregistry.info/Elements/u/" />
  <reg:status rdf:resource="http://metadataregistry.org/uri/RegStatus/1001" />
  <reg:name xml:lang="en">producerOf</reg:name>
  <rdfs:label xml:lang="en">is producer of</rdfs:label>
  <skos:definition xml:lang="en">Relates an agent responsible for most of the business aspects of a production for screen, sound recording, television, webcast, etc. to a resource.</skos:definition>
  <rdf:type rdf:resource="http://www.w3.org/1999/02/22-rdf-syntax-ns#Property" />
  <rdfs:subPropertyOf rdf:resource="http://rdaregistry.info/Elements/u/P60602" />
  <owl:inverseOf rdf:resource="http://rdaregistry.info/Elements/u/P60441" />
  <reg:hasSubproperty rdf:resource="http://rdaregistry.info/Elements/u/P60033" />
  <reg:hasSubproperty rdf:resource="http://rdaregistry.info/Elements/u/P60034" />
  <reg:hasSubproperty rdf:resource="http://rdaregistry.info/Elements/u/P60035" />
  <reg:hasSubproperty rdf:resource="http://rdaregistry.info/Elements/a/P50201" />
  <reg:lexicalAlias rdf:resource="http://rdaregistry.info/Elements/u/producerOf.en" />
  <reg:hasSubproperty rdf:resource="http://rdaregistry.info/Elements/u/P60883" />
</owl:ObjectProperty>

<!-- Property: has producer of unpublished resource -->
<owl:ObjectProperty rdf:about="http://rdaregistry.info/Elements/u/P60440">
  <rdfs:isDefinedBy rdf:resource="http://rdaregistry.info/Elements/u/" />
  <reg:status rdf:resource="http://metadataregistry.org/uri/RegStatus/1001" />
  <reg:name xml:lang="en">producerOfUnpublishedResource</reg:name>
  <rdfs:label xml:lang="en">has producer of unpublished resource</rdfs:label>
  <skos:definition xml:lang="en">Relates a resource to an agent responsible for inscribing, fabricating, constructing, etc., a resource in an unpublished form.</skos:definition>
  <rdf:type rdf:resource="http://www.w3.org/1999/02/22-rdf-syntax-ns#Property" />
  <reg:hasSubproperty rdf:resource="http://rdaregistry.info/Elements/m/P30081" />
  <reg:lexicalAlias rdf:resource="http://rdaregistry.info/Elements/u/producerOfUnpublishedResource.en" />
</owl:ObjectProperty>

<!-- Property: is producer of unpublished resource of -->
<owl:ObjectProperty rdf:about="http://rdaregistry.info/Elements/u/P60817">
  <rdfs:isDefinedBy rdf:resource="http://rdaregistry.info/Elements/u/" />
  <reg:status rdf:resource="http://metadataregistry.org/uri/RegStatus/1001" />
  <rdf:type rdf:resource="http://www.w3.org/1999/02/22-rdf-syntax-ns#Property" />
  <reg:name xml:lang="en">producerOfUnpublishedResourceOf</reg:name>
  <rdfs:label xml:lang="en">is producer of unpublished resource of</rdfs:label>
  <reg:lexicalAlias rdf:resource="http://rdaregistry.info/Elements/u/producerOfUnpublishedResourceOf.en" />
  <skos:definition xml:lang="en">Relates an agent responsible for inscribing, fabricating, constructing, etc. to a resource.</skos:definition>
</owl:ObjectProperty>

<!-- Property: has producers name -->
<owl:ObjectProperty rdf:about="http://rdaregistry.info/Elements/u/P60545">
  <rdfs:isDefinedBy rdf:resource="http://rdaregistry.info/Elements/u/" />
  <reg:status rdf:resource="http://metadataregistry.org/uri/RegStatus/1001" />
  <reg:name xml:lang="en">producersName</reg:name>
  <rdfs:label xml:lang="en">has producers name</rdfs:label>
  <skos:definition xml:lang="en">Relates a resource to a name of an agent responsible for inscribing, fabricating, constructing, etc., a resource in an unpublished form.</skos:definition>
  <rdf:type rdf:resource="http://www.w3.org/1999/02/22-rdf-syntax-ns#Property" />
  <reg:hasSubproperty rdf:resource="http://rdaregistry.info/Elements/m/P30174" />
  <reg:lexicalAlias rdf:resource="http://rdaregistry.info/Elements/u/producersName.en" />
</owl:ObjectProperty>

<!-- Property: has production company -->
<owl:ObjectProperty rdf:about="http://rdaregistry.info/Elements/u/P60062">
  <rdfs:isDefinedBy rdf:resource="http://rdaregistry.info/Elements/u/" />
  <reg:status rdf:resource="http://metadataregistry.org/uri/RegStatus/1001" />
  <reg:name xml:lang="en">productionCompany</reg:name>
  <rdfs:label xml:lang="en">has production company</rdfs:label>
  <skos:definition xml:lang="en">Relates a resource to an agent that is responsible for financial, technical, and organizational management of a production for stage, screen, sound recording, television, webcast, etc.</skos:definition>
  <rdf:type rdf:resource="http://www.w3.org/1999/02/22-rdf-syntax-ns#Property" />
  <rdfs:subPropertyOf rdf:resource="http://rdaregistry.info/Elements/u/P60374" />
  <owl:inverseOf rdf:resource="http://rdaregistry.info/Elements/u/P60004" />
  <reg:lexicalAlias rdf:resource="http://rdaregistry.info/Elements/u/productionCompany.en" />
</owl:ObjectProperty>

<!-- Property: is production company of -->
<owl:ObjectProperty rdf:about="http://rdaregistry.info/Elements/u/P60004">
  <rdfs:isDefinedBy rdf:resource="http://rdaregistry.info/Elements/u/" />
  <reg:status rdf:resource="http://metadataregistry.org/uri/RegStatus/1001" />
  <reg:name xml:lang="en">productionCompanyOf</reg:name>
  <rdfs:label xml:lang="en">is production company of</rdfs:label>
  <skos:definition xml:lang="en">Relates an agent that is responsible for financial, technical, and organizational management of a production for stage, screen, sound recording, television, webcast, etc. to a resource.</skos:definition>
  <rdf:type rdf:resource="http://www.w3.org/1999/02/22-rdf-syntax-ns#Property" />
  <rdfs:subPropertyOf rdf:resource="http://rdaregistry.info/Elements/u/P60602" />
  <owl:inverseOf rdf:resource="http://rdaregistry.info/Elements/u/P60062" />
  <reg:hasSubproperty rdf:resource="http://rdaregistry.info/Elements/a/P50005" />
  <reg:lexicalAlias rdf:resource="http://rdaregistry.info/Elements/u/productionCompanyOf.en" />
</owl:ObjectProperty>

<!-- Property: has production designer -->
<owl:ObjectProperty rdf:about="http://rdaregistry.info/Elements/u/P60437">
  <rdfs:isDefinedBy rdf:resource="http://rdaregistry.info/Elements/u/" />
  <reg:status rdf:resource="http://metadataregistry.org/uri/RegStatus/1001" />
  <reg:name xml:lang="en">productionDesigner</reg:name>
  <rdfs:label xml:lang="en">has production designer</rdfs:label>
  <skos:definition xml:lang="en">Relates a resource to an agent responsible for designing the overall visual appearance of a moving image production.</skos:definition>
  <rdf:type rdf:resource="http://www.w3.org/1999/02/22-rdf-syntax-ns#Property" />
  <rdfs:subPropertyOf rdf:resource="http://rdaregistry.info/Elements/u/P60398" />
  <owl:inverseOf rdf:resource="http://rdaregistry.info/Elements/u/P60666" />
  <reg:hasSubproperty rdf:resource="http://rdaregistry.info/Elements/e/P20056" />
  <reg:lexicalAlias rdf:resource="http://rdaregistry.info/Elements/u/productionDesigner.en" />
</owl:ObjectProperty>

<!-- Property: is production designer of -->
<owl:ObjectProperty rdf:about="http://rdaregistry.info/Elements/u/P60666">
  <rdfs:isDefinedBy rdf:resource="http://rdaregistry.info/Elements/u/" />
  <reg:status rdf:resource="http://metadataregistry.org/uri/RegStatus/1001" />
  <reg:name xml:lang="en">productionDesignerOf</reg:name>
  <rdfs:label xml:lang="en">is production designer of</rdfs:label>
  <skos:definition xml:lang="en">Relates an agent responsible for designing the overall visual appearance of a moving image production to a resource.</skos:definition>
  <rdf:type rdf:resource="http://www.w3.org/1999/02/22-rdf-syntax-ns#Property" />
  <rdfs:subPropertyOf rdf:resource="http://rdaregistry.info/Elements/u/P60626" />
  <owl:inverseOf rdf:resource="http://rdaregistry.info/Elements/u/P60437" />
  <reg:hasSubproperty rdf:resource="http://rdaregistry.info/Elements/a/P50198" />
  <reg:lexicalAlias rdf:resource="http://rdaregistry.info/Elements/u/productionDesignerOf.en" />
</owl:ObjectProperty>

<!-- Property: has production method -->
<owl:ObjectProperty rdf:about="http://rdaregistry.info/Elements/u/P60560">
  <rdfs:isDefinedBy rdf:resource="http://rdaregistry.info/Elements/u/" />
  <reg:status rdf:resource="http://metadataregistry.org/uri/RegStatus/1001" />
  <reg:name xml:lang="en">productionMethod</reg:name>
  <rdfs:label xml:lang="en">has production method</rdfs:label>
  <skos:definition xml:lang="en">Relates a resource to a process used to produce a resource.</skos:definition>
  <rdf:type rdf:resource="http://www.w3.org/1999/02/22-rdf-syntax-ns#Property" />
  <reg:hasSubproperty rdf:resource="http://rdaregistry.info/Elements/u/P60561" />
  <reg:hasSubproperty rdf:resource="http://rdaregistry.info/Elements/u/P60562" />
  <reg:hasSubproperty rdf:resource="http://rdaregistry.info/Elements/m/P30187" />
  <reg:lexicalAlias rdf:resource="http://rdaregistry.info/Elements/u/productionMethod.en" />
</owl:ObjectProperty>

<!-- Property: DEPRECATED -->
<owl:ObjectProperty rdf:about="http://rdaregistry.info/Elements/u/P60562">
  <rdfs:isDefinedBy rdf:resource="http://rdaregistry.info/Elements/u/" />
  <reg:status rdf:resource="http://metadataregistry.org/uri/RegStatus/1008" />
  <reg:name xml:lang="en">productionMethodForManuscript</reg:name>
  <skos:definition xml:lang="en">Relates a resource to the process used to produce an original manuscript or a copy.</skos:definition>
  <rdf:type rdf:resource="http://www.w3.org/1999/02/22-rdf-syntax-ns#Property" />
  <rdfs:subPropertyOf rdf:resource="http://rdaregistry.info/Elements/u/P60560" />
  <reg:hasSubproperty rdf:resource="http://rdaregistry.info/Elements/m/P30189" />
  <reg:lexicalAlias rdf:resource="http://rdaregistry.info/Elements/u/productionMethodForManuscript.en" />
</owl:ObjectProperty>

<!-- Property: DEPRECATED -->
<owl:ObjectProperty rdf:about="http://rdaregistry.info/Elements/u/P60561">
  <rdfs:isDefinedBy rdf:resource="http://rdaregistry.info/Elements/u/" />
  <reg:status rdf:resource="http://metadataregistry.org/uri/RegStatus/1008" />
  <reg:name xml:lang="en">productionMethodForTactileResource</reg:name>
  <skos:definition xml:lang="en">Relates a resource to the process used to produce a tactile resource (e.g., embossing, thermoform).</skos:definition>
  <rdf:type rdf:resource="http://www.w3.org/1999/02/22-rdf-syntax-ns#Property" />
  <rdfs:subPropertyOf rdf:resource="http://rdaregistry.info/Elements/u/P60560" />
  <reg:hasSubproperty rdf:resource="http://rdaregistry.info/Elements/m/P30188" />
  <reg:lexicalAlias rdf:resource="http://rdaregistry.info/Elements/u/productionMethodForTactileResource.en" />
</owl:ObjectProperty>

<!-- Property: has production statement -->
<owl:ObjectProperty rdf:about="http://rdaregistry.info/Elements/u/P60332">
  <rdfs:isDefinedBy rdf:resource="http://rdaregistry.info/Elements/u/" />
  <reg:status rdf:resource="http://metadataregistry.org/uri/RegStatus/1001" />
  <reg:name xml:lang="en">productionStatement</reg:name>
  <rdfs:label xml:lang="en">has production statement</rdfs:label>
  <skos:definition xml:lang="en">Relates a resource to a statement identifying a place or places of production, producer or producers, and date or dates of production of a resource in an unpublished form.</skos:definition>
  <rdf:type rdf:resource="http://www.w3.org/1999/02/22-rdf-syntax-ns#Property" />
  <reg:hasSubproperty rdf:resource="http://rdaregistry.info/Elements/m/P30110" />
  <reg:lexicalAlias rdf:resource="http://rdaregistry.info/Elements/u/productionStatement.en" />
</owl:ObjectProperty>

<!-- Property: has product of merger -->
<owl:ObjectProperty rdf:about="http://rdaregistry.info/Elements/u/P60684">
  <rdfs:isDefinedBy rdf:resource="http://rdaregistry.info/Elements/u/" />
  <reg:status rdf:resource="http://metadataregistry.org/uri/RegStatus/1001" />
  <reg:name xml:lang="en">productOfAMerger</reg:name>
  <rdfs:label xml:lang="en">has product of merger</rdfs:label>
  <skos:definition xml:lang="en">Relates a agent that resulted from a merger of two or more other agents to an agent.</skos:definition>
  <rdf:type rdf:resource="http://www.w3.org/1999/02/22-rdf-syntax-ns#Property" />
  <owl:inverseOf rdf:resource="http://rdaregistry.info/Elements/u/P60736" />
  <reg:hasSubproperty rdf:resource="http://rdaregistry.info/Elements/a/P50013" />
  <reg:lexicalAlias rdf:resource="http://rdaregistry.info/Elements/u/productOfAMerger.en" />
</owl:ObjectProperty>

<!-- Property: has product of split -->
<owl:ObjectProperty rdf:about="http://rdaregistry.info/Elements/u/P60685">
  <rdfs:isDefinedBy rdf:resource="http://rdaregistry.info/Elements/u/" />
  <reg:status rdf:resource="http://metadataregistry.org/uri/RegStatus/1001" />
  <reg:name xml:lang="en">productOfASplit</reg:name>
  <rdfs:label xml:lang="en">has product of split</rdfs:label>
  <skos:definition xml:lang="en">Relates a agent that resulted from a split or division of another agent to an agent.</skos:definition>
  <rdf:type rdf:resource="http://www.w3.org/1999/02/22-rdf-syntax-ns#Property" />
  <owl:inverseOf rdf:resource="http://rdaregistry.info/Elements/u/P60733" />
  <reg:hasSubproperty rdf:resource="http://rdaregistry.info/Elements/a/P50014" />
  <reg:lexicalAlias rdf:resource="http://rdaregistry.info/Elements/u/productOfASplit.en" />
</owl:ObjectProperty>

<!-- Property: has profession or occupation -->
<owl:ObjectProperty rdf:about="http://rdaregistry.info/Elements/u/P60468">
  <rdfs:isDefinedBy rdf:resource="http://rdaregistry.info/Elements/u/" />
  <reg:status rdf:resource="http://metadataregistry.org/uri/RegStatus/1001" />
  <reg:name xml:lang="en">professionOrOccupation</reg:name>
  <rdfs:label xml:lang="en">has profession or occupation</rdfs:label>
  <skos:definition xml:lang="en">Relates a resource to an agent's vocation or avocation.</skos:definition>
  <rdf:type rdf:resource="http://www.w3.org/1999/02/22-rdf-syntax-ns#Property" />
  <reg:hasSubproperty rdf:resource="http://rdaregistry.info/Elements/a/P50104" />
  <reg:lexicalAlias rdf:resource="http://rdaregistry.info/Elements/u/professionOrOccupation.en" />
</owl:ObjectProperty>

<!-- Property: has programmer -->
<owl:ObjectProperty rdf:about="http://rdaregistry.info/Elements/u/P60423">
  <rdfs:isDefinedBy rdf:resource="http://rdaregistry.info/Elements/u/" />
  <reg:status rdf:resource="http://metadataregistry.org/uri/RegStatus/1001" />
  <reg:name xml:lang="en">programmer</reg:name>
  <rdfs:label xml:lang="en">has programmer</rdfs:label>
  <skos:definition xml:lang="en">Relates a resource to an agent responsible for creating a computer program.</skos:definition>
  <rdf:type rdf:resource="http://www.w3.org/1999/02/22-rdf-syntax-ns#Property" />
  <rdfs:subPropertyOf rdf:resource="http://rdaregistry.info/Elements/u/P60447" />
  <owl:inverseOf rdf:resource="http://rdaregistry.info/Elements/u/P60652" />
  <reg:lexicalAlias rdf:resource="http://rdaregistry.info/Elements/u/programmer.en" />
</owl:ObjectProperty>

<!-- Property: is programmer of -->
<owl:ObjectProperty rdf:about="http://rdaregistry.info/Elements/u/P60652">
  <rdfs:isDefinedBy rdf:resource="http://rdaregistry.info/Elements/u/" />
  <reg:status rdf:resource="http://metadataregistry.org/uri/RegStatus/1001" />
  <reg:name xml:lang="en">programmerOf</reg:name>
  <rdfs:label xml:lang="en">is programmer of</rdfs:label>
  <skos:definition xml:lang="en">Relates an agent responsible for creating a computer program to a resource.</skos:definition>
  <rdf:type rdf:resource="http://www.w3.org/1999/02/22-rdf-syntax-ns#Property" />
  <rdfs:subPropertyOf rdf:resource="http://rdaregistry.info/Elements/u/P60672" />
  <owl:inverseOf rdf:resource="http://rdaregistry.info/Elements/u/P60423" />
  <reg:hasSubproperty rdf:resource="http://rdaregistry.info/Elements/a/P50184" />
  <reg:lexicalAlias rdf:resource="http://rdaregistry.info/Elements/u/programmerOf.en" />
</owl:ObjectProperty>

<!-- Property: has projection characteristic of motion picture film -->
<owl:ObjectProperty rdf:about="http://rdaregistry.info/Elements/u/P60353">
  <rdfs:isDefinedBy rdf:resource="http://rdaregistry.info/Elements/u/" />
  <reg:status rdf:resource="http://metadataregistry.org/uri/RegStatus/1001" />
  <reg:name xml:lang="en">projectionCharacteristicOfMotionPictureFilm</reg:name>
  <rdfs:label xml:lang="en">has projection characteristic of motion picture film</rdfs:label>
  <skos:definition xml:lang="en">Relates a resource to a technical specification relating to the projection of a motion picture film.</skos:definition>
  <rdf:type rdf:resource="http://www.w3.org/1999/02/22-rdf-syntax-ns#Property" />
  <reg:hasSubproperty rdf:resource="http://rdaregistry.info/Elements/u/P60529" />
  <reg:hasSubproperty rdf:resource="http://rdaregistry.info/Elements/u/P60585" />
  <reg:hasSubproperty rdf:resource="http://rdaregistry.info/Elements/m/P30127" />
  <reg:lexicalAlias rdf:resource="http://rdaregistry.info/Elements/u/projectionCharacteristicOfMotionPictureFilm.en" />
</owl:ObjectProperty>

<!-- Property: has projection of cartographic content -->
<owl:ObjectProperty rdf:about="http://rdaregistry.info/Elements/u/P60542">
  <rdfs:isDefinedBy rdf:resource="http://rdaregistry.info/Elements/u/" />
  <reg:status rdf:resource="http://metadataregistry.org/uri/RegStatus/1001" />
  <reg:name xml:lang="en">projectionOfCartographicContent</reg:name>
  <rdfs:label xml:lang="en">has projection of cartographic content</rdfs:label>
  <skos:definition xml:lang="en">Relates a resource to a method or system used to represent the surface of the earth or of a celestial sphere on a plane.</skos:definition>
  <rdf:type rdf:resource="http://www.w3.org/1999/02/22-rdf-syntax-ns#Property" />
  <reg:hasSubproperty rdf:resource="http://rdaregistry.info/Elements/e/P20216" />
  <reg:lexicalAlias rdf:resource="http://rdaregistry.info/Elements/u/projectionOfCartographicContent.en" />
</owl:ObjectProperty>

<!-- Property: has projection speed -->
<owl:ObjectProperty rdf:about="http://rdaregistry.info/Elements/u/P60585">
  <rdfs:isDefinedBy rdf:resource="http://rdaregistry.info/Elements/u/" />
  <reg:status rdf:resource="http://metadataregistry.org/uri/RegStatus/1001" />
  <reg:name xml:lang="en">projectionSpeed</reg:name>
  <rdfs:label xml:lang="en">has projection speed</rdfs:label>
  <skos:definition xml:lang="en">Relates a resource to a speed at which a projected carrier must be operated to produce the moving image intended.</skos:definition>
  <rdf:type rdf:resource="http://www.w3.org/1999/02/22-rdf-syntax-ns#Property" />
  <rdfs:subPropertyOf rdf:resource="http://rdaregistry.info/Elements/u/P60353" />
  <reg:hasSubproperty rdf:resource="http://rdaregistry.info/Elements/m/P30200" />
  <reg:lexicalAlias rdf:resource="http://rdaregistry.info/Elements/u/projectionSpeed.en" />
</owl:ObjectProperty>

<!-- Property: has prominent member of agent -->
<owl:ObjectProperty rdf:about="http://rdaregistry.info/Elements/u/P60362">
  <rdfs:isDefinedBy rdf:resource="http://rdaregistry.info/Elements/u/" />
  <reg:status rdf:resource="http://metadataregistry.org/uri/RegStatus/1001" />
  <reg:name xml:lang="en">prominentMemberOfAgent</reg:name>
  <rdfs:label xml:lang="en">has prominent member of agent</rdfs:label>
  <skos:definition xml:lang="en">Relates a resource to a well-known individual who is a member of an agent.</skos:definition>
  <rdf:type rdf:resource="http://www.w3.org/1999/02/22-rdf-syntax-ns#Property" />
  <reg:hasSubproperty rdf:resource="http://rdaregistry.info/Elements/a/P50060" />
  <reg:lexicalAlias rdf:resource="http://rdaregistry.info/Elements/u/prominentMemberOfTheFamily.en" />
</owl:ObjectProperty>

<!-- Property: has publication statement -->
<owl:ObjectProperty rdf:about="http://rdaregistry.info/Elements/u/P60333">
  <rdfs:isDefinedBy rdf:resource="http://rdaregistry.info/Elements/u/" />
  <reg:status rdf:resource="http://metadataregistry.org/uri/RegStatus/1001" />
  <reg:name xml:lang="en">publicationStatement</reg:name>
  <rdfs:label xml:lang="en">has publication statement</rdfs:label>
  <skos:definition xml:lang="en">Relates a resource to a statement identifying a place or places of publication, publisher or publishers, and date or dates of publication of a resource.</skos:definition>
  <rdf:type rdf:resource="http://www.w3.org/1999/02/22-rdf-syntax-ns#Property" />
  <reg:hasSubproperty rdf:resource="http://rdaregistry.info/Elements/m/P30111" />
  <reg:lexicalAlias rdf:resource="http://rdaregistry.info/Elements/u/publicationStatement.en" />
</owl:ObjectProperty>

<!-- Property: has publisher -->
<owl:ObjectProperty rdf:about="http://rdaregistry.info/Elements/u/P60444">
  <rdfs:isDefinedBy rdf:resource="http://rdaregistry.info/Elements/u/" />
  <reg:status rdf:resource="http://metadataregistry.org/uri/RegStatus/1001" />
  <reg:name xml:lang="en">publisher</reg:name>
  <rdfs:label xml:lang="en">has publisher</rdfs:label>
  <skos:definition xml:lang="en">Relates a resource to an agent responsible for publishing, releasing, or issuing a resource.</skos:definition>
  <rdf:type rdf:resource="http://www.w3.org/1999/02/22-rdf-syntax-ns#Property" />
  <owl:inverseOf rdf:resource="http://rdaregistry.info/Elements/u/P60670" />
  <reg:hasSubproperty rdf:resource="http://rdaregistry.info/Elements/u/P60407" />
  <reg:hasSubproperty rdf:resource="http://rdaregistry.info/Elements/m/P30083" />
  <reg:lexicalAlias rdf:resource="http://rdaregistry.info/Elements/u/publisher.en" />
</owl:ObjectProperty>

<!-- Property: is publisher of -->
<owl:ObjectProperty rdf:about="http://rdaregistry.info/Elements/u/P60670">
  <rdfs:isDefinedBy rdf:resource="http://rdaregistry.info/Elements/u/" />
  <reg:status rdf:resource="http://metadataregistry.org/uri/RegStatus/1001" />
  <reg:name xml:lang="en">publisherOf</reg:name>
  <rdfs:label xml:lang="en">is publisher of</rdfs:label>
  <skos:definition xml:lang="en">Relates an agent responsible for publishing, releasing, or issuing a resource to a resource.</skos:definition>
  <rdf:type rdf:resource="http://www.w3.org/1999/02/22-rdf-syntax-ns#Property" />
  <owl:inverseOf rdf:resource="http://rdaregistry.info/Elements/u/P60444" />
  <reg:hasSubproperty rdf:resource="http://rdaregistry.info/Elements/u/P60635" />
  <reg:hasSubproperty rdf:resource="http://rdaregistry.info/Elements/a/P50203" />
  <reg:lexicalAlias rdf:resource="http://rdaregistry.info/Elements/u/publisherOf.en" />
</owl:ObjectProperty>

<!-- Property: has publishers name -->
<owl:ObjectProperty rdf:about="http://rdaregistry.info/Elements/u/P60547">
  <rdfs:isDefinedBy rdf:resource="http://rdaregistry.info/Elements/u/" />
  <reg:status rdf:resource="http://metadataregistry.org/uri/RegStatus/1001" />
  <reg:name xml:lang="en">publishersName</reg:name>
  <rdfs:label xml:lang="en">has publishers name</rdfs:label>
  <skos:definition xml:lang="en">Relates a resource to a name of an agent responsible for publishing, releasing, or issuing a resource.</skos:definition>
  <rdf:type rdf:resource="http://www.w3.org/1999/02/22-rdf-syntax-ns#Property" />
  <reg:hasSubproperty rdf:resource="http://rdaregistry.info/Elements/m/P30176" />
  <reg:lexicalAlias rdf:resource="http://rdaregistry.info/Elements/u/publishersName.en" />
</owl:ObjectProperty>

<!-- Property: has publishers number for music -->
<owl:ObjectProperty rdf:about="http://rdaregistry.info/Elements/u/P60139">
  <rdfs:isDefinedBy rdf:resource="http://rdaregistry.info/Elements/u/" />
  <reg:status rdf:resource="http://metadataregistry.org/uri/RegStatus/1001" />
  <reg:name xml:lang="en">publishersNumberForMusic</reg:name>
  <rdfs:label xml:lang="en">has publishers number for music</rdfs:label>
  <skos:definition xml:lang="en">Relates a resource to a numbering designation assigned to a notated music resource by a publisher.</skos:definition>
  <rdf:type rdf:resource="http://www.w3.org/1999/02/22-rdf-syntax-ns#Property" />
  <rdfs:subPropertyOf rdf:resource="http://rdaregistry.info/Elements/u/P60052" />
  <reg:hasSubproperty rdf:resource="http://rdaregistry.info/Elements/m/P30065" />
  <reg:lexicalAlias rdf:resource="http://rdaregistry.info/Elements/u/publishersNumberForMusic.en" />
  <skos:scopeNote xml:lang="en">A publishers number for notated music sometimes includes initials, abbreviations, or words identifying the publisher.</skos:scopeNote>
</owl:ObjectProperty>

<!-- Property: has puppeteer -->
<owl:ObjectProperty rdf:about="http://rdaregistry.info/Elements/u/P60148">
  <rdfs:isDefinedBy rdf:resource="http://rdaregistry.info/Elements/u/" />
  <reg:status rdf:resource="http://metadataregistry.org/uri/RegStatus/1001" />
  <reg:name xml:lang="en">puppeteer</reg:name>
  <rdfs:label xml:lang="en">has puppeteer</rdfs:label>
  <skos:definition xml:lang="en">Relates a resource to a performer contributing to a resource by manipulating, controlling, or directing puppets or marionettes in a moving image production or a musical or dramatic presentation or entertainment.</skos:definition>
  <rdf:type rdf:resource="http://www.w3.org/1999/02/22-rdf-syntax-ns#Property" />
  <rdfs:subPropertyOf rdf:resource="http://rdaregistry.info/Elements/u/P60387" />
  <owl:inverseOf rdf:resource="http://rdaregistry.info/Elements/u/P60023" />
  <reg:hasSubproperty rdf:resource="http://rdaregistry.info/Elements/e/P20018" />
  <reg:lexicalAlias rdf:resource="http://rdaregistry.info/Elements/u/puppeteer.en" />
</owl:ObjectProperty>

<!-- Property: is puppeteer of -->
<owl:ObjectProperty rdf:about="http://rdaregistry.info/Elements/u/P60023">
  <rdfs:isDefinedBy rdf:resource="http://rdaregistry.info/Elements/u/" />
  <reg:status rdf:resource="http://metadataregistry.org/uri/RegStatus/1001" />
  <reg:name xml:lang="en">puppeteerOf</reg:name>
  <rdfs:label xml:lang="en">is puppeteer of</rdfs:label>
  <skos:definition xml:lang="en">Relates a performer contributing to a resource by manipulating, controlling, or directing puppets or marionettes in a moving image production or a musical or dramatic presentation or entertainment to a resource.</skos:definition>
  <rdf:type rdf:resource="http://www.w3.org/1999/02/22-rdf-syntax-ns#Property" />
  <rdfs:subPropertyOf rdf:resource="http://rdaregistry.info/Elements/u/P60615" />
  <owl:inverseOf rdf:resource="http://rdaregistry.info/Elements/u/P60148" />
  <reg:hasSubproperty rdf:resource="http://rdaregistry.info/Elements/a/P50077" />
  <reg:lexicalAlias rdf:resource="http://rdaregistry.info/Elements/u/puppeteerOf.en" />
</owl:ObjectProperty>

<!-- Property: is radio adaptation of -->
<owl:ObjectProperty rdf:about="http://rdaregistry.info/Elements/u/P60229">
  <rdfs:isDefinedBy rdf:resource="http://rdaregistry.info/Elements/u/" />
  <reg:status rdf:resource="http://metadataregistry.org/uri/RegStatus/1001" />
  <reg:name xml:lang="en">radioAdaptationOf</reg:name>
  <rdfs:label xml:lang="en">is radio adaptation of</rdfs:label>
  <skos:definition xml:lang="en">Relates a resource to a resource that has been adapted as a radio program.</skos:definition>
  <rdf:type rdf:resource="http://www.w3.org/1999/02/22-rdf-syntax-ns#Property" />
  <rdfs:subPropertyOf rdf:resource="http://rdaregistry.info/Elements/u/P60241" />
  <owl:inverseOf rdf:resource="http://rdaregistry.info/Elements/u/P60174" />
  <reg:hasSubproperty rdf:resource="http://rdaregistry.info/Elements/e/P20127" />
  <reg:lexicalAlias rdf:resource="http://rdaregistry.info/Elements/u/radioAdaptationOf.en" />
</owl:ObjectProperty>

<!-- Property: has radio director -->
<owl:ObjectProperty rdf:about="http://rdaregistry.info/Elements/u/P60085">
  <rdfs:isDefinedBy rdf:resource="http://rdaregistry.info/Elements/u/" />
  <reg:status rdf:resource="http://metadataregistry.org/uri/RegStatus/1001" />
  <reg:name xml:lang="en">radioDirector</reg:name>
  <rdfs:label xml:lang="en">has radio director</rdfs:label>
  <skos:definition xml:lang="en">Relates a resource to a director responsible for the general management and supervision of a radio program.</skos:definition>
  <rdf:type rdf:resource="http://www.w3.org/1999/02/22-rdf-syntax-ns#Property" />
  <rdfs:subPropertyOf rdf:resource="http://rdaregistry.info/Elements/u/P60449" />
  <owl:inverseOf rdf:resource="http://rdaregistry.info/Elements/u/P60010" />
  <reg:lexicalAlias rdf:resource="http://rdaregistry.info/Elements/u/radioDirector.en" />
</owl:ObjectProperty>

<!-- Property: is radio director of -->
<owl:ObjectProperty rdf:about="http://rdaregistry.info/Elements/u/P60010">
  <rdfs:isDefinedBy rdf:resource="http://rdaregistry.info/Elements/u/" />
  <reg:status rdf:resource="http://metadataregistry.org/uri/RegStatus/1001" />
  <reg:name xml:lang="en">radioDirectorOf</reg:name>
  <rdfs:label xml:lang="en">is radio director of</rdfs:label>
  <skos:definition xml:lang="en">Relates a director responsible for the general management and supervision of a radio program to a resource.</skos:definition>
  <rdf:type rdf:resource="http://www.w3.org/1999/02/22-rdf-syntax-ns#Property" />
  <rdfs:subPropertyOf rdf:resource="http://rdaregistry.info/Elements/u/P60673" />
  <owl:inverseOf rdf:resource="http://rdaregistry.info/Elements/u/P60085" />
  <reg:hasSubproperty rdf:resource="http://rdaregistry.info/Elements/a/P50049" />
  <reg:lexicalAlias rdf:resource="http://rdaregistry.info/Elements/u/radioDirectorOf.en" />
</owl:ObjectProperty>

<!-- Property: has radio producer -->
<owl:ObjectProperty rdf:about="http://rdaregistry.info/Elements/u/P60170">
  <rdfs:isDefinedBy rdf:resource="http://rdaregistry.info/Elements/u/" />
  <reg:status rdf:resource="http://metadataregistry.org/uri/RegStatus/1001" />
  <reg:name xml:lang="en">radioProducer</reg:name>
  <rdfs:label xml:lang="en">has radio producer</rdfs:label>
  <skos:definition xml:lang="en">Relates a resource to a producer responsible for most of the business aspects of a radio program.</skos:definition>
  <rdf:type rdf:resource="http://www.w3.org/1999/02/22-rdf-syntax-ns#Property" />
  <rdfs:subPropertyOf rdf:resource="http://rdaregistry.info/Elements/u/P60441" />
  <owl:inverseOf rdf:resource="http://rdaregistry.info/Elements/u/P60034" />
  <reg:lexicalAlias rdf:resource="http://rdaregistry.info/Elements/u/radioProducer.en" />
</owl:ObjectProperty>

<!-- Property: is radio producer of -->
<owl:ObjectProperty rdf:about="http://rdaregistry.info/Elements/u/P60034">
  <rdfs:isDefinedBy rdf:resource="http://rdaregistry.info/Elements/u/" />
  <reg:status rdf:resource="http://metadataregistry.org/uri/RegStatus/1001" />
  <reg:name xml:lang="en">radioProducerOf</reg:name>
  <rdfs:label xml:lang="en">is radio producer of</rdfs:label>
  <skos:definition xml:lang="en">Relates a producer responsible for most of the business aspects of a radio program to a resource.</skos:definition>
  <rdf:type rdf:resource="http://www.w3.org/1999/02/22-rdf-syntax-ns#Property" />
  <rdfs:subPropertyOf rdf:resource="http://rdaregistry.info/Elements/u/P60668" />
  <owl:inverseOf rdf:resource="http://rdaregistry.info/Elements/u/P60170" />
  <reg:hasSubproperty rdf:resource="http://rdaregistry.info/Elements/a/P50214" />
  <reg:lexicalAlias rdf:resource="http://rdaregistry.info/Elements/u/radioProducerOf.en" />
</owl:ObjectProperty>

<!-- Property: is radio program music -->
<owl:ObjectProperty rdf:about="http://rdaregistry.info/Elements/u/P60729">
  <rdfs:isDefinedBy rdf:resource="http://rdaregistry.info/Elements/u/" />
  <reg:status rdf:resource="http://metadataregistry.org/uri/RegStatus/1001" />
  <reg:name xml:lang="en">radioProgramMusic</reg:name>
  <rdfs:label xml:lang="en">is radio program music</rdfs:label>
  <skos:definition xml:lang="en">Relates a resource to a musical resource that is used in a radio program.</skos:definition>
  <rdf:type rdf:resource="http://www.w3.org/1999/02/22-rdf-syntax-ns#Property" />
  <rdfs:subPropertyOf rdf:resource="http://rdaregistry.info/Elements/u/P60723" />
  <owl:inverseOf rdf:resource="http://rdaregistry.info/Elements/u/P60730" />
  <reg:hasSubproperty rdf:resource="http://rdaregistry.info/Elements/e/P20249" />
  <reg:lexicalAlias rdf:resource="http://rdaregistry.info/Elements/u/radioProgramMusic.en" />
</owl:ObjectProperty>

<!-- Property: is radio script -->
<owl:ObjectProperty rdf:about="http://rdaregistry.info/Elements/u/P60267">
  <rdfs:isDefinedBy rdf:resource="http://rdaregistry.info/Elements/u/" />
  <reg:status rdf:resource="http://metadataregistry.org/uri/RegStatus/1001" />
  <reg:name xml:lang="en">radioScript</reg:name>
  <rdfs:label xml:lang="en">is radio script</rdfs:label>
  <skos:definition xml:lang="en">Relates a resource to a resource that provides text for a radio program.</skos:definition>
  <rdf:type rdf:resource="http://www.w3.org/1999/02/22-rdf-syntax-ns#Property" />
  <rdfs:subPropertyOf rdf:resource="http://rdaregistry.info/Elements/u/P60198" />
  <owl:inverseOf rdf:resource="http://rdaregistry.info/Elements/u/P60285" />
  <reg:hasSubproperty rdf:resource="http://rdaregistry.info/Elements/e/P20160" />
  <reg:lexicalAlias rdf:resource="http://rdaregistry.info/Elements/u/radioScript.en" />
</owl:ObjectProperty>

<!-- Property: is radio script based on -->
<owl:ObjectProperty rdf:about="http://rdaregistry.info/Elements/u/P60235">
  <rdfs:isDefinedBy rdf:resource="http://rdaregistry.info/Elements/u/" />
  <reg:status rdf:resource="http://metadataregistry.org/uri/RegStatus/1001" />
  <reg:name xml:lang="en">radioScriptBasedOn</reg:name>
  <rdfs:label xml:lang="en">is radio script based on</rdfs:label>
  <skos:definition xml:lang="en">Relates a resource to a resource that has been adapted as a script for a radio program.</skos:definition>
  <rdf:type rdf:resource="http://www.w3.org/1999/02/22-rdf-syntax-ns#Property" />
  <rdfs:subPropertyOf rdf:resource="http://rdaregistry.info/Elements/u/P60241" />
  <owl:inverseOf rdf:resource="http://rdaregistry.info/Elements/u/P60188" />
  <reg:hasSubproperty rdf:resource="http://rdaregistry.info/Elements/e/P20133" />
  <reg:lexicalAlias rdf:resource="http://rdaregistry.info/Elements/u/radioScriptBasedOn.en" />
</owl:ObjectProperty>

<!-- Property: has rapporteur -->
<owl:ObjectProperty rdf:about="http://rdaregistry.info/Elements/u/P60751">
  <rdfs:isDefinedBy rdf:resource="http://rdaregistry.info/Elements/u/" />
  <reg:status rdf:resource="http://metadataregistry.org/uri/RegStatus/1001" />
  <rdf:type rdf:resource="http://www.w3.org/1999/02/22-rdf-syntax-ns#Property" />
  <reg:name xml:lang="en">rapporteur</reg:name>
  <rdfs:label xml:lang="en">has rapporteur</rdfs:label>
  <reg:lexicalAlias rdf:resource="http://rdaregistry.info/Elements/u/rapporteur.en" />
  <skos:definition xml:lang="en">Relates a resource to an author who is appointed by an organization to report on the proceedings of its meetings.</skos:definition>
  <owl:inverseOf rdf:resource="http://rdaregistry.info/Elements/u/P60757" />
  <skos:scopeNote xml:lang="en">Responsibility limited to taking minutes is excluded.</skos:scopeNote>
  <rdfs:subPropertyOf rdf:resource="http://rdaregistry.info/Elements/u/P60434" />
  <rdakit:seeAlso rdf:resource="http://rdaregistry.info/Elements/u/P60446" />
</owl:ObjectProperty>

<!-- Property: is rapporteur of -->
<owl:ObjectProperty rdf:about="http://rdaregistry.info/Elements/u/P60757">
  <rdfs:isDefinedBy rdf:resource="http://rdaregistry.info/Elements/u/" />
  <reg:status rdf:resource="http://metadataregistry.org/uri/RegStatus/1001" />
  <rdf:type rdf:resource="http://www.w3.org/1999/02/22-rdf-syntax-ns#Property" />
  <reg:name xml:lang="en">rapporteurOf</reg:name>
  <rdfs:label xml:lang="en">is rapporteur of</rdfs:label>
  <reg:lexicalAlias rdf:resource="http://rdaregistry.info/Elements/u/rapporteurOf.en" />
  <skos:definition xml:lang="en">Relates an author who is appointed by an organization to report on the proceedings of its meetings to a resource.</skos:definition>
  <owl:inverseOf rdf:resource="http://rdaregistry.info/Elements/u/P60751" />
  <rdfs:subPropertyOf rdf:resource="http://rdaregistry.info/Elements/u/P60663" />
  <rdakit:seeAlso rdf:resource="http://rdaregistry.info/Elements/u/P60708" />
</owl:ObjectProperty>

<!-- Property: has real identity -->
<owl:ObjectProperty rdf:about="http://rdaregistry.info/Elements/u/P60037">
  <rdfs:isDefinedBy rdf:resource="http://rdaregistry.info/Elements/u/" />
  <reg:status rdf:resource="http://metadataregistry.org/uri/RegStatus/1001" />
  <reg:name xml:lang="en">realIdentity</reg:name>
  <rdfs:label xml:lang="en">has real identity</rdfs:label>
  <skos:definition xml:lang="en">Relates a real agent who assumes an alternate identity to an agent.</skos:definition>
  <rdf:type rdf:resource="http://www.w3.org/1999/02/22-rdf-syntax-ns#Property" />
  <owl:inverseOf rdf:resource="http://rdaregistry.info/Elements/u/P60036" />
  <reg:hasSubproperty rdf:resource="http://rdaregistry.info/Elements/a/P50106" />
  <reg:lexicalAlias rdf:resource="http://rdaregistry.info/Elements/u/realIdentity.en" />
</owl:ObjectProperty>

<!-- Property: has recording engineer -->
<owl:ObjectProperty rdf:about="http://rdaregistry.info/Elements/u/P60395">
  <rdfs:isDefinedBy rdf:resource="http://rdaregistry.info/Elements/u/" />
  <reg:status rdf:resource="http://metadataregistry.org/uri/RegStatus/1001" />
  <reg:name xml:lang="en">recordingEngineer</reg:name>
  <rdfs:label xml:lang="en">has recording engineer</rdfs:label>
  <skos:definition xml:lang="en">Relates a resource to an agent contributing to a resource by supervising the technical aspects of a sound or video recording session.</skos:definition>
  <rdf:type rdf:resource="http://www.w3.org/1999/02/22-rdf-syntax-ns#Property" />
  <rdfs:subPropertyOf rdf:resource="http://rdaregistry.info/Elements/u/P60398" />
  <owl:inverseOf rdf:resource="http://rdaregistry.info/Elements/u/P60623" />
  <reg:hasSubproperty rdf:resource="http://rdaregistry.info/Elements/e/P20050" />
  <reg:lexicalAlias rdf:resource="http://rdaregistry.info/Elements/u/recordingEngineer.en" />
</owl:ObjectProperty>

<!-- Property: is recording engineer of -->
<owl:ObjectProperty rdf:about="http://rdaregistry.info/Elements/u/P60623">
  <rdfs:isDefinedBy rdf:resource="http://rdaregistry.info/Elements/u/" />
  <reg:status rdf:resource="http://metadataregistry.org/uri/RegStatus/1001" />
  <reg:name xml:lang="en">recordingEngineerOf</reg:name>
  <rdfs:label xml:lang="en">is recording engineer of</rdfs:label>
  <skos:definition xml:lang="en">Relates an agent contributing to a resource by supervising the technical aspects of a sound or video recording session to a resource.</skos:definition>
  <rdf:type rdf:resource="http://www.w3.org/1999/02/22-rdf-syntax-ns#Property" />
  <rdfs:subPropertyOf rdf:resource="http://rdaregistry.info/Elements/u/P60626" />
  <owl:inverseOf rdf:resource="http://rdaregistry.info/Elements/u/P60395" />
  <reg:hasSubproperty rdf:resource="http://rdaregistry.info/Elements/a/P50158" />
  <reg:lexicalAlias rdf:resource="http://rdaregistry.info/Elements/u/recordingEngineerOf.en" />
</owl:ObjectProperty>

<!-- Property: has recording medium -->
<owl:ObjectProperty rdf:about="http://rdaregistry.info/Elements/u/P60594">
  <rdfs:isDefinedBy rdf:resource="http://rdaregistry.info/Elements/u/" />
  <reg:status rdf:resource="http://metadataregistry.org/uri/RegStatus/1001" />
  <reg:name xml:lang="en">recordingMedium</reg:name>
  <rdfs:label xml:lang="en">has recording medium</rdfs:label>
  <skos:definition xml:lang="en">Relates a resource to a type of medium used to record sound on an audio carrier.</skos:definition>
  <rdf:type rdf:resource="http://www.w3.org/1999/02/22-rdf-syntax-ns#Property" />
  <rdfs:subPropertyOf rdf:resource="http://rdaregistry.info/Elements/u/P60351" />
  <reg:hasSubproperty rdf:resource="http://rdaregistry.info/Elements/m/P30206" />
  <reg:lexicalAlias rdf:resource="http://rdaregistry.info/Elements/u/recordingMedium.en" />
</owl:ObjectProperty>

<!-- Property: has recordist -->
<owl:ObjectProperty rdf:about="http://rdaregistry.info/Elements/u/P60397">
  <rdfs:isDefinedBy rdf:resource="http://rdaregistry.info/Elements/u/" />
  <reg:status rdf:resource="http://metadataregistry.org/uri/RegStatus/1001" />
  <reg:name xml:lang="en">recordist</reg:name>
  <rdfs:label xml:lang="en">has recordist</rdfs:label>
  <skos:definition xml:lang="en">Relates a resource to an agent contributing to a resource by using a recording device to capture sound or video during a recording session, including field recordings of natural sounds, folkloric events, music, etc.</skos:definition>
  <rdf:type rdf:resource="http://www.w3.org/1999/02/22-rdf-syntax-ns#Property" />
  <rdfs:subPropertyOf rdf:resource="http://rdaregistry.info/Elements/u/P60398" />
  <owl:inverseOf rdf:resource="http://rdaregistry.info/Elements/u/P60625" />
  <reg:hasSubproperty rdf:resource="http://rdaregistry.info/Elements/e/P20052" />
  <reg:lexicalAlias rdf:resource="http://rdaregistry.info/Elements/u/recordist.en" />
</owl:ObjectProperty>

<!-- Property: is recordist of -->
<owl:ObjectProperty rdf:about="http://rdaregistry.info/Elements/u/P60625">
  <rdfs:isDefinedBy rdf:resource="http://rdaregistry.info/Elements/u/" />
  <reg:status rdf:resource="http://metadataregistry.org/uri/RegStatus/1001" />
  <reg:name xml:lang="en">recordistOf</reg:name>
  <rdfs:label xml:lang="en">is recordist of</rdfs:label>
  <skos:definition xml:lang="en">Relates an agent contributing to a resource by using a recording device to capture sound or video during a recording session, including field recordings of natural sounds, folkloric events, music, etc. to a resource.</skos:definition>
  <rdf:type rdf:resource="http://www.w3.org/1999/02/22-rdf-syntax-ns#Property" />
  <rdfs:subPropertyOf rdf:resource="http://rdaregistry.info/Elements/u/P60626" />
  <owl:inverseOf rdf:resource="http://rdaregistry.info/Elements/u/P60397" />
  <reg:hasSubproperty rdf:resource="http://rdaregistry.info/Elements/a/P50160" />
  <reg:lexicalAlias rdf:resource="http://rdaregistry.info/Elements/u/recordistOf.en" />
</owl:ObjectProperty>

<!-- Property: has reduction ratio -->
<owl:ObjectProperty rdf:about="http://rdaregistry.info/Elements/u/P60581">
  <rdfs:isDefinedBy rdf:resource="http://rdaregistry.info/Elements/u/" />
  <reg:status rdf:resource="http://metadataregistry.org/uri/RegStatus/1001" />
  <reg:name xml:lang="en">reductionRatio</reg:name>
  <rdfs:label xml:lang="en">has reduction ratio</rdfs:label>
  <skos:definition xml:lang="en">Relates a resource to a numerical ratio of the size of a micro-image in relation to an original from which it was produced.</skos:definition>
  <rdf:type rdf:resource="http://www.w3.org/1999/02/22-rdf-syntax-ns#Property" />
  <reg:hasSubproperty rdf:resource="http://rdaregistry.info/Elements/m/P30198" />
  <reg:lexicalAlias rdf:resource="http://rdaregistry.info/Elements/u/reductionRatio.en" />
</owl:ObjectProperty>

<!-- Property: has reduction ratio designation -->
<owl:ObjectProperty rdf:about="http://rdaregistry.info/Elements/u/P60877">
  <rdfs:isDefinedBy rdf:resource="http://rdaregistry.info/Elements/u/" />
  <reg:status rdf:resource="http://metadataregistry.org/uri/RegStatus/1001" />
  <rdf:type rdf:resource="http://www.w3.org/1999/02/22-rdf-syntax-ns#Property" />
  <reg:name xml:lang="en">reductionRatioDesignation</reg:name>
  <rdfs:label xml:lang="en">has reduction ratio designation</rdfs:label>
  <reg:lexicalAlias rdf:resource="http://rdaregistry.info/Elements/u/reductionRatioDesignation.en" />
  <skos:definition xml:lang="en">Relates a resource to a general designation of the size of a micro-image in relation to an original from which it was produced.</skos:definition>
  <reg:hasSubproperty rdf:resource="http://rdaregistry.info/Elements/m/P30263" />
</owl:ObjectProperty>

<!-- Property: has referential resource relationship with -->
<owl:ObjectProperty rdf:about="http://rdaregistry.info/Elements/u/P60848">
  <rdfs:isDefinedBy rdf:resource="http://rdaregistry.info/Elements/u/" />
  <reg:status rdf:resource="http://metadataregistry.org/uri/RegStatus/1001" />
  <rdf:type rdf:resource="http://www.w3.org/1999/02/22-rdf-syntax-ns#Property" />
  <reg:name xml:lang="en">referentialResourceRelationship</reg:name>
  <rdfs:label xml:lang="en">has referential resource relationship with</rdfs:label>
  <reg:lexicalAlias rdf:resource="http://rdaregistry.info/Elements/u/referentialResourceRelationship.en" />
  <skos:definition xml:lang="en">Relates a resource to a resource that references a resource.</skos:definition>
  <owl:inverseOf rdf:resource="http://rdaregistry.info/Elements/u/P60848" />
  <reg:hasSubproperty rdf:resource="http://rdaregistry.info/Elements/u/P60846" />
  <reg:hasSubproperty rdf:resource="http://rdaregistry.info/Elements/u/P60847" />
</owl:ObjectProperty>

<!-- Property: has regional encoding -->
<owl:ObjectProperty rdf:about="http://rdaregistry.info/Elements/u/P60059">
  <rdfs:isDefinedBy rdf:resource="http://rdaregistry.info/Elements/u/" />
  <reg:status rdf:resource="http://metadataregistry.org/uri/RegStatus/1001" />
  <reg:name xml:lang="en">regionalEncoding</reg:name>
  <rdfs:label xml:lang="en">has regional encoding</rdfs:label>
  <skos:definition xml:lang="en">Relates a resource to a code identifying a region of the world for which a videodisc has been encoded and preventing the disc from being played on a player sold in a different region.</skos:definition>
  <rdf:type rdf:resource="http://www.w3.org/1999/02/22-rdf-syntax-ns#Property" />
  <rdfs:subPropertyOf rdf:resource="http://rdaregistry.info/Elements/u/P60350" />
  <reg:hasSubproperty rdf:resource="http://rdaregistry.info/Elements/m/P30006" />
  <reg:lexicalAlias rdf:resource="http://rdaregistry.info/Elements/u/regionalEncoding.en" />
</owl:ObjectProperty>

<!-- Property: has related agent -->
<owl:ObjectProperty rdf:about="http://rdaregistry.info/Elements/u/P60454">
  <rdfs:isDefinedBy rdf:resource="http://rdaregistry.info/Elements/u/" />
  <reg:status rdf:resource="http://metadataregistry.org/uri/RegStatus/1001" />
  <reg:name xml:lang="en">relatedAgent</reg:name>
  <rdfs:label xml:lang="en">has related agent</rdfs:label>
  <skos:definition xml:lang="en">Relates an agent to an agent that is associated with an agent being described.</skos:definition>
  <rdf:type rdf:resource="http://www.w3.org/1999/02/22-rdf-syntax-ns#Property" />
  <reg:lexicalAlias rdf:resource="http://rdaregistry.info/Elements/u/relatedAgent.en" />
  <reg:hasSubproperty rdf:resource="http://rdaregistry.info/Elements/u/P60737" />
  <reg:hasSubproperty rdf:resource="http://rdaregistry.info/Elements/u/P60853" />
  <reg:hasSubproperty rdf:resource="http://rdaregistry.info/Elements/u/P60854" />
  <reg:hasSubproperty rdf:resource="http://rdaregistry.info/Elements/u/P60855" />
  <reg:hasSubproperty rdf:resource="http://rdaregistry.info/Elements/u/P60856" />
  <reg:hasSubproperty rdf:resource="http://rdaregistry.info/Elements/u/P60861" />
  <reg:hasSubproperty rdf:resource="http://rdaregistry.info/Elements/u/P60862" />
  <reg:hasSubproperty rdf:resource="http://rdaregistry.info/Elements/u/P60863" />
  <reg:hasSubproperty rdf:resource="http://rdaregistry.info/Elements/u/P60633" />
</owl:ObjectProperty>

<!-- Property: has related resource -->
<owl:ObjectProperty rdf:about="http://rdaregistry.info/Elements/u/P60313">
  <rdfs:isDefinedBy rdf:resource="http://rdaregistry.info/Elements/u/" />
  <reg:status rdf:resource="http://metadataregistry.org/uri/RegStatus/1001" />
  <reg:name xml:lang="en">relatedResource</reg:name>
  <rdfs:label xml:lang="en">has related resource</rdfs:label>
  <skos:definition xml:lang="en">Relates a resource to a resource that is related to a resource being described.</skos:definition>
  <rdf:type rdf:resource="http://www.w3.org/1999/02/22-rdf-syntax-ns#Property" />
  <reg:hasSubproperty rdf:resource="http://rdaregistry.info/Elements/e/P20205" />
  <reg:hasSubproperty rdf:resource="http://rdaregistry.info/Elements/m/P30048" />
  <reg:hasSubproperty rdf:resource="http://rdaregistry.info/Elements/m/P30140" />
  <reg:lexicalAlias rdf:resource="http://rdaregistry.info/Elements/u/relatedResource.en" />
  <reg:hasSubproperty rdf:resource="http://rdaregistry.info/Elements/m/P30265" />
  <reg:hasSubproperty rdf:resource="http://rdaregistry.info/Elements/m/P30266" />
  <reg:hasSubproperty rdf:resource="http://rdaregistry.info/Elements/i/P40046" />
  <reg:hasSubproperty rdf:resource="http://rdaregistry.info/Elements/i/P40069" />
  <reg:hasSubproperty rdf:resource="http://rdaregistry.info/Elements/i/P40070" />
  <reg:hasSubproperty rdf:resource="http://rdaregistry.info/Elements/i/P40071" />
</owl:ObjectProperty>

<!-- Property: is remade as -->
<owl:ObjectProperty rdf:about="http://rdaregistry.info/Elements/u/P60120">
  <rdfs:isDefinedBy rdf:resource="http://rdaregistry.info/Elements/u/" />
  <reg:status rdf:resource="http://metadataregistry.org/uri/RegStatus/1001" />
  <reg:name xml:lang="en">remadeAs</reg:name>
  <rdfs:label xml:lang="en">is remade as</rdfs:label>
  <skos:definition xml:lang="en">Relates a resource to a motion picture, radio program, television program, or video based on an earlier resource.</skos:definition>
  <rdf:type rdf:resource="http://www.w3.org/1999/02/22-rdf-syntax-ns#Property" />
  <rdfs:subPropertyOf rdf:resource="http://rdaregistry.info/Elements/u/P60250" />
  <owl:inverseOf rdf:resource="http://rdaregistry.info/Elements/u/P60295" />
  <reg:hasSubproperty rdf:resource="http://rdaregistry.info/Elements/e/P20086" />
  <reg:lexicalAlias rdf:resource="http://rdaregistry.info/Elements/u/remadeAs.en" />
</owl:ObjectProperty>

<!-- Property: is remake of -->
<owl:ObjectProperty rdf:about="http://rdaregistry.info/Elements/u/P60295">
  <rdfs:isDefinedBy rdf:resource="http://rdaregistry.info/Elements/u/" />
  <reg:status rdf:resource="http://metadataregistry.org/uri/RegStatus/1001" />
  <reg:name xml:lang="en">remakeOf</reg:name>
  <rdfs:label xml:lang="en">is remake of</rdfs:label>
  <skos:definition xml:lang="en">Relates a resource to a resource used as a basis for a new motion picture, radio program, television program, or video.</skos:definition>
  <rdf:type rdf:resource="http://www.w3.org/1999/02/22-rdf-syntax-ns#Property" />
  <rdfs:subPropertyOf rdf:resource="http://rdaregistry.info/Elements/u/P60305" />
  <owl:inverseOf rdf:resource="http://rdaregistry.info/Elements/u/P60120" />
  <reg:hasSubproperty rdf:resource="http://rdaregistry.info/Elements/e/P20185" />
  <reg:lexicalAlias rdf:resource="http://rdaregistry.info/Elements/u/remakeOf.en" />
</owl:ObjectProperty>

<!-- Property: has remix artist -->
<owl:ObjectProperty rdf:about="http://rdaregistry.info/Elements/u/P60891">
  <rdfs:isDefinedBy rdf:resource="http://rdaregistry.info/Elements/u/" />
  <reg:status rdf:resource="http://metadataregistry.org/uri/RegStatus/1001" />
  <rdf:type rdf:resource="http://www.w3.org/1999/02/22-rdf-syntax-ns#Property" />
  <reg:name xml:lang="en">remixArtist</reg:name>
  <rdfs:label xml:lang="en">has remix artist</rdfs:label>
  <reg:lexicalAlias rdf:resource="http://rdaregistry.info/Elements/u/remixArtist.en" />
  <skos:definition xml:lang="en">Relates a resource to an agent responsible for creating an audio resource by manipulating, recombining, mixing, and reproducing previously recorded sounds.</skos:definition>
  <skos:scopeNote xml:lang="en">Remixing activities that do not substantially change the nature and content of the original resource, and mixing recorded tracks together to appear as one continuous track are excluded.</skos:scopeNote>
  <owl:inverseOf rdf:resource="http://rdaregistry.info/Elements/u/P60881" />
  <reg:hasSubproperty rdf:resource="http://rdaregistry.info/Elements/w/P10306" />
  <rdfs:subPropertyOf rdf:resource="http://rdaregistry.info/Elements/u/P60447" />
  <rdakit:seeAlso rdf:resource="http://rdaregistry.info/Elements/u/P60896" />
</owl:ObjectProperty>

<!-- Property: is remix artist of -->
<owl:ObjectProperty rdf:about="http://rdaregistry.info/Elements/u/P60881">
  <rdfs:isDefinedBy rdf:resource="http://rdaregistry.info/Elements/u/" />
  <reg:status rdf:resource="http://metadataregistry.org/uri/RegStatus/1001" />
  <rdf:type rdf:resource="http://www.w3.org/1999/02/22-rdf-syntax-ns#Property" />
  <reg:name xml:lang="en">remixArtistOf</reg:name>
  <rdfs:label xml:lang="en">is remix artist of</rdfs:label>
  <reg:lexicalAlias rdf:resource="http://rdaregistry.info/Elements/u/remixArtistOf.en" />
  <skos:definition xml:lang="en">Relates an agent to an audio resource created by manipulating, recombining, mixing, and reproducing previously recorded sounds to a resource.</skos:definition>
  <skos:scopeNote xml:lang="en">Remixing activities that do not substantially change the nature and content of the original resource, and mixing recorded tracks together to appear as one continuous track are excluded.</skos:scopeNote>
  <owl:inverseOf rdf:resource="http://rdaregistry.info/Elements/u/P60891" />
  <rdfs:subPropertyOf rdf:resource="http://rdaregistry.info/Elements/u/P60672" />
  <reg:hasSubproperty rdf:resource="http://rdaregistry.info/Elements/a/P50293" />
  <rdakit:seeAlso rdf:resource="http://rdaregistry.info/Elements/u/P60886" />
</owl:ObjectProperty>

<!-- Property: is replaced by -->
<owl:ObjectProperty rdf:about="http://rdaregistry.info/Elements/u/P60104">
  <rdfs:isDefinedBy rdf:resource="http://rdaregistry.info/Elements/u/" />
  <reg:status rdf:resource="http://metadataregistry.org/uri/RegStatus/1001" />
  <reg:name xml:lang="en">replacedBy</reg:name>
  <rdfs:label xml:lang="en">is replaced by</rdfs:label>
  <skos:definition xml:lang="en">Relates a resource to a later resource used in place of an earlier resource, usually because the later resource contains updated or new information that makes the earlier resource obsolete.</skos:definition>
  <rdf:type rdf:resource="http://www.w3.org/1999/02/22-rdf-syntax-ns#Property" />
  <rdfs:subPropertyOf rdf:resource="http://rdaregistry.info/Elements/u/P60278" />
  <owl:inverseOf rdf:resource="http://rdaregistry.info/Elements/u/P60480" />
  <reg:hasSubproperty rdf:resource="http://rdaregistry.info/Elements/e/P20076" />
  <reg:lexicalAlias rdf:resource="http://rdaregistry.info/Elements/u/replacedBy.en" />
  <skos:scopeNote xml:lang="en">This relationship applies generally to single-part units, multipart monographs, and integrating resources.</skos:scopeNote>
</owl:ObjectProperty>

<!-- Property: is replaced in part by -->
<owl:ObjectProperty rdf:about="http://rdaregistry.info/Elements/u/P60103">
  <rdfs:isDefinedBy rdf:resource="http://rdaregistry.info/Elements/u/" />
  <reg:status rdf:resource="http://metadataregistry.org/uri/RegStatus/1001" />
  <reg:name xml:lang="en">replacedInPartBy</reg:name>
  <rdfs:label xml:lang="en">is replaced in part by</rdfs:label>
  <skos:definition xml:lang="en">Relates a resource to a later resource used in part in place of an earlier resource, usually because the later resource contains updated or new information that makes part of the earlier resource obsolete.</skos:definition>
  <rdf:type rdf:resource="http://www.w3.org/1999/02/22-rdf-syntax-ns#Property" />
  <rdfs:subPropertyOf rdf:resource="http://rdaregistry.info/Elements/u/P60278" />
  <owl:inverseOf rdf:resource="http://rdaregistry.info/Elements/u/P60479" />
  <reg:hasSubproperty rdf:resource="http://rdaregistry.info/Elements/e/P20075" />
  <reg:lexicalAlias rdf:resource="http://rdaregistry.info/Elements/u/replacedInPartBy.en" />
  <skos:scopeNote xml:lang="en">This relationship applies generally to single-part units, multipart monographs, and integrating resources.</skos:scopeNote>
</owl:ObjectProperty>

<!-- Property: is replacement in part of -->
<owl:ObjectProperty rdf:about="http://rdaregistry.info/Elements/u/P60479">
  <rdfs:isDefinedBy rdf:resource="http://rdaregistry.info/Elements/u/" />
  <reg:status rdf:resource="http://metadataregistry.org/uri/RegStatus/1001" />
  <reg:name xml:lang="en">replacementInPartOf</reg:name>
  <rdfs:label xml:lang="en">is replacement in part of</rdfs:label>
  <skos:definition xml:lang="en">Relates a resource to an earlier resource whose content has been partially replaced by a later resource, usually because the later resource contains updated or new information that makes the earlier resource obsolete.</skos:definition>
  <rdf:type rdf:resource="http://www.w3.org/1999/02/22-rdf-syntax-ns#Property" />
  <rdfs:subPropertyOf rdf:resource="http://rdaregistry.info/Elements/u/P60261" />
  <owl:inverseOf rdf:resource="http://rdaregistry.info/Elements/u/P60103" />
  <reg:hasSubproperty rdf:resource="http://rdaregistry.info/Elements/e/P20198" />
  <reg:lexicalAlias rdf:resource="http://rdaregistry.info/Elements/u/replacementInPartOf.en" />
  <skos:scopeNote xml:lang="en">This relationship applies generally to single-part units, multipart monographs, and integrating resources.</skos:scopeNote>
</owl:ObjectProperty>

<!-- Property: is replacement of -->
<owl:ObjectProperty rdf:about="http://rdaregistry.info/Elements/u/P60480">
  <rdfs:isDefinedBy rdf:resource="http://rdaregistry.info/Elements/u/" />
  <reg:status rdf:resource="http://metadataregistry.org/uri/RegStatus/1001" />
  <reg:name xml:lang="en">replacementOf</reg:name>
  <rdfs:label xml:lang="en">is replacement of</rdfs:label>
  <skos:definition xml:lang="en">Relates a resource to an earlier resource whose content has been replaced by a later resource, usually because the later resource contains updated or new information that makes the earlier resource obsolete.</skos:definition>
  <rdf:type rdf:resource="http://www.w3.org/1999/02/22-rdf-syntax-ns#Property" />
  <rdfs:subPropertyOf rdf:resource="http://rdaregistry.info/Elements/u/P60261" />
  <owl:inverseOf rdf:resource="http://rdaregistry.info/Elements/u/P60104" />
  <reg:hasSubproperty rdf:resource="http://rdaregistry.info/Elements/e/P20199" />
  <reg:lexicalAlias rdf:resource="http://rdaregistry.info/Elements/u/replacementOf.en" />
  <skos:scopeNote xml:lang="en">This relationship applies generally to single-part units, multipart monographs, and integrating resources.</skos:scopeNote>
</owl:ObjectProperty>

<!-- Property: is reprinted as -->
<owl:ObjectProperty rdf:about="http://rdaregistry.info/Elements/u/P60271">
  <rdfs:isDefinedBy rdf:resource="http://rdaregistry.info/Elements/u/" />
  <reg:status rdf:resource="http://metadataregistry.org/uri/RegStatus/1001" />
  <reg:name xml:lang="en">reprintedAs</reg:name>
  <rdfs:label xml:lang="en">is reprinted as</rdfs:label>
  <skos:definition xml:lang="en">Relates a resource to a resource that reissues the same resource as a printed resource being described.</skos:definition>
  <rdf:type rdf:resource="http://www.w3.org/1999/02/22-rdf-syntax-ns#Property" />
  <rdfs:subPropertyOf rdf:resource="http://rdaregistry.info/Elements/u/P60272" />
  <owl:inverseOf rdf:resource="http://rdaregistry.info/Elements/u/P60168" />
  <reg:hasSubproperty rdf:resource="http://rdaregistry.info/Elements/i/P40060" />
  <reg:hasSubproperty rdf:resource="http://rdaregistry.info/Elements/m/P30038" />
  <reg:lexicalAlias rdf:resource="http://rdaregistry.info/Elements/u/reprintedAs.en" />
</owl:ObjectProperty>

<!-- Property: is reprint of -->
<owl:ObjectProperty rdf:about="http://rdaregistry.info/Elements/u/P60168">
  <rdfs:isDefinedBy rdf:resource="http://rdaregistry.info/Elements/u/" />
  <reg:status rdf:resource="http://metadataregistry.org/uri/RegStatus/1001" />
  <reg:name xml:lang="en">reprintOf</reg:name>
  <rdfs:label xml:lang="en">is reprint of</rdfs:label>
  <skos:definition xml:lang="en">Relates a resource to a resource that reissues the same resource as a printed resource being described.</skos:definition>
  <rdf:type rdf:resource="http://www.w3.org/1999/02/22-rdf-syntax-ns#Property" />
  <rdfs:subPropertyOf rdf:resource="http://rdaregistry.info/Elements/u/P60297" />
  <owl:inverseOf rdf:resource="http://rdaregistry.info/Elements/u/P60271" />
  <reg:hasSubproperty rdf:resource="http://rdaregistry.info/Elements/i/P40038" />
  <reg:hasSubproperty rdf:resource="http://rdaregistry.info/Elements/m/P30093" />
  <reg:lexicalAlias rdf:resource="http://rdaregistry.info/Elements/u/reprintOf.en" />
</owl:ObjectProperty>

<!-- Property: is reproduced as -->
<owl:ObjectProperty rdf:about="http://rdaregistry.info/Elements/u/P60272">
  <rdfs:isDefinedBy rdf:resource="http://rdaregistry.info/Elements/u/" />
  <reg:status rdf:resource="http://metadataregistry.org/uri/RegStatus/1001" />
  <reg:name xml:lang="en">reproducedAs</reg:name>
  <rdfs:label xml:lang="en">is reproduced as</rdfs:label>
  <skos:definition xml:lang="en">Relates a resource to a resource that reproduces another resource.</skos:definition>
  <rdf:type rdf:resource="http://www.w3.org/1999/02/22-rdf-syntax-ns#Property" />
  <rdfs:subPropertyOf rdf:resource="http://rdaregistry.info/Elements/u/P60191" />
  <owl:inverseOf rdf:resource="http://rdaregistry.info/Elements/u/P60297" />
  <reg:hasSubproperty rdf:resource="http://rdaregistry.info/Elements/u/P60083" />
  <reg:hasSubproperty rdf:resource="http://rdaregistry.info/Elements/u/P60200" />
  <reg:hasSubproperty rdf:resource="http://rdaregistry.info/Elements/u/P60217" />
  <reg:hasSubproperty rdf:resource="http://rdaregistry.info/Elements/u/P60271" />
  <reg:hasSubproperty rdf:resource="http://rdaregistry.info/Elements/i/P40055" />
  <reg:hasSubproperty rdf:resource="http://rdaregistry.info/Elements/m/P30039" />
  <reg:lexicalAlias rdf:resource="http://rdaregistry.info/Elements/u/reproducedAs.en" />
</owl:ObjectProperty>

<!-- Property: is reproduction of -->
<owl:ObjectProperty rdf:about="http://rdaregistry.info/Elements/u/P60297">
  <rdfs:isDefinedBy rdf:resource="http://rdaregistry.info/Elements/u/" />
  <reg:status rdf:resource="http://metadataregistry.org/uri/RegStatus/1001" />
  <reg:name xml:lang="en">reproductionOf</reg:name>
  <rdfs:label xml:lang="en">is reproduction of</rdfs:label>
  <skos:definition xml:lang="en">Relates a resource to a resource that is used as a basis for a reproduction.</skos:definition>
  <rdf:type rdf:resource="http://www.w3.org/1999/02/22-rdf-syntax-ns#Property" />
  <rdfs:subPropertyOf rdf:resource="http://rdaregistry.info/Elements/u/P60191" />
  <owl:inverseOf rdf:resource="http://rdaregistry.info/Elements/u/P60272" />
  <reg:hasSubproperty rdf:resource="http://rdaregistry.info/Elements/u/P60168" />
  <reg:hasSubproperty rdf:resource="http://rdaregistry.info/Elements/u/P60287" />
  <reg:hasSubproperty rdf:resource="http://rdaregistry.info/Elements/u/P60301" />
  <reg:hasSubproperty rdf:resource="http://rdaregistry.info/Elements/u/P60469" />
  <reg:hasSubproperty rdf:resource="http://rdaregistry.info/Elements/i/P40042" />
  <reg:hasSubproperty rdf:resource="http://rdaregistry.info/Elements/m/P30043" />
  <reg:lexicalAlias rdf:resource="http://rdaregistry.info/Elements/u/reproductionOf.en" />
</owl:ObjectProperty>

<!-- Property: has researcher -->
<owl:ObjectProperty rdf:about="http://rdaregistry.info/Elements/u/P60836">
  <rdfs:isDefinedBy rdf:resource="http://rdaregistry.info/Elements/u/" />
  <reg:status rdf:resource="http://metadataregistry.org/uri/RegStatus/1001" />
  <rdf:type rdf:resource="http://www.w3.org/1999/02/22-rdf-syntax-ns#Property" />
  <reg:name xml:lang="en">researcher</reg:name>
  <rdfs:label xml:lang="en">has researcher</rdfs:label>
  <reg:lexicalAlias rdf:resource="http://rdaregistry.info/Elements/u/researcher.en" />
  <skos:definition xml:lang="en">Relates a resource to an agent who does research in support of the creation of a resource.</skos:definition>
  <owl:inverseOf rdf:resource="http://rdaregistry.info/Elements/u/P60837" />
  <rdfs:subPropertyOf rdf:resource="http://rdaregistry.info/Elements/u/P60374" />
</owl:ObjectProperty>

<!-- Property: is researcher of -->
<owl:ObjectProperty rdf:about="http://rdaregistry.info/Elements/u/P60837">
  <rdfs:isDefinedBy rdf:resource="http://rdaregistry.info/Elements/u/" />
  <reg:status rdf:resource="http://metadataregistry.org/uri/RegStatus/1001" />
  <rdf:type rdf:resource="http://www.w3.org/1999/02/22-rdf-syntax-ns#Property" />
  <reg:name xml:lang="en">researcherOf</reg:name>
  <rdfs:label xml:lang="en">is researcher of</rdfs:label>
  <reg:lexicalAlias rdf:resource="http://rdaregistry.info/Elements/u/researchOf.en" />
  <skos:definition xml:lang="en">Relates an agent who does research in support of the creation of a resource to a resource.</skos:definition>
  <owl:inverseOf rdf:resource="http://rdaregistry.info/Elements/u/P60836" />
  <reg:hasSubproperty rdf:resource="http://rdaregistry.info/Elements/a/P50265" />
  <rdfs:subPropertyOf rdf:resource="http://rdaregistry.info/Elements/u/P60602" />
</owl:ObjectProperty>

<!-- Property: has resolution -->
<owl:ObjectProperty rdf:about="http://rdaregistry.info/Elements/u/P60519">
  <rdfs:isDefinedBy rdf:resource="http://rdaregistry.info/Elements/u/" />
  <reg:status rdf:resource="http://metadataregistry.org/uri/RegStatus/1001" />
  <reg:name xml:lang="en">resolution</reg:name>
  <rdfs:label xml:lang="en">has resolution</rdfs:label>
  <skos:definition xml:lang="en">Relates a resource to a clarity or fineness of detail in a digital image, expressed by a measurement of the image in pixels, etc.</skos:definition>
  <rdf:type rdf:resource="http://www.w3.org/1999/02/22-rdf-syntax-ns#Property" />
  <rdfs:subPropertyOf rdf:resource="http://rdaregistry.info/Elements/u/P60350" />
  <reg:hasSubproperty rdf:resource="http://rdaregistry.info/Elements/m/P30159" />
  <reg:lexicalAlias rdf:resource="http://rdaregistry.info/Elements/u/resolution.en" />
</owl:ObjectProperty>

<!-- Property: has respondent -->
<owl:ObjectProperty rdf:about="http://rdaregistry.info/Elements/u/P60045">
  <rdfs:isDefinedBy rdf:resource="http://rdaregistry.info/Elements/u/" />
  <reg:status rdf:resource="http://metadataregistry.org/uri/RegStatus/1001" />
  <reg:name xml:lang="en">respondent</reg:name>
  <rdfs:label xml:lang="en">has respondent</rdfs:label>
  <skos:definition xml:lang="en">Relates a resource to a candidate for a degree who defends or opposes a thesis provided by a praeses in an academic disputation.</skos:definition>
  <rdf:type rdf:resource="http://www.w3.org/1999/02/22-rdf-syntax-ns#Property" />
  <rdfs:subPropertyOf rdf:resource="http://rdaregistry.info/Elements/u/P60447" />
  <owl:inverseOf rdf:resource="http://rdaregistry.info/Elements/u/P60001" />
  <reg:lexicalAlias rdf:resource="http://rdaregistry.info/Elements/u/respondent.en" />
</owl:ObjectProperty>

<!-- Property: is respondent of -->
<owl:ObjectProperty rdf:about="http://rdaregistry.info/Elements/u/P60001">
  <rdfs:isDefinedBy rdf:resource="http://rdaregistry.info/Elements/u/" />
  <reg:status rdf:resource="http://metadataregistry.org/uri/RegStatus/1001" />
  <reg:name xml:lang="en">respondentOf</reg:name>
  <rdfs:label xml:lang="en">is respondent of</rdfs:label>
  <skos:definition xml:lang="en">Relates a candidate for a degree who defends or opposes a thesis provided by a praeses in an academic disputation to a resource.</skos:definition>
  <rdf:type rdf:resource="http://www.w3.org/1999/02/22-rdf-syntax-ns#Property" />
  <rdfs:subPropertyOf rdf:resource="http://rdaregistry.info/Elements/u/P60672" />
  <owl:inverseOf rdf:resource="http://rdaregistry.info/Elements/u/P60045" />
  <reg:hasSubproperty rdf:resource="http://rdaregistry.info/Elements/a/P50001" />
  <reg:lexicalAlias rdf:resource="http://rdaregistry.info/Elements/u/respondentOf.en" />
</owl:ObjectProperty>

<!-- Property: has restorationist -->
<owl:ObjectProperty rdf:about="http://rdaregistry.info/Elements/u/P60450">
  <rdfs:isDefinedBy rdf:resource="http://rdaregistry.info/Elements/u/" />
  <reg:status rdf:resource="http://metadataregistry.org/uri/RegStatus/1001" />
  <reg:name xml:lang="en">restorationist</reg:name>
  <rdfs:label xml:lang="en">has restorationist</rdfs:label>
  <skos:definition xml:lang="en">Relates a resource to an agent responsible for the set of technical, editorial, and intellectual procedures aimed at compensating for the degradation of a resource by bringing it back to a state as close as possible to its original condition.</skos:definition>
  <rdf:type rdf:resource="http://www.w3.org/1999/02/22-rdf-syntax-ns#Property" />
  <rdfs:subPropertyOf rdf:resource="http://rdaregistry.info/Elements/u/P60374" />
  <owl:inverseOf rdf:resource="http://rdaregistry.info/Elements/u/P60674" />
  <reg:hasSubproperty rdf:resource="http://rdaregistry.info/Elements/i/P40024" />
  <reg:lexicalAlias rdf:resource="http://rdaregistry.info/Elements/u/restorationist.en" />
  <reg:hasSubproperty rdf:resource="http://rdaregistry.info/Elements/e/P20289" />
</owl:ObjectProperty>

<!-- Property: is restorationist of -->
<owl:ObjectProperty rdf:about="http://rdaregistry.info/Elements/u/P60674">
  <rdfs:isDefinedBy rdf:resource="http://rdaregistry.info/Elements/u/" />
  <reg:status rdf:resource="http://metadataregistry.org/uri/RegStatus/1001" />
  <reg:name xml:lang="en">restorationistOf</reg:name>
  <rdfs:label xml:lang="en">is restorationist of</rdfs:label>
  <skos:definition xml:lang="en">Relates an agent responsible for the set of technical, editorial, and intellectual procedures aimed at compensating for the degradation of a resource by bringing it back to a state as close as possible to its original condition to a resource.</skos:definition>
  <rdf:type rdf:resource="http://www.w3.org/1999/02/22-rdf-syntax-ns#Property" />
  <rdfs:subPropertyOf rdf:resource="http://rdaregistry.info/Elements/u/P60602" />
  <owl:inverseOf rdf:resource="http://rdaregistry.info/Elements/u/P60450" />
  <reg:hasSubproperty rdf:resource="http://rdaregistry.info/Elements/a/P50206" />
  <reg:lexicalAlias rdf:resource="http://rdaregistry.info/Elements/u/restorationistOf.en" />
  <reg:hasSubproperty rdf:resource="http://rdaregistry.info/Elements/a/P50273" />
</owl:ObjectProperty>

<!-- Property: has restrictions on access -->
<owl:ObjectProperty rdf:about="http://rdaregistry.info/Elements/u/P60496">
  <rdfs:isDefinedBy rdf:resource="http://rdaregistry.info/Elements/u/" />
  <reg:status rdf:resource="http://metadataregistry.org/uri/RegStatus/1001" />
  <reg:name xml:lang="en">restrictionsOnAccess</reg:name>
  <rdfs:label xml:lang="en">has restrictions on access</rdfs:label>
  <skos:definition xml:lang="en">Relates a resource to limitations placed on access to a resource.</skos:definition>
  <rdf:type rdf:resource="http://www.w3.org/1999/02/22-rdf-syntax-ns#Property" />
  <reg:hasSubproperty rdf:resource="http://rdaregistry.info/Elements/i/P40047" />
  <reg:hasSubproperty rdf:resource="http://rdaregistry.info/Elements/m/P30145" />
  <reg:lexicalAlias rdf:resource="http://rdaregistry.info/Elements/u/restrictionsOnAccess.en" />
</owl:ObjectProperty>

<!-- Property: has restrictions on use -->
<owl:ObjectProperty rdf:about="http://rdaregistry.info/Elements/u/P60497">
  <rdfs:isDefinedBy rdf:resource="http://rdaregistry.info/Elements/u/" />
  <reg:status rdf:resource="http://metadataregistry.org/uri/RegStatus/1001" />
  <reg:name xml:lang="en">restrictionsOnUse</reg:name>
  <rdfs:label xml:lang="en">has restrictions on use</rdfs:label>
  <skos:definition xml:lang="en">Relates a resource to a limitation placed on reproduction, publication, exhibition, etc., of a resource.</skos:definition>
  <rdf:type rdf:resource="http://www.w3.org/1999/02/22-rdf-syntax-ns#Property" />
  <reg:hasSubproperty rdf:resource="http://rdaregistry.info/Elements/i/P40048" />
  <reg:hasSubproperty rdf:resource="http://rdaregistry.info/Elements/m/P30146" />
  <reg:lexicalAlias rdf:resource="http://rdaregistry.info/Elements/u/restrictionsOnUse.en" />
</owl:ObjectProperty>

<!-- Property: is reviewed in -->
<owl:ObjectProperty rdf:about="http://rdaregistry.info/Elements/u/P60211">
  <rdfs:isDefinedBy rdf:resource="http://rdaregistry.info/Elements/u/" />
  <reg:status rdf:resource="http://metadataregistry.org/uri/RegStatus/1001" />
  <reg:name xml:lang="en">reviewedIn</reg:name>
  <rdfs:label xml:lang="en">is reviewed in</rdfs:label>
  <skos:definition xml:lang="en">Relates a resource to a resource that contains a brief evaluation of a described resource.</skos:definition>
  <rdf:type rdf:resource="http://www.w3.org/1999/02/22-rdf-syntax-ns#Property" />
  <rdfs:subPropertyOf rdf:resource="http://rdaregistry.info/Elements/u/P60215" />
  <owl:inverseOf rdf:resource="http://rdaregistry.info/Elements/u/P60288" />
  <reg:hasSubproperty rdf:resource="http://rdaregistry.info/Elements/e/P20274" />
  <reg:hasSubproperty rdf:resource="http://rdaregistry.info/Elements/i/P40067" />
  <reg:hasSubproperty rdf:resource="http://rdaregistry.info/Elements/m/P30259" />
  <reg:lexicalAlias rdf:resource="http://rdaregistry.info/Elements/u/reviewedIn.en" />
</owl:ObjectProperty>

<!-- Property: is review of -->
<owl:ObjectProperty rdf:about="http://rdaregistry.info/Elements/u/P60288">
  <rdfs:isDefinedBy rdf:resource="http://rdaregistry.info/Elements/u/" />
  <reg:status rdf:resource="http://metadataregistry.org/uri/RegStatus/1001" />
  <reg:name xml:lang="en">reviewOf</reg:name>
  <rdfs:label xml:lang="en">is review of</rdfs:label>
  <skos:definition xml:lang="en">Relates a resource to a resource used as a basis for a brief evaluation.</skos:definition>
  <rdf:type rdf:resource="http://www.w3.org/1999/02/22-rdf-syntax-ns#Property" />
  <rdfs:subPropertyOf rdf:resource="http://rdaregistry.info/Elements/u/P60190" />
  <owl:inverseOf rdf:resource="http://rdaregistry.info/Elements/u/P60211" />
  <reg:hasSubproperty rdf:resource="http://rdaregistry.info/Elements/w/P10268" />
  <reg:hasSubproperty rdf:resource="http://rdaregistry.info/Elements/w/P10274" />
  <reg:hasSubproperty rdf:resource="http://rdaregistry.info/Elements/w/P10280" />
  <reg:lexicalAlias rdf:resource="http://rdaregistry.info/Elements/u/reviewOf.en" />
</owl:ObjectProperty>

<!-- Property: is revised as -->
<owl:ObjectProperty rdf:about="http://rdaregistry.info/Elements/u/P60245">
  <rdfs:isDefinedBy rdf:resource="http://rdaregistry.info/Elements/u/" />
  <reg:status rdf:resource="http://metadataregistry.org/uri/RegStatus/1001" />
  <reg:name xml:lang="en">revisedAs</reg:name>
  <rdfs:label xml:lang="en">is revised as</rdfs:label>
  <skos:definition xml:lang="en">Relates a resource to a resource that has been updated, corrected, or expanded.</skos:definition>
  <rdf:type rdf:resource="http://www.w3.org/1999/02/22-rdf-syntax-ns#Property" />
  <rdfs:subPropertyOf rdf:resource="http://rdaregistry.info/Elements/u/P60250" />
  <owl:inverseOf rdf:resource="http://rdaregistry.info/Elements/u/P60303" />
  <reg:hasSubproperty rdf:resource="http://rdaregistry.info/Elements/e/P20211" />
  <reg:lexicalAlias rdf:resource="http://rdaregistry.info/Elements/u/revisedAs.en" />
</owl:ObjectProperty>

<!-- Property: is revision of -->
<owl:ObjectProperty rdf:about="http://rdaregistry.info/Elements/u/P60303">
  <rdfs:isDefinedBy rdf:resource="http://rdaregistry.info/Elements/u/" />
  <reg:status rdf:resource="http://metadataregistry.org/uri/RegStatus/1001" />
  <reg:name xml:lang="en">revisionOf</reg:name>
  <rdfs:label xml:lang="en">is revision of</rdfs:label>
  <skos:definition xml:lang="en">Relates a resource to a resource used as a basis for an updated, corrected, or expanded version.</skos:definition>
  <rdf:type rdf:resource="http://www.w3.org/1999/02/22-rdf-syntax-ns#Property" />
  <rdfs:subPropertyOf rdf:resource="http://rdaregistry.info/Elements/u/P60305" />
  <owl:inverseOf rdf:resource="http://rdaregistry.info/Elements/u/P60245" />
  <reg:hasSubproperty rdf:resource="http://rdaregistry.info/Elements/e/P20189" />
  <reg:lexicalAlias rdf:resource="http://rdaregistry.info/Elements/u/revisionOf.en" />
</owl:ObjectProperty>

<!-- Property: has right ascension -->
<owl:ObjectProperty rdf:about="http://rdaregistry.info/Elements/u/P60899">
  <rdfs:isDefinedBy rdf:resource="http://rdaregistry.info/Elements/u/" />
  <reg:status rdf:resource="http://metadataregistry.org/uri/RegStatus/1001" />
  <rdf:type rdf:resource="http://www.w3.org/1999/02/22-rdf-syntax-ns#Property" />
  <reg:name xml:lang="en">rightAscension</reg:name>
  <rdfs:label xml:lang="en">has right ascension</rdfs:label>
  <reg:lexicalAlias rdf:resource="http://rdaregistry.info/Elements/u/rightAscension.en" />
  <skos:definition xml:lang="en">Relates a resource to an angular distance measured eastward on the equator from the vernal equinox to the hour circle through a celestial body, from 0 to 24 hours..</skos:definition>
</owl:ObjectProperty>

<!-- Property: has right ascension and declination -->
<owl:ObjectProperty rdf:about="http://rdaregistry.info/Elements/u/P60346">
  <rdfs:isDefinedBy rdf:resource="http://rdaregistry.info/Elements/u/" />
  <reg:status rdf:resource="http://metadataregistry.org/uri/RegStatus/1001" />
  <reg:name xml:lang="en">rightAscensionAndDeclination</reg:name>
  <rdfs:label xml:lang="en">has right ascension and declination</rdfs:label>
  <skos:definition xml:lang="en">Relates a resource to a system for identifying the location of a celestial object in the sky covered by the cartographic content of a resource using angles of right ascension and declination.</skos:definition>
  <rdf:type rdf:resource="http://www.w3.org/1999/02/22-rdf-syntax-ns#Property" />
  <rdfs:subPropertyOf rdf:resource="http://rdaregistry.info/Elements/u/P60109" />
  <reg:lexicalAlias rdf:resource="http://rdaregistry.info/Elements/u/rightAscensionAndDeclination.en" />
</owl:ObjectProperty>

<!-- Property: has scale -->
<owl:ObjectProperty rdf:about="http://rdaregistry.info/Elements/u/P60565">
  <rdfs:isDefinedBy rdf:resource="http://rdaregistry.info/Elements/u/" />
  <reg:status rdf:resource="http://metadataregistry.org/uri/RegStatus/1001" />
  <reg:name xml:lang="en">scale</reg:name>
  <rdfs:label xml:lang="en">has scale</rdfs:label>
  <skos:definition xml:lang="en">Relates a resource to a ratio of the dimensions of the content of an image or three-dimensional form to the dimensions of the thing it represents</skos:definition>
  <rdf:type rdf:resource="http://www.w3.org/1999/02/22-rdf-syntax-ns#Property" />
  <reg:hasSubproperty rdf:resource="http://rdaregistry.info/Elements/u/P60510" />
  <reg:hasSubproperty rdf:resource="http://rdaregistry.info/Elements/u/P60563" />
  <reg:hasSubproperty rdf:resource="http://rdaregistry.info/Elements/u/P60564" />
  <reg:hasSubproperty rdf:resource="http://rdaregistry.info/Elements/u/P60579" />
  <reg:hasSubproperty rdf:resource="http://rdaregistry.info/Elements/e/P20228" />
  <reg:lexicalAlias rdf:resource="http://rdaregistry.info/Elements/u/scale.en" />
  <skos:scopeNote xml:lang="en">Scale can apply to horizontal, vertical, angular, and/or other measurements represented in the resource.</skos:scopeNote>
</owl:ObjectProperty>

<!-- Property: has scale designation -->
<owl:ObjectProperty rdf:about="http://rdaregistry.info/Elements/u/P60874">
  <rdfs:isDefinedBy rdf:resource="http://rdaregistry.info/Elements/u/" />
  <reg:status rdf:resource="http://metadataregistry.org/uri/RegStatus/1001" />
  <rdf:type rdf:resource="http://www.w3.org/1999/02/22-rdf-syntax-ns#Property" />
  <reg:name xml:lang="en">scaleDesignation</reg:name>
  <rdfs:label xml:lang="en">has scale designation</rdfs:label>
  <reg:lexicalAlias rdf:resource="http://rdaregistry.info/Elements/u/scaleDesignation.en" />
  <skos:definition xml:lang="en">Relates a resource to a general designation of a lack of a ratio of the dimensions of the content of an image or three-dimensional form to the dimensions of the thing it represents.</skos:definition>
  <reg:hasSubproperty rdf:resource="http://rdaregistry.info/Elements/e/P20291" />
</owl:ObjectProperty>

<!-- Property: has scale of still image or three-dimensional form -->
<owl:ObjectProperty rdf:about="http://rdaregistry.info/Elements/u/P60564">
  <rdfs:isDefinedBy rdf:resource="http://rdaregistry.info/Elements/u/" />
  <reg:status rdf:resource="http://metadataregistry.org/uri/RegStatus/1001" />
  <reg:name xml:lang="en">scaleOfStillImageOrThreeDimensionalForm</reg:name>
  <rdfs:label xml:lang="en">has scale of still image or three-dimensional form</rdfs:label>
  <skos:definition xml:lang="en">Relates a resource to a ratio of the dimensions of a still image or three-dimensional form contained or embodied in a resource to the dimensions of the thing it represents.</skos:definition>
  <rdf:type rdf:resource="http://www.w3.org/1999/02/22-rdf-syntax-ns#Property" />
  <rdfs:subPropertyOf rdf:resource="http://rdaregistry.info/Elements/u/P60565" />
  <reg:hasSubproperty rdf:resource="http://rdaregistry.info/Elements/e/P20227" />
  <reg:lexicalAlias rdf:resource="http://rdaregistry.info/Elements/u/scaleOfStillImageOrThreeDimensionalForm.en" />
</owl:ObjectProperty>

<!-- Property: has scope of usage -->
<owl:ObjectProperty rdf:about="http://rdaregistry.info/Elements/u/P60822">
  <rdfs:isDefinedBy rdf:resource="http://rdaregistry.info/Elements/u/" />
  <reg:status rdf:resource="http://metadataregistry.org/uri/RegStatus/1001" />
  <rdf:type rdf:resource="http://www.w3.org/1999/02/22-rdf-syntax-ns#Property" />
  <reg:name xml:lang="en">scopeOfUsage</reg:name>
  <rdfs:label xml:lang="en">has scope of usage</rdfs:label>
  <reg:lexicalAlias rdf:resource="http://rdaregistry.info/Elements/u/scopeOfUsage.en" />
  <skos:definition xml:lang="en">Relates a name to a type or form of resource associated with a name chosen as a preferred name for an agent.</skos:definition>
</owl:ObjectProperty>

<!-- Property: is screenplay -->
<owl:ObjectProperty rdf:about="http://rdaregistry.info/Elements/u/P60264">
  <rdfs:isDefinedBy rdf:resource="http://rdaregistry.info/Elements/u/" />
  <reg:status rdf:resource="http://metadataregistry.org/uri/RegStatus/1001" />
  <reg:name xml:lang="en">screenplay</reg:name>
  <rdfs:label xml:lang="en">is screenplay</rdfs:label>
  <skos:definition xml:lang="en">Relates a resource to a resource that provides text for a motion picture, television program or video.</skos:definition>
  <rdf:type rdf:resource="http://www.w3.org/1999/02/22-rdf-syntax-ns#Property" />
  <rdfs:subPropertyOf rdf:resource="http://rdaregistry.info/Elements/u/P60198" />
  <owl:inverseOf rdf:resource="http://rdaregistry.info/Elements/u/P60201" />
  <reg:hasSubproperty rdf:resource="http://rdaregistry.info/Elements/u/P60265" />
  <reg:hasSubproperty rdf:resource="http://rdaregistry.info/Elements/u/P60268" />
  <reg:hasSubproperty rdf:resource="http://rdaregistry.info/Elements/u/P60269" />
  <reg:hasSubproperty rdf:resource="http://rdaregistry.info/Elements/e/P20157" />
  <reg:lexicalAlias rdf:resource="http://rdaregistry.info/Elements/u/screenplay.en" />
</owl:ObjectProperty>

<!-- Property: is screenplay based on -->
<owl:ObjectProperty rdf:about="http://rdaregistry.info/Elements/u/P60231">
  <rdfs:isDefinedBy rdf:resource="http://rdaregistry.info/Elements/u/" />
  <reg:status rdf:resource="http://metadataregistry.org/uri/RegStatus/1001" />
  <reg:name xml:lang="en">screenplayBasedOn</reg:name>
  <rdfs:label xml:lang="en">is screenplay based on</rdfs:label>
  <skos:definition xml:lang="en">Relates a resource to a resource that has been adapted as a screenplay for a motion picture, television program, or video.</skos:definition>
  <rdf:type rdf:resource="http://www.w3.org/1999/02/22-rdf-syntax-ns#Property" />
  <rdfs:subPropertyOf rdf:resource="http://rdaregistry.info/Elements/u/P60241" />
  <owl:inverseOf rdf:resource="http://rdaregistry.info/Elements/u/P60185" />
  <reg:hasSubproperty rdf:resource="http://rdaregistry.info/Elements/u/P60232" />
  <reg:hasSubproperty rdf:resource="http://rdaregistry.info/Elements/u/P60233" />
  <reg:hasSubproperty rdf:resource="http://rdaregistry.info/Elements/u/P60234" />
  <reg:hasSubproperty rdf:resource="http://rdaregistry.info/Elements/e/P20129" />
  <reg:lexicalAlias rdf:resource="http://rdaregistry.info/Elements/u/screenplayBasedOn.en" />
</owl:ObjectProperty>

<!-- Property: is screenplay for -->
<owl:ObjectProperty rdf:about="http://rdaregistry.info/Elements/u/P60201">
  <rdfs:isDefinedBy rdf:resource="http://rdaregistry.info/Elements/u/" />
  <reg:status rdf:resource="http://metadataregistry.org/uri/RegStatus/1001" />
  <reg:name xml:lang="en">screenplayFor</reg:name>
  <rdfs:label xml:lang="en">is screenplay for</rdfs:label>
  <skos:definition xml:lang="en">Relates a resource to a resource such as a motion picture, television program, or video, that uses a text of a resource as a screenplay.</skos:definition>
  <rdf:type rdf:resource="http://www.w3.org/1999/02/22-rdf-syntax-ns#Property" />
  <rdfs:subPropertyOf rdf:resource="http://rdaregistry.info/Elements/u/P60198" />
  <owl:inverseOf rdf:resource="http://rdaregistry.info/Elements/u/P60264" />
  <reg:hasSubproperty rdf:resource="http://rdaregistry.info/Elements/u/P60282" />
  <reg:hasSubproperty rdf:resource="http://rdaregistry.info/Elements/u/P60283" />
  <reg:hasSubproperty rdf:resource="http://rdaregistry.info/Elements/u/P60284" />
  <reg:hasSubproperty rdf:resource="http://rdaregistry.info/Elements/e/P20102" />
  <reg:lexicalAlias rdf:resource="http://rdaregistry.info/Elements/u/screenplayFor.en" />
</owl:ObjectProperty>

<!-- Property: is screenplay for motion picture -->
<owl:ObjectProperty rdf:about="http://rdaregistry.info/Elements/u/P60282">
  <rdfs:isDefinedBy rdf:resource="http://rdaregistry.info/Elements/u/" />
  <reg:status rdf:resource="http://metadataregistry.org/uri/RegStatus/1001" />
  <reg:name xml:lang="en">screenplayForMotionPicture</reg:name>
  <rdfs:label xml:lang="en">is screenplay for motion picture</rdfs:label>
  <skos:definition xml:lang="en">Relates a resource to a resource that uses a text as a screenplay for a motion picture.</skos:definition>
  <rdf:type rdf:resource="http://www.w3.org/1999/02/22-rdf-syntax-ns#Property" />
  <rdfs:subPropertyOf rdf:resource="http://rdaregistry.info/Elements/u/P60201" />
  <owl:inverseOf rdf:resource="http://rdaregistry.info/Elements/u/P60265" />
  <reg:hasSubproperty rdf:resource="http://rdaregistry.info/Elements/e/P20173" />
  <reg:lexicalAlias rdf:resource="http://rdaregistry.info/Elements/u/screenplayForMotionPicture.en" />
</owl:ObjectProperty>

<!-- Property: is screenplay for television program -->
<owl:ObjectProperty rdf:about="http://rdaregistry.info/Elements/u/P60283">
  <rdfs:isDefinedBy rdf:resource="http://rdaregistry.info/Elements/u/" />
  <reg:status rdf:resource="http://metadataregistry.org/uri/RegStatus/1001" />
  <reg:name xml:lang="en">screenplayForTelevisionProgram</reg:name>
  <rdfs:label xml:lang="en">is screenplay for television program</rdfs:label>
  <skos:definition xml:lang="en">Relates a resource to a resource that uses a text as a screenplay for a television program.</skos:definition>
  <rdf:type rdf:resource="http://www.w3.org/1999/02/22-rdf-syntax-ns#Property" />
  <rdfs:subPropertyOf rdf:resource="http://rdaregistry.info/Elements/u/P60201" />
  <owl:inverseOf rdf:resource="http://rdaregistry.info/Elements/u/P60268" />
  <reg:hasSubproperty rdf:resource="http://rdaregistry.info/Elements/e/P20174" />
  <reg:lexicalAlias rdf:resource="http://rdaregistry.info/Elements/u/screenplayForTelevisionProgram.en" />
</owl:ObjectProperty>

<!-- Property: is screenplay for video -->
<owl:ObjectProperty rdf:about="http://rdaregistry.info/Elements/u/P60284">
  <rdfs:isDefinedBy rdf:resource="http://rdaregistry.info/Elements/u/" />
  <reg:status rdf:resource="http://metadataregistry.org/uri/RegStatus/1001" />
  <reg:name xml:lang="en">screenplayForVideo</reg:name>
  <rdfs:label xml:lang="en">is screenplay for video</rdfs:label>
  <skos:definition xml:lang="en">Relates a resource to a resource that uses a text as a screenplay for a video.</skos:definition>
  <rdf:type rdf:resource="http://www.w3.org/1999/02/22-rdf-syntax-ns#Property" />
  <rdfs:subPropertyOf rdf:resource="http://rdaregistry.info/Elements/u/P60201" />
  <owl:inverseOf rdf:resource="http://rdaregistry.info/Elements/u/P60269" />
  <reg:hasSubproperty rdf:resource="http://rdaregistry.info/Elements/e/P20175" />
  <reg:lexicalAlias rdf:resource="http://rdaregistry.info/Elements/u/screenplayForVideo.en" />
</owl:ObjectProperty>

<!-- Property: has screenwriter -->
<owl:ObjectProperty rdf:about="http://rdaregistry.info/Elements/u/P60476">
  <rdfs:isDefinedBy rdf:resource="http://rdaregistry.info/Elements/u/" />
  <reg:status rdf:resource="http://metadataregistry.org/uri/RegStatus/1001" />
  <reg:name xml:lang="en">screenwriter</reg:name>
  <rdfs:label xml:lang="en">has screenwriter</rdfs:label>
  <skos:definition xml:lang="en">Relates a resource to an author of a screenplay, script, or scene.</skos:definition>
  <rdf:type rdf:resource="http://www.w3.org/1999/02/22-rdf-syntax-ns#Property" />
  <rdfs:subPropertyOf rdf:resource="http://rdaregistry.info/Elements/u/P60434" />
  <owl:inverseOf rdf:resource="http://rdaregistry.info/Elements/u/P60706" />
  <reg:lexicalAlias rdf:resource="http://rdaregistry.info/Elements/u/screenwriter.en" />
</owl:ObjectProperty>

<!-- Property: is screenwriter of -->
<owl:ObjectProperty rdf:about="http://rdaregistry.info/Elements/u/P60706">
  <rdfs:isDefinedBy rdf:resource="http://rdaregistry.info/Elements/u/" />
  <reg:status rdf:resource="http://metadataregistry.org/uri/RegStatus/1001" />
  <reg:name xml:lang="en">screenwriterOf</reg:name>
  <rdfs:label xml:lang="en">is screenwriter of</rdfs:label>
  <skos:definition xml:lang="en">Relates an author of a screenplay, script, or scene to a resource.</skos:definition>
  <rdf:type rdf:resource="http://www.w3.org/1999/02/22-rdf-syntax-ns#Property" />
  <rdfs:subPropertyOf rdf:resource="http://rdaregistry.info/Elements/u/P60663" />
  <owl:inverseOf rdf:resource="http://rdaregistry.info/Elements/u/P60476" />
  <reg:hasSubproperty rdf:resource="http://rdaregistry.info/Elements/a/P50223" />
  <reg:lexicalAlias rdf:resource="http://rdaregistry.info/Elements/u/screenwriterOf.en" />
</owl:ObjectProperty>

<!-- Property: has script -->
<owl:ObjectProperty rdf:about="http://rdaregistry.info/Elements/u/P60322">
  <rdfs:isDefinedBy rdf:resource="http://rdaregistry.info/Elements/u/" />
  <reg:status rdf:resource="http://metadataregistry.org/uri/RegStatus/1001" />
  <reg:name xml:lang="en">script</reg:name>
  <rdfs:label xml:lang="en">has script</rdfs:label>
  <skos:definition xml:lang="en">Relates a resource to a set of characters or symbols used to express written language content of a resource.</skos:definition>
  <rdf:type rdf:resource="http://www.w3.org/1999/02/22-rdf-syntax-ns#Property" />
  <rdfs:subPropertyOf rdf:resource="http://rdaregistry.info/Elements/u/P60319" />
  <reg:hasSubproperty rdf:resource="http://rdaregistry.info/Elements/e/P20065" />
  <reg:lexicalAlias rdf:resource="http://rdaregistry.info/Elements/u/script.en" />
</owl:ObjectProperty>

<!-- Property: is script for radio program -->
<owl:ObjectProperty rdf:about="http://rdaregistry.info/Elements/u/P60285">
  <rdfs:isDefinedBy rdf:resource="http://rdaregistry.info/Elements/u/" />
  <reg:status rdf:resource="http://metadataregistry.org/uri/RegStatus/1001" />
  <reg:name xml:lang="en">scriptForRadioProgram</reg:name>
  <rdfs:label xml:lang="en">is script for radio program</rdfs:label>
  <skos:definition xml:lang="en">Relates a resource to a resource that uses a text of a source resource as a script for a radio program.</skos:definition>
  <rdf:type rdf:resource="http://www.w3.org/1999/02/22-rdf-syntax-ns#Property" />
  <rdfs:subPropertyOf rdf:resource="http://rdaregistry.info/Elements/u/P60198" />
  <owl:inverseOf rdf:resource="http://rdaregistry.info/Elements/u/P60267" />
  <reg:hasSubproperty rdf:resource="http://rdaregistry.info/Elements/e/P20176" />
  <reg:lexicalAlias rdf:resource="http://rdaregistry.info/Elements/u/scriptForRadioProgram.en" />
</owl:ObjectProperty>

<!-- Property: has sculptor -->
<owl:ObjectProperty rdf:about="http://rdaregistry.info/Elements/u/P60475">
  <rdfs:isDefinedBy rdf:resource="http://rdaregistry.info/Elements/u/" />
  <reg:status rdf:resource="http://metadataregistry.org/uri/RegStatus/1001" />
  <reg:name xml:lang="en">sculptor</reg:name>
  <rdfs:label xml:lang="en">has sculptor</rdfs:label>
  <skos:definition xml:lang="en">Relates a resource to an artist responsible for creating a three-dimensional resource by modeling, carving, or similar technique.</skos:definition>
  <rdf:type rdf:resource="http://www.w3.org/1999/02/22-rdf-syntax-ns#Property" />
  <rdfs:subPropertyOf rdf:resource="http://rdaregistry.info/Elements/u/P60431" />
  <owl:inverseOf rdf:resource="http://rdaregistry.info/Elements/u/P60705" />
  <reg:lexicalAlias rdf:resource="http://rdaregistry.info/Elements/u/sculptor.en" />
</owl:ObjectProperty>

<!-- Property: is sculptor of -->
<owl:ObjectProperty rdf:about="http://rdaregistry.info/Elements/u/P60705">
  <rdfs:isDefinedBy rdf:resource="http://rdaregistry.info/Elements/u/" />
  <reg:status rdf:resource="http://metadataregistry.org/uri/RegStatus/1001" />
  <reg:name xml:lang="en">sculptorOf</reg:name>
  <rdfs:label xml:lang="en">is sculptor of</rdfs:label>
  <skos:definition xml:lang="en">Relates an artist responsible for creating a three-dimensional resource by modeling, carving, or similar technique to a resource.</skos:definition>
  <rdf:type rdf:resource="http://www.w3.org/1999/02/22-rdf-syntax-ns#Property" />
  <rdfs:subPropertyOf rdf:resource="http://rdaregistry.info/Elements/u/P60660" />
  <owl:inverseOf rdf:resource="http://rdaregistry.info/Elements/u/P60475" />
  <reg:hasSubproperty rdf:resource="http://rdaregistry.info/Elements/a/P50222" />
  <reg:lexicalAlias rdf:resource="http://rdaregistry.info/Elements/u/sculptorOf.en" />
</owl:ObjectProperty>

<!-- Property: has seller -->
<owl:ObjectProperty rdf:about="http://rdaregistry.info/Elements/u/P60092">
  <rdfs:isDefinedBy rdf:resource="http://rdaregistry.info/Elements/u/" />
  <reg:status rdf:resource="http://metadataregistry.org/uri/RegStatus/1001" />
  <reg:name xml:lang="en">seller</reg:name>
  <rdfs:label xml:lang="en">has seller</rdfs:label>
  <skos:definition xml:lang="en">Relates a resource to a former owner of a resource who sold that resource to another owner.</skos:definition>
  <rdf:type rdf:resource="http://www.w3.org/1999/02/22-rdf-syntax-ns#Property" />
  <rdfs:subPropertyOf rdf:resource="http://rdaregistry.info/Elements/u/P60401" />
  <owl:inverseOf rdf:resource="http://rdaregistry.info/Elements/u/P60013" />
  <reg:hasSubproperty rdf:resource="http://rdaregistry.info/Elements/i/P40008" />
  <reg:lexicalAlias rdf:resource="http://rdaregistry.info/Elements/u/seller.en" />
</owl:ObjectProperty>

<!-- Property: is seller of -->
<owl:ObjectProperty rdf:about="http://rdaregistry.info/Elements/u/P60013">
  <rdfs:isDefinedBy rdf:resource="http://rdaregistry.info/Elements/u/" />
  <reg:status rdf:resource="http://metadataregistry.org/uri/RegStatus/1001" />
  <reg:name xml:lang="en">sellerOf</reg:name>
  <rdfs:label xml:lang="en">is seller of</rdfs:label>
  <skos:definition xml:lang="en">Relates a former owner of a resource who sold that resource to another owner to a resource.</skos:definition>
  <rdf:type rdf:resource="http://www.w3.org/1999/02/22-rdf-syntax-ns#Property" />
  <rdfs:subPropertyOf rdf:resource="http://rdaregistry.info/Elements/u/P60630" />
  <owl:inverseOf rdf:resource="http://rdaregistry.info/Elements/u/P60092" />
  <reg:hasSubproperty rdf:resource="http://rdaregistry.info/Elements/a/P50067" />
  <reg:lexicalAlias rdf:resource="http://rdaregistry.info/Elements/u/sellerOf.en" />
</owl:ObjectProperty>

<!-- Property: is separated from -->
<owl:ObjectProperty rdf:about="http://rdaregistry.info/Elements/u/P60277">
  <rdfs:isDefinedBy rdf:resource="http://rdaregistry.info/Elements/u/" />
  <reg:status rdf:resource="http://metadataregistry.org/uri/RegStatus/1001" />
  <reg:name xml:lang="en">separatedFrom</reg:name>
  <rdfs:label xml:lang="en">is separated from</rdfs:label>
  <skos:definition xml:lang="en">Relates a resource to a resource that spun off a part of its content to form a new resource.</skos:definition>
  <rdf:type rdf:resource="http://www.w3.org/1999/02/22-rdf-syntax-ns#Property" />
  <rdfs:subPropertyOf rdf:resource="http://rdaregistry.info/Elements/u/P60261" />
  <owl:inverseOf rdf:resource="http://rdaregistry.info/Elements/u/P60199" />
  <reg:hasSubproperty rdf:resource="http://rdaregistry.info/Elements/e/P20168" />
  <reg:lexicalAlias rdf:resource="http://rdaregistry.info/Elements/u/separatedFrom.en" />
</owl:ObjectProperty>

<!-- Property: is sequel -->
<owl:ObjectProperty rdf:about="http://rdaregistry.info/Elements/u/P60102">
  <rdfs:isDefinedBy rdf:resource="http://rdaregistry.info/Elements/u/" />
  <reg:status rdf:resource="http://metadataregistry.org/uri/RegStatus/1001" />
  <reg:name xml:lang="en">sequel</reg:name>
  <rdfs:label xml:lang="en">is sequel</rdfs:label>
  <skos:definition xml:lang="en">Relates a resource to a later resource that continues the narrative of an earlier resource.</skos:definition>
  <rdf:type rdf:resource="http://www.w3.org/1999/02/22-rdf-syntax-ns#Property" />
  <rdfs:subPropertyOf rdf:resource="http://rdaregistry.info/Elements/u/P60278" />
  <owl:inverseOf rdf:resource="http://rdaregistry.info/Elements/u/P60577" />
  <reg:lexicalAlias rdf:resource="http://rdaregistry.info/Elements/u/sequel.en" />
</owl:ObjectProperty>

<!-- Property: is sequel to -->
<owl:ObjectProperty rdf:about="http://rdaregistry.info/Elements/u/P60577">
  <rdfs:isDefinedBy rdf:resource="http://rdaregistry.info/Elements/u/" />
  <reg:status rdf:resource="http://metadataregistry.org/uri/RegStatus/1001" />
  <reg:name xml:lang="en">sequelTo</reg:name>
  <rdfs:label xml:lang="en">is sequel to</rdfs:label>
  <skos:definition xml:lang="en">Relates a resource to a resource whose narrative is continued by a later resource.</skos:definition>
  <rdf:type rdf:resource="http://www.w3.org/1999/02/22-rdf-syntax-ns#Property" />
  <rdfs:subPropertyOf rdf:resource="http://rdaregistry.info/Elements/u/P60261" />
  <owl:inverseOf rdf:resource="http://rdaregistry.info/Elements/u/P60102" />
  <reg:lexicalAlias rdf:resource="http://rdaregistry.info/Elements/u/sequelTo.en" />
</owl:ObjectProperty>

<!-- Property: has sequential resource relationship with -->
<owl:ObjectProperty rdf:about="http://rdaregistry.info/Elements/u/P60713">
  <rdfs:isDefinedBy rdf:resource="http://rdaregistry.info/Elements/u/" />
  <reg:status rdf:resource="http://metadataregistry.org/uri/RegStatus/1001" />
  <reg:name xml:lang="en">sequentialResourceRelationshipWith</reg:name>
  <rdfs:label xml:lang="en">has sequential resource relationship with</rdfs:label>
  <rdf:type rdf:resource="http://www.w3.org/1999/02/22-rdf-syntax-ns#Property" />
  <reg:hasSubproperty rdf:resource="http://rdaregistry.info/Elements/u/P60261" />
  <reg:hasSubproperty rdf:resource="http://rdaregistry.info/Elements/u/P60278" />
  <owl:inverseOf rdf:resource="http://rdaregistry.info/Elements/u/P60713" />
  <skos:definition xml:lang="en">Relates a resource to a resource that is preceded by or succeeded by a resource.</skos:definition>
  <reg:hasSubproperty rdf:resource="http://rdaregistry.info/Elements/e/P20235" />
  <reg:lexicalAlias rdf:resource="http://rdaregistry.info/Elements/u/sequentialResourceRelationshipWith.en" />
</owl:ObjectProperty>

<!-- Property: is series container of -->
<owl:ObjectProperty rdf:about="http://rdaregistry.info/Elements/u/P60240">
  <rdfs:isDefinedBy rdf:resource="http://rdaregistry.info/Elements/u/" />
  <reg:status rdf:resource="http://metadataregistry.org/uri/RegStatus/1001" />
  <reg:name xml:lang="en">seriesContainerOf</reg:name>
  <rdfs:label xml:lang="en">is series container of</rdfs:label>
  <skos:definition xml:lang="en">Relates a resource to a resource that has been issued as part of a series.</skos:definition>
  <rdf:type rdf:resource="http://www.w3.org/1999/02/22-rdf-syntax-ns#Property" />
  <rdfs:subPropertyOf rdf:resource="http://rdaregistry.info/Elements/u/P60249" />
  <owl:inverseOf rdf:resource="http://rdaregistry.info/Elements/u/P60193" />
  <reg:lexicalAlias rdf:resource="http://rdaregistry.info/Elements/u/seriesContainerOf.en" />
</owl:ObjectProperty>

<!-- Property: has series statement -->
<owl:ObjectProperty rdf:about="http://rdaregistry.info/Elements/u/P60328">
  <rdfs:isDefinedBy rdf:resource="http://rdaregistry.info/Elements/u/" />
  <reg:status rdf:resource="http://metadataregistry.org/uri/RegStatus/1001" />
  <reg:name xml:lang="en">seriesStatement</reg:name>
  <rdfs:label xml:lang="en">has series statement</rdfs:label>
  <skos:definition xml:lang="en">Relates a resource to a statement identifying a series to which a resource belongs and a numbering of a resource within the series.</skos:definition>
  <rdf:type rdf:resource="http://www.w3.org/1999/02/22-rdf-syntax-ns#Property" />
  <reg:hasSubproperty rdf:resource="http://rdaregistry.info/Elements/m/P30106" />
  <reg:lexicalAlias rdf:resource="http://rdaregistry.info/Elements/u/seriesStatement.en" />
  <skos:scopeNote xml:lang="en">A series statement may also include information identifying one or more subseries to which the resource being described belongs. A series statement sometimes includes statements of responsibility relating to a series or subseries.</skos:scopeNote>
</owl:ObjectProperty>

<!-- Property: is set to music as -->
<owl:ObjectProperty rdf:about="http://rdaregistry.info/Elements/u/P60121">
  <rdfs:isDefinedBy rdf:resource="http://rdaregistry.info/Elements/u/" />
  <reg:status rdf:resource="http://metadataregistry.org/uri/RegStatus/1001" />
  <reg:name xml:lang="en">setToMusicAs</reg:name>
  <rdfs:label xml:lang="en">is set to music as</rdfs:label>
  <skos:definition xml:lang="en">Relates a resource to a non-dramatic musical resource, other than an oratorio, that uses a text of a source resource.</skos:definition>
  <rdf:type rdf:resource="http://www.w3.org/1999/02/22-rdf-syntax-ns#Property" />
  <rdfs:subPropertyOf rdf:resource="http://rdaregistry.info/Elements/u/P60250" />
  <owl:inverseOf rdf:resource="http://rdaregistry.info/Elements/u/P60266" />
  <reg:hasSubproperty rdf:resource="http://rdaregistry.info/Elements/e/P20087" />
  <reg:lexicalAlias rdf:resource="http://rdaregistry.info/Elements/u/setToMusicAs.en" />
</owl:ObjectProperty>

<!-- Property: has singer -->
<owl:ObjectProperty rdf:about="http://rdaregistry.info/Elements/u/P60156">
  <rdfs:isDefinedBy rdf:resource="http://rdaregistry.info/Elements/u/" />
  <reg:status rdf:resource="http://metadataregistry.org/uri/RegStatus/1001" />
  <reg:name xml:lang="en">singer</reg:name>
  <rdfs:label xml:lang="en">has singer</rdfs:label>
  <skos:definition xml:lang="en">Relates a resource to a performer contributing to a resource by using his/her/their voice, with or without instrumental accompaniment, to produce music. a singers performance may or may not include actual words.</skos:definition>
  <rdf:type rdf:resource="http://www.w3.org/1999/02/22-rdf-syntax-ns#Property" />
  <rdfs:subPropertyOf rdf:resource="http://rdaregistry.info/Elements/u/P60387" />
  <owl:inverseOf rdf:resource="http://rdaregistry.info/Elements/u/P60031" />
  <reg:hasSubproperty rdf:resource="http://rdaregistry.info/Elements/e/P20025" />
  <reg:lexicalAlias rdf:resource="http://rdaregistry.info/Elements/u/singer.en" />
</owl:ObjectProperty>

<!-- Property: is singer of -->
<owl:ObjectProperty rdf:about="http://rdaregistry.info/Elements/u/P60031">
  <rdfs:isDefinedBy rdf:resource="http://rdaregistry.info/Elements/u/" />
  <reg:status rdf:resource="http://metadataregistry.org/uri/RegStatus/1001" />
  <reg:name xml:lang="en">singerOf</reg:name>
  <rdfs:label xml:lang="en">is singer of</rdfs:label>
  <skos:definition xml:lang="en">Relates a performer contributing to a resource by using his/her/their voice, with or without instrumental accompaniment, to produce music. a singer's performance may or may not include actual words to a resource.</skos:definition>
  <rdf:type rdf:resource="http://www.w3.org/1999/02/22-rdf-syntax-ns#Property" />
  <rdfs:subPropertyOf rdf:resource="http://rdaregistry.info/Elements/u/P60615" />
  <owl:inverseOf rdf:resource="http://rdaregistry.info/Elements/u/P60156" />
  <reg:hasSubproperty rdf:resource="http://rdaregistry.info/Elements/a/P50084" />
  <reg:lexicalAlias rdf:resource="http://rdaregistry.info/Elements/u/singerOf.en" />
</owl:ObjectProperty>

<!-- Property: has software developer -->
<owl:ObjectProperty rdf:about="http://rdaregistry.info/Elements/u/P60828">
  <rdfs:isDefinedBy rdf:resource="http://rdaregistry.info/Elements/u/" />
  <reg:status rdf:resource="http://metadataregistry.org/uri/RegStatus/1001" />
  <rdf:type rdf:resource="http://www.w3.org/1999/02/22-rdf-syntax-ns#Property" />
  <reg:name xml:lang="en">softwareDeveloper</reg:name>
  <rdfs:label xml:lang="en">has software developer</rdfs:label>
  <reg:lexicalAlias rdf:resource="http://rdaregistry.info/Elements/u/softwareDeveloper.en" />
  <skos:definition xml:lang="en">Relates a resource to an agent contributing to a resource by researching, designing, implementing, or testing software.</skos:definition>
  <owl:inverseOf rdf:resource="http://rdaregistry.info/Elements/u/P60829" />
  <reg:hasSubproperty rdf:resource="http://rdaregistry.info/Elements/e/P20280" />
  <rdfs:subPropertyOf rdf:resource="http://rdaregistry.info/Elements/u/P60398" />
</owl:ObjectProperty>

<!-- Property: is software developer of -->
<owl:ObjectProperty rdf:about="http://rdaregistry.info/Elements/u/P60829">
  <rdfs:isDefinedBy rdf:resource="http://rdaregistry.info/Elements/u/" />
  <reg:status rdf:resource="http://metadataregistry.org/uri/RegStatus/1001" />
  <rdf:type rdf:resource="http://www.w3.org/1999/02/22-rdf-syntax-ns#Property" />
  <reg:name xml:lang="en">softwareDeveloperOf</reg:name>
  <rdfs:label xml:lang="en">is software developer of</rdfs:label>
  <reg:lexicalAlias rdf:resource="http://rdaregistry.info/Elements/u/softwareDeveloperOf.en" />
  <skos:definition xml:lang="en">Relates an agent contributing to a resource by researching, designing, implementing, or testing software to a resource.</skos:definition>
  <owl:inverseOf rdf:resource="http://rdaregistry.info/Elements/u/P60828" />
  <reg:hasSubproperty rdf:resource="http://rdaregistry.info/Elements/a/P50263" />
  <rdfs:subPropertyOf rdf:resource="http://rdaregistry.info/Elements/u/P60626" />
</owl:ObjectProperty>

<!-- Property: has sound characteristic -->
<owl:ObjectProperty rdf:about="http://rdaregistry.info/Elements/u/P60351">
  <rdfs:isDefinedBy rdf:resource="http://rdaregistry.info/Elements/u/" />
  <reg:status rdf:resource="http://metadataregistry.org/uri/RegStatus/1001" />
  <reg:name xml:lang="en">soundCharacteristic</reg:name>
  <rdfs:label xml:lang="en">has sound characteristic</rdfs:label>
  <skos:definition xml:lang="en">Relates a resource to a technical specification relating to an encoding of sound in a resource.</skos:definition>
  <rdf:type rdf:resource="http://www.w3.org/1999/02/22-rdf-syntax-ns#Property" />
  <reg:hasSubproperty rdf:resource="http://rdaregistry.info/Elements/u/P60481" />
  <reg:hasSubproperty rdf:resource="http://rdaregistry.info/Elements/u/P60522" />
  <reg:hasSubproperty rdf:resource="http://rdaregistry.info/Elements/u/P60532" />
  <reg:hasSubproperty rdf:resource="http://rdaregistry.info/Elements/u/P60543" />
  <reg:hasSubproperty rdf:resource="http://rdaregistry.info/Elements/u/P60552" />
  <reg:hasSubproperty rdf:resource="http://rdaregistry.info/Elements/u/P60553" />
  <reg:hasSubproperty rdf:resource="http://rdaregistry.info/Elements/u/P60586" />
  <reg:hasSubproperty rdf:resource="http://rdaregistry.info/Elements/u/P60594" />
  <reg:hasSubproperty rdf:resource="http://rdaregistry.info/Elements/m/P30125" />
  <reg:lexicalAlias rdf:resource="http://rdaregistry.info/Elements/u/soundCharacteristic.en" />
</owl:ObjectProperty>

<!-- Property: has sound content -->
<owl:ObjectProperty rdf:about="http://rdaregistry.info/Elements/u/P60559">
  <rdfs:isDefinedBy rdf:resource="http://rdaregistry.info/Elements/u/" />
  <reg:status rdf:resource="http://metadataregistry.org/uri/RegStatus/1001" />
  <reg:name xml:lang="en">soundContent</reg:name>
  <rdfs:label xml:lang="en">has sound content</rdfs:label>
  <skos:definition xml:lang="en">Relates a resource to a presence or absence of sound in a resource.</skos:definition>
  <rdf:type rdf:resource="http://www.w3.org/1999/02/22-rdf-syntax-ns#Property" />
  <reg:hasSubproperty rdf:resource="http://rdaregistry.info/Elements/e/P20225" />
  <reg:lexicalAlias rdf:resource="http://rdaregistry.info/Elements/u/soundContent.en" />
</owl:ObjectProperty>

<!-- Property: has sound designer -->
<owl:ObjectProperty rdf:about="http://rdaregistry.info/Elements/u/P60811">
  <rdfs:isDefinedBy rdf:resource="http://rdaregistry.info/Elements/u/" />
  <reg:status rdf:resource="http://metadataregistry.org/uri/RegStatus/1001" />
  <rdf:type rdf:resource="http://www.w3.org/1999/02/22-rdf-syntax-ns#Property" />
  <reg:name xml:lang="en">soundDesigner</reg:name>
  <rdfs:label xml:lang="en">has sound designer</rdfs:label>
  <reg:lexicalAlias rdf:resource="http://rdaregistry.info/Elements/u/soundDesigner.en" />
  <skos:definition xml:lang="en">Relates a resource to an agent contributing to a resource by designing and creating audio/sound components.</skos:definition>
  <owl:inverseOf rdf:resource="http://rdaregistry.info/Elements/u/P60812" />
  <rdfs:subPropertyOf rdf:resource="http://rdaregistry.info/Elements/u/P60398" />
</owl:ObjectProperty>

<!-- Property: is sound designer of -->
<owl:ObjectProperty rdf:about="http://rdaregistry.info/Elements/u/P60812">
  <rdfs:isDefinedBy rdf:resource="http://rdaregistry.info/Elements/u/" />
  <reg:status rdf:resource="http://metadataregistry.org/uri/RegStatus/1001" />
  <rdf:type rdf:resource="http://www.w3.org/1999/02/22-rdf-syntax-ns#Property" />
  <reg:name xml:lang="en">soundDesignerOf</reg:name>
  <rdfs:label xml:lang="en">is sound designer of</rdfs:label>
  <reg:lexicalAlias rdf:resource="http://rdaregistry.info/Elements/u/soundDesignerOf.en" />
  <skos:definition xml:lang="en">Relates an agent contributing to a resource by designing and creating audio/sound components to a resource.</skos:definition>
  <owl:inverseOf rdf:resource="http://rdaregistry.info/Elements/u/P60811" />
  <rdfs:subPropertyOf rdf:resource="http://rdaregistry.info/Elements/u/P60626" />
</owl:ObjectProperty>

<!-- Property: has speaker -->
<owl:ObjectProperty rdf:about="http://rdaregistry.info/Elements/u/P60155">
  <rdfs:isDefinedBy rdf:resource="http://rdaregistry.info/Elements/u/" />
  <reg:status rdf:resource="http://metadataregistry.org/uri/RegStatus/1001" />
  <reg:name xml:lang="en">speaker</reg:name>
  <rdfs:label xml:lang="en">has speaker</rdfs:label>
  <skos:definition xml:lang="en">Relates a resource to a performer contributing to a resource by speaking words, such as a lecture, speech, etc.</skos:definition>
  <rdf:type rdf:resource="http://www.w3.org/1999/02/22-rdf-syntax-ns#Property" />
  <rdfs:subPropertyOf rdf:resource="http://rdaregistry.info/Elements/u/P60387" />
  <owl:inverseOf rdf:resource="http://rdaregistry.info/Elements/u/P60030" />
  <reg:hasSubproperty rdf:resource="http://rdaregistry.info/Elements/e/P20024" />
  <reg:lexicalAlias rdf:resource="http://rdaregistry.info/Elements/u/speaker.en" />
</owl:ObjectProperty>

<!-- Property: is speaker of -->
<owl:ObjectProperty rdf:about="http://rdaregistry.info/Elements/u/P60030">
  <rdfs:isDefinedBy rdf:resource="http://rdaregistry.info/Elements/u/" />
  <reg:status rdf:resource="http://metadataregistry.org/uri/RegStatus/1001" />
  <reg:name xml:lang="en">speakerOf</reg:name>
  <rdfs:label xml:lang="en">is speaker of</rdfs:label>
  <skos:definition xml:lang="en">Relates a performer contributing to a resource by speaking words, such as a lecture, speech, etc. to a resource.</skos:definition>
  <rdf:type rdf:resource="http://www.w3.org/1999/02/22-rdf-syntax-ns#Property" />
  <rdfs:subPropertyOf rdf:resource="http://rdaregistry.info/Elements/u/P60615" />
  <owl:inverseOf rdf:resource="http://rdaregistry.info/Elements/u/P60155" />
  <reg:hasSubproperty rdf:resource="http://rdaregistry.info/Elements/a/P50083" />
  <reg:lexicalAlias rdf:resource="http://rdaregistry.info/Elements/u/speakerOf.en" />
</owl:ObjectProperty>

<!-- Property: has special effects provider -->
<owl:ObjectProperty rdf:about="http://rdaregistry.info/Elements/u/P60749">
  <rdfs:isDefinedBy rdf:resource="http://rdaregistry.info/Elements/u/" />
  <reg:status rdf:resource="http://metadataregistry.org/uri/RegStatus/1001" />
  <rdf:type rdf:resource="http://www.w3.org/1999/02/22-rdf-syntax-ns#Property" />
  <reg:name xml:lang="en">specialEffectsProvider</reg:name>
  <rdfs:label xml:lang="en">has special effects provider</rdfs:label>
  <reg:lexicalAlias rdf:resource="http://rdaregistry.info/Elements/u/specialEffectsProvider.en" />
  <skos:definition xml:lang="en">Relates a resource to an agent contributing to a moving image or audio resource by designing and creating on-set special effects such as on-set mechanical effects and in-camera optical effects.</skos:definition>
  <owl:inverseOf rdf:resource="http://rdaregistry.info/Elements/u/P60755" />
  <rdfs:subPropertyOf rdf:resource="http://rdaregistry.info/Elements/u/P60398" />
</owl:ObjectProperty>

<!-- Property: is special effects provider of -->
<owl:ObjectProperty rdf:about="http://rdaregistry.info/Elements/u/P60755">
  <rdfs:isDefinedBy rdf:resource="http://rdaregistry.info/Elements/u/" />
  <reg:status rdf:resource="http://metadataregistry.org/uri/RegStatus/1001" />
  <rdf:type rdf:resource="http://www.w3.org/1999/02/22-rdf-syntax-ns#Property" />
  <reg:name xml:lang="en">specialEffectsProviderOf</reg:name>
  <rdfs:label xml:lang="en">is special effects provider of</rdfs:label>
  <reg:lexicalAlias rdf:resource="http://rdaregistry.info/Elements/u/specialEffectsProviderOf.en" />
  <skos:definition xml:lang="en">Relates an agent contributing to a moving image or audio resource by designing and creating on-set special effects, such as on-set mechanical effects and in-camera optical effects, to a resource.</skos:definition>
  <owl:inverseOf rdf:resource="http://rdaregistry.info/Elements/u/P60749" />
  <rdfs:subPropertyOf rdf:resource="http://rdaregistry.info/Elements/u/P60626" />
</owl:ObjectProperty>

<!-- Property: is special issue -->
<owl:ObjectProperty rdf:about="http://rdaregistry.info/Elements/u/P60207">
  <rdfs:isDefinedBy rdf:resource="http://rdaregistry.info/Elements/u/" />
  <reg:status rdf:resource="http://metadataregistry.org/uri/RegStatus/1001" />
  <reg:name xml:lang="en">specialIssue</reg:name>
  <rdfs:label xml:lang="en">is special issue</rdfs:label>
  <skos:definition xml:lang="en">Relates a resource to a resource that consists of a single issue or a supplementary section of a periodical or newspaper devoted to a special subject, with or without serial numbering.</skos:definition>
  <rdf:type rdf:resource="http://www.w3.org/1999/02/22-rdf-syntax-ns#Property" />
  <rdfs:subPropertyOf rdf:resource="http://rdaregistry.info/Elements/u/P60249" />
  <owl:inverseOf rdf:resource="http://rdaregistry.info/Elements/u/P60317" />
  <reg:hasSubproperty rdf:resource="http://rdaregistry.info/Elements/m/P30030" />
  <reg:lexicalAlias rdf:resource="http://rdaregistry.info/Elements/u/specialIssue.en" />
</owl:ObjectProperty>

<!-- Property: is special issue of -->
<owl:ObjectProperty rdf:about="http://rdaregistry.info/Elements/u/P60317">
  <rdfs:isDefinedBy rdf:resource="http://rdaregistry.info/Elements/u/" />
  <reg:status rdf:resource="http://metadataregistry.org/uri/RegStatus/1001" />
  <reg:name xml:lang="en">specialIssueOf</reg:name>
  <rdfs:label xml:lang="en">is special issue of</rdfs:label>
  <skos:definition xml:lang="en">Relates a resource to a serial or newspaper containing a single issue or a supplementary section devoted to a special subject, with or without serial numbering, such as an anniversary number of a periodical or newspaper.</skos:definition>
  <rdf:type rdf:resource="http://www.w3.org/1999/02/22-rdf-syntax-ns#Property" />
  <rdfs:subPropertyOf rdf:resource="http://rdaregistry.info/Elements/u/P60101" />
  <owl:inverseOf rdf:resource="http://rdaregistry.info/Elements/u/P60207" />
  <reg:hasSubproperty rdf:resource="http://rdaregistry.info/Elements/m/P30101" />
  <reg:lexicalAlias rdf:resource="http://rdaregistry.info/Elements/u/specialIssueOf.en" />
</owl:ObjectProperty>

<!-- Property: has special playback characteristic -->
<owl:ObjectProperty rdf:about="http://rdaregistry.info/Elements/u/P60481">
  <rdfs:isDefinedBy rdf:resource="http://rdaregistry.info/Elements/u/" />
  <reg:status rdf:resource="http://metadataregistry.org/uri/RegStatus/1001" />
  <reg:name xml:lang="en">specialPlaybackCharacteristic</reg:name>
  <rdfs:label xml:lang="en">has special playback characteristic</rdfs:label>
  <skos:definition xml:lang="en">Relates a resource to an equalization system, noise reduction system, etc., used in making an audio recording.</skos:definition>
  <rdf:type rdf:resource="http://www.w3.org/1999/02/22-rdf-syntax-ns#Property" />
  <rdfs:subPropertyOf rdf:resource="http://rdaregistry.info/Elements/u/P60351" />
  <reg:hasSubproperty rdf:resource="http://rdaregistry.info/Elements/m/P30138" />
  <reg:lexicalAlias rdf:resource="http://rdaregistry.info/Elements/u/specialPlaybackCharacteristic.en" />
</owl:ObjectProperty>

<!-- Property: is split into -->
<owl:ObjectProperty rdf:about="http://rdaregistry.info/Elements/u/P60503">
  <rdfs:isDefinedBy rdf:resource="http://rdaregistry.info/Elements/u/" />
  <reg:status rdf:resource="http://metadataregistry.org/uri/RegStatus/1001" />
  <reg:name xml:lang="en">splitInto</reg:name>
  <rdfs:label xml:lang="en">is split into</rdfs:label>
  <skos:definition xml:lang="en">Relates a resource to a resource resulting from a division of an earlier resource into two or more separate resources.</skos:definition>
  <rdf:type rdf:resource="http://www.w3.org/1999/02/22-rdf-syntax-ns#Property" />
  <rdfs:subPropertyOf rdf:resource="http://rdaregistry.info/Elements/u/P60278" />
  <owl:inverseOf rdf:resource="http://rdaregistry.info/Elements/u/P60276" />
  <reg:hasSubproperty rdf:resource="http://rdaregistry.info/Elements/e/P20200" />
  <reg:lexicalAlias rdf:resource="http://rdaregistry.info/Elements/u/splitInto.en" />
</owl:ObjectProperty>

<!-- Property: has sponsor -->
<owl:ObjectProperty rdf:about="http://rdaregistry.info/Elements/u/P60676">
  <rdfs:isDefinedBy rdf:resource="http://rdaregistry.info/Elements/u/" />
  <reg:status rdf:resource="http://metadataregistry.org/uri/RegStatus/1001" />
  <reg:name xml:lang="en">sponsor</reg:name>
  <rdfs:label xml:lang="en">has sponsor</rdfs:label>
  <skos:definition xml:lang="en">Relates an agent sponsoring an agent to an agent.</skos:definition>
  <rdf:type rdf:resource="http://www.w3.org/1999/02/22-rdf-syntax-ns#Property" />
  <owl:inverseOf rdf:resource="http://rdaregistry.info/Elements/u/P60688" />
  <reg:hasSubproperty rdf:resource="http://rdaregistry.info/Elements/a/P50015" />
  <reg:hasSubproperty rdf:resource="http://rdaregistry.info/Elements/a/P50021" />
  <reg:hasSubproperty rdf:resource="http://rdaregistry.info/Elements/a/P50028" />
  <reg:lexicalAlias rdf:resource="http://rdaregistry.info/Elements/u/sponsor.en" />
</owl:ObjectProperty>

<!-- Property: has sponsored entity -->
<owl:ObjectProperty rdf:about="http://rdaregistry.info/Elements/u/P60688">
  <rdfs:isDefinedBy rdf:resource="http://rdaregistry.info/Elements/u/" />
  <reg:status rdf:resource="http://metadataregistry.org/uri/RegStatus/1001" />
  <reg:name xml:lang="en">sponsoredEntity</reg:name>
  <rdfs:label xml:lang="en">has sponsored entity</rdfs:label>
  <skos:definition xml:lang="en">Relates an agent that an agent sponsors to an agent.</skos:definition>
  <rdf:type rdf:resource="http://www.w3.org/1999/02/22-rdf-syntax-ns#Property" />
  <owl:inverseOf rdf:resource="http://rdaregistry.info/Elements/u/P60676" />
  <reg:hasSubproperty rdf:resource="http://rdaregistry.info/Elements/a/P50009" />
  <reg:hasSubproperty rdf:resource="http://rdaregistry.info/Elements/a/P50063" />
  <reg:lexicalAlias rdf:resource="http://rdaregistry.info/Elements/u/sponsoredEntity.en" />
</owl:ObjectProperty>

<!-- Property: has sponsoring body -->
<owl:ObjectProperty rdf:about="http://rdaregistry.info/Elements/u/P60451">
  <rdfs:isDefinedBy rdf:resource="http://rdaregistry.info/Elements/u/" />
  <reg:status rdf:resource="http://metadataregistry.org/uri/RegStatus/1001" />
  <reg:name xml:lang="en">sponsoringBody</reg:name>
  <rdfs:label xml:lang="en">has sponsoring body</rdfs:label>
  <skos:definition xml:lang="en">Relates a resource to an agent sponsoring some aspect of a resource, such as funding research or sponsoring an event.</skos:definition>
  <rdf:type rdf:resource="http://www.w3.org/1999/02/22-rdf-syntax-ns#Property" />
  <rdfs:subPropertyOf rdf:resource="http://rdaregistry.info/Elements/u/P60374" />
  <owl:inverseOf rdf:resource="http://rdaregistry.info/Elements/u/P60675" />
  <reg:lexicalAlias rdf:resource="http://rdaregistry.info/Elements/u/sponsoringBody.en" />
</owl:ObjectProperty>

<!-- Property: is sponsoring body of -->
<owl:ObjectProperty rdf:about="http://rdaregistry.info/Elements/u/P60675">
  <rdfs:isDefinedBy rdf:resource="http://rdaregistry.info/Elements/u/" />
  <reg:status rdf:resource="http://metadataregistry.org/uri/RegStatus/1001" />
  <reg:name xml:lang="en">sponsoringBodyOf</reg:name>
  <rdfs:label xml:lang="en">is sponsoring body of</rdfs:label>
  <skos:definition xml:lang="en">Relates an agent sponsoring some aspect of a resource, e.g., funding research, sponsoring an event to a resource.</skos:definition>
  <rdf:type rdf:resource="http://www.w3.org/1999/02/22-rdf-syntax-ns#Property" />
  <rdfs:subPropertyOf rdf:resource="http://rdaregistry.info/Elements/u/P60602" />
  <owl:inverseOf rdf:resource="http://rdaregistry.info/Elements/u/P60451" />
  <reg:hasSubproperty rdf:resource="http://rdaregistry.info/Elements/a/P50226" />
  <reg:lexicalAlias rdf:resource="http://rdaregistry.info/Elements/u/sponsoringBodyOf.en" />
</owl:ObjectProperty>

<!-- Property: has stage director -->
<owl:ObjectProperty rdf:about="http://rdaregistry.info/Elements/u/P60399">
  <rdfs:isDefinedBy rdf:resource="http://rdaregistry.info/Elements/u/" />
  <reg:status rdf:resource="http://metadataregistry.org/uri/RegStatus/1001" />
  <reg:name xml:lang="en">stageDirector</reg:name>
  <rdfs:label xml:lang="en">has stage director</rdfs:label>
  <skos:definition xml:lang="en">Relates a resource to an agent contributing to a stage resource through the general management and supervision of a performance.</skos:definition>
  <rdf:type rdf:resource="http://www.w3.org/1999/02/22-rdf-syntax-ns#Property" />
  <rdfs:subPropertyOf rdf:resource="http://rdaregistry.info/Elements/u/P60398" />
  <owl:inverseOf rdf:resource="http://rdaregistry.info/Elements/u/P60627" />
  <reg:hasSubproperty rdf:resource="http://rdaregistry.info/Elements/e/P20031" />
  <reg:lexicalAlias rdf:resource="http://rdaregistry.info/Elements/u/stageDirector.en" />
</owl:ObjectProperty>

<!-- Property: is stage director of -->
<owl:ObjectProperty rdf:about="http://rdaregistry.info/Elements/u/P60627">
  <rdfs:isDefinedBy rdf:resource="http://rdaregistry.info/Elements/u/" />
  <reg:status rdf:resource="http://metadataregistry.org/uri/RegStatus/1001" />
  <reg:name xml:lang="en">stageDirectorOf</reg:name>
  <rdfs:label xml:lang="en">is stage director of</rdfs:label>
  <skos:definition xml:lang="en">Relates an agent contributing to a stage resource through the general management and supervision of a performance to a resource.</skos:definition>
  <rdf:type rdf:resource="http://www.w3.org/1999/02/22-rdf-syntax-ns#Property" />
  <rdfs:subPropertyOf rdf:resource="http://rdaregistry.info/Elements/u/P60626" />
  <owl:inverseOf rdf:resource="http://rdaregistry.info/Elements/u/P60399" />
  <reg:hasSubproperty rdf:resource="http://rdaregistry.info/Elements/a/P50139" />
  <reg:lexicalAlias rdf:resource="http://rdaregistry.info/Elements/u/stageDirectorOf.en" />
</owl:ObjectProperty>

<!-- Property: has statement of responsibility -->
<owl:ObjectProperty rdf:about="http://rdaregistry.info/Elements/u/P60339">
  <rdfs:isDefinedBy rdf:resource="http://rdaregistry.info/Elements/u/" />
  <reg:status rdf:resource="http://metadataregistry.org/uri/RegStatus/1001" />
  <reg:name xml:lang="en">statementOfResponsibility</reg:name>
  <rdfs:label xml:lang="en">has statement of responsibility</rdfs:label>
  <skos:definition xml:lang="en">Relates a resource to a statement relating to anidentification or function of any agents responsible for the creation of, or contributing to a realization of, the intellectual or artistic content of a resource.</skos:definition>
  <rdf:type rdf:resource="http://www.w3.org/1999/02/22-rdf-syntax-ns#Property" />
  <reg:hasSubproperty rdf:resource="http://rdaregistry.info/Elements/u/P60327" />
  <reg:hasSubproperty rdf:resource="http://rdaregistry.info/Elements/u/P60338" />
  <reg:hasSubproperty rdf:resource="http://rdaregistry.info/Elements/m/P30117" />
  <reg:lexicalAlias rdf:resource="http://rdaregistry.info/Elements/u/statementOfResponsibility.en" />
</owl:ObjectProperty>

<!-- Property: has statement of responsibility relating to edition -->
<owl:ObjectProperty rdf:about="http://rdaregistry.info/Elements/u/P60343">
  <rdfs:isDefinedBy rdf:resource="http://rdaregistry.info/Elements/u/" />
  <reg:status rdf:resource="http://metadataregistry.org/uri/RegStatus/1001" />
  <reg:name xml:lang="en">statementOfResponsibilityRelatingToEdition</reg:name>
  <rdfs:label xml:lang="en">has statement of responsibility relating to edition</rdfs:label>
  <skos:definition xml:lang="en">Relates a resource to a statement relating to an identification of agents responsible for an edition being described but not to all editions.</skos:definition>
  <rdf:type rdf:resource="http://www.w3.org/1999/02/22-rdf-syntax-ns#Property" />
  <reg:hasSubproperty rdf:resource="http://rdaregistry.info/Elements/m/P30121" />
  <reg:lexicalAlias rdf:resource="http://rdaregistry.info/Elements/u/statementOfResponsibilityRelatingToEdition.en" />
</owl:ObjectProperty>

<!-- Property: has statement of responsibility relating to named revision of edition -->
<owl:ObjectProperty rdf:about="http://rdaregistry.info/Elements/u/P60340">
  <rdfs:isDefinedBy rdf:resource="http://rdaregistry.info/Elements/u/" />
  <reg:status rdf:resource="http://metadataregistry.org/uri/RegStatus/1001" />
  <reg:name xml:lang="en">statementOfResponsibilityRelatingToNamedRevisionOfEdition</reg:name>
  <rdfs:label xml:lang="en">has statement of responsibility relating to named revision of edition</rdfs:label>
  <skos:definition xml:lang="en">Relates a resource to a statement relating to an identification of agents responsible for a named revision of an edition.</skos:definition>
  <rdf:type rdf:resource="http://www.w3.org/1999/02/22-rdf-syntax-ns#Property" />
  <reg:hasSubproperty rdf:resource="http://rdaregistry.info/Elements/m/P30118" />
  <reg:lexicalAlias rdf:resource="http://rdaregistry.info/Elements/u/statementOfResponsibilityRelatingToNamedRevisionOfEdition.en" />
</owl:ObjectProperty>

<!-- Property: has statement of responsibility relating to series -->
<owl:ObjectProperty rdf:about="http://rdaregistry.info/Elements/u/P60341">
  <rdfs:isDefinedBy rdf:resource="http://rdaregistry.info/Elements/u/" />
  <reg:status rdf:resource="http://metadataregistry.org/uri/RegStatus/1001" />
  <reg:name xml:lang="en">statementOfResponsibilityRelatingToSeries</reg:name>
  <rdfs:label xml:lang="en">has statement of responsibility relating to series</rdfs:label>
  <skos:definition xml:lang="en">Relates a resource to a statement relating to an identification of agents responsible for a series.</skos:definition>
  <rdf:type rdf:resource="http://www.w3.org/1999/02/22-rdf-syntax-ns#Property" />
  <reg:hasSubproperty rdf:resource="http://rdaregistry.info/Elements/m/P30119" />
  <reg:lexicalAlias rdf:resource="http://rdaregistry.info/Elements/u/statementOfResponsibilityRelatingToSeries.en" />
</owl:ObjectProperty>

<!-- Property: has statement of responsibility relating to subseries -->
<owl:ObjectProperty rdf:about="http://rdaregistry.info/Elements/u/P60342">
  <rdfs:isDefinedBy rdf:resource="http://rdaregistry.info/Elements/u/" />
  <reg:status rdf:resource="http://metadataregistry.org/uri/RegStatus/1001" />
  <reg:name xml:lang="en">statementOfResponsibilityRelatingToSubseries</reg:name>
  <rdfs:label xml:lang="en">has statement of responsibility relating to subseries</rdfs:label>
  <skos:definition xml:lang="en">Relates a resource to a statement relating to an identification of agents responsible for a subseries.</skos:definition>
  <rdf:type rdf:resource="http://www.w3.org/1999/02/22-rdf-syntax-ns#Property" />
  <reg:hasSubproperty rdf:resource="http://rdaregistry.info/Elements/m/P30120" />
  <reg:lexicalAlias rdf:resource="http://rdaregistry.info/Elements/u/statementOfResponsibilityRelatingToSubseries.en" />
</owl:ObjectProperty>

<!-- Property: has statement of responsibility relating to title proper -->
<owl:ObjectProperty rdf:about="http://rdaregistry.info/Elements/u/P60327">
  <rdfs:isDefinedBy rdf:resource="http://rdaregistry.info/Elements/u/" />
  <reg:status rdf:resource="http://metadataregistry.org/uri/RegStatus/1001" />
  <reg:name xml:lang="en">statementOfResponsibilityRelatingToTitleProper</reg:name>
  <rdfs:label xml:lang="en">has statement of responsibility relating to title proper</rdfs:label>
  <skos:definition xml:lang="en">Relates a resource to a statement associated with a title proper of a resource that relates to an identification or function of agents responsible for the creation of, or contributing to a realization of, the intellectual or artistic content of a resource.</skos:definition>
  <rdf:type rdf:resource="http://www.w3.org/1999/02/22-rdf-syntax-ns#Property" />
  <rdfs:subPropertyOf rdf:resource="http://rdaregistry.info/Elements/u/P60339" />
  <reg:hasSubproperty rdf:resource="http://rdaregistry.info/Elements/m/P30105" />
  <reg:lexicalAlias rdf:resource="http://rdaregistry.info/Elements/u/statementOfResponsibilityRelatingToTitleProper.en" />
</owl:ObjectProperty>

<!-- Property: has storyteller -->
<owl:ObjectProperty rdf:about="http://rdaregistry.info/Elements/u/P60154">
  <rdfs:isDefinedBy rdf:resource="http://rdaregistry.info/Elements/u/" />
  <reg:status rdf:resource="http://metadataregistry.org/uri/RegStatus/1001" />
  <reg:name xml:lang="en">storyteller</reg:name>
  <rdfs:label xml:lang="en">has storyteller</rdfs:label>
  <skos:definition xml:lang="en">Relates a resource to a performer contributing to a resource by relaying a creator's original story with dramatic or theatrical interpretation.</skos:definition>
  <rdf:type rdf:resource="http://www.w3.org/1999/02/22-rdf-syntax-ns#Property" />
  <rdfs:subPropertyOf rdf:resource="http://rdaregistry.info/Elements/u/P60387" />
  <owl:inverseOf rdf:resource="http://rdaregistry.info/Elements/u/P60029" />
  <reg:hasSubproperty rdf:resource="http://rdaregistry.info/Elements/e/P20023" />
  <reg:lexicalAlias rdf:resource="http://rdaregistry.info/Elements/u/storyteller.en" />
</owl:ObjectProperty>

<!-- Property: is storyteller of -->
<owl:ObjectProperty rdf:about="http://rdaregistry.info/Elements/u/P60029">
  <rdfs:isDefinedBy rdf:resource="http://rdaregistry.info/Elements/u/" />
  <reg:status rdf:resource="http://metadataregistry.org/uri/RegStatus/1001" />
  <reg:name xml:lang="en">storytellerOf</reg:name>
  <rdfs:label xml:lang="en">is storyteller of</rdfs:label>
  <skos:definition xml:lang="en">Relates a performer contributing to a resource by relaying a creator's original story with dramatic or theatrical interpretation to a resource.</skos:definition>
  <rdf:type rdf:resource="http://www.w3.org/1999/02/22-rdf-syntax-ns#Property" />
  <rdfs:subPropertyOf rdf:resource="http://rdaregistry.info/Elements/u/P60615" />
  <owl:inverseOf rdf:resource="http://rdaregistry.info/Elements/u/P60154" />
  <reg:hasSubproperty rdf:resource="http://rdaregistry.info/Elements/a/P50082" />
  <reg:lexicalAlias rdf:resource="http://rdaregistry.info/Elements/u/storytellerOf.en" />
</owl:ObjectProperty>

<!-- Property: has strings of coordinate pairs -->
<owl:ObjectProperty rdf:about="http://rdaregistry.info/Elements/u/P60347">
  <rdfs:isDefinedBy rdf:resource="http://rdaregistry.info/Elements/u/" />
  <reg:status rdf:resource="http://metadataregistry.org/uri/RegStatus/1001" />
  <reg:name xml:lang="en">stringsOfCoordinatePairs</reg:name>
  <rdfs:label xml:lang="en">has strings of coordinate pairs</rdfs:label>
  <skos:definition xml:lang="en">Relates a resource to a system for identifying the precise area covered by the cartographic content of a resource using coordinates for each vertex of a polygon.</skos:definition>
  <rdf:type rdf:resource="http://www.w3.org/1999/02/22-rdf-syntax-ns#Property" />
  <rdfs:subPropertyOf rdf:resource="http://rdaregistry.info/Elements/u/P60109" />
  <reg:lexicalAlias rdf:resource="http://rdaregistry.info/Elements/u/stringsOfCoordinatePairs.en" />
</owl:ObjectProperty>

<!-- Property: has student -->
<owl:ObjectProperty rdf:about="http://rdaregistry.info/Elements/u/P60862">
  <rdfs:isDefinedBy rdf:resource="http://rdaregistry.info/Elements/u/" />
  <reg:status rdf:resource="http://metadataregistry.org/uri/RegStatus/1001" />
  <rdf:type rdf:resource="http://www.w3.org/1999/02/22-rdf-syntax-ns#Property" />
  <reg:name xml:lang="en">student</reg:name>
  <rdfs:label xml:lang="en">has student</rdfs:label>
  <reg:lexicalAlias rdf:resource="http://rdaregistry.info/Elements/u/student.en" />
  <skos:definition xml:lang="en">Relates an agent to an agent who receives instruction from another agent.</skos:definition>
  <owl:inverseOf rdf:resource="http://rdaregistry.info/Elements/u/P60863" />
  <reg:hasSubproperty rdf:resource="http://rdaregistry.info/Elements/a/P50281" />
  <rdfs:subPropertyOf rdf:resource="http://rdaregistry.info/Elements/u/P60454" />
</owl:ObjectProperty>

<!-- Property: is student at -->
<owl:ObjectProperty rdf:about="http://rdaregistry.info/Elements/u/P60856">
  <rdfs:isDefinedBy rdf:resource="http://rdaregistry.info/Elements/u/" />
  <reg:status rdf:resource="http://metadataregistry.org/uri/RegStatus/1001" />
  <rdf:type rdf:resource="http://www.w3.org/1999/02/22-rdf-syntax-ns#Property" />
  <reg:name xml:lang="en">studentAt</reg:name>
  <rdfs:label xml:lang="en">is student at</rdfs:label>
  <reg:lexicalAlias rdf:resource="http://rdaregistry.info/Elements/u/studentAt.en" />
  <skos:definition xml:lang="en">Relates an agent to an educational institution that provides instruction to an agent.</skos:definition>
  <owl:inverseOf rdf:resource="http://rdaregistry.info/Elements/u/P60855" />
  <reg:hasSubproperty rdf:resource="http://rdaregistry.info/Elements/a/P50288" />
  <rdfs:subPropertyOf rdf:resource="http://rdaregistry.info/Elements/u/P60454" />
</owl:ObjectProperty>

<!-- Property: has subject -->
<owl:ObjectProperty rdf:about="http://rdaregistry.info/Elements/u/P60805">
  <rdfs:isDefinedBy rdf:resource="http://rdaregistry.info/Elements/u/" />
  <reg:status rdf:resource="http://metadataregistry.org/uri/RegStatus/1001" />
  <rdf:type rdf:resource="http://www.w3.org/1999/02/22-rdf-syntax-ns#Property" />
  <reg:name xml:lang="en">subject</reg:name>
  <rdfs:label xml:lang="en">has subject</rdfs:label>
  <reg:lexicalAlias rdf:resource="http://rdaregistry.info/Elements/u/subject.en" />
  <skos:definition xml:lang="en">Relates a resource to a subject of a resource; i.e., an indication of what a resource is about.</skos:definition>
  <owl:inverseOf rdf:resource="http://rdaregistry.info/Elements/u/P60806" />
</owl:ObjectProperty>

<!-- Property: is subject of -->
<owl:ObjectProperty rdf:about="http://rdaregistry.info/Elements/u/P60806">
  <rdfs:isDefinedBy rdf:resource="http://rdaregistry.info/Elements/u/" />
  <reg:status rdf:resource="http://metadataregistry.org/uri/RegStatus/1001" />
  <rdf:type rdf:resource="http://www.w3.org/1999/02/22-rdf-syntax-ns#Property" />
  <reg:name xml:lang="en">subjectOf</reg:name>
  <rdfs:label xml:lang="en">is subject of</rdfs:label>
  <reg:lexicalAlias rdf:resource="http://rdaregistry.info/Elements/u/subjectOf.en" />
  <skos:definition xml:lang="en">Relates a resource to a resource that is about a resource.</skos:definition>
  <owl:inverseOf rdf:resource="http://rdaregistry.info/Elements/u/P60805" />
</owl:ObjectProperty>

<!-- Property: is subseries -->
<owl:ObjectProperty rdf:about="http://rdaregistry.info/Elements/u/P60316">
  <rdfs:isDefinedBy rdf:resource="http://rdaregistry.info/Elements/u/" />
  <reg:status rdf:resource="http://metadataregistry.org/uri/RegStatus/1001" />
  <reg:name xml:lang="en">subseries</reg:name>
  <rdfs:label xml:lang="en">is subseries</rdfs:label>
  <skos:definition xml:lang="en">Relates a resource to a serial or multipart resource that consistently appears in a larger resource; a title of the larger resource appears on all issues or parts of a subseries</skos:definition>
  <rdf:type rdf:resource="http://www.w3.org/1999/02/22-rdf-syntax-ns#Property" />
  <rdfs:subPropertyOf rdf:resource="http://rdaregistry.info/Elements/u/P60249" />
  <owl:inverseOf rdf:resource="http://rdaregistry.info/Elements/u/P60192" />
  <reg:lexicalAlias rdf:resource="http://rdaregistry.info/Elements/u/subseries.en" />
</owl:ObjectProperty>

<!-- Property: is subseries of -->
<owl:ObjectProperty rdf:about="http://rdaregistry.info/Elements/u/P60192">
  <rdfs:isDefinedBy rdf:resource="http://rdaregistry.info/Elements/u/" />
  <reg:status rdf:resource="http://metadataregistry.org/uri/RegStatus/1001" />
  <reg:name xml:lang="en">subseriesOf</reg:name>
  <rdfs:label xml:lang="en">is subseries of</rdfs:label>
  <skos:definition xml:lang="en">Relates a resource to a resource in which a part consistently appears; a title of the larger resource appears on all issues or parts of a subseries.</skos:definition>
  <rdf:type rdf:resource="http://www.w3.org/1999/02/22-rdf-syntax-ns#Property" />
  <rdfs:subPropertyOf rdf:resource="http://rdaregistry.info/Elements/u/P60101" />
  <owl:inverseOf rdf:resource="http://rdaregistry.info/Elements/u/P60316" />
  <reg:lexicalAlias rdf:resource="http://rdaregistry.info/Elements/u/subseriesOf.en" />
</owl:ObjectProperty>

<!-- Property: is succeeded by -->
<owl:ObjectProperty rdf:about="http://rdaregistry.info/Elements/u/P60278">
  <rdfs:isDefinedBy rdf:resource="http://rdaregistry.info/Elements/u/" />
  <reg:status rdf:resource="http://metadataregistry.org/uri/RegStatus/1001" />
  <reg:name xml:lang="en">succeededBy</reg:name>
  <rdfs:label xml:lang="en">is succeeded by</rdfs:label>
  <skos:definition xml:lang="en">Relates a resource to a resource that succeeds, that is, is later in time or after in a narrative, etc., a preceding resource.</skos:definition>
  <rdf:type rdf:resource="http://www.w3.org/1999/02/22-rdf-syntax-ns#Property" />
  <rdfs:subPropertyOf rdf:resource="http://rdaregistry.info/Elements/u/P60713" />
  <owl:inverseOf rdf:resource="http://rdaregistry.info/Elements/u/P60261" />
  <reg:hasSubproperty rdf:resource="http://rdaregistry.info/Elements/u/P60102" />
  <reg:hasSubproperty rdf:resource="http://rdaregistry.info/Elements/u/P60103" />
  <reg:hasSubproperty rdf:resource="http://rdaregistry.info/Elements/u/P60104" />
  <reg:hasSubproperty rdf:resource="http://rdaregistry.info/Elements/u/P60199" />
  <reg:hasSubproperty rdf:resource="http://rdaregistry.info/Elements/u/P60247" />
  <reg:hasSubproperty rdf:resource="http://rdaregistry.info/Elements/u/P60248" />
  <reg:hasSubproperty rdf:resource="http://rdaregistry.info/Elements/u/P60306" />
  <reg:hasSubproperty rdf:resource="http://rdaregistry.info/Elements/u/P60310" />
  <reg:hasSubproperty rdf:resource="http://rdaregistry.info/Elements/u/P60503" />
  <reg:hasSubproperty rdf:resource="http://rdaregistry.info/Elements/u/P60504" />
  <reg:hasSubproperty rdf:resource="http://rdaregistry.info/Elements/e/P20169" />
  <reg:lexicalAlias rdf:resource="http://rdaregistry.info/Elements/u/succeededBy.en" />
</owl:ObjectProperty>

<!-- Property: has successor -->
<owl:ObjectProperty rdf:about="http://rdaregistry.info/Elements/u/P60686">
  <rdfs:isDefinedBy rdf:resource="http://rdaregistry.info/Elements/u/" />
  <reg:status rdf:resource="http://metadataregistry.org/uri/RegStatus/1001" />
  <reg:name xml:lang="en">successor</reg:name>
  <rdfs:label xml:lang="en">has successor</rdfs:label>
  <skos:definition xml:lang="en">Relates an agent that succeeds or follows another agent to an agent.</skos:definition>
  <rdf:type rdf:resource="http://www.w3.org/1999/02/22-rdf-syntax-ns#Property" />
  <owl:inverseOf rdf:resource="http://rdaregistry.info/Elements/u/P60683" />
  <reg:hasSubproperty rdf:resource="http://rdaregistry.info/Elements/a/P50016" />
  <reg:hasSubproperty rdf:resource="http://rdaregistry.info/Elements/a/P50053" />
  <reg:hasSubproperty rdf:resource="http://rdaregistry.info/Elements/a/P50099" />
  <reg:lexicalAlias rdf:resource="http://rdaregistry.info/Elements/u/successor.en" />
</owl:ObjectProperty>

<!-- Property: has summarization of content -->
<owl:ObjectProperty rdf:about="http://rdaregistry.info/Elements/u/P60372">
  <rdfs:isDefinedBy rdf:resource="http://rdaregistry.info/Elements/u/" />
  <reg:status rdf:resource="http://metadataregistry.org/uri/RegStatus/1001" />
  <reg:name xml:lang="en">summarizationOfContent</reg:name>
  <rdfs:label xml:lang="en">has summarization of content</rdfs:label>
  <skos:definition xml:lang="en">Relates a resource to an abstract, summary, synopsis, etc., of the content of a resource.</skos:definition>
  <rdf:type rdf:resource="http://www.w3.org/1999/02/22-rdf-syntax-ns#Property" />
  <reg:hasSubproperty rdf:resource="http://rdaregistry.info/Elements/e/P20069" />
  <reg:lexicalAlias rdf:resource="http://rdaregistry.info/Elements/u/summarizationOfContent.en" />
</owl:ObjectProperty>

<!-- Property: is summarized as -->
<owl:ObjectProperty rdf:about="http://rdaregistry.info/Elements/u/P60205">
  <rdfs:isDefinedBy rdf:resource="http://rdaregistry.info/Elements/u/" />
  <reg:status rdf:resource="http://metadataregistry.org/uri/RegStatus/1001" />
  <reg:name xml:lang="en">summarizedAs</reg:name>
  <rdfs:label xml:lang="en">is summarized as</rdfs:label>
  <skos:definition xml:lang="en">Relates a resource to a resource that consists of a brief recapitulation of the content of a source resource.</skos:definition>
  <rdf:type rdf:resource="http://www.w3.org/1999/02/22-rdf-syntax-ns#Property" />
  <rdfs:subPropertyOf rdf:resource="http://rdaregistry.info/Elements/u/P60250" />
  <owl:inverseOf rdf:resource="http://rdaregistry.info/Elements/u/P60289" />
  <reg:hasSubproperty rdf:resource="http://rdaregistry.info/Elements/e/P20106" />
  <reg:lexicalAlias rdf:resource="http://rdaregistry.info/Elements/u/summarizedAs.en" />
</owl:ObjectProperty>

<!-- Property: is summary of -->
<owl:ObjectProperty rdf:about="http://rdaregistry.info/Elements/u/P60289">
  <rdfs:isDefinedBy rdf:resource="http://rdaregistry.info/Elements/u/" />
  <reg:status rdf:resource="http://metadataregistry.org/uri/RegStatus/1001" />
  <reg:name xml:lang="en">summaryOf</reg:name>
  <rdfs:label xml:lang="en">is summary of</rdfs:label>
  <skos:definition xml:lang="en">Relates a resource to a resource used as a basis for a brief recapitulation of its content.</skos:definition>
  <rdf:type rdf:resource="http://www.w3.org/1999/02/22-rdf-syntax-ns#Property" />
  <rdfs:subPropertyOf rdf:resource="http://rdaregistry.info/Elements/u/P60305" />
  <owl:inverseOf rdf:resource="http://rdaregistry.info/Elements/u/P60205" />
  <reg:hasSubproperty rdf:resource="http://rdaregistry.info/Elements/e/P20179" />
  <reg:lexicalAlias rdf:resource="http://rdaregistry.info/Elements/u/summaryOf.en" />
</owl:ObjectProperty>

<!-- Property: is supplement -->
<owl:ObjectProperty rdf:about="http://rdaregistry.info/Elements/u/P60281">
  <rdfs:isDefinedBy rdf:resource="http://rdaregistry.info/Elements/u/" />
  <reg:status rdf:resource="http://metadataregistry.org/uri/RegStatus/1001" />
  <reg:name xml:lang="en">supplement</reg:name>
  <rdfs:label xml:lang="en">is supplement</rdfs:label>
  <skos:definition xml:lang="en">Relates a resource to a resource that updates or otherwise complements a predominant resource.</skos:definition>
  <rdf:type rdf:resource="http://www.w3.org/1999/02/22-rdf-syntax-ns#Property" />
  <rdfs:subPropertyOf rdf:resource="http://rdaregistry.info/Elements/u/P60204" />
  <owl:inverseOf rdf:resource="http://rdaregistry.info/Elements/u/P60259" />
  <reg:hasSubproperty rdf:resource="http://rdaregistry.info/Elements/e/P20172" />
  <reg:lexicalAlias rdf:resource="http://rdaregistry.info/Elements/u/supplement.en" />
</owl:ObjectProperty>

<!-- Property: has supplementary content -->
<owl:ObjectProperty rdf:about="http://rdaregistry.info/Elements/u/P60485">
  <rdfs:isDefinedBy rdf:resource="http://rdaregistry.info/Elements/u/" />
  <reg:status rdf:resource="http://metadataregistry.org/uri/RegStatus/1001" />
  <reg:name xml:lang="en">supplementaryContent</reg:name>
  <rdfs:label xml:lang="en">has supplementary content</rdfs:label>
  <skos:definition xml:lang="en">Relates a resource to an indication of content that updates or complements a primary content of a resource.</skos:definition>
  <rdf:type rdf:resource="http://www.w3.org/1999/02/22-rdf-syntax-ns#Property" />
  <reg:hasSubproperty rdf:resource="http://rdaregistry.info/Elements/e/P20206" />
  <reg:lexicalAlias rdf:resource="http://rdaregistry.info/Elements/u/supplementaryContent.en" />
  <skos:scopeNote xml:lang="en">Supplementary content may include an index, a bibliography, or an appendix.</skos:scopeNote>
</owl:ObjectProperty>

<!-- Property: is supplement to -->
<owl:ObjectProperty rdf:about="http://rdaregistry.info/Elements/u/P60259">
  <rdfs:isDefinedBy rdf:resource="http://rdaregistry.info/Elements/u/" />
  <reg:status rdf:resource="http://metadataregistry.org/uri/RegStatus/1001" />
  <reg:name xml:lang="en">supplementTo</reg:name>
  <rdfs:label xml:lang="en">is supplement to</rdfs:label>
  <skos:definition xml:lang="en">Relates a resource to a resource that is updated or otherwise complemented by an augmenting resource.</skos:definition>
  <rdf:type rdf:resource="http://www.w3.org/1999/02/22-rdf-syntax-ns#Property" />
  <rdfs:subPropertyOf rdf:resource="http://rdaregistry.info/Elements/u/P60307" />
  <owl:inverseOf rdf:resource="http://rdaregistry.info/Elements/u/P60281" />
  <reg:hasSubproperty rdf:resource="http://rdaregistry.info/Elements/e/P20151" />
  <reg:lexicalAlias rdf:resource="http://rdaregistry.info/Elements/u/supplementTo.en" />
</owl:ObjectProperty>

<!-- Property: has surname -->
<owl:ObjectProperty rdf:about="http://rdaregistry.info/Elements/u/P60878">
  <rdfs:isDefinedBy rdf:resource="http://rdaregistry.info/Elements/u/" />
  <reg:status rdf:resource="http://metadataregistry.org/uri/RegStatus/1001" />
  <rdf:type rdf:resource="http://www.w3.org/1999/02/22-rdf-syntax-ns#Property" />
  <reg:name xml:lang="en">surname</reg:name>
  <rdfs:label xml:lang="en">has surname</rdfs:label>
  <reg:lexicalAlias rdf:resource="http://rdaregistry.info/Elements/u/surname.en" />
  <skos:definition xml:lang="en">Relates an agent to a name used as a family name.</skos:definition>
  <reg:hasSubproperty rdf:resource="http://rdaregistry.info/Elements/a/P50291" />
</owl:ObjectProperty>

<!-- Property: has surveyor -->
<owl:ObjectProperty rdf:about="http://rdaregistry.info/Elements/u/P60377">
  <rdfs:isDefinedBy rdf:resource="http://rdaregistry.info/Elements/u/" />
  <reg:status rdf:resource="http://metadataregistry.org/uri/RegStatus/1001" />
  <reg:name xml:lang="en">surveyor</reg:name>
  <rdfs:label xml:lang="en">has surveyor</rdfs:label>
  <skos:definition xml:lang="en">Relates a resource to an agent contributing to a cartographic resource by providing measurements or dimensional relationships for a geographic area represented.</skos:definition>
  <rdf:type rdf:resource="http://www.w3.org/1999/02/22-rdf-syntax-ns#Property" />
  <rdfs:subPropertyOf rdf:resource="http://rdaregistry.info/Elements/u/P60398" />
  <owl:inverseOf rdf:resource="http://rdaregistry.info/Elements/u/P60605" />
  <reg:hasSubproperty rdf:resource="http://rdaregistry.info/Elements/e/P20027" />
  <reg:lexicalAlias rdf:resource="http://rdaregistry.info/Elements/u/surveyor.en" />
</owl:ObjectProperty>

<!-- Property: is surveyor of -->
<owl:ObjectProperty rdf:about="http://rdaregistry.info/Elements/u/P60605">
  <rdfs:isDefinedBy rdf:resource="http://rdaregistry.info/Elements/u/" />
  <reg:status rdf:resource="http://metadataregistry.org/uri/RegStatus/1001" />
  <reg:name xml:lang="en">surveyorOf</reg:name>
  <rdfs:label xml:lang="en">is surveyor of</rdfs:label>
  <skos:definition xml:lang="en">Relates an agent contributing to a cartographic resource by providing measurements or dimensional relationships for a geographic area represented to a resource.</skos:definition>
  <rdf:type rdf:resource="http://www.w3.org/1999/02/22-rdf-syntax-ns#Property" />
  <rdfs:subPropertyOf rdf:resource="http://rdaregistry.info/Elements/u/P60626" />
  <owl:inverseOf rdf:resource="http://rdaregistry.info/Elements/u/P60377" />
  <reg:hasSubproperty rdf:resource="http://rdaregistry.info/Elements/a/P50135" />
  <reg:lexicalAlias rdf:resource="http://rdaregistry.info/Elements/u/surveyorOf.en" />
</owl:ObjectProperty>

<!-- Property: has system of organization -->
<owl:ObjectProperty rdf:about="http://rdaregistry.info/Elements/u/P60348">
  <rdfs:isDefinedBy rdf:resource="http://rdaregistry.info/Elements/u/" />
  <reg:status rdf:resource="http://metadataregistry.org/uri/RegStatus/1001" />
  <reg:name xml:lang="en">systemOfOrganization</reg:name>
  <rdfs:label xml:lang="en">has system of organization</rdfs:label>
  <skos:definition xml:lang="en">Relates a resource to a system of arranging materials in an archival resource or a collection.</skos:definition>
  <rdf:type rdf:resource="http://www.w3.org/1999/02/22-rdf-syntax-ns#Property" />
  <reg:lexicalAlias rdf:resource="http://rdaregistry.info/Elements/u/systemOfOrganization.en" />
</owl:ObjectProperty>

<!-- Property: has tape configuration -->
<owl:ObjectProperty rdf:about="http://rdaregistry.info/Elements/u/P60553">
  <rdfs:isDefinedBy rdf:resource="http://rdaregistry.info/Elements/u/" />
  <reg:status rdf:resource="http://metadataregistry.org/uri/RegStatus/1001" />
  <reg:name xml:lang="en">tapeConfiguration</reg:name>
  <rdfs:label xml:lang="en">has tape configuration</rdfs:label>
  <skos:definition xml:lang="en">Relates a resource to a number of tracks on an audiotape.</skos:definition>
  <rdf:type rdf:resource="http://www.w3.org/1999/02/22-rdf-syntax-ns#Property" />
  <rdfs:subPropertyOf rdf:resource="http://rdaregistry.info/Elements/u/P60351" />
  <reg:hasSubproperty rdf:resource="http://rdaregistry.info/Elements/m/P30185" />
  <reg:lexicalAlias rdf:resource="http://rdaregistry.info/Elements/u/tapeConfiguration.en" />
</owl:ObjectProperty>

<!-- Property: has teacher -->
<owl:ObjectProperty rdf:about="http://rdaregistry.info/Elements/u/P60863">
  <rdfs:isDefinedBy rdf:resource="http://rdaregistry.info/Elements/u/" />
  <reg:status rdf:resource="http://metadataregistry.org/uri/RegStatus/1001" />
  <rdf:type rdf:resource="http://www.w3.org/1999/02/22-rdf-syntax-ns#Property" />
  <reg:name xml:lang="en">teacher</reg:name>
  <rdfs:label xml:lang="en">has teacher</rdfs:label>
  <reg:lexicalAlias rdf:resource="http://rdaregistry.info/Elements/u/teacher.en" />
  <skos:definition xml:lang="en">Relates an agent to an agent who instructs another agent.</skos:definition>
  <owl:inverseOf rdf:resource="http://rdaregistry.info/Elements/u/P60862" />
  <reg:hasSubproperty rdf:resource="http://rdaregistry.info/Elements/a/P50282" />
  <rdfs:subPropertyOf rdf:resource="http://rdaregistry.info/Elements/u/P60454" />
</owl:ObjectProperty>

<!-- Property: has teacher -->
<owl:ObjectProperty rdf:about="http://rdaregistry.info/Elements/u/P60145">
  <rdfs:isDefinedBy rdf:resource="http://rdaregistry.info/Elements/u/" />
  <reg:status rdf:resource="http://metadataregistry.org/uri/RegStatus/1001" />
  <reg:name xml:lang="en">teacher</reg:name>
  <rdfs:label xml:lang="en">has teacher</rdfs:label>
  <skos:definition xml:lang="en">Relates a resource to a performer contributing to a resource by giving instruction or providing a demonstration.</skos:definition>
  <rdf:type rdf:resource="http://www.w3.org/1999/02/22-rdf-syntax-ns#Property" />
  <rdfs:subPropertyOf rdf:resource="http://rdaregistry.info/Elements/u/P60387" />
  <owl:inverseOf rdf:resource="http://rdaregistry.info/Elements/u/P60020" />
  <reg:hasSubproperty rdf:resource="http://rdaregistry.info/Elements/e/P20015" />
  <reg:lexicalAlias rdf:resource="http://rdaregistry.info/Elements/u/teacher.en" />
</owl:ObjectProperty>

<!-- Property: is teacher of -->
<owl:ObjectProperty rdf:about="http://rdaregistry.info/Elements/u/P60020">
  <rdfs:isDefinedBy rdf:resource="http://rdaregistry.info/Elements/u/" />
  <reg:status rdf:resource="http://metadataregistry.org/uri/RegStatus/1001" />
  <reg:name xml:lang="en">teacherOf</reg:name>
  <rdfs:label xml:lang="en">is teacher of</rdfs:label>
  <skos:definition xml:lang="en">Relates a performer contributing to a resource by giving instruction or providing a demonstration to a resource.</skos:definition>
  <rdf:type rdf:resource="http://www.w3.org/1999/02/22-rdf-syntax-ns#Property" />
  <rdfs:subPropertyOf rdf:resource="http://rdaregistry.info/Elements/u/P60615" />
  <owl:inverseOf rdf:resource="http://rdaregistry.info/Elements/u/P60145" />
  <reg:hasSubproperty rdf:resource="http://rdaregistry.info/Elements/a/P50074" />
  <reg:lexicalAlias rdf:resource="http://rdaregistry.info/Elements/u/teacherOf.en" />
</owl:ObjectProperty>

<!-- Property: is television adaptation of -->
<owl:ObjectProperty rdf:about="http://rdaregistry.info/Elements/u/P60230">
  <rdfs:isDefinedBy rdf:resource="http://rdaregistry.info/Elements/u/" />
  <reg:status rdf:resource="http://metadataregistry.org/uri/RegStatus/1001" />
  <reg:name xml:lang="en">televisionAdaptationOf</reg:name>
  <rdfs:label xml:lang="en">is television adaptation of</rdfs:label>
  <skos:definition xml:lang="en">Relates a resource to a resource that has been adapted as a television program.</skos:definition>
  <rdf:type rdf:resource="http://www.w3.org/1999/02/22-rdf-syntax-ns#Property" />
  <rdfs:subPropertyOf rdf:resource="http://rdaregistry.info/Elements/u/P60241" />
  <owl:inverseOf rdf:resource="http://rdaregistry.info/Elements/u/P60354" />
  <reg:hasSubproperty rdf:resource="http://rdaregistry.info/Elements/e/P20128" />
  <reg:lexicalAlias rdf:resource="http://rdaregistry.info/Elements/u/televisionAdaptationOf.en" />
</owl:ObjectProperty>

<!-- Property: has television director -->
<owl:ObjectProperty rdf:about="http://rdaregistry.info/Elements/u/P60086">
  <rdfs:isDefinedBy rdf:resource="http://rdaregistry.info/Elements/u/" />
  <reg:status rdf:resource="http://metadataregistry.org/uri/RegStatus/1001" />
  <reg:name xml:lang="en">televisionDirector</reg:name>
  <rdfs:label xml:lang="en">has television director</rdfs:label>
  <skos:definition xml:lang="en">Relates a resource to a director responsible for the general management and supervision of a television program.</skos:definition>
  <rdf:type rdf:resource="http://www.w3.org/1999/02/22-rdf-syntax-ns#Property" />
  <rdfs:subPropertyOf rdf:resource="http://rdaregistry.info/Elements/u/P60449" />
  <owl:inverseOf rdf:resource="http://rdaregistry.info/Elements/u/P60011" />
  <reg:lexicalAlias rdf:resource="http://rdaregistry.info/Elements/u/televisionDirector.en" />
</owl:ObjectProperty>

<!-- Property: is television director of -->
<owl:ObjectProperty rdf:about="http://rdaregistry.info/Elements/u/P60011">
  <rdfs:isDefinedBy rdf:resource="http://rdaregistry.info/Elements/u/" />
  <reg:status rdf:resource="http://metadataregistry.org/uri/RegStatus/1001" />
  <reg:name xml:lang="en">televisionDirectorOf</reg:name>
  <rdfs:label xml:lang="en">is television director of</rdfs:label>
  <skos:definition xml:lang="en">Relates a director responsible for the general management and supervision of a television program to a resource.</skos:definition>
  <rdf:type rdf:resource="http://www.w3.org/1999/02/22-rdf-syntax-ns#Property" />
  <rdfs:subPropertyOf rdf:resource="http://rdaregistry.info/Elements/u/P60673" />
  <owl:inverseOf rdf:resource="http://rdaregistry.info/Elements/u/P60086" />
  <reg:hasSubproperty rdf:resource="http://rdaregistry.info/Elements/a/P50050" />
  <reg:lexicalAlias rdf:resource="http://rdaregistry.info/Elements/u/televisionDirectorOf.en" />
</owl:ObjectProperty>

<!-- Property: has television producer -->
<owl:ObjectProperty rdf:about="http://rdaregistry.info/Elements/u/P60171">
  <rdfs:isDefinedBy rdf:resource="http://rdaregistry.info/Elements/u/" />
  <reg:status rdf:resource="http://metadataregistry.org/uri/RegStatus/1001" />
  <reg:name xml:lang="en">televisionProducer</reg:name>
  <rdfs:label xml:lang="en">has television producer</rdfs:label>
  <skos:definition xml:lang="en">Relates a resource to a producer responsible for most of the business aspects of a television program.</skos:definition>
  <rdf:type rdf:resource="http://www.w3.org/1999/02/22-rdf-syntax-ns#Property" />
  <rdfs:subPropertyOf rdf:resource="http://rdaregistry.info/Elements/u/P60441" />
  <owl:inverseOf rdf:resource="http://rdaregistry.info/Elements/u/P60035" />
  <reg:lexicalAlias rdf:resource="http://rdaregistry.info/Elements/u/televisionProducer.en" />
</owl:ObjectProperty>

<!-- Property: is television producer of -->
<owl:ObjectProperty rdf:about="http://rdaregistry.info/Elements/u/P60035">
  <rdfs:isDefinedBy rdf:resource="http://rdaregistry.info/Elements/u/" />
  <reg:status rdf:resource="http://metadataregistry.org/uri/RegStatus/1001" />
  <reg:name xml:lang="en">televisionProducerOf</reg:name>
  <rdfs:label xml:lang="en">is television producer of</rdfs:label>
  <skos:definition xml:lang="en">Relates a producer responsible for most of the business aspects of a television program to a resource.</skos:definition>
  <rdf:type rdf:resource="http://www.w3.org/1999/02/22-rdf-syntax-ns#Property" />
  <rdfs:subPropertyOf rdf:resource="http://rdaregistry.info/Elements/u/P60668" />
  <owl:inverseOf rdf:resource="http://rdaregistry.info/Elements/u/P60171" />
  <reg:hasSubproperty rdf:resource="http://rdaregistry.info/Elements/a/P50215" />
  <reg:lexicalAlias rdf:resource="http://rdaregistry.info/Elements/u/televisionProducerOf.en" />
</owl:ObjectProperty>

<!-- Property: is television program music -->
<owl:ObjectProperty rdf:about="http://rdaregistry.info/Elements/u/P60727">
  <rdfs:isDefinedBy rdf:resource="http://rdaregistry.info/Elements/u/" />
  <reg:status rdf:resource="http://metadataregistry.org/uri/RegStatus/1001" />
  <reg:name xml:lang="en">televisionProgramMusic</reg:name>
  <rdfs:label xml:lang="en">is television program music</rdfs:label>
  <skos:definition xml:lang="en">Relates a resource to a musical resource that is used in a television program.</skos:definition>
  <rdf:type rdf:resource="http://www.w3.org/1999/02/22-rdf-syntax-ns#Property" />
  <rdfs:subPropertyOf rdf:resource="http://rdaregistry.info/Elements/u/P60723" />
  <owl:inverseOf rdf:resource="http://rdaregistry.info/Elements/u/P60728" />
  <reg:hasSubproperty rdf:resource="http://rdaregistry.info/Elements/e/P20247" />
  <reg:lexicalAlias rdf:resource="http://rdaregistry.info/Elements/u/televisionProgramMusic.en" />
</owl:ObjectProperty>

<!-- Property: is television screenplay -->
<owl:ObjectProperty rdf:about="http://rdaregistry.info/Elements/u/P60268">
  <rdfs:isDefinedBy rdf:resource="http://rdaregistry.info/Elements/u/" />
  <reg:status rdf:resource="http://metadataregistry.org/uri/RegStatus/1001" />
  <reg:name xml:lang="en">televisionScreenplay</reg:name>
  <rdfs:label xml:lang="en">is television screenplay</rdfs:label>
  <skos:definition xml:lang="en">Relates a resource to a resource that provides text for a television program.</skos:definition>
  <rdf:type rdf:resource="http://www.w3.org/1999/02/22-rdf-syntax-ns#Property" />
  <rdfs:subPropertyOf rdf:resource="http://rdaregistry.info/Elements/u/P60264" />
  <owl:inverseOf rdf:resource="http://rdaregistry.info/Elements/u/P60283" />
  <reg:hasSubproperty rdf:resource="http://rdaregistry.info/Elements/e/P20161" />
  <reg:lexicalAlias rdf:resource="http://rdaregistry.info/Elements/u/televisionScreenplay.en" />
</owl:ObjectProperty>

<!-- Property: is television screenplay based on -->
<owl:ObjectProperty rdf:about="http://rdaregistry.info/Elements/u/P60233">
  <rdfs:isDefinedBy rdf:resource="http://rdaregistry.info/Elements/u/" />
  <reg:status rdf:resource="http://metadataregistry.org/uri/RegStatus/1001" />
  <reg:name xml:lang="en">televisionScreenplayBasedOn</reg:name>
  <rdfs:label xml:lang="en">is television screenplay based on</rdfs:label>
  <skos:definition xml:lang="en">Relates a resource to a resource that has been adapted as a screenplay for a television program.</skos:definition>
  <rdf:type rdf:resource="http://www.w3.org/1999/02/22-rdf-syntax-ns#Property" />
  <rdfs:subPropertyOf rdf:resource="http://rdaregistry.info/Elements/u/P60231" />
  <owl:inverseOf rdf:resource="http://rdaregistry.info/Elements/u/P60186" />
  <reg:hasSubproperty rdf:resource="http://rdaregistry.info/Elements/e/P20131" />
  <reg:lexicalAlias rdf:resource="http://rdaregistry.info/Elements/u/televisionScreenplayBasedOn.en" />
</owl:ObjectProperty>

<!-- Property: has terms of availability -->
<owl:ObjectProperty rdf:about="http://rdaregistry.info/Elements/u/P60521">
  <rdfs:isDefinedBy rdf:resource="http://rdaregistry.info/Elements/u/" />
  <reg:status rdf:resource="http://metadataregistry.org/uri/RegStatus/1001" />
  <reg:name xml:lang="en">termsOfAvailability</reg:name>
  <rdfs:label xml:lang="en">has terms of availability</rdfs:label>
  <skos:definition xml:lang="en">Relates a resource to a condition under which a publisher, distributor, etc., will normally supply a resource or the price of a resource.</skos:definition>
  <rdf:type rdf:resource="http://www.w3.org/1999/02/22-rdf-syntax-ns#Property" />
  <reg:hasSubproperty rdf:resource="http://rdaregistry.info/Elements/m/P30160" />
  <reg:lexicalAlias rdf:resource="http://rdaregistry.info/Elements/u/termsOfAvailability.en" />
</owl:ObjectProperty>

<!-- Property: has title -->
<owl:ObjectProperty rdf:about="http://rdaregistry.info/Elements/u/P60369">
  <rdfs:isDefinedBy rdf:resource="http://rdaregistry.info/Elements/u/" />
  <reg:status rdf:resource="http://metadataregistry.org/uri/RegStatus/1001" />
  <reg:name xml:lang="en">title</reg:name>
  <rdfs:label xml:lang="en">has title</rdfs:label>
  <skos:definition xml:lang="en">Relates a resource to a word, character, or group of words or characters that names a resource or a resource embodied in it.</skos:definition>
  <rdf:type rdf:resource="http://www.w3.org/1999/02/22-rdf-syntax-ns#Property" />
  <reg:hasSubproperty rdf:resource="http://rdaregistry.info/Elements/u/P60355" />
  <reg:hasSubproperty rdf:resource="http://rdaregistry.info/Elements/u/P60357" />
  <reg:hasSubproperty rdf:resource="http://rdaregistry.info/Elements/u/P60358" />
  <reg:hasSubproperty rdf:resource="http://rdaregistry.info/Elements/u/P60359" />
  <reg:hasSubproperty rdf:resource="http://rdaregistry.info/Elements/u/P60493" />
  <reg:hasSubproperty rdf:resource="http://rdaregistry.info/Elements/u/P60507" />
  <reg:hasSubproperty rdf:resource="http://rdaregistry.info/Elements/u/P60515" />
  <reg:hasSubproperty rdf:resource="http://rdaregistry.info/Elements/u/P60589" />
  <reg:hasSubproperty rdf:resource="http://rdaregistry.info/Elements/u/P60597" />
  <reg:hasSubproperty rdf:resource="http://rdaregistry.info/Elements/m/P30134" />
  <reg:lexicalAlias rdf:resource="http://rdaregistry.info/Elements/u/title.en" />
</owl:ObjectProperty>

<!-- Property: has title of agent -->
<owl:ObjectProperty rdf:about="http://rdaregistry.info/Elements/u/P60363">
  <rdfs:isDefinedBy rdf:resource="http://rdaregistry.info/Elements/u/" />
  <reg:status rdf:resource="http://metadataregistry.org/uri/RegStatus/1001" />
  <reg:name xml:lang="en">titleOfAgent</reg:name>
  <rdfs:label xml:lang="en">has title of agent</rdfs:label>
  <skos:definition xml:lang="en">Relates a resource to a word or phrase indicative of royalty, nobility, or ecclesiastical rank or office, a term of address for an agent of religious vocation, or another term indicative of rank, honour, or office.</skos:definition>
  <rdf:type rdf:resource="http://www.w3.org/1999/02/22-rdf-syntax-ns#Property" />
  <reg:hasSubproperty rdf:resource="http://rdaregistry.info/Elements/a/P50110" />
  <reg:lexicalAlias rdf:resource="http://rdaregistry.info/Elements/u/titleOfAgent.en" />
</owl:ObjectProperty>

<!-- Property: has title of resource -->
<owl:ObjectProperty rdf:about="http://rdaregistry.info/Elements/u/P60367">
  <rdfs:isDefinedBy rdf:resource="http://rdaregistry.info/Elements/u/" />
  <reg:status rdf:resource="http://metadataregistry.org/uri/RegStatus/1001" />
  <reg:name xml:lang="en">titleOfResource</reg:name>
  <rdfs:label xml:lang="en">has title of resource</rdfs:label>
  <skos:definition xml:lang="en">Relates a resource to a word, character, or group of words or characters by which a resource is known.</skos:definition>
  <rdf:type rdf:resource="http://www.w3.org/1999/02/22-rdf-syntax-ns#Property" />
  <reg:hasSubproperty rdf:resource="http://rdaregistry.info/Elements/u/P60588" />
  <reg:lexicalAlias rdf:resource="http://rdaregistry.info/Elements/u/titleOfResource.en" />
</owl:ObjectProperty>

<!-- Property: has title proper -->
<owl:ObjectProperty rdf:about="http://rdaregistry.info/Elements/u/P60515">
  <rdfs:isDefinedBy rdf:resource="http://rdaregistry.info/Elements/u/" />
  <reg:status rdf:resource="http://metadataregistry.org/uri/RegStatus/1001" />
  <reg:name xml:lang="en">titleProper</reg:name>
  <rdfs:label xml:lang="en">has title proper</rdfs:label>
  <skos:definition xml:lang="en">Relates a resource to a chief name of a resource, that is, a title normally used when naming a resource.</skos:definition>
  <rdf:type rdf:resource="http://www.w3.org/1999/02/22-rdf-syntax-ns#Property" />
  <rdfs:subPropertyOf rdf:resource="http://rdaregistry.info/Elements/u/P60369" />
  <reg:hasSubproperty rdf:resource="http://rdaregistry.info/Elements/m/P30156" />
  <reg:lexicalAlias rdf:resource="http://rdaregistry.info/Elements/u/titleProper.en" />
  <skos:scopeNote xml:lang="en">An alternative title is treated as part of the title proper.</skos:scopeNote>
</owl:ObjectProperty>

<!-- Property: has title proper of series -->
<owl:ObjectProperty rdf:about="http://rdaregistry.info/Elements/u/P60516">
  <rdfs:isDefinedBy rdf:resource="http://rdaregistry.info/Elements/u/" />
  <reg:status rdf:resource="http://metadataregistry.org/uri/RegStatus/1001" />
  <reg:name xml:lang="en">titleProperOfSeries</reg:name>
  <rdfs:label xml:lang="en">has title proper of series</rdfs:label>
  <skos:definition xml:lang="en">Relates a resource to a name of a series appearing on a resource of a part of a series.</skos:definition>
  <rdf:type rdf:resource="http://www.w3.org/1999/02/22-rdf-syntax-ns#Property" />
  <reg:hasSubproperty rdf:resource="http://rdaregistry.info/Elements/m/P30157" />
  <reg:lexicalAlias rdf:resource="http://rdaregistry.info/Elements/u/titleProperOfSeries.en" />
</owl:ObjectProperty>

<!-- Property: has title proper of subseries -->
<owl:ObjectProperty rdf:about="http://rdaregistry.info/Elements/u/P60517">
  <rdfs:isDefinedBy rdf:resource="http://rdaregistry.info/Elements/u/" />
  <reg:status rdf:resource="http://metadataregistry.org/uri/RegStatus/1001" />
  <reg:name xml:lang="en">titleProperOfSubseries</reg:name>
  <rdfs:label xml:lang="en">has title proper of subseries</rdfs:label>
  <skos:definition xml:lang="en">Relates a resource to a name of a series appearing on a resource of a part of a subseries.</skos:definition>
  <rdf:type rdf:resource="http://www.w3.org/1999/02/22-rdf-syntax-ns#Property" />
  <reg:hasSubproperty rdf:resource="http://rdaregistry.info/Elements/m/P30158" />
  <reg:lexicalAlias rdf:resource="http://rdaregistry.info/Elements/u/titleProperOfSubseries.en" />
</owl:ObjectProperty>

<!-- Property: has track configuration -->
<owl:ObjectProperty rdf:about="http://rdaregistry.info/Elements/u/P60522">
  <rdfs:isDefinedBy rdf:resource="http://rdaregistry.info/Elements/u/" />
  <reg:status rdf:resource="http://metadataregistry.org/uri/RegStatus/1001" />
  <reg:name xml:lang="en">trackConfiguration</reg:name>
  <rdfs:label xml:lang="en">has track configuration</rdfs:label>
  <skos:definition xml:lang="en">Relates a reource to a configuration of an audio track on a sound-track film.</skos:definition>
  <rdf:type rdf:resource="http://www.w3.org/1999/02/22-rdf-syntax-ns#Property" />
  <rdfs:subPropertyOf rdf:resource="http://rdaregistry.info/Elements/u/P60351" />
  <reg:hasSubproperty rdf:resource="http://rdaregistry.info/Elements/m/P30161" />
  <reg:lexicalAlias rdf:resource="http://rdaregistry.info/Elements/u/trackConfiguration.en" />
</owl:ObjectProperty>

<!-- Property: has transcriber -->
<owl:ObjectProperty rdf:about="http://rdaregistry.info/Elements/u/P60382">
  <rdfs:isDefinedBy rdf:resource="http://rdaregistry.info/Elements/u/" />
  <reg:status rdf:resource="http://metadataregistry.org/uri/RegStatus/1001" />
  <reg:name xml:lang="en">transcriber</reg:name>
  <rdfs:label xml:lang="en">has transcriber</rdfs:label>
  <skos:definition xml:lang="en">Relates a resource to an agent contributing to a resource by writing down or notating unwritten or unnotated content, or by changing it from one system of notation to another.</skos:definition>
  <rdf:type rdf:resource="http://www.w3.org/1999/02/22-rdf-syntax-ns#Property" />
  <rdfs:subPropertyOf rdf:resource="http://rdaregistry.info/Elements/u/P60398" />
  <owl:inverseOf rdf:resource="http://rdaregistry.info/Elements/u/P60610" />
  <reg:hasSubproperty rdf:resource="http://rdaregistry.info/Elements/e/P20034" />
  <reg:lexicalAlias rdf:resource="http://rdaregistry.info/Elements/u/transcriber.en" />
  <skos:scopeNote xml:lang="en">Transcription of a musical resource for a different instrument or performing group is excluded.</skos:scopeNote>
  <rdakit:seeAlso rdf:resource="http://rdaregistry.info/Elements/u/P60379" />
</owl:ObjectProperty>

<!-- Property: is transcriber of -->
<owl:ObjectProperty rdf:about="http://rdaregistry.info/Elements/u/P60610">
  <rdfs:isDefinedBy rdf:resource="http://rdaregistry.info/Elements/u/" />
  <reg:status rdf:resource="http://metadataregistry.org/uri/RegStatus/1001" />
  <reg:name xml:lang="en">transcriberOf</reg:name>
  <rdfs:label xml:lang="en">is transcriber of</rdfs:label>
  <skos:definition xml:lang="en">Relates an agent contributing to a resource by writing down or notating previously unwritten or unnotated content, or by changing it from one system of notation to another to a resource.</skos:definition>
  <rdf:type rdf:resource="http://www.w3.org/1999/02/22-rdf-syntax-ns#Property" />
  <rdfs:subPropertyOf rdf:resource="http://rdaregistry.info/Elements/u/P60626" />
  <owl:inverseOf rdf:resource="http://rdaregistry.info/Elements/u/P60382" />
  <reg:hasSubproperty rdf:resource="http://rdaregistry.info/Elements/a/P50142" />
  <reg:lexicalAlias rdf:resource="http://rdaregistry.info/Elements/u/transcriberOf.en" />
  <skos:scopeNote xml:lang="en">Transcription of a musical resource for a different instrument or performing group is excluded.</skos:scopeNote>
  <rdakit:seeAlso rdf:resource="http://rdaregistry.info/Elements/u/P60607" />
</owl:ObjectProperty>

<!-- Property: is translated as -->
<owl:ObjectProperty rdf:about="http://rdaregistry.info/Elements/u/P60280">
  <rdfs:isDefinedBy rdf:resource="http://rdaregistry.info/Elements/u/" />
  <reg:status rdf:resource="http://metadataregistry.org/uri/RegStatus/1001" />
  <reg:name xml:lang="en">translatedAs</reg:name>
  <rdfs:label xml:lang="en">is translated as</rdfs:label>
  <skos:definition xml:lang="en">Relates a resource to a resource that translates the text of a source entity into a language different from that of an original resource.</skos:definition>
  <rdf:type rdf:resource="http://www.w3.org/1999/02/22-rdf-syntax-ns#Property" />
  <rdfs:subPropertyOf rdf:resource="http://rdaregistry.info/Elements/u/P60250" />
  <owl:inverseOf rdf:resource="http://rdaregistry.info/Elements/u/P60244" />
  <reg:hasSubproperty rdf:resource="http://rdaregistry.info/Elements/u/P60112" />
  <reg:hasSubproperty rdf:resource="http://rdaregistry.info/Elements/e/P20171" />
  <reg:lexicalAlias rdf:resource="http://rdaregistry.info/Elements/u/translatedAs.en" />
</owl:ObjectProperty>

<!-- Property: is translation of -->
<owl:ObjectProperty rdf:about="http://rdaregistry.info/Elements/u/P60244">
  <rdfs:isDefinedBy rdf:resource="http://rdaregistry.info/Elements/u/" />
  <reg:status rdf:resource="http://metadataregistry.org/uri/RegStatus/1001" />
  <reg:name xml:lang="en">translationOf</reg:name>
  <rdfs:label xml:lang="en">is translation of</rdfs:label>
  <skos:definition xml:lang="en">Relates a resource to a resource that has been translated, i.e., the text expressed in a language different from that of an original resource.</skos:definition>
  <rdf:type rdf:resource="http://www.w3.org/1999/02/22-rdf-syntax-ns#Property" />
  <rdfs:subPropertyOf rdf:resource="http://rdaregistry.info/Elements/u/P60305" />
  <owl:inverseOf rdf:resource="http://rdaregistry.info/Elements/u/P60280" />
  <reg:hasSubproperty rdf:resource="http://rdaregistry.info/Elements/u/P60111" />
  <reg:hasSubproperty rdf:resource="http://rdaregistry.info/Elements/e/P20141" />
  <reg:lexicalAlias rdf:resource="http://rdaregistry.info/Elements/u/translationOf.en" />
</owl:ObjectProperty>

<!-- Property: has translator -->
<owl:ObjectProperty rdf:about="http://rdaregistry.info/Elements/u/P60385">
  <rdfs:isDefinedBy rdf:resource="http://rdaregistry.info/Elements/u/" />
  <reg:status rdf:resource="http://metadataregistry.org/uri/RegStatus/1001" />
  <reg:name xml:lang="en">translator</reg:name>
  <rdfs:label xml:lang="en">has translator</rdfs:label>
  <skos:definition xml:lang="en">Relates a resource to an agent contributing to an expression of a resource by expressing linguistic content of a resource in a language different from that of previous expressions of an original resource.</skos:definition>
  <rdf:type rdf:resource="http://www.w3.org/1999/02/22-rdf-syntax-ns#Property" />
  <rdfs:subPropertyOf rdf:resource="http://rdaregistry.info/Elements/u/P60398" />
  <owl:inverseOf rdf:resource="http://rdaregistry.info/Elements/u/P60613" />
  <reg:hasSubproperty rdf:resource="http://rdaregistry.info/Elements/e/P20037" />
  <reg:lexicalAlias rdf:resource="http://rdaregistry.info/Elements/u/translator.en" />
  <skos:scopeNote xml:lang="en">Translation of linguistic content between forms of the same language from different time periods is included.</skos:scopeNote>
</owl:ObjectProperty>

<!-- Property: is translator of -->
<owl:ObjectProperty rdf:about="http://rdaregistry.info/Elements/u/P60613">
  <rdfs:isDefinedBy rdf:resource="http://rdaregistry.info/Elements/u/" />
  <reg:status rdf:resource="http://metadataregistry.org/uri/RegStatus/1001" />
  <reg:name xml:lang="en">translatorOf</reg:name>
  <rdfs:label xml:lang="en">is translator of</rdfs:label>
  <skos:definition xml:lang="en">Relates an agent contributing to a resource by expressing linguistic content of a resource in a language different from that of previous expressions of an original resource to a resource.</skos:definition>
  <rdf:type rdf:resource="http://www.w3.org/1999/02/22-rdf-syntax-ns#Property" />
  <rdfs:subPropertyOf rdf:resource="http://rdaregistry.info/Elements/u/P60626" />
  <owl:inverseOf rdf:resource="http://rdaregistry.info/Elements/u/P60385" />
  <reg:hasSubproperty rdf:resource="http://rdaregistry.info/Elements/a/P50145" />
  <reg:lexicalAlias rdf:resource="http://rdaregistry.info/Elements/u/translatorOf.en" />
  <skos:scopeNote xml:lang="en">Translation of linguistic content between forms of the same language from different time periods is included.</skos:scopeNote>
</owl:ObjectProperty>

<!-- Property: has trustee -->
<owl:ObjectProperty rdf:about="http://rdaregistry.info/Elements/u/P60866">
  <rdfs:isDefinedBy rdf:resource="http://rdaregistry.info/Elements/u/" />
  <reg:status rdf:resource="http://metadataregistry.org/uri/RegStatus/1001" />
  <rdf:type rdf:resource="http://www.w3.org/1999/02/22-rdf-syntax-ns#Property" />
  <reg:name xml:lang="en">trustee</reg:name>
  <rdfs:label xml:lang="en">has trustee</rdfs:label>
  <reg:lexicalAlias rdf:resource="http://rdaregistry.info/Elements/u/trustee.en" />
  <skos:definition xml:lang="en">Relates an agent to an officer granted powers of administration in an agent in order to act for its benefit.</skos:definition>
  <owl:inverseOf rdf:resource="http://rdaregistry.info/Elements/u/P60867" />
  <reg:hasSubproperty rdf:resource="http://rdaregistry.info/Elements/a/P50285" />
  <rdfs:subPropertyOf rdf:resource="http://rdaregistry.info/Elements/u/P60633" />
</owl:ObjectProperty>

<!-- Property: is trustee of -->
<owl:ObjectProperty rdf:about="http://rdaregistry.info/Elements/u/P60867">
  <rdfs:isDefinedBy rdf:resource="http://rdaregistry.info/Elements/u/" />
  <reg:status rdf:resource="http://metadataregistry.org/uri/RegStatus/1001" />
  <rdf:type rdf:resource="http://www.w3.org/1999/02/22-rdf-syntax-ns#Property" />
  <reg:name xml:lang="en">trusteeOf</reg:name>
  <rdfs:label xml:lang="en">is trustee of</rdfs:label>
  <reg:lexicalAlias rdf:resource="http://rdaregistry.info/Elements/u/trusteeOf.en" />
  <skos:definition xml:lang="en">Relates an agent to an agent that grants powers of administration to an officer in order to act for its benefit.</skos:definition>
  <owl:inverseOf rdf:resource="http://rdaregistry.info/Elements/u/P60866" />
  <reg:hasSubproperty rdf:resource="http://rdaregistry.info/Elements/a/P50287" />
  <rdfs:subPropertyOf rdf:resource="http://rdaregistry.info/Elements/u/P60737" />
</owl:ObjectProperty>

<!-- Property: has type of agent -->
<owl:ObjectProperty rdf:about="http://rdaregistry.info/Elements/u/P60047">
  <rdfs:isDefinedBy rdf:resource="http://rdaregistry.info/Elements/u/" />
  <reg:status rdf:resource="http://metadataregistry.org/uri/RegStatus/1001" />
  <reg:name xml:lang="en">typeOfAgent</reg:name>
  <rdfs:label xml:lang="en">has type of agent</rdfs:label>
  <skos:definition xml:lang="en">Relates a resource to a categorization or generic descriptor for a type of agent.</skos:definition>
  <rdf:type rdf:resource="http://www.w3.org/1999/02/22-rdf-syntax-ns#Property" />
  <reg:hasSubproperty rdf:resource="http://rdaregistry.info/Elements/a/P50237" />
  <reg:hasSubproperty rdf:resource="http://rdaregistry.info/Elements/a/P50238" />
  <reg:hasSubproperty rdf:resource="http://rdaregistry.info/Elements/a/P50051" />
  <reg:lexicalAlias rdf:resource="http://rdaregistry.info/Elements/u/typeOfAgent.en" />
</owl:ObjectProperty>

<!-- Property: has type of recording -->
<owl:ObjectProperty rdf:about="http://rdaregistry.info/Elements/u/P60543">
  <rdfs:isDefinedBy rdf:resource="http://rdaregistry.info/Elements/u/" />
  <reg:status rdf:resource="http://metadataregistry.org/uri/RegStatus/1001" />
  <reg:name xml:lang="en">typeOfRecording</reg:name>
  <rdfs:label xml:lang="en">has type of recording</rdfs:label>
  <skos:definition xml:lang="en">Relates a resource to a method used to encode audio content for playback.</skos:definition>
  <rdf:type rdf:resource="http://www.w3.org/1999/02/22-rdf-syntax-ns#Property" />
  <rdfs:subPropertyOf rdf:resource="http://rdaregistry.info/Elements/u/P60351" />
  <reg:hasSubproperty rdf:resource="http://rdaregistry.info/Elements/m/P30172" />
  <reg:lexicalAlias rdf:resource="http://rdaregistry.info/Elements/u/typeOfRecording.en" />
</owl:ObjectProperty>

<!-- Property: has undifferentiated name indicator -->
<owl:ObjectProperty rdf:about="http://rdaregistry.info/Elements/u/P60046">
  <rdfs:isDefinedBy rdf:resource="http://rdaregistry.info/Elements/u/" />
  <reg:status rdf:resource="http://metadataregistry.org/uri/RegStatus/1001" />
  <reg:name xml:lang="en">undifferentiatedNameIndicator</reg:name>
  <rdfs:label xml:lang="en">has undifferentiated name indicator</rdfs:label>
  <skos:definition xml:lang="en">Relates a resource to a categorization indicating that the core elements recorded are insufficient to differentiate between two or more agents with the same name.</skos:definition>
  <rdf:type rdf:resource="http://www.w3.org/1999/02/22-rdf-syntax-ns#Property" />
  <reg:hasSubproperty rdf:resource="http://rdaregistry.info/Elements/a/P50093" />
  <reg:lexicalAlias rdf:resource="http://rdaregistry.info/Elements/u/undifferentiatedNameIndicator.en" />
</owl:ObjectProperty>

<!-- Property: has uniform resource locator -->
<owl:ObjectProperty rdf:about="http://rdaregistry.info/Elements/u/P60511">
  <rdfs:isDefinedBy rdf:resource="http://rdaregistry.info/Elements/u/" />
  <reg:status rdf:resource="http://metadataregistry.org/uri/RegStatus/1001" />
  <reg:name xml:lang="en">uniformResourceLocator</reg:name>
  <rdfs:label xml:lang="en">has uniform resource locator</rdfs:label>
  <skos:definition xml:lang="en">Relates a resource to an address of an online resource.</skos:definition>
  <rdf:type rdf:resource="http://www.w3.org/1999/02/22-rdf-syntax-ns#Property" />
  <reg:hasSubproperty rdf:resource="http://rdaregistry.info/Elements/m/P30154" />
  <reg:lexicalAlias rdf:resource="http://rdaregistry.info/Elements/u/uniformResourceLocator.en" />
  <skos:scopeNote xml:lang="en">A Uniform Resource Locators includes all resource identifiers intended to provide online access to a resource using a standard Internet browser.</skos:scopeNote>
  <skos:altLabel xml:lang="en">URL</skos:altLabel>
</owl:ObjectProperty>

<!-- Property: has variant name for agent -->
<owl:ObjectProperty rdf:about="http://rdaregistry.info/Elements/u/P60119">
  <rdfs:isDefinedBy rdf:resource="http://rdaregistry.info/Elements/u/" />
  <reg:status rdf:resource="http://metadataregistry.org/uri/RegStatus/1001" />
  <reg:name xml:lang="en">variantNameForAgent</reg:name>
  <rdfs:label xml:lang="en">has variant name for agent</rdfs:label>
  <skos:definition xml:lang="en">Relates a resource to a name or form of name by which an agent is known that differs from a name or form of name chosen as a preferred name.</skos:definition>
  <rdf:type rdf:resource="http://www.w3.org/1999/02/22-rdf-syntax-ns#Property" />
  <rdfs:subPropertyOf rdf:resource="http://rdaregistry.info/Elements/u/P60368" />
  <reg:hasSubproperty rdf:resource="http://rdaregistry.info/Elements/a/P50025" />
  <reg:hasSubproperty rdf:resource="http://rdaregistry.info/Elements/a/P50054" />
  <reg:hasSubproperty rdf:resource="http://rdaregistry.info/Elements/a/P50103" />
  <reg:lexicalAlias rdf:resource="http://rdaregistry.info/Elements/u/variantNameForAgent.en" />
</owl:ObjectProperty>

<!-- Property: has variant name of place -->
<owl:ObjectProperty rdf:about="http://rdaregistry.info/Elements/u/P60880">
  <rdfs:isDefinedBy rdf:resource="http://rdaregistry.info/Elements/u/" />
  <reg:status rdf:resource="http://metadataregistry.org/uri/RegStatus/1001" />
  <rdf:type rdf:resource="http://www.w3.org/1999/02/22-rdf-syntax-ns#Property" />
  <reg:name xml:lang="en">variantNameOfPlace</reg:name>
  <rdfs:label xml:lang="en">has variant name of place</rdfs:label>
  <reg:lexicalAlias rdf:resource="http://rdaregistry.info/Elements/u/variantNameOfPlace.en" />
  <skos:definition xml:lang="en">Relates a place to a name or form of name by which a place is known that differs from a name or form of name chosen as a preferred name.</skos:definition>
  <reg:hasSubproperty rdf:resource="http://rdaregistry.info/Elements/p/P70003" />
</owl:ObjectProperty>

<!-- Property: has variant title -->
<owl:ObjectProperty rdf:about="http://rdaregistry.info/Elements/u/P60355">
  <rdfs:isDefinedBy rdf:resource="http://rdaregistry.info/Elements/u/" />
  <reg:status rdf:resource="http://metadataregistry.org/uri/RegStatus/1001" />
  <reg:name xml:lang="en">variantTitle</reg:name>
  <rdfs:label xml:lang="en">has variant title</rdfs:label>
  <skos:definition xml:lang="en">Relates a resource to a title associated with a resource that differs from a title recorded as a preferred title, title proper, a parallel title proper, other title information, parallel other title information, earlier title proper, later title proper, key title, or abbreviated title.</skos:definition>
  <rdf:type rdf:resource="http://www.w3.org/1999/02/22-rdf-syntax-ns#Property" />
  <rdfs:subPropertyOf rdf:resource="http://rdaregistry.info/Elements/u/P60369" />
  <reg:hasSubproperty rdf:resource="http://rdaregistry.info/Elements/m/P30128" />
  <reg:lexicalAlias rdf:resource="http://rdaregistry.info/Elements/u/variantTitle.en" />
</owl:ObjectProperty>

<!-- Property: is variations based on -->
<owl:ObjectProperty rdf:about="http://rdaregistry.info/Elements/u/P60114">
  <rdfs:isDefinedBy rdf:resource="http://rdaregistry.info/Elements/u/" />
  <reg:status rdf:resource="http://metadataregistry.org/uri/RegStatus/1001" />
  <reg:name xml:lang="en">variationsBasedOn</reg:name>
  <rdfs:label xml:lang="en">is variations based on</rdfs:label>
  <skos:definition xml:lang="en">Relates a resource to a musical resource from which melodic, thematic, or harmonic material is taken to form a discrete theme, which is repeated one or more times with subsequent modifications.</skos:definition>
  <rdf:type rdf:resource="http://www.w3.org/1999/02/22-rdf-syntax-ns#Property" />
  <rdfs:subPropertyOf rdf:resource="http://rdaregistry.info/Elements/u/P60305" />
  <owl:inverseOf rdf:resource="http://rdaregistry.info/Elements/u/P60115" />
  <reg:hasSubproperty rdf:resource="http://rdaregistry.info/Elements/e/P20081" />
  <reg:lexicalAlias rdf:resource="http://rdaregistry.info/Elements/u/variationsBasedOn.en" />
</owl:ObjectProperty>

<!-- Property: is verse adaptation of -->
<owl:ObjectProperty rdf:about="http://rdaregistry.info/Elements/u/P60226">
  <rdfs:isDefinedBy rdf:resource="http://rdaregistry.info/Elements/u/" />
  <reg:status rdf:resource="http://metadataregistry.org/uri/RegStatus/1001" />
  <reg:name xml:lang="en">verseAdaptationOf</reg:name>
  <rdfs:label xml:lang="en">is verse adaptation of</rdfs:label>
  <skos:definition xml:lang="en">Relates a resource to a resource that has been adapted as a literary composition in verse form.</skos:definition>
  <rdf:type rdf:resource="http://www.w3.org/1999/02/22-rdf-syntax-ns#Property" />
  <rdfs:subPropertyOf rdf:resource="http://rdaregistry.info/Elements/u/P60241" />
  <owl:inverseOf rdf:resource="http://rdaregistry.info/Elements/u/P60106" />
  <reg:hasSubproperty rdf:resource="http://rdaregistry.info/Elements/e/P20124" />
  <reg:lexicalAlias rdf:resource="http://rdaregistry.info/Elements/u/verseAdaptationOf.en" />
</owl:ObjectProperty>

<!-- Property: has vertical scale of cartographic content -->
<owl:ObjectProperty rdf:about="http://rdaregistry.info/Elements/u/P60579">
  <rdfs:isDefinedBy rdf:resource="http://rdaregistry.info/Elements/u/" />
  <reg:status rdf:resource="http://metadataregistry.org/uri/RegStatus/1001" />
  <reg:name xml:lang="en">verticalScaleOfCartographicContent</reg:name>
  <rdfs:label xml:lang="en">has vertical scale of cartographic content</rdfs:label>
  <skos:definition xml:lang="en">Relates a resource to a scale of elevation or vertical dimension of the cartographic content of a resource.</skos:definition>
  <rdf:type rdf:resource="http://www.w3.org/1999/02/22-rdf-syntax-ns#Property" />
  <rdfs:subPropertyOf rdf:resource="http://rdaregistry.info/Elements/u/P60565" />
  <reg:hasSubproperty rdf:resource="http://rdaregistry.info/Elements/e/P20230" />
  <reg:lexicalAlias rdf:resource="http://rdaregistry.info/Elements/u/verticalScaleOfCartographicContent.en" />
</owl:ObjectProperty>

<!-- Property: is video adaptation of -->
<owl:ObjectProperty rdf:about="http://rdaregistry.info/Elements/u/P60236">
  <rdfs:isDefinedBy rdf:resource="http://rdaregistry.info/Elements/u/" />
  <reg:status rdf:resource="http://metadataregistry.org/uri/RegStatus/1001" />
  <reg:name xml:lang="en">videoAdaptationOf</reg:name>
  <rdfs:label xml:lang="en">is video adaptation of</rdfs:label>
  <skos:definition xml:lang="en">Relates a resource to a resource that has been adapted for video.</skos:definition>
  <rdf:type rdf:resource="http://www.w3.org/1999/02/22-rdf-syntax-ns#Property" />
  <rdfs:subPropertyOf rdf:resource="http://rdaregistry.info/Elements/u/P60241" />
  <owl:inverseOf rdf:resource="http://rdaregistry.info/Elements/u/P60361" />
  <reg:hasSubproperty rdf:resource="http://rdaregistry.info/Elements/e/P20134" />
  <reg:lexicalAlias rdf:resource="http://rdaregistry.info/Elements/u/videoAdaptationOf.en" />
</owl:ObjectProperty>

<!-- Property: has video characteristic -->
<owl:ObjectProperty rdf:about="http://rdaregistry.info/Elements/u/P60352">
  <rdfs:isDefinedBy rdf:resource="http://rdaregistry.info/Elements/u/" />
  <reg:status rdf:resource="http://metadataregistry.org/uri/RegStatus/1001" />
  <reg:name xml:lang="en">videoCharacteristic</reg:name>
  <rdfs:label xml:lang="en">has video characteristic</rdfs:label>
  <skos:definition xml:lang="en">Relates a resource to a technical specification relating to an encoding of video images in a resource.</skos:definition>
  <rdf:type rdf:resource="http://www.w3.org/1999/02/22-rdf-syntax-ns#Property" />
  <reg:hasSubproperty rdf:resource="http://rdaregistry.info/Elements/u/P60326" />
  <reg:hasSubproperty rdf:resource="http://rdaregistry.info/Elements/u/P60349" />
  <reg:hasSubproperty rdf:resource="http://rdaregistry.info/Elements/m/P30126" />
  <reg:lexicalAlias rdf:resource="http://rdaregistry.info/Elements/u/videoCharacteristic.en" />
</owl:ObjectProperty>

<!-- Property: has video format -->
<owl:ObjectProperty rdf:about="http://rdaregistry.info/Elements/u/P60326">
  <rdfs:isDefinedBy rdf:resource="http://rdaregistry.info/Elements/u/" />
  <reg:status rdf:resource="http://metadataregistry.org/uri/RegStatus/1001" />
  <reg:name xml:lang="en">videoFormat</reg:name>
  <rdfs:label xml:lang="en">has video format</rdfs:label>
  <skos:definition xml:lang="en">Relates a resource to a standard, etc., used to encode the analog video content of a resource.</skos:definition>
  <rdf:type rdf:resource="http://www.w3.org/1999/02/22-rdf-syntax-ns#Property" />
  <rdfs:subPropertyOf rdf:resource="http://rdaregistry.info/Elements/u/P60352" />
  <reg:hasSubproperty rdf:resource="http://rdaregistry.info/Elements/m/P30104" />
  <reg:lexicalAlias rdf:resource="http://rdaregistry.info/Elements/u/videoFormat.en" />
</owl:ObjectProperty>

<!-- Property: is video game adaptation of -->
<owl:ObjectProperty rdf:about="http://rdaregistry.info/Elements/u/P60745">
  <rdfs:isDefinedBy rdf:resource="http://rdaregistry.info/Elements/u/" />
  <reg:status rdf:resource="http://metadataregistry.org/uri/RegStatus/1001" />
  <rdf:type rdf:resource="http://www.w3.org/1999/02/22-rdf-syntax-ns#Property" />
  <reg:name xml:lang="en">videoGameAdaptationOf</reg:name>
  <rdfs:label xml:lang="en">is video game adaptation of</rdfs:label>
  <reg:lexicalAlias rdf:resource="http://rdaregistry.info/Elements/u/videoGameAdaptationOf.en" />
  <skos:definition xml:lang="en">Relates a resource to a resource that has been adapted as a video game.</skos:definition>
  <owl:inverseOf rdf:resource="http://rdaregistry.info/Elements/u/P60744" />
  <rdfs:subPropertyOf rdf:resource="http://rdaregistry.info/Elements/u/P60241" />
</owl:ObjectProperty>

<!-- Property: is video music -->
<owl:ObjectProperty rdf:about="http://rdaregistry.info/Elements/u/P60725">
  <rdfs:isDefinedBy rdf:resource="http://rdaregistry.info/Elements/u/" />
  <reg:status rdf:resource="http://metadataregistry.org/uri/RegStatus/1001" />
  <reg:name xml:lang="en">videoMusic</reg:name>
  <rdfs:label xml:lang="en">is video music</rdfs:label>
  <skos:definition xml:lang="en">Relates a resource to a musical resource that is used in a video.</skos:definition>
  <rdf:type rdf:resource="http://www.w3.org/1999/02/22-rdf-syntax-ns#Property" />
  <rdfs:subPropertyOf rdf:resource="http://rdaregistry.info/Elements/u/P60723" />
  <owl:inverseOf rdf:resource="http://rdaregistry.info/Elements/u/P60726" />
  <reg:hasSubproperty rdf:resource="http://rdaregistry.info/Elements/e/P20245" />
  <reg:lexicalAlias rdf:resource="http://rdaregistry.info/Elements/u/videoMusic.en" />
</owl:ObjectProperty>

<!-- Property: is video screenplay -->
<owl:ObjectProperty rdf:about="http://rdaregistry.info/Elements/u/P60269">
  <rdfs:isDefinedBy rdf:resource="http://rdaregistry.info/Elements/u/" />
  <reg:status rdf:resource="http://metadataregistry.org/uri/RegStatus/1001" />
  <reg:name xml:lang="en">videoScreenplay</reg:name>
  <rdfs:label xml:lang="en">is video screenplay</rdfs:label>
  <skos:definition xml:lang="en">Relates a resource to a resource that provides text for a video.</skos:definition>
  <rdf:type rdf:resource="http://www.w3.org/1999/02/22-rdf-syntax-ns#Property" />
  <rdfs:subPropertyOf rdf:resource="http://rdaregistry.info/Elements/u/P60264" />
  <owl:inverseOf rdf:resource="http://rdaregistry.info/Elements/u/P60284" />
  <reg:hasSubproperty rdf:resource="http://rdaregistry.info/Elements/e/P20162" />
  <reg:lexicalAlias rdf:resource="http://rdaregistry.info/Elements/u/videoScreenplay.en" />
</owl:ObjectProperty>

<!-- Property: is video screenplay based on -->
<owl:ObjectProperty rdf:about="http://rdaregistry.info/Elements/u/P60234">
  <rdfs:isDefinedBy rdf:resource="http://rdaregistry.info/Elements/u/" />
  <reg:status rdf:resource="http://metadataregistry.org/uri/RegStatus/1001" />
  <reg:name xml:lang="en">videoScreenplayBasedOn</reg:name>
  <rdfs:label xml:lang="en">is video screenplay based on</rdfs:label>
  <skos:definition xml:lang="en">Relates a resource to a resource that has been adapted as a screenplay for a video.</skos:definition>
  <rdf:type rdf:resource="http://www.w3.org/1999/02/22-rdf-syntax-ns#Property" />
  <rdfs:subPropertyOf rdf:resource="http://rdaregistry.info/Elements/u/P60231" />
  <owl:inverseOf rdf:resource="http://rdaregistry.info/Elements/u/P60187" />
  <reg:hasSubproperty rdf:resource="http://rdaregistry.info/Elements/e/P20132" />
  <reg:lexicalAlias rdf:resource="http://rdaregistry.info/Elements/u/videoScreenplayBasedOn.en" />
</owl:ObjectProperty>

<!-- Property: has visual effects provider -->
<owl:ObjectProperty rdf:about="http://rdaregistry.info/Elements/u/P60748">
  <rdfs:isDefinedBy rdf:resource="http://rdaregistry.info/Elements/u/" />
  <reg:status rdf:resource="http://metadataregistry.org/uri/RegStatus/1001" />
  <rdf:type rdf:resource="http://www.w3.org/1999/02/22-rdf-syntax-ns#Property" />
  <reg:name xml:lang="en">visualEffectsProvider</reg:name>
  <rdfs:label xml:lang="en">has visual effects provider</rdfs:label>
  <reg:lexicalAlias rdf:resource="http://rdaregistry.info/Elements/u/visualEffectsProvider.en" />
  <skos:definition xml:lang="en">Relates a resource to an agent contributing to an expression of a moving image resource by designing and creating post-production visual effects.</skos:definition>
  <owl:inverseOf rdf:resource="http://rdaregistry.info/Elements/u/P60754" />
  <rdfs:subPropertyOf rdf:resource="http://rdaregistry.info/Elements/u/P60398" />
</owl:ObjectProperty>

<!-- Property: is visual effects provider of -->
<owl:ObjectProperty rdf:about="http://rdaregistry.info/Elements/u/P60754">
  <rdfs:isDefinedBy rdf:resource="http://rdaregistry.info/Elements/u/" />
  <reg:status rdf:resource="http://metadataregistry.org/uri/RegStatus/1001" />
  <rdf:type rdf:resource="http://www.w3.org/1999/02/22-rdf-syntax-ns#Property" />
  <reg:name xml:lang="en">visualEffectsProviderOf</reg:name>
  <rdfs:label xml:lang="en">is visual effects provider of</rdfs:label>
  <reg:lexicalAlias rdf:resource="http://rdaregistry.info/Elements/u/visualEffectsProviderOf.en" />
  <skos:definition xml:lang="en">Relates an agent contributing to an expression of a moving image resource by designing and creating post-production visual effects to a resource.</skos:definition>
  <owl:inverseOf rdf:resource="http://rdaregistry.info/Elements/u/P60748" />
  <rdfs:subPropertyOf rdf:resource="http://rdaregistry.info/Elements/u/P60626" />
</owl:ObjectProperty>

<!-- Property: has voice actor -->
<owl:ObjectProperty rdf:about="http://rdaregistry.info/Elements/u/P60152">
  <rdfs:isDefinedBy rdf:resource="http://rdaregistry.info/Elements/u/" />
  <reg:status rdf:resource="http://metadataregistry.org/uri/RegStatus/1001" />
  <reg:name xml:lang="en">voiceActor</reg:name>
  <rdfs:label xml:lang="en">has voice actor</rdfs:label>
  <skos:definition xml:lang="en">Relates a resource to a performer contributing to a resource by providing a voice for characters in radio and audio productions and for animated characters in moving image resources as well as by providing voice-overs in radio and television commercials, dubbed resources, etc.</skos:definition>
  <rdf:type rdf:resource="http://www.w3.org/1999/02/22-rdf-syntax-ns#Property" />
  <rdfs:subPropertyOf rdf:resource="http://rdaregistry.info/Elements/u/P60142" />
  <owl:inverseOf rdf:resource="http://rdaregistry.info/Elements/u/P60027" />
  <reg:hasSubproperty rdf:resource="http://rdaregistry.info/Elements/e/P20070" />
  <reg:lexicalAlias rdf:resource="http://rdaregistry.info/Elements/u/voiceActor.en" />
</owl:ObjectProperty>

<!-- Property: is voice actor of -->
<owl:ObjectProperty rdf:about="http://rdaregistry.info/Elements/u/P60027">
  <rdfs:isDefinedBy rdf:resource="http://rdaregistry.info/Elements/u/" />
  <reg:status rdf:resource="http://metadataregistry.org/uri/RegStatus/1001" />
  <reg:name xml:lang="en">voiceActorOf</reg:name>
  <rdfs:label xml:lang="en">is voice actor of</rdfs:label>
  <skos:definition xml:lang="en">Relates a performer contributing to a resource by providing the voice for characters in radio and audio productions and for animated characters in moving image resources as well as by providing voice-overs in radio and television commercials, dubbed resources, etc. to a resource.</skos:definition>
  <rdf:type rdf:resource="http://www.w3.org/1999/02/22-rdf-syntax-ns#Property" />
  <rdfs:subPropertyOf rdf:resource="http://rdaregistry.info/Elements/u/P60017" />
  <owl:inverseOf rdf:resource="http://rdaregistry.info/Elements/u/P60152" />
  <reg:hasSubproperty rdf:resource="http://rdaregistry.info/Elements/a/P50217" />
  <reg:lexicalAlias rdf:resource="http://rdaregistry.info/Elements/u/voiceActorOf.en" />
</owl:ObjectProperty>

<!-- Property: has whole-part resource relationship with -->
<owl:ObjectProperty rdf:about="http://rdaregistry.info/Elements/u/P60714">
  <rdfs:isDefinedBy rdf:resource="http://rdaregistry.info/Elements/u/" />
  <reg:status rdf:resource="http://metadataregistry.org/uri/RegStatus/1001" />
  <reg:name xml:lang="en">wholePartResourceRelationshipWith</reg:name>
  <rdfs:label xml:lang="en">has whole-part resource relationship with</rdfs:label>
  <rdf:type rdf:resource="http://www.w3.org/1999/02/22-rdf-syntax-ns#Property" />
  <reg:hasSubproperty rdf:resource="http://rdaregistry.info/Elements/u/P60101" />
  <reg:hasSubproperty rdf:resource="http://rdaregistry.info/Elements/u/P60249" />
  <owl:inverseOf rdf:resource="http://rdaregistry.info/Elements/u/P60714" />
  <skos:definition xml:lang="en">Relates a resource to a resource that is contained in or contains a resource.</skos:definition>
  <reg:hasSubproperty rdf:resource="http://rdaregistry.info/Elements/e/P20236" />
  <reg:hasSubproperty rdf:resource="http://rdaregistry.info/Elements/i/P40054" />
  <reg:hasSubproperty rdf:resource="http://rdaregistry.info/Elements/m/P30213" />
  <reg:lexicalAlias rdf:resource="http://rdaregistry.info/Elements/u/wholePartResourceRelationshipWith.en" />
</owl:ObjectProperty>

<!-- Property: has writer of added commentary -->
<owl:ObjectProperty rdf:about="http://rdaregistry.info/Elements/u/P60390">
  <rdfs:isDefinedBy rdf:resource="http://rdaregistry.info/Elements/u/" />
  <reg:status rdf:resource="http://metadataregistry.org/uri/RegStatus/1001" />
  <reg:name xml:lang="en">writerOfAddedCommentary</reg:name>
  <rdfs:label xml:lang="en">has writer of added commentary</rdfs:label>
  <skos:definition xml:lang="en">Relates a resource to an agent contributing to a resource by providing an interpretation or critical explanation of an original resource.</skos:definition>
  <rdf:type rdf:resource="http://www.w3.org/1999/02/22-rdf-syntax-ns#Property" />
  <rdfs:subPropertyOf rdf:resource="http://rdaregistry.info/Elements/u/P60392" />
  <owl:inverseOf rdf:resource="http://rdaregistry.info/Elements/u/P60618" />
  <reg:hasSubproperty rdf:resource="http://rdaregistry.info/Elements/e/P20044" />
  <reg:lexicalAlias rdf:resource="http://rdaregistry.info/Elements/u/writerOfAddedCommentary.en" />
</owl:ObjectProperty>

<!-- Property: is writer of added commentary of -->
<owl:ObjectProperty rdf:about="http://rdaregistry.info/Elements/u/P60618">
  <rdfs:isDefinedBy rdf:resource="http://rdaregistry.info/Elements/u/" />
  <reg:status rdf:resource="http://metadataregistry.org/uri/RegStatus/1001" />
  <reg:name xml:lang="en">writerOfAddedCommentaryOf</reg:name>
  <rdfs:label xml:lang="en">is writer of added commentary of</rdfs:label>
  <skos:definition xml:lang="en">Relates an agent contributing to a resource by providing an interpretation or critical explanation of an original resource to a resource.</skos:definition>
  <rdf:type rdf:resource="http://www.w3.org/1999/02/22-rdf-syntax-ns#Property" />
  <rdfs:subPropertyOf rdf:resource="http://rdaregistry.info/Elements/u/P60620" />
  <owl:inverseOf rdf:resource="http://rdaregistry.info/Elements/u/P60390" />
  <reg:hasSubproperty rdf:resource="http://rdaregistry.info/Elements/a/P50152" />
  <reg:lexicalAlias rdf:resource="http://rdaregistry.info/Elements/u/writerOfAddedCommentaryOf.en" />
</owl:ObjectProperty>

<!-- Property: has writer of added lyrics -->
<owl:ObjectProperty rdf:about="http://rdaregistry.info/Elements/u/P60371">
  <rdfs:isDefinedBy rdf:resource="http://rdaregistry.info/Elements/u/" />
  <reg:status rdf:resource="http://metadataregistry.org/uri/RegStatus/1001" />
  <reg:name xml:lang="en">writerOfAddedLyrics</reg:name>
  <rdfs:label xml:lang="en">has writer of added lyrics</rdfs:label>
  <skos:definition xml:lang="en">Relates a resource to a writer of words added to a musical resource.</skos:definition>
  <rdf:type rdf:resource="http://www.w3.org/1999/02/22-rdf-syntax-ns#Property" />
  <rdfs:subPropertyOf rdf:resource="http://rdaregistry.info/Elements/u/P60380" />
  <owl:inverseOf rdf:resource="http://rdaregistry.info/Elements/u/P60600" />
  <reg:hasSubproperty rdf:resource="http://rdaregistry.info/Elements/e/P20068" />
  <reg:lexicalAlias rdf:resource="http://rdaregistry.info/Elements/u/writerOfAddedLyrics.en" />
  <skos:scopeNote xml:lang="en">Writing of lyrics in collaboration with a composer to form an original resource is excluded.</skos:scopeNote>
  <rdakit:seeAlso rdf:resource="http://rdaregistry.info/Elements/u/P60477" />
</owl:ObjectProperty>

<!-- Property: is writer of added lyrics of -->
<owl:ObjectProperty rdf:about="http://rdaregistry.info/Elements/u/P60600">
  <rdfs:isDefinedBy rdf:resource="http://rdaregistry.info/Elements/u/" />
  <reg:status rdf:resource="http://metadataregistry.org/uri/RegStatus/1001" />
  <reg:name xml:lang="en">writerOfAddedLyricsOf</reg:name>
  <rdfs:label xml:lang="en">is writer of added lyrics of</rdfs:label>
  <skos:definition xml:lang="en">Relates a writer of words added to a musical resource to a resource.</skos:definition>
  <rdf:type rdf:resource="http://www.w3.org/1999/02/22-rdf-syntax-ns#Property" />
  <rdfs:subPropertyOf rdf:resource="http://rdaregistry.info/Elements/u/P60608" />
  <owl:inverseOf rdf:resource="http://rdaregistry.info/Elements/u/P60371" />
  <reg:hasSubproperty rdf:resource="http://rdaregistry.info/Elements/a/P50216" />
  <reg:lexicalAlias rdf:resource="http://rdaregistry.info/Elements/u/writerOfAddedLyricsOf.en" />
  <skos:scopeNote xml:lang="en">Writing of lyrics in collaboration with a composer to form an original resource is excluded.</skos:scopeNote>
  <rdakit:seeAlso rdf:resource="http://rdaregistry.info/Elements/u/P60707" />
</owl:ObjectProperty>

<!-- Property: has writer of added text -->
<owl:ObjectProperty rdf:about="http://rdaregistry.info/Elements/u/P60380">
  <rdfs:isDefinedBy rdf:resource="http://rdaregistry.info/Elements/u/" />
  <reg:status rdf:resource="http://metadataregistry.org/uri/RegStatus/1001" />
  <reg:name xml:lang="en">writerOfAddedText</reg:name>
  <rdfs:label xml:lang="en">has writer of added text</rdfs:label>
  <skos:definition xml:lang="en">Relates a resource to an agent contributing to a primarily non-textual resource by providing text, such as writing captions for photographs or descriptions of maps.</skos:definition>
  <rdf:type rdf:resource="http://www.w3.org/1999/02/22-rdf-syntax-ns#Property" />
  <rdfs:subPropertyOf rdf:resource="http://rdaregistry.info/Elements/u/P60392" />
  <owl:inverseOf rdf:resource="http://rdaregistry.info/Elements/u/P60608" />
  <reg:hasSubproperty rdf:resource="http://rdaregistry.info/Elements/u/P60371" />
  <reg:hasSubproperty rdf:resource="http://rdaregistry.info/Elements/e/P20030" />
  <reg:lexicalAlias rdf:resource="http://rdaregistry.info/Elements/u/writerOfAddedText.en" />
</owl:ObjectProperty>

<!-- Property: is writer of added text of -->
<owl:ObjectProperty rdf:about="http://rdaregistry.info/Elements/u/P60608">
  <rdfs:isDefinedBy rdf:resource="http://rdaregistry.info/Elements/u/" />
  <reg:status rdf:resource="http://metadataregistry.org/uri/RegStatus/1001" />
  <reg:name xml:lang="en">writerOfAddedTextOf</reg:name>
  <rdfs:label xml:lang="en">is writer of added text of</rdfs:label>
  <skos:definition xml:lang="en">Relates an agent contributing to a primarily non-textual resource by providing text, such as captions for photographs or descriptions of maps to a resource.</skos:definition>
  <rdf:type rdf:resource="http://www.w3.org/1999/02/22-rdf-syntax-ns#Property" />
  <rdfs:subPropertyOf rdf:resource="http://rdaregistry.info/Elements/u/P60620" />
  <owl:inverseOf rdf:resource="http://rdaregistry.info/Elements/u/P60380" />
  <reg:hasSubproperty rdf:resource="http://rdaregistry.info/Elements/u/P60600" />
  <reg:hasSubproperty rdf:resource="http://rdaregistry.info/Elements/a/P50138" />
  <reg:lexicalAlias rdf:resource="http://rdaregistry.info/Elements/u/writerOfAddedTextOf.en" />
</owl:ObjectProperty>

<!-- Property: has writer of afterword -->
<owl:ObjectProperty rdf:about="http://rdaregistry.info/Elements/u/P60715">
  <rdfs:isDefinedBy rdf:resource="http://rdaregistry.info/Elements/u/" />
  <reg:status rdf:resource="http://metadataregistry.org/uri/RegStatus/1001" />
  <reg:name xml:lang="en">writerOfAfterword</reg:name>
  <rdfs:label xml:lang="en">has writer of afterword</rdfs:label>
  <skos:definition xml:lang="en">Relates a resource to an agent contributing to a resource by providing an afterword to an original resource.</skos:definition>
  <rdf:type rdf:resource="http://www.w3.org/1999/02/22-rdf-syntax-ns#Property" />
  <rdfs:subPropertyOf rdf:resource="http://rdaregistry.info/Elements/u/P60392" />
  <owl:inverseOf rdf:resource="http://rdaregistry.info/Elements/u/P60717" />
  <reg:hasSubproperty rdf:resource="http://rdaregistry.info/Elements/e/P20237" />
  <reg:lexicalAlias rdf:resource="http://rdaregistry.info/Elements/u/writerOfAfterword.en" />
</owl:ObjectProperty>

<!-- Property: is writer of preface of -->
<owl:ObjectProperty rdf:about="http://rdaregistry.info/Elements/u/P60717">
  <rdfs:isDefinedBy rdf:resource="http://rdaregistry.info/Elements/u/" />
  <reg:status rdf:resource="http://metadataregistry.org/uri/RegStatus/1001" />
  <reg:name xml:lang="en">writerOfAfterwordOf</reg:name>
  <rdfs:label xml:lang="en">is writer of preface of</rdfs:label>
  <skos:definition xml:lang="en">Relates an agent contributing to a resource by providing a preface to an original resource to a resource.</skos:definition>
  <rdf:type rdf:resource="http://www.w3.org/1999/02/22-rdf-syntax-ns#Property" />
  <rdfs:subPropertyOf rdf:resource="http://rdaregistry.info/Elements/u/P60620" />
  <owl:inverseOf rdf:resource="http://rdaregistry.info/Elements/u/P60715" />
  <reg:hasSubproperty rdf:resource="http://rdaregistry.info/Elements/a/P50227" />
  <reg:lexicalAlias rdf:resource="http://rdaregistry.info/Elements/u/writerOfAfterwordOf.en" />
</owl:ObjectProperty>

<!-- Property: has writer of foreword -->
<owl:ObjectProperty rdf:about="http://rdaregistry.info/Elements/u/P60809">
  <rdfs:isDefinedBy rdf:resource="http://rdaregistry.info/Elements/u/" />
  <reg:status rdf:resource="http://metadataregistry.org/uri/RegStatus/1001" />
  <rdf:type rdf:resource="http://www.w3.org/1999/02/22-rdf-syntax-ns#Property" />
  <reg:name xml:lang="en">writerOfForeword</reg:name>
  <rdfs:label xml:lang="en">has writer of foreword</rdfs:label>
  <reg:lexicalAlias rdf:resource="http://rdaregistry.info/Elements/u/writerOfForeword.en" />
  <skos:definition xml:lang="en">Relates a resource to an agent contributing to a resource by providing a foreword to an original resource.</skos:definition>
  <owl:inverseOf rdf:resource="http://rdaregistry.info/Elements/u/P60810" />
  <rdfs:subPropertyOf rdf:resource="http://rdaregistry.info/Elements/u/P60398" />
</owl:ObjectProperty>

<!-- Property: is writer of foreword of -->
<owl:ObjectProperty rdf:about="http://rdaregistry.info/Elements/u/P60810">
  <rdfs:isDefinedBy rdf:resource="http://rdaregistry.info/Elements/u/" />
  <reg:status rdf:resource="http://metadataregistry.org/uri/RegStatus/1001" />
  <rdf:type rdf:resource="http://www.w3.org/1999/02/22-rdf-syntax-ns#Property" />
  <reg:name xml:lang="en">writerOfForewordOf</reg:name>
  <rdfs:label xml:lang="en">is writer of foreword of</rdfs:label>
  <reg:lexicalAlias rdf:resource="http://rdaregistry.info/Elements/u/writerOfForewordOf.en" />
  <skos:definition xml:lang="en">Relates an agent contributing to a resource by providing a foreword to an original resource to a resource.</skos:definition>
  <owl:inverseOf rdf:resource="http://rdaregistry.info/Elements/u/P60809" />
  <rdfs:subPropertyOf rdf:resource="http://rdaregistry.info/Elements/u/P60626" />
</owl:ObjectProperty>

<!-- Property: has writer of introduction -->
<owl:ObjectProperty rdf:about="http://rdaregistry.info/Elements/u/P60391">
  <rdfs:isDefinedBy rdf:resource="http://rdaregistry.info/Elements/u/" />
  <reg:status rdf:resource="http://metadataregistry.org/uri/RegStatus/1001" />
  <reg:name xml:lang="en">writerOfIntroduction</reg:name>
  <rdfs:label xml:lang="en">has writer of introduction</rdfs:label>
  <skos:definition xml:lang="en">Relates a resource to an agent contributing to a resource by providing an introduction to an original resource.</skos:definition>
  <rdf:type rdf:resource="http://www.w3.org/1999/02/22-rdf-syntax-ns#Property" />
  <rdfs:subPropertyOf rdf:resource="http://rdaregistry.info/Elements/u/P60392" />
  <owl:inverseOf rdf:resource="http://rdaregistry.info/Elements/u/P60619" />
  <reg:hasSubproperty rdf:resource="http://rdaregistry.info/Elements/e/P20045" />
  <reg:lexicalAlias rdf:resource="http://rdaregistry.info/Elements/u/writerOfIntroduction.en" />
</owl:ObjectProperty>

<!-- Property: is writer of afterword of -->
<owl:ObjectProperty rdf:about="http://rdaregistry.info/Elements/u/P60619">
  <rdfs:isDefinedBy rdf:resource="http://rdaregistry.info/Elements/u/" />
  <reg:status rdf:resource="http://metadataregistry.org/uri/RegStatus/1001" />
  <reg:name xml:lang="en">writerOfIntroductionOf</reg:name>
  <rdfs:label xml:lang="en">is writer of afterword of</rdfs:label>
  <skos:definition xml:lang="en">Relates an agent contributing to a resource by providing an afterword to an original resource to a resource.</skos:definition>
  <rdf:type rdf:resource="http://www.w3.org/1999/02/22-rdf-syntax-ns#Property" />
  <rdfs:subPropertyOf rdf:resource="http://rdaregistry.info/Elements/u/P60620" />
  <owl:inverseOf rdf:resource="http://rdaregistry.info/Elements/u/P60391" />
  <reg:hasSubproperty rdf:resource="http://rdaregistry.info/Elements/a/P50153" />
  <reg:lexicalAlias rdf:resource="http://rdaregistry.info/Elements/u/writerOfIntroductionOf.en" />
</owl:ObjectProperty>

<!-- Property: has writer of postface -->
<owl:ObjectProperty rdf:about="http://rdaregistry.info/Elements/u/P60716">
  <rdfs:isDefinedBy rdf:resource="http://rdaregistry.info/Elements/u/" />
  <reg:status rdf:resource="http://metadataregistry.org/uri/RegStatus/1001" />
  <reg:name xml:lang="en">writerOfPostface</reg:name>
  <rdfs:label xml:lang="en">has writer of postface</rdfs:label>
  <skos:definition xml:lang="en">Relates a resource to an agent contributing to a resource by providing a postface to an original resource.</skos:definition>
  <rdf:type rdf:resource="http://www.w3.org/1999/02/22-rdf-syntax-ns#Property" />
  <rdfs:subPropertyOf rdf:resource="http://rdaregistry.info/Elements/u/P60392" />
  <owl:inverseOf rdf:resource="http://rdaregistry.info/Elements/u/P60718" />
  <reg:hasSubproperty rdf:resource="http://rdaregistry.info/Elements/e/P20238" />
  <reg:lexicalAlias rdf:resource="http://rdaregistry.info/Elements/u/writerOfPostface.en" />
</owl:ObjectProperty>

<!-- Property: is writer of supplementary textual content of -->
<owl:ObjectProperty rdf:about="http://rdaregistry.info/Elements/u/P60718">
  <rdfs:isDefinedBy rdf:resource="http://rdaregistry.info/Elements/u/" />
  <reg:status rdf:resource="http://metadataregistry.org/uri/RegStatus/1001" />
  <reg:name xml:lang="en">writerOfPostfaceOf</reg:name>
  <rdfs:label xml:lang="en">is writer of supplementary textual content of</rdfs:label>
  <skos:definition xml:lang="en">Relates an agent contributing to a resource by providing supplementary textual content (e.g., an appendix, an introduction, a preface) to an original resource to a resource.</skos:definition>
  <rdf:type rdf:resource="http://www.w3.org/1999/02/22-rdf-syntax-ns#Property" />
  <rdfs:subPropertyOf rdf:resource="http://rdaregistry.info/Elements/u/P60620" />
  <owl:inverseOf rdf:resource="http://rdaregistry.info/Elements/u/P60716" />
  <reg:hasSubproperty rdf:resource="http://rdaregistry.info/Elements/a/P50228" />
  <reg:lexicalAlias rdf:resource="http://rdaregistry.info/Elements/u/writerOfPostfaceOf.en" />
</owl:ObjectProperty>

<!-- Property: has writer of preface -->
<owl:ObjectProperty rdf:about="http://rdaregistry.info/Elements/u/P60389">
  <rdfs:isDefinedBy rdf:resource="http://rdaregistry.info/Elements/u/" />
  <reg:status rdf:resource="http://metadataregistry.org/uri/RegStatus/1001" />
  <reg:name xml:lang="en">writerOfPreface</reg:name>
  <rdfs:label xml:lang="en">has writer of preface</rdfs:label>
  <skos:definition xml:lang="en">Relates a resource to an agent contributing to a resource by providing a preface to an original resource.</skos:definition>
  <rdf:type rdf:resource="http://www.w3.org/1999/02/22-rdf-syntax-ns#Property" />
  <rdfs:subPropertyOf rdf:resource="http://rdaregistry.info/Elements/u/P60392" />
  <owl:inverseOf rdf:resource="http://rdaregistry.info/Elements/u/P60617" />
  <reg:hasSubproperty rdf:resource="http://rdaregistry.info/Elements/e/P20041" />
  <reg:lexicalAlias rdf:resource="http://rdaregistry.info/Elements/u/writerOfPreface.en" />
</owl:ObjectProperty>

<!-- Property: is writer of introduction of -->
<owl:ObjectProperty rdf:about="http://rdaregistry.info/Elements/u/P60617">
  <rdfs:isDefinedBy rdf:resource="http://rdaregistry.info/Elements/u/" />
  <reg:status rdf:resource="http://metadataregistry.org/uri/RegStatus/1001" />
  <reg:name xml:lang="en">writerOfPrefaceOf</reg:name>
  <rdfs:label xml:lang="en">is writer of introduction of</rdfs:label>
  <skos:definition xml:lang="en">Relates an agent contributing to a resource by providing an introduction to an original resource to a resource.</skos:definition>
  <rdf:type rdf:resource="http://www.w3.org/1999/02/22-rdf-syntax-ns#Property" />
  <rdfs:subPropertyOf rdf:resource="http://rdaregistry.info/Elements/u/P60620" />
  <owl:inverseOf rdf:resource="http://rdaregistry.info/Elements/u/P60389" />
  <reg:hasSubproperty rdf:resource="http://rdaregistry.info/Elements/a/P50149" />
  <reg:lexicalAlias rdf:resource="http://rdaregistry.info/Elements/u/writerOfPrefaceOf.en" />
</owl:ObjectProperty>

<!-- Property: has writer of supplementary textual content -->
<owl:ObjectProperty rdf:about="http://rdaregistry.info/Elements/u/P60392">
  <rdfs:isDefinedBy rdf:resource="http://rdaregistry.info/Elements/u/" />
  <reg:status rdf:resource="http://metadataregistry.org/uri/RegStatus/1001" />
  <reg:name xml:lang="en">writerOfSupplementaryTextualContent</reg:name>
  <rdfs:label xml:lang="en">has writer of supplementary textual content</rdfs:label>
  <skos:definition xml:lang="en">Relates a resource to an agent contributing to a resource by providing supplementary textual content (e.g., an appendix, an introduction, a preface) to an original resource.</skos:definition>
  <rdf:type rdf:resource="http://www.w3.org/1999/02/22-rdf-syntax-ns#Property" />
  <rdfs:subPropertyOf rdf:resource="http://rdaregistry.info/Elements/u/P60398" />
  <owl:inverseOf rdf:resource="http://rdaregistry.info/Elements/u/P60620" />
  <reg:hasSubproperty rdf:resource="http://rdaregistry.info/Elements/u/P60380" />
  <reg:hasSubproperty rdf:resource="http://rdaregistry.info/Elements/u/P60389" />
  <reg:hasSubproperty rdf:resource="http://rdaregistry.info/Elements/u/P60390" />
  <reg:hasSubproperty rdf:resource="http://rdaregistry.info/Elements/u/P60391" />
  <reg:hasSubproperty rdf:resource="http://rdaregistry.info/Elements/e/P20046" />
  <reg:lexicalAlias rdf:resource="http://rdaregistry.info/Elements/u/writerOfSupplementaryTextualContent.en" />
</owl:ObjectProperty>

<!-- Property: is writer of postface of -->
<owl:ObjectProperty rdf:about="http://rdaregistry.info/Elements/u/P60620">
  <rdfs:isDefinedBy rdf:resource="http://rdaregistry.info/Elements/u/" />
  <reg:status rdf:resource="http://metadataregistry.org/uri/RegStatus/1001" />
  <reg:name xml:lang="en">writerOfSupplementaryTextualContentOf</reg:name>
  <rdfs:label xml:lang="en">is writer of postface of</rdfs:label>
  <skos:definition xml:lang="en">Relates an agent contributing to a resource by providing supplementary textual content, such as an introduction or a preface, to an original resource to a resource.</skos:definition>
  <rdf:type rdf:resource="http://www.w3.org/1999/02/22-rdf-syntax-ns#Property" />
  <rdfs:subPropertyOf rdf:resource="http://rdaregistry.info/Elements/u/P60626" />
  <owl:inverseOf rdf:resource="http://rdaregistry.info/Elements/u/P60392" />
  <reg:hasSubproperty rdf:resource="http://rdaregistry.info/Elements/u/P60608" />
  <reg:hasSubproperty rdf:resource="http://rdaregistry.info/Elements/u/P60617" />
  <reg:hasSubproperty rdf:resource="http://rdaregistry.info/Elements/u/P60618" />
  <reg:hasSubproperty rdf:resource="http://rdaregistry.info/Elements/u/P60619" />
  <reg:hasSubproperty rdf:resource="http://rdaregistry.info/Elements/a/P50154" />
  <reg:lexicalAlias rdf:resource="http://rdaregistry.info/Elements/u/writerOfSupplementaryTextualContentOf.en" />
</owl:ObjectProperty>

<!-- Property: has year degree granted -->
<owl:ObjectProperty rdf:about="http://rdaregistry.info/Elements/u/P60514">
  <rdfs:isDefinedBy rdf:resource="http://rdaregistry.info/Elements/u/" />
  <reg:status rdf:resource="http://metadataregistry.org/uri/RegStatus/1001" />
  <reg:name xml:lang="en">yearDegreeGranted</reg:name>
  <rdfs:label xml:lang="en">has year degree granted</rdfs:label>
  <skos:definition xml:lang="en">Relates a resource to a calendar year in which a granting institution or faculty conferred an academic degree on a candidate.</skos:definition>
  <rdf:type rdf:resource="http://www.w3.org/1999/02/22-rdf-syntax-ns#Property" />
  <reg:lexicalAlias rdf:resource="http://rdaregistry.info/Elements/u/yearDegreeGranted.en" />
</owl:ObjectProperty>


<!-- Status properties used in this document  -->
    <skos:Concept rdf:about="http://metadataregistry.org/uri/RegStatus/1001">
        <skos:prefLabel xml:lang="en">Published</skos:prefLabel>
    </skos:Concept>
    <skos:Concept rdf:about="http://metadataregistry.org/uri/RegStatus/1008">
        <skos:prefLabel xml:lang="en">Deprecated</skos:prefLabel>
    </skos:Concept>
</rdf:RDF>
